@prefix ns1: <http://ffrdc.ebiquity.umbc.edu/ns/ontology/#> .
@prefix ns2: <http://ffrdc.ebiquity.umbc.edu/ns/ontology/> .
@prefix owl: <http://www.w3.org/2002/07/owl#> .
@prefix rdf: <http://www.w3.org/1999/02/22-rdf-syntax-ns#> .
@prefix rdfs: <http://www.w3.org/2000/01/rdf-schema#> .
@prefix xsd: <http://www.w3.org/2001/XMLSchema#> .

<http://capec.mitre.org/capec_v1#Indicator> a owl:Class ;
    rdfs:comment "Formal definition for Indicator within the cybersecurity domain."^^xsd:string ;
    rdfs:subClassOf ns1:UCOThing ;
    owl:equivalentClass ns2:Indicator .

<http://capec.mitre.org/capec_v1#Observable> a owl:Class ;
    rdfs:comment "Formal definition for Observable within the cybersecurity domain."^^xsd:string ;
    rdfs:subClassOf ns1:UCOThing ;
    owl:equivalentClass <http://cybox.mitre.org/cybox_v1#Observable> .

<http://capec.mitre.org/capec_v1#Weakness> a owl:Class ;
    rdfs:comment "Formal definition for Weakness within the cybersecurity domain."^^xsd:string ;
    rdfs:subClassOf ns1:UCOThing ;
    owl:equivalentClass ns1:CWE .

ns1:AtError a owl:Class ;
    rdfs:comment "Formal definition for AtError within the cybersecurity domain."^^xsd:string ;
    rdfs:subClassOf ns1:LogicExploit .

ns1:BoundaryCondition a owl:Class ;
    rdfs:comment "Formal definition for BoundaryCondition within the cybersecurity domain."^^xsd:string ;
    rdfs:seeAlso "http://dbpedia.org/resource/Off-by-one_error"^^xsd:anyURI ;
    rdfs:subClassOf ns1:InputValidationError .

ns1:BufferOverFlow a owl:Class ;
    rdfs:comment "Formal definition for BufferOverFlow within the cybersecurity domain."^^xsd:string ;
    rdfs:seeAlso "http://dbpedia.org/resource/Buffer_overflow"^^xsd:anyURI ;
    rdfs:subClassOf [ a owl:Restriction ;
            owl:onProperty ns1:resultsIn ;
            owl:someValuesFrom ns1:DenialOfService ],
        ns1:Means .

ns1:ConfigurationError a owl:Class ;
    rdfs:comment "Formal definition for ConfigurationError within the cybersecurity domain."^^xsd:string ;
    rdfs:subClassOf [ a owl:Restriction ;
            owl:onProperty ns1:resultsIn ;
            owl:someValuesFrom ns1:DenialOfService ],
        ns1:Means .

ns1:DistributedCode a owl:Class ;
    rdfs:comment "Formal definition for DistributedCode within the cybersecurity domain."^^xsd:string ;
    rdfs:subClassOf [ a owl:Restriction ;
            owl:onProperty ns1:resultsIn ;
            owl:someValuesFrom ns1:BotnetAttack ],
        ns1:MaliciousCodeExecution .

ns1:DomainExpert a owl:Class ;
    rdfs:comment "Formal definition for DomainExpert within the cybersecurity domain."^^xsd:string ;
    rdfs:subClassOf ns1:Source .

ns1:ExICMPEchoReq a owl:Class ;
    rdfs:comment "Formal definition for ExICMPEchoReq within the cybersecurity domain."^^xsd:string ;
    rdfs:subClassOf ns1:Means .

ns1:ExIPPacketSize a owl:Class ;
    rdfs:comment "Formal definition for ExIPPacketSize within the cybersecurity domain."^^xsd:string ;
    rdfs:subClassOf ns1:Means .

ns1:ExceptionCondition a owl:Class ;
    rdfs:comment "Formal definition for ExceptionCondition within the cybersecurity domain."^^xsd:string ;
    rdfs:seeAlso "http://dbpedia.org/resource/Exception_handling"^^xsd:anyURI ;
    rdfs:subClassOf ns1:LogicExploit .

ns1:ExcessForks a owl:Class ;
    rdfs:comment "Formal definition for ExcessForks within the cybersecurity domain."^^xsd:string ;
    rdfs:subClassOf ns1:DenialOfService .

ns1:IPFrag a owl:Class ;
    rdfs:comment "Formal definition for IPFrag within the cybersecurity domain."^^xsd:string ;
    rdfs:seeAlso "http://dbpedia.org/resource/IP_fragmentation_attacks"^^xsd:anyURI ;
    rdfs:subClassOf [ a owl:Restriction ;
            owl:onProperty ns1:resultsIn ;
            owl:someValuesFrom ns1:DenialOfService ],
        ns1:Means .

ns1:IPv4Address a owl:Class ;
    rdfs:comment "Formal definition for IPv4Address within the cybersecurity domain."^^xsd:string ;
    rdfs:subClassOf ns1:IPAddress .

ns1:IPv6Address a owl:Class ;
    rdfs:comment "Formal definition for IPv6Address within the cybersecurity domain."^^xsd:string ;
    rdfs:subClassOf ns1:IPAddress .

ns1:MACAddress a owl:Class ;
    rdfs:comment "Formal definition for MACAddress within the cybersecurity domain."^^xsd:string ;
    rdfs:subClassOf ns1:Address .

ns1:MalformedInput a owl:Class ;
    rdfs:comment "Formal definition for MalformedInput within the cybersecurity domain."^^xsd:string ;
    rdfs:seeAlso "http://sw.opencyc.org/concept/Mx4rwQShKJwpEbGdrcN5Y29ycA"^^xsd:anyURI ;
    rdfs:subClassOf ns1:InputValidationError .

ns1:MemoryConsumption a owl:Class ;
    rdfs:comment "Formal definition for MemoryConsumption within the cybersecurity domain."^^xsd:string ;
    rdfs:subClassOf ns1:DenialOfService .

ns1:ParisiticCode a owl:Class ;
    rdfs:comment "Formal definition for ParisiticCode within the cybersecurity domain."^^xsd:string ;
    rdfs:subClassOf [ a owl:Restriction ;
            owl:onProperty ns1:resultsIn ;
            owl:someValuesFrom ns1:LossOfIntegrity ],
        ns1:MaliciousCodeExecution .

ns1:PingOfDeath a owl:Class ;
    rdfs:comment "Formal definition for PingOfDeath within the cybersecurity domain."^^xsd:string ;
    rdfs:seeAlso "http://dbpedia.org/resource/Ping_of_death"^^xsd:anyURI ;
    rdfs:subClassOf ns1:DenialOfService .

ns1:PingScan a owl:Class ;
    rdfs:comment "Formal definition for PingScan within the cybersecurity domain."^^xsd:string ;
    rdfs:subClassOf ns1:Probe .

ns1:RSTProbe a owl:Class ;
    rdfs:comment "Formal definition for RSTProbe within the cybersecurity domain."^^xsd:string ;
    rdfs:subClassOf ns1:Probe .

ns1:RaceCondition a owl:Class ;
    rdfs:comment "Formal definition for RaceCondition within the cybersecurity domain."^^xsd:string ;
    rdfs:seeAlso "http://dbpedia.org/resource/Race_condition"^^xsd:anyURI ;
    rdfs:subClassOf ns1:LogicExploit .

ns1:Rootkit a owl:Class ;
    rdfs:comment "Formal definition for Rootkit within the cybersecurity domain."^^xsd:string ;
    rdfs:seeAlso "http://dbpedia.org/resource/Rootkit"^^xsd:anyURI ;
    rdfs:subClassOf [ a owl:Restriction ;
            owl:onProperty ns1:resultsIn ;
            owl:someValuesFrom ns1:DenialOfService ],
        [ a owl:Restriction ;
            owl:onProperty ns1:resultsIn ;
            owl:someValuesFrom ns1:LossOfConf ],
        ns1:MaliciousCodeExecution .

ns1:SerialError a owl:Class ;
    rdfs:comment "Formal definition for SerialError within the cybersecurity domain."^^xsd:string ;
    rdfs:subClassOf ns1:LogicExploit .

ns1:SynFlood a owl:Class ;
    rdfs:comment "Formal definition for SynFlood within the cybersecurity domain."^^xsd:string ;
    rdfs:subClassOf [ a owl:Restriction ;
            owl:onProperty ns1:resultsIn ;
            owl:someValuesFrom ns1:NetFlood ],
        ns1:Means .

ns1:SynScan a owl:Class ;
    rdfs:comment "Formal definition for SynScan within the cybersecurity domain."^^xsd:string ;
    rdfs:subClassOf ns1:Probe .

ns1:SysCrash a owl:Class ;
    rdfs:comment "Formal definition for SysCrash within the cybersecurity domain."^^xsd:string ;
    rdfs:seeAlso "http://dbpedia.org/resource/Fatal_system_error"^^xsd:anyURI ;
    rdfs:subClassOf ns1:DenialOfService .

ns1:TCPConnect a owl:Class ;
    rdfs:comment "Formal definition for TCPConnect within the cybersecurity domain."^^xsd:string ;
    rdfs:subClassOf ns1:Probe .

ns1:TCPPortScan a owl:Class ;
    rdfs:comment "Formal definition for TCPPortScan within the cybersecurity domain."^^xsd:string ;
    rdfs:subClassOf [ a owl:Restriction ;
            owl:onProperty ns1:resultsIn ;
            owl:someValuesFrom ns1:DirectoryExposure ],
        ns1:Probe .

ns1:Time a owl:Class ;
    rdfs:comment "Formal definition for Time within the cybersecurity domain."^^xsd:string ;
    rdfs:subClassOf ns1:TriggeredCode .

ns1:Trojans a owl:Class ;
    rdfs:comment "Formal definition for Trojans within the cybersecurity domain."^^xsd:string ;
    rdfs:subClassOf [ a owl:Restriction ;
            owl:onProperty ns1:resultsIn ;
            owl:someValuesFrom ns1:RemoteAccess ],
        [ a owl:Restriction ;
            owl:onProperty ns1:resultsIn ;
            owl:someValuesFrom ns1:LossOfConf ],
        ns1:MaliciousCodeExecution .

ns1:UnauthRoot a owl:Class ;
    rdfs:comment "Formal definition for UnauthRoot within the cybersecurity domain."^^xsd:string ;
    rdfs:subClassOf ns1:PrivilegeEsc .

ns1:UserEnumeration a owl:Class ;
    rdfs:comment "Formal definition for UserEnumeration within the cybersecurity domain."^^xsd:string ;
    rdfs:subClassOf [ a owl:Restriction ;
            owl:onProperty ns1:resultsIn ;
            owl:someValuesFrom ns1:PrivilegeEsc ],
        ns1:Means .

ns1:Virus a owl:Class ;
    rdfs:comment "Formal definition for Virus within the cybersecurity domain."^^xsd:string ;
    rdfs:seeAlso "http://dbpedia.org/resource/Computer_virus"^^xsd:anyURI ;
    rdfs:subClassOf ns1:SelfPropagatingCode .

ns1:WebBrowser a owl:Class ;
    rdfs:comment "Formal definition for WebBrowser within the cybersecurity domain."^^xsd:string ;
    rdfs:seeAlso "http://dbpedia.org/class/yago/WebBrowser"^^xsd:anyURI ;
    rdfs:subClassOf ns1:Software .

ns1:Worm a owl:Class ;
    rdfs:comment "Formal definition for Worm within the cybersecurity domain."^^xsd:string ;
    rdfs:seeAlso "http://dbpedia.org/resource/Computer_worm"^^xsd:anyURI ;
    rdfs:subClassOf ns1:SelfPropagatingCode .

ns1:anomolousDataOutFlow a owl:DatatypeProperty ;
    rdfs:domain ns1:NetworkState ;
    rdfs:range xsd:boolean .

ns1:chgGid a owl:DatatypeProperty ;
    rdfs:domain ns1:Process ;
    rdfs:range xsd:boolean .

ns1:chgPPid a owl:DatatypeProperty ;
    rdfs:domain ns1:Process ;
    rdfs:range xsd:boolean .

ns1:chgSUid a owl:DatatypeProperty ;
    rdfs:domain ns1:Process ;
    rdfs:range xsd:boolean .

ns1:chgUid a owl:DatatypeProperty ;
    rdfs:domain ns1:Process ;
    rdfs:range xsd:boolean .

ns1:commonConsequences a owl:DatatypeProperty ;
    rdfs:domain ns1:CWE ;
    rdfs:range xsd:string .

ns1:connectedTo a owl:IrreflexiveProperty,
        owl:ObjectProperty,
        owl:SymmetricProperty ;
    rdfs:domain ns1:System ;
    rdfs:range ns1:System .

ns1:cweExtendedSummary a owl:DatatypeProperty ;
    rdfs:domain ns1:CWE ;
    rdfs:range xsd:string .

ns1:cweID a owl:DatatypeProperty ;
    rdfs:domain ns1:CWE ;
    rdfs:range xsd:string .

ns1:cweName a owl:DatatypeProperty ;
    rdfs:domain ns1:CWE ;
    rdfs:range xsd:string .

ns1:cweSummary a owl:DatatypeProperty ;
    rdfs:domain ns1:CWE ;
    rdfs:range xsd:string .

ns1:dataSize a owl:DatatypeProperty ;
    rdfs:domain ns1:Process ;
    rdfs:range xsd:integer .

ns1:description a owl:DatatypeProperty ;
    rdfs:domain ns1:CWE ;
    rdfs:range xsd:string .

ns1:generated-on-datetime a owl:DatatypeProperty ;
    rdfs:domain ns1:Vulnerability ;
    rdfs:range xsd:string ;
    rdfs:subPropertyOf ns1:hasSeverityScore .

ns1:hasAccessComplexity a owl:DatatypeProperty ;
    rdfs:domain ns1:Vulnerability ;
    rdfs:range xsd:string ;
    rdfs:subPropertyOf ns1:hasSeverityScore .

ns1:hasAccessVector a owl:DatatypeProperty ;
    rdfs:domain ns1:Vulnerability ;
    rdfs:range xsd:string ;
    rdfs:subPropertyOf ns1:hasSeverityScore .

ns1:hasAuthentication a owl:DatatypeProperty ;
    rdfs:domain ns1:Vulnerability ;
    rdfs:range xsd:string ;
    rdfs:subPropertyOf ns1:hasSeverityScore .

ns1:hasAvailabilityImpact a owl:DatatypeProperty ;
    rdfs:domain ns1:Vulnerability ;
    rdfs:range xsd:string ;
    rdfs:subPropertyOf ns1:hasSeverityScore .

ns1:hasCodeSize a owl:DatatypeProperty ;
    rdfs:domain ns1:Process ;
    rdfs:range xsd:integer .

ns1:hasConfidentialityImpact a owl:DatatypeProperty ;
    rdfs:domain ns1:Vulnerability ;
    rdfs:range xsd:string ;
    rdfs:subPropertyOf ns1:hasSeverityScore .

ns1:hasDataSize a owl:DatatypeProperty ;
    rdfs:domain ns1:Process,
        ns1:UCOThing ;
    rdfs:range xsd:integer .

ns1:hasIntegrityImpact a owl:DatatypeProperty ;
    rdfs:domain ns1:Vulnerability ;
    rdfs:range xsd:string ;
    rdfs:subPropertyOf ns1:hasSeverityScore .

ns1:hasLibSize a owl:DatatypeProperty ;
    rdfs:domain ns1:Process ;
    rdfs:range xsd:integer .

ns1:hasVulnerabilityTerm a owl:DatatypeProperty ;
    rdfs:domain ns1:Web ;
    rdfs:range xsd:boolean .

ns1:isNew a owl:DatatypeProperty ;
    rdfs:domain ns1:Hardware,
        ns1:KernelModule ;
    rdfs:range xsd:boolean .

ns1:isResultOf a owl:IrreflexiveProperty,
        owl:ObjectProperty ;
    rdfs:domain ns1:Consequence ;
    rdfs:range ns1:Means ;
    owl:inverseOf ns1:resultsIn .

ns1:lastModifiedDateTime a owl:DatatypeProperty ;
    rdfs:domain ns1:Vulnerability ;
    rdfs:range xsd:dateTime .

ns1:newDestIP a owl:DatatypeProperty ;
    rdfs:domain ns1:NetworkState ;
    rdfs:range xsd:boolean .

ns1:newPortsOpened a owl:DatatypeProperty ;
    rdfs:domain ns1:NetworkState ;
    rdfs:range xsd:boolean .

ns1:numChildProcesses a owl:DatatypeProperty ;
    rdfs:domain ns1:Process ;
    rdfs:range xsd:integer .

ns1:numOpenFiles a owl:DatatypeProperty ;
    rdfs:domain ns1:Process ;
    rdfs:range xsd:integer .

ns1:numProcessesRunning a owl:DatatypeProperty ;
    rdfs:domain ns1:System ;
    rdfs:range xsd:integer .

ns1:opensPort a owl:DatatypeProperty ;
    rdfs:domain ns1:Process ;
    rdfs:range xsd:integer .

ns1:publishedDateTime a owl:DatatypeProperty ;
    rdfs:domain ns1:Vulnerability ;
    rdfs:range xsd:dateTime .

ns1:rstProbe a owl:Class ;
    rdfs:comment "Formal definition for rstProbe within the cybersecurity domain."^^xsd:string ;
    rdfs:subClassOf ns1:Probe .

ns1:score a owl:DatatypeProperty ;
    rdfs:domain ns1:Vulnerability ;
    rdfs:range xsd:float ;
    rdfs:subPropertyOf ns1:hasSeverityScore .

ns1:selfDist a owl:DatatypeProperty ;
    rdfs:domain ns1:Process ;
    rdfs:range xsd:integer .

ns1:showsInfectionSigns a owl:DatatypeProperty ;
    rdfs:domain ns1:Process ;
    rdfs:range xsd:boolean .

ns1:summary a owl:DatatypeProperty ;
    rdfs:domain ns1:Vulnerability ;
    rdfs:range xsd:string .

ns1:timeOfIntroduction a owl:DatatypeProperty ;
    rdfs:domain ns1:CWE ;
    rdfs:range xsd:dateTime .

ns2:008a59674de43150 a ns2:AnonymousAttack,
        owl:NamedIndividual ;
    ns1:associatedCampaigns ns2:British_National_Party ;
    ns2:hasActor "Anonymous"^^xsd:string ;
    ns2:hasActorType "Hacktivist"^^xsd:string ;
    ns2:hasCountry "United Kingdom of Great Britain and Northern Ireland"^^xsd:string ;
    ns2:hasEventDate "2014-05-02T00:00:00"^^xsd:dateTime ;
    ns2:hasEventSubtype "Message Manipulation"^^xsd:string ;
    ns2:hasEventType "Disruptive"^^xsd:string ;
    ns2:hasIndustry "Other Services (except Public Administration)"^^xsd:string ;
    ns2:hasMonth 5 ;
    ns2:hasOrganization "British National Party"^^xsd:string ;
    ns2:hasYear 2014 ;
    ns2:isType_of ns2:Hacktivist,
        ns2:Message_Manipulation ;
    rdfs:comment "The official Twitter account of the British National Party and its leader is hacked by Anon_0x03,  an individual claiming to be affiliated to the infamous collective Anonymous."^^xsd:string .

ns2:02bbc332422baf37 a ns2:DDoS,
        owl:NamedIndividual ;
    ns1:associatedCampaigns ns2:Hootsuite ;
    ns1:description "Financial"^^xsd:string ;
    ns2:behaviour ns2:Financial ;
    ns2:hasActorType "Criminal"^^xsd:string ;
    ns2:hasCountry "Canada"^^xsd:string ;
    ns2:hasEventDate "2014-03-21T00:00:00"^^xsd:dateTime ;
    ns2:hasEventSubtype "External Denial of Service"^^xsd:string ;
    ns2:hasEventType "Disruptive"^^xsd:string ;
    ns2:hasIndustry "Professional, Scientific, and Technical Services"^^xsd:string ;
    ns2:hasMonth 3 ;
    ns2:hasOrganization "Hootsuite"^^xsd:string ;
    ns2:hasYear 2014 ;
    ns2:isType_of ns2:Criminal,
        ns2:External_Denial_of_Service ;
    rdfs:comment "Hootsuite is the victim of a DDoS Attack."^^xsd:string .

ns2:0300580af5e9ab8b a ns2:DDoS,
        owl:NamedIndividual ;
    ns1:associatedCampaigns ns2:Move__Inc ;
    ns2:hasActorType "Criminal"^^xsd:string ;
    ns2:hasCampaign ns2:California ;
    ns2:hasCountry "United States of America"^^xsd:string ;
    ns2:hasCounty "Santa Clara"^^xsd:string ;
    ns2:hasEventDate "2014-06-18T00:00:00"^^xsd:dateTime ;
    ns2:hasEventSubtype "External Denial of Service"^^xsd:string ;
    ns2:hasEventType "Disruptive"^^xsd:string ;
    ns2:hasIndustry "Real Estate and Rental and Leasing"^^xsd:string ;
    ns2:hasMonth 6 ;
    ns2:hasOrganization "Move, Inc."^^xsd:string ;
    ns2:hasState "California"^^xsd:string ;
    ns2:hasYear 2014 ;
    ns2:isType_of ns2:Criminal,
        ns2:External_Denial_of_Service ;
    rdfs:comment "Move, Inc. is hit by a major DDoS attack."^^xsd:string .

ns2:03a2f82efbca7bd8 a ns2:AccountAttack,
        owl:NamedIndividual ;
    ns1:associatedCampaigns ns2:Butler_University ;
    ns1:description "Financial"^^xsd:string ;
    ns2:behaviour ns2:Financial ;
    ns2:hasActorType "Criminal"^^xsd:string ;
    ns2:hasCampaign ns2:Indiana ;
    ns2:hasCountry "United States of America"^^xsd:string ;
    ns2:hasCounty "Marion"^^xsd:string ;
    ns2:hasEventDate "2014-06-30T00:00:00"^^xsd:dateTime ;
    ns2:hasEventSubtype "Exploitation of Application Server"^^xsd:string ;
    ns2:hasEventType "Exploitive"^^xsd:string ;
    ns2:hasIndustry "Educational Services"^^xsd:string ;
    ns2:hasMonth 6 ;
    ns2:hasOrganization "Butler University"^^xsd:string ;
    ns2:hasState "Indiana"^^xsd:string ;
    ns2:hasYear 2014 ;
    ns2:isType_of ns2:Criminal,
        ns2:Exploitation_of_Application_Server ;
    rdfs:comment "Personal and financial information of some 163,000 students, alumni, faculty, staff, and past applicants of Indianapolis-based Butler University have been stolen following a hack of the university's computer network."^^xsd:string .

ns2:040a55840f4107f1 a ns2:DDoS,
        owl:NamedIndividual ;
    ns1:associatedCampaigns ns2:UltraDNS ;
    ns2:hasActorType "Criminal"^^xsd:string ;
    ns2:hasCampaign ns2:California ;
    ns2:hasCountry "United States of America"^^xsd:string ;
    ns2:hasCounty "Los Angeles"^^xsd:string ;
    ns2:hasEventDate "2014-04-30T00:00:00"^^xsd:dateTime ;
    ns2:hasEventSubtype "External Denial of Service"^^xsd:string ;
    ns2:hasEventType "Disruptive"^^xsd:string ;
    ns2:hasIndustry "Professional, Scientific, and Technical Services"^^xsd:string ;
    ns2:hasMonth 4 ;
    ns2:hasOrganization "UltraDNS"^^xsd:string ;
    ns2:hasState "California"^^xsd:string ;
    ns2:hasYear 2014 ;
    ns2:isType_of ns2:Criminal,
        ns2:External_Denial_of_Service ;
    rdfs:comment "UltraDNS is the victim of a DDoS Attack."^^xsd:string .

ns2:04574788ee636fe5 a ns2:CyberattackData,
        owl:NamedIndividual ;
    ns1:associatedCampaigns ns2:Chevrolet ;
    ns1:isLaunchedBy ns2:Pakistan ;
    ns2:hasActor "Team Cyber Criminals"^^xsd:string ;
    ns2:hasActorCountry "Pakistan"^^xsd:string ;
    ns2:hasActorType "Hobbyist"^^xsd:string ;
    ns2:hasCountry "Guatemala"^^xsd:string ;
    ns2:hasEventDate "2014-03-18T00:00:00"^^xsd:dateTime ;
    ns2:hasEventSubtype "Message Manipulation"^^xsd:string ;
    ns2:hasEventType "Disruptive"^^xsd:string ;
    ns2:hasIndustry "Manufacturing"^^xsd:string ;
    ns2:hasMonth 3 ;
    ns2:hasOrganization "Chevrolet"^^xsd:string ;
    ns2:hasYear 2014 ;
    ns2:isType_of ns2:Hobbyist,
        ns2:Message_Manipulation ;
    rdfs:comment "The Guatemala websites of Renault, Toyota and Chevrolet are hacked and defaced by a member of a Pakistani group called Team Cyber Criminals."^^xsd:string .

ns2:047a31dcdf071666 a ns2:AccountAttack,
        owl:NamedIndividual ;
    ns1:associatedCampaigns ns2:Church_of_Cyprus ;
    ns2:hasActor "@security_511"^^xsd:string ;
    ns2:hasActorType "Hobbyist"^^xsd:string ;
    ns2:hasCountry "Cyprus"^^xsd:string ;
    ns2:hasEventDate "2014-03-05T00:00:00"^^xsd:dateTime ;
    ns2:hasEventSubtype "Exploitation of Application Server"^^xsd:string ;
    ns2:hasEventType "Exploitive"^^xsd:string ;
    ns2:hasIndustry "Other Services (except Public Administration)"^^xsd:string ;
    ns2:hasMonth 3 ;
    ns2:hasOrganization "Church of Cyprus"^^xsd:string ;
    ns2:hasYear 2014 ;
    ns2:isType_of ns2:Exploitation_of_Application_Server,
        ns2:Hobbyist ;
    rdfs:comment "The hacker @security_511 hacks the Church of Cyprus website (churchofcyprus.org.cy) and dumps 1,476 user account credentials with full names, email addresses and encrypted passwords."^^xsd:string .

ns2:0483005f1ecd785e a ns2:HackerSecurity,
        owl:NamedIndividual ;
    ns1:associatedCampaigns ns2:Boxee_tv ;
    ns2:hasActorType "Criminal"^^xsd:string ;
    ns2:hasCountry "United States of America"^^xsd:string ;
    ns2:hasEventDate "2014-04-01T00:00:00"^^xsd:dateTime ;
    ns2:hasEventSubtype "Exploitation of Application Server"^^xsd:string ;
    ns2:hasEventType "Exploitive"^^xsd:string ;
    ns2:hasIndustry "Information"^^xsd:string ;
    ns2:hasMonth 4 ;
    ns2:hasOrganization "Boxee.tv"^^xsd:string ;
    ns2:hasYear 2014 ;
    ns2:isType_of ns2:Criminal,
        ns2:Exploitation_of_Application_Server ;
    rdfs:comment "Hackers post names, e-mail addresses, message histories, and partially protected login credentials for more than 158,000 forum users of Boxee.tv, the Web-based television service that was acquired by Samsung last year."^^xsd:string .

ns2:0515d0acb723dc43 a ns2:BreachSecurity,
        owl:NamedIndividual ;
    ns1:associatedCampaigns ns2:Iowa_State_University ;
    ns1:description "Financial"^^xsd:string ;
    ns2:behaviour ns2:Financial ;
    ns2:hasActorType "Criminal"^^xsd:string ;
    ns2:hasCampaign ns2:Iowa ;
    ns2:hasCountry "United States of America"^^xsd:string ;
    ns2:hasCounty "Story"^^xsd:string ;
    ns2:hasEventDate "2014-04-22T00:00:00"^^xsd:dateTime ;
    ns2:hasEventSubtype "Exploitation of Application Server"^^xsd:string ;
    ns2:hasEventType "Exploitive"^^xsd:string ;
    ns2:hasIndustry "Educational Services"^^xsd:string ;
    ns2:hasMonth 4 ;
    ns2:hasOrganization "Iowa State University"^^xsd:string ;
    ns2:hasState "Iowa"^^xsd:string ;
    ns2:hasYear 2014 ;
    ns2:isType_of ns2:Criminal,
        ns2:Exploitation_of_Application_Server ;
    rdfs:comment "Information technology staff at Iowa State University discovers a breach affecting five departmental servers on campus potentially compromising Social Security numbers of 29,780 students enrolled at Iowa State between 1995 and 2012."^^xsd:string .

ns2:05a2251c85707580 a ns2:AttackWebsite,
        owl:NamedIndividual ;
    ns1:associatedCampaigns ns2:Armenian_President_Website ;
    ns1:description "Protest"^^xsd:string ;
    ns1:isLaunchedBy ns2:Azerbaijan ;
    ns2:behaviour ns2:Protest ;
    ns2:hasActor "Anti-Armenia Team"^^xsd:string ;
    ns2:hasActorCountry "Azerbaijan"^^xsd:string ;
    ns2:hasActorType "Hacktivist"^^xsd:string ;
    ns2:hasCountry "Armenia"^^xsd:string ;
    ns2:hasEventDate "2014-06-28T00:00:00"^^xsd:dateTime ;
    ns2:hasEventSubtype "Message Manipulation"^^xsd:string ;
    ns2:hasEventType "Disruptive"^^xsd:string ;
    ns2:hasIndustry "Public Administration"^^xsd:string ;
    ns2:hasMonth 6 ;
    ns2:hasOrganization "Armenian President Website"^^xsd:string ;
    ns2:hasYear 2014 ;
    ns2:isType_of ns2:Hacktivist,
        ns2:Message_Manipulation ;
    rdfs:comment "On the day of the celebration of the Armed Forces of Azerbaijan, Azerbaijani hackers from Anti-Armenia Team deface the official website of the Armenian President and other government sites."^^xsd:string .

ns2:05b062e6e3d67e7e a ns2:BreachSecurity,
        owl:NamedIndividual ;
    ns1:associatedCampaigns ns2:The_Straight_Dope ;
    ns2:hasActorType "Criminal"^^xsd:string ;
    ns2:hasCampaign ns2:Illinois ;
    ns2:hasCountry "United States of America"^^xsd:string ;
    ns2:hasCounty "Cook"^^xsd:string ;
    ns2:hasEventDate "2014-01-09T00:00:00"^^xsd:dateTime ;
    ns2:hasEventSubtype "Exploitation of Application Server"^^xsd:string ;
    ns2:hasEventType "Exploitive"^^xsd:string ;
    ns2:hasIndustry "Information"^^xsd:string ;
    ns2:hasMonth 1 ;
    ns2:hasOrganization "The Straight Dope"^^xsd:string ;
    ns2:hasState "Illinois"^^xsd:string ;
    ns2:hasYear 2014 ;
    ns2:isType_of ns2:Criminal,
        ns2:Exploitation_of_Application_Server ;
    rdfs:comment "The Straight Dope, the popular online question and answer newspaper column, advises users of its forum to change their passwords because the information might have been compromised in a recent attack targeted at the bulletin board."^^xsd:string .

ns2:05e203d87f5a086a a ns2:CyberattackData,
        owl:NamedIndividual ;
    ns1:associatedCampaigns ns2:Belgian_Foreign_Ministry ;
    ns1:description "Political-Espionage"^^xsd:string ;
    ns2:behaviour ns2:Political_Espionage ;
    ns2:hasActorType "Criminal"^^xsd:string ;
    ns2:hasCountry "Belgium"^^xsd:string ;
    ns2:hasEventDate "2014-05-12T00:00:00"^^xsd:dateTime ;
    ns2:hasEventSubtype "Exploitation of Application Server"^^xsd:string ;
    ns2:hasEventType "Exploitive"^^xsd:string ;
    ns2:hasIndustry "Public Administration"^^xsd:string ;
    ns2:hasMonth 5 ;
    ns2:hasOrganization "Belgian Foreign Ministry"^^xsd:string ;
    ns2:hasYear 2014 ;
    ns2:isType_of ns2:Criminal,
        ns2:Exploitation_of_Application_Server ;
    rdfs:comment "Unknown hackers steal data related to the Ukraine crisis from Belgian foreign ministry servers, prompting a security crackdown which has left diplomats without Internet or email."^^xsd:string .

ns2:05eb17480d1a9a08 a ns2:AttackSchool,
        owl:NamedIndividual ;
    ns1:associatedCampaigns ns2:Dr__Micharl_M__Krop_Senior_High_School ;
    ns1:isLaunchedBy ns2:United_States_of_America ;
    ns2:hasActor "Jose Bautista"^^xsd:string ;
    ns2:hasActorCountry "United States of America"^^xsd:string ;
    ns2:hasActorType "Criminal"^^xsd:string ;
    ns2:hasCampaign ns2:Florida ;
    ns2:hasCountry "United States of America"^^xsd:string ;
    ns2:hasCounty "Miami-Dade"^^xsd:string ;
    ns2:hasEventDate "2014-05-02T00:00:00"^^xsd:dateTime ;
    ns2:hasEventSubtype "Data Attack"^^xsd:string ;
    ns2:hasEventType "Disruptive"^^xsd:string ;
    ns2:hasIndustry "Educational Services"^^xsd:string ;
    ns2:hasMonth 5 ;
    ns2:hasOrganization "Dr. Micharl M. Krop Senior High School"^^xsd:string ;
    ns2:hasState "Florida"^^xsd:string ;
    ns2:hasYear 2014 ;
    ns2:isType_of ns2:Criminal,
        ns2:Data_Attack ;
    rdfs:comment "An 18-year old student appears before a judge after he was arrested for allegedlyÃÆÃ'Ãâ 'ÃÆÃ¢â¬Â 'ÃÆÃ'ÃÂ¢Ã¢'Â¬ÃÂ ''ÃÆÃ'Ãâ 'ÃÆÃ¢â¬Â ''ÃÆÃ'Ãâ ''ÃÆÃ''ÃÆ'Ã'ÃÂ changing grades for students in Dr. Michael M. Krop Senior High School."^^xsd:string .

ns2:06131416eaf6fa1d a ns2:Phishing,
        owl:NamedIndividual ;
    ns1:associatedCampaigns ns2:National_Informatics_Center ;
    ns2:hasActorType "Criminal"^^xsd:string ;
    ns2:hasCountry "India"^^xsd:string ;
    ns2:hasEventDate "2014-07-09T00:00:00"^^xsd:dateTime ;
    ns2:hasEventSubtype "Exploitation of Data in Transit"^^xsd:string ;
    ns2:hasEventType "Exploitive"^^xsd:string ;
    ns2:hasIndustry "Public Administration"^^xsd:string ;
    ns2:hasMonth 7 ;
    ns2:hasOrganization "National Informatics Center"^^xsd:string ;
    ns2:hasYear 2014 ;
    ns2:isType_of ns2:Criminal,
        ns2:Exploitation_of_Data_in_Transit ;
    rdfs:comment "The Indian NIC is compromised to issue fake digital certificates. Google immediately revokes them."^^xsd:string .

ns2:06470105603e5210 a ns2:DefaceHacker,
        owl:NamedIndividual ;
    ns1:associatedCampaigns ns2:Bihar_Bharatiya_Janata_Party ;
    ns1:isLaunchedBy ns2:India ;
    ns2:hasActor "Muhammad Bilal"^^xsd:string ;
    ns2:hasActorCountry "India"^^xsd:string ;
    ns2:hasActorType "Hacktivist"^^xsd:string ;
    ns2:hasCountry "India"^^xsd:string ;
    ns2:hasEventDate "2014-04-19T00:00:00"^^xsd:dateTime ;
    ns2:hasEventSubtype "Message Manipulation"^^xsd:string ;
    ns2:hasEventType "Disruptive"^^xsd:string ;
    ns2:hasIndustry "Other Services (except Public Administration)"^^xsd:string ;
    ns2:hasMonth 4 ;
    ns2:hasOrganization "Bihar Bharatiya Janata Party"^^xsd:string ;
    ns2:hasYear 2014 ;
    ns2:isType_of ns2:Hacktivist,
        ns2:Message_Manipulation ;
    rdfs:comment "A hacker called Muhammad Bilal from Pak Cyber Experts group defaces the official Bihar BJP website (biharbjp.org)."^^xsd:string .

ns2:06f1349d3738afcf a ns2:CyberattackData,
        owl:NamedIndividual ;
    ns1:associatedCampaigns ns2:Monju_Nuclear_Power_Plant ;
    ns2:hasActorType "Criminal"^^xsd:string ;
    ns2:hasCountry "Japan"^^xsd:string ;
    ns2:hasEventDate "2014-01-06T00:00:00"^^xsd:dateTime ;
    ns2:hasEventSubtype "Exploitation of Application Server"^^xsd:string ;
    ns2:hasEventType "Exploitive"^^xsd:string ;
    ns2:hasIndustry "Utilities"^^xsd:string ;
    ns2:hasMonth 1 ;
    ns2:hasOrganization "Monju Nuclear Power Plant"^^xsd:string ;
    ns2:hasYear 2014 ;
    ns2:isType_of ns2:Criminal,
        ns2:Exploitation_of_Application_Server ;
    rdfs:comment "A server administrator discovers that one of the eight computers in the reactor control room of the Monju Nuclear Plant has been accessed over 30 times in the last five days. More than 42,000 e-mails and staff training reports were stored on the computer."^^xsd:string .

ns2:075e48641f9fa231 a ns2:CyberattackData,
        owl:NamedIndividual ;
    ns1:associatedCampaigns ns2:Gas_Distribution_Authority_of_Sakarya ;
    ns1:description "Protest"^^xsd:string ;
    ns1:isLaunchedBy ns2:Turkey ;
    ns2:behaviour ns2:Protest ;
    ns2:hasActor "RedHack"^^xsd:string ;
    ns2:hasActorCountry "Turkey"^^xsd:string ;
    ns2:hasActorType "Hacktivist"^^xsd:string ;
    ns2:hasCountry "Turkey"^^xsd:string ;
    ns2:hasEventDate "2014-02-10T00:00:00"^^xsd:dateTime ;
    ns2:hasEventSubtype "Message Manipulation"^^xsd:string ;
    ns2:hasEventType "Disruptive"^^xsd:string ;
    ns2:hasIndustry "Public Administration"^^xsd:string ;
    ns2:hasMonth 2 ;
    ns2:hasOrganization "Gas Distribution Authority of Sakarya"^^xsd:string ;
    ns2:hasYear 2014 ;
    ns2:isType_of ns2:Hacktivist,
        ns2:Message_Manipulation ;
    rdfs:comment "The infamous RedHack collective joins the protests against the new Internet Law, and leak around two dozen records. They also deface a couple of local sites and hack the Ministry of Education."^^xsd:string .

ns2:07b2cbeeecd4e11b a ns2:AnonymousAttack,
        owl:NamedIndividual ;
    ns1:associatedCampaigns ns2:Mossad ;
    ns1:description "Protest"^^xsd:string ;
    ns2:behaviour ns2:Protest ;
    ns2:hasActor "Anonymous"^^xsd:string ;
    ns2:hasActorType "Hacktivist"^^xsd:string ;
    ns2:hasCountry "Israel"^^xsd:string ;
    ns2:hasEventDate "2014-08-02T00:00:00"^^xsd:dateTime ;
    ns2:hasEventSubtype "External Denial of Service"^^xsd:string ;
    ns2:hasEventType "Disruptive"^^xsd:string ;
    ns2:hasIndustry "Public Administration"^^xsd:string ;
    ns2:hasMonth 8 ;
    ns2:hasOrganization "Mossad"^^xsd:string ;
    ns2:hasYear 2014 ;
    ns2:isType_of ns2:External_Denial_of_Service,
        ns2:Hacktivist ;
    rdfs:comment "In name of #OpSaveGaza, the Anonymous collective claims responsibility of taking down the websites of: bankisrael.gov.il, mossad.gov.il, justice.gov.il, edu.gov.il, idf.gov.il, telaviv.police.gov.il."^^xsd:string .

ns2:07e56a3d9e72e35d a ns2:AttackWebsite,
        owl:NamedIndividual ;
    ns1:associatedCampaigns ns2:Ministry_of_Health ;
    ns1:description "Protest"^^xsd:string ;
    ns1:isLaunchedBy ns2:Saudi_Arabia ;
    ns2:behaviour ns2:Protest ;
    ns2:hasActor "Moroccan Islamic Union-Mail"^^xsd:string ;
    ns2:hasActorCountry "Saudi Arabia"^^xsd:string ;
    ns2:hasActorType "Hacktivist"^^xsd:string ;
    ns2:hasCountry "Saudi Arabia"^^xsd:string ;
    ns2:hasEventDate "2014-04-10T00:00:00"^^xsd:dateTime ;
    ns2:hasEventSubtype "Message Manipulation"^^xsd:string ;
    ns2:hasEventType "Disruptive"^^xsd:string ;
    ns2:hasIndustry "Public Administration"^^xsd:string ;
    ns2:hasMonth 4 ;
    ns2:hasOrganization "Ministry of Health"^^xsd:string ;
    ns2:hasYear 2014 ;
    ns2:isType_of ns2:Hacktivist,
        ns2:Message_Manipulation ;
    rdfs:comment "Hackers of Moroccan Islamic Union-Mail deface the official website of prevention program of injuries and accidents - Ministry of Health Saudi Arabia (moh-ncd.gov.sa)."^^xsd:string .

ns2:0851399a0462bcb5 a ns2:BreachInformation,
        owl:NamedIndividual ;
    ns1:associatedCampaigns ns2:McKayla_Maroney ;
    ns1:description "Personal Attack"^^xsd:string ;
    ns2:behaviour ns2:Personal_Attack ;
    ns2:hasActorType "Criminal"^^xsd:string ;
    ns2:hasCountry "United States of America"^^xsd:string ;
    ns2:hasEventDate "2014-08-31T00:00:00"^^xsd:dateTime ;
    ns2:hasEventSubtype "Exploitation of Application Server"^^xsd:string ;
    ns2:hasEventType "Exploitive"^^xsd:string ;
    ns2:hasIndustry "Other Services (except Public Administration)"^^xsd:string ;
    ns2:hasMonth 8 ;
    ns2:hasOrganization "McKayla Maroney"^^xsd:string ;
    ns2:hasYear 2014 ;
    ns2:isType_of ns2:Criminal,
        ns2:Exploitation_of_Application_Server ;
    rdfs:comment "Yet another leak of celebrities pictures. A massive leak of nude and risque photos appearing to be of huge stars like is leaked online, first appearing on 4chan."^^xsd:string .

ns2:08c366124c18b433 a ns2:HackerSecurity,
        owl:NamedIndividual ;
    ns1:associatedCampaigns ns2:ESET ;
    ns2:hasActor "Hmei7"^^xsd:string ;
    ns2:hasActorType "Hobbyist"^^xsd:string ;
    ns2:hasCountry "Slovakia"^^xsd:string ;
    ns2:hasEventDate "2014-06-04T00:00:00"^^xsd:dateTime ;
    ns2:hasEventSubtype "Message Manipulation"^^xsd:string ;
    ns2:hasEventType "Disruptive"^^xsd:string ;
    ns2:hasIndustry "Professional, Scientific, and Technical Services"^^xsd:string ;
    ns2:hasMonth 6 ;
    ns2:hasOrganization "ESET"^^xsd:string ;
    ns2:hasYear 2014 ;
    ns2:isType_of ns2:Hobbyist,
        ns2:Message_Manipulation ;
    rdfs:comment "A hacker called Hmeidefaces the official website of ESETand 4 of itsSpanish domains."^^xsd:string .

ns2:0991398a506e7029 a ns2:AnonymousAttack,
        owl:NamedIndividual ;
    ns1:associatedCampaigns ns2:Israel_Defense_Forces ;
    ns1:description "Protest"^^xsd:string ;
    ns2:behaviour ns2:Protest ;
    ns2:hasActor "Anonymous"^^xsd:string ;
    ns2:hasActorType "Hacktivist"^^xsd:string ;
    ns2:hasCountry "Israel"^^xsd:string ;
    ns2:hasEventDate "2014-08-25T00:00:00"^^xsd:dateTime ;
    ns2:hasEventSubtype "External Denial of Service"^^xsd:string ;
    ns2:hasEventType "Disruptive"^^xsd:string ;
    ns2:hasIndustry "Public Administration"^^xsd:string ;
    ns2:hasMonth 8 ;
    ns2:hasOrganization "Israel Defense Forces"^^xsd:string ;
    ns2:hasYear 2014 ;
    ns2:isType_of ns2:External_Denial_of_Service,
        ns2:Hacktivist ;
    rdfs:comment "In name of #OpSaveGaza, the Anonymous collective claims to have taken down some key Israeli governmental websites, including those of the Israeli Defense Forces, the Bank of Israel, the Israeli Prime Minister."^^xsd:string .

ns2:09c78aef49c8957f a ns2:AttackWebsite,
        owl:NamedIndividual ;
    ns1:associatedCampaigns ns2:helpmaidan_org_ua ;
    ns2:hasActorType "Criminal"^^xsd:string ;
    ns2:hasCountry "Ukraine"^^xsd:string ;
    ns2:hasEventDate "2014-02-28T00:00:00"^^xsd:dateTime ;
    ns2:hasEventSubtype "External Denial of Service"^^xsd:string ;
    ns2:hasEventType "Disruptive"^^xsd:string ;
    ns2:hasIndustry "Other Services (except Public Administration)"^^xsd:string ;
    ns2:hasMonth 2 ;
    ns2:hasOrganization "helpmaidan.org.ua"^^xsd:string ;
    ns2:hasYear 2014 ;
    ns2:isType_of ns2:Criminal,
        ns2:External_Denial_of_Service ;
    rdfs:comment "Hacktivists continue to launch attacks against Ukrainian government websites. The latest targets are the sites of the parliament, or the Verkhovna Rada (rada.gov.ua), the Right Sector nationalist movement (banderivets.org.ua), but also some Euromaidan websites."^^xsd:string .

ns2:09f06060c9ba0953 a ns2:CyberattackInformation,
        owl:NamedIndividual ;
    ns1:associatedCampaigns ns2:Malaysian_Department_of_Civil_Aviation ;
    ns2:hasActorType "Criminal"^^xsd:string ;
    ns2:hasCountry "Malaysia"^^xsd:string ;
    ns2:hasEventDate "2014-08-20T00:00:00"^^xsd:dateTime ;
    ns2:hasEventSubtype "Exploitation of End Hosts"^^xsd:string ;
    ns2:hasEventType "Exploitive"^^xsd:string ;
    ns2:hasIndustry "Public Administration"^^xsd:string ;
    ns2:hasMonth 8 ;
    ns2:hasOrganization "Malaysian Department of Civil Aviation"^^xsd:string ;
    ns2:hasYear 2014 ;
    ns2:isType_of ns2:Criminal,
        ns2:Exploitation_of_End_Hosts ;
    rdfs:comment "The computers of high-ranking officials in Malaysian agencies involved in the MH370 investigation are hacked and classified information is stolen. Suspects are directed to China."^^xsd:string .

ns2:09f38af706e7beda a ns2:Phishing,
        owl:NamedIndividual ;
    ns1:associatedCampaigns ns2:British_Academy_of_Film_and_Television_A ;
    ns2:hasActorType "Criminal"^^xsd:string ;
    ns2:hasCountry "United Kingdom of Great Britain and Northern Ireland"^^xsd:string ;
    ns2:hasEventDate "2014-01-30T00:00:00"^^xsd:dateTime ;
    ns2:hasEventSubtype "Exploitation of Application Server"^^xsd:string ;
    ns2:hasEventType "Exploitive"^^xsd:string ;
    ns2:hasIndustry "Other Services (except Public Administration)"^^xsd:string ;
    ns2:hasMonth 1 ;
    ns2:hasOrganization "British Academy of Film and Television Arts"^^xsd:string ;
    ns2:hasYear 2014 ;
    ns2:isType_of ns2:Criminal,
        ns2:Exploitation_of_Application_Server ;
    rdfs:comment "The British Academy of Film and Television Arts (BAFTA) reveals that part of its website has been \"compromised by illegal means\" and it's not currently guaranteed that hackers haven't made off with details of individuals on the  BAFTA Guru mailing list."^^xsd:string .

ns2:0a28e8aee437968b a ns2:AnonymousAttack,
        owl:NamedIndividual ;
    ns1:associatedCampaigns ns2:DNB ;
    ns1:description "Protest"^^xsd:string ;
    ns1:isLaunchedBy ns2:Norway ;
    ns2:behaviour ns2:Protest ;
    ns2:hasActor "Anonymous (Norway)"^^xsd:string ;
    ns2:hasActorCountry "Norway"^^xsd:string ;
    ns2:hasActorType "Hacktivist"^^xsd:string ;
    ns2:hasCountry "Norway"^^xsd:string ;
    ns2:hasEventDate "2014-07-09T00:00:00"^^xsd:dateTime ;
    ns2:hasEventSubtype "External Denial of Service"^^xsd:string ;
    ns2:hasEventType "Disruptive"^^xsd:string ;
    ns2:hasIndustry "Finance and Insurance"^^xsd:string ;
    ns2:hasMonth 7 ;
    ns2:hasOrganization "DNB"^^xsd:string ;
    ns2:hasYear 2014 ;
    ns2:isType_of ns2:External_Denial_of_Service,
        ns2:Hacktivist ;
    rdfs:comment "Anonymous Norway starts multiple DDoS attacks towards major banks and insurance companies in Norway, including the country's largest telecommunications company, Telenor."^^xsd:string .

ns2:0a4b8ccabede4b76 a ns2:CyberattackData,
        owl:NamedIndividual ;
    ns1:associatedCampaigns ns2:Turkish_Ministry_of_Education ;
    ns1:description "Protest"^^xsd:string ;
    ns1:isLaunchedBy ns2:Turkey ;
    ns2:behaviour ns2:Protest ;
    ns2:hasActor "RedHack"^^xsd:string ;
    ns2:hasActorCountry "Turkey"^^xsd:string ;
    ns2:hasActorType "Hacktivist"^^xsd:string ;
    ns2:hasCountry "Turkey"^^xsd:string ;
    ns2:hasEventDate "2014-02-10T00:00:00"^^xsd:dateTime ;
    ns2:hasEventSubtype "Exploitation of Application Server"^^xsd:string ;
    ns2:hasEventType "Exploitive"^^xsd:string ;
    ns2:hasIndustry "Public Administration"^^xsd:string ;
    ns2:hasMonth 2 ;
    ns2:hasOrganization "Turkish Ministry of Education"^^xsd:string ;
    ns2:hasYear 2014 ;
    ns2:isType_of ns2:Exploitation_of_Application_Server,
        ns2:Hacktivist ;
    rdfs:comment "The infamous RedHack collective joins the protests against the new Internet Law, and leak around two dozen records. They also deface a couple of local sites and hack the Ministry of Education."^^xsd:string .

ns2:0c416574a35168f6 a ns2:AgencyAttack,
        owl:NamedIndividual ;
    ns1:associatedCampaigns ns2:Delaware_Treasury_Division ;
    ns1:description "Protest"^^xsd:string ;
    ns1:isLaunchedBy ns2:United_States_of_America ;
    ns2:behaviour ns2:Protest ;
    ns2:hasActor "SaLeM"^^xsd:string ;
    ns2:hasActorCountry "United States of America"^^xsd:string ;
    ns2:hasActorType "Hacktivist"^^xsd:string ;
    ns2:hasCampaign ns2:Delaware ;
    ns2:hasCountry "United States of America"^^xsd:string ;
    ns2:hasCounty "New Castle"^^xsd:string ;
    ns2:hasEventDate "2014-08-19T00:00:00"^^xsd:dateTime ;
    ns2:hasEventSubtype "Message Manipulation"^^xsd:string ;
    ns2:hasEventType "Disruptive"^^xsd:string ;
    ns2:hasIndustry "Public Administration"^^xsd:string ;
    ns2:hasMonth 8 ;
    ns2:hasOrganization "Delaware Treasury Division"^^xsd:string ;
    ns2:hasState "Delaware"^^xsd:string ;
    ns2:hasYear 2014 ;
    ns2:isType_of ns2:Hacktivist,
        ns2:Message_Manipulation ;
    rdfs:comment "Delaware's treasury division website (treasury.delaware.gov) is defaced with anti-Israel and pro-Palestine messages by a collective calling itself SaLeM."^^xsd:string .

ns2:0c6e7d31b84f3096 a ns2:HackUsernames,
        ns2:HackerSecurity,
        owl:NamedIndividual ;
    ns1:associatedCampaigns ns2:40dni_sk ;
    ns2:hasActor "r3dm0v3"^^xsd:string ;
    ns2:hasCountry "Slovakia"^^xsd:string ;
    ns2:hasEventDate "2014-04-12T00:00:00"^^xsd:dateTime ;
    ns2:hasEventSubtype "Exploitation of Application Server"^^xsd:string ;
    ns2:hasEventType "Exploitive"^^xsd:string ;
    ns2:hasIndustry "Other Services (except Public Administration)"^^xsd:string ;
    ns2:hasMonth 4 ;
    ns2:hasOrganization "40dni.sk"^^xsd:string ;
    ns2:hasYear 2014 ;
    ns2:isType_of ns2:Exploitation_of_Application_Server ;
    rdfs:comment "A hacker called r3dm0v3 hacks 40dni.sk and dumps about 4,800 usernames and hashed passwords."^^xsd:string .

ns2:0d5eda48eee60e38 a ns2:HackerSecurity,
        owl:NamedIndividual ;
    ns1:associatedCampaigns ns2:Lockheed_Martin ;
    ns1:description "Industrial-Espionage"^^xsd:string ;
    ns1:isLaunchedBy ns2:China ;
    ns2:behaviour ns2:Industrial_Espionage ;
    ns2:hasActor "Su Bin"^^xsd:string ;
    ns2:hasActorCountry "China"^^xsd:string ;
    ns2:hasActorType "Nation-State"^^xsd:string ;
    ns2:hasCampaign ns2:Maryland ;
    ns2:hasCountry "United States of America"^^xsd:string ;
    ns2:hasCounty "Montgomery"^^xsd:string ;
    ns2:hasEventDate "2014-07-13T00:00:00"^^xsd:dateTime ;
    ns2:hasEventSubtype "Exploitation of Application Server"^^xsd:string ;
    ns2:hasEventType "Exploitive"^^xsd:string ;
    ns2:hasIndustry "Manufacturing"^^xsd:string ;
    ns2:hasMonth 7 ;
    ns2:hasOrganization "Lockheed Martin"^^xsd:string ;
    ns2:hasState "Maryland"^^xsd:string ;
    ns2:hasYear 2014 ;
    ns2:isType_of ns2:Exploitation_of_Application_Server,
        ns2:Nation_State ;
    rdfs:comment "The US Department of Justice announces that a Chinese businessman, Su Bin, has been charged with hacking into the computer systems of Boeing, Lockheed Martin and other aerospace companies."^^xsd:string .

ns2:0d8abd5482fddce6 a ns2:DDoS,
        owl:NamedIndividual ;
    ns1:associatedCampaigns ns2:Grinding_Gear_Games ;
    ns2:hasActorType "Criminal"^^xsd:string ;
    ns2:hasCountry "New Zealand"^^xsd:string ;
    ns2:hasEventDate "2014-08-25T00:00:00"^^xsd:dateTime ;
    ns2:hasEventSubtype "External Denial of Service"^^xsd:string ;
    ns2:hasEventType "Disruptive"^^xsd:string ;
    ns2:hasIndustry "Information"^^xsd:string ;
    ns2:hasMonth 8 ;
    ns2:hasOrganization "Grinding Gear Games"^^xsd:string ;
    ns2:hasYear 2014 ;
    ns2:isType_of ns2:Criminal,
        ns2:External_Denial_of_Service ;
    rdfs:comment "Sony admits that a DDoS attack impacted online services, Sony's PlayStation Network and the Sony Entertainment Network. Other affected services involve: Xbox Live, Blizzard's Battle.net, and Grinding Gear Games."^^xsd:string .

ns2:0e75f5a77fe02e43 a ns2:AccountAttack,
        owl:NamedIndividual ;
    ns1:associatedCampaigns ns2:MMMOOO ;
    ns2:hasActor "HitlerSec"^^xsd:string ;
    ns2:hasCountry "China"^^xsd:string ;
    ns2:hasEventDate "2014-01-06T00:00:00"^^xsd:dateTime ;
    ns2:hasEventSubtype "Exploitation of Application Server"^^xsd:string ;
    ns2:hasEventType "Exploitive"^^xsd:string ;
    ns2:hasIndustry "Information"^^xsd:string ;
    ns2:hasMonth 1 ;
    ns2:hasOrganization "MMMOOO"^^xsd:string ;
    ns2:hasYear 2014 ;
    ns2:isType_of ns2:Exploitation_of_Application_Server ;
    rdfs:comment "A group of hackers going by the name HitlerSec hack a Chinese mobile application MMMOOO (immmooo.com) and dump 85,753 email addresses and encrypted passwords."^^xsd:string .

ns2:0f314709f6a68656 a ns2:CyberattackData,
        owl:NamedIndividual ;
    ns1:associatedCampaigns ns2:City_of_Amasya ;
    ns1:description "Protest"^^xsd:string ;
    ns1:isLaunchedBy ns2:Turkey ;
    ns2:behaviour ns2:Protest ;
    ns2:hasActor "RedHack"^^xsd:string ;
    ns2:hasActorCountry "Turkey"^^xsd:string ;
    ns2:hasActorType "Hacktivist"^^xsd:string ;
    ns2:hasCountry "Turkey"^^xsd:string ;
    ns2:hasEventDate "2014-02-10T00:00:00"^^xsd:dateTime ;
    ns2:hasEventSubtype "Exploitation of Application Server"^^xsd:string ;
    ns2:hasEventType "Exploitive"^^xsd:string ;
    ns2:hasIndustry "Public Administration"^^xsd:string ;
    ns2:hasMonth 2 ;
    ns2:hasOrganization "City of Amasya"^^xsd:string ;
    ns2:hasYear 2014 ;
    ns2:isType_of ns2:Exploitation_of_Application_Server,
        ns2:Hacktivist ;
    rdfs:comment "The infamous RedHack collective joins the protests against the new Internet Law, and leak around two dozen records. They also deface a couple of local sites and hack the Ministry of Education."^^xsd:string .

ns2:107431fe0d8096f1 a ns2:AttackMalware,
        owl:NamedIndividual ;
    ns1:associatedCampaigns ns2:WooThemes ;
    ns1:description "Financial"^^xsd:string ;
    ns2:behaviour ns2:Financial ;
    ns2:hasActorType "Criminal"^^xsd:string ;
    ns2:hasCountry "United States of America"^^xsd:string ;
    ns2:hasEventDate "2014-05-09T00:00:00"^^xsd:dateTime ;
    ns2:hasEventSubtype "Exploitation of Application Server"^^xsd:string ;
    ns2:hasEventType "Exploitive"^^xsd:string ;
    ns2:hasIndustry "Information"^^xsd:string ;
    ns2:hasMonth 5 ;
    ns2:hasOrganization "WooThemes"^^xsd:string ;
    ns2:hasYear 2014 ;
    ns2:isType_of ns2:Criminal,
        ns2:Exploitation_of_Application_Server ;
    rdfs:comment "WooThemes, the popular Theme Creator for Wordpress confirms to have been hacked after many users complained of fraudulent credit card transactions."^^xsd:string .

ns2:10a3a6b6de2052c6 a ns2:CyberattackSystem,
        owl:NamedIndividual ;
    ns1:associatedCampaigns ns2:The_Wall_Street_Journal ;
    ns1:description "Personal Attack"^^xsd:string ;
    ns1:isLaunchedBy ns2:Syrian_Arab_Republic ;
    ns2:behaviour ns2:Personal_Attack ;
    ns2:hasActor "Syrian Electronic Army"^^xsd:string ;
    ns2:hasActorCountry "Syrian Arab Republic"^^xsd:string ;
    ns2:hasActorType "Hacktivist"^^xsd:string ;
    ns2:hasCampaign ns2:New_York ;
    ns2:hasCountry "United States of America"^^xsd:string ;
    ns2:hasCounty "New York"^^xsd:string ;
    ns2:hasEventDate "2014-05-07T00:00:00"^^xsd:dateTime ;
    ns2:hasEventSubtype "Message Manipulation"^^xsd:string ;
    ns2:hasEventType "Disruptive"^^xsd:string ;
    ns2:hasIndustry "Information"^^xsd:string ;
    ns2:hasMonth 5 ;
    ns2:hasOrganization "The Wall Street Journal"^^xsd:string ;
    ns2:hasState "New York"^^xsd:string ;
    ns2:hasYear 2014 ;
    ns2:isType_of ns2:Hacktivist,
        ns2:Message_Manipulation ;
    rdfs:comment "The Syrian Electronic Army is back and hijacks a total of four Twitter accounts of the Wall Street Journal (WSJ)."^^xsd:string .

ns2:1125c775c8edb7a9 a ns2:HackerSecurity,
        owl:NamedIndividual ;
    ns1:associatedCampaigns ns2:Dubai_Police ;
    ns1:description "Protest"^^xsd:string ;
    ns2:behaviour ns2:Protest ;
    ns2:hasActor "TheHorsemen"^^xsd:string ;
    ns2:hasActorType "Hacktivist"^^xsd:string ;
    ns2:hasCountry "United Arab Emirates"^^xsd:string ;
    ns2:hasEventDate "2014-02-10T00:00:00"^^xsd:dateTime ;
    ns2:hasEventSubtype "Message Manipulation"^^xsd:string ;
    ns2:hasEventType "Disruptive"^^xsd:string ;
    ns2:hasIndustry "Public Administration"^^xsd:string ;
    ns2:hasMonth 2 ;
    ns2:hasOrganization "Dubai Police"^^xsd:string ;
    ns2:hasYear 2014 ;
    ns2:isType_of ns2:Hacktivist,
        ns2:Message_Manipulation ;
    rdfs:comment "Hackers of a group called TheHorsemen have hijacked the official Twitter, Pinterest, LinkedIn and Tumblr accounts of the Dubai Police (@DubaiPoliceHQ)."^^xsd:string .

ns2:113c6ad2b6e837b0 a ns1:Backdoor,
        owl:NamedIndividual ;
    ns1:associatedCampaigns ns2:Dairy_Queen ;
    ns1:description "Financial"^^xsd:string ;
    ns2:behaviour ns2:Financial ;
    ns2:hasActorType "Criminal"^^xsd:string ;
    ns2:hasCampaign ns2:Minnesota ;
    ns2:hasCountry "United States of America"^^xsd:string ;
    ns2:hasCounty "Hennepin"^^xsd:string ;
    ns2:hasEventDate "2014-08-28T00:00:00"^^xsd:dateTime ;
    ns2:hasEventSubtype "Exploitation of Sensors"^^xsd:string ;
    ns2:hasEventType "Exploitive"^^xsd:string ;
    ns2:hasIndustry "Accommodation and Food Services"^^xsd:string ;
    ns2:hasMonth 8 ;
    ns2:hasOrganization "Dairy Queen"^^xsd:string ;
    ns2:hasState "Minnesota"^^xsd:string ;
    ns2:hasYear 2014 ;
    ns2:isType_of ns2:Criminal,
        ns2:Exploitation_of_Sensors ;
    rdfs:comment "Fast food restaurant Dairy Queen confirms that systems in some of their locations have been infected with Backoff."^^xsd:string .

ns2:117f86828012d22d a ns2:AttackWebsite,
        owl:NamedIndividual ;
    ns1:associatedCampaigns ns2:Youth_for_Achievements ;
    ns1:description "Protest"^^xsd:string ;
    ns1:isLaunchedBy ns2:Azerbaijan ;
    ns2:behaviour ns2:Protest ;
    ns2:hasActor "Anti-Armenia Team"^^xsd:string ;
    ns2:hasActorCountry "Azerbaijan"^^xsd:string ;
    ns2:hasActorType "Hacktivist"^^xsd:string ;
    ns2:hasCountry "Armenia"^^xsd:string ;
    ns2:hasEventDate "2014-01-23T00:00:00"^^xsd:dateTime ;
    ns2:hasEventSubtype "Message Manipulation"^^xsd:string ;
    ns2:hasEventType "Disruptive"^^xsd:string ;
    ns2:hasIndustry "Other Services (except Public Administration)"^^xsd:string ;
    ns2:hasMonth 1 ;
    ns2:hasOrganization "Youth for Achievements"^^xsd:string ;
    ns2:hasYear 2014 ;
    ns2:isType_of ns2:Hacktivist,
        ns2:Message_Manipulation ;
    rdfs:comment "Azerbaijan Hackers from Anti-Armenia Team have hacked and defaced several Armenian government ministries websites."^^xsd:string .

ns2:11a7a57a6b720a04 a ns2:CyberattackInformation,
        owl:NamedIndividual ;
    ns1:associatedCampaigns ns2:Pakistan_Ministry_of_Interior ;
    ns1:isLaunchedBy ns2:Pakistan ;
    ns2:hasActor "Anonymous (Pakistan)"^^xsd:string ;
    ns2:hasActorCountry "Pakistan"^^xsd:string ;
    ns2:hasActorType "Hacktivist"^^xsd:string ;
    ns2:hasCountry "Pakistan"^^xsd:string ;
    ns2:hasEventDate "2014-09-06T00:00:00"^^xsd:dateTime ;
    ns2:hasEventSubtype "Message Manipulation"^^xsd:string ;
    ns2:hasEventType "Disruptive"^^xsd:string ;
    ns2:hasIndustry "Public Administration"^^xsd:string ;
    ns2:hasMonth 9 ;
    ns2:hasOrganization "Pakistan Ministry of Interior"^^xsd:string ;
    ns2:hasYear 2014 ;
    ns2:isType_of ns2:Hacktivist,
        ns2:Message_Manipulation ;
    rdfs:comment "Yet another cyber attack in Pakistan. Anonymous Pakistan defaces the official website of the Pakistan Ministry of Interior (interior.gov.pk)."^^xsd:string .

ns2:128ad0dc650499fa a ns2:DDoS,
        owl:NamedIndividual ;
    ns1:associatedCampaigns ns2:Dota_2 ;
    ns2:hasActor "DERP Trolling"^^xsd:string ;
    ns2:hasCampaign ns2:Washington ;
    ns2:hasCountry "United States of America"^^xsd:string ;
    ns2:hasCounty "King"^^xsd:string ;
    ns2:hasEventDate "2014-01-03T00:00:00"^^xsd:dateTime ;
    ns2:hasEventSubtype "External Denial of Service"^^xsd:string ;
    ns2:hasEventType "Disruptive"^^xsd:string ;
    ns2:hasIndustry "Information"^^xsd:string ;
    ns2:hasMonth 1 ;
    ns2:hasOrganization "Dota 2"^^xsd:string ;
    ns2:hasState "Washington"^^xsd:string ;
    ns2:hasYear 2014 ;
    ns2:isType_of ns2:External_Denial_of_Service ;
    rdfs:comment "The servers for Steam, Origin, Battle.net, and League of Legends are brought down temporarily by apparent DDoS attacks that seem to be related to a swatting attack on an individual known for streaming games."^^xsd:string .

ns2:130bcd90d01c4db1 a ns2:DDoS,
        owl:NamedIndividual ;
    ns1:associatedCampaigns ns2:European_Court_of_Human_Rights ;
    ns1:description "Protest"^^xsd:string ;
    ns1:isLaunchedBy ns2:France ;
    ns2:behaviour ns2:Protest ;
    ns2:hasActor "Anka Neferler Timi"^^xsd:string ;
    ns2:hasActorCountry "France"^^xsd:string ;
    ns2:hasActorType "Hacktivist"^^xsd:string ;
    ns2:hasCountry "France"^^xsd:string ;
    ns2:hasEventDate "2020-12-22T00:00:00"^^xsd:dateTime ;
    ns2:hasEventSubtype "External Denial of Service"^^xsd:string ;
    ns2:hasEventType "Disruptive"^^xsd:string ;
    ns2:hasIndustry "Public Administration"^^xsd:string ;
    ns2:hasMonth 12 ;
    ns2:hasOrganization "European Court of Human Rights"^^xsd:string ;
    ns2:hasYear 2020 ;
    ns2:isType_of ns2:External_Denial_of_Service,
        ns2:Hacktivist ;
    rdfs:comment "The website of the European Court of Human Rights was knocked offline after issuing a ruling that called on Turkey to release a prominent Kurdish politician."^^xsd:string .

ns2:13561e2a1bf0c3b4 a ns2:HackerSecurity,
        owl:NamedIndividual ;
    ns1:associatedCampaigns ns2:Rural_King ;
    ns1:description "Financial"^^xsd:string ;
    ns2:behaviour ns2:Financial ;
    ns2:hasActorType "Criminal"^^xsd:string ;
    ns2:hasCampaign ns2:Illinois ;
    ns2:hasCountry "United States of America"^^xsd:string ;
    ns2:hasCounty "Coles"^^xsd:string ;
    ns2:hasEventDate "2014-04-05T00:00:00"^^xsd:dateTime ;
    ns2:hasEventSubtype "Exploitation of Application Server"^^xsd:string ;
    ns2:hasEventType "Exploitive"^^xsd:string ;
    ns2:hasIndustry "Retail Trade"^^xsd:string ;
    ns2:hasMonth 4 ;
    ns2:hasOrganization "Rural King"^^xsd:string ;
    ns2:hasState "Illinois"^^xsd:string ;
    ns2:hasYear 2014 ;
    ns2:isType_of ns2:Criminal,
        ns2:Exploitation_of_Application_Server ;
    rdfs:comment "Farm supply store Rural King notifies its customers after hackers gained access to their personal and financial information. The number of impacted users is not known."^^xsd:string .

ns2:1389e2776dea37ba a ns2:DDoS,
        owl:NamedIndividual ;
    ns1:associatedCampaigns ns2:World_of_Tanks ;
    ns2:hasActor "DERP Trolling"^^xsd:string ;
    ns2:hasCountry "United States of America"^^xsd:string ;
    ns2:hasEventDate "2014-01-03T00:00:00"^^xsd:dateTime ;
    ns2:hasEventSubtype "External Denial of Service"^^xsd:string ;
    ns2:hasEventType "Disruptive"^^xsd:string ;
    ns2:hasIndustry "Information"^^xsd:string ;
    ns2:hasMonth 1 ;
    ns2:hasOrganization "World of Tanks"^^xsd:string ;
    ns2:hasYear 2014 ;
    ns2:isType_of ns2:External_Denial_of_Service ;
    rdfs:comment "The servers for Steam, Origin, Battle.net, and League of Legends are brought down temporarily by apparent DDoS attacks that seem to be related to a swatting attack on an individual known for streaming games."^^xsd:string .

ns2:144f78e0a07b547e a ns2:DDoS,
        owl:NamedIndividual ;
    ns1:associatedCampaigns ns2:Kansas_Interactive_Testing_Engine ;
    ns2:hasActorType "Criminal"^^xsd:string ;
    ns2:hasCampaign ns2:Kansas ;
    ns2:hasCountry "United States of America"^^xsd:string ;
    ns2:hasCounty "Douglas"^^xsd:string ;
    ns2:hasEventDate "2014-04-04T00:00:00"^^xsd:dateTime ;
    ns2:hasEventSubtype "External Denial of Service"^^xsd:string ;
    ns2:hasEventType "Disruptive"^^xsd:string ;
    ns2:hasIndustry "Educational Services"^^xsd:string ;
    ns2:hasMonth 4 ;
    ns2:hasOrganization "Kansas Interactive Testing Engine"^^xsd:string ;
    ns2:hasState "Kansas"^^xsd:string ;
    ns2:hasYear 2014 ;
    ns2:isType_of ns2:Criminal,
        ns2:External_Denial_of_Service ;
    rdfs:comment "A DDoS attack takes down the Kansas Interactive Testing Engine (KITE, ksassessments.org), Kansas' new online student testing system."^^xsd:string .

ns2:14dc84ca6a44c145 a ns2:AttackWebsite,
        owl:NamedIndividual ;
    ns1:associatedCampaigns ns2:Froco_Fresh_Frozen ;
    ns2:hasActorType "Criminal"^^xsd:string ;
    ns2:hasCampaign ns2:Texas ;
    ns2:hasCountry "United States of America"^^xsd:string ;
    ns2:hasCounty "Travis"^^xsd:string ;
    ns2:hasEventDate "2014-07-10T00:00:00"^^xsd:dateTime ;
    ns2:hasEventSubtype "Message Manipulation"^^xsd:string ;
    ns2:hasEventType "Disruptive"^^xsd:string ;
    ns2:hasIndustry "Wholesale Trade"^^xsd:string ;
    ns2:hasMonth 7 ;
    ns2:hasOrganization "Froco Fresh Frozen"^^xsd:string ;
    ns2:hasState "Texas"^^xsd:string ;
    ns2:hasYear 2014 ;
    ns2:isType_of ns2:Criminal,
        ns2:Message_Manipulation ;
    rdfs:comment "The website for Farrah Abraham's new frozen yogurt shop is hacked, and its homepage replaced with a graphic clip from her sex tape."^^xsd:string .

ns2:1553addc450ba801 a ns2:BreachInformation,
        owl:NamedIndividual ;
    ns1:associatedCampaigns ns2:Spotify ;
    ns2:hasActorType "Criminal"^^xsd:string ;
    ns2:hasCountry "Sweden"^^xsd:string ;
    ns2:hasEventDate "2014-05-27T00:00:00"^^xsd:dateTime ;
    ns2:hasEventSubtype "Exploitation of Application Server"^^xsd:string ;
    ns2:hasEventType "Exploitive"^^xsd:string ;
    ns2:hasIndustry "Information"^^xsd:string ;
    ns2:hasMonth 5 ;
    ns2:hasOrganization "Spotify"^^xsd:string ;
    ns2:hasYear 2014 ;
    ns2:isType_of ns2:Criminal,
        ns2:Exploitation_of_Application_Server ;
    rdfs:comment "Spotify warns of unauthorized access to the company's network and internal data. The unauthorized access appears to involve data for a single, unspecified person."^^xsd:string .

ns2:15990c26ce209558 a ns2:AttackWebsite,
        owl:NamedIndividual ;
    ns1:associatedCampaigns ns2:Riyadh_Principality ;
    ns1:description "Protest"^^xsd:string ;
    ns1:isLaunchedBy ns2:Syrian_Arab_Republic ;
    ns2:behaviour ns2:Protest ;
    ns2:hasActor "Syrian Electronic Army"^^xsd:string ;
    ns2:hasActorCountry "Syrian Arab Republic"^^xsd:string ;
    ns2:hasActorType "Hacktivist"^^xsd:string ;
    ns2:hasCountry "Saudi Arabia"^^xsd:string ;
    ns2:hasEventDate "2014-01-16T00:00:00"^^xsd:dateTime ;
    ns2:hasEventSubtype "Message Manipulation"^^xsd:string ;
    ns2:hasEventType "Disruptive"^^xsd:string ;
    ns2:hasIndustry "Public Administration"^^xsd:string ;
    ns2:hasMonth 1 ;
    ns2:hasOrganization "Riyadh Principality"^^xsd:string ;
    ns2:hasYear 2014 ;
    ns2:isType_of ns2:Hacktivist,
        ns2:Message_Manipulation ;
    rdfs:comment "The Syrian Electronic Army deface 16 Saudi Arabian government websites. The targeted sites are the ones of various administrative regions."^^xsd:string .

ns2:1610f97a3c61fb74 a ns2:HackerSecurity,
        owl:NamedIndividual ;
    ns1:associatedCampaigns ns2:FBI_Fusion_Center ;
    ns1:description "Protest"^^xsd:string ;
    ns2:behaviour ns2:Protest ;
    ns2:hasActor "TeamBerserk"^^xsd:string ;
    ns2:hasActorType "Hacktivist"^^xsd:string ;
    ns2:hasCountry "United States of America"^^xsd:string ;
    ns2:hasEventDate "2014-01-17T00:00:00"^^xsd:dateTime ;
    ns2:hasEventSubtype "Exploitation of Application Server"^^xsd:string ;
    ns2:hasEventType "Exploitive"^^xsd:string ;
    ns2:hasIndustry "Public Administration"^^xsd:string ;
    ns2:hasMonth 1 ;
    ns2:hasOrganization "FBI Fusion Center"^^xsd:string ;
    ns2:hasYear 2014 ;
    ns2:isType_of ns2:Exploitation_of_Application_Server,
        ns2:Hacktivist ;
    rdfs:comment "Hackers from TeamBerserk announce a leak of documents allegedly obtained from a FBI Fusion Center."^^xsd:string .

ns2:176c1534ac14be4c a ns2:CyberattackInformation,
        owl:NamedIndividual ;
    ns1:associatedCampaigns ns2:Malaysian_National_Security_Council ;
    ns2:hasActorType "Criminal"^^xsd:string ;
    ns2:hasCountry "Malaysia"^^xsd:string ;
    ns2:hasEventDate "2014-08-20T00:00:00"^^xsd:dateTime ;
    ns2:hasEventSubtype "Exploitation of End Hosts"^^xsd:string ;
    ns2:hasEventType "Exploitive"^^xsd:string ;
    ns2:hasIndustry "Public Administration"^^xsd:string ;
    ns2:hasMonth 8 ;
    ns2:hasOrganization "Malaysian National Security Council"^^xsd:string ;
    ns2:hasYear 2014 ;
    ns2:isType_of ns2:Criminal,
        ns2:Exploitation_of_End_Hosts ;
    rdfs:comment "The computers of high-ranking officials in Malaysian agencies involved in the MH370 investigation are hacked and classified information is stolen. Suspects are directed to China."^^xsd:string .

ns2:179305debc36f399 a ns2:DDoS,
        owl:NamedIndividual ;
    ns1:associatedCampaigns ns2:Evernote ;
    ns2:hasActorType "Criminal"^^xsd:string ;
    ns2:hasCampaign ns2:California ;
    ns2:hasCountry "United States of America"^^xsd:string ;
    ns2:hasCounty "San Mateo"^^xsd:string ;
    ns2:hasEventDate "2014-06-10T00:00:00"^^xsd:dateTime ;
    ns2:hasEventSubtype "External Denial of Service"^^xsd:string ;
    ns2:hasEventType "Disruptive"^^xsd:string ;
    ns2:hasIndustry "Information"^^xsd:string ;
    ns2:hasMonth 6 ;
    ns2:hasOrganization "Evernote"^^xsd:string ;
    ns2:hasState "California"^^xsd:string ;
    ns2:hasYear 2014 ;
    ns2:isType_of ns2:Criminal,
        ns2:External_Denial_of_Service ;
    rdfs:comment "Mobile and online note app Evernote was hit with a DDoS attack, taking its servers offline for several hours."^^xsd:string .

ns2:17bbee8b997fe0fc a ns2:CyberattackData,
        owl:NamedIndividual ;
    ns1:associatedCampaigns ns2:Xbox_Instagram_account ;
    ns1:isLaunchedBy ns2:Syrian_Arab_Republic ;
    ns2:hasActor "Syrian Electronic Army"^^xsd:string ;
    ns2:hasActorCountry "Syrian Arab Republic"^^xsd:string ;
    ns2:hasActorType "Hacktivist"^^xsd:string ;
    ns2:hasCampaign ns2:Washington ;
    ns2:hasCountry "United States of America"^^xsd:string ;
    ns2:hasCounty "King"^^xsd:string ;
    ns2:hasEventDate "2014-01-13T00:00:00"^^xsd:dateTime ;
    ns2:hasEventSubtype "Message Manipulation"^^xsd:string ;
    ns2:hasEventType "Disruptive"^^xsd:string ;
    ns2:hasIndustry "Information"^^xsd:string ;
    ns2:hasMonth 1 ;
    ns2:hasOrganization "Xbox Instagram account"^^xsd:string ;
    ns2:hasState "Washington"^^xsd:string ;
    ns2:hasYear 2014 ;
    ns2:isType_of ns2:Hacktivist,
        ns2:Message_Manipulation ;
    rdfs:comment "In the same campaign the Syrian Electronic Army hacks the Twitter Xbox Support account, the Xbox Twitter and Instagram, and Microsoft employees."^^xsd:string .

ns2:17de741fd81a0adf a ns2:Phishing,
        owl:NamedIndividual ;
    ns1:associatedCampaigns ns2:University_of_Louisiana_at_Monroe ;
    ns2:hasActorType "Criminal"^^xsd:string ;
    ns2:hasCampaign ns2:Louisiana ;
    ns2:hasCountry "United States of America"^^xsd:string ;
    ns2:hasCounty "Ouachita"^^xsd:string ;
    ns2:hasEventDate "2014-08-21T00:00:00"^^xsd:dateTime ;
    ns2:hasEventSubtype "Exploitation of Application Server"^^xsd:string ;
    ns2:hasEventType "Exploitive"^^xsd:string ;
    ns2:hasIndustry "Educational Services"^^xsd:string ;
    ns2:hasMonth 8 ;
    ns2:hasOrganization "University of Louisiana at Monroe"^^xsd:string ;
    ns2:hasState "Louisiana"^^xsd:string ;
    ns2:hasYear 2014 ;
    ns2:isType_of ns2:Criminal,
        ns2:Exploitation_of_Application_Server ;
    rdfs:comment "An employee of the University of Louisiana at Monroe falls victim of a phishing attempt, possibly compromising the personal information of students who graduated from ULM in fall 2013, and spring 2014."^^xsd:string .

ns2:17f648b744da19a0 a ns2:DataSecurity,
        owl:NamedIndividual ;
    ns1:associatedCampaigns ns2:Lubbock_Cardiology_Clinic ;
    ns2:hasActorType "Criminal"^^xsd:string ;
    ns2:hasCampaign ns2:Texas ;
    ns2:hasCountry "United States of America"^^xsd:string ;
    ns2:hasCounty "Lubbock"^^xsd:string ;
    ns2:hasEventDate "2014-04-11T00:00:00"^^xsd:dateTime ;
    ns2:hasEventSubtype "Exploitation of Application Server"^^xsd:string ;
    ns2:hasEventType "Exploitive"^^xsd:string ;
    ns2:hasIndustry "Health Care and Social Assistance"^^xsd:string ;
    ns2:hasMonth 4 ;
    ns2:hasOrganization "Lubbock Cardiology Clinic"^^xsd:string ;
    ns2:hasState "Texas"^^xsd:string ;
    ns2:hasYear 2014 ;
    ns2:isType_of ns2:Criminal,
        ns2:Exploitation_of_Application_Server ;
    rdfs:comment "Unauthorized access is gained to the Electronic Health Record system used by Texas-based Lubbock Cardiology Clinic (LCC), which resulted in the compromise of more than 1,400 medical records."^^xsd:string .

ns2:182e9d15c3d5da2c a ns2:BreachSecurity,
        owl:NamedIndividual ;
    ns1:associatedCampaigns ns2:ReadingRockets_org ;
    ns2:hasActor "DeleteSec"^^xsd:string ;
    ns2:hasActorType "Hacktivist"^^xsd:string ;
    ns2:hasCampaign ns2:Washington_D_C ;
    ns2:hasCountry "United States of America"^^xsd:string ;
    ns2:hasEventDate "2014-02-13T00:00:00"^^xsd:dateTime ;
    ns2:hasEventSubtype "Exploitation of Application Server"^^xsd:string ;
    ns2:hasEventType "Exploitive"^^xsd:string ;
    ns2:hasIndustry "Other Services (except Public Administration)"^^xsd:string ;
    ns2:hasMonth 2 ;
    ns2:hasOrganization "ReadingRockets.org"^^xsd:string ;
    ns2:hasState "Washington D.C."^^xsd:string ;
    ns2:hasYear 2014 ;
    ns2:isType_of ns2:Exploitation_of_Application_Server,
        ns2:Hacktivist ;
    rdfs:comment "DeleteSec hacks ReadingRockets.org and leaks around 5,800 accounts. Leaked credentials contain full names, addresses, contact information, email addresses and clear text passwords."^^xsd:string .

ns2:1a8bd2d4c07d213c a ns1:BotnetAttack,
        owl:NamedIndividual ;
    ns1:associatedCampaigns ns2:Tajikistan_Domain_Registrar ;
    ns1:isLaunchedBy ns2:Iran__Islamic_Republic_of ;
    ns2:hasActor "Mr.Xhat"^^xsd:string ;
    ns2:hasActorCountry "Iran (Islamic Republic of)"^^xsd:string ;
    ns2:hasActorType "Hobbyist"^^xsd:string ;
    ns2:hasCountry "Tajikistan"^^xsd:string ;
    ns2:hasEventDate "2014-01-06T00:00:00"^^xsd:dateTime ;
    ns2:hasEventSubtype "Message Manipulation"^^xsd:string ;
    ns2:hasEventType "Disruptive"^^xsd:string ;
    ns2:hasIndustry "Professional, Scientific, and Technical Services"^^xsd:string ;
    ns2:hasMonth 1 ;
    ns2:hasOrganization "Tajikistan Domain Registrar"^^xsd:string ;
    ns2:hasYear 2014 ;
    ns2:isType_of ns2:Hobbyist,
        ns2:Message_Manipulation ;
    rdfs:comment "An Iranian hacker called Mr.Xhat hacks the national domain registrar for Tajikistan (domain.tj), and as a consequence, the local primary domains for Google, Yahoo, Twitter, Amazon are redirected to a defaced page."^^xsd:string .

ns2:1aa3a134e8a1f32b a ns2:BreachInformation,
        owl:NamedIndividual ;
    ns1:associatedCampaigns ns2:Score ;
    ns1:description "Financial"^^xsd:string ;
    ns2:behaviour ns2:Financial ;
    ns2:hasActorType "Criminal"^^xsd:string ;
    ns2:hasCampaign ns2:California ;
    ns2:hasCountry "United States of America"^^xsd:string ;
    ns2:hasCounty "Orange"^^xsd:string ;
    ns2:hasEventDate "2014-09-04T00:00:00"^^xsd:dateTime ;
    ns2:hasEventSubtype "Exploitation of Application Server"^^xsd:string ;
    ns2:hasEventType "Exploitive"^^xsd:string ;
    ns2:hasIndustry "Manufacturing"^^xsd:string ;
    ns2:hasMonth 9 ;
    ns2:hasOrganization "Score"^^xsd:string ;
    ns2:hasState "California"^^xsd:string ;
    ns2:hasYear 2014 ;
    ns2:isType_of ns2:Criminal,
        ns2:Exploitation_of_Application_Server ;
    rdfs:comment "Score, a sport uniform manufacturer, discovers a potential unauthorized data breach occurred on September 4, 2014. 500 customers who shopped online may have been compromised."^^xsd:string .

ns2:1bbd24ee070300b7 a ns2:BreachInformation,
        owl:NamedIndividual ;
    ns1:associatedCampaigns ns2:California_Department_of_Motor_Vehicles ;
    ns1:description "Financial"^^xsd:string ;
    ns2:behaviour ns2:Financial ;
    ns2:hasActorType "Criminal"^^xsd:string ;
    ns2:hasCampaign ns2:California ;
    ns2:hasCountry "United States of America"^^xsd:string ;
    ns2:hasCounty "Sacramento"^^xsd:string ;
    ns2:hasEventDate "2014-03-22T00:00:00"^^xsd:dateTime ;
    ns2:hasEventSubtype "Exploitation of Application Server"^^xsd:string ;
    ns2:hasEventType "Exploitive"^^xsd:string ;
    ns2:hasIndustry "Public Administration"^^xsd:string ;
    ns2:hasMonth 3 ;
    ns2:hasOrganization "California Department of Motor Vehicles"^^xsd:string ;
    ns2:hasState "California"^^xsd:string ;
    ns2:hasYear 2014 ;
    ns2:isType_of ns2:Criminal,
        ns2:Exploitation_of_Application_Server ;
    rdfs:comment "The California Department of Motor VehiclesÃÆÃ'Ãâ 'ÃÆÃ¢â¬Â 'ÃÆÃ'ÃÂ¢Ã¢'Â¬ÃÂ ''ÃÆÃ'Ãâ 'ÃÆÃ¢â¬Â ''ÃÆÃ'Ãâ ''ÃÆÃ''ÃÆ'Ã'ÃÂ appears to have suffered a wide-ranging credit card data breach involving online payments. The Department states that its computers were not breached directly, but rather the breach happened to a card processor. "^^xsd:string .

ns2:1cdda8608d81b16d a ns2:AnonymousAttack,
        owl:NamedIndividual ;
    ns1:associatedCampaigns ns2:Massachusetts_Institute_of_Technology ;
    ns1:description "Protest"^^xsd:string ;
    ns2:behaviour ns2:Protest ;
    ns2:hasActor "Anonymous"^^xsd:string ;
    ns2:hasActorType "Hacktivist"^^xsd:string ;
    ns2:hasCampaign ns2:Massachusetts ;
    ns2:hasCountry "United States of America"^^xsd:string ;
    ns2:hasCounty "Middlesex"^^xsd:string ;
    ns2:hasEventDate "2014-01-11T00:00:00"^^xsd:dateTime ;
    ns2:hasEventSubtype "Message Manipulation"^^xsd:string ;
    ns2:hasEventType "Disruptive"^^xsd:string ;
    ns2:hasIndustry "Educational Services"^^xsd:string ;
    ns2:hasMonth 1 ;
    ns2:hasOrganization "Massachusetts Institute of Technology"^^xsd:string ;
    ns2:hasState "Massachusetts"^^xsd:string ;
    ns2:hasYear 2014 ;
    ns2:isType_of ns2:Hacktivist,
        ns2:Message_Manipulation ;
    rdfs:comment "Exactly one year since Aaron Swartz passed away, hacktivists of the Anonymous collective deface a subdomain of MIT (cogen.mit.edu) in the name of #OpLastResort."^^xsd:string .

ns2:1cfb8a5395419562 a ns2:AttackWebsite,
        owl:NamedIndividual ;
    ns1:associatedCampaigns ns2:Supercell_Facebook_Pages ;
    ns2:hasActor "Ethical Spectrum"^^xsd:string ;
    ns2:hasActorType "Hacktivist"^^xsd:string ;
    ns2:hasCountry "Finland"^^xsd:string ;
    ns2:hasEventDate "2014-02-11T00:00:00"^^xsd:dateTime ;
    ns2:hasEventSubtype "Message Manipulation,Exploitation of Application Server"^^xsd:string ;
    ns2:hasEventType "Mixed"^^xsd:string ;
    ns2:hasIndustry "Information"^^xsd:string ;
    ns2:hasMonth 2 ;
    ns2:hasOrganization "Supercell Facebook Pages"^^xsd:string ;
    ns2:hasYear 2014 ;
    ns2:isType_of ns2:Hacktivist,
        ns2:Message_Manipulation_Exploitation_of_App ;
    rdfs:comment "The Facebook pages of two games, Hay Day and Clash of Clans, developed by the Helsinki-based video game developer Supercell are hacked. The attack is executed by hijacking the emails of two Supercell employees. "^^xsd:string .

ns2:1ec2f777aa22c77f a ns2:AccountAttack,
        owl:NamedIndividual ;
    ns1:associatedCampaigns ns2:CNN ;
    ns1:description "Protest"^^xsd:string ;
    ns1:isLaunchedBy ns2:Syrian_Arab_Republic ;
    ns2:behaviour ns2:Protest ;
    ns2:hasActor "Syrian Electronic Army"^^xsd:string ;
    ns2:hasActorCountry "Syrian Arab Republic"^^xsd:string ;
    ns2:hasActorType "Hacktivist"^^xsd:string ;
    ns2:hasCampaign ns2:Georgia ;
    ns2:hasCountry "United States of America"^^xsd:string ;
    ns2:hasCounty "Fulton"^^xsd:string ;
    ns2:hasEventDate "2014-01-24T00:00:00"^^xsd:dateTime ;
    ns2:hasEventSubtype "Message Manipulation"^^xsd:string ;
    ns2:hasEventType "Disruptive"^^xsd:string ;
    ns2:hasIndustry "Information"^^xsd:string ;
    ns2:hasMonth 1 ;
    ns2:hasOrganization "CNN"^^xsd:string ;
    ns2:hasState "Georgia"^^xsd:string ;
    ns2:hasYear 2014 ;
    ns2:isType_of ns2:Hacktivist,
        ns2:Message_Manipulation ;
    rdfs:comment "The Syrian Electronic Army hacks several accounts belonging to CNN. Targets include: CNN's main Facebook account, CNN Politics' Facebook account and the Twitter pages for CNN and CNN's Security Clearance. Blogs for Political Ticker, The Lead, Security Clearance, The Situation Room and Crossfire were also hacked."^^xsd:string .

ns2:1f72c2eb8ab303e4 a ns2:Malware,
        owl:NamedIndividual ;
    ns1:associatedCampaigns ns2:Barry_University ;
    ns2:hasActorType "Criminal"^^xsd:string ;
    ns2:hasCampaign ns2:Florida ;
    ns2:hasCountry "United States of America"^^xsd:string ;
    ns2:hasCounty "Miami-Dade"^^xsd:string ;
    ns2:hasEventDate "2014-01-01T00:00:00"^^xsd:dateTime ;
    ns2:hasEventSubtype "Exploitation of End Hosts"^^xsd:string ;
    ns2:hasEventType "Exploitive"^^xsd:string ;
    ns2:hasIndustry "Educational Services"^^xsd:string ;
    ns2:hasMonth 1 ;
    ns2:hasOrganization "Barry University"^^xsd:string ;
    ns2:hasState "Florida"^^xsd:string ;
    ns2:hasYear 2014 ;
    ns2:isType_of ns2:Criminal,
        ns2:Exploitation_of_End_Hosts ;
    rdfs:comment "Barry University notifies patients of its Foot and Ankle Institute that their medical records and personal information may have been hacked by a malware found in May."^^xsd:string .

ns2:1f971bf819389290 a ns2:CyberattackData,
        owl:NamedIndividual ;
    ns1:associatedCampaigns ns2:Dnipropetrovsk_Department_of_Law_Enforce ;
    ns1:isLaunchedBy ns2:Ukraine ;
    ns2:hasActor "CyberBerkut"^^xsd:string ;
    ns2:hasActorCountry "Ukraine"^^xsd:string ;
    ns2:hasActorType "Hacktivist"^^xsd:string ;
    ns2:hasCountry "Ukraine"^^xsd:string ;
    ns2:hasEventDate "2014-08-09T00:00:00"^^xsd:dateTime ;
    ns2:hasEventSubtype "Exploitation of Application Server"^^xsd:string ;
    ns2:hasEventType "Exploitive"^^xsd:string ;
    ns2:hasIndustry "Public Administration"^^xsd:string ;
    ns2:hasMonth 8 ;
    ns2:hasOrganization "Dnipropetrovsk Department of Law Enforcement"^^xsd:string ;
    ns2:hasYear 2014 ;
    ns2:isType_of ns2:Exploitation_of_Application_Server,
        ns2:Hacktivist ;
    rdfs:comment "Pro Russian Hacker collective CyberBerkut accesses the information resources of the regional department of the military law and order service in Dnipropetrovsk and leaks some private correspondence."^^xsd:string .

ns2:20028e4883d60f37 a ns2:Phishing,
        owl:NamedIndividual ;
    ns1:associatedCampaigns ns2:Moshtix ;
    ns1:description "Financial"^^xsd:string ;
    ns2:behaviour ns2:Financial ;
    ns2:hasActorType "Criminal"^^xsd:string ;
    ns2:hasCountry "Australia"^^xsd:string ;
    ns2:hasEventDate "2014-05-08T00:00:00"^^xsd:dateTime ;
    ns2:hasEventSubtype "Exploitation of Application Server"^^xsd:string ;
    ns2:hasEventType "Exploitive"^^xsd:string ;
    ns2:hasIndustry "Arts, Entertainment, and Recreation"^^xsd:string ;
    ns2:hasMonth 5 ;
    ns2:hasOrganization "Moshtix"^^xsd:string ;
    ns2:hasYear 2014 ;
    ns2:isType_of ns2:Criminal,
        ns2:Exploitation_of_Application_Server ;
    rdfs:comment "Moshtix, Australia's largest ticket website, is hacked. As a consequence customers report money going missing, spam and scam emails asking for credit card information."^^xsd:string .

ns2:204844c1e51a4fef a ns2:CyberattackData,
        owl:NamedIndividual ;
    ns1:associatedCampaigns ns2:Various_Government_Websites ;
    ns1:description "Protest"^^xsd:string ;
    ns1:isLaunchedBy ns2:Ukraine ;
    ns2:behaviour ns2:Protest ;
    ns2:hasActor "CyberBerkut"^^xsd:string ;
    ns2:hasActorCountry "Ukraine"^^xsd:string ;
    ns2:hasActorType "Hacktivist"^^xsd:string ;
    ns2:hasCountry "Poland"^^xsd:string ;
    ns2:hasEventDate "2014-08-14T00:00:00"^^xsd:dateTime ;
    ns2:hasEventSubtype "Message Manipulation"^^xsd:string ;
    ns2:hasEventType "Disruptive"^^xsd:string ;
    ns2:hasIndustry "Public Administration"^^xsd:string ;
    ns2:hasMonth 8 ;
    ns2:hasOrganization "Various Government Websites"^^xsd:string ;
    ns2:hasYear 2014 ;
    ns2:isType_of ns2:Hacktivist,
        ns2:Message_Manipulation ;
    rdfs:comment "Pro Russian Hacker collective CyberBerkut defaces several dozens of Polish sites to protest against the pro-Ukraine support of the country."^^xsd:string .

ns2:204e8439ddd8d2bc a ns2:HackerSecurity,
        owl:NamedIndividual ;
    ns1:associatedCampaigns ns2:Energie_Steiermark ;
    ns2:hasActorType "Criminal"^^xsd:string ;
    ns2:hasCountry "Austria"^^xsd:string ;
    ns2:hasEventDate "2014-02-20T00:00:00"^^xsd:dateTime ;
    ns2:hasEventSubtype "Exploitation of Application Server"^^xsd:string ;
    ns2:hasEventType "Exploitive"^^xsd:string ;
    ns2:hasIndustry "Utilities"^^xsd:string ;
    ns2:hasMonth 2 ;
    ns2:hasOrganization "Energie Steiermark"^^xsd:string ;
    ns2:hasYear 2014 ;
    ns2:isType_of ns2:Criminal,
        ns2:Exploitation_of_Application_Server ;
    rdfs:comment "Energie Steiermark, an energy company in Austria's Styria province, put out a notice that they have been hacked. "^^xsd:string .

ns2:208229ac32164cbc a ns2:AccountAttack,
        owl:NamedIndividual ;
    ns1:associatedCampaigns ns2:University_of_Wisconsin_Parkside ;
    ns2:hasActorType "Criminal"^^xsd:string ;
    ns2:hasCampaign ns2:Wisconsin ;
    ns2:hasCountry "United States of America"^^xsd:string ;
    ns2:hasCounty "Kenosha"^^xsd:string ;
    ns2:hasEventDate "2014-03-28T00:00:00"^^xsd:dateTime ;
    ns2:hasEventSubtype "Exploitation of Application Server"^^xsd:string ;
    ns2:hasEventType "Exploitive"^^xsd:string ;
    ns2:hasIndustry "Educational Services"^^xsd:string ;
    ns2:hasMonth 3 ;
    ns2:hasOrganization "University of Wisconsin Parkside"^^xsd:string ;
    ns2:hasState "Wisconsin"^^xsd:string ;
    ns2:hasYear 2014 ;
    ns2:isType_of ns2:Criminal,
        ns2:Exploitation_of_Application_Server ;
    rdfs:comment "About 15,000 University of Wisconsin-Parkside (UW-Parkside) students are notified that their personal information, including Social Security numbers, may have been compromised by hackers who installed malware on a server."^^xsd:string .

ns2:22cf2b8d844b227b a ns2:HackerSecurity,
        owl:NamedIndividual ;
    ns1:associatedCampaigns ns2:Pakistani_Consulate_in_Jeddah ;
    ns1:description "Protest"^^xsd:string ;
    ns1:isLaunchedBy ns2:Pakistan ;
    ns2:behaviour ns2:Protest ;
    ns2:hasActor "H4$N4!N H4XOR"^^xsd:string ;
    ns2:hasActorCountry "Pakistan"^^xsd:string ;
    ns2:hasActorType "Hacktivist"^^xsd:string ;
    ns2:hasCountry "Pakistan"^^xsd:string ;
    ns2:hasEventDate "2014-03-30T00:00:00"^^xsd:dateTime ;
    ns2:hasEventSubtype "Message Manipulation"^^xsd:string ;
    ns2:hasEventType "Disruptive"^^xsd:string ;
    ns2:hasIndustry "Public Administration"^^xsd:string ;
    ns2:hasMonth 3 ;
    ns2:hasOrganization "Pakistani Consulate in Jeddah"^^xsd:string ;
    ns2:hasYear 2014 ;
    ns2:isType_of ns2:Hacktivist,
        ns2:Message_Manipulation ;
    rdfs:comment "A Pakistani hacker going with the handle H4$N4!N H4XOR from Pakistan Haxor Crew hacks and defaces the official website of Pakistani consulate in Jeddah, Saudi Arabia against corrupt government in the country."^^xsd:string .

ns2:2398447c7480cffd a ns1:Probe,
        owl:NamedIndividual ;
    ns1:associatedCampaigns ns2:Bharat_Sanchar_Nigam_Limited__BSNL ;
    ns1:description "Political-Espionage"^^xsd:string ;
    ns1:isLaunchedBy ns2:China ;
    ns2:behaviour ns2:Political_Espionage ;
    ns2:hasActor "Huawei"^^xsd:string ;
    ns2:hasActorCountry "China"^^xsd:string ;
    ns2:hasCountry "India"^^xsd:string ;
    ns2:hasEventDate "2014-02-06T00:00:00"^^xsd:dateTime ;
    ns2:hasEventSubtype "Exploitation of Network Infrastructure"^^xsd:string ;
    ns2:hasEventType "Exploitive"^^xsd:string ;
    ns2:hasIndustry "Information"^^xsd:string ;
    ns2:hasMonth 2 ;
    ns2:hasOrganization "Bharat Sanchar Nigam Limited (BSNL)"^^xsd:string ;
    ns2:hasYear 2014 ;
    ns2:isType_of ns2:Exploitation_of_Network_Infrastructure ;
    rdfs:comment "India launches an investigation after a media report alleged that Chinese telecoms company Huawei had hacked into state-run telecoms carrier BSNL."^^xsd:string .

ns2:2517894581706036 a ns2:CyberattackData,
        owl:NamedIndividual ;
    ns1:associatedCampaigns ns2:Various_Government_Websites ;
    ns1:description "Protest"^^xsd:string ;
    ns1:isLaunchedBy ns2:Pakistan ;
    ns2:behaviour ns2:Protest ;
    ns2:hasActor "ASOR Hack Team"^^xsd:string ;
    ns2:hasActorCountry "Pakistan"^^xsd:string ;
    ns2:hasActorType "Hacktivist"^^xsd:string ;
    ns2:hasCountry "Pakistan"^^xsd:string ;
    ns2:hasEventDate "2014-09-04T00:00:00"^^xsd:dateTime ;
    ns2:hasEventSubtype "Exploitation of Application Server"^^xsd:string ;
    ns2:hasEventType "Exploitive"^^xsd:string ;
    ns2:hasIndustry "Public Administration"^^xsd:string ;
    ns2:hasMonth 9 ;
    ns2:hasOrganization "Various Government Websites"^^xsd:string ;
    ns2:hasYear 2014 ;
    ns2:isType_of ns2:Exploitation_of_Application_Server,
        ns2:Hacktivist ;
    rdfs:comment "Asor Hack Team dumps 23,000 records purportedly containing bank accounts of Government officials."^^xsd:string .

ns2:269bc8a1f79af806 a ns2:AccountAttack,
        owl:NamedIndividual ;
    ns1:associatedCampaigns ns2:Summit_County_Fair ;
    ns1:description "Financial"^^xsd:string ;
    ns2:behaviour ns2:Financial ;
    ns2:hasActorType "Criminal"^^xsd:string ;
    ns2:hasCampaign ns2:Utah ;
    ns2:hasCountry "United States of America"^^xsd:string ;
    ns2:hasCounty "Summit"^^xsd:string ;
    ns2:hasEventDate "2014-08-28T00:00:00"^^xsd:dateTime ;
    ns2:hasEventSubtype "Exploitation of Application Server"^^xsd:string ;
    ns2:hasEventType "Exploitive"^^xsd:string ;
    ns2:hasIndustry "Arts, Entertainment, and Recreation"^^xsd:string ;
    ns2:hasMonth 8 ;
    ns2:hasOrganization "Summit County Fair"^^xsd:string ;
    ns2:hasState "Utah"^^xsd:string ;
    ns2:hasYear 2014 ;
    ns2:isType_of ns2:Criminal,
        ns2:Exploitation_of_Application_Server ;
    rdfs:comment "Hundreds of personal bank accounts are at risk after a security breach was discovered involving ticket sales for the Summit County Fair rodeo and demolition derby."^^xsd:string .

ns2:2772c86463348aa7 a ns2:HackerSecurity,
        owl:NamedIndividual ;
    ns1:associatedCampaigns ns2:Klas_Telecom ;
    ns2:hasActor "NullCrew"^^xsd:string ;
    ns2:hasActorType "Hacktivist"^^xsd:string ;
    ns2:hasCampaign ns2:Virginia ;
    ns2:hasCountry "United States of America"^^xsd:string ;
    ns2:hasCounty "Fairfax"^^xsd:string ;
    ns2:hasEventDate "2014-04-06T00:00:00"^^xsd:dateTime ;
    ns2:hasEventSubtype "Exploitation of Application Server"^^xsd:string ;
    ns2:hasEventType "Exploitive"^^xsd:string ;
    ns2:hasIndustry "Information"^^xsd:string ;
    ns2:hasMonth 4 ;
    ns2:hasOrganization "Klas Telecom"^^xsd:string ;
    ns2:hasState "Virginia"^^xsd:string ;
    ns2:hasYear 2014 ;
    ns2:isType_of ns2:Exploitation_of_Application_Server,
        ns2:Hacktivist ;
    rdfs:comment "NullCrew hacks a legacy help desk system of the government contractor Klas Telecom, and leaks several accounts and passwords."^^xsd:string .

ns2:27d292a336279ebe a ns2:HackerSecurity,
        owl:NamedIndividual ;
    ns1:associatedCampaigns ns2:Turkcell ;
    ns1:description "Protest"^^xsd:string ;
    ns1:isLaunchedBy ns2:Turkey ;
    ns2:behaviour ns2:Protest ;
    ns2:hasActor "RedHack"^^xsd:string ;
    ns2:hasActorCountry "Turkey"^^xsd:string ;
    ns2:hasActorType "Hacktivist"^^xsd:string ;
    ns2:hasCountry "Turkey"^^xsd:string ;
    ns2:hasEventDate "2014-02-04T00:00:00"^^xsd:dateTime ;
    ns2:hasEventSubtype "Exploitation of Application Server"^^xsd:string ;
    ns2:hasEventType "Exploitive"^^xsd:string ;
    ns2:hasIndustry "Information"^^xsd:string ;
    ns2:hasMonth 2 ;
    ns2:hasOrganization "Turkcell"^^xsd:string ;
    ns2:hasYear 2014 ;
    ns2:isType_of ns2:Exploitation_of_Application_Server,
        ns2:Hacktivist ;
    rdfs:comment "Hackers of the RedHack group claim to have breached the systems of three major telecoms companies: TTNET, Vodafone and Turkcell. After the attack they leak the details of hundreds of individuals from TTNET and 5,000 Vodafone customers."^^xsd:string .

ns2:2813f649130ee3ac a ns2:HackerSecurity,
        owl:NamedIndividual ;
    ns1:associatedCampaigns ns2:Office_of_Personnel_Management ;
    ns1:description "Political-Espionage"^^xsd:string ;
    ns2:behaviour ns2:Political_Espionage ;
    ns2:hasActorType "Criminal"^^xsd:string ;
    ns2:hasCampaign ns2:Washington_D_C ;
    ns2:hasCountry "United States of America"^^xsd:string ;
    ns2:hasEventDate "2014-07-09T00:00:00"^^xsd:dateTime ;
    ns2:hasEventSubtype "Exploitation of Application Server"^^xsd:string ;
    ns2:hasEventType "Exploitive"^^xsd:string ;
    ns2:hasIndustry "Public Administration"^^xsd:string ;
    ns2:hasMonth 7 ;
    ns2:hasOrganization "Office of Personnel Management"^^xsd:string ;
    ns2:hasState "Washington D.C."^^xsd:string ;
    ns2:hasYear 2014 ;
    ns2:isType_of ns2:Criminal,
        ns2:Exploitation_of_Application_Server ;
    rdfs:comment "The New York Times reports that in March, Chinese hackers broke into the computer networks of the United States government agency that houses the personal information of all federal employees (the Office of Personnel Management)."^^xsd:string .

ns2:2914364202f37762 a ns2:CyberattackData,
        owl:NamedIndividual ;
    ns1:associatedCampaigns ns2:Reuters ;
    ns1:description "Protest"^^xsd:string ;
    ns1:isLaunchedBy ns2:Syrian_Arab_Republic ;
    ns2:behaviour ns2:Protest ;
    ns2:hasActor "Syrian Electronic Army"^^xsd:string ;
    ns2:hasActorCountry "Syrian Arab Republic"^^xsd:string ;
    ns2:hasActorType "Hacktivist"^^xsd:string ;
    ns2:hasCampaign ns2:New_York ;
    ns2:hasCountry "United States of America"^^xsd:string ;
    ns2:hasCounty "New York"^^xsd:string ;
    ns2:hasEventDate "2014-06-22T00:00:00"^^xsd:dateTime ;
    ns2:hasEventSubtype "Message Manipulation"^^xsd:string ;
    ns2:hasEventType "Disruptive"^^xsd:string ;
    ns2:hasIndustry "Management of Companies and Enterprises"^^xsd:string ;
    ns2:hasMonth 6 ;
    ns2:hasOrganization "Reuters"^^xsd:string ;
    ns2:hasState "New York"^^xsd:string ;
    ns2:hasYear 2014 ;
    ns2:isType_of ns2:Hacktivist,
        ns2:Message_Manipulation ;
    rdfs:comment "The Syrian Electronic Army is back and hacks Reuters redirecting the users to a web page supporting the Syrian regime. However the hack was possible after allegedly compromising Taboola, the ad provider."^^xsd:string .

ns2:29de69aee2862f57 a ns2:AccessSecurity,
        owl:NamedIndividual ;
    ns1:associatedCampaigns ns2:Arkansas_State_University ;
    ns1:description "Financial"^^xsd:string ;
    ns2:behaviour ns2:Financial ;
    ns2:hasActorType "Criminal"^^xsd:string ;
    ns2:hasCampaign ns2:Arkansas ;
    ns2:hasCountry "United States of America"^^xsd:string ;
    ns2:hasCounty "Craighead"^^xsd:string ;
    ns2:hasEventDate "2014-06-02T00:00:00"^^xsd:dateTime ;
    ns2:hasEventSubtype "Exploitation of Application Server"^^xsd:string ;
    ns2:hasEventType "Exploitive"^^xsd:string ;
    ns2:hasIndustry "Educational Services"^^xsd:string ;
    ns2:hasMonth 6 ;
    ns2:hasOrganization "Arkansas State University"^^xsd:string ;
    ns2:hasState "Arkansas"^^xsd:string ;
    ns2:hasYear 2014 ;
    ns2:isType_of ns2:Criminal,
        ns2:Exploitation_of_Application_Server ;
    rdfs:comment "At Arkansas State University (A-State), full and partial Social Security numbers are compromised for about 50,000 early childhood practitioners after unauthorized access is gained to databases related to the Traveling Arkansas Professional Pathways (TAPP)."^^xsd:string .

ns2:2a4df0d477113349 a ns2:CyberattackData,
        owl:NamedIndividual ;
    ns1:associatedCampaigns ns2:Kars_Municipality ;
    ns1:description "Protest"^^xsd:string ;
    ns1:isLaunchedBy ns2:Turkey ;
    ns2:behaviour ns2:Protest ;
    ns2:hasActor "RedHack"^^xsd:string ;
    ns2:hasActorCountry "Turkey"^^xsd:string ;
    ns2:hasActorType "Hacktivist"^^xsd:string ;
    ns2:hasCountry "Turkey"^^xsd:string ;
    ns2:hasEventDate "2014-02-10T00:00:00"^^xsd:dateTime ;
    ns2:hasEventSubtype "Message Manipulation"^^xsd:string ;
    ns2:hasEventType "Disruptive"^^xsd:string ;
    ns2:hasIndustry "Public Administration"^^xsd:string ;
    ns2:hasMonth 2 ;
    ns2:hasOrganization "Kars Municipality"^^xsd:string ;
    ns2:hasYear 2014 ;
    ns2:isType_of ns2:Hacktivist,
        ns2:Message_Manipulation ;
    rdfs:comment "The infamous RedHack collective joins the protests against the new Internet Law, and leak around two dozen records. They also deface a couple of local sites and hack the Ministry of Education."^^xsd:string .

ns2:2aa2ef042460fbba a ns2:AccountAttack,
        owl:NamedIndividual ;
    ns1:associatedCampaigns ns2:Carlo_Ancelotti ;
    ns2:hasActorType "Criminal"^^xsd:string ;
    ns2:hasCountry "Italy"^^xsd:string ;
    ns2:hasEventDate "2014-02-01T00:00:00"^^xsd:dateTime ;
    ns2:hasEventSubtype "Message Manipulation"^^xsd:string ;
    ns2:hasEventType "Disruptive"^^xsd:string ;
    ns2:hasIndustry "Other Services (except Public Administration)"^^xsd:string ;
    ns2:hasMonth 2 ;
    ns2:hasOrganization "Carlo Ancelotti"^^xsd:string ;
    ns2:hasYear 2014 ;
    ns2:isType_of ns2:Criminal,
        ns2:Message_Manipulation ;
    rdfs:comment "The Twitter account of Carlo Ancelotti (@MrAncelotti), the manager of the Spanish football team Real Madrid, has been hacked."^^xsd:string .

ns2:2b1f119a58e8d733 a ns2:AttackWebsite,
        owl:NamedIndividual ;
    ns1:associatedCampaigns ns2:Connecticut_State_Government_website ;
    ns1:description "Protest"^^xsd:string ;
    ns2:behaviour ns2:Protest ;
    ns2:hasActor "AnonGhost"^^xsd:string ;
    ns2:hasActorType "Hacktivist"^^xsd:string ;
    ns2:hasCampaign ns2:Connecticut ;
    ns2:hasCountry "United States of America"^^xsd:string ;
    ns2:hasCounty "Hartford"^^xsd:string ;
    ns2:hasEventDate "2014-07-31T00:00:00"^^xsd:dateTime ;
    ns2:hasEventSubtype "Message Manipulation"^^xsd:string ;
    ns2:hasEventType "Disruptive"^^xsd:string ;
    ns2:hasIndustry "Public Administration"^^xsd:string ;
    ns2:hasMonth 7 ;
    ns2:hasOrganization "Connecticut State Government website"^^xsd:string ;
    ns2:hasState "Connecticut"^^xsd:string ;
    ns2:hasYear 2014 ;
    ns2:isType_of ns2:Hacktivist,
        ns2:Message_Manipulation ;
    rdfs:comment "In name of #OpSaveGaza, AnonGhost, defaces the official web portal of State of Connecticut (ct.gov) along with the website of Connecticut's Governor (governor.ct.gov)."^^xsd:string .

ns2:2b47ee08e18be451 a ns2:HackerSecurity,
        owl:NamedIndividual ;
    ns1:associatedCampaigns ns2:Flight_Centre_Travel_Group ;
    ns1:description "Financial"^^xsd:string ;
    ns2:behaviour ns2:Financial ;
    ns2:hasActor "MrNervous"^^xsd:string ;
    ns2:hasActorType "Criminal"^^xsd:string ;
    ns2:hasCountry "Australia"^^xsd:string ;
    ns2:hasEventDate "2014-04-04T00:00:00"^^xsd:dateTime ;
    ns2:hasEventSubtype "Exploitation of Application Server"^^xsd:string ;
    ns2:hasEventType "Exploitive"^^xsd:string ;
    ns2:hasIndustry "Accommodation and Food Services"^^xsd:string ;
    ns2:hasMonth 4 ;
    ns2:hasOrganization "Flight Centre Travel Group"^^xsd:string ;
    ns2:hasYear 2014 ;
    ns2:isType_of ns2:Criminal,
        ns2:Exploitation_of_Application_Server ;
    rdfs:comment "A hacker who goes by the handle MrNervous or WhiteHatMrNervous tries to blackmail the Flight Centre Travel Group and dumps the information of 2,798 users including cleartext passwords."^^xsd:string .

ns2:2bded7a6d5e7d6d4 a ns2:BreachInformation,
        owl:NamedIndividual ;
    ns1:associatedCampaigns ns2:North_East_King_County_Regional_Public_S ;
    ns2:hasActorType "Criminal"^^xsd:string ;
    ns2:hasCampaign ns2:Washington ;
    ns2:hasCountry "United States of America"^^xsd:string ;
    ns2:hasCounty "King"^^xsd:string ;
    ns2:hasEventDate "2014-01-14T00:00:00"^^xsd:dateTime ;
    ns2:hasEventSubtype "Exploitation of Application Server"^^xsd:string ;
    ns2:hasEventType "Exploitive"^^xsd:string ;
    ns2:hasIndustry "Administrative and Support and Waste Management and Remediation Services"^^xsd:string ;
    ns2:hasMonth 1 ;
    ns2:hasOrganization "North East King County Regional Public Safety Communication Agency (NORCOM)"^^xsd:string ;
    ns2:hasState "Washington"^^xsd:string ;
    ns2:hasYear 2014 ;
    ns2:isType_of ns2:Criminal,
        ns2:Exploitation_of_Application_Server ;
    rdfs:comment "North East King County Regional Public Safety Communication Agency (NORCOM), a company that provides emergency communication services to the public, fire and police agencies, admits it suffered a server breach in late December. 6,000 records are affected."^^xsd:string .

ns2:2be7d3b46defe772 a ns2:AttackEmail,
        owl:NamedIndividual ;
    ns1:associatedCampaigns ns2:Sao_Paulo_State_Government ;
    ns2:hasActor "Anonymous"^^xsd:string ;
    ns2:hasActorType "Hacktivist"^^xsd:string ;
    ns2:hasCountry "Brazil"^^xsd:string ;
    ns2:hasEventDate "2014-01-28T00:00:00"^^xsd:dateTime ;
    ns2:hasEventSubtype "Exploitation of Application Server"^^xsd:string ;
    ns2:hasEventType "Exploitive"^^xsd:string ;
    ns2:hasIndustry "Public Administration"^^xsd:string ;
    ns2:hasMonth 1 ;
    ns2:hasOrganization "Sao Paulo State Government"^^xsd:string ;
    ns2:hasYear 2014 ;
    ns2:isType_of ns2:Exploitation_of_Application_Server,
        ns2:Hacktivist ;
    rdfs:comment "A hacker affiliated with the Anonymous hacks the official email account belonging to the press and communication department of Sao Paulo state government (saopaulo.sp.gov.br/)."^^xsd:string .

ns2:2c470e54622da9a6 a ns2:HackerSecurity,
        owl:NamedIndividual ;
    ns1:associatedCampaigns ns2:General_Directorate_of_the_EGO ;
    ns1:isLaunchedBy ns2:Turkey ;
    ns2:hasActor "RedHack"^^xsd:string ;
    ns2:hasActorCountry "Turkey"^^xsd:string ;
    ns2:hasActorType "Hacktivist"^^xsd:string ;
    ns2:hasCountry "Turkey"^^xsd:string ;
    ns2:hasEventDate "2014-01-15T00:00:00"^^xsd:dateTime ;
    ns2:hasEventSubtype "Exploitation of Application Server"^^xsd:string ;
    ns2:hasEventType "Exploitive"^^xsd:string ;
    ns2:hasIndustry "Public Administration"^^xsd:string ;
    ns2:hasMonth 1 ;
    ns2:hasOrganization "General Directorate of the EGO"^^xsd:string ;
    ns2:hasYear 2014 ;
    ns2:isType_of ns2:Exploitation_of_Application_Server,
        ns2:Hacktivist ;
    rdfs:comment "Hackers of the RedHack collective breach the systems of the General Directorate of EGO (ego.gov.tr), the organization that serves as the public transport department for the municipality of Ankara, the capital city of Turkey."^^xsd:string .

ns2:2c993f8fe38d8ffa a ns2:AccessAttack,
        owl:NamedIndividual ;
    ns1:associatedCampaigns ns2:University_of_West_Florida ;
    ns2:hasActorType "Criminal"^^xsd:string ;
    ns2:hasCampaign ns2:Florida ;
    ns2:hasCountry "United States of America"^^xsd:string ;
    ns2:hasCounty "Escambia"^^xsd:string ;
    ns2:hasEventDate "2014-07-31T00:00:00"^^xsd:dateTime ;
    ns2:hasEventSubtype "Exploitation of Application Server"^^xsd:string ;
    ns2:hasEventType "Exploitive"^^xsd:string ;
    ns2:hasIndustry "Educational Services"^^xsd:string ;
    ns2:hasMonth 7 ;
    ns2:hasOrganization "University of West Florida"^^xsd:string ;
    ns2:hasState "Florida"^^xsd:string ;
    ns2:hasYear 2014 ;
    ns2:isType_of ns2:Criminal,
        ns2:Exploitation_of_Application_Server ;
    rdfs:comment "The University of West Florida announces that passwords and usernames for about 160 people may have been compromised by some individuals attacking the network to intercept ArgoNet usernames and passwords."^^xsd:string .

ns2:2cd3d7f92f0a23ef a ns2:AccountAttack,
        owl:NamedIndividual ;
    ns1:associatedCampaigns ns2:Supervalu ;
    ns1:description "Financial"^^xsd:string ;
    ns2:behaviour ns2:Financial ;
    ns2:hasActorType "Criminal"^^xsd:string ;
    ns2:hasCampaign ns2:Minnesota ;
    ns2:hasCountry "United States of America"^^xsd:string ;
    ns2:hasCounty "Hennepin"^^xsd:string ;
    ns2:hasEventDate "2014-08-15T00:00:00"^^xsd:dateTime ;
    ns2:hasEventSubtype "Exploitation of Sensors"^^xsd:string ;
    ns2:hasEventType "Exploitive"^^xsd:string ;
    ns2:hasIndustry "Retail Trade"^^xsd:string ;
    ns2:hasMonth 8 ;
    ns2:hasOrganization "Supervalu"^^xsd:string ;
    ns2:hasState "Minnesota"^^xsd:string ;
    ns2:hasYear 2014 ;
    ns2:isType_of ns2:Criminal,
        ns2:Exploitation_of_Sensors ;
    rdfs:comment "SuperValu, announces that its customers' credit card information may have been stolen during a network intrusion. As a consequence, even AB Acquisition LLC, to which SuperValu provides IT services, is affected."^^xsd:string .

ns2:2cdbdec039b5cc2f a ns2:HackerSecurity,
        owl:NamedIndividual ;
    ns1:associatedCampaigns ns2:National_Socialist_Party_of_Canada ;
    ns1:description "Protest"^^xsd:string ;
    ns2:behaviour ns2:Protest ;
    ns2:hasActor "nairb"^^xsd:string ;
    ns2:hasActorType "Hacktivist"^^xsd:string ;
    ns2:hasCountry "Canada"^^xsd:string ;
    ns2:hasEventDate "2014-02-13T00:00:00"^^xsd:dateTime ;
    ns2:hasEventSubtype "Exploitation of Application Server"^^xsd:string ;
    ns2:hasEventType "Exploitive"^^xsd:string ;
    ns2:hasIndustry "Other Services (except Public Administration)"^^xsd:string ;
    ns2:hasMonth 2 ;
    ns2:hasOrganization "National-Socialist Party of Canada"^^xsd:string ;
    ns2:hasYear 2014 ;
    ns2:isType_of ns2:Exploitation_of_Application_Server,
        ns2:Hacktivist ;
    rdfs:comment "nairb AKA @SQLiNairb hacks the National-Socialist Party of Canada official (nspcanada.nfshost.com) and leaks around 1,500 accounts."^^xsd:string .

ns2:2d56fed299b962b7 a ns2:BreachSecurity,
        owl:NamedIndividual ;
    ns1:associatedCampaigns ns2:California_State_University ;
    ns2:hasActorType "Criminal"^^xsd:string ;
    ns2:hasCampaign ns2:California ;
    ns2:hasCountry "United States of America"^^xsd:string ;
    ns2:hasCounty "Alameda"^^xsd:string ;
    ns2:hasEventDate "2014-09-06T00:00:00"^^xsd:dateTime ;
    ns2:hasEventSubtype "Exploitation of Application Server"^^xsd:string ;
    ns2:hasEventType "Exploitive"^^xsd:string ;
    ns2:hasIndustry "Educational Services"^^xsd:string ;
    ns2:hasMonth 9 ;
    ns2:hasOrganization "California State University"^^xsd:string ;
    ns2:hasState "California"^^xsd:string ;
    ns2:hasYear 2014 ;
    ns2:isType_of ns2:Criminal,
        ns2:Exploitation_of_Application_Server ;
    rdfs:comment "California State University officials reveal a breach in an East Bay web server used to store personal employee information. The security breach occurred on Aug. 23, 2013 and was discovered Aug. 11 of this year."^^xsd:string .

ns2:2db7da5170ced481 a ns2:DefaceHacker,
        owl:NamedIndividual ;
    ns1:associatedCampaigns ns2:Pakistan_Official_Portal ;
    ns1:description "Protest"^^xsd:string ;
    ns2:behaviour ns2:Protest ;
    ns2:hasActorType "Criminal"^^xsd:string ;
    ns2:hasCountry "Pakistan"^^xsd:string ;
    ns2:hasEventDate "2014-09-01T00:00:00"^^xsd:dateTime ;
    ns2:hasEventSubtype "Message Manipulation"^^xsd:string ;
    ns2:hasEventType "Disruptive"^^xsd:string ;
    ns2:hasIndustry "Public Administration"^^xsd:string ;
    ns2:hasMonth 9 ;
    ns2:hasOrganization "Pakistan Official Portal"^^xsd:string ;
    ns2:hasYear 2014 ;
    ns2:isType_of ns2:Criminal,
        ns2:Message_Manipulation ;
    rdfs:comment "In name of OpPakistan, unknown Hacktivists deface the official portal of Pakistan (pakistan.gov.pk), demanding resignation of prime minister Nawaz Shareef."^^xsd:string .

ns2:2ebb3f8bf502a2a5 a ns2:AttackWebsite,
        owl:NamedIndividual ;
    ns1:associatedCampaigns ns2:eyeofdubai_ae ;
    ns2:hasActor "Smitt3nz AKA Rubber"^^xsd:string ;
    ns2:hasCountry "United Arab Emirates"^^xsd:string ;
    ns2:hasEventDate "2014-08-12T00:00:00"^^xsd:dateTime ;
    ns2:hasEventSubtype "Exploitation of Application Server"^^xsd:string ;
    ns2:hasEventType "Exploitive"^^xsd:string ;
    ns2:hasIndustry "Information"^^xsd:string ;
    ns2:hasMonth 8 ;
    ns2:hasOrganization "eyeofdubai.ae"^^xsd:string ;
    ns2:hasYear 2014 ;
    ns2:isType_of ns2:Exploitation_of_Application_Server ;
    rdfs:comment "@smitt3nz hacks eyeofdubai.ae and dumps nearly 1,000 usernames and plain text passwords."^^xsd:string .

ns2:30cafd89b274c88a a ns2:HackerSecurity,
        owl:NamedIndividual ;
    ns1:associatedCampaigns ns2:Boeing ;
    ns1:description "Industrial-Espionage"^^xsd:string ;
    ns1:isLaunchedBy ns2:China ;
    ns2:behaviour ns2:Industrial_Espionage ;
    ns2:hasActor "Su Bin"^^xsd:string ;
    ns2:hasActorCountry "China"^^xsd:string ;
    ns2:hasActorType "Nation-State"^^xsd:string ;
    ns2:hasCampaign ns2:Washington ;
    ns2:hasCountry "United States of America"^^xsd:string ;
    ns2:hasCounty "King"^^xsd:string ;
    ns2:hasEventDate "2014-07-13T00:00:00"^^xsd:dateTime ;
    ns2:hasEventSubtype "Exploitation of Application Server"^^xsd:string ;
    ns2:hasEventType "Exploitive"^^xsd:string ;
    ns2:hasIndustry "Manufacturing"^^xsd:string ;
    ns2:hasMonth 7 ;
    ns2:hasOrganization "Boeing"^^xsd:string ;
    ns2:hasState "Washington"^^xsd:string ;
    ns2:hasYear 2014 ;
    ns2:isType_of ns2:Exploitation_of_Application_Server,
        ns2:Nation_State ;
    rdfs:comment "The US Department of Justice announces that a Chinese businessman, Su Bin, has been charged with hacking into the computer systems of Boeing, Lockheed Martin and other aerospace companies."^^xsd:string .

ns2:311eec3442f50041 a ns2:Phishing,
        owl:NamedIndividual ;
    ns1:associatedCampaigns ns2:Dartmouth_Hitchcock ;
    ns1:description "Financial"^^xsd:string ;
    ns2:behaviour ns2:Financial ;
    ns2:hasActorType "Criminal"^^xsd:string ;
    ns2:hasCampaign ns2:New_Hampshire ;
    ns2:hasCountry "United States of America"^^xsd:string ;
    ns2:hasCounty "Grafton"^^xsd:string ;
    ns2:hasEventDate "2014-01-31T00:00:00"^^xsd:dateTime ;
    ns2:hasEventSubtype "Exploitation of End Hosts"^^xsd:string ;
    ns2:hasEventType "Exploitive"^^xsd:string ;
    ns2:hasIndustry "Health Care and Social Assistance"^^xsd:string ;
    ns2:hasMonth 1 ;
    ns2:hasOrganization "Dartmouth-Hitchcock"^^xsd:string ;
    ns2:hasState "New Hampshire"^^xsd:string ;
    ns2:hasYear 2014 ;
    ns2:isType_of ns2:Criminal,
        ns2:Exploitation_of_End_Hosts ;
    rdfs:comment "Dartmouth-Hitchcock notifies some employees that their names and direct deposit bank account information were compromised after some employees fell  for a phishing attempt."^^xsd:string .

ns2:319dbf1330b8c584 a ns2:Malware,
        owl:NamedIndividual ;
    ns1:associatedCampaigns ns2:Chicago_Yacht_Club ;
    ns2:hasActorType "Criminal"^^xsd:string ;
    ns2:hasCampaign ns2:Illinois ;
    ns2:hasCountry "United States of America"^^xsd:string ;
    ns2:hasCounty "Cook"^^xsd:string ;
    ns2:hasEventDate "2014-08-08T00:00:00"^^xsd:dateTime ;
    ns2:hasEventSubtype "Exploitation of Application Server"^^xsd:string ;
    ns2:hasEventType "Exploitive"^^xsd:string ;
    ns2:hasIndustry "Other Services (except Public Administration)"^^xsd:string ;
    ns2:hasMonth 8 ;
    ns2:hasOrganization "Chicago Yacht Club"^^xsd:string ;
    ns2:hasState "Illinois"^^xsd:string ;
    ns2:hasYear 2014 ;
    ns2:isType_of ns2:Criminal,
        ns2:Exploitation_of_Application_Server ;
    rdfs:comment "Following an investigation into a PoS system crash, Chicago Yacht Club finds evidence of malware installation on one of their servers and notifies guests who made purchases."^^xsd:string .

ns2:33360a84f1d88f08 a ns2:HackerSecurity,
        owl:NamedIndividual ;
    ns1:associatedCampaigns ns2:Mercantile_Communications_Pvt ;
    ns1:isLaunchedBy ns2:Turkey ;
    ns2:hasActor "Turkish Ajan"^^xsd:string ;
    ns2:hasActorCountry "Turkey"^^xsd:string ;
    ns2:hasActorType "Hacktivist"^^xsd:string ;
    ns2:hasCountry "Nepal"^^xsd:string ;
    ns2:hasEventDate "2014-02-20T00:00:00"^^xsd:dateTime ;
    ns2:hasEventSubtype "Exploitation of Application Server"^^xsd:string ;
    ns2:hasEventType "Exploitive"^^xsd:string ;
    ns2:hasIndustry "Information"^^xsd:string ;
    ns2:hasMonth 2 ;
    ns2:hasOrganization "Mercantile Communications Pvt"^^xsd:string ;
    ns2:hasYear 2014 ;
    ns2:isType_of ns2:Exploitation_of_Application_Server,
        ns2:Hacktivist ;
    rdfs:comment "Hackers of the Turkish Ajan group are back and target Mercantile Communications Pvt (mos.com.np), a major Nepali Internet service provider (ISP), leaking the database structure information, and over 100 records containing the names and email addresses of the company's employees."^^xsd:string .

ns2:34e34c61cf03b1e7 a ns2:CyberattackSystem,
        owl:NamedIndividual ;
    ns1:associatedCampaigns ns2:INVALSI ;
    ns2:hasActorType "Criminal"^^xsd:string ;
    ns2:hasCountry "Italy"^^xsd:string ;
    ns2:hasEventDate "2014-06-15T00:00:00"^^xsd:dateTime ;
    ns2:hasEventSubtype "Exploitation of End Hosts"^^xsd:string ;
    ns2:hasEventType "Exploitive"^^xsd:string ;
    ns2:hasIndustry "Educational Services"^^xsd:string ;
    ns2:hasMonth 6 ;
    ns2:hasOrganization "INVALSI"^^xsd:string ;
    ns2:hasYear 2014 ;
    ns2:isType_of ns2:Criminal,
        ns2:Exploitation_of_End_Hosts ;
    rdfs:comment "An unknown hacker illegitimately accesses the systems of INVALSI, the public Italian System for School Assessment. This happens few days before the official start of the assessments affecting 600,000 students."^^xsd:string .

ns2:355d01e769b2ff87 a ns2:CyberattackData,
        owl:NamedIndividual ;
    ns1:associatedCampaigns ns2:Harley_Medical_Group ;
    ns1:description "Financial"^^xsd:string ;
    ns2:behaviour ns2:Financial ;
    ns2:hasActorType "Criminal"^^xsd:string ;
    ns2:hasCountry "United Kingdom of Great Britain and Northern Ireland"^^xsd:string ;
    ns2:hasEventDate "2014-04-14T00:00:00"^^xsd:dateTime ;
    ns2:hasEventSubtype "Exploitation of Application Server"^^xsd:string ;
    ns2:hasEventType "Exploitive"^^xsd:string ;
    ns2:hasIndustry "Health Care and Social Assistance"^^xsd:string ;
    ns2:hasMonth 4 ;
    ns2:hasOrganization "Harley Medical Group"^^xsd:string ;
    ns2:hasYear 2014 ;
    ns2:isType_of ns2:Criminal,
        ns2:Exploitation_of_Application_Server ;
    rdfs:comment "The personal details of nearly half a million people, considering cosmetic surgery, may have been accessed by hackers who then attempted to blackmail Harley Medical Group, a leading chain of clinics."^^xsd:string .

ns2:35f1da5548e66e4c a ns2:HackerSecurity,
        owl:NamedIndividual ;
    ns1:associatedCampaigns ns2:Medtronic ;
    ns1:description "Industrial-Espionage"^^xsd:string ;
    ns2:behaviour ns2:Industrial_Espionage ;
    ns2:hasActorType "Criminal"^^xsd:string ;
    ns2:hasCampaign ns2:Minnesota ;
    ns2:hasCountry "United States of America"^^xsd:string ;
    ns2:hasCounty "Hennepin"^^xsd:string ;
    ns2:hasEventDate "2014-02-10T00:00:00"^^xsd:dateTime ;
    ns2:hasEventSubtype "Exploitation of Application Server"^^xsd:string ;
    ns2:hasEventType "Exploitive"^^xsd:string ;
    ns2:hasIndustry "Manufacturing"^^xsd:string ;
    ns2:hasMonth 2 ;
    ns2:hasOrganization "Medtronic"^^xsd:string ;
    ns2:hasState "Minnesota"^^xsd:string ;
    ns2:hasYear 2014 ;
    ns2:isType_of ns2:Criminal,
        ns2:Exploitation_of_Application_Server ;
    rdfs:comment "The computer networks of three big medical device makers are breached by unknown attackers likely interested in the companies' intellectual property. The companies in question are Medtronic, Boston Scientific and St. Jude Medical."^^xsd:string .

ns2:364e2da514270f98 a ns2:CyberattackInformation,
        owl:NamedIndividual ;
    ns1:associatedCampaigns ns2:Malaysia_Airlines ;
    ns2:hasActorType "Criminal"^^xsd:string ;
    ns2:hasCountry "Malaysia"^^xsd:string ;
    ns2:hasEventDate "2014-08-20T00:00:00"^^xsd:dateTime ;
    ns2:hasEventSubtype "Exploitation of End Hosts"^^xsd:string ;
    ns2:hasEventType "Exploitive"^^xsd:string ;
    ns2:hasIndustry "Transportation and Warehousing"^^xsd:string ;
    ns2:hasMonth 8 ;
    ns2:hasOrganization "Malaysia Airlines"^^xsd:string ;
    ns2:hasYear 2014 ;
    ns2:isType_of ns2:Criminal,
        ns2:Exploitation_of_End_Hosts ;
    rdfs:comment "The computers of high-ranking officials in Malaysian agencies involved in the MH370 investigation are hacked and classified information is stolen. Suspects are directed to China."^^xsd:string .

ns2:36dd985b3af801b5 a ns2:CyberattackInformation,
        owl:NamedIndividual ;
    ns1:associatedCampaigns ns2:PrezidentBank ;
    ns2:hasActor "Dr.SHA6H"^^xsd:string ;
    ns2:hasActorType "Hacktivist"^^xsd:string ;
    ns2:hasCountry "Turkmenistan"^^xsd:string ;
    ns2:hasEventDate "2014-02-07T00:00:00"^^xsd:dateTime ;
    ns2:hasEventSubtype "Message Manipulation"^^xsd:string ;
    ns2:hasEventType "Disruptive"^^xsd:string ;
    ns2:hasIndustry "Finance and Insurance"^^xsd:string ;
    ns2:hasMonth 2 ;
    ns2:hasOrganization "PrezidentBank"^^xsd:string ;
    ns2:hasYear 2014 ;
    ns2:isType_of ns2:Hacktivist,
        ns2:Message_Manipulation ;
    rdfs:comment "The official websites of two Turkmenistan state-owned commercial banks are hacked and defaced by Dr.Sha6h, to raise awareness of the situation in Syria. The victims are: Turkmenbashi Bank (tbbank.gov.tm), PrezidentBank (presidentbank.gov.tm)."^^xsd:string .

ns2:3722459375612f98 a ns2:AttackInformation,
        owl:NamedIndividual ;
    ns1:associatedCampaigns ns2:West_Bengal_Public_Health_Engineering_De ;
    ns1:description "Protest"^^xsd:string ;
    ns1:isLaunchedBy ns2:Pakistan ;
    ns2:behaviour ns2:Protest ;
    ns2:hasActor "Pakistan Haxors Crew"^^xsd:string ;
    ns2:hasActorCountry "Pakistan"^^xsd:string ;
    ns2:hasActorType "Hacktivist"^^xsd:string ;
    ns2:hasCountry "India"^^xsd:string ;
    ns2:hasEventDate "2014-02-04T00:00:00"^^xsd:dateTime ;
    ns2:hasEventSubtype "Message Manipulation"^^xsd:string ;
    ns2:hasEventType "Disruptive"^^xsd:string ;
    ns2:hasIndustry "Public Administration"^^xsd:string ;
    ns2:hasMonth 2 ;
    ns2:hasOrganization "West Bengal Public Health Engineering Department"^^xsd:string ;
    ns2:hasYear 2014 ;
    ns2:isType_of ns2:Hacktivist,
        ns2:Message_Manipulation ;
    rdfs:comment "West Bengal's Public Health Engineering Department (wbphed.gov.in) is attacked and defaced by a group of Pakistani hacktivists demanding to \"free Kashmir\" among other things."^^xsd:string .

ns2:37e75f22d0e75f4d a ns2:AttackWebsite,
        owl:NamedIndividual ;
    ns1:associatedCampaigns ns2:Ministry_of_Education_of_Armenia ;
    ns1:description "Protest"^^xsd:string ;
    ns1:isLaunchedBy ns2:Azerbaijan ;
    ns2:behaviour ns2:Protest ;
    ns2:hasActor "Anti-Armenia Team"^^xsd:string ;
    ns2:hasActorCountry "Azerbaijan"^^xsd:string ;
    ns2:hasActorType "Hacktivist"^^xsd:string ;
    ns2:hasCountry "Armenia"^^xsd:string ;
    ns2:hasEventDate "2014-01-23T00:00:00"^^xsd:dateTime ;
    ns2:hasEventSubtype "Message Manipulation"^^xsd:string ;
    ns2:hasEventType "Disruptive"^^xsd:string ;
    ns2:hasIndustry "Public Administration"^^xsd:string ;
    ns2:hasMonth 1 ;
    ns2:hasOrganization "Ministry of Education of Armenia"^^xsd:string ;
    ns2:hasYear 2014 ;
    ns2:isType_of ns2:Hacktivist,
        ns2:Message_Manipulation ;
    rdfs:comment "Azerbaijan Hackers from Anti-Armenia Team have hacked and defaced several Armenian government ministries websites."^^xsd:string .

ns2:37e96b8f0c2ce8ca a ns2:AccountAttack,
        owl:NamedIndividual ;
    ns1:associatedCampaigns ns2:Craftsman_Book ;
    ns1:description "Financial"^^xsd:string ;
    ns2:behaviour ns2:Financial ;
    ns2:hasActorType "Criminal"^^xsd:string ;
    ns2:hasCampaign ns2:California ;
    ns2:hasCountry "United States of America"^^xsd:string ;
    ns2:hasCounty "San Diego"^^xsd:string ;
    ns2:hasEventDate "2014-06-12T00:00:00"^^xsd:dateTime ;
    ns2:hasEventSubtype "Exploitation of Application Server"^^xsd:string ;
    ns2:hasEventType "Exploitive"^^xsd:string ;
    ns2:hasIndustry "Wholesale Trade"^^xsd:string ;
    ns2:hasMonth 6 ;
    ns2:hasOrganization "Craftsman Book"^^xsd:string ;
    ns2:hasState "California"^^xsd:string ;
    ns2:hasYear 2014 ;
    ns2:isType_of ns2:Criminal,
        ns2:Exploitation_of_Application_Server ;
    rdfs:comment "An estimated 11,000 customers who bought products from Craftsman-book.com have their credit card details compromised after the company website is compromised."^^xsd:string .

ns2:38bc58f9ce5dd886 a ns2:AnonymousAttack,
        owl:NamedIndividual ;
    ns1:associatedCampaigns ns2:Ferguson_Police ;
    ns1:description "Protest"^^xsd:string ;
    ns2:behaviour ns2:Protest ;
    ns2:hasActor "Anonymous"^^xsd:string ;
    ns2:hasActorType "Hacktivist"^^xsd:string ;
    ns2:hasCampaign ns2:Missouri ;
    ns2:hasCountry "United States of America"^^xsd:string ;
    ns2:hasCounty "St. Louis"^^xsd:string ;
    ns2:hasEventDate "2014-08-13T00:00:00"^^xsd:dateTime ;
    ns2:hasEventSubtype "Exploitation of Application Server"^^xsd:string ;
    ns2:hasEventType "Exploitive"^^xsd:string ;
    ns2:hasIndustry "Public Administration"^^xsd:string ;
    ns2:hasMonth 8 ;
    ns2:hasOrganization "Ferguson Police"^^xsd:string ;
    ns2:hasState "Missouri"^^xsd:string ;
    ns2:hasYear 2014 ;
    ns2:isType_of ns2:Exploitation_of_Application_Server,
        ns2:Hacktivist ;
    rdfs:comment "The Anonymous collective publish hours of alleged police dispatch tapes on Twitter and YouTube from the day unarmed teenager Michael Brown was shot to death by police in a St. Louis suburb."^^xsd:string .

ns2:38c0c29902a3ed04 a ns2:BreachInformation,
        owl:NamedIndividual ;
    ns1:associatedCampaigns ns2:Houston_Astros ;
    ns2:hasActorType "Criminal"^^xsd:string ;
    ns2:hasCampaign ns2:Texas ;
    ns2:hasCountry "United States of America"^^xsd:string ;
    ns2:hasCounty "Harris"^^xsd:string ;
    ns2:hasEventDate "2014-07-01T00:00:00"^^xsd:dateTime ;
    ns2:hasEventSubtype "Exploitation of Application Server"^^xsd:string ;
    ns2:hasEventType "Exploitive"^^xsd:string ;
    ns2:hasIndustry "Arts, Entertainment, and Recreation"^^xsd:string ;
    ns2:hasMonth 7 ;
    ns2:hasOrganization "Houston Astros"^^xsd:string ;
    ns2:hasState "Texas"^^xsd:string ;
    ns2:hasYear 2014 ;
    ns2:isType_of ns2:Criminal,
        ns2:Exploitation_of_Application_Server ;
    rdfs:comment "The systems of the Houston Astros baseball team are accessed by an unauthorized person, who extracted content revealing internal trade talks."^^xsd:string .

ns2:39c2b71d9b14c510 a ns2:AttackWebsite,
        owl:NamedIndividual ;
    ns1:associatedCampaigns ns2:Las_Vegas_Sands_Corp ;
    ns1:description "Political-Espionage"^^xsd:string ;
    ns1:isLaunchedBy ns2:Iran__Islamic_Republic_of ;
    ns2:behaviour ns2:Political_Espionage ;
    ns2:hasActor "Anti WMD Team"^^xsd:string ;
    ns2:hasActorCountry "Iran (Islamic Republic of)"^^xsd:string ;
    ns2:hasActorType "Hacktivist"^^xsd:string ;
    ns2:hasCampaign ns2:Nevada ;
    ns2:hasCountry "United States of America"^^xsd:string ;
    ns2:hasCounty "Clark"^^xsd:string ;
    ns2:hasEventDate "2014-02-10T00:00:00"^^xsd:dateTime ;
    ns2:hasEventSubtype "Data Attack,Exploitation of Application Server,Message Manipulation"^^xsd:string ;
    ns2:hasEventType "Mixed"^^xsd:string ;
    ns2:hasIndustry "Accommodation and Food Services"^^xsd:string ;
    ns2:hasMonth 2 ;
    ns2:hasOrganization "Las Vegas Sands Corp"^^xsd:string ;
    ns2:hasState "Nevada"^^xsd:string ;
    ns2:hasYear 2014 ;
    ns2:isType_of ns2:Data_Attack_Exploitation_of_Application_,
        ns2:Hacktivist ;
    rdfs:comment "Some websites owned by Las Vegas Sands Corp, one of the world's largest casino operators, have been hacked and defaced by a group called the Anti WMD Team. The defaced page also contains personal information of Sands employees including e-mail ID and social security numbers. Additionally, the attackers deployed data-wiping malware on the Sands networks, severely disrupting their operation. The attack was allegedly carried out by Iranian hackers in retaliation for a remark by Sands Corp CEO Sheldon Adelson."^^xsd:string .

ns2:3a52161e35a08ea0 a ns2:DefaceHacker,
        owl:NamedIndividual ;
    ns1:associatedCampaigns ns2:Directorate_General_Public_Relations__Go ;
    ns1:description "Protest"^^xsd:string ;
    ns1:isLaunchedBy ns2:Pakistan ;
    ns2:behaviour ns2:Protest ;
    ns2:hasActor "Team Pak Cyber Experts"^^xsd:string ;
    ns2:hasActorCountry "Pakistan"^^xsd:string ;
    ns2:hasActorType "Hacktivist"^^xsd:string ;
    ns2:hasCountry "Pakistan"^^xsd:string ;
    ns2:hasEventDate "2014-06-25T00:00:00"^^xsd:dateTime ;
    ns2:hasEventSubtype "Message Manipulation"^^xsd:string ;
    ns2:hasEventType "Disruptive"^^xsd:string ;
    ns2:hasIndustry "Public Administration"^^xsd:string ;
    ns2:hasMonth 6 ;
    ns2:hasOrganization "Directorate General Public Relations, Government of the Punjab"^^xsd:string ;
    ns2:hasYear 2014 ;
    ns2:isType_of ns2:Hacktivist,
        ns2:Message_Manipulation ;
    rdfs:comment "Again a defacement to protest against police brutality. Hackers of the Team Pak Cyber Experts deface the official website of Directorate General Public Relations, Government of the Punjab (dgpr.gop.pk)."^^xsd:string .

ns2:3a94b8cf6dde1f66 a ns2:DDoS,
        owl:NamedIndividual ;
    ns1:associatedCampaigns ns2:Battle_net ;
    ns2:hasActor "DERP Trolling"^^xsd:string ;
    ns2:hasCampaign ns2:California ;
    ns2:hasCountry "United States of America"^^xsd:string ;
    ns2:hasCounty "Orange"^^xsd:string ;
    ns2:hasEventDate "2014-01-03T00:00:00"^^xsd:dateTime ;
    ns2:hasEventSubtype "External Denial of Service"^^xsd:string ;
    ns2:hasEventType "Disruptive"^^xsd:string ;
    ns2:hasIndustry "Information"^^xsd:string ;
    ns2:hasMonth 1 ;
    ns2:hasOrganization "Battle.net"^^xsd:string ;
    ns2:hasState "California"^^xsd:string ;
    ns2:hasYear 2014 ;
    ns2:isType_of ns2:External_Denial_of_Service ;
    rdfs:comment "The servers for Steam, Origin, Battle.net, and League of Legends are brought down temporarily by apparent DDoS attacks that seem to be related to a swatting attack on an individual known for streaming games."^^xsd:string .

ns2:3aab5fad206b01aa a ns2:AccountAttack,
        owl:NamedIndividual ;
    ns1:associatedCampaigns ns2:comicbookdb_com ;
    ns2:hasActor "Smitt3nz AKA Rubber"^^xsd:string ;
    ns2:hasCountry "United States of America"^^xsd:string ;
    ns2:hasEventDate "2014-09-08T00:00:00"^^xsd:dateTime ;
    ns2:hasEventSubtype "Exploitation of Application Server"^^xsd:string ;
    ns2:hasEventType "Exploitive"^^xsd:string ;
    ns2:hasIndustry "Information"^^xsd:string ;
    ns2:hasMonth 9 ;
    ns2:hasOrganization "comicbookdb.com"^^xsd:string ;
    ns2:hasYear 2014 ;
    ns2:isType_of ns2:Exploitation_of_Application_Server ;
    rdfs:comment "Smitt3nz hacks comicbookdb.com and dumps 52,000 plaintext accounts (usernames and passwords)."^^xsd:string .

ns2:3ad9b96e2972e495 a ns2:AttackWebsite,
        owl:NamedIndividual ;
    ns1:associatedCampaigns ns2:Central_Bank_of_Turkey ;
    ns1:description "Protest"^^xsd:string ;
    ns1:isLaunchedBy ns2:Turkey ;
    ns2:behaviour ns2:Protest ;
    ns2:hasActor "RedHack"^^xsd:string ;
    ns2:hasActorCountry "Turkey"^^xsd:string ;
    ns2:hasActorType "Hacktivist"^^xsd:string ;
    ns2:hasCountry "Turkey"^^xsd:string ;
    ns2:hasEventDate "2014-01-16T00:00:00"^^xsd:dateTime ;
    ns2:hasEventSubtype "External Denial of Service"^^xsd:string ;
    ns2:hasEventType "Disruptive"^^xsd:string ;
    ns2:hasIndustry "Finance and Insurance"^^xsd:string ;
    ns2:hasMonth 1 ;
    ns2:hasOrganization "Central Bank of Turkey"^^xsd:string ;
    ns2:hasYear 2014 ;
    ns2:isType_of ns2:External_Denial_of_Service,
        ns2:Hacktivist ;
    rdfs:comment "The RedHack collective takes down the official website of the Central Bank of Turkey (tcmb.gov.tr) to protest poor monetary policy."^^xsd:string .

ns2:3b7ef47d630ccbc4 a ns2:HackerSecurity,
        owl:NamedIndividual ;
    ns1:associatedCampaigns ns2:University_of_Virginia ;
    ns1:description "Protest"^^xsd:string ;
    ns2:behaviour ns2:Protest ;
    ns2:hasActor "NullCrew"^^xsd:string ;
    ns2:hasActorType "Hacktivist"^^xsd:string ;
    ns2:hasCampaign ns2:Virginia ;
    ns2:hasCountry "United States of America"^^xsd:string ;
    ns2:hasCounty "Albemarle"^^xsd:string ;
    ns2:hasEventDate "2014-04-21T00:00:00"^^xsd:dateTime ;
    ns2:hasEventSubtype "Exploitation of Application Server"^^xsd:string ;
    ns2:hasEventType "Exploitive"^^xsd:string ;
    ns2:hasIndustry "Educational Services"^^xsd:string ;
    ns2:hasMonth 4 ;
    ns2:hasOrganization "University of Virginia"^^xsd:string ;
    ns2:hasState "Virginia"^^xsd:string ;
    ns2:hasYear 2014 ;
    ns2:isType_of ns2:Exploitation_of_Application_Server,
        ns2:Hacktivist ;
    rdfs:comment "University of Virginia (1 million files leaked)."^^xsd:string .

ns2:3bbaff69a61c8a44 a ns2:AttackWebsite,
        owl:NamedIndividual ;
    ns1:associatedCampaigns ns2:Rumah_Principality ;
    ns1:description "Protest"^^xsd:string ;
    ns1:isLaunchedBy ns2:Syrian_Arab_Republic ;
    ns2:behaviour ns2:Protest ;
    ns2:hasActor "Syrian Electronic Army"^^xsd:string ;
    ns2:hasActorCountry "Syrian Arab Republic"^^xsd:string ;
    ns2:hasActorType "Hacktivist"^^xsd:string ;
    ns2:hasCountry "Saudi Arabia"^^xsd:string ;
    ns2:hasEventDate "2014-01-16T00:00:00"^^xsd:dateTime ;
    ns2:hasEventSubtype "Message Manipulation"^^xsd:string ;
    ns2:hasEventType "Disruptive"^^xsd:string ;
    ns2:hasIndustry "Public Administration"^^xsd:string ;
    ns2:hasMonth 1 ;
    ns2:hasOrganization "Rumah Principality"^^xsd:string ;
    ns2:hasYear 2014 ;
    ns2:isType_of ns2:Hacktivist,
        ns2:Message_Manipulation ;
    rdfs:comment "The Syrian Electronic Army deface 16 Saudi Arabian government websites. The targeted sites are the ones of various administrative regions."^^xsd:string .

ns2:3bbe0695e2d019f3 a ns2:HackerSecurity,
        owl:NamedIndividual ;
    ns1:associatedCampaigns ns2:Skype_s_Social_Media ;
    ns1:description "Protest"^^xsd:string ;
    ns1:isLaunchedBy ns2:Syrian_Arab_Republic ;
    ns2:behaviour ns2:Protest ;
    ns2:hasActor "Syrian Electronic Army"^^xsd:string ;
    ns2:hasActorCountry "Syrian Arab Republic"^^xsd:string ;
    ns2:hasActorType "Hacktivist"^^xsd:string ;
    ns2:hasCampaign ns2:Washington ;
    ns2:hasCountry "United States of America"^^xsd:string ;
    ns2:hasCounty "King"^^xsd:string ;
    ns2:hasEventDate "2014-01-01T00:00:00"^^xsd:dateTime ;
    ns2:hasEventSubtype "Message Manipulation"^^xsd:string ;
    ns2:hasEventType "Disruptive"^^xsd:string ;
    ns2:hasIndustry "Professional, Scientific, and Technical Services"^^xsd:string ;
    ns2:hasMonth 1 ;
    ns2:hasOrganization "Skype's Social Media"^^xsd:string ;
    ns2:hasState "Washington"^^xsd:string ;
    ns2:hasYear 2014 ;
    ns2:isType_of ns2:Hacktivist,
        ns2:Message_Manipulation ;
    rdfs:comment "The Syrian Electronic Army hacks Skype's Twitter account, Facebook page, and blog with a message against NSA surveillane."^^xsd:string .

ns2:3c1af0769c4486a4 a ns2:AccessSecurity,
        owl:NamedIndividual ;
    ns1:associatedCampaigns ns2:Service_Coordination_Inc ;
    ns2:hasActorType "Criminal"^^xsd:string ;
    ns2:hasCampaign ns2:Maryland ;
    ns2:hasCountry "United States of America"^^xsd:string ;
    ns2:hasCounty "Howard"^^xsd:string ;
    ns2:hasEventDate "2014-03-18T00:00:00"^^xsd:dateTime ;
    ns2:hasEventSubtype "Exploitation of Application Server"^^xsd:string ;
    ns2:hasEventType "Exploitive"^^xsd:string ;
    ns2:hasIndustry "Other Services (except Public Administration)"^^xsd:string ;
    ns2:hasMonth 3 ;
    ns2:hasOrganization "Service Coordination Inc."^^xsd:string ;
    ns2:hasState "Maryland"^^xsd:string ;
    ns2:hasYear 2014 ;
    ns2:isType_of ns2:Criminal,
        ns2:Exploitation_of_Application_Server ;
    rdfs:comment "Nearly 10,000 clients of Maryland-based Service Coordination Inc. (SCI) may have personal information at risk after an individual gained unauthorized access to SCI computer systems."^^xsd:string .

ns2:3c2e79c06c62e0d2 a ns2:AttackWebsite,
        owl:NamedIndividual ;
    ns1:associatedCampaigns ns2:Ankara_Chamber_of_Industry ;
    ns1:description "Protest"^^xsd:string ;
    ns1:isLaunchedBy ns2:Turkey ;
    ns2:behaviour ns2:Protest ;
    ns2:hasActor "RedHack"^^xsd:string ;
    ns2:hasActorCountry "Turkey"^^xsd:string ;
    ns2:hasActorType "Hacktivist"^^xsd:string ;
    ns2:hasCountry "Turkey"^^xsd:string ;
    ns2:hasEventDate "2014-05-30T00:00:00"^^xsd:dateTime ;
    ns2:hasEventSubtype "Message Manipulation"^^xsd:string ;
    ns2:hasEventType "Disruptive"^^xsd:string ;
    ns2:hasIndustry "Other Services (except Public Administration)"^^xsd:string ;
    ns2:hasMonth 5 ;
    ns2:hasOrganization "Ankara Chamber of Industry"^^xsd:string ;
    ns2:hasYear 2014 ;
    ns2:isType_of ns2:Hacktivist,
        ns2:Message_Manipulation ;
    rdfs:comment "The infamous group of TurkishÃÆÃ'Ãâ 'ÃÆÃ¢â¬Â 'ÃÆÃ'ÃÂ¢Ã¢'Â¬ÃÂ ''ÃÆÃ'Ãâ 'ÃÆÃ¢â¬Â ''ÃÆÃ'Ãâ ''ÃÆÃ''ÃÆ'Ã'ÃÂ hacktivists RedHack defaces the official website of theÃÆÃ'Ãâ 'ÃÆÃ¢â¬Â 'ÃÆÃ'ÃÂ¢Ã¢'Â¬ÃÂ ''ÃÆÃ'Ãâ 'ÃÆÃ¢â¬Â ''ÃÆÃ'Ãâ ''ÃÆÃ''ÃÆ'Ã'ÃÂ Ankara Chamber of Industry ASO (aso.org.tr)."^^xsd:string .

ns2:3c64ae43d699f949 a ns2:AccountAttack,
        owl:NamedIndividual ;
    ns1:associatedCampaigns ns2:Splash_Car_Wash ;
    ns1:description "Financial"^^xsd:string ;
    ns2:behaviour ns2:Financial ;
    ns2:hasActorType "Criminal"^^xsd:string ;
    ns2:hasCampaign ns2:Connecticut ;
    ns2:hasCountry "United States of America"^^xsd:string ;
    ns2:hasCounty "New Haven"^^xsd:string ;
    ns2:hasEventDate "2014-06-25T00:00:00"^^xsd:dateTime ;
    ns2:hasEventSubtype "Exploitation of Sensors"^^xsd:string ;
    ns2:hasEventType "Exploitive"^^xsd:string ;
    ns2:hasIndustry "Other Services (except Public Administration)"^^xsd:string ;
    ns2:hasMonth 6 ;
    ns2:hasOrganization "Splash Car Wash"^^xsd:string ;
    ns2:hasState "Connecticut"^^xsd:string ;
    ns2:hasYear 2014 ;
    ns2:isType_of ns2:Criminal,
        ns2:Exploitation_of_Sensors ;
    rdfs:comment "1,400 customer credit card details are stolen by hackers from Splash Car Wash exploiting a pcAnywhere vulnerability on point of sale terminals."^^xsd:string .

ns2:3c780e8ebc839c4c a ns2:AttackWebsite,
        owl:NamedIndividual ;
    ns1:associatedCampaigns ns2:Earth_Hour_Philippines ;
    ns1:isLaunchedBy ns2:Indonesia ;
    ns2:hasActor "Gantengers Crew"^^xsd:string ;
    ns2:hasActorCountry "Indonesia"^^xsd:string ;
    ns2:hasActorType "Hobbyist"^^xsd:string ;
    ns2:hasCountry "Philippines"^^xsd:string ;
    ns2:hasEventDate "2014-02-25T00:00:00"^^xsd:dateTime ;
    ns2:hasEventSubtype "Message Manipulation"^^xsd:string ;
    ns2:hasEventType "Disruptive"^^xsd:string ;
    ns2:hasIndustry "Other Services (except Public Administration)"^^xsd:string ;
    ns2:hasMonth 2 ;
    ns2:hasOrganization "Earth Hour Philippines"^^xsd:string ;
    ns2:hasYear 2014 ;
    ns2:isType_of ns2:Hobbyist,
        ns2:Message_Manipulation ;
    rdfs:comment "The official websites of World Wildlife Fund (WWF) and Earth Hour Philippines (wwwf.org.ph and earth our.wwf.org.ph) are hacked and defaced by an Indonesian based hacking group called Gantengers Crew."^^xsd:string .

ns2:3d0eaaac8d1d0128 a ns2:AccountAttack,
        owl:NamedIndividual ;
    ns1:associatedCampaigns ns2:Evernote ;
    ns2:hasActorType "Criminal"^^xsd:string ;
    ns2:hasCampaign ns2:California ;
    ns2:hasCountry "United States of America"^^xsd:string ;
    ns2:hasCounty "San Mateo"^^xsd:string ;
    ns2:hasEventDate "2014-06-16T00:00:00"^^xsd:dateTime ;
    ns2:hasEventSubtype "Exploitation of Application Server"^^xsd:string ;
    ns2:hasEventType "Exploitive"^^xsd:string ;
    ns2:hasIndustry "Information"^^xsd:string ;
    ns2:hasMonth 6 ;
    ns2:hasOrganization "Evernote"^^xsd:string ;
    ns2:hasState "California"^^xsd:string ;
    ns2:hasYear 2014 ;
    ns2:isType_of ns2:Criminal,
        ns2:Exploitation_of_Application_Server ;
    rdfs:comment "Evernote's forum site, which hosts 164,644 members, is hacked, and the company sends an email to affected members recommending they change their passwords if those credentials were reused on other sites. Compromised data includes profile data, password hashes, email addresses and birth dates."^^xsd:string .

ns2:3da288c7c840b9fc a ns2:BreachInformation,
        owl:NamedIndividual ;
    ns1:associatedCampaigns ns2:Office ;
    ns1:description "Financial"^^xsd:string ;
    ns2:behaviour ns2:Financial ;
    ns2:hasActorType "Criminal"^^xsd:string ;
    ns2:hasCountry "United Kingdom of Great Britain and Northern Ireland"^^xsd:string ;
    ns2:hasEventDate "2014-05-29T00:00:00"^^xsd:dateTime ;
    ns2:hasEventSubtype "Exploitation of Application Server"^^xsd:string ;
    ns2:hasEventType "Exploitive"^^xsd:string ;
    ns2:hasIndustry "Retail Trade"^^xsd:string ;
    ns2:hasMonth 5 ;
    ns2:hasOrganization "Office"^^xsd:string ;
    ns2:hasYear 2014 ;
    ns2:isType_of ns2:Criminal,
        ns2:Exploitation_of_Application_Server ;
    rdfs:comment "UK shoe retailer Office sends its customers an email, explaining that it has suffered a serious security breach. Information accessed includes customers' names, addresses, birth date and month (but not year), password and phone number of accounts created prior to August 2013."^^xsd:string .

ns2:3e8e90dd39c1951a a ns2:CyberattackData,
        owl:NamedIndividual ;
    ns1:associatedCampaigns ns2:Ukrainian_Election_Commission ;
    ns1:description "Sabotage"^^xsd:string ;
    ns1:isLaunchedBy ns2:Ukraine ;
    ns2:behaviour ns2:Sabotage ;
    ns2:hasActor "CyberBerkut"^^xsd:string ;
    ns2:hasActorCountry "Ukraine"^^xsd:string ;
    ns2:hasActorType "Hacktivist"^^xsd:string ;
    ns2:hasCountry "Ukraine"^^xsd:string ;
    ns2:hasEventDate "2014-05-22T00:00:00"^^xsd:dateTime ;
    ns2:hasEventSubtype "Data Attack,Message Manipulation,Exploitation of Application Server,External Denial of Service"^^xsd:string ;
    ns2:hasEventType "Mixed"^^xsd:string ;
    ns2:hasIndustry "Public Administration"^^xsd:string ;
    ns2:hasMonth 5 ;
    ns2:hasOrganization "Ukrainian Election Commission"^^xsd:string ;
    ns2:hasYear 2014 ;
    ns2:isType_of ns2:Data_Attack_Message_Manipulation_Exploit,
        ns2:Hacktivist ;
    rdfs:comment "The official website of Ukraine's election commission (cvk.gov) is targeted by a massive DDoSÃÆÃ'Ãâ 'ÃÆÃ¢â¬Â 'ÃÆÃ'ÃÂ¢Ã¢'Â¬ÃÂ ''ÃÆÃ'Ãâ 'ÃÆÃ¢â¬Â ''ÃÆÃ'Ãâ ''ÃÆÃ''ÃÆ'Ã'ÃÂ attack on the eve of country's presidential polls. The pro-Russian CyberBerkut collective claims responsibility for the attack."^^xsd:string .

ns2:3ee3df51e535a80c a ns2:CyberattackData,
        owl:NamedIndividual ;
    ns1:associatedCampaigns ns2:ARY_News ;
    ns1:description "Protest"^^xsd:string ;
    ns1:isLaunchedBy ns2:Pakistan ;
    ns2:behaviour ns2:Protest ;
    ns2:hasActor "H4$N4!N H4XOR"^^xsd:string ;
    ns2:hasActorCountry "Pakistan"^^xsd:string ;
    ns2:hasActorType "Hacktivist"^^xsd:string ;
    ns2:hasCountry "Pakistan"^^xsd:string ;
    ns2:hasEventDate "2014-05-29T00:00:00"^^xsd:dateTime ;
    ns2:hasEventSubtype "Message Manipulation"^^xsd:string ;
    ns2:hasEventType "Disruptive"^^xsd:string ;
    ns2:hasIndustry "Information"^^xsd:string ;
    ns2:hasMonth 5 ;
    ns2:hasOrganization "ARY News"^^xsd:string ;
    ns2:hasYear 2014 ;
    ns2:isType_of ns2:Hacktivist,
        ns2:Message_Manipulation ;
    rdfs:comment "The official website of Pakistan'sÃÆÃ'Ãâ 'ÃÆÃ¢â¬Â 'ÃÆÃ'ÃÂ¢Ã¢'Â¬ÃÂ ''ÃÆÃ'Ãâ 'ÃÆÃ¢â¬Â ''ÃÆÃ'Ãâ ''ÃÆÃ''ÃÆ'Ã'ÃÂ ARY News Channel website is hacked and defaced by Pakistani hacker H4$N4!N H4XOR. According to the author of the attack, \"You have been punished for broadcasting blasphemous, vulgar and Indian material\"."^^xsd:string .

ns2:3eecac2f298a7d91 a ns2:CyberattackInformation,
        owl:NamedIndividual ;
    ns1:associatedCampaigns ns2:Spec_s ;
    ns1:description "Financial"^^xsd:string ;
    ns2:behaviour ns2:Financial ;
    ns2:hasActorType "Criminal"^^xsd:string ;
    ns2:hasCampaign ns2:Texas ;
    ns2:hasCountry "United States of America"^^xsd:string ;
    ns2:hasCounty "Harris"^^xsd:string ;
    ns2:hasEventDate "2014-03-28T00:00:00"^^xsd:dateTime ;
    ns2:hasEventSubtype "Exploitation of Application Server,Exploitation of Sensors"^^xsd:string ;
    ns2:hasEventType "Exploitive"^^xsd:string ;
    ns2:hasIndustry "Retail Trade"^^xsd:string ;
    ns2:hasMonth 3 ;
    ns2:hasOrganization "Spec's"^^xsd:string ;
    ns2:hasState "Texas"^^xsd:string ;
    ns2:hasYear 2014 ;
    ns2:isType_of ns2:Criminal,
        ns2:Exploitation_of_Application_Server_Explo ;
    rdfs:comment "About 550,000 customers, as well as employees of Spec's may have had personal information compromised in a malware attack that impacted 34 locations (and dates back to Oct. 31, 2012)."^^xsd:string .

ns2:3f5470f7089fff57 a ns2:AttackerData,
        owl:NamedIndividual ;
    ns1:associatedCampaigns ns2:Frankie_Grande ;
    ns2:hasActorType "Criminal"^^xsd:string ;
    ns2:hasCountry "United States of America"^^xsd:string ;
    ns2:hasEventDate "2014-08-22T00:00:00"^^xsd:dateTime ;
    ns2:hasEventSubtype "Message Manipulation"^^xsd:string ;
    ns2:hasEventType "Disruptive"^^xsd:string ;
    ns2:hasIndustry "Other Services (except Public Administration)"^^xsd:string ;
    ns2:hasMonth 8 ;
    ns2:hasOrganization "Frankie Grande"^^xsd:string ;
    ns2:hasYear 2014 ;
    ns2:isType_of ns2:Criminal,
        ns2:Message_Manipulation ;
    rdfs:comment "The Twitter account of Ariana Grande's brother, Frankie Grande is hacked. The attacker leaves an explicit message to his sister."^^xsd:string .

ns2:412a8a2674ae04a7 a ns2:BreachInformation,
        owl:NamedIndividual ;
    ns1:associatedCampaigns ns2:Undisclosed_number_of_Delaware_restauran ;
    ns1:description "Financial"^^xsd:string ;
    ns2:behaviour ns2:Financial ;
    ns2:hasActorType "Criminal"^^xsd:string ;
    ns2:hasCampaign ns2:Delaware ;
    ns2:hasCountry "United States of America"^^xsd:string ;
    ns2:hasEventDate "2014-07-31T00:00:00"^^xsd:dateTime ;
    ns2:hasEventSubtype "Exploitation of Sensors"^^xsd:string ;
    ns2:hasEventType "Exploitive"^^xsd:string ;
    ns2:hasIndustry "Accommodation and Food Services"^^xsd:string ;
    ns2:hasMonth 7 ;
    ns2:hasOrganization "Undisclosed number of Delaware restaurants"^^xsd:string ;
    ns2:hasState "Delaware"^^xsd:string ;
    ns2:hasYear 2014 ;
    ns2:isType_of ns2:Criminal,
        ns2:Exploitation_of_Sensors ;
    rdfs:comment "An undisclosed number of Delaware restaurants may have been affected by a remote-access breach that compromised point-of-sale software,  LogMeIn, according to the Delaware Restaurant Association."^^xsd:string .

ns2:416754517c51bb5f a ns2:AttackWebsite,
        owl:NamedIndividual ;
    ns1:associatedCampaigns ns2:Alduwadimi_Principality ;
    ns1:description "Protest"^^xsd:string ;
    ns1:isLaunchedBy ns2:Syrian_Arab_Republic ;
    ns2:behaviour ns2:Protest ;
    ns2:hasActor "Syrian Electronic Army"^^xsd:string ;
    ns2:hasActorCountry "Syrian Arab Republic"^^xsd:string ;
    ns2:hasActorType "Hacktivist"^^xsd:string ;
    ns2:hasCountry "Saudi Arabia"^^xsd:string ;
    ns2:hasEventDate "2014-01-16T00:00:00"^^xsd:dateTime ;
    ns2:hasEventSubtype "Message Manipulation"^^xsd:string ;
    ns2:hasEventType "Disruptive"^^xsd:string ;
    ns2:hasIndustry "Public Administration"^^xsd:string ;
    ns2:hasMonth 1 ;
    ns2:hasOrganization "Alduwadimi Principality"^^xsd:string ;
    ns2:hasYear 2014 ;
    ns2:isType_of ns2:Hacktivist,
        ns2:Message_Manipulation ;
    rdfs:comment "The Syrian Electronic Army deface 16 Saudi Arabian government websites. The targeted sites are the ones of various administrative regions."^^xsd:string .

ns2:41d42065a1707115 a ns2:HackerSecurity,
        owl:NamedIndividual ;
    ns1:associatedCampaigns ns2:ESET_s_Spain_domain ;
    ns2:hasActor "Hmei7"^^xsd:string ;
    ns2:hasActorType "Hobbyist"^^xsd:string ;
    ns2:hasCountry "Spain"^^xsd:string ;
    ns2:hasEventDate "2014-06-04T00:00:00"^^xsd:dateTime ;
    ns2:hasEventSubtype "Message Manipulation"^^xsd:string ;
    ns2:hasEventType "Disruptive"^^xsd:string ;
    ns2:hasIndustry "Professional, Scientific, and Technical Services"^^xsd:string ;
    ns2:hasMonth 6 ;
    ns2:hasOrganization "ESET's Spain domain"^^xsd:string ;
    ns2:hasYear 2014 ;
    ns2:isType_of ns2:Hobbyist,
        ns2:Message_Manipulation ;
    rdfs:comment "A hacker called Hmeidefaces the official website of ESETand 4 of itsSpanish domains."^^xsd:string .

ns2:422fe8b3adf7e8af a ns2:CyberattackInformation,
        owl:NamedIndividual ;
    ns1:associatedCampaigns ns2:Total_Bank ;
    ns1:description "Financial"^^xsd:string ;
    ns2:behaviour ns2:Financial ;
    ns2:hasActorType "Criminal"^^xsd:string ;
    ns2:hasCampaign ns2:Florida ;
    ns2:hasCountry "United States of America"^^xsd:string ;
    ns2:hasCounty "Miami-Dade"^^xsd:string ;
    ns2:hasEventDate "2014-07-03T00:00:00"^^xsd:dateTime ;
    ns2:hasEventSubtype "Exploitation of Application Server"^^xsd:string ;
    ns2:hasEventType "Exploitive"^^xsd:string ;
    ns2:hasIndustry "Finance and Insurance"^^xsd:string ;
    ns2:hasMonth 7 ;
    ns2:hasOrganization "Total Bank"^^xsd:string ;
    ns2:hasState "Florida"^^xsd:string ;
    ns2:hasYear 2014 ;
    ns2:isType_of ns2:Criminal,
        ns2:Exploitation_of_Application_Server ;
    rdfs:comment "Total Bank notifies its users following a compromise of the institution's computer network."^^xsd:string .

ns2:423b7ea3a2ac3396 a ns2:HackerSecurity,
        owl:NamedIndividual ;
    ns1:associatedCampaigns ns2:Synology_NAS_Boxes ;
    ns1:description "Financial"^^xsd:string ;
    ns2:behaviour ns2:Financial ;
    ns2:hasActorType "Criminal"^^xsd:string ;
    ns2:hasCountry "Taiwan (Province of China)"^^xsd:string ;
    ns2:hasEventDate "2014-06-13T00:00:00"^^xsd:dateTime ;
    ns2:hasEventSubtype "Exploitation of Application Server"^^xsd:string ;
    ns2:hasEventType "Exploitive"^^xsd:string ;
    ns2:hasIndustry "Information"^^xsd:string ;
    ns2:hasMonth 6 ;
    ns2:hasOrganization "Synology NAS Boxes"^^xsd:string ;
    ns2:hasYear 2014 ;
    ns2:isType_of ns2:Criminal,
        ns2:Exploitation_of_Application_Server ;
    rdfs:comment "Dell SecureWorks reveals that unknown hackers were able to hijack Synology NAS Boxes for mining Dogecoin, reaping $620,000 in two months."^^xsd:string .

ns2:4244201130175adb a ns2:AttackInformation,
        owl:NamedIndividual ;
    ns1:associatedCampaigns ns2:International_Civil_Aviation_Organizatio ;
    ns1:description "Protest"^^xsd:string ;
    ns2:behaviour ns2:Protest ;
    ns2:hasActor "NullCrew"^^xsd:string ;
    ns2:hasActorType "Hacktivist"^^xsd:string ;
    ns2:hasCountry "Canada"^^xsd:string ;
    ns2:hasEventDate "2014-04-21T00:00:00"^^xsd:dateTime ;
    ns2:hasEventSubtype "Exploitation of Application Server"^^xsd:string ;
    ns2:hasEventType "Exploitive"^^xsd:string ;
    ns2:hasIndustry "Other Services (except Public Administration)"^^xsd:string ;
    ns2:hasMonth 4 ;
    ns2:hasOrganization "International Civil Aviation Organization"^^xsd:string ;
    ns2:hasYear 2014 ;
    ns2:isType_of ns2:Exploitation_of_Application_Server,
        ns2:Hacktivist ;
    rdfs:comment "Montreal-based ICAO (International Civil Aviation Organization) is another target in a string of attacks by NullCrew."^^xsd:string .

ns2:4368740142d043a7 a ns2:DDoS,
        owl:NamedIndividual ;
    ns1:associatedCampaigns ns2:Broadcasthe_net ;
    ns2:hasActorType "Criminal"^^xsd:string ;
    ns2:hasEventDate "2014-01-06T00:00:00"^^xsd:dateTime ;
    ns2:hasEventSubtype "External Denial of Service"^^xsd:string ;
    ns2:hasEventType "Disruptive"^^xsd:string ;
    ns2:hasIndustry "Other Services (except Public Administration)"^^xsd:string ;
    ns2:hasMonth 1 ;
    ns2:hasOrganization "Broadcasthe.net"^^xsd:string ;
    ns2:hasYear 2014 ;
    ns2:isType_of ns2:Criminal,
        ns2:External_Denial_of_Service ;
    rdfs:comment "Three of the largest private BitTorrent trackers are offline due to prolonged DDoS attacks. The targets are: What.cd, Broadcasthe.net, PassthePopcorn.me."^^xsd:string .

ns2:43ed355793dfc2cd a ns2:HackerSecurity,
        owl:NamedIndividual ;
    ns1:associatedCampaigns ns2:ESET_Security_Forum ;
    ns2:hasActor "Hmei7"^^xsd:string ;
    ns2:hasActorType "Hobbyist"^^xsd:string ;
    ns2:hasCountry "Spain"^^xsd:string ;
    ns2:hasEventDate "2014-06-04T00:00:00"^^xsd:dateTime ;
    ns2:hasEventSubtype "Message Manipulation"^^xsd:string ;
    ns2:hasEventType "Disruptive"^^xsd:string ;
    ns2:hasIndustry "Professional, Scientific, and Technical Services"^^xsd:string ;
    ns2:hasMonth 6 ;
    ns2:hasOrganization "ESET Security Forum"^^xsd:string ;
    ns2:hasYear 2014 ;
    ns2:isType_of ns2:Hobbyist,
        ns2:Message_Manipulation ;
    rdfs:comment "A hacker called Hmeidefaces the official website of ESETand 4 of itsSpanish domains."^^xsd:string .

ns2:445496fa5419875f a ns2:BreachSecurity,
        owl:NamedIndividual ;
    ns1:associatedCampaigns ns2:Dominion_Resources ;
    ns1:description "Financial"^^xsd:string ;
    ns2:behaviour ns2:Financial ;
    ns2:hasActorType "Criminal"^^xsd:string ;
    ns2:hasCampaign ns2:Virginia ;
    ns2:hasCountry "United States of America"^^xsd:string ;
    ns2:hasCounty "Richmond"^^xsd:string ;
    ns2:hasEventDate "2014-07-17T00:00:00"^^xsd:dateTime ;
    ns2:hasEventSubtype "Exploitation of Application Server"^^xsd:string ;
    ns2:hasEventType "Exploitive"^^xsd:string ;
    ns2:hasIndustry "Utilities"^^xsd:string ;
    ns2:hasMonth 7 ;
    ns2:hasOrganization "Dominion Resources"^^xsd:string ;
    ns2:hasState "Virginia"^^xsd:string ;
    ns2:hasYear 2014 ;
    ns2:isType_of ns2:Criminal,
        ns2:Exploitation_of_Application_Server ;
    rdfs:comment "About 1,700 people in the employee wellness program for Virginia-based Dominion Resources are notified that their personal information was accessed by an attacker who gained entry to the systems of a subcontractor, Onsite Health Diagnostics."^^xsd:string .

ns2:451a1317b33e6874 a ns2:CyberattackSystem,
        owl:NamedIndividual ;
    ns1:associatedCampaigns ns2:Cabinet_Ministry_of_Pakistan ;
    ns1:isLaunchedBy ns2:Pakistan ;
    ns2:hasActor "Bl@Ck Dr@GoN; Haxor T0du; Spider64"^^xsd:string ;
    ns2:hasActorCountry "Pakistan"^^xsd:string ;
    ns2:hasActorType "Hacktivist"^^xsd:string ;
    ns2:hasCountry "Pakistan"^^xsd:string ;
    ns2:hasEventDate "2014-04-25T00:00:00"^^xsd:dateTime ;
    ns2:hasEventSubtype "Message Manipulation"^^xsd:string ;
    ns2:hasEventType "Disruptive"^^xsd:string ;
    ns2:hasIndustry "Public Administration"^^xsd:string ;
    ns2:hasMonth 4 ;
    ns2:hasOrganization "Cabinet Ministry of Pakistan"^^xsd:string ;
    ns2:hasYear 2014 ;
    ns2:isType_of ns2:Hacktivist,
        ns2:Message_Manipulation ;
    rdfs:comment "The cyber battle between Indian and Pakistani hacktivists continues. In name of OpPakistan Indian hackers deface several Pakistani government websites."^^xsd:string .

ns2:458c35d71fcb8103 a ns2:AccountAttack,
        owl:NamedIndividual ;
    ns1:associatedCampaigns ns2:United_Socialist_Party_of_Venezuela ;
    ns1:description "Protest"^^xsd:string ;
    ns1:isLaunchedBy ns2:Peru ;
    ns2:behaviour ns2:Protest ;
    ns2:hasActor "LulzSec (Peru)"^^xsd:string ;
    ns2:hasActorCountry "Peru"^^xsd:string ;
    ns2:hasActorType "Hacktivist"^^xsd:string ;
    ns2:hasCountry "Venezuela (Bolivarian Republic of)"^^xsd:string ;
    ns2:hasEventDate "2014-02-15T00:00:00"^^xsd:dateTime ;
    ns2:hasEventSubtype "Message Manipulation"^^xsd:string ;
    ns2:hasEventType "Disruptive"^^xsd:string ;
    ns2:hasIndustry "Other Services (except Public Administration)"^^xsd:string ;
    ns2:hasMonth 2 ;
    ns2:hasOrganization "United Socialist Party of Venezuela"^^xsd:string ;
    ns2:hasYear 2014 ;
    ns2:isType_of ns2:Hacktivist,
        ns2:Message_Manipulation ;
    rdfs:comment "The verified Twitter account (@PartidoPSUV) of the United Socialist Party of Venezuela (PSUV) is hacked by LulzSec Peru."^^xsd:string .

ns2:459733780ce77e35 a ns2:Malware,
        owl:NamedIndividual ;
    ns1:associatedCampaigns ns2:Department_of_Agriculture ;
    ns1:description "Financial"^^xsd:string ;
    ns2:behaviour ns2:Financial ;
    ns2:hasActorType "Criminal"^^xsd:string ;
    ns2:hasCountry "Philippines"^^xsd:string ;
    ns2:hasEventDate "2014-07-25T00:00:00"^^xsd:dateTime ;
    ns2:hasEventSubtype "Message Manipulation"^^xsd:string ;
    ns2:hasEventType "Disruptive"^^xsd:string ;
    ns2:hasIndustry "Public Administration"^^xsd:string ;
    ns2:hasMonth 7 ;
    ns2:hasOrganization "Department of Agriculture"^^xsd:string ;
    ns2:hasYear 2014 ;
    ns2:isType_of ns2:Criminal,
        ns2:Message_Manipulation ;
    rdfs:comment "The official website of Philippine Department of Agriculture (da.gov.ph) is infected with malicious code that promotes a gambling-related website."^^xsd:string .

ns2:459a5d1860e1c7b3 a ns2:AttackWebsite,
        owl:NamedIndividual ;
    ns1:associatedCampaigns ns2:Bangalore_City_Police ;
    ns1:description "Protest"^^xsd:string ;
    ns1:isLaunchedBy ns2:India ;
    ns2:behaviour ns2:Protest ;
    ns2:hasActor "H4x0r10ux m1nd"^^xsd:string ;
    ns2:hasActorCountry "India"^^xsd:string ;
    ns2:hasActorType "Hacktivist"^^xsd:string ;
    ns2:hasCountry "India"^^xsd:string ;
    ns2:hasEventDate "2014-04-20T00:00:00"^^xsd:dateTime ;
    ns2:hasEventSubtype "Message Manipulation"^^xsd:string ;
    ns2:hasEventType "Disruptive"^^xsd:string ;
    ns2:hasIndustry "Public Administration"^^xsd:string ;
    ns2:hasMonth 4 ;
    ns2:hasOrganization "Bangalore City Police"^^xsd:string ;
    ns2:hasYear 2014 ;
    ns2:isType_of ns2:Hacktivist,
        ns2:Message_Manipulation ;
    rdfs:comment "A Pakistani hacker going with the handle of H4x0r10ux m1nd defaces the official website of Bangalore City Police India (bcp.gov.in)."^^xsd:string .

ns2:467a1b3ddb73cd29 a ns2:AttackWebsite,
        owl:NamedIndividual ;
    ns1:associatedCampaigns ns2:Huraymila_Principality ;
    ns1:description "Protest"^^xsd:string ;
    ns1:isLaunchedBy ns2:Syrian_Arab_Republic ;
    ns2:behaviour ns2:Protest ;
    ns2:hasActor "Syrian Electronic Army"^^xsd:string ;
    ns2:hasActorCountry "Syrian Arab Republic"^^xsd:string ;
    ns2:hasActorType "Hacktivist"^^xsd:string ;
    ns2:hasCountry "Saudi Arabia"^^xsd:string ;
    ns2:hasEventDate "2014-01-16T00:00:00"^^xsd:dateTime ;
    ns2:hasEventSubtype "Message Manipulation"^^xsd:string ;
    ns2:hasEventType "Disruptive"^^xsd:string ;
    ns2:hasIndustry "Public Administration"^^xsd:string ;
    ns2:hasMonth 1 ;
    ns2:hasOrganization "Huraymila Principality"^^xsd:string ;
    ns2:hasYear 2014 ;
    ns2:isType_of ns2:Hacktivist,
        ns2:Message_Manipulation ;
    rdfs:comment "The Syrian Electronic Army deface 16 Saudi Arabian government websites. The targeted sites are the ones of various administrative regions."^^xsd:string .

ns2:49aab2197cbb5f4a a ns2:HackerSecurity,
        owl:NamedIndividual ;
    ns1:associatedCampaigns ns2:National_Portal_of_India ;
    ns1:description "Protest"^^xsd:string ;
    ns2:behaviour ns2:Protest ;
    ns2:hasActor "Zcompany Hacking Crew"^^xsd:string ;
    ns2:hasActorType "Hacktivist"^^xsd:string ;
    ns2:hasCountry "India"^^xsd:string ;
    ns2:hasEventDate "2014-02-19T00:00:00"^^xsd:dateTime ;
    ns2:hasEventSubtype "Message Manipulation"^^xsd:string ;
    ns2:hasEventType "Disruptive"^^xsd:string ;
    ns2:hasIndustry "Public Administration"^^xsd:string ;
    ns2:hasMonth 2 ;
    ns2:hasOrganization "National Portal of India"^^xsd:string ;
    ns2:hasYear 2014 ;
    ns2:isType_of ns2:Hacktivist,
        ns2:Message_Manipulation ;
    rdfs:comment "Hackers of ZCompany Hacking Crew (ZHC) hack india.gov.in, the National Portal of India, posting a message in favor of Kashmir."^^xsd:string .

ns2:49f1240bd478eda3 a ns2:AttackWebsite,
        owl:NamedIndividual ;
    ns1:associatedCampaigns ns2:Alikhbaria ;
    ns1:isLaunchedBy ns2:Saudi_Arabia ;
    ns2:hasActor "Mr.Rocky; Mr.Slyman"^^xsd:string ;
    ns2:hasActorCountry "Saudi Arabia"^^xsd:string ;
    ns2:hasActorType "Hacktivist"^^xsd:string ;
    ns2:hasCountry "Saudi Arabia"^^xsd:string ;
    ns2:hasEventDate "2014-08-15T00:00:00"^^xsd:dateTime ;
    ns2:hasEventSubtype "Message Manipulation,Exploitation of Application Server"^^xsd:string ;
    ns2:hasEventType "Mixed"^^xsd:string ;
    ns2:hasIndustry "Information"^^xsd:string ;
    ns2:hasMonth 8 ;
    ns2:hasOrganization "Alikhbaria"^^xsd:string ;
    ns2:hasYear 2014 ;
    ns2:isType_of ns2:Hacktivist,
        ns2:Message_Manipulation_Exploitation_of_App ;
    rdfs:comment "Two Libyan hackers going with the handle of Mr.Rocky and Mr. Slyman deface the official website of Saudi government-owned satellite news TV channel Alikhbaria (ekhbariyatv.sa) and also steal the database of the website."^^xsd:string .

ns2:4b3a4d10393d9068 a ns2:AttackWebsite,
        owl:NamedIndividual ;
    ns1:associatedCampaigns ns2:Stanford_University ;
    ns2:hasActor "Sahoo"^^xsd:string ;
    ns2:hasActorType "Hobbyist"^^xsd:string ;
    ns2:hasCampaign ns2:California ;
    ns2:hasCountry "United States of America"^^xsd:string ;
    ns2:hasCounty "Santa Clara"^^xsd:string ;
    ns2:hasEventDate "2014-08-28T00:00:00"^^xsd:dateTime ;
    ns2:hasEventSubtype "Message Manipulation"^^xsd:string ;
    ns2:hasEventType "Disruptive"^^xsd:string ;
    ns2:hasIndustry "Educational Services"^^xsd:string ;
    ns2:hasMonth 8 ;
    ns2:hasOrganization "Stanford University"^^xsd:string ;
    ns2:hasState "California"^^xsd:string ;
    ns2:hasYear 2014 ;
    ns2:isType_of ns2:Hobbyist,
        ns2:Message_Manipulation ;
    rdfs:comment "Sahoo defaces a subdomain of Stanford (web.stanford.edu)."^^xsd:string .

ns2:4bdd8d3d458f2cba a ns2:AttackWebsite,
        owl:NamedIndividual ;
    ns1:associatedCampaigns ns2:maidansupport_com ;
    ns2:hasActorType "Criminal"^^xsd:string ;
    ns2:hasCountry "Ukraine"^^xsd:string ;
    ns2:hasEventDate "2014-02-28T00:00:00"^^xsd:dateTime ;
    ns2:hasEventSubtype "External Denial of Service"^^xsd:string ;
    ns2:hasEventType "Disruptive"^^xsd:string ;
    ns2:hasIndustry "Other Services (except Public Administration)"^^xsd:string ;
    ns2:hasMonth 2 ;
    ns2:hasOrganization "maidansupport.com"^^xsd:string ;
    ns2:hasYear 2014 ;
    ns2:isType_of ns2:Criminal,
        ns2:External_Denial_of_Service ;
    rdfs:comment "Hacktivists continue to launch attacks against Ukrainian government websites. The latest targets are the sites of the parliament, or the Verkhovna Rada (rada.gov.ua), the Right Sector nationalist movement (banderivets.org.ua), but also some Euromaidan websites."^^xsd:string .

ns2:4c3b1506a788132b a ns2:AttackWebsite,
        owl:NamedIndividual ;
    ns1:associatedCampaigns ns2:Linkin_Park ;
    ns2:hasActorType "Criminal"^^xsd:string ;
    ns2:hasCountry "United States of America"^^xsd:string ;
    ns2:hasEventDate "2014-06-02T00:00:00"^^xsd:dateTime ;
    ns2:hasEventSubtype "Message Manipulation"^^xsd:string ;
    ns2:hasEventType "Disruptive"^^xsd:string ;
    ns2:hasIndustry "Arts, Entertainment, and Recreation"^^xsd:string ;
    ns2:hasMonth 6 ;
    ns2:hasOrganization "Linkin Park"^^xsd:string ;
    ns2:hasYear 2014 ;
    ns2:isType_of ns2:Criminal,
        ns2:Message_Manipulation ;
    rdfs:comment "The official Facebook fan page of the famous rock band Linkin Park (63M fans) is hacked by an unknown hacker and starts spamming vulgar images with links."^^xsd:string .

ns2:4d8cb0dca9697948 a ns2:CyberattackInformation,
        owl:NamedIndividual ;
    ns1:associatedCampaigns ns2:UPS ;
    ns1:description "Financial"^^xsd:string ;
    ns2:behaviour ns2:Financial ;
    ns2:hasActorType "Criminal"^^xsd:string ;
    ns2:hasCountry "United States of America"^^xsd:string ;
    ns2:hasEventDate "2014-08-20T00:00:00"^^xsd:dateTime ;
    ns2:hasEventSubtype "Exploitation of Sensors"^^xsd:string ;
    ns2:hasEventType "Exploitive"^^xsd:string ;
    ns2:hasMonth 8 ;
    ns2:hasOrganization "UPS"^^xsd:string ;
    ns2:hasYear 2014 ;
    ns2:isType_of ns2:Criminal,
        ns2:Exploitation_of_Sensors ;
    rdfs:comment "UPS admits that 51 of its franchised stores were hit with a malware attack that put customer credit and debit card data at risk from January 20 to August 11."^^xsd:string .

ns2:4df21ba269bb4fc9 a ns2:AttackWebsite,
        owl:NamedIndividual ;
    ns1:associatedCampaigns ns2:Alquwayiyah_Principality ;
    ns1:description "Protest"^^xsd:string ;
    ns1:isLaunchedBy ns2:Syrian_Arab_Republic ;
    ns2:behaviour ns2:Protest ;
    ns2:hasActor "Syrian Electronic Army"^^xsd:string ;
    ns2:hasActorCountry "Syrian Arab Republic"^^xsd:string ;
    ns2:hasActorType "Hacktivist"^^xsd:string ;
    ns2:hasCountry "Saudi Arabia"^^xsd:string ;
    ns2:hasEventDate "2014-01-16T00:00:00"^^xsd:dateTime ;
    ns2:hasEventSubtype "Message Manipulation"^^xsd:string ;
    ns2:hasEventType "Disruptive"^^xsd:string ;
    ns2:hasIndustry "Public Administration"^^xsd:string ;
    ns2:hasMonth 1 ;
    ns2:hasOrganization "Alquwayiyah Principality"^^xsd:string ;
    ns2:hasYear 2014 ;
    ns2:isType_of ns2:Hacktivist,
        ns2:Message_Manipulation ;
    rdfs:comment "The Syrian Electronic Army deface 16 Saudi Arabian government websites. The targeted sites are the ones of various administrative regions."^^xsd:string .

ns2:4e716ff4458c6f9e a ns2:DDoS,
        owl:NamedIndividual ;
    ns1:associatedCampaigns ns2:Feedly ;
    ns1:description "Financial"^^xsd:string ;
    ns2:behaviour ns2:Financial ;
    ns2:hasActorType "Criminal"^^xsd:string ;
    ns2:hasCampaign ns2:California ;
    ns2:hasCountry "United States of America"^^xsd:string ;
    ns2:hasCounty "Santa Clara"^^xsd:string ;
    ns2:hasEventDate "2014-06-11T00:00:00"^^xsd:dateTime ;
    ns2:hasEventSubtype "External Denial of Service"^^xsd:string ;
    ns2:hasEventType "Disruptive"^^xsd:string ;
    ns2:hasIndustry "Information"^^xsd:string ;
    ns2:hasMonth 6 ;
    ns2:hasOrganization "Feedly"^^xsd:string ;
    ns2:hasState "California"^^xsd:string ;
    ns2:hasYear 2014 ;
    ns2:isType_of ns2:Criminal,
        ns2:External_Denial_of_Service ;
    rdfs:comment "News aggregator Feedly is made inaccessible by a DDoS attack. Attackers demand a ransom to stop their crippling assault, which the company refuses to pay."^^xsd:string .

ns2:4f99aa333554a365 a ns2:BreachInformation,
        owl:NamedIndividual ;
    ns1:associatedCampaigns ns2:Children_s_Mercy_Hospital ;
    ns2:hasActorType "Criminal"^^xsd:string ;
    ns2:hasCampaign ns2:Missouri ;
    ns2:hasCountry "United States of America"^^xsd:string ;
    ns2:hasCounty "Jackson"^^xsd:string ;
    ns2:hasEventDate "2014-08-19T00:00:00"^^xsd:dateTime ;
    ns2:hasEventSubtype "Exploitation of Application Server"^^xsd:string ;
    ns2:hasEventType "Exploitive"^^xsd:string ;
    ns2:hasIndustry "Health Care and Social Assistance"^^xsd:string ;
    ns2:hasMonth 8 ;
    ns2:hasOrganization "Children's Mercy Hospital"^^xsd:string ;
    ns2:hasState "Missouri"^^xsd:string ;
    ns2:hasYear 2014 ;
    ns2:isType_of ns2:Criminal,
        ns2:Exploitation_of_Application_Server ;
    rdfs:comment "Children's Mercy Hospital in Kansas City notifies 4,076 individuals that Onsite Health Diagnostics, a vendor used by wellness program provider StayWell Health Management, experienced a breach that affected their personal information."^^xsd:string .

ns2:4fe7dcb63e455044 a ns2:AttackWebsite,
        owl:NamedIndividual ;
    ns1:associatedCampaigns ns2:Alohtah_Principality ;
    ns1:description "Protest"^^xsd:string ;
    ns1:isLaunchedBy ns2:Syrian_Arab_Republic ;
    ns2:behaviour ns2:Protest ;
    ns2:hasActor "Syrian Electronic Army"^^xsd:string ;
    ns2:hasActorCountry "Syrian Arab Republic"^^xsd:string ;
    ns2:hasActorType "Hacktivist"^^xsd:string ;
    ns2:hasCountry "Saudi Arabia"^^xsd:string ;
    ns2:hasEventDate "2014-01-16T00:00:00"^^xsd:dateTime ;
    ns2:hasEventSubtype "Message Manipulation"^^xsd:string ;
    ns2:hasEventType "Disruptive"^^xsd:string ;
    ns2:hasIndustry "Public Administration"^^xsd:string ;
    ns2:hasMonth 1 ;
    ns2:hasOrganization "Alohtah Principality"^^xsd:string ;
    ns2:hasYear 2014 ;
    ns2:isType_of ns2:Hacktivist,
        ns2:Message_Manipulation ;
    rdfs:comment "The Syrian Electronic Army deface 16 Saudi Arabian government websites. The targeted sites are the ones of various administrative regions."^^xsd:string .

ns2:50036e5047d8cf10 a ns2:AccountAttack,
        owl:NamedIndividual ;
    ns1:associatedCampaigns ns2:El_Agave_Restaurant ;
    ns1:description "Financial"^^xsd:string ;
    ns2:behaviour ns2:Financial ;
    ns2:hasActorType "Criminal"^^xsd:string ;
    ns2:hasCampaign ns2:Minnesota ;
    ns2:hasCountry "United States of America"^^xsd:string ;
    ns2:hasCounty "Martin"^^xsd:string ;
    ns2:hasEventDate "2014-03-26T00:00:00"^^xsd:dateTime ;
    ns2:hasEventSubtype "Exploitation of Sensors"^^xsd:string ;
    ns2:hasEventType "Exploitive"^^xsd:string ;
    ns2:hasIndustry "Accommodation and Food Services"^^xsd:string ;
    ns2:hasMonth 3 ;
    ns2:hasOrganization "El Agave Restaurant"^^xsd:string ;
    ns2:hasState "Minnesota"^^xsd:string ;
    ns2:hasYear 2014 ;
    ns2:isType_of ns2:Criminal,
        ns2:Exploitation_of_Sensors ;
    rdfs:comment "Over 200 credit and debit card numbers stolen by hackers who installed malware on the point of sale system of El Agave Restaurant."^^xsd:string .

ns2:5024c0539c5753d0 a ns2:CyberattackData,
        owl:NamedIndividual ;
    ns1:associatedCampaigns ns2:Autonation ;
    ns1:description "Financial"^^xsd:string ;
    ns2:behaviour ns2:Financial ;
    ns2:hasActorType "Criminal"^^xsd:string ;
    ns2:hasCampaign ns2:Florida ;
    ns2:hasCountry "United States of America"^^xsd:string ;
    ns2:hasCounty "Broward"^^xsd:string ;
    ns2:hasEventDate "2014-06-05T00:00:00"^^xsd:dateTime ;
    ns2:hasEventSubtype "Exploitation of Application Server"^^xsd:string ;
    ns2:hasEventType "Exploitive"^^xsd:string ;
    ns2:hasIndustry "Retail Trade"^^xsd:string ;
    ns2:hasMonth 6 ;
    ns2:hasOrganization "Autonation"^^xsd:string ;
    ns2:hasState "Florida"^^xsd:string ;
    ns2:hasYear 2014 ;
    ns2:isType_of ns2:Criminal,
        ns2:Exploitation_of_Application_Server ;
    rdfs:comment "National automobile retailer AutoNation notifies an undisclosed number of customers that their payment card data, as well as other information, may have been captured by hackers that compromised AutoNation websites hosted and operated by TradeMotion."^^xsd:string .

ns2:5121a023efc8f42f a ns2:BreachInformation,
        owl:NamedIndividual ;
    ns1:associatedCampaigns ns2:Kate_Upton ;
    ns1:description "Personal Attack"^^xsd:string ;
    ns2:behaviour ns2:Personal_Attack ;
    ns2:hasActorType "Criminal"^^xsd:string ;
    ns2:hasCountry "United States of America"^^xsd:string ;
    ns2:hasEventDate "2014-08-31T00:00:00"^^xsd:dateTime ;
    ns2:hasEventSubtype "Exploitation of Application Server"^^xsd:string ;
    ns2:hasEventType "Exploitive"^^xsd:string ;
    ns2:hasIndustry "Other Services (except Public Administration)"^^xsd:string ;
    ns2:hasMonth 8 ;
    ns2:hasOrganization "Kate Upton"^^xsd:string ;
    ns2:hasYear 2014 ;
    ns2:isType_of ns2:Criminal,
        ns2:Exploitation_of_Application_Server ;
    rdfs:comment "Yet another leak of celebrities pictures. A massive leak of nude and risque photos appearing to be of huge stars like is leaked online, first appearing on 4chan."^^xsd:string .

ns2:51d2d381b04a8917 a ns2:AttackWebsite,
        owl:NamedIndividual ;
    ns1:associatedCampaigns ns2:Artsakh_State_University ;
    ns1:description "Protest"^^xsd:string ;
    ns1:isLaunchedBy ns2:Azerbaijan ;
    ns2:behaviour ns2:Protest ;
    ns2:hasActor "Anti-Armenia Team"^^xsd:string ;
    ns2:hasActorCountry "Azerbaijan"^^xsd:string ;
    ns2:hasActorType "Hacktivist"^^xsd:string ;
    ns2:hasCountry "Armenia"^^xsd:string ;
    ns2:hasEventDate "2014-01-23T00:00:00"^^xsd:dateTime ;
    ns2:hasEventSubtype "Message Manipulation"^^xsd:string ;
    ns2:hasEventType "Disruptive"^^xsd:string ;
    ns2:hasIndustry "Educational Services"^^xsd:string ;
    ns2:hasMonth 1 ;
    ns2:hasOrganization "Artsakh State University"^^xsd:string ;
    ns2:hasYear 2014 ;
    ns2:isType_of ns2:Hacktivist,
        ns2:Message_Manipulation ;
    rdfs:comment "Azerbaijan Hackers from Anti-Armenia Team have hacked and defaced several Armenian government ministries websites."^^xsd:string .

ns2:51de7a6f8a84858e a ns2:HackerSecurity,
        owl:NamedIndividual ;
    ns1:associatedCampaigns ns2:Privatbank ;
    ns1:description "Protest"^^xsd:string ;
    ns1:isLaunchedBy ns2:Ukraine ;
    ns2:behaviour ns2:Protest ;
    ns2:hasActor "Green Dragon Crew"^^xsd:string ;
    ns2:hasActorCountry "Ukraine"^^xsd:string ;
    ns2:hasActorType "Hacktivist"^^xsd:string ;
    ns2:hasCountry "Ukraine"^^xsd:string ;
    ns2:hasEventDate "2014-06-30T00:00:00"^^xsd:dateTime ;
    ns2:hasEventSubtype "External Denial of Service"^^xsd:string ;
    ns2:hasEventType "Disruptive"^^xsd:string ;
    ns2:hasIndustry "Finance and Insurance"^^xsd:string ;
    ns2:hasMonth 6 ;
    ns2:hasOrganization "Privatbank"^^xsd:string ;
    ns2:hasYear 2014 ;
    ns2:isType_of ns2:External_Denial_of_Service,
        ns2:Hacktivist ;
    rdfs:comment "Hackers from the Green Dragon Crew hack Privatbank, the bank owned by Ukrainian businessman Ihor Kolomoyskyi."^^xsd:string .

ns2:51f8acaedf45bbd1 a ns2:DDoS,
        owl:NamedIndividual ;
    ns1:associatedCampaigns ns2:Bitstamp ;
    ns2:hasActorType "Criminal"^^xsd:string ;
    ns2:hasCountry "United Kingdom of Great Britain and Northern Ireland"^^xsd:string ;
    ns2:hasEventDate "2014-02-12T00:00:00"^^xsd:dateTime ;
    ns2:hasEventSubtype "External Denial of Service"^^xsd:string ;
    ns2:hasEventType "Disruptive"^^xsd:string ;
    ns2:hasIndustry "Finance and Insurance"^^xsd:string ;
    ns2:hasMonth 2 ;
    ns2:hasOrganization "Bitstamp"^^xsd:string ;
    ns2:hasYear 2014 ;
    ns2:isType_of ns2:Criminal,
        ns2:External_Denial_of_Service ;
    rdfs:comment "Bitcoin exchange service Bitstamp suspends withdrawals while dealing with a denial-of-service (DOS) attack."^^xsd:string .

ns2:52017707785c4332 a ns2:AttackWebsite,
        owl:NamedIndividual ;
    ns1:associatedCampaigns ns2:Kali ;
    ns1:isLaunchedBy ns2:Libya ;
    ns2:hasActor "The GreaT Team"^^xsd:string ;
    ns2:hasActorCountry "Libya"^^xsd:string ;
    ns2:hasActorType "Hobbyist"^^xsd:string ;
    ns2:hasCountry "United States of America"^^xsd:string ;
    ns2:hasEventDate "2014-04-30T00:00:00"^^xsd:dateTime ;
    ns2:hasEventSubtype "Message Manipulation"^^xsd:string ;
    ns2:hasEventType "Disruptive"^^xsd:string ;
    ns2:hasIndustry "Other Services (except Public Administration)"^^xsd:string ;
    ns2:hasMonth 4 ;
    ns2:hasOrganization "Kali"^^xsd:string ;
    ns2:hasYear 2014 ;
    ns2:isType_of ns2:Hobbyist,
        ns2:Message_Manipulation ;
    rdfs:comment "A Libyan Hackers group called \"The GreaT Team\"ÃÆÃ'Ãâ 'ÃÆÃ¢â¬Â 'ÃÆÃ'ÃÂ¢Ã¢'Â¬ÃÂ ''ÃÆÃ'Ãâ 'ÃÆÃ¢â¬Â ''ÃÆÃ'Ãâ ''ÃÆÃ''ÃÆ'Ã'ÃÂ (TGT) defaces the mailing list subdomain of Kali website (lists.kali.org)."^^xsd:string .

ns2:52572d7717648805 a ns2:AttackWebsite,
        owl:NamedIndividual ;
    ns1:associatedCampaigns ns2:Various_Government_Websites ;
    ns1:description "Protest"^^xsd:string ;
    ns1:isLaunchedBy ns2:China ;
    ns2:behaviour ns2:Protest ;
    ns2:hasActor "Paw Security"^^xsd:string ;
    ns2:hasActorCountry "China"^^xsd:string ;
    ns2:hasActorType "Hacktivist"^^xsd:string ;
    ns2:hasCountry "China"^^xsd:string ;
    ns2:hasEventDate "2014-08-07T00:00:00"^^xsd:dateTime ;
    ns2:hasEventSubtype "External Denial of Service"^^xsd:string ;
    ns2:hasEventType "Disruptive"^^xsd:string ;
    ns2:hasIndustry "Public Administration"^^xsd:string ;
    ns2:hasMonth 8 ;
    ns2:hasOrganization "Various Government Websites"^^xsd:string ;
    ns2:hasYear 2014 ;
    ns2:isType_of ns2:External_Denial_of_Service,
        ns2:Hacktivist ;
    rdfs:comment "In name of #OpNoHunt, a collective called Paw Security takes down several Chinese websites to protest against violences on pets."^^xsd:string .

ns2:529074d2ef362542 a ns2:CyberattackData,
        owl:NamedIndividual ;
    ns1:associatedCampaigns ns2:Israeli_Channel_10 ;
    ns1:description "Protest"^^xsd:string ;
    ns1:isLaunchedBy ns2:Israel ;
    ns2:behaviour ns2:Protest ;
    ns2:hasActor "Al-Qassam Brigades"^^xsd:string ;
    ns2:hasActorCountry "Israel"^^xsd:string ;
    ns2:hasActorType "Hacktivist"^^xsd:string ;
    ns2:hasCountry "Israel"^^xsd:string ;
    ns2:hasEventDate "2014-07-17T00:00:00"^^xsd:dateTime ;
    ns2:hasEventSubtype "Message Manipulation"^^xsd:string ;
    ns2:hasEventType "Disruptive"^^xsd:string ;
    ns2:hasIndustry "Information"^^xsd:string ;
    ns2:hasMonth 7 ;
    ns2:hasOrganization "Israeli Channel 10"^^xsd:string ;
    ns2:hasYear 2014 ;
    ns2:isType_of ns2:Hacktivist,
        ns2:Message_Manipulation ;
    rdfs:comment "Al-Qassam Brigades claim responsibility for the hack of the satellite feed of Israeli-based Channel 10 for a few minutes to broadcast images of wounded civilians and propaganda messages directed at Israeli citizens."^^xsd:string .

ns2:5294ae50e79c6008 a ns2:AccountAttack,
        owl:NamedIndividual ;
    ns1:associatedCampaigns ns2:Give_Me_Coins ;
    ns1:description "Financial"^^xsd:string ;
    ns2:behaviour ns2:Financial ;
    ns2:hasActorType "Criminal"^^xsd:string ;
    ns2:hasEventDate "2014-01-23T00:00:00"^^xsd:dateTime ;
    ns2:hasEventSubtype "Exploitation of Application Server"^^xsd:string ;
    ns2:hasEventType "Exploitive"^^xsd:string ;
    ns2:hasIndustry "Finance and Insurance"^^xsd:string ;
    ns2:hasMonth 1 ;
    ns2:hasOrganization "Give Me Coins"^^xsd:string ;
    ns2:hasYear 2014 ;
    ns2:isType_of ns2:Criminal,
        ns2:Exploitation_of_Application_Server ;
    rdfs:comment "The popular Litecoin mining pool Give Me Coins (give-me-coins.com) is hacked. The attackers have reportedly stolen a total of 10,000 Litecoins, currently worth around $230,000."^^xsd:string .

ns2:55036966af31ae1a a ns2:BreachData,
        owl:NamedIndividual ;
    ns1:associatedCampaigns ns2:University_of_Maryland__College_Park ;
    ns1:description "Financial"^^xsd:string ;
    ns2:behaviour ns2:Financial ;
    ns2:hasActorType "Criminal"^^xsd:string ;
    ns2:hasCampaign ns2:Maryland ;
    ns2:hasCountry "United States of America"^^xsd:string ;
    ns2:hasCounty "Prince George's"^^xsd:string ;
    ns2:hasEventDate "2014-02-19T00:00:00"^^xsd:dateTime ;
    ns2:hasEventSubtype "Exploitation of Application Server"^^xsd:string ;
    ns2:hasEventType "Exploitive"^^xsd:string ;
    ns2:hasIndustry "Educational Services"^^xsd:string ;
    ns2:hasMonth 2 ;
    ns2:hasOrganization "University of Maryland, College Park"^^xsd:string ;
    ns2:hasState "Maryland"^^xsd:string ;
    ns2:hasYear 2014 ;
    ns2:isType_of ns2:Criminal,
        ns2:Exploitation_of_Application_Server ;
    rdfs:comment "The University of Maryland announces that a database containing 309,079 records of faculty, staff, students and affiliated personnel from the College Park and Shady Grove campuses has been breached."^^xsd:string .

ns2:570212f0cab7b641 a ns2:CyberattackData,
        owl:NamedIndividual ;
    ns1:associatedCampaigns ns2:Valley_View_Hospital ;
    ns1:description "Financial"^^xsd:string ;
    ns2:behaviour ns2:Financial ;
    ns2:hasActorType "Criminal"^^xsd:string ;
    ns2:hasCampaign ns2:Colorado ;
    ns2:hasCountry "United States of America"^^xsd:string ;
    ns2:hasCounty "Garfield"^^xsd:string ;
    ns2:hasEventDate "2014-03-17T00:00:00"^^xsd:dateTime ;
    ns2:hasEventSubtype "Exploitation of End Hosts"^^xsd:string ;
    ns2:hasEventType "Exploitive"^^xsd:string ;
    ns2:hasIndustry "Health Care and Social Assistance"^^xsd:string ;
    ns2:hasMonth 3 ;
    ns2:hasOrganization "Valley View Hospital"^^xsd:string ;
    ns2:hasState "Colorado"^^xsd:string ;
    ns2:hasYear 2014 ;
    ns2:isType_of ns2:Criminal,
        ns2:Exploitation_of_End_Hosts ;
    rdfs:comment "Social Security numbers and payment card data is among the personal information that may have been compromised for about 5,400 patients of Colorado-based Valley View Hospital after a computer virus was identified on some hospital computers."^^xsd:string .

ns2:57e9e8ab5fcd632e a ns2:AccessSecurity,
        owl:NamedIndividual ;
    ns1:associatedCampaigns ns2:Assisted_Living_Concepts ;
    ns1:description "Financial"^^xsd:string ;
    ns2:behaviour ns2:Financial ;
    ns2:hasActorType "Criminal"^^xsd:string ;
    ns2:hasCampaign ns2:Wisconsin ;
    ns2:hasCountry "United States of America"^^xsd:string ;
    ns2:hasCounty "Waukesha"^^xsd:string ;
    ns2:hasEventDate "2014-03-05T00:00:00"^^xsd:dateTime ;
    ns2:hasEventSubtype "Exploitation of Application Server"^^xsd:string ;
    ns2:hasEventType "Exploitive"^^xsd:string ;
    ns2:hasIndustry "Health Care and Social Assistance"^^xsd:string ;
    ns2:hasMonth 3 ;
    ns2:hasOrganization "Assisted Living Concepts"^^xsd:string ;
    ns2:hasState "Wisconsin"^^xsd:string ;
    ns2:hasYear 2014 ;
    ns2:isType_of ns2:Criminal,
        ns2:Exploitation_of_Application_Server ;
    rdfs:comment "Assisted Living Concepts notifies approximately 43,600 current and former employees that their personal information may have been exposed after an unauthorised access."^^xsd:string .

ns2:595d817ab9815f5d a ns2:AccountAttack,
        owl:NamedIndividual ;
    ns1:associatedCampaigns ns2:CoinEX_pw ;
    ns1:description "Financial"^^xsd:string ;
    ns2:behaviour ns2:Financial ;
    ns2:hasActorType "Criminal"^^xsd:string ;
    ns2:hasCountry "Palau"^^xsd:string ;
    ns2:hasEventDate "2014-03-19T00:00:00"^^xsd:dateTime ;
    ns2:hasEventSubtype "Exploitation of Application Server"^^xsd:string ;
    ns2:hasEventType "Exploitive"^^xsd:string ;
    ns2:hasIndustry "Finance and Insurance"^^xsd:string ;
    ns2:hasMonth 3 ;
    ns2:hasOrganization "CoinEX.pw"^^xsd:string ;
    ns2:hasYear 2014 ;
    ns2:isType_of ns2:Criminal,
        ns2:Exploitation_of_Application_Server ;
    rdfs:comment "CoinEX.pw confirms it recently suffered a hack resulting in the theft of all the bitcoins in its possession."^^xsd:string .

ns2:5a1d936e8a52541e a ns2:AccountAttack,
        owl:NamedIndividual ;
    ns1:associatedCampaigns ns2:JPMorgan ;
    ns1:description "Financial"^^xsd:string ;
    ns2:behaviour ns2:Financial ;
    ns2:hasActorType "Criminal"^^xsd:string ;
    ns2:hasCampaign ns2:New_York ;
    ns2:hasCountry "United States of America"^^xsd:string ;
    ns2:hasCounty "New York"^^xsd:string ;
    ns2:hasEventDate "2014-08-27T00:00:00"^^xsd:dateTime ;
    ns2:hasEventSubtype "Exploitation of Application Server"^^xsd:string ;
    ns2:hasEventType "Exploitive"^^xsd:string ;
    ns2:hasIndustry "Finance and Insurance"^^xsd:string ;
    ns2:hasMonth 8 ;
    ns2:hasOrganization "JPMorgan"^^xsd:string ;
    ns2:hasState "New York"^^xsd:string ;
    ns2:hasYear 2014 ;
    ns2:isType_of ns2:Criminal,
        ns2:Exploitation_of_Application_Server ;
    rdfs:comment "Bloomberg news reveals that hackers allegedly from Russia targeted JPMorgan Chase & Co. (JPM) and at least four other banks in a coordinated attack on major financial institutions."^^xsd:string .

ns2:5a8e31edabf1e03c a ns2:AttackWebsite,
        owl:NamedIndividual ;
    ns1:associatedCampaigns ns2:Board_of_Control_for_Cricket_in_India ;
    ns1:description "Protest"^^xsd:string ;
    ns1:isLaunchedBy ns2:Bangladesh ;
    ns2:behaviour ns2:Protest ;
    ns2:hasActor "Ashik Iqbal Chy"^^xsd:string ;
    ns2:hasActorCountry "Bangladesh"^^xsd:string ;
    ns2:hasActorType "Hacktivist"^^xsd:string ;
    ns2:hasCountry "India"^^xsd:string ;
    ns2:hasEventDate "2014-01-27T00:00:00"^^xsd:dateTime ;
    ns2:hasEventSubtype "Message Manipulation"^^xsd:string ;
    ns2:hasEventType "Disruptive"^^xsd:string ;
    ns2:hasIndustry "Arts, Entertainment, and Recreation"^^xsd:string ;
    ns2:hasMonth 1 ;
    ns2:hasOrganization "Board of Control for Cricket in India"^^xsd:string ;
    ns2:hasYear 2014 ;
    ns2:isType_of ns2:Hacktivist,
        ns2:Message_Manipulation ;
    rdfs:comment "A Bangladeshi hacker called Ashik Iqbal Chy defaces the official website of Indian cricket's Governing body (bcci.tv) to protest against takeover proposal."^^xsd:string .

ns2:5b7908d285d2c28a a ns2:CyberattackData,
        owl:NamedIndividual ;
    ns1:associatedCampaigns ns2:Finnish_Foreign_Ministry ;
    ns1:description "Political-Espionage"^^xsd:string ;
    ns2:behaviour ns2:Political_Espionage ;
    ns2:hasActorType "Criminal"^^xsd:string ;
    ns2:hasCountry "Finland"^^xsd:string ;
    ns2:hasEventDate "2014-07-02T00:00:00"^^xsd:dateTime ;
    ns2:hasEventSubtype "Exploitation of End Hosts"^^xsd:string ;
    ns2:hasEventType "Exploitive"^^xsd:string ;
    ns2:hasIndustry "Public Administration"^^xsd:string ;
    ns2:hasMonth 7 ;
    ns2:hasOrganization "Finnish Foreign Ministry"^^xsd:string ;
    ns2:hasYear 2014 ;
    ns2:isType_of ns2:Criminal,
        ns2:Exploitation_of_End_Hosts ;
    rdfs:comment "Finland admits to have been attacked by hackers working for one or several foreign nations who stole a \"remarkable\" number of files over a period of several years."^^xsd:string .

ns2:5c50abbf0049bc8a a ns2:Phishing,
        owl:NamedIndividual ;
    ns1:associatedCampaigns ns2:TheNaturalOnline_com ;
    ns1:description "Financial"^^xsd:string ;
    ns2:behaviour ns2:Financial ;
    ns2:hasActorType "Criminal"^^xsd:string ;
    ns2:hasCampaign ns2:California ;
    ns2:hasCountry "United States of America"^^xsd:string ;
    ns2:hasCounty "Los Angeles"^^xsd:string ;
    ns2:hasEventDate "2014-08-14T00:00:00"^^xsd:dateTime ;
    ns2:hasEventSubtype "Exploitation of Application Server"^^xsd:string ;
    ns2:hasEventType "Exploitive"^^xsd:string ;
    ns2:hasIndustry "Retail Trade"^^xsd:string ;
    ns2:hasMonth 8 ;
    ns2:hasOrganization "TheNaturalOnline.com"^^xsd:string ;
    ns2:hasState "California"^^xsd:string ;
    ns2:hasYear 2014 ;
    ns2:isType_of ns2:Criminal,
        ns2:Exploitation_of_Application_Server ;
    rdfs:comment "TheNaturalOnline.com is compromised by an unknown attacker, who gains access to names, addresses, email addresses, phone numbers, passwords, credit and debit cards, expiration dates and CVV codes. "^^xsd:string .

ns2:5c52b1665bc24233 a ns2:CyberattackInformation,
        owl:NamedIndividual ;
    ns1:associatedCampaigns ns2:Mt__Gox ;
    ns2:hasActorType "Criminal"^^xsd:string ;
    ns2:hasCountry "Japan"^^xsd:string ;
    ns2:hasEventDate "2014-02-11T00:00:00"^^xsd:dateTime ;
    ns2:hasEventSubtype "External Denial of Service"^^xsd:string ;
    ns2:hasEventType "Disruptive"^^xsd:string ;
    ns2:hasIndustry "Finance and Insurance"^^xsd:string ;
    ns2:hasMonth 2 ;
    ns2:hasOrganization "Mt. Gox"^^xsd:string ;
    ns2:hasYear 2014 ;
    ns2:isType_of ns2:Criminal,
        ns2:External_Denial_of_Service ;
    rdfs:comment "Reuters reports that the virtual currency Bitcoin is being hit by attacks from unknown hackers sending \"mutated\" lines of code into the program that runs the virtual currency. Two exchanges, Bitstamp and Mt. Gox, are affected."^^xsd:string .

ns2:5c829742c764b6b1 a ns2:AccountAttack,
        owl:NamedIndividual ;
    ns1:associatedCampaigns ns2:Lutheran_Church_of_Australia ;
    ns2:hasActor "@security_511"^^xsd:string ;
    ns2:hasActorType "Hobbyist"^^xsd:string ;
    ns2:hasCountry "Australia"^^xsd:string ;
    ns2:hasEventDate "2014-03-05T00:00:00"^^xsd:dateTime ;
    ns2:hasEventSubtype "Exploitation of Application Server"^^xsd:string ;
    ns2:hasEventType "Exploitive"^^xsd:string ;
    ns2:hasIndustry "Other Services (except Public Administration)"^^xsd:string ;
    ns2:hasMonth 3 ;
    ns2:hasOrganization "Lutheran Church of Australia"^^xsd:string ;
    ns2:hasYear 2014 ;
    ns2:isType_of ns2:Exploitation_of_Application_Server,
        ns2:Hobbyist ;
    rdfs:comment "And here it is the third hack from @security_511 against a Church. This time the victim is the Lutheran Church of Australia (lca.org.au) with 1,484 user accounts containing user names, email addresses and encrypted passwords dumped."^^xsd:string .

ns2:5c9605b9d2d392e4 a ns2:DDoS,
        owl:NamedIndividual ;
    ns1:associatedCampaigns ns2:Wurm_Online ;
    ns2:hasActorType "Criminal"^^xsd:string ;
    ns2:hasCountry "Sweden"^^xsd:string ;
    ns2:hasEventDate "2014-02-18T00:00:00"^^xsd:dateTime ;
    ns2:hasEventSubtype "External Denial of Service"^^xsd:string ;
    ns2:hasEventType "Disruptive"^^xsd:string ;
    ns2:hasIndustry "Information"^^xsd:string ;
    ns2:hasMonth 2 ;
    ns2:hasOrganization "Wurm Online"^^xsd:string ;
    ns2:hasYear 2014 ;
    ns2:isType_of ns2:Criminal,
        ns2:External_Denial_of_Service ;
    rdfs:comment "After being knocked down by a DDoS attack, the operator of the online playing-game Wurm online offer a bounty of 10,000 euros ($13,000) to gather any information about the author of the attack."^^xsd:string .

ns2:5cc8c1294f98842e a ns2:BreachInformation,
        owl:NamedIndividual ;
    ns1:associatedCampaigns ns2:Metropolitan_Companies__Inc ;
    ns1:description "Financial"^^xsd:string ;
    ns2:behaviour ns2:Financial ;
    ns2:hasActorType "Criminal"^^xsd:string ;
    ns2:hasCampaign ns2:New_York ;
    ns2:hasCountry "United States of America"^^xsd:string ;
    ns2:hasCounty "New York"^^xsd:string ;
    ns2:hasEventDate "2014-06-20T00:00:00"^^xsd:dateTime ;
    ns2:hasEventSubtype "Exploitation of Application Server"^^xsd:string ;
    ns2:hasEventType "Exploitive"^^xsd:string ;
    ns2:hasIndustry "Administrative and Support and Waste Management and Remediation Services"^^xsd:string ;
    ns2:hasMonth 6 ;
    ns2:hasOrganization "Metropolitan Companies, Inc."^^xsd:string ;
    ns2:hasState "New York"^^xsd:string ;
    ns2:hasYear 2014 ;
    ns2:isType_of ns2:Criminal,
        ns2:Exploitation_of_Application_Server ;
    rdfs:comment "About 8,500 notification letters are sent out to individuals employed by, or who submitted an application to, The Metropolitan Companies, Inc., alerting them that an unauthorized third party may have gained access to their personal information."^^xsd:string .

ns2:5d0b8cfe51f1ddb1 a ns2:DefaceHacker,
        owl:NamedIndividual ;
    ns1:associatedCampaigns ns2:Federal_Customs_Service ;
    ns1:description "Protest"^^xsd:string ;
    ns2:behaviour ns2:Protest ;
    ns2:hasActor "MaXiMiZerS"^^xsd:string ;
    ns2:hasActorType "Hacktivist"^^xsd:string ;
    ns2:hasCountry "Russian Federation"^^xsd:string ;
    ns2:hasEventDate "2014-02-03T00:00:00"^^xsd:dateTime ;
    ns2:hasEventSubtype "Message Manipulation"^^xsd:string ;
    ns2:hasEventType "Disruptive"^^xsd:string ;
    ns2:hasIndustry "Public Administration"^^xsd:string ;
    ns2:hasMonth 2 ;
    ns2:hasOrganization "Federal Customs Service"^^xsd:string ;
    ns2:hasYear 2014 ;
    ns2:isType_of ns2:Hacktivist,
        ns2:Message_Manipulation ;
    rdfs:comment "The official English language website of Russia's Federal Customs Service (eng.customs.ru) is defaced by members of Team MaXiMiZerS."^^xsd:string .

ns2:5dd3ed696f89008a a ns2:CyberattackData,
        owl:NamedIndividual ;
    ns1:associatedCampaigns ns2:Gamma_Group ;
    ns1:isLaunchedBy ns2:United_Kingdom_of_Great_Britain_and_Nort ;
    ns2:hasActor "PhineasFisher"^^xsd:string ;
    ns2:hasActorCountry "United Kingdom of Great Britain and Northern Ireland"^^xsd:string ;
    ns2:hasActorType "Hacktivist"^^xsd:string ;
    ns2:hasCountry "United Kingdom of Great Britain and Northern Ireland"^^xsd:string ;
    ns2:hasEventDate "2014-08-08T00:00:00"^^xsd:dateTime ;
    ns2:hasEventSubtype "Exploitation of End Hosts"^^xsd:string ;
    ns2:hasEventType "Exploitive"^^xsd:string ;
    ns2:hasIndustry "Information"^^xsd:string ;
    ns2:hasMonth 8 ;
    ns2:hasOrganization "Gamma Group"^^xsd:string ;
    ns2:hasYear 2014 ;
    ns2:isType_of ns2:Exploitation_of_End_Hosts,
        ns2:Hacktivist ;
    rdfs:comment "Gamma International UK Ltd, the company that makes and sells the world's most elusive cyber weapon, FinFisher spyware, is hacked by a group called Phineas Fisher (@GammaGroupPR), and has a 40G file dumped on the internet."^^xsd:string .

ns2:5e4a887e898ce76f a ns2:BreachInformation,
        owl:NamedIndividual ;
    ns1:associatedCampaigns ns2:The_Houstonian_Hotel ;
    ns1:description "Financial"^^xsd:string ;
    ns2:behaviour ns2:Financial ;
    ns2:hasActorType "Criminal"^^xsd:string ;
    ns2:hasCampaign ns2:Texas ;
    ns2:hasCountry "United States of America"^^xsd:string ;
    ns2:hasCounty "Harris"^^xsd:string ;
    ns2:hasEventDate "2014-07-10T00:00:00"^^xsd:dateTime ;
    ns2:hasEventSubtype "Exploitation of Sensors"^^xsd:string ;
    ns2:hasEventType "Exploitive"^^xsd:string ;
    ns2:hasIndustry "Accommodation and Food Services"^^xsd:string ;
    ns2:hasMonth 7 ;
    ns2:hasOrganization "The Houstonian Hotel"^^xsd:string ;
    ns2:hasState "Texas"^^xsd:string ;
    ns2:hasYear 2014 ;
    ns2:isType_of ns2:Criminal,
        ns2:Exploitation_of_Sensors ;
    rdfs:comment "More than 10,000 customers are notified of six-month payment card breach at The Houstonian Hotel."^^xsd:string .

ns2:5e60d304e9a1ba74 a ns2:DDoS,
        owl:NamedIndividual ;
    ns1:associatedCampaigns ns2:League_of_Legends ;
    ns2:hasActor "DERP Trolling"^^xsd:string ;
    ns2:hasCampaign ns2:California ;
    ns2:hasCountry "United States of America"^^xsd:string ;
    ns2:hasCounty "Los Angeles"^^xsd:string ;
    ns2:hasEventDate "2014-01-03T00:00:00"^^xsd:dateTime ;
    ns2:hasEventSubtype "External Denial of Service"^^xsd:string ;
    ns2:hasEventType "Disruptive"^^xsd:string ;
    ns2:hasIndustry "Information"^^xsd:string ;
    ns2:hasMonth 1 ;
    ns2:hasOrganization "League of Legends"^^xsd:string ;
    ns2:hasState "California"^^xsd:string ;
    ns2:hasYear 2014 ;
    ns2:isType_of ns2:External_Denial_of_Service ;
    rdfs:comment "The servers for Steam, Origin, Battle.net, and League of Legends are brought down temporarily by apparent DDoS attacks that seem to be related to a swatting attack on an individual known for streaming games."^^xsd:string .

ns2:5ebd2458b3058bd8 a ns2:BreachSecurity,
        owl:NamedIndividual ;
    ns1:associatedCampaigns ns2:Department_of_Homeland_Securiety ;
    ns2:hasActorType "Criminal"^^xsd:string ;
    ns2:hasCountry "United States of America"^^xsd:string ;
    ns2:hasEventDate "2014-01-21T00:00:00"^^xsd:dateTime ;
    ns2:hasEventSubtype "Exploitation of Application Server"^^xsd:string ;
    ns2:hasEventType "Exploitive"^^xsd:string ;
    ns2:hasIndustry "Public Administration"^^xsd:string ;
    ns2:hasMonth 1 ;
    ns2:hasOrganization "Department of Homeland Securiety"^^xsd:string ;
    ns2:hasYear 2014 ;
    ns2:isType_of ns2:Criminal,
        ns2:Exploitation_of_Application_Server ;
    rdfs:comment "A security breach at a Web portal for the U.S. Department of Homeland Security exposes private documents and some financial information belonging to at least 114 contractors."^^xsd:string .

ns2:5f1e2354e7fe1af1 a ns2:AttackWebsite,
        owl:NamedIndividual ;
    ns1:associatedCampaigns ns2:antiwar_com ;
    ns2:hasActorType "Criminal"^^xsd:string ;
    ns2:hasCountry "United States of America"^^xsd:string ;
    ns2:hasEventDate "2014-05-14T00:00:00"^^xsd:dateTime ;
    ns2:hasEventSubtype "Exploitation of Application Server"^^xsd:string ;
    ns2:hasEventType "Exploitive"^^xsd:string ;
    ns2:hasIndustry "Other Services (except Public Administration)"^^xsd:string ;
    ns2:hasMonth 5 ;
    ns2:hasOrganization "antiwar.com"^^xsd:string ;
    ns2:hasYear 2014 ;
    ns2:isType_of ns2:Criminal,
        ns2:Exploitation_of_Application_Server ;
    rdfs:comment "antiwar.com, aÃÆÃ'Ãâ 'ÃÆÃ¢â¬Â 'ÃÆÃ'ÃÂ¢Ã¢'Â¬ÃÂ ''ÃÆÃ'Ãâ 'ÃÆÃ¢â¬Â ''ÃÆÃ'Ãâ ''ÃÆÃ''ÃÆ'Ã'ÃÂ website known for itsÃÆÃ'Ãâ 'ÃÆÃ¢â¬Â 'ÃÆÃ'ÃÂ¢Ã¢'Â¬ÃÂ ''ÃÆÃ'Ãâ 'ÃÆÃ¢â¬Â ''ÃÆÃ'Ãâ ''ÃÆÃ''ÃÆ'Ã'ÃÂ non-interventionism and war opposingÃÆÃ'Ãâ 'ÃÆÃ¢â¬Â 'ÃÆÃ'ÃÂ¢Ã¢'Â¬ÃÂ ''ÃÆÃ'Ãâ 'ÃÆÃ¢â¬Â ''ÃÆÃ'Ãâ ''ÃÆÃ''ÃÆ'Ã'ÃÂ views is hacked just a few hours after launching itsÃÆÃ'Ãâ 'ÃÆÃ¢â¬Â 'ÃÆÃ'ÃÂ¢Ã¢'Â¬ÃÂ ''ÃÆÃ'Ãâ 'ÃÆÃ¢â¬Â ''ÃÆÃ'Ãâ ''ÃÆÃ''ÃÆ'Ã'ÃÂ fundraising drive."^^xsd:string .

ns2:5f3c348d571b34e1 a ns2:AnonymousAttack,
        owl:NamedIndividual ;
    ns1:associatedCampaigns ns2:Various_Government_Websites ;
    ns1:description "Protest"^^xsd:string ;
    ns2:behaviour ns2:Protest ;
    ns2:hasActor "Anonymous"^^xsd:string ;
    ns2:hasActorType "Hacktivist"^^xsd:string ;
    ns2:hasCountry "Philippines"^^xsd:string ;
    ns2:hasEventDate "2014-02-26T00:00:00"^^xsd:dateTime ;
    ns2:hasEventSubtype "Message Manipulation"^^xsd:string ;
    ns2:hasEventType "Disruptive"^^xsd:string ;
    ns2:hasIndustry "Public Administration"^^xsd:string ;
    ns2:hasMonth 2 ;
    ns2:hasOrganization "Various Government Websites"^^xsd:string ;
    ns2:hasYear 2014 ;
    ns2:isType_of ns2:Hacktivist,
        ns2:Message_Manipulation ;
    rdfs:comment "Anonymous hackers once again target several websites of the Philippines government. The hacktivists are protesting against a provision of the Cybercrime Prevention Act that violates freedom of speech."^^xsd:string .

ns2:5f94407e263536ab a ns2:AccessAttack,
        owl:NamedIndividual ;
    ns1:associatedCampaigns ns2:ClamCase ;
    ns1:description "Financial"^^xsd:string ;
    ns2:behaviour ns2:Financial ;
    ns2:hasActorType "Criminal"^^xsd:string ;
    ns2:hasCampaign ns2:California ;
    ns2:hasCountry "United States of America"^^xsd:string ;
    ns2:hasCounty "Los Angeles"^^xsd:string ;
    ns2:hasEventDate "2014-08-29T00:00:00"^^xsd:dateTime ;
    ns2:hasEventSubtype "Exploitation of Application Server"^^xsd:string ;
    ns2:hasEventType "Exploitive"^^xsd:string ;
    ns2:hasIndustry "Wholesale Trade"^^xsd:string ;
    ns2:hasMonth 8 ;
    ns2:hasOrganization "ClamCase"^^xsd:string ;
    ns2:hasState "California"^^xsd:string ;
    ns2:hasYear 2014 ;
    ns2:isType_of ns2:Criminal,
        ns2:Exploitation_of_Application_Server ;
    rdfs:comment "ClamCase, a maker of keyboards and protective cases for iPads, notifies its customers that unidentified intruders gained access to personal information and payment details."^^xsd:string .

ns2:5fc1396786dea62a a ns2:AccessSecurity,
        owl:NamedIndividual ;
    ns1:associatedCampaigns ns2:University_of_North_Carolina_Wilmington ;
    ns2:hasActorType "Criminal"^^xsd:string ;
    ns2:hasCampaign ns2:North_Carolina ;
    ns2:hasCountry "United States of America"^^xsd:string ;
    ns2:hasCounty "New Hanover"^^xsd:string ;
    ns2:hasEventDate "2014-05-02T00:00:00"^^xsd:dateTime ;
    ns2:hasEventSubtype "Exploitation of Application Server"^^xsd:string ;
    ns2:hasEventType "Exploitive"^^xsd:string ;
    ns2:hasIndustry "Educational Services"^^xsd:string ;
    ns2:hasMonth 5 ;
    ns2:hasOrganization "University of North Carolina Wilmington"^^xsd:string ;
    ns2:hasState "North Carolina"^^xsd:string ;
    ns2:hasYear 2014 ;
    ns2:isType_of ns2:Criminal,
        ns2:Exploitation_of_Application_Server ;
    rdfs:comment "An undisclosed number of employees, graduate students and adjunct instructors with the University of North Carolina Wilmington (uncw.edu) may have had personal information compromised after unauthorized access was gained to an applications server."^^xsd:string .

ns2:5fd4e8683b3bdd28 a ns2:HackerSecurity,
        owl:NamedIndividual ;
    ns1:associatedCampaigns ns2:New_Zealand_National_Institute_of_Water_ ;
    ns2:hasActorType "Criminal"^^xsd:string ;
    ns2:hasCountry "New Zealand"^^xsd:string ;
    ns2:hasEventDate "2014-05-26T00:00:00"^^xsd:dateTime ;
    ns2:hasEventSubtype "Exploitation of Application Server"^^xsd:string ;
    ns2:hasEventType "Exploitive"^^xsd:string ;
    ns2:hasIndustry "Public Administration"^^xsd:string ;
    ns2:hasMonth 5 ;
    ns2:hasOrganization "New Zealand National Institute of Water and Atmospheric Research"^^xsd:string ;
    ns2:hasYear 2014 ;
    ns2:isType_of ns2:Criminal,
        ns2:Exploitation_of_Application_Server ;
    rdfs:comment "A $12.7 million supercomputer owned by Niwa (New Zealand National Institute for Water and Atmospheric Research) is targeted by a computer hacker believed to have come from China."^^xsd:string .

ns2:604291100b416921 a ns2:CyberattackSystem,
        owl:NamedIndividual ;
    ns1:associatedCampaigns ns2:Pakistan_Ministry_of_Railways ;
    ns1:isLaunchedBy ns2:Pakistan ;
    ns2:hasActor "Bl@Ck Dr@GoN; Haxor T0du; Spider64"^^xsd:string ;
    ns2:hasActorCountry "Pakistan"^^xsd:string ;
    ns2:hasActorType "Hacktivist"^^xsd:string ;
    ns2:hasCountry "Pakistan"^^xsd:string ;
    ns2:hasEventDate "2014-04-25T00:00:00"^^xsd:dateTime ;
    ns2:hasEventSubtype "Message Manipulation"^^xsd:string ;
    ns2:hasEventType "Disruptive"^^xsd:string ;
    ns2:hasIndustry "Public Administration"^^xsd:string ;
    ns2:hasMonth 4 ;
    ns2:hasOrganization "Pakistan Ministry of Railways"^^xsd:string ;
    ns2:hasYear 2014 ;
    ns2:isType_of ns2:Hacktivist,
        ns2:Message_Manipulation ;
    rdfs:comment "The cyber battle between Indian and Pakistani hacktivists continues. In name of OpPakistan Indian hackers deface several Pakistani government websites."^^xsd:string .

ns2:60671f83d08c5e2b a ns2:CyberattackInformation,
        owl:NamedIndividual ;
    ns1:associatedCampaigns ns2:Alaska_Communications ;
    ns1:description "Financial"^^xsd:string ;
    ns2:behaviour ns2:Financial ;
    ns2:hasActorType "Criminal"^^xsd:string ;
    ns2:hasCampaign ns2:Alaska ;
    ns2:hasCountry "United States of America"^^xsd:string ;
    ns2:hasCounty "Anchorage"^^xsd:string ;
    ns2:hasEventDate "2014-02-27T00:00:00"^^xsd:dateTime ;
    ns2:hasEventSubtype "Exploitation of End Hosts"^^xsd:string ;
    ns2:hasEventType "Exploitive"^^xsd:string ;
    ns2:hasIndustry "Information"^^xsd:string ;
    ns2:hasMonth 2 ;
    ns2:hasOrganization "Alaska Communications"^^xsd:string ;
    ns2:hasState "Alaska"^^xsd:string ;
    ns2:hasYear 2014 ;
    ns2:isType_of ns2:Criminal,
        ns2:Exploitation_of_End_Hosts ;
    rdfs:comment "Alaska Communications notifies an undisclosed number of current and former employees that their names, addresses, birthdates and Social Security numbers may have been exposed when a company computer was infected with a malware."^^xsd:string .

ns2:60704a5fc16599ff a ns2:AttackWebsite,
        owl:NamedIndividual ;
    ns1:associatedCampaigns ns2:Verkhovna_Rada ;
    ns2:hasActorType "Criminal"^^xsd:string ;
    ns2:hasCountry "Ukraine"^^xsd:string ;
    ns2:hasEventDate "2014-02-28T00:00:00"^^xsd:dateTime ;
    ns2:hasEventSubtype "External Denial of Service"^^xsd:string ;
    ns2:hasEventType "Disruptive"^^xsd:string ;
    ns2:hasIndustry "Public Administration"^^xsd:string ;
    ns2:hasMonth 2 ;
    ns2:hasOrganization "Verkhovna Rada"^^xsd:string ;
    ns2:hasYear 2014 ;
    ns2:isType_of ns2:Criminal,
        ns2:External_Denial_of_Service ;
    rdfs:comment "Hacktivists continue to launch attacks against Ukrainian government websites. The latest targets are the sites of the parliament, or the Verkhovna Rada (rada.gov.ua), the Right Sector nationalist movement (banderivets.org.ua), but also some Euromaidan websites."^^xsd:string .

ns2:60c43b8ef0ed4910 a ns2:CyberattackSystem,
        owl:NamedIndividual ;
    ns1:associatedCampaigns ns2:Ministry_of_Defense_of_Pakistan ;
    ns1:isLaunchedBy ns2:Pakistan ;
    ns2:hasActor "Bl@Ck Dr@GoN; Haxor T0du; Spider64"^^xsd:string ;
    ns2:hasActorCountry "Pakistan"^^xsd:string ;
    ns2:hasActorType "Hacktivist"^^xsd:string ;
    ns2:hasCountry "Pakistan"^^xsd:string ;
    ns2:hasEventDate "2014-04-25T00:00:00"^^xsd:dateTime ;
    ns2:hasEventSubtype "Message Manipulation"^^xsd:string ;
    ns2:hasEventType "Disruptive"^^xsd:string ;
    ns2:hasIndustry "Public Administration"^^xsd:string ;
    ns2:hasMonth 4 ;
    ns2:hasOrganization "Ministry of Defense of Pakistan"^^xsd:string ;
    ns2:hasYear 2014 ;
    ns2:isType_of ns2:Hacktivist,
        ns2:Message_Manipulation ;
    rdfs:comment "The cyber battle between Indian and Pakistani hacktivists continues. In name of OpPakistan Indian hackers deface several Pakistani government websites."^^xsd:string .

ns2:6100014f6ca84b3d a ns2:BreachInformation,
        owl:NamedIndividual ;
    ns1:associatedCampaigns ns2:Snapchat ;
    ns2:hasActorType "Criminal"^^xsd:string ;
    ns2:hasCampaign ns2:California ;
    ns2:hasCountry "United States of America"^^xsd:string ;
    ns2:hasCounty "Los Angeles"^^xsd:string ;
    ns2:hasEventDate "2014-01-02T00:00:00"^^xsd:dateTime ;
    ns2:hasEventSubtype "Exploitation of Application Server"^^xsd:string ;
    ns2:hasEventType "Exploitive"^^xsd:string ;
    ns2:hasIndustry "Information"^^xsd:string ;
    ns2:hasMonth 1 ;
    ns2:hasOrganization "Snapchat"^^xsd:string ;
    ns2:hasState "California"^^xsd:string ;
    ns2:hasYear 2014 ;
    ns2:isType_of ns2:Criminal,
        ns2:Exploitation_of_Application_Server ;
    rdfs:comment "Greyhat hackers publish the partial phone numbers belonging to more than 4.5 million Snapchat users after exploiting a recently disclosed security weakness that officials of the service had described as theoretical."^^xsd:string .

ns2:62acc1ac6e80b728 a ns2:AttackWebsite,
        owl:NamedIndividual ;
    ns1:associatedCampaigns ns2:Thadiq_Principality ;
    ns1:description "Protest"^^xsd:string ;
    ns1:isLaunchedBy ns2:Syrian_Arab_Republic ;
    ns2:behaviour ns2:Protest ;
    ns2:hasActor "Syrian Electronic Army"^^xsd:string ;
    ns2:hasActorCountry "Syrian Arab Republic"^^xsd:string ;
    ns2:hasActorType "Hacktivist"^^xsd:string ;
    ns2:hasCountry "Saudi Arabia"^^xsd:string ;
    ns2:hasEventDate "2014-01-16T00:00:00"^^xsd:dateTime ;
    ns2:hasEventSubtype "Message Manipulation"^^xsd:string ;
    ns2:hasEventType "Disruptive"^^xsd:string ;
    ns2:hasIndustry "Public Administration"^^xsd:string ;
    ns2:hasMonth 1 ;
    ns2:hasOrganization "Thadiq Principality"^^xsd:string ;
    ns2:hasYear 2014 ;
    ns2:isType_of ns2:Hacktivist,
        ns2:Message_Manipulation ;
    rdfs:comment "The Syrian Electronic Army deface 16 Saudi Arabian government websites. The targeted sites are the ones of various administrative regions."^^xsd:string .

ns2:62efcc269f5ff3e7 a ns2:AccountAttack,
        owl:NamedIndividual ;
    ns1:associatedCampaigns ns2:St__Aldhelm_s_Academy ;
    ns1:description "Financial"^^xsd:string ;
    ns2:behaviour ns2:Financial ;
    ns2:hasActorType "Criminal"^^xsd:string ;
    ns2:hasCountry "United Kingdom of Great Britain and Northern Ireland"^^xsd:string ;
    ns2:hasEventDate "2014-04-08T00:00:00"^^xsd:dateTime ;
    ns2:hasEventSubtype "Exploitation of Application Server"^^xsd:string ;
    ns2:hasEventType "Exploitive"^^xsd:string ;
    ns2:hasIndustry "Educational Services"^^xsd:string ;
    ns2:hasMonth 4 ;
    ns2:hasOrganization "St. Aldhelm's Academy"^^xsd:string ;
    ns2:hasYear 2014 ;
    ns2:isType_of ns2:Criminal,
        ns2:Exploitation_of_Application_Server ;
    rdfs:comment "Members of the finance staff at the UK's St. Aldhelm's Academy were fooled in July of 2013 by an e-mail that appeared to come from the school's bank. As a consequence, more than ÃÆÃ'Ãâ 'ÃÆÃ¢â¬Â 'ÃÆÃ'ÃÂ¢Ã¢'Â¬ÃÂ ''ÃÆÃ'Ãâ 'ÃÆÃ¢â¬Â ''ÃÆÃ'Ãâ ''ÃÆÃ''ÃÆ'Ã'ÃÂ£1 million ($1.7 million) was stolen."^^xsd:string .

ns2:6356ff181a67721c a ns2:BreachSecurity,
        owl:NamedIndividual ;
    ns1:associatedCampaigns ns2:Spirol_International ;
    ns2:hasActor "DeleteSec"^^xsd:string ;
    ns2:hasActorType "Hacktivist"^^xsd:string ;
    ns2:hasCampaign ns2:Connecticut ;
    ns2:hasCountry "United States of America"^^xsd:string ;
    ns2:hasCounty "Windham"^^xsd:string ;
    ns2:hasEventDate "2014-02-21T00:00:00"^^xsd:dateTime ;
    ns2:hasEventSubtype "Exploitation of Application Server"^^xsd:string ;
    ns2:hasEventType "Exploitive"^^xsd:string ;
    ns2:hasIndustry "Professional, Scientific, and Technical Services"^^xsd:string ;
    ns2:hasMonth 2 ;
    ns2:hasOrganization "Spirol International"^^xsd:string ;
    ns2:hasState "Connecticut"^^xsd:string ;
    ns2:hasYear 2014 ;
    ns2:isType_of ns2:Exploitation_of_Application_Server,
        ns2:Hacktivist ;
    rdfs:comment "Yet another attack by @DeleteSec. This time the victim is Spirol International (spirol.com) and as a result over 70,889 of the company's affected credentials are leaked online."^^xsd:string .

ns2:63c4e9367f748f5a a ns2:AccountAttack,
        owl:NamedIndividual ;
    ns1:associatedCampaigns ns2:SingPass ;
    ns2:hasActorType "Criminal"^^xsd:string ;
    ns2:hasCountry "Singapore"^^xsd:string ;
    ns2:hasEventDate "2014-06-05T00:00:00"^^xsd:dateTime ;
    ns2:hasEventSubtype "Exploitation of Application Server"^^xsd:string ;
    ns2:hasEventType "Exploitive"^^xsd:string ;
    ns2:hasIndustry "Public Administration"^^xsd:string ;
    ns2:hasMonth 6 ;
    ns2:hasOrganization "SingPass"^^xsd:string ;
    ns2:hasYear 2014 ;
    ns2:isType_of ns2:Criminal,
        ns2:Exploitation_of_Application_Server ;
    rdfs:comment "1,500 online identification accounts used for accessing Singapore government services may have been accessed illicitly."^^xsd:string .

ns2:6576adad6cf8d94d a ns2:HackerSecurity,
        owl:NamedIndividual ;
    ns1:associatedCampaigns ns2:Nuclear_Regulatory_Commission ;
    ns1:description "Political-Espionage"^^xsd:string ;
    ns2:behaviour ns2:Political_Espionage ;
    ns2:hasActorType "Criminal"^^xsd:string ;
    ns2:hasCampaign ns2:Maryland ;
    ns2:hasCountry "United States of America"^^xsd:string ;
    ns2:hasCounty "Montgomery"^^xsd:string ;
    ns2:hasEventDate "2014-08-18T00:00:00"^^xsd:dateTime ;
    ns2:hasEventSubtype "Exploitation of Application Server,Exploitation of End Hosts"^^xsd:string ;
    ns2:hasEventType "Exploitive"^^xsd:string ;
    ns2:hasIndustry "Public Administration"^^xsd:string ;
    ns2:hasMonth 8 ;
    ns2:hasOrganization "Nuclear Regulatory Commission"^^xsd:string ;
    ns2:hasState "Maryland"^^xsd:string ;
    ns2:hasYear 2014 ;
    ns2:isType_of ns2:Criminal,
        ns2:Exploitation_of_Application_Server_Explo ;
    rdfs:comment "A new report reveals that Nuclear Regulatory Commission computers were successfully hacked within the past three years by foreigners twice and also by an unidentifiable individual."^^xsd:string .

ns2:6578f5505982bc5b a ns2:AttackWebsite,
        owl:NamedIndividual ;
    ns1:associatedCampaigns ns2:Tehreek_e_Taliban_Pakistan ;
    ns1:isLaunchedBy ns2:Pakistan ;
    ns2:hasActor "Godzilla"^^xsd:string ;
    ns2:hasActorCountry "Pakistan"^^xsd:string ;
    ns2:hasActorType "Hacktivist"^^xsd:string ;
    ns2:hasCountry "Pakistan"^^xsd:string ;
    ns2:hasEventDate "2014-04-08T00:00:00"^^xsd:dateTime ;
    ns2:hasEventSubtype "External Denial of Service"^^xsd:string ;
    ns2:hasEventType "Disruptive"^^xsd:string ;
    ns2:hasIndustry "Other Services (except Public Administration)"^^xsd:string ;
    ns2:hasMonth 4 ;
    ns2:hasOrganization "Tehreek e Taliban Pakistan"^^xsd:string ;
    ns2:hasYear 2014 ;
    ns2:isType_of ns2:External_Denial_of_Service,
        ns2:Hacktivist ;
    rdfs:comment "The official website of terrorist organizationÃÆÃ'Ãâ 'ÃÆÃ¢â¬Â 'ÃÆÃ'ÃÂ¢Ã¢'Â¬ÃÂ ''ÃÆÃ'Ãâ 'ÃÆÃ¢â¬Â ''ÃÆÃ'Ãâ ''ÃÆÃ''ÃÆ'Ã'ÃÂ Tehreek-e-Taliban PakistanÃÆÃ'Ãâ 'ÃÆÃ¢â¬Â 'ÃÆÃ'ÃÂ¢Ã¢'Â¬ÃÂ ''ÃÆÃ'Ãâ 'ÃÆÃ¢â¬Â ''ÃÆÃ'Ãâ ''ÃÆÃ''ÃÆ'Ã'ÃÂ (TTP) (umarmedia.com)ÃÆÃ'Ãâ 'ÃÆÃ¢â¬Â 'ÃÆÃ'ÃÂ¢Ã¢'Â¬ÃÂ ''ÃÆÃ'Ãâ 'ÃÆÃ¢â¬Â ''ÃÆÃ'Ãâ ''ÃÆÃ''ÃÆ'Ã'ÃÂ is taken down by an Indian hacker calledÃÆÃ'Ãâ 'ÃÆÃ¢â¬Â 'ÃÆÃ'ÃÂ¢Ã¢'Â¬ÃÂ ''ÃÆÃ'Ãâ 'ÃÆÃ¢â¬Â ''ÃÆÃ'Ãâ ''ÃÆÃ''ÃÆ'Ã'ÃÂ Godzilla."^^xsd:string .

ns2:659dd8fd5348e70e a ns2:HackerSecurity,
        owl:NamedIndividual ;
    ns1:associatedCampaigns ns2:Gingerbread_Shed_Corporation ;
    ns1:description "Financial"^^xsd:string ;
    ns2:behaviour ns2:Financial ;
    ns2:hasActorType "Criminal"^^xsd:string ;
    ns2:hasCampaign ns2:Arizona ;
    ns2:hasCountry "United States of America"^^xsd:string ;
    ns2:hasCounty "Coconino"^^xsd:string ;
    ns2:hasEventDate "2014-05-13T00:00:00"^^xsd:dateTime ;
    ns2:hasEventSubtype "Exploitation of Application Server"^^xsd:string ;
    ns2:hasEventType "Exploitive"^^xsd:string ;
    ns2:hasIndustry "Arts, Entertainment, and Recreation"^^xsd:string ;
    ns2:hasMonth 5 ;
    ns2:hasOrganization "Gingerbread Shed Corporation"^^xsd:string ;
    ns2:hasState "Arizona"^^xsd:string ;
    ns2:hasYear 2014 ;
    ns2:isType_of ns2:Criminal,
        ns2:Exploitation_of_Application_Server ;
    rdfs:comment "Arizona-based Gingerbread Shed Corporation notifies customers that an unauthorized individual gained access to its systems for roughly three months and may have compromised about 50,000 transactions, as well as other data."^^xsd:string .

ns2:6645aca76cb83649 a ns2:AttackWebsite,
        owl:NamedIndividual ;
    ns1:associatedCampaigns ns2:Aldoriyah_Principality ;
    ns1:description "Protest"^^xsd:string ;
    ns1:isLaunchedBy ns2:Syrian_Arab_Republic ;
    ns2:behaviour ns2:Protest ;
    ns2:hasActor "Syrian Electronic Army"^^xsd:string ;
    ns2:hasActorCountry "Syrian Arab Republic"^^xsd:string ;
    ns2:hasActorType "Hacktivist"^^xsd:string ;
    ns2:hasCountry "Saudi Arabia"^^xsd:string ;
    ns2:hasEventDate "2014-01-16T00:00:00"^^xsd:dateTime ;
    ns2:hasEventSubtype "Message Manipulation"^^xsd:string ;
    ns2:hasEventType "Disruptive"^^xsd:string ;
    ns2:hasIndustry "Public Administration"^^xsd:string ;
    ns2:hasMonth 1 ;
    ns2:hasOrganization "Aldoriyah Principality"^^xsd:string ;
    ns2:hasYear 2014 ;
    ns2:isType_of ns2:Hacktivist,
        ns2:Message_Manipulation ;
    rdfs:comment "The Syrian Electronic Army deface 16 Saudi Arabian government websites. The targeted sites are the ones of various administrative regions."^^xsd:string .

ns2:68e43bad75b31bbb a ns2:CyberattackData,
        owl:NamedIndividual ;
    ns1:associatedCampaigns ns2:Syrian_National_Coalition ;
    ns1:isLaunchedBy ns2:Syrian_Arab_Republic ;
    ns2:hasActor "Syrian Electronic Army"^^xsd:string ;
    ns2:hasActorCountry "Syrian Arab Republic"^^xsd:string ;
    ns2:hasActorType "Hacktivist"^^xsd:string ;
    ns2:hasCountry "Syrian Arab Republic"^^xsd:string ;
    ns2:hasEventDate "2014-03-17T00:00:00"^^xsd:dateTime ;
    ns2:hasEventSubtype "Message Manipulation"^^xsd:string ;
    ns2:hasEventType "Disruptive"^^xsd:string ;
    ns2:hasIndustry "Other Services (except Public Administration)"^^xsd:string ;
    ns2:hasMonth 3 ;
    ns2:hasOrganization "Syrian National Coalition"^^xsd:string ;
    ns2:hasYear 2014 ;
    ns2:isType_of ns2:Hacktivist,
        ns2:Message_Manipulation ;
    rdfs:comment "The Syrian Electronic Army breaches and defaces the official website of the National Coalition for Syrian Revolutionary and Opposition Forces (etilaf.org). A number of other sites related to the organization have also been targeted."^^xsd:string .

ns2:698abbcd5fa60cd1 a ns2:HackerUser,
        owl:NamedIndividual ;
    ns1:associatedCampaigns ns2:marigold_in ;
    ns1:isLaunchedBy ns2:India ;
    ns2:hasActor "Kami Haxor"^^xsd:string ;
    ns2:hasActorCountry "India"^^xsd:string ;
    ns2:hasActorType "Hacktivist"^^xsd:string ;
    ns2:hasCountry "India"^^xsd:string ;
    ns2:hasEventDate "2014-04-15T00:00:00"^^xsd:dateTime ;
    ns2:hasEventSubtype "Exploitation of Application Server"^^xsd:string ;
    ns2:hasEventType "Exploitive"^^xsd:string ;
    ns2:hasMonth 4 ;
    ns2:hasOrganization "marigold.in"^^xsd:string ;
    ns2:hasYear 2014 ;
    ns2:isType_of ns2:Exploitation_of_Application_Server,
        ns2:Hacktivist ;
    rdfs:comment "Kami Haxor hacks marigold.in and dumps 1,351 usernames and clear text passwords."^^xsd:string .

ns2:6b0796917dcb27b0 a ns2:CyberattackData,
        owl:NamedIndividual ;
    ns1:associatedCampaigns ns2:Undisclosed_industrial_software_company ;
    ns2:hasActorType "Criminal"^^xsd:string ;
    ns2:hasEventDate "2014-09-02T00:00:00"^^xsd:dateTime ;
    ns2:hasEventSubtype "Exploitation of Application Server,Exploitation of End Hosts"^^xsd:string ;
    ns2:hasEventType "Exploitive"^^xsd:string ;
    ns2:hasIndustry "Information"^^xsd:string ;
    ns2:hasMonth 9 ;
    ns2:hasOrganization "Undisclosed industrial software company"^^xsd:string ;
    ns2:hasYear 2014 ;
    ns2:isType_of ns2:Criminal,
        ns2:Exploitation_of_Application_Server_Explo ;
    rdfs:comment "AlienVault reveals the details of Scanbox, a watering hole attack compromising the website of an industrial software company to collect information on the site's visitors."^^xsd:string .

ns2:6b436012b5b5f504 a ns2:CyberattackData,
        owl:NamedIndividual ;
    ns1:associatedCampaigns ns2:Office_of_the_Prime_Minister_of_Ukraine ;
    ns1:description "Political-Espionage"^^xsd:string ;
    ns2:behaviour ns2:Political_Espionage ;
    ns2:hasActorType "Criminal"^^xsd:string ;
    ns2:hasCountry "Ukraine"^^xsd:string ;
    ns2:hasEventDate "2014-08-08T00:00:00"^^xsd:dateTime ;
    ns2:hasEventSubtype "Exploitation of Application Server,Exploitation of End Hosts"^^xsd:string ;
    ns2:hasEventType "Exploitive"^^xsd:string ;
    ns2:hasIndustry "Public Administration"^^xsd:string ;
    ns2:hasMonth 8 ;
    ns2:hasOrganization "Office of the Prime Minister of Ukraine"^^xsd:string ;
    ns2:hasYear 2014 ;
    ns2:isType_of ns2:Criminal,
        ns2:Exploitation_of_Application_Server_Explo ;
    rdfs:comment "Dozens of computers in the Ukrainian prime minister's office and at least 10 of Ukraine's embassies abroad are infected with a cyber espionage weapon linked to Russia."^^xsd:string .

ns2:6c4748e621f40786 a ns2:CyberattackData,
        owl:NamedIndividual ;
    ns1:associatedCampaigns ns2:Israel_Defense_Forces ;
    ns1:isLaunchedBy ns2:Syrian_Arab_Republic ;
    ns2:hasActor "Syrian Electronic Army"^^xsd:string ;
    ns2:hasActorCountry "Syrian Arab Republic"^^xsd:string ;
    ns2:hasActorType "Hacktivist"^^xsd:string ;
    ns2:hasCountry "Israel"^^xsd:string ;
    ns2:hasEventDate "2014-07-04T00:00:00"^^xsd:dateTime ;
    ns2:hasEventSubtype "Message Manipulation"^^xsd:string ;
    ns2:hasEventType "Disruptive"^^xsd:string ;
    ns2:hasIndustry "Public Administration"^^xsd:string ;
    ns2:hasMonth 7 ;
    ns2:hasOrganization "Israel Defense Forces"^^xsd:string ;
    ns2:hasYear 2014 ;
    ns2:isType_of ns2:Hacktivist,
        ns2:Message_Manipulation ;
    rdfs:comment "The Syrian Electronic Army hacks the Twitter account and official blog of the Israel Defence Forces (@IDFSpokeperson) and posts a fake tweet related to a possible nuclear leak to the 300,000 account followers."^^xsd:string .

ns2:6c99ea3c0029707b a ns2:BreachInformation,
        owl:NamedIndividual ;
    ns1:associatedCampaigns ns2:Singapore_government_employees ;
    ns1:description "Protest"^^xsd:string ;
    ns2:behaviour ns2:Protest ;
    ns2:hasActor "Anonymous"^^xsd:string ;
    ns2:hasActorType "Hacktivist"^^xsd:string ;
    ns2:hasCountry "Singapore"^^xsd:string ;
    ns2:hasEventDate "2014-02-07T00:00:00"^^xsd:dateTime ;
    ns2:hasEventSubtype "Exploitation of Application Server"^^xsd:string ;
    ns2:hasEventType "Exploitive"^^xsd:string ;
    ns2:hasIndustry "Public Administration"^^xsd:string ;
    ns2:hasMonth 2 ;
    ns2:hasOrganization "Singapore government employees"^^xsd:string ;
    ns2:hasYear 2014 ;
    ns2:isType_of ns2:Exploitation_of_Application_Server,
        ns2:Hacktivist ;
    rdfs:comment "In response to recent arrests in Singapore linked to Anonymous, the hacktivist group releases the details of 10 Singapore Government employes and threaten to release more."^^xsd:string .

ns2:6ca6cf75d44b6e3c a ns2:DDoS,
        owl:NamedIndividual ;
    ns1:associatedCampaigns ns2:Albuquerque_Police_Department ;
    ns1:description "Protest"^^xsd:string ;
    ns2:behaviour ns2:Protest ;
    ns2:hasActor "Anonymous"^^xsd:string ;
    ns2:hasActorType "Hacktivist"^^xsd:string ;
    ns2:hasCampaign ns2:New_Mexico ;
    ns2:hasCountry "United States of America"^^xsd:string ;
    ns2:hasCounty "Bernalillo"^^xsd:string ;
    ns2:hasEventDate "2014-03-31T00:00:00"^^xsd:dateTime ;
    ns2:hasEventSubtype "External Denial of Service"^^xsd:string ;
    ns2:hasEventType "Disruptive"^^xsd:string ;
    ns2:hasIndustry "Public Administration"^^xsd:string ;
    ns2:hasMonth 3 ;
    ns2:hasOrganization "Albuquerque Police Department"^^xsd:string ;
    ns2:hasState "New Mexico"^^xsd:string ;
    ns2:hasYear 2014 ;
    ns2:isType_of ns2:External_Denial_of_Service,
        ns2:Hacktivist ;
    rdfs:comment "The Albuquerque Police Department is the target of a DDoS attack carried on by the Infamous Anonymous collective."^^xsd:string .

ns2:6cb1197f4099b27e a ns2:CyberattackInformation,
        owl:NamedIndividual ;
    ns1:associatedCampaigns ns2:Turkmenbashi_Bank ;
    ns2:hasActor "Dr.SHA6H"^^xsd:string ;
    ns2:hasActorType "Hacktivist"^^xsd:string ;
    ns2:hasCountry "Turkmenistan"^^xsd:string ;
    ns2:hasEventDate "2014-02-07T00:00:00"^^xsd:dateTime ;
    ns2:hasEventSubtype "Message Manipulation"^^xsd:string ;
    ns2:hasEventType "Disruptive"^^xsd:string ;
    ns2:hasIndustry "Finance and Insurance"^^xsd:string ;
    ns2:hasMonth 2 ;
    ns2:hasOrganization "Turkmenbashi Bank"^^xsd:string ;
    ns2:hasYear 2014 ;
    ns2:isType_of ns2:Hacktivist,
        ns2:Message_Manipulation ;
    rdfs:comment "The official websites of two Turkmenistan state-owned commercial banks are hacked and defaced by Dr.Sha6h, to raise awareness of the situation in Syria. The victims are: Turkmenbashi Bank (tbbank.gov.tm), PrezidentBank (presidentbank.gov.tm)."^^xsd:string .

ns2:6dc4c9822a775d59 a ns2:HackerSecurity,
        owl:NamedIndividual ;
    ns1:associatedCampaigns ns2:Plexor ;
    ns1:description "Protest"^^xsd:string ;
    ns1:isLaunchedBy ns2:United_States_of_America ;
    ns2:behaviour ns2:Protest ;
    ns2:hasActor "CoMoDo"^^xsd:string ;
    ns2:hasActorCountry "United States of America"^^xsd:string ;
    ns2:hasActorType "Hacktivist"^^xsd:string ;
    ns2:hasCampaign ns2:California ;
    ns2:hasCountry "United States of America"^^xsd:string ;
    ns2:hasCounty "Santa Clara"^^xsd:string ;
    ns2:hasEventDate "2014-08-07T00:00:00"^^xsd:dateTime ;
    ns2:hasEventSubtype "Message Manipulation"^^xsd:string ;
    ns2:hasEventType "Disruptive"^^xsd:string ;
    ns2:hasIndustry "Manufacturing"^^xsd:string ;
    ns2:hasMonth 8 ;
    ns2:hasOrganization "Plexor"^^xsd:string ;
    ns2:hasState "California"^^xsd:string ;
    ns2:hasYear 2014 ;
    ns2:isType_of ns2:Hacktivist,
        ns2:Message_Manipulation ;
    rdfs:comment "The US website of computer hardware manufacturer Plextor is taken over by a group of hackers identifying themselves as CoMoDo."^^xsd:string .

ns2:6e4e1298ceb177af a ns2:HackerSecurity,
        owl:NamedIndividual ;
    ns1:associatedCampaigns ns2:MarkMonitor ;
    ns1:isLaunchedBy ns2:Syrian_Arab_Republic ;
    ns2:hasActor "Syrian Electronic Army"^^xsd:string ;
    ns2:hasActorCountry "Syrian Arab Republic"^^xsd:string ;
    ns2:hasActorType "Hacktivist"^^xsd:string ;
    ns2:hasCampaign ns2:Idaho ;
    ns2:hasCountry "United States of America"^^xsd:string ;
    ns2:hasCounty "Ada"^^xsd:string ;
    ns2:hasEventDate "2014-02-06T00:00:00"^^xsd:dateTime ;
    ns2:hasEventSubtype "External Denial of Service"^^xsd:string ;
    ns2:hasEventType "Disruptive"^^xsd:string ;
    ns2:hasIndustry "Information"^^xsd:string ;
    ns2:hasMonth 2 ;
    ns2:hasOrganization "MarkMonitor"^^xsd:string ;
    ns2:hasState "Idaho"^^xsd:string ;
    ns2:hasYear 2014 ;
    ns2:isType_of ns2:External_Denial_of_Service,
        ns2:Hacktivist ;
    rdfs:comment "A failed attempt that's worth to be mentioned: the Syrian Electronic Army attempts to hack a number of high profile websites, including Yahoo, Amazon, Facebook and Google, by hacking into the domain management service provider MarkMonitor."^^xsd:string .

ns2:6e61c271c6adc1cd a ns2:AnonymousAttack,
        owl:NamedIndividual ;
    ns1:associatedCampaigns ns2:Nordea ;
    ns1:description "Protest"^^xsd:string ;
    ns1:isLaunchedBy ns2:Norway ;
    ns2:behaviour ns2:Protest ;
    ns2:hasActor "Anonymous (Norway)"^^xsd:string ;
    ns2:hasActorCountry "Norway"^^xsd:string ;
    ns2:hasActorType "Hacktivist"^^xsd:string ;
    ns2:hasCountry "Norway"^^xsd:string ;
    ns2:hasEventDate "2014-07-09T00:00:00"^^xsd:dateTime ;
    ns2:hasEventSubtype "External Denial of Service"^^xsd:string ;
    ns2:hasEventType "Disruptive"^^xsd:string ;
    ns2:hasIndustry "Finance and Insurance"^^xsd:string ;
    ns2:hasMonth 7 ;
    ns2:hasOrganization "Nordea"^^xsd:string ;
    ns2:hasYear 2014 ;
    ns2:isType_of ns2:External_Denial_of_Service,
        ns2:Hacktivist ;
    rdfs:comment "Anonymous Norway starts multiple DDoS attacks towards major banks and insurance companies in Norway, including the country's largest telecommunications company, Telenor."^^xsd:string .

ns2:6eaa8cb6b6dc0194 a ns2:AnonymousAttack,
        owl:NamedIndividual ;
    ns1:associatedCampaigns ns2:Parkistan_Army ;
    ns2:hasActor "Anonymous"^^xsd:string ;
    ns2:hasActorType "Hacktivist"^^xsd:string ;
    ns2:hasCountry "Pakistan"^^xsd:string ;
    ns2:hasEventDate "2014-08-30T00:00:00"^^xsd:dateTime ;
    ns2:hasEventSubtype "External Denial of Service"^^xsd:string ;
    ns2:hasEventType "Disruptive"^^xsd:string ;
    ns2:hasIndustry "Public Administration"^^xsd:string ;
    ns2:hasMonth 8 ;
    ns2:hasOrganization "Parkistan Army"^^xsd:string ;
    ns2:hasYear 2014 ;
    ns2:isType_of ns2:External_Denial_of_Service,
        ns2:Hacktivist ;
    rdfs:comment "In the name of #OpPakistan, Anonymous conducts a massive cyber attack against many Pakistani government websites, including Parkistan Army's recruitment website, government of Punjab's official portal, Pakistan Meteorological Department, Employees Old-Age Benefits Institution, and several other high-profile sites."^^xsd:string .

ns2:6eb9381090e64eb5 a ns2:DDoS,
        owl:NamedIndividual ;
    ns1:associatedCampaigns ns2:Club_Penguin ;
    ns2:hasActor "DERP Trolling"^^xsd:string ;
    ns2:hasCountry "United States of America"^^xsd:string ;
    ns2:hasEventDate "2014-01-03T00:00:00"^^xsd:dateTime ;
    ns2:hasEventSubtype "External Denial of Service"^^xsd:string ;
    ns2:hasEventType "Disruptive"^^xsd:string ;
    ns2:hasIndustry "Information"^^xsd:string ;
    ns2:hasMonth 1 ;
    ns2:hasOrganization "Club Penguin"^^xsd:string ;
    ns2:hasYear 2014 ;
    ns2:isType_of ns2:External_Denial_of_Service ;
    rdfs:comment "The servers for Steam, Origin, Battle.net, and League of Legends are brought down temporarily by apparent DDoS attacks that seem to be related to a swatting attack on an individual known for streaming games."^^xsd:string .

ns2:6f7ef6029ac453f3 a ns2:AnonymousAttack,
        owl:NamedIndividual ;
    ns1:associatedCampaigns ns2:New_York_Board_of_Elections ;
    ns1:description "Protest"^^xsd:string ;
    ns2:behaviour ns2:Protest ;
    ns2:hasActor "Anonymous"^^xsd:string ;
    ns2:hasActorType "Hacktivist"^^xsd:string ;
    ns2:hasCampaign ns2:New_York ;
    ns2:hasCountry "United States of America"^^xsd:string ;
    ns2:hasCounty "Albany"^^xsd:string ;
    ns2:hasEventDate "2014-06-09T00:00:00"^^xsd:dateTime ;
    ns2:hasEventSubtype "Message Manipulation"^^xsd:string ;
    ns2:hasEventType "Disruptive"^^xsd:string ;
    ns2:hasIndustry "Public Administration"^^xsd:string ;
    ns2:hasMonth 6 ;
    ns2:hasOrganization "New York Board of Elections"^^xsd:string ;
    ns2:hasState "New York"^^xsd:string ;
    ns2:hasYear 2014 ;
    ns2:isType_of ns2:Hacktivist,
        ns2:Message_Manipulation ;
    rdfs:comment "The Anonymous protest against the FIFA World Cup starts here: the hacktivist collective defaces the New York State Board of ElectionsÃÆÃ'Ãâ 'ÃÆÃ¢â¬Â 'ÃÆÃ'ÃÂ¢Ã¢'Â¬ÃÂ ''ÃÆÃ'Ãâ 'ÃÆÃ¢â¬Â ''ÃÆÃ'Ãâ ''ÃÆÃ''ÃÆ'Ã'ÃÂ official websiteÃÆÃ'Ãâ 'ÃÆÃ¢â¬Â 'ÃÆÃ'ÃÂ¢Ã¢'Â¬ÃÂ ''ÃÆÃ'Ãâ 'ÃÆÃ¢â¬Â ''ÃÆÃ'Ãâ ''ÃÆÃ''ÃÆ'Ã'ÃÂ (elections.ny.gov)."^^xsd:string .

ns2:70ab6b62895b12f7 a ns2:BreachInformation,
        owl:NamedIndividual ;
    ns1:associatedCampaigns ns2:College_of_Physicians_and_Surgeons ;
    ns2:hasActorType "Criminal"^^xsd:string ;
    ns2:hasCountry "United States of America"^^xsd:string ;
    ns2:hasEventDate "2014-01-17T00:00:00"^^xsd:dateTime ;
    ns2:hasEventSubtype "Exploitation of Application Server"^^xsd:string ;
    ns2:hasEventType "Exploitive"^^xsd:string ;
    ns2:hasIndustry "Other Services (except Public Administration)"^^xsd:string ;
    ns2:hasMonth 1 ;
    ns2:hasOrganization "College of Physicians and Surgeons"^^xsd:string ;
    ns2:hasYear 2014 ;
    ns2:isType_of ns2:Criminal,
        ns2:Exploitation_of_Application_Server ;
    rdfs:comment "AP reveals that the personal information of all licensed  medical doctors in Puerto Rico is allegedly compromised in a recent hack. Up to 10,000 users may have been compromised."^^xsd:string .

ns2:711bfe3d86e81232 a ns2:DDoS,
        owl:NamedIndividual ;
    ns1:associatedCampaigns ns2:Mad_Mimi ;
    ns1:description "Financial"^^xsd:string ;
    ns2:behaviour ns2:Financial ;
    ns2:hasActor "Mark Nsd"^^xsd:string ;
    ns2:hasActorType "Criminal"^^xsd:string ;
    ns2:hasCampaign ns2:New_York ;
    ns2:hasCountry "United States of America"^^xsd:string ;
    ns2:hasCounty "New York"^^xsd:string ;
    ns2:hasEventDate "2014-04-01T00:00:00"^^xsd:dateTime ;
    ns2:hasEventSubtype "External Denial of Service"^^xsd:string ;
    ns2:hasEventType "Disruptive"^^xsd:string ;
    ns2:hasIndustry "Professional, Scientific, and Technical Services"^^xsd:string ;
    ns2:hasMonth 4 ;
    ns2:hasOrganization "Mad Mimi"^^xsd:string ;
    ns2:hasState "New York"^^xsd:string ;
    ns2:hasYear 2014 ;
    ns2:isType_of ns2:Criminal,
        ns2:External_Denial_of_Service ;
    rdfs:comment "Email marketing service Mad Mimi is hit by a DDoS attack. Shortly after, they receive an email from someone who asked for 1.8 Bitcoins to stop launching attacks."^^xsd:string .

ns2:711c06638a817365 a ns2:DDoS,
        owl:NamedIndividual ;
    ns1:associatedCampaigns ns2:Typepad ;
    ns2:hasActorType "Criminal"^^xsd:string ;
    ns2:hasCountry "United States of America"^^xsd:string ;
    ns2:hasEventDate "2014-05-19T00:00:00"^^xsd:dateTime ;
    ns2:hasEventSubtype "External Denial of Service"^^xsd:string ;
    ns2:hasEventType "Disruptive"^^xsd:string ;
    ns2:hasIndustry "Information"^^xsd:string ;
    ns2:hasMonth 5 ;
    ns2:hasOrganization "Typepad"^^xsd:string ;
    ns2:hasYear 2014 ;
    ns2:isType_of ns2:Criminal,
        ns2:External_Denial_of_Service ;
    rdfs:comment "Typepad, the famous blogging platform is under a sustained DDoS attack."^^xsd:string .

ns2:7136e63237294f84 a ns2:AttackWebsite,
        owl:NamedIndividual ;
    ns1:associatedCampaigns ns2:Soma_Municipality ;
    ns1:description "Protest"^^xsd:string ;
    ns1:isLaunchedBy ns2:Turkey ;
    ns2:behaviour ns2:Protest ;
    ns2:hasActor "RedHack"^^xsd:string ;
    ns2:hasActorCountry "Turkey"^^xsd:string ;
    ns2:hasActorType "Hacktivist"^^xsd:string ;
    ns2:hasCountry "Turkey"^^xsd:string ;
    ns2:hasEventDate "2014-05-14T00:00:00"^^xsd:dateTime ;
    ns2:hasEventSubtype "Message Manipulation"^^xsd:string ;
    ns2:hasEventType "Disruptive"^^xsd:string ;
    ns2:hasIndustry "Public Administration"^^xsd:string ;
    ns2:hasMonth 5 ;
    ns2:hasOrganization "Soma Municipality"^^xsd:string ;
    ns2:hasYear 2014 ;
    ns2:isType_of ns2:Hacktivist,
        ns2:Message_Manipulation ;
    rdfs:comment "Hacktivists of the RedHack collective blame authorities for the incident in the mine of Soma, and as a consequence they deface the official website of the Soma Municipality."^^xsd:string .

ns2:71b7a8ae5b5e9f5f a ns2:AnonymousAttack,
        owl:NamedIndividual ;
    ns1:associatedCampaigns ns2:Fullerton_Police_Department ;
    ns1:description "Protest"^^xsd:string ;
    ns2:behaviour ns2:Protest ;
    ns2:hasActor "Anonymous"^^xsd:string ;
    ns2:hasActorType "Hacktivist"^^xsd:string ;
    ns2:hasCampaign ns2:California ;
    ns2:hasCountry "United States of America"^^xsd:string ;
    ns2:hasCounty "Orange"^^xsd:string ;
    ns2:hasEventDate "2014-01-19T00:00:00"^^xsd:dateTime ;
    ns2:hasEventSubtype "External Denial of Service"^^xsd:string ;
    ns2:hasEventType "Disruptive"^^xsd:string ;
    ns2:hasIndustry "Public Administration"^^xsd:string ;
    ns2:hasMonth 1 ;
    ns2:hasOrganization "Fullerton Police Department"^^xsd:string ;
    ns2:hasState "California"^^xsd:string ;
    ns2:hasYear 2014 ;
    ns2:isType_of ns2:External_Denial_of_Service,
        ns2:Hacktivist ;
    rdfs:comment "Anonymous takes down the official website of Fullerton police department against the arrest of protesters and acquittal of police officers who had beaten the homeless Kelly Thomas to death in 2011."^^xsd:string .

ns2:71cacdfcb6ddb007 a ns2:CyberattackInformation,
        owl:NamedIndividual ;
    ns1:associatedCampaigns ns2:Official_website_of_the_President_of_Nep ;
    ns2:hasActorType "Criminal"^^xsd:string ;
    ns2:hasCountry "Nepal"^^xsd:string ;
    ns2:hasEventDate "2014-02-08T00:00:00"^^xsd:dateTime ;
    ns2:hasEventSubtype "Message Manipulation"^^xsd:string ;
    ns2:hasEventType "Disruptive"^^xsd:string ;
    ns2:hasIndustry "Public Administration"^^xsd:string ;
    ns2:hasMonth 2 ;
    ns2:hasOrganization "Official website of the President of Nepal"^^xsd:string ;
    ns2:hasYear 2014 ;
    ns2:isType_of ns2:Criminal,
        ns2:Message_Manipulation ;
    rdfs:comment "Two separate attacks deface the official website of Nepal's Office of the President (presidentofnepal.gov.np). In the first case, the attacker who goes by Dr.3v1l, also leaked some information stolen from the DB. The second attack was carried out by an Indian hacker."^^xsd:string .

ns2:7238ce487b748e04 a ns2:CyberattackData,
        owl:NamedIndividual ;
    ns1:associatedCampaigns ns2:Penn_State_College_of_Medicine ;
    ns1:description "Financial"^^xsd:string ;
    ns2:behaviour ns2:Financial ;
    ns2:hasActorType "Criminal"^^xsd:string ;
    ns2:hasCampaign ns2:Pennsylvania ;
    ns2:hasCountry "United States of America"^^xsd:string ;
    ns2:hasCounty "Dauphin"^^xsd:string ;
    ns2:hasEventDate "2014-07-10T00:00:00"^^xsd:dateTime ;
    ns2:hasEventSubtype "Exploitation of End Hosts"^^xsd:string ;
    ns2:hasEventType "Exploitive"^^xsd:string ;
    ns2:hasIndustry "Educational Services"^^xsd:string ;
    ns2:hasMonth 7 ;
    ns2:hasOrganization "Penn State College of Medicine"^^xsd:string ;
    ns2:hasState "Pennsylvania"^^xsd:string ;
    ns2:hasYear 2014 ;
    ns2:isType_of ns2:Criminal,
        ns2:Exploitation_of_End_Hosts ;
    rdfs:comment "1176 Penn State College of Medicine alumni's Social Security numbers might have been compromised after malware was found on a university computer."^^xsd:string .

ns2:728947be50991bce a ns2:BreachInformation,
        owl:NamedIndividual ;
    ns1:associatedCampaigns ns2:Sorenson_Communications ;
    ns1:description "Financial"^^xsd:string ;
    ns2:behaviour ns2:Financial ;
    ns2:hasActorType "Criminal"^^xsd:string ;
    ns2:hasCampaign ns2:Utah ;
    ns2:hasCountry "United States of America"^^xsd:string ;
    ns2:hasCounty "Salt Lake"^^xsd:string ;
    ns2:hasEventDate "2014-03-27T00:00:00"^^xsd:dateTime ;
    ns2:hasEventSubtype "Exploitation of Application Server"^^xsd:string ;
    ns2:hasEventType "Exploitive"^^xsd:string ;
    ns2:hasIndustry "Information"^^xsd:string ;
    ns2:hasMonth 3 ;
    ns2:hasOrganization "Sorenson Communications"^^xsd:string ;
    ns2:hasState "Utah"^^xsd:string ;
    ns2:hasYear 2014 ;
    ns2:isType_of ns2:Criminal,
        ns2:Exploitation_of_Application_Server ;
    rdfs:comment "All employees with Utah-based Sorenson Communications, and a branch named CaptionCall, are notified that their personal information may have been compromised after the data was accessed in an attack on an unnamed payroll vendor."^^xsd:string .

ns2:7331c6ab27af2274 a ns2:AnonymousAttack,
        owl:NamedIndividual ;
    ns1:associatedCampaigns ns2:Office_of_the_Israeli_Prime_Minister ;
    ns1:description "Protest"^^xsd:string ;
    ns2:behaviour ns2:Protest ;
    ns2:hasActor "Anonymous"^^xsd:string ;
    ns2:hasActorType "Hacktivist"^^xsd:string ;
    ns2:hasCountry "Israel"^^xsd:string ;
    ns2:hasEventDate "2014-08-25T00:00:00"^^xsd:dateTime ;
    ns2:hasEventSubtype "External Denial of Service"^^xsd:string ;
    ns2:hasEventType "Disruptive"^^xsd:string ;
    ns2:hasIndustry "Public Administration"^^xsd:string ;
    ns2:hasMonth 8 ;
    ns2:hasOrganization "Office of the Israeli Prime Minister"^^xsd:string ;
    ns2:hasYear 2014 ;
    ns2:isType_of ns2:External_Denial_of_Service,
        ns2:Hacktivist ;
    rdfs:comment "In name of #OpSaveGaza, the Anonymous collective claims to have taken down some key Israeli governmental websites, including those of the Israeli Defense Forces, the Bank of Israel, the Israeli Prime Minister."^^xsd:string .

ns2:7336d12d76042490 a ns2:AttackWebsite,
        owl:NamedIndividual ;
    ns1:associatedCampaigns ns2:Air_France ;
    ns1:isLaunchedBy ns2:France ;
    ns2:hasActor "Algerian Mujahideen"^^xsd:string ;
    ns2:hasActorCountry "France"^^xsd:string ;
    ns2:hasActorType "Hacktivist"^^xsd:string ;
    ns2:hasCountry "France"^^xsd:string ;
    ns2:hasEventDate "2015-03-30T00:00:00"^^xsd:dateTime ;
    ns2:hasEventSubtype "Message Manipulation"^^xsd:string ;
    ns2:hasEventType "Disruptive"^^xsd:string ;
    ns2:hasIndustry "Transportation and Warehousing"^^xsd:string ;
    ns2:hasMonth 3 ;
    ns2:hasOrganization "Air France"^^xsd:string ;
    ns2:hasYear 2015 ;
    ns2:isType_of ns2:Hacktivist,
        ns2:Message_Manipulation ;
    rdfs:comment "The website of Air France's national mutual society (mnpaf.fr) is defaced by a group calling itself Moujahidin Team, in retaliation for the Setif and Guelma massacres that happened on May 8, 1945."^^xsd:string .

ns2:737e2414b0083541 a ns2:AccountAttack,
        owl:NamedIndividual ;
    ns1:associatedCampaigns ns2:Gary_Barlow ;
    ns2:hasActorType "Criminal"^^xsd:string ;
    ns2:hasCountry "United Kingdom of Great Britain and Northern Ireland"^^xsd:string ;
    ns2:hasEventDate "2014-05-12T00:00:00"^^xsd:dateTime ;
    ns2:hasEventSubtype "Message Manipulation"^^xsd:string ;
    ns2:hasEventType "Disruptive"^^xsd:string ;
    ns2:hasIndustry "Other Services (except Public Administration)"^^xsd:string ;
    ns2:hasMonth 5 ;
    ns2:hasOrganization "Gary Barlow"^^xsd:string ;
    ns2:hasYear 2014 ;
    ns2:isType_of ns2:Criminal,
        ns2:Message_Manipulation ;
    rdfs:comment "The Twitter account of Gary Barlow (@GaryBarlow) the former frontman of the famous boy band Take That is hacked."^^xsd:string .

ns2:7413d4d78b4c882b a ns2:AccountAttack,
        owl:NamedIndividual ;
    ns1:associatedCampaigns ns2:Naver ;
    ns1:description "Financial"^^xsd:string ;
    ns1:isLaunchedBy ns2:Korea__the_Republic_of ;
    ns2:behaviour ns2:Financial ;
    ns2:hasActor "SEO"^^xsd:string ;
    ns2:hasActorCountry "Korea (the Republic of)"^^xsd:string ;
    ns2:hasActorType "Criminal"^^xsd:string ;
    ns2:hasCountry "Korea (the Republic of)"^^xsd:string ;
    ns2:hasEventDate "2014-03-26T00:00:00"^^xsd:dateTime ;
    ns2:hasEventSubtype "Exploitation of Application Server"^^xsd:string ;
    ns2:hasEventType "Exploitive"^^xsd:string ;
    ns2:hasIndustry "Professional, Scientific, and Technical Services"^^xsd:string ;
    ns2:hasMonth 3 ;
    ns2:hasOrganization "Naver"^^xsd:string ;
    ns2:hasYear 2014 ;
    ns2:isType_of ns2:Criminal,
        ns2:Exploitation_of_Application_Server ;
    rdfs:comment "A 31-year-old man is arrested for infiltrating the accounts of 25 million people on Naver, the nation's largest Web portal. According to the National Police Agency, the suspect, surnamed Seo, purchased the private information from a Korean-Chinese in August."^^xsd:string .

ns2:742737e0be789cf1 a ns2:BreachInformation,
        owl:NamedIndividual ;
    ns1:associatedCampaigns ns2:iiNet ;
    ns2:hasActorType "Criminal"^^xsd:string ;
    ns2:hasCountry "Australia"^^xsd:string ;
    ns2:hasEventDate "2014-01-10T00:00:00"^^xsd:dateTime ;
    ns2:hasEventSubtype "Exploitation of Application Server,Exploitation of Network Infrastructure"^^xsd:string ;
    ns2:hasEventType "Exploitive"^^xsd:string ;
    ns2:hasIndustry "Information"^^xsd:string ;
    ns2:hasMonth 1 ;
    ns2:hasOrganization "iiNet"^^xsd:string ;
    ns2:hasYear 2014 ;
    ns2:isType_of ns2:Criminal,
        ns2:Exploitation_of_Application_Server_Explo ;
    rdfs:comment "Australia's third-largest ISP, iiNet, launches a full investigation into a security breach of its TransACT network, believed to be affecting the email servers of one of its subsidiaries."^^xsd:string .

ns2:746e282b187844b9 a ns2:AnonymousAttack,
        owl:NamedIndividual ;
    ns1:associatedCampaigns ns2:Monsanto ;
    ns1:description "Protest"^^xsd:string ;
    ns2:behaviour ns2:Protest ;
    ns2:hasActor "Anonymous"^^xsd:string ;
    ns2:hasActorType "Hacktivist"^^xsd:string ;
    ns2:hasCountry "Korea (the Republic of)"^^xsd:string ;
    ns2:hasEventDate "2014-01-20T00:00:00"^^xsd:dateTime ;
    ns2:hasEventSubtype "Message Manipulation,Exploitation of Application Server"^^xsd:string ;
    ns2:hasEventType "Mixed"^^xsd:string ;
    ns2:hasIndustry "Agriculture, Forestry, Fishing and Hunting"^^xsd:string ;
    ns2:hasMonth 1 ;
    ns2:hasOrganization "Monsanto"^^xsd:string ;
    ns2:hasYear 2014 ;
    ns2:isType_of ns2:Hacktivist,
        ns2:Message_Manipulation_Exploitation_of_App ;
    rdfs:comment "The Anonymous continue the campaign called OpGreenRights. Their latest target is the South Korean website of Monsanto (monsantokorea.com), that is defaced and has some information leaked."^^xsd:string .

ns2:75461edd8a88b7e6 a ns2:BreachSecurity,
        owl:NamedIndividual ;
    ns1:associatedCampaigns ns2:Neiman_Marcus ;
    ns1:description "Financial"^^xsd:string ;
    ns2:behaviour ns2:Financial ;
    ns2:hasActorType "Criminal"^^xsd:string ;
    ns2:hasCountry "United States of America"^^xsd:string ;
    ns2:hasEventDate "2014-01-11T00:00:00"^^xsd:dateTime ;
    ns2:hasEventSubtype "Exploitation of Application Server"^^xsd:string ;
    ns2:hasEventType "Exploitive"^^xsd:string ;
    ns2:hasIndustry "Retail Trade"^^xsd:string ;
    ns2:hasMonth 1 ;
    ns2:hasOrganization "Neiman Marcus"^^xsd:string ;
    ns2:hasYear 2014 ;
    ns2:isType_of ns2:Criminal,
        ns2:Exploitation_of_Application_Server ;
    rdfs:comment "Luxury retailer Neiman Marcus admits to have suffered a data breach exposing customers' credit card information."^^xsd:string .

ns2:7743a213eda9c933 a ns2:AttackWebsite,
        owl:NamedIndividual ;
    ns1:associatedCampaigns ns2:Taj_Mahal_Website ;
    ns1:description "Protest"^^xsd:string ;
    ns1:isLaunchedBy ns2:Pakistan ;
    ns2:behaviour ns2:Protest ;
    ns2:hasActor "H4$N4!N H4XOR"^^xsd:string ;
    ns2:hasActorCountry "Pakistan"^^xsd:string ;
    ns2:hasActorType "Hacktivist"^^xsd:string ;
    ns2:hasCountry "India"^^xsd:string ;
    ns2:hasEventDate "2014-05-27T00:00:00"^^xsd:dateTime ;
    ns2:hasEventSubtype "Message Manipulation"^^xsd:string ;
    ns2:hasEventType "Disruptive"^^xsd:string ;
    ns2:hasIndustry "Public Administration"^^xsd:string ;
    ns2:hasMonth 5 ;
    ns2:hasOrganization "Taj Mahal Website"^^xsd:string ;
    ns2:hasYear 2014 ;
    ns2:isType_of ns2:Hacktivist,
        ns2:Message_Manipulation ;
    rdfs:comment "Another episode of the Cyber War between India and Pakistan, The main page of Taj Mahal website (tajmahal.gov.in) is hacked by H4$N4!N H4XOR, displaying the Pakistan's flag."^^xsd:string .

ns2:78011c7933b73974 a ns2:BreachInformation,
        owl:NamedIndividual ;
    ns1:associatedCampaigns ns2:Bulk_Reef_Supply ;
    ns1:description "Financial"^^xsd:string ;
    ns2:behaviour ns2:Financial ;
    ns2:hasActorType "Criminal"^^xsd:string ;
    ns2:hasCampaign ns2:Minnesota ;
    ns2:hasCountry "United States of America"^^xsd:string ;
    ns2:hasCounty "Hennepin"^^xsd:string ;
    ns2:hasEventDate "2014-02-27T00:00:00"^^xsd:dateTime ;
    ns2:hasEventSubtype "Exploitation of Application Server"^^xsd:string ;
    ns2:hasEventType "Exploitive"^^xsd:string ;
    ns2:hasIndustry "Retail Trade"^^xsd:string ;
    ns2:hasMonth 2 ;
    ns2:hasOrganization "Bulk Reef Supply"^^xsd:string ;
    ns2:hasState "Minnesota"^^xsd:string ;
    ns2:hasYear 2014 ;
    ns2:isType_of ns2:Criminal,
        ns2:Exploitation_of_Application_Server ;
    rdfs:comment "Saltwater aquarium supplies seller Bulk Reef Supply (bulkreefsupply.com) announces that its website was compromised for about six months, and the company is notifying an undisclosed number of customers that their personal data, including credit card information, may have been compromised."^^xsd:string .

ns2:7840d49c33002279 a ns2:CyberattackData,
        owl:NamedIndividual ;
    ns1:associatedCampaigns ns2:Embassy_of_India_in_Russia ;
    ns1:description "Protest"^^xsd:string ;
    ns2:behaviour ns2:Protest ;
    ns2:hasActor "@Rucyborg"^^xsd:string ;
    ns2:hasActorType "Hacktivist"^^xsd:string ;
    ns2:hasCountry "India"^^xsd:string ;
    ns2:hasEventDate "2014-03-06T00:00:00"^^xsd:dateTime ;
    ns2:hasEventSubtype "Exploitation of Application Server"^^xsd:string ;
    ns2:hasEventType "Exploitive"^^xsd:string ;
    ns2:hasIndustry "Public Administration"^^xsd:string ;
    ns2:hasMonth 3 ;
    ns2:hasOrganization "Embassy of India in Russia"^^xsd:string ;
    ns2:hasYear 2014 ;
    ns2:isType_of ns2:Exploitation_of_Application_Server,
        ns2:Hacktivist ;
    rdfs:comment "The Russian CyberCommand (AKA @Rucyborg) hacks the Indian Embassy in Moscow leaking documents detailing Rosoboronexport's sales to India."^^xsd:string .

ns2:7855bd0f8be0d51d a ns2:HackerSecurity,
        owl:NamedIndividual ;
    ns1:associatedCampaigns ns2:Certification_ESET_Spain ;
    ns2:hasActor "Hmei7"^^xsd:string ;
    ns2:hasActorType "Hobbyist"^^xsd:string ;
    ns2:hasCountry "Spain"^^xsd:string ;
    ns2:hasEventDate "2014-06-04T00:00:00"^^xsd:dateTime ;
    ns2:hasEventSubtype "Message Manipulation"^^xsd:string ;
    ns2:hasEventType "Disruptive"^^xsd:string ;
    ns2:hasIndustry "Professional, Scientific, and Technical Services"^^xsd:string ;
    ns2:hasMonth 6 ;
    ns2:hasOrganization "Certification ESET Spain"^^xsd:string ;
    ns2:hasYear 2014 ;
    ns2:isType_of ns2:Hobbyist,
        ns2:Message_Manipulation ;
    rdfs:comment "A hacker called Hmeidefaces the official website of ESETand 4 of itsSpanish domains."^^xsd:string .

ns2:7885f9b77bdb9cad a ns2:AttackWebsite,
        owl:NamedIndividual ;
    ns1:associatedCampaigns ns2:Bangladesh_Airport_Armed_Police ;
    ns1:isLaunchedBy ns2:Nigeria ;
    ns2:hasActor "Nigerian Cyber Hunters"^^xsd:string ;
    ns2:hasActorCountry "Nigeria"^^xsd:string ;
    ns2:hasCountry "Bangladesh"^^xsd:string ;
    ns2:hasEventDate "2014-08-25T00:00:00"^^xsd:dateTime ;
    ns2:hasEventSubtype "Message Manipulation"^^xsd:string ;
    ns2:hasEventType "Disruptive"^^xsd:string ;
    ns2:hasIndustry "Public Administration"^^xsd:string ;
    ns2:hasMonth 8 ;
    ns2:hasOrganization "Bangladesh Airport Armed Police"^^xsd:string ;
    ns2:hasYear 2014 ;
    ns2:isType_of ns2:Message_Manipulation ;
    rdfs:comment "Nigerian Hackers from Nigerian Cyber Hunters (NCH) deface the official website of Bangladesh Airport Armed Police (aap.gov.bd)."^^xsd:string .

ns2:78ebedfc85a6a17c a ns2:CyberattackInformation,
        owl:NamedIndividual ;
    ns1:associatedCampaigns ns2:Israel_Defense ;
    ns1:isLaunchedBy ns2:Palestine__State_of ;
    ns2:hasActor "HAMAS"^^xsd:string ;
    ns2:hasActorCountry "Palestine, State of"^^xsd:string ;
    ns2:hasActorType "Terrorist"^^xsd:string ;
    ns2:hasCountry "Israel"^^xsd:string ;
    ns2:hasEventDate "2014-03-22T00:00:00"^^xsd:dateTime ;
    ns2:hasEventSubtype "Message Manipulation"^^xsd:string ;
    ns2:hasEventType "Disruptive"^^xsd:string ;
    ns2:hasIndustry "Information"^^xsd:string ;
    ns2:hasMonth 3 ;
    ns2:hasOrganization "Israel Defense"^^xsd:string ;
    ns2:hasYear 2014 ;
    ns2:isType_of ns2:Message_Manipulation,
        ns2:Terrorist ;
    rdfs:comment "Hamas activists hack into the news website Israel Defense and also flood  many Israeli cell phone users with text messages threatening them with Qassam rockets or kidnappings."^^xsd:string .

ns2:798d243a0112e169 a ns2:AnonymousAttack,
        owl:NamedIndividual ;
    ns1:associatedCampaigns ns2:Federal_Police_of_Brazil ;
    ns1:description "Protest"^^xsd:string ;
    ns2:behaviour ns2:Protest ;
    ns2:hasActor "Anonymous"^^xsd:string ;
    ns2:hasActorType "Hacktivist"^^xsd:string ;
    ns2:hasCountry "Brazil"^^xsd:string ;
    ns2:hasEventDate "2014-06-17T00:00:00"^^xsd:dateTime ;
    ns2:hasEventSubtype "Exploitation of Application Server"^^xsd:string ;
    ns2:hasEventType "Exploitive"^^xsd:string ;
    ns2:hasIndustry "Arts, Entertainment, and Recreation"^^xsd:string ;
    ns2:hasMonth 6 ;
    ns2:hasOrganization "Federal Police of Brazil"^^xsd:string ;
    ns2:hasYear 2014 ;
    ns2:isType_of ns2:Exploitation_of_Application_Server,
        ns2:Hacktivist ;
    rdfs:comment "As part of #OpWorldCup and #OpHackingCup, Anonymous hacks a number of Brazilian organizations during the World Cup. "^^xsd:string .

ns2:79fa7d3ff14f2e1c a ns2:DDoS,
        owl:NamedIndividual ;
    ns1:associatedCampaigns ns2:EA_com ;
    ns2:hasActor "DERP Trolling"^^xsd:string ;
    ns2:hasCampaign ns2:California ;
    ns2:hasCountry "United States of America"^^xsd:string ;
    ns2:hasCounty "San Mateo"^^xsd:string ;
    ns2:hasEventDate "2014-01-03T00:00:00"^^xsd:dateTime ;
    ns2:hasEventSubtype "External Denial of Service"^^xsd:string ;
    ns2:hasEventType "Disruptive"^^xsd:string ;
    ns2:hasIndustry "Information"^^xsd:string ;
    ns2:hasMonth 1 ;
    ns2:hasOrganization "EA.com"^^xsd:string ;
    ns2:hasState "California"^^xsd:string ;
    ns2:hasYear 2014 ;
    ns2:isType_of ns2:External_Denial_of_Service ;
    rdfs:comment "The servers for Steam, Origin, Battle.net, and League of Legends are brought down temporarily by apparent DDoS attacks that seem to be related to a swatting attack on an individual known for streaming games."^^xsd:string .

ns2:7a09cc87eb4b9ef7 a ns2:HackerSecurity,
        owl:NamedIndividual ;
    ns1:associatedCampaigns ns2:CNET ;
    ns1:description "Financial"^^xsd:string ;
    ns1:isLaunchedBy ns2:Russian_Federation ;
    ns2:behaviour ns2:Financial ;
    ns2:hasActor "W0rm"^^xsd:string ;
    ns2:hasActorCountry "Russian Federation"^^xsd:string ;
    ns2:hasActorType "Criminal"^^xsd:string ;
    ns2:hasCampaign ns2:California ;
    ns2:hasCountry "United States of America"^^xsd:string ;
    ns2:hasCounty "San Francisco"^^xsd:string ;
    ns2:hasEventDate "2014-07-14T00:00:00"^^xsd:dateTime ;
    ns2:hasEventSubtype "Exploitation of Application Server"^^xsd:string ;
    ns2:hasEventType "Exploitive"^^xsd:string ;
    ns2:hasIndustry "Information"^^xsd:string ;
    ns2:hasMonth 7 ;
    ns2:hasOrganization "CNET"^^xsd:string ;
    ns2:hasState "California"^^xsd:string ;
    ns2:hasYear 2014 ;
    ns2:isType_of ns2:Criminal,
        ns2:Exploitation_of_Application_Server ;
    rdfs:comment "A Russian hacker group calling itself W0rm claims to have penetrated CNET's website stealing a database of registered reader data (1 million users). Hackers demand 1 bitcoin."^^xsd:string .

ns2:7ade9c019cd40d6d a ns2:CyberattackData,
        owl:NamedIndividual ;
    ns1:associatedCampaigns ns2:eBay ;
    ns2:hasActorType "Criminal"^^xsd:string ;
    ns2:hasCampaign ns2:California ;
    ns2:hasCountry "United States of America"^^xsd:string ;
    ns2:hasCounty "Santa Clara"^^xsd:string ;
    ns2:hasEventDate "2014-05-21T00:00:00"^^xsd:dateTime ;
    ns2:hasEventSubtype "Exploitation of Application Server"^^xsd:string ;
    ns2:hasEventType "Exploitive"^^xsd:string ;
    ns2:hasIndustry "Retail Trade"^^xsd:string ;
    ns2:hasMonth 5 ;
    ns2:hasOrganization "eBay"^^xsd:string ;
    ns2:hasState "California"^^xsd:string ;
    ns2:hasYear 2014 ;
    ns2:isType_of ns2:Criminal,
        ns2:Exploitation_of_Application_Server ;
    rdfs:comment "eBay revealsÃ'ÃÂ that attackers \"compromised a database containing encrypted passwords and other non-financial data\" between late February and early March. The database included names, e-mail addresses, home addresses, phone numbers, and dates of birth. "^^xsd:string .

ns2:7b47d05fbd4c26be a ns2:AnonymousAttack,
        owl:NamedIndividual ;
    ns1:associatedCampaigns ns2:Kenyan_Defence_Forces ;
    ns1:description "Protest"^^xsd:string ;
    ns2:behaviour ns2:Protest ;
    ns2:hasActor "Anonymous"^^xsd:string ;
    ns2:hasActorType "Hacktivist"^^xsd:string ;
    ns2:hasCountry "Kenya"^^xsd:string ;
    ns2:hasEventDate "2014-07-21T00:00:00"^^xsd:dateTime ;
    ns2:hasEventSubtype "Message Manipulation"^^xsd:string ;
    ns2:hasEventType "Disruptive"^^xsd:string ;
    ns2:hasIndustry "Public Administration"^^xsd:string ;
    ns2:hasMonth 7 ;
    ns2:hasOrganization "Kenyan Defence Forces"^^xsd:string ;
    ns2:hasYear 2014 ;
    ns2:isType_of ns2:Hacktivist,
        ns2:Message_Manipulation ;
    rdfs:comment "The Twitter accounts of the Kenyan Defence Forces (@kdfinfo) and its spokesman are hacked by activists claiming to be affiliated to Anonymous (Anon_0x03), to protest against  corruption."^^xsd:string .

ns2:7babf58c07b56912 a ns2:BreachInformation,
        owl:NamedIndividual ;
    ns1:associatedCampaigns ns2:wirelessemporium_com ;
    ns1:description "Financial"^^xsd:string ;
    ns2:behaviour ns2:Financial ;
    ns2:hasActorType "Criminal"^^xsd:string ;
    ns2:hasCampaign ns2:California ;
    ns2:hasCountry "United States of America"^^xsd:string ;
    ns2:hasCounty "Orange"^^xsd:string ;
    ns2:hasEventDate "2014-08-05T00:00:00"^^xsd:dateTime ;
    ns2:hasEventSubtype "Exploitation of Application Server"^^xsd:string ;
    ns2:hasEventType "Exploitive"^^xsd:string ;
    ns2:hasIndustry "Retail Trade"^^xsd:string ;
    ns2:hasMonth 8 ;
    ns2:hasOrganization "wirelessemporium.com"^^xsd:string ;
    ns2:hasState "California"^^xsd:string ;
    ns2:hasYear 2014 ;
    ns2:isType_of ns2:Criminal,
        ns2:Exploitation_of_Application_Server ;
    rdfs:comment "After a malware is discovered on wirelessemporium.com, the company begins notifying an undisclosed number of individuals that their personal information, including payment card data, might have been compromised."^^xsd:string .

ns2:7c56c469593d3f7f a ns2:AttackWebsite,
        owl:NamedIndividual ;
    ns1:associatedCampaigns ns2:Alshariq_Principality ;
    ns1:description "Protest"^^xsd:string ;
    ns1:isLaunchedBy ns2:Syrian_Arab_Republic ;
    ns2:behaviour ns2:Protest ;
    ns2:hasActor "Syrian Electronic Army"^^xsd:string ;
    ns2:hasActorCountry "Syrian Arab Republic"^^xsd:string ;
    ns2:hasActorType "Hacktivist"^^xsd:string ;
    ns2:hasCountry "Saudi Arabia"^^xsd:string ;
    ns2:hasEventDate "2014-01-16T00:00:00"^^xsd:dateTime ;
    ns2:hasEventSubtype "Message Manipulation"^^xsd:string ;
    ns2:hasEventType "Disruptive"^^xsd:string ;
    ns2:hasIndustry "Public Administration"^^xsd:string ;
    ns2:hasMonth 1 ;
    ns2:hasOrganization "Alshariq Principality"^^xsd:string ;
    ns2:hasYear 2014 ;
    ns2:isType_of ns2:Hacktivist,
        ns2:Message_Manipulation ;
    rdfs:comment "The Syrian Electronic Army deface 16 Saudi Arabian government websites. The targeted sites are the ones of various administrative regions."^^xsd:string .

ns2:7c95df2405dcd262 a ns1:BotnetAttack,
        owl:NamedIndividual ;
    ns1:associatedCampaigns ns2:Network_Information_Center_of_Paraguay ;
    ns1:isLaunchedBy ns2:Iran__Islamic_Republic_of ;
    ns2:hasActor "Mormoroth"^^xsd:string ;
    ns2:hasActorCountry "Iran (Islamic Republic of)"^^xsd:string ;
    ns2:hasActorType "Hacktivist"^^xsd:string ;
    ns2:hasCountry "Paraguay"^^xsd:string ;
    ns2:hasEventDate "2014-02-25T00:00:00"^^xsd:dateTime ;
    ns2:hasEventSubtype "Message Manipulation"^^xsd:string ;
    ns2:hasEventType "Disruptive"^^xsd:string ;
    ns2:hasIndustry "Professional, Scientific, and Technical Services"^^xsd:string ;
    ns2:hasMonth 2 ;
    ns2:hasOrganization "Network Information Center of Paraguay"^^xsd:string ;
    ns2:hasYear 2014 ;
    ns2:isType_of ns2:Hacktivist,
        ns2:Message_Manipulation ;
    rdfs:comment "An Iranian hacker calling himself Mormoroth hacks the systems of the Network Information Center of Paraguay (nic.py), hijacking the DNS entries of Google Paraguay (google.com.py)."^^xsd:string .

ns2:7cad5a23688bdd6b a ns2:HackerSecurity,
        owl:NamedIndividual ;
    ns1:associatedCampaigns ns2:Code_Spaces ;
    ns1:description "Financial"^^xsd:string ;
    ns2:behaviour ns2:Financial ;
    ns2:hasActorType "Criminal"^^xsd:string ;
    ns2:hasCountry "United States of America"^^xsd:string ;
    ns2:hasEventDate "2014-06-18T00:00:00"^^xsd:dateTime ;
    ns2:hasEventSubtype "Data Attack,External Denial of Service"^^xsd:string ;
    ns2:hasEventType "Disruptive"^^xsd:string ;
    ns2:hasIndustry "Information"^^xsd:string ;
    ns2:hasMonth 6 ;
    ns2:hasOrganization "Code Spaces"^^xsd:string ;
    ns2:hasYear 2014 ;
    ns2:isType_of ns2:Criminal,
        ns2:Data_Attack_External_Denial_of_Service ;
    rdfs:comment "Code Spaces, a code-hosting service  abruptly closes after someone gains unauthorized access to its Amazon Web Service account and deletes most of the customer data. The company refused to pay a ransom after being extorted via a DDoS attack."^^xsd:string .

ns2:7d3649d43e6b1fd0 a ns2:BreachSecurity,
        owl:NamedIndividual ;
    ns1:associatedCampaigns ns2:USIS ;
    ns1:description "Political-Espionage"^^xsd:string ;
    ns2:behaviour ns2:Political_Espionage ;
    ns2:hasActorType "Criminal"^^xsd:string ;
    ns2:hasCampaign ns2:Virginia ;
    ns2:hasCountry "United States of America"^^xsd:string ;
    ns2:hasCounty "Loudoun"^^xsd:string ;
    ns2:hasEventDate "2014-08-06T00:00:00"^^xsd:dateTime ;
    ns2:hasEventSubtype "Exploitation of Application Server"^^xsd:string ;
    ns2:hasEventType "Exploitive"^^xsd:string ;
    ns2:hasIndustry "Administrative and Support and Waste Management and Remediation Services"^^xsd:string ;
    ns2:hasMonth 8 ;
    ns2:hasOrganization "USIS"^^xsd:string ;
    ns2:hasState "Virginia"^^xsd:string ;
    ns2:hasYear 2014 ;
    ns2:isType_of ns2:Criminal,
        ns2:Exploitation_of_Application_Server ;
    rdfs:comment "USIS, a major US contractor that conducts background checks for the Department of Homeland Security suffers a computer breach that probably resulted in the theft of employees' personal information. The breach is believed to be related to the Office of Personnel Management hack."^^xsd:string .

ns2:7deb93a8ef656b50 a ns2:AccountAttack,
        owl:NamedIndividual ;
    ns1:associatedCampaigns ns2:BigMoneyJobs_com ;
    ns2:hasActor "ProbablyOnion"^^xsd:string ;
    ns2:hasCountry "United States of America"^^xsd:string ;
    ns2:hasEventDate "2014-04-02T00:00:00"^^xsd:dateTime ;
    ns2:hasEventSubtype "Exploitation of Application Server"^^xsd:string ;
    ns2:hasEventType "Exploitive"^^xsd:string ;
    ns2:hasIndustry "Administrative and Support and Waste Management and Remediation Services"^^xsd:string ;
    ns2:hasMonth 4 ;
    ns2:hasOrganization "BigMoneyJobs.com"^^xsd:string ;
    ns2:hasYear 2014 ;
    ns2:isType_of ns2:Exploitation_of_Application_Server ;
    rdfs:comment "ProbablyOnion hacks a job seeker website (bigmoneyjobs.com) and dumps over 36,000 accounts online."^^xsd:string .

ns2:7e2ce295cdd16184 a ns2:CyberattackSystem,
        owl:NamedIndividual ;
    ns1:associatedCampaigns ns2:Pakistan_National_Portal ;
    ns1:isLaunchedBy ns2:Pakistan ;
    ns2:hasActor "Bl@Ck Dr@GoN; Haxor T0du; Spider64"^^xsd:string ;
    ns2:hasActorCountry "Pakistan"^^xsd:string ;
    ns2:hasActorType "Hacktivist"^^xsd:string ;
    ns2:hasCountry "Pakistan"^^xsd:string ;
    ns2:hasEventDate "2014-04-25T00:00:00"^^xsd:dateTime ;
    ns2:hasEventSubtype "Message Manipulation"^^xsd:string ;
    ns2:hasEventType "Disruptive"^^xsd:string ;
    ns2:hasIndustry "Public Administration"^^xsd:string ;
    ns2:hasMonth 4 ;
    ns2:hasOrganization "Pakistan National Portal"^^xsd:string ;
    ns2:hasYear 2014 ;
    ns2:isType_of ns2:Hacktivist,
        ns2:Message_Manipulation ;
    rdfs:comment "The cyber battle between Indian and Pakistani hacktivists continues. In name of OpPakistan Indian hackers deface several Pakistani government websites."^^xsd:string .

ns2:7e5bf588837171e7 a ns2:AnonymousAttack,
        owl:NamedIndividual ;
    ns1:associatedCampaigns ns2:Centrais_El_tricas_do_Norte_do_Brasil ;
    ns1:description "Protest"^^xsd:string ;
    ns2:behaviour ns2:Protest ;
    ns2:hasActor "Anonymous"^^xsd:string ;
    ns2:hasActorType "Hacktivist"^^xsd:string ;
    ns2:hasCountry "Brazil"^^xsd:string ;
    ns2:hasEventDate "2014-06-17T00:00:00"^^xsd:dateTime ;
    ns2:hasEventSubtype "Exploitation of Application Server"^^xsd:string ;
    ns2:hasEventType "Exploitive"^^xsd:string ;
    ns2:hasIndustry "Utilities"^^xsd:string ;
    ns2:hasMonth 6 ;
    ns2:hasOrganization "Centrais El tricas do Norte do Brasil"^^xsd:string ;
    ns2:hasYear 2014 ;
    ns2:isType_of ns2:Exploitation_of_Application_Server,
        ns2:Hacktivist ;
    rdfs:comment "As part of #OpWorldCup and #OpHackingCup, Anonymous hacks a number of Brazilian organizations during the World Cup. "^^xsd:string .

ns2:7e5ed3f76a70db21 a ns2:CyberattackData,
        owl:NamedIndividual ;
    ns1:associatedCampaigns ns2:Department_of_Culture__Media_and_Sport ;
    ns1:description "Protest"^^xsd:string ;
    ns2:behaviour ns2:Protest ;
    ns2:hasActorType "Criminal"^^xsd:string ;
    ns2:hasCountry "United Kingdom of Great Britain and Northern Ireland"^^xsd:string ;
    ns2:hasEventDate "2014-04-07T00:00:00"^^xsd:dateTime ;
    ns2:hasEventSubtype "Message Manipulation"^^xsd:string ;
    ns2:hasEventType "Disruptive"^^xsd:string ;
    ns2:hasIndustry "Public Administration"^^xsd:string ;
    ns2:hasMonth 4 ;
    ns2:hasOrganization "Department of Culture, Media and Sport"^^xsd:string ;
    ns2:hasYear 2014 ;
    ns2:isType_of ns2:Criminal,
        ns2:Message_Manipulation ;
    rdfs:comment "The verified Twitter account of the United Kingdom's Department of Culture, Media and Sport (@DCMS) is hacked over the weekend. The hacker posts three messages referencing MP Maria Miller on the compromised feed."^^xsd:string .

ns2:7f01a9f94efc2ac1 a ns2:AccessSecurity,
        owl:NamedIndividual ;
    ns1:associatedCampaigns ns2:PharmaNet ;
    ns2:hasActorType "Criminal"^^xsd:string ;
    ns2:hasCountry "Canada"^^xsd:string ;
    ns2:hasEventDate "2014-07-11T00:00:00"^^xsd:dateTime ;
    ns2:hasEventSubtype "Exploitation of Application Server"^^xsd:string ;
    ns2:hasEventType "Exploitive"^^xsd:string ;
    ns2:hasIndustry "Public Administration"^^xsd:string ;
    ns2:hasMonth 7 ;
    ns2:hasOrganization "PharmaNet"^^xsd:string ;
    ns2:hasYear 2014 ;
    ns2:isType_of ns2:Criminal,
        ns2:Exploitation_of_Application_Server ;
    rdfs:comment "1,600 names, dates of birth, phone numbers, addresses, and personal health numbers are accessed by an unauthorized individual using a doctor's PharmaNet account."^^xsd:string .

ns2:7f0eabc1a027d85d a ns2:AttackWebsite,
        owl:NamedIndividual ;
    ns1:associatedCampaigns ns2:Israeli_Embassy_for_Uzbekistan ;
    ns1:description "Protest"^^xsd:string ;
    ns2:behaviour ns2:Protest ;
    ns2:hasActor "Dr.SHA6H"^^xsd:string ;
    ns2:hasActorType "Hacktivist"^^xsd:string ;
    ns2:hasCountry "Israel"^^xsd:string ;
    ns2:hasEventDate "2014-08-30T00:00:00"^^xsd:dateTime ;
    ns2:hasEventSubtype "Message Manipulation"^^xsd:string ;
    ns2:hasEventType "Disruptive"^^xsd:string ;
    ns2:hasIndustry "Public Administration"^^xsd:string ;
    ns2:hasMonth 8 ;
    ns2:hasOrganization "Israeli Embassy for Uzbekistan"^^xsd:string ;
    ns2:hasYear 2014 ;
    ns2:isType_of ns2:Hacktivist,
        ns2:Message_Manipulation ;
    rdfs:comment "An anti-Assad Syrian Ã'ÃÂ hacker going with the handle of Dr.SHA6H defaces the official website of Israeli Embassy for Uzbekistan (israelbiz.uz) in solidarity with Palestine."^^xsd:string .

ns2:7f43e545442f6c21 a ns2:AnonymousAttack,
        owl:NamedIndividual ;
    ns1:associatedCampaigns ns2:Website_of_the_Israeli_Prime_Minister ;
    ns1:description "Protest"^^xsd:string ;
    ns2:behaviour ns2:Protest ;
    ns2:hasActor "Anonymous"^^xsd:string ;
    ns2:hasActorType "Hacktivist"^^xsd:string ;
    ns2:hasCountry "Israel"^^xsd:string ;
    ns2:hasEventDate "2014-08-25T00:00:00"^^xsd:dateTime ;
    ns2:hasEventSubtype "External Denial of Service"^^xsd:string ;
    ns2:hasEventType "Disruptive"^^xsd:string ;
    ns2:hasIndustry "Public Administration"^^xsd:string ;
    ns2:hasMonth 8 ;
    ns2:hasOrganization "Website of the Israeli Prime Minister"^^xsd:string ;
    ns2:hasYear 2014 ;
    ns2:isType_of ns2:External_Denial_of_Service,
        ns2:Hacktivist ;
    rdfs:comment "In name of #OpSaveGaza, the Anonymous collective claims to have taken down some key Israeli governmental websites, including those of the Israeli Defense Forces, the Bank of Israel, the Israeli Prime Minister."^^xsd:string .

ns2:7f5afa38d82f70c7 a ns2:CyberattackInformation,
        owl:NamedIndividual ;
    ns1:associatedCampaigns ns2:US_Army ;
    ns2:hasActorType "Criminal"^^xsd:string ;
    ns2:hasCountry "United States of America"^^xsd:string ;
    ns2:hasEventDate "2014-06-06T00:00:00"^^xsd:dateTime ;
    ns2:hasEventSubtype "Exploitation of Application Server"^^xsd:string ;
    ns2:hasEventType "Exploitive"^^xsd:string ;
    ns2:hasIndustry "Public Administration"^^xsd:string ;
    ns2:hasMonth 6 ;
    ns2:hasOrganization "US Army"^^xsd:string ;
    ns2:hasYear 2014 ;
    ns2:isType_of ns2:Criminal,
        ns2:Exploitation_of_Application_Server ;
    rdfs:comment "The US Army warns that databases holding information on 16,000 South Korean civilian employees of the US military and applicants for base jobs may have been compromised."^^xsd:string .

ns2:7fca8172c231dae6 a ns2:AttackSchool,
        owl:NamedIndividual ;
    ns1:associatedCampaigns ns2:College_in_Shanghai_s_Songjiang_District ;
    ns2:hasActor "Two Students"^^xsd:string ;
    ns2:hasActorType "Hobbyist"^^xsd:string ;
    ns2:hasCountry "China"^^xsd:string ;
    ns2:hasEventDate "2014-03-08T00:00:00"^^xsd:dateTime ;
    ns2:hasEventSubtype "Data Attack"^^xsd:string ;
    ns2:hasEventType "Disruptive"^^xsd:string ;
    ns2:hasIndustry "Educational Services"^^xsd:string ;
    ns2:hasMonth 3 ;
    ns2:hasOrganization "College in Shanghai's Songjiang District"^^xsd:string ;
    ns2:hasYear 2014 ;
    ns2:isType_of ns2:Data_Attack,
        ns2:Hobbyist ;
    rdfs:comment "Two students at a college in Shanghai's Songjiang District are arrested for allegedly changing grades for 200 of their colleagues."^^xsd:string .

ns2:807af42881024f01 a ns2:AnonymousAttack,
        owl:NamedIndividual ;
    ns1:associatedCampaigns ns2:Cemig_Telecom ;
    ns1:description "Protest"^^xsd:string ;
    ns2:behaviour ns2:Protest ;
    ns2:hasActor "Anonymous"^^xsd:string ;
    ns2:hasActorType "Hacktivist"^^xsd:string ;
    ns2:hasCountry "Brazil"^^xsd:string ;
    ns2:hasEventDate "2014-06-17T00:00:00"^^xsd:dateTime ;
    ns2:hasEventSubtype "Exploitation of Application Server"^^xsd:string ;
    ns2:hasEventType "Exploitive"^^xsd:string ;
    ns2:hasIndustry "Information"^^xsd:string ;
    ns2:hasMonth 6 ;
    ns2:hasOrganization "Cemig Telecom"^^xsd:string ;
    ns2:hasYear 2014 ;
    ns2:isType_of ns2:Exploitation_of_Application_Server,
        ns2:Hacktivist ;
    rdfs:comment "As part of #OpWorldCup and #OpHackingCup, Anonymous hacks a number of Brazilian organizations during the World Cup. "^^xsd:string .

ns2:8088a15c8ed5acc4 a ns2:DDoS,
        owl:NamedIndividual ;
    ns1:associatedCampaigns ns2:What_cd ;
    ns2:hasActorType "Criminal"^^xsd:string ;
    ns2:hasEventDate "2014-01-06T00:00:00"^^xsd:dateTime ;
    ns2:hasEventSubtype "External Denial of Service"^^xsd:string ;
    ns2:hasEventType "Disruptive"^^xsd:string ;
    ns2:hasIndustry "Other Services (except Public Administration)"^^xsd:string ;
    ns2:hasMonth 1 ;
    ns2:hasOrganization "What.cd"^^xsd:string ;
    ns2:hasYear 2014 ;
    ns2:isType_of ns2:Criminal,
        ns2:External_Denial_of_Service ;
    rdfs:comment "Three of the largest private BitTorrent trackers are offline due to prolonged DDoS attacks. The targets are: What.cd, Broadcasthe.net, PassthePopcorn.me."^^xsd:string .

ns2:8139a43a3fc3b8c5 a ns2:AccountAttack,
        owl:NamedIndividual ;
    ns1:associatedCampaigns ns2:MyCause ;
    ns1:description "Financial"^^xsd:string ;
    ns2:behaviour ns2:Financial ;
    ns2:hasActorType "Criminal"^^xsd:string ;
    ns2:hasCountry "Australia"^^xsd:string ;
    ns2:hasEventDate "2014-08-01T00:00:00"^^xsd:dateTime ;
    ns2:hasEventSubtype "Exploitation of Application Server"^^xsd:string ;
    ns2:hasEventType "Exploitive"^^xsd:string ;
    ns2:hasIndustry "Other Services (except Public Administration)"^^xsd:string ;
    ns2:hasMonth 8 ;
    ns2:hasOrganization "MyCause"^^xsd:string ;
    ns2:hasYear 2014 ;
    ns2:isType_of ns2:Criminal,
        ns2:Exploitation_of_Application_Server ;
    rdfs:comment "Up to 12,000 people donating to charities through the Australian website mycause.com.au have their credit card details stolen and used for thousands of dollars worth of fraudulent charges."^^xsd:string .

ns2:816c06f1ff88dd3d a ns2:HackerSecurity,
        owl:NamedIndividual ;
    ns1:associatedCampaigns ns2:Ohio_State_Government ;
    ns1:isLaunchedBy ns2:United_States_of_America ;
    ns2:hasActor "Rajol Hazin"^^xsd:string ;
    ns2:hasActorCountry "United States of America"^^xsd:string ;
    ns2:hasActorType "Hacktivist"^^xsd:string ;
    ns2:hasCampaign ns2:Ohio ;
    ns2:hasCountry "United States of America"^^xsd:string ;
    ns2:hasCounty "Franklin"^^xsd:string ;
    ns2:hasEventDate "2014-08-17T00:00:00"^^xsd:dateTime ;
    ns2:hasEventSubtype "Message Manipulation"^^xsd:string ;
    ns2:hasEventType "Disruptive"^^xsd:string ;
    ns2:hasIndustry "Public Administration"^^xsd:string ;
    ns2:hasMonth 8 ;
    ns2:hasOrganization "Ohio State Government"^^xsd:string ;
    ns2:hasState "Ohio"^^xsd:string ;
    ns2:hasYear 2014 ;
    ns2:isType_of ns2:Hacktivist,
        ns2:Message_Manipulation ;
    rdfs:comment "A hacker going with the handle of Rajol Hazin defaces the official sub-domain of Ohio State Government (bta.ohio.gov)."^^xsd:string .

ns2:81761c586d02db79 a ns2:BreachSecurity,
        owl:NamedIndividual ;
    ns1:associatedCampaigns ns2:Cerberus ;
    ns2:hasActorType "Criminal"^^xsd:string ;
    ns2:hasCountry "Italy"^^xsd:string ;
    ns2:hasEventDate "2014-03-28T00:00:00"^^xsd:dateTime ;
    ns2:hasEventSubtype "Exploitation of Application Server"^^xsd:string ;
    ns2:hasEventType "Exploitive"^^xsd:string ;
    ns2:hasIndustry "Information"^^xsd:string ;
    ns2:hasMonth 3 ;
    ns2:hasOrganization "Cerberus"^^xsd:string ;
    ns2:hasYear 2014 ;
    ns2:isType_of ns2:Criminal,
        ns2:Exploitation_of_Application_Server ;
    rdfs:comment "Over 96,000 users of the Cerberus anti-theft application for Android are advised to change their passwords after the company suffered a data breach."^^xsd:string .

ns2:817c6ca4b434c1ac a ns2:Phishing,
        owl:NamedIndividual ;
    ns1:associatedCampaigns ns2:eBay ;
    ns1:description "Protest"^^xsd:string ;
    ns1:isLaunchedBy ns2:Syrian_Arab_Republic ;
    ns2:behaviour ns2:Protest ;
    ns2:hasActor "Syrian Electronic Army"^^xsd:string ;
    ns2:hasActorCountry "Syrian Arab Republic"^^xsd:string ;
    ns2:hasActorType "Hacktivist"^^xsd:string ;
    ns2:hasCountry "India"^^xsd:string ;
    ns2:hasEventDate "2014-02-05T00:00:00"^^xsd:dateTime ;
    ns2:hasEventSubtype "Exploitation of End Hosts"^^xsd:string ;
    ns2:hasEventType "Exploitive"^^xsd:string ;
    ns2:hasIndustry "Retail Trade"^^xsd:string ;
    ns2:hasMonth 2 ;
    ns2:hasOrganization "eBay"^^xsd:string ;
    ns2:hasYear 2014 ;
    ns2:isType_of ns2:Exploitation_of_End_Hosts,
        ns2:Hacktivist ;
    rdfs:comment "Hackers have compromised the eBay and PayPal marketing webpages in the UK, France, and India, causing some visitors to be redirected to fraudulent destinations."^^xsd:string .

ns2:81db842bdfff3a3d a ns2:HackerSecurity,
        owl:NamedIndividual ;
    ns1:associatedCampaigns ns2:Meteo_France__meteofrance_com ;
    ns1:isLaunchedBy ns2:Mexico ;
    ns2:hasActor "Amar^SHG"^^xsd:string ;
    ns2:hasActorCountry "Mexico"^^xsd:string ;
    ns2:hasActorType "Hacktivist"^^xsd:string ;
    ns2:hasCountry "France"^^xsd:string ;
    ns2:hasEventDate "2016-05-23T00:00:00"^^xsd:dateTime ;
    ns2:hasEventSubtype "Message Manipulation"^^xsd:string ;
    ns2:hasEventType "Disruptive"^^xsd:string ;
    ns2:hasIndustry "Professional, Scientific, and Technical Services"^^xsd:string ;
    ns2:hasMonth 5 ;
    ns2:hasOrganization "Meteo France (meteofrance.com)"^^xsd:string ;
    ns2:hasYear 2016 ;
    ns2:isType_of ns2:Hacktivist,
        ns2:Message_Manipulation ;
    rdfs:comment "A hacker who goes by the nickname ofÃÆÃ'Ãâ 'ÃÆÃ¢â¬Â 'ÃÆÃ'ÃÂ¢Ã¢'Â¬ÃÂ ''ÃÆÃ'Ãâ 'ÃÆÃ¢â¬Â ''ÃÆÃ'Ãâ ''ÃÆÃ''ÃÆ'Ã'ÃÂ Amar^SHG (formerly Kuroi'SH) defaces France's most visited weather portal, MÃÆÃ'Ãâ 'ÃÆÃ¢â¬Â 'ÃÆÃ'ÃÂ¢Ã¢'Â¬ÃÂ 'ÃÆÃ'Ãâ 'ÃÆÃÂ¢ÃÂ¢'ÃÂ¬Ã'ÃÂ 'ÃÆÃ'Ãâ 'ÃÆÃ¢â¬Â ''ÃÆÃ'Ãâ ''ÃÆÃ''ÃÆ'Ã'ÃÂ©tÃÆÃ'Ãâ 'ÃÆÃ¢â¬Â 'ÃÆÃ'ÃÂ¢Ã¢'Â¬ÃÂ 'ÃÆÃ'Ãâ 'ÃÆÃÂ¢ÃÂ¢'ÃÂ¬Ã'ÃÂ 'ÃÆÃ'Ãâ 'ÃÆÃ¢â¬Â ''ÃÆÃ'Ãâ ''ÃÆÃ''ÃÆ'Ã'ÃÂ©o France."^^xsd:string .

ns2:820dcd35acd7671b a ns2:EmailPhishing,
        owl:NamedIndividual ;
    ns1:associatedCampaigns ns2:AOL_Mail ;
    ns1:description "Financial"^^xsd:string ;
    ns2:behaviour ns2:Financial ;
    ns2:hasActorType "Criminal"^^xsd:string ;
    ns2:hasCampaign ns2:New_York ;
    ns2:hasCountry "United States of America"^^xsd:string ;
    ns2:hasCounty "New York"^^xsd:string ;
    ns2:hasEventDate "2014-04-28T00:00:00"^^xsd:dateTime ;
    ns2:hasEventSubtype "Exploitation of Application Server"^^xsd:string ;
    ns2:hasEventType "Exploitive"^^xsd:string ;
    ns2:hasIndustry "Information"^^xsd:string ;
    ns2:hasMonth 4 ;
    ns2:hasOrganization "AOL Mail"^^xsd:string ;
    ns2:hasState "New York"^^xsd:string ;
    ns2:hasYear 2014 ;
    ns2:isType_of ns2:Criminal,
        ns2:Exploitation_of_Application_Server ;
    rdfs:comment "AOL Mail is hacked and several users report their accounts are being used to send spam to others. The potential impact affects 50 million and all users are urged to change their passwords."^^xsd:string .

ns2:82441a9022b3c9aa a ns2:AccountAttack,
        owl:NamedIndividual ;
    ns1:associatedCampaigns ns2:Rafael_Correa_Twitter_account ;
    ns1:isLaunchedBy ns2:Ecuador ;
    ns2:hasActor "Anonymous (Ecuador)"^^xsd:string ;
    ns2:hasActorCountry "Ecuador"^^xsd:string ;
    ns2:hasActorType "Hacktivist"^^xsd:string ;
    ns2:hasCountry "Ecuador"^^xsd:string ;
    ns2:hasEventDate "2014-03-29T00:00:00"^^xsd:dateTime ;
    ns2:hasEventSubtype "Message Manipulation"^^xsd:string ;
    ns2:hasEventType "Disruptive"^^xsd:string ;
    ns2:hasIndustry "Public Administration"^^xsd:string ;
    ns2:hasMonth 3 ;
    ns2:hasOrganization "Rafael Correa Twitter account"^^xsd:string ;
    ns2:hasYear 2014 ;
    ns2:isType_of ns2:Hacktivist,
        ns2:Message_Manipulation ;
    rdfs:comment "The official Twitter account of Rafael Correa (@MashiRafael), the president of Ecuador, has been hijacked. Anonymous Ecuador hackers are apparently behind the attack."^^xsd:string .

ns2:827ad935929a2f43 a ns2:AttackWebsite,
        owl:NamedIndividual ;
    ns1:associatedCampaigns ns2:City_of_Dubois__PA ;
    ns1:description "Protest"^^xsd:string ;
    ns1:isLaunchedBy ns2:United_States_of_America ;
    ns2:behaviour ns2:Protest ;
    ns2:hasActor "MaeSTro-GhoL"^^xsd:string ;
    ns2:hasActorCountry "United States of America"^^xsd:string ;
    ns2:hasActorType "Hacktivist"^^xsd:string ;
    ns2:hasCampaign ns2:Pennsylvania ;
    ns2:hasCountry "United States of America"^^xsd:string ;
    ns2:hasCounty "Clearfield"^^xsd:string ;
    ns2:hasEventDate "2014-08-28T00:00:00"^^xsd:dateTime ;
    ns2:hasEventSubtype "Message Manipulation"^^xsd:string ;
    ns2:hasEventType "Disruptive"^^xsd:string ;
    ns2:hasIndustry "Public Administration"^^xsd:string ;
    ns2:hasMonth 8 ;
    ns2:hasOrganization "City of Dubois, PA"^^xsd:string ;
    ns2:hasState "Pennsylvania"^^xsd:string ;
    ns2:hasYear 2014 ;
    ns2:isType_of ns2:Hacktivist,
        ns2:Message_Manipulation ;
    rdfs:comment "AÃÆÃ'Ãâ 'ÃÆÃ¢â¬Â 'ÃÆÃ'ÃÂ¢Ã¢'Â¬ÃÂ ''ÃÆÃ'Ãâ 'ÃÆÃ¢â¬Â ''ÃÆÃ'Ãâ ''ÃÆÃ''ÃÆ'Ã'ÃÂ MoroccanÃÆÃ'Ãâ 'ÃÆÃ¢â¬Â 'ÃÆÃ'ÃÂ¢Ã¢'Â¬ÃÂ ''ÃÆÃ'Ãâ 'ÃÆÃ¢â¬Â ''ÃÆÃ'Ãâ ''ÃÆÃ''ÃÆ'Ã'ÃÂ hacker going with the handle of MaeSTro-GhoL defaces the official website ofÃÆÃ'Ãâ 'ÃÆÃ¢â¬Â 'ÃÆÃ'ÃÂ¢Ã¢'Â¬ÃÂ ''ÃÆÃ'Ãâ 'ÃÆÃ¢â¬Â ''ÃÆÃ'Ãâ ''ÃÆÃ''ÃÆ'Ã'ÃÂ the City of DuBois, Pennsylvania (duboispa.gov) inÃÆÃ'Ãâ 'ÃÆÃ¢â¬Â 'ÃÆÃ'ÃÂ¢Ã¢'Â¬ÃÂ ''ÃÆÃ'Ãâ 'ÃÆÃ¢â¬Â ''ÃÆÃ'Ãâ ''ÃÆÃ''ÃÆ'Ã'ÃÂ solidarity with Palestine."^^xsd:string .

ns2:82ff7daa6aa16324 a ns2:AttackWebsite,
        owl:NamedIndividual ;
    ns1:associatedCampaigns ns2:Armed_Forces_Training_Authority ;
    ns1:isLaunchedBy ns2:Afghanistan ;
    ns2:hasActor "YMH"^^xsd:string ;
    ns2:hasActorCountry "Afghanistan"^^xsd:string ;
    ns2:hasActorType "Hobbyist"^^xsd:string ;
    ns2:hasCountry "Egypt"^^xsd:string ;
    ns2:hasEventDate "2014-03-31T00:00:00"^^xsd:dateTime ;
    ns2:hasEventSubtype "Message Manipulation"^^xsd:string ;
    ns2:hasEventType "Disruptive"^^xsd:string ;
    ns2:hasIndustry "Public Administration"^^xsd:string ;
    ns2:hasMonth 3 ;
    ns2:hasOrganization "Armed Forces Training Authority"^^xsd:string ;
    ns2:hasYear 2014 ;
    ns2:isType_of ns2:Hobbyist,
        ns2:Message_Manipulation ;
    rdfs:comment "A Yemeni hacker going with the handle of YMH defaces the official website of Egyptian Armed Forces Training Authority (mtc.edu.eg)."^^xsd:string .

ns2:833863509c7bc8c9 a ns2:BreachInformation,
        owl:NamedIndividual ;
    ns1:associatedCampaigns ns2:JCM_Partners ;
    ns1:description "Financial"^^xsd:string ;
    ns2:behaviour ns2:Financial ;
    ns2:hasActorType "Criminal"^^xsd:string ;
    ns2:hasCampaign ns2:California ;
    ns2:hasCountry "United States of America"^^xsd:string ;
    ns2:hasCounty "Alameda"^^xsd:string ;
    ns2:hasEventDate "2014-03-06T00:00:00"^^xsd:dateTime ;
    ns2:hasEventSubtype "Exploitation of Application Server"^^xsd:string ;
    ns2:hasEventType "Exploitive"^^xsd:string ;
    ns2:hasIndustry "Real Estate and Rental and Leasing"^^xsd:string ;
    ns2:hasMonth 3 ;
    ns2:hasOrganization "JCM Partners"^^xsd:string ;
    ns2:hasState "California"^^xsd:string ;
    ns2:hasYear 2014 ;
    ns2:isType_of ns2:Criminal,
        ns2:Exploitation_of_Application_Server ;
    rdfs:comment "Real estate management company JCM Partners notifies an undisclosed number of housing applicants that their personal information has been exposed online."^^xsd:string .

ns2:843ea73e3231b2c8 a ns2:AccountAttack,
        owl:NamedIndividual ;
    ns1:associatedCampaigns ns2:Bank_of_the_West ;
    ns1:description "Financial"^^xsd:string ;
    ns2:behaviour ns2:Financial ;
    ns2:hasActorType "Criminal"^^xsd:string ;
    ns2:hasCampaign ns2:California ;
    ns2:hasCountry "United States of America"^^xsd:string ;
    ns2:hasCounty "San Francisco"^^xsd:string ;
    ns2:hasEventDate "2014-02-14T00:00:00"^^xsd:dateTime ;
    ns2:hasEventSubtype "Exploitation of Application Server"^^xsd:string ;
    ns2:hasEventType "Exploitive"^^xsd:string ;
    ns2:hasIndustry "Finance and Insurance"^^xsd:string ;
    ns2:hasMonth 2 ;
    ns2:hasOrganization "Bank of the West"^^xsd:string ;
    ns2:hasState "California"^^xsd:string ;
    ns2:hasYear 2014 ;
    ns2:isType_of ns2:Criminal,
        ns2:Exploitation_of_Application_Server ;
    rdfs:comment "An undisclosed number of individuals who applied online for a position with San Francisco-based Bank of the West have their personal information (including Social Security numbers) compromised after an unauthorized party gained access to a job application system."^^xsd:string .

ns2:854b72adac34d215 a ns2:EmailPhishing,
        owl:NamedIndividual ;
    ns1:associatedCampaigns ns2:Brazilian_Ministry_of_External_Relations ;
    ns2:hasActorType "Criminal"^^xsd:string ;
    ns2:hasCountry "Brazil"^^xsd:string ;
    ns2:hasEventDate "2014-05-30T00:00:00"^^xsd:dateTime ;
    ns2:hasEventSubtype "Exploitation of Application Server,Exploitation of End Hosts"^^xsd:string ;
    ns2:hasEventType "Exploitive"^^xsd:string ;
    ns2:hasIndustry "Public Administration"^^xsd:string ;
    ns2:hasMonth 5 ;
    ns2:hasOrganization "Brazilian Ministry of External Relations"^^xsd:string ;
    ns2:hasYear 2014 ;
    ns2:isType_of ns2:Criminal,
        ns2:Exploitation_of_Application_Server_Explo ;
    rdfs:comment "The internal communications system of the Brazilian Ministry of External Relations has been hit by hackers carried on with spear-phishing emails."^^xsd:string .

ns2:85c4cfe046eddc9b a ns2:CyberattackInformation,
        owl:NamedIndividual ;
    ns1:associatedCampaigns ns2:Ministry_of_Communications_and_Informati ;
    ns2:hasActorType "Criminal"^^xsd:string ;
    ns2:hasCountry "Myanmar"^^xsd:string ;
    ns2:hasEventDate "2014-07-06T00:00:00"^^xsd:dateTime ;
    ns2:hasEventSubtype "Message Manipulation"^^xsd:string ;
    ns2:hasEventType "Disruptive"^^xsd:string ;
    ns2:hasIndustry "Public Administration"^^xsd:string ;
    ns2:hasMonth 7 ;
    ns2:hasOrganization "Ministry of Communications and Information Technology"^^xsd:string ;
    ns2:hasYear 2014 ;
    ns2:isType_of ns2:Criminal,
        ns2:Message_Manipulation ;
    rdfs:comment "The website of Myanmar's Ministry of Communications and Information Technology is hacked, with the hackers replacing two government seals with turtles alluding to the country's slow internet connection."^^xsd:string .

ns2:875679a1722c2e9a a ns2:AttackWebsite,
        owl:NamedIndividual ;
    ns1:associatedCampaigns ns2:World_Wildlife_Fund ;
    ns1:isLaunchedBy ns2:Indonesia ;
    ns2:hasActor "Gantengers Crew"^^xsd:string ;
    ns2:hasActorCountry "Indonesia"^^xsd:string ;
    ns2:hasActorType "Hobbyist"^^xsd:string ;
    ns2:hasCountry "Philippines"^^xsd:string ;
    ns2:hasEventDate "2014-02-25T00:00:00"^^xsd:dateTime ;
    ns2:hasEventSubtype "Message Manipulation"^^xsd:string ;
    ns2:hasEventType "Disruptive"^^xsd:string ;
    ns2:hasIndustry "Other Services (except Public Administration)"^^xsd:string ;
    ns2:hasMonth 2 ;
    ns2:hasOrganization "World Wildlife Fund"^^xsd:string ;
    ns2:hasYear 2014 ;
    ns2:isType_of ns2:Hobbyist,
        ns2:Message_Manipulation ;
    rdfs:comment "The official websites of World Wildlife Fund (WWF) and Earth Hour Philippines (wwwf.org.ph and earth our.wwf.org.ph) are hacked and defaced by an Indonesian based hacking group called Gantengers Crew."^^xsd:string .

ns2:876e3228d05fbb5b a ns2:CyberattackSystem,
        owl:NamedIndividual ;
    ns1:associatedCampaigns ns2:Pakistan_Manpower_Institute ;
    ns1:isLaunchedBy ns2:Pakistan ;
    ns2:hasActor "Bl@Ck Dr@GoN; Haxor T0du; Spider64"^^xsd:string ;
    ns2:hasActorCountry "Pakistan"^^xsd:string ;
    ns2:hasActorType "Hacktivist"^^xsd:string ;
    ns2:hasCountry "Pakistan"^^xsd:string ;
    ns2:hasEventDate "2014-04-25T00:00:00"^^xsd:dateTime ;
    ns2:hasEventSubtype "Message Manipulation"^^xsd:string ;
    ns2:hasEventType "Disruptive"^^xsd:string ;
    ns2:hasIndustry "Public Administration"^^xsd:string ;
    ns2:hasMonth 4 ;
    ns2:hasOrganization "Pakistan Manpower Institute"^^xsd:string ;
    ns2:hasYear 2014 ;
    ns2:isType_of ns2:Hacktivist,
        ns2:Message_Manipulation ;
    rdfs:comment "The cyber battle between Indian and Pakistani hacktivists continues. In name of OpPakistan Indian hackers deface several Pakistani government websites."^^xsd:string .

ns2:87cdff886d5d1031 a ns2:HackerSecurity,
        owl:NamedIndividual ;
    ns1:associatedCampaigns ns2:Road_sign_in_San_Francisco ;
    ns2:hasActorType "Criminal"^^xsd:string ;
    ns2:hasCampaign ns2:California ;
    ns2:hasCountry "United States of America"^^xsd:string ;
    ns2:hasCounty "San Francisco"^^xsd:string ;
    ns2:hasEventDate "2014-05-16T00:00:00"^^xsd:dateTime ;
    ns2:hasEventSubtype "Message Manipulation"^^xsd:string ;
    ns2:hasEventType "Disruptive"^^xsd:string ;
    ns2:hasIndustry "Transportation and Warehousing"^^xsd:string ;
    ns2:hasMonth 5 ;
    ns2:hasOrganization "Road sign in San Francisco"^^xsd:string ;
    ns2:hasState "California"^^xsd:string ;
    ns2:hasYear 2014 ;
    ns2:isType_of ns2:Criminal,
        ns2:Message_Manipulation ;
    rdfs:comment "An unknown prankster hacker hacks an electronic traffic sign in San Francisco warning of a Godzilla Attack."^^xsd:string .

ns2:8815d521bdcf7a52 a ns2:DDoS,
        owl:NamedIndividual ;
    ns1:associatedCampaigns ns2:Origin ;
    ns2:hasActor "DERP Trolling"^^xsd:string ;
    ns2:hasCampaign ns2:California ;
    ns2:hasCountry "United States of America"^^xsd:string ;
    ns2:hasCounty "San Mateo"^^xsd:string ;
    ns2:hasEventDate "2014-01-03T00:00:00"^^xsd:dateTime ;
    ns2:hasEventSubtype "External Denial of Service"^^xsd:string ;
    ns2:hasEventType "Disruptive"^^xsd:string ;
    ns2:hasIndustry "Information"^^xsd:string ;
    ns2:hasMonth 1 ;
    ns2:hasOrganization "Origin"^^xsd:string ;
    ns2:hasState "California"^^xsd:string ;
    ns2:hasYear 2014 ;
    ns2:isType_of ns2:External_Denial_of_Service ;
    rdfs:comment "The servers for Steam, Origin, Battle.net, and League of Legends are brought down temporarily by apparent DDoS attacks that seem to be related to a swatting attack on an individual known for streaming games."^^xsd:string .

ns2:881facc26f63e238 a ns2:AnonymousAttack,
        owl:NamedIndividual ;
    ns1:associatedCampaigns ns2:Areva ;
    ns1:description "Protest"^^xsd:string ;
    ns2:behaviour ns2:Protest ;
    ns2:hasActor "Anonymous"^^xsd:string ;
    ns2:hasActorType "Hacktivist"^^xsd:string ;
    ns2:hasCountry "France"^^xsd:string ;
    ns2:hasEventDate "2015-05-05T00:00:00"^^xsd:dateTime ;
    ns2:hasEventSubtype "External Denial of Service"^^xsd:string ;
    ns2:hasEventType "Disruptive"^^xsd:string ;
    ns2:hasIndustry "Construction"^^xsd:string ;
    ns2:hasMonth 5 ;
    ns2:hasOrganization "Areva"^^xsd:string ;
    ns2:hasYear 2015 ;
    ns2:isType_of ns2:External_Denial_of_Service,
        ns2:Hacktivist ;
    rdfs:comment "In name of OpGreenRights, the Anonymous take down the website of Areva, a French conglomerate in charge of building a Nuclear reactor"^^xsd:string .

ns2:884bf33a3f048833 a ns2:AttackWebsite,
        owl:NamedIndividual ;
    ns1:associatedCampaigns ns2:Various_Government_Websites ;
    ns1:isLaunchedBy ns2:Ukraine ;
    ns2:hasActor "Ukranian Svoboda Party"^^xsd:string ;
    ns2:hasActorCountry "Ukraine"^^xsd:string ;
    ns2:hasActorType "Hacktivist"^^xsd:string ;
    ns2:hasCountry "Ukraine"^^xsd:string ;
    ns2:hasEventDate "2014-02-01T00:00:00"^^xsd:dateTime ;
    ns2:hasEventSubtype "Message Manipulation"^^xsd:string ;
    ns2:hasEventType "Disruptive"^^xsd:string ;
    ns2:hasIndustry "Public Administration"^^xsd:string ;
    ns2:hasMonth 2 ;
    ns2:hasOrganization "Various Government Websites"^^xsd:string ;
    ns2:hasYear 2014 ;
    ns2:isType_of ns2:Hacktivist,
        ns2:Message_Manipulation ;
    rdfs:comment "Hacktivists from Ukrainian neo-fascist Svoboda party deface more than 30 Ukrainian government and media websites."^^xsd:string .

ns2:8864253f4f7ccf42 a ns2:AccountAttack,
        owl:NamedIndividual ;
    ns1:associatedCampaigns ns2:Otto_Pizza ;
    ns1:description "Financial"^^xsd:string ;
    ns2:behaviour ns2:Financial ;
    ns2:hasActorType "Criminal"^^xsd:string ;
    ns2:hasCampaign ns2:Oregon ;
    ns2:hasCountry "United States of America"^^xsd:string ;
    ns2:hasCounty "Multnomah"^^xsd:string ;
    ns2:hasEventDate "2014-08-23T00:00:00"^^xsd:dateTime ;
    ns2:hasEventSubtype "Exploitation of Sensors"^^xsd:string ;
    ns2:hasEventType "Exploitive"^^xsd:string ;
    ns2:hasIndustry "Accommodation and Food Services"^^xsd:string ;
    ns2:hasMonth 8 ;
    ns2:hasOrganization "Otto Pizza"^^xsd:string ;
    ns2:hasState "Oregon"^^xsd:string ;
    ns2:hasYear 2014 ;
    ns2:isType_of ns2:Criminal,
        ns2:Exploitation_of_Sensors ;
    rdfs:comment "An intrusion on the systems of the Otto Pizza restaurant in Portland, Oregon, causes credit card information of 900 customers to be exposed to unauthorized individuals."^^xsd:string .

ns2:88a3d8cdbc615f63 a ns2:AccessAttack,
        owl:NamedIndividual ;
    ns1:associatedCampaigns ns2:City_To_Bay_Fun_Run ;
    ns2:hasActorType "Criminal"^^xsd:string ;
    ns2:hasCountry "Australia"^^xsd:string ;
    ns2:hasEventDate "2014-08-11T00:00:00"^^xsd:dateTime ;
    ns2:hasEventSubtype "Exploitation of Application Server"^^xsd:string ;
    ns2:hasEventType "Exploitive"^^xsd:string ;
    ns2:hasIndustry "Other Services (except Public Administration)"^^xsd:string ;
    ns2:hasMonth 8 ;
    ns2:hasOrganization "City To Bay Fun Run"^^xsd:string ;
    ns2:hasYear 2014 ;
    ns2:isType_of ns2:Criminal,
        ns2:Exploitation_of_Application_Server ;
    rdfs:comment "Adelaide police investigate a possible illegitimate access into the City To Bay Fun Run website (city-bay.org.au), viewing the details of 12,000 individuals."^^xsd:string .

ns2:88ed4446a07f9b14 a ns2:CyberattackData,
        owl:NamedIndividual ;
    ns1:associatedCampaigns ns2:St__Louis_County_Police ;
    ns1:description "Protest"^^xsd:string ;
    ns2:behaviour ns2:Protest ;
    ns2:hasActorType "Criminal"^^xsd:string ;
    ns2:hasCampaign ns2:Missouri ;
    ns2:hasCountry "United States of America"^^xsd:string ;
    ns2:hasCounty "St. Louis"^^xsd:string ;
    ns2:hasEventDate "2014-08-14T00:00:00"^^xsd:dateTime ;
    ns2:hasEventSubtype "External Denial of Service"^^xsd:string ;
    ns2:hasEventType "Disruptive"^^xsd:string ;
    ns2:hasIndustry "Public Administration"^^xsd:string ;
    ns2:hasMonth 8 ;
    ns2:hasOrganization "St. Louis County Police"^^xsd:string ;
    ns2:hasState "Missouri"^^xsd:string ;
    ns2:hasYear 2014 ;
    ns2:isType_of ns2:Criminal,
        ns2:External_Denial_of_Service ;
    rdfs:comment "In the wake of the shooting of unarmed teen Michael Brown, hackers launch a cyberattack to take out the St. Louis County Police department's website and email."^^xsd:string .

ns2:89b68278558ec42e a ns2:DefaceHacker,
        owl:NamedIndividual ;
    ns1:associatedCampaigns ns2:Rescator ;
    ns1:description "Protest"^^xsd:string ;
    ns2:behaviour ns2:Protest ;
    ns2:hasActorType "Criminal"^^xsd:string ;
    ns2:hasEventDate "2014-05-17T00:00:00"^^xsd:dateTime ;
    ns2:hasEventSubtype "Message Manipulation"^^xsd:string ;
    ns2:hasEventType "Disruptive"^^xsd:string ;
    ns2:hasIndustry "Information"^^xsd:string ;
    ns2:hasMonth 5 ;
    ns2:hasOrganization "Rescator"^^xsd:string ;
    ns2:hasYear 2014 ;
    ns2:isType_of ns2:Criminal,
        ns2:Message_Manipulation ;
    rdfs:comment "Rescator, a popular underground website that sells payment card data, is hacked and defaced."^^xsd:string .

ns2:8a881758599ea9e2 a ns2:BreachInformation,
        owl:NamedIndividual ;
    ns1:associatedCampaigns ns2:MangaGamer ;
    ns2:hasActorType "Criminal"^^xsd:string ;
    ns2:hasCountry "Japan"^^xsd:string ;
    ns2:hasEventDate "2014-08-29T00:00:00"^^xsd:dateTime ;
    ns2:hasEventSubtype "Exploitation of Application Server"^^xsd:string ;
    ns2:hasEventType "Exploitive"^^xsd:string ;
    ns2:hasMonth 8 ;
    ns2:hasOrganization "MangaGamer"^^xsd:string ;
    ns2:hasYear 2014 ;
    ns2:isType_of ns2:Criminal,
        ns2:Exploitation_of_Application_Server ;
    rdfs:comment "Visual novel distributorÃÆÃ'Ãâ 'ÃÆÃ¢â¬Â 'ÃÆÃ'ÃÂ¢Ã¢'Â¬ÃÂ ''ÃÆÃ'Ãâ 'ÃÆÃ¢â¬Â ''ÃÆÃ'Ãâ ''ÃÆÃ''ÃÆ'Ã'ÃÂ MangaGamer  notifies its users to have suffered a security breach. The full member database is posted on pastebin."^^xsd:string .

ns2:8b2976020b51ab00 a ns2:HackerSecurity,
        owl:NamedIndividual ;
    ns1:associatedCampaigns ns2:Boston_Scientific ;
    ns1:description "Industrial-Espionage"^^xsd:string ;
    ns2:behaviour ns2:Industrial_Espionage ;
    ns2:hasActorType "Criminal"^^xsd:string ;
    ns2:hasCampaign ns2:Massachusetts ;
    ns2:hasCountry "United States of America"^^xsd:string ;
    ns2:hasCounty "Middlesex"^^xsd:string ;
    ns2:hasEventDate "2014-02-10T00:00:00"^^xsd:dateTime ;
    ns2:hasEventSubtype "Exploitation of Application Server"^^xsd:string ;
    ns2:hasEventType "Exploitive"^^xsd:string ;
    ns2:hasIndustry "Manufacturing"^^xsd:string ;
    ns2:hasMonth 2 ;
    ns2:hasOrganization "Boston Scientific"^^xsd:string ;
    ns2:hasState "Massachusetts"^^xsd:string ;
    ns2:hasYear 2014 ;
    ns2:isType_of ns2:Criminal,
        ns2:Exploitation_of_Application_Server ;
    rdfs:comment "The computer networks of three big medical device makers are breached by unknown attackers likely interested in the companies' intellectual property. The companies in question are Medtronic, Boston Scientific and St. Jude Medical."^^xsd:string .

ns2:8b33e3ead069dcef a ns2:BreachInformation,
        owl:NamedIndividual ;
    ns1:associatedCampaigns ns2:Jennifer_Lawrence ;
    ns1:description "Personal Attack"^^xsd:string ;
    ns2:behaviour ns2:Personal_Attack ;
    ns2:hasActorType "Criminal"^^xsd:string ;
    ns2:hasCountry "United States of America"^^xsd:string ;
    ns2:hasEventDate "2014-08-31T00:00:00"^^xsd:dateTime ;
    ns2:hasEventSubtype "Exploitation of Application Server"^^xsd:string ;
    ns2:hasEventType "Exploitive"^^xsd:string ;
    ns2:hasIndustry "Other Services (except Public Administration)"^^xsd:string ;
    ns2:hasMonth 8 ;
    ns2:hasOrganization "Jennifer Lawrence"^^xsd:string ;
    ns2:hasYear 2014 ;
    ns2:isType_of ns2:Criminal,
        ns2:Exploitation_of_Application_Server ;
    rdfs:comment "Yet another leak of celebrities pictures. A massive leak of nude and risque photos appearing to be of huge stars like is leaked online, first appearing on 4chan."^^xsd:string .

ns2:8bedaf7c6e7ba249 a ns2:AttackWebsite,
        owl:NamedIndividual ;
    ns1:associatedCampaigns ns2:Lal_Krishna_Advani_website ;
    ns1:description "Protest"^^xsd:string ;
    ns1:isLaunchedBy ns2:India ;
    ns2:behaviour ns2:Protest ;
    ns2:hasActor "Muhammad Bilalhas"^^xsd:string ;
    ns2:hasActorCountry "India"^^xsd:string ;
    ns2:hasActorType "Hacktivist"^^xsd:string ;
    ns2:hasCountry "India"^^xsd:string ;
    ns2:hasEventDate "2014-08-21T00:00:00"^^xsd:dateTime ;
    ns2:hasEventSubtype "Message Manipulation"^^xsd:string ;
    ns2:hasEventType "Disruptive"^^xsd:string ;
    ns2:hasIndustry "Other Services (except Public Administration)"^^xsd:string ;
    ns2:hasMonth 8 ;
    ns2:hasOrganization "Lal Krishna Advani website"^^xsd:string ;
    ns2:hasYear 2014 ;
    ns2:isType_of ns2:Hacktivist,
        ns2:Message_Manipulation ;
    rdfs:comment "A Pakistani hacker called Muhammad Bilal defaces the official website of senior leader of the Indian Bharatiya Janata Party, Lal Krishna Advani (lkadvani.in)."^^xsd:string .

ns2:8c470e2bb164beef a ns2:CyberattackData,
        owl:NamedIndividual ;
    ns1:associatedCampaigns ns2:job_sy ;
    ns1:isLaunchedBy ns2:Syrian_Arab_Republic ;
    ns2:hasActor "Zer0Pwn"^^xsd:string ;
    ns2:hasActorCountry "Syrian Arab Republic"^^xsd:string ;
    ns2:hasActorType "Hacktivist"^^xsd:string ;
    ns2:hasCountry "Syrian Arab Republic"^^xsd:string ;
    ns2:hasEventDate "2014-04-06T00:00:00"^^xsd:dateTime ;
    ns2:hasEventSubtype "Exploitation of Application Server"^^xsd:string ;
    ns2:hasEventType "Exploitive"^^xsd:string ;
    ns2:hasIndustry "Information"^^xsd:string ;
    ns2:hasMonth 4 ;
    ns2:hasOrganization "job.sy"^^xsd:string ;
    ns2:hasYear 2014 ;
    ns2:isType_of ns2:Exploitation_of_Application_Server,
        ns2:Hacktivist ;
    rdfs:comment "Zer0Pwn, a member of the European Cyber Arm (ECA), hacks two Syrian Web sites, Job.sy and RealEstate.sy, and dumps 60,000 accounts."^^xsd:string .

ns2:8c5e7bc0c84cdffb a ns2:AnonymousAttack,
        owl:NamedIndividual ;
    ns1:associatedCampaigns ns2:Tails_OS ;
    ns2:hasActor "Sum Guy"^^xsd:string ;
    ns2:hasActorType "Hobbyist"^^xsd:string ;
    ns2:hasCountry "United States of America"^^xsd:string ;
    ns2:hasEventDate "2014-06-30T00:00:00"^^xsd:dateTime ;
    ns2:hasEventSubtype "Message Manipulation"^^xsd:string ;
    ns2:hasEventType "Disruptive"^^xsd:string ;
    ns2:hasIndustry "Other Services (except Public Administration)"^^xsd:string ;
    ns2:hasMonth 6 ;
    ns2:hasOrganization "Tails OS"^^xsd:string ;
    ns2:hasYear 2014 ;
    ns2:isType_of ns2:Hobbyist,
        ns2:Message_Manipulation ;
    rdfs:comment "The official website of the Tails live operating system is defaced. The author of the hack, dubbed Sum Guy, claims to have done it by accident."^^xsd:string .

ns2:8cc4224d934612ba a ns2:AttackWebsite,
        owl:NamedIndividual ;
    ns1:associatedCampaigns ns2:Haaretz ;
    ns1:description "Protest"^^xsd:string ;
    ns2:behaviour ns2:Protest ;
    ns2:hasActor "AnonGhost"^^xsd:string ;
    ns2:hasActorType "Hacktivist"^^xsd:string ;
    ns2:hasCountry "Israel"^^xsd:string ;
    ns2:hasEventDate "2014-07-15T00:00:00"^^xsd:dateTime ;
    ns2:hasEventSubtype "Message Manipulation"^^xsd:string ;
    ns2:hasEventType "Disruptive"^^xsd:string ;
    ns2:hasIndustry "Information"^^xsd:string ;
    ns2:hasMonth 7 ;
    ns2:hasOrganization "Haaretz"^^xsd:string ;
    ns2:hasYear 2014 ;
    ns2:isType_of ns2:Hacktivist,
        ns2:Message_Manipulation ;
    rdfs:comment "Again, in the name of OPSaveGaza, AnonGhost defaces a sub-domain of Israel's largest and oldest newspaper Haaretz against Israeli bombing over Gaza, Palestine."^^xsd:string .

ns2:8d8a2781d0c92842 a ns2:Ransomware,
        owl:NamedIndividual ;
    ns1:associatedCampaigns ns2:Automatic_Systems ;
    ns1:description "Financial"^^xsd:string ;
    ns1:isLaunchedBy ns2:Russian_Federation ;
    ns2:behaviour ns2:Financial ;
    ns2:hasActor "ALPHVM"^^xsd:string ;
    ns2:hasActorCountry "Russian Federation"^^xsd:string ;
    ns2:hasActorType "Criminal"^^xsd:string ;
    ns2:hasCountry "France"^^xsd:string ;
    ns2:hasEventDate "2023-06-03T00:00:00"^^xsd:dateTime ;
    ns2:hasEventSubtype "Data Attack"^^xsd:string ;
    ns2:hasEventType "Mixed"^^xsd:string ;
    ns2:hasIndustry "Manufacturing"^^xsd:string ;
    ns2:hasMonth 6 ;
    ns2:hasOrganization "Automatic Systems"^^xsd:string ;
    ns2:hasYear 2023 ;
    ns2:isType_of ns2:Criminal,
        ns2:Data_Attack ;
    rdfs:comment "The ALPHV/BlackCat ransomware gang claims responsibility for the attack on Automatic Systems, a subsidiary of French conglomerate BollorÃÆÃ'Ã'ÃÂ©. The gang's post on its leak site includes over a hundred samples of stolen data, ranging from non-disclosure agreements (NDAs) to copies of passports."^^xsd:string .

ns2:8d8cbe0bab9ca4b7 a ns2:CyberattackInformation,
        owl:NamedIndividual ;
    ns1:associatedCampaigns ns2:Kaiser_Permanente ;
    ns2:hasActorType "Criminal"^^xsd:string ;
    ns2:hasCampaign ns2:California ;
    ns2:hasCountry "United States of America"^^xsd:string ;
    ns2:hasCounty "Alameda"^^xsd:string ;
    ns2:hasEventDate "2014-02-28T00:00:00"^^xsd:dateTime ;
    ns2:hasEventSubtype "Exploitation of Application Server"^^xsd:string ;
    ns2:hasEventType "Exploitive"^^xsd:string ;
    ns2:hasIndustry "Health Care and Social Assistance"^^xsd:string ;
    ns2:hasMonth 2 ;
    ns2:hasOrganization "Kaiser Permanente"^^xsd:string ;
    ns2:hasState "California"^^xsd:string ;
    ns2:hasYear 2014 ;
    ns2:isType_of ns2:Criminal,
        ns2:Exploitation_of_Application_Server ;
    rdfs:comment "Health services provider Kaiser Permanente notifies roughly 5,100 members that their personal information may be at risk after malware was discovered on a server used by the Kaiser Permanente Northern California Division of Research."^^xsd:string .

ns2:8da805adac3625b4 a ns2:CyberattackData,
        owl:NamedIndividual ;
    ns1:associatedCampaigns ns2:Silk_Road ;
    ns1:description "Financial"^^xsd:string ;
    ns2:behaviour ns2:Financial ;
    ns2:hasActorType "Criminal"^^xsd:string ;
    ns2:hasCountry "United States of America"^^xsd:string ;
    ns2:hasEventDate "2014-02-13T00:00:00"^^xsd:dateTime ;
    ns2:hasEventSubtype "Exploitation of Application Server"^^xsd:string ;
    ns2:hasEventType "Exploitive"^^xsd:string ;
    ns2:hasIndustry "Other Services (except Public Administration)"^^xsd:string ;
    ns2:hasMonth 2 ;
    ns2:hasOrganization "Silk Road"^^xsd:string ;
    ns2:hasYear 2014 ;
    ns2:isType_of ns2:Criminal,
        ns2:Exploitation_of_Application_Server ;
    rdfs:comment "Using a known Bitcoin vulnerability the popular marketplace Silk Road is hacked, losing approximately 4,400 bitcoins, presently worth around $2.6 million."^^xsd:string .

ns2:8dc37e6b511ccd65 a ns2:CyberattackData,
        owl:NamedIndividual ;
    ns1:associatedCampaigns ns2:European_Central_Bank ;
    ns1:description "Financial"^^xsd:string ;
    ns2:behaviour ns2:Financial ;
    ns2:hasActorType "Criminal"^^xsd:string ;
    ns2:hasCountry "Germany"^^xsd:string ;
    ns2:hasEventDate "2014-07-24T00:00:00"^^xsd:dateTime ;
    ns2:hasEventSubtype "Exploitation of Application Server"^^xsd:string ;
    ns2:hasEventType "Exploitive"^^xsd:string ;
    ns2:hasIndustry "Finance and Insurance"^^xsd:string ;
    ns2:hasMonth 7 ;
    ns2:hasOrganization "European Central Bank"^^xsd:string ;
    ns2:hasYear 2014 ;
    ns2:isType_of ns2:Criminal,
        ns2:Exploitation_of_Application_Server ;
    rdfs:comment "The website of the European Central Bank (ECB) is hacked, with personal information stolen. The anonymous hacker claims to have stolen around 20,000 email addresses, and a smaller number of telephone numbers and addresses, relating to people who had registered for ECB conferences and visits."^^xsd:string .

ns2:8ed342609ea7a521 a ns2:HackerSecurity,
        owl:NamedIndividual ;
    ns1:associatedCampaigns ns2:ESET ;
    ns1:description "Financial"^^xsd:string ;
    ns2:behaviour ns2:Financial ;
    ns2:hasActorType "Criminal"^^xsd:string ;
    ns2:hasCountry "Slovakia"^^xsd:string ;
    ns2:hasEventDate "2014-06-06T00:00:00"^^xsd:dateTime ;
    ns2:hasEventSubtype "Exploitation of Application Server"^^xsd:string ;
    ns2:hasEventType "Exploitive"^^xsd:string ;
    ns2:hasIndustry "Professional, Scientific, and Technical Services"^^xsd:string ;
    ns2:hasMonth 6 ;
    ns2:hasOrganization "ESET"^^xsd:string ;
    ns2:hasYear 2014 ;
    ns2:isType_of ns2:Criminal,
        ns2:Exploitation_of_Application_Server ;
    rdfs:comment "The ESET Security Forum is hacked and the company confirms that account credentials of itsÃÆÃ'Ãâ 'ÃÆÃ¢â¬Â 'ÃÆÃ'ÃÂ¢Ã¢'Â¬ÃÂ ''ÃÆÃ'Ãâ 'ÃÆÃ¢â¬Â ''ÃÆÃ'Ãâ ''ÃÆÃ''ÃÆ'Ã'ÃÂ roughly 2,700 members have been accessed by the attackers."^^xsd:string .

ns2:8f57b0566dda7c77 a ns2:HackerSecurity,
        owl:NamedIndividual ;
    ns1:associatedCampaigns ns2:Justice_Minister_Judith_Collins ;
    ns1:isLaunchedBy ns2:New_Zealand ;
    ns2:hasActor "RawShark"^^xsd:string ;
    ns2:hasActorCountry "New Zealand"^^xsd:string ;
    ns2:hasActorType "Hacktivist"^^xsd:string ;
    ns2:hasCountry "New Zealand"^^xsd:string ;
    ns2:hasEventDate "2014-09-01T00:00:00"^^xsd:dateTime ;
    ns2:hasEventSubtype "Exploitation of Application Server"^^xsd:string ;
    ns2:hasEventType "Exploitive"^^xsd:string ;
    ns2:hasIndustry "Public Administration"^^xsd:string ;
    ns2:hasMonth 9 ;
    ns2:hasOrganization "Justice Minister Judith Collins"^^xsd:string ;
    ns2:hasYear 2014 ;
    ns2:isType_of ns2:Exploitation_of_Application_Server,
        ns2:Hacktivist ;
    rdfs:comment "A hacker known as RawShark (@whaledump) causes the resignation of New Zealand Justice Minister Judith Collins after releasing information showing a purported campaign to undermine government officials."^^xsd:string .

ns2:8f80aa4966ec50e1 a ns2:AnonymousAttack,
        owl:NamedIndividual ;
    ns1:associatedCampaigns ns2:Storebrand ;
    ns1:description "Protest"^^xsd:string ;
    ns1:isLaunchedBy ns2:Norway ;
    ns2:behaviour ns2:Protest ;
    ns2:hasActor "Anonymous (Norway)"^^xsd:string ;
    ns2:hasActorCountry "Norway"^^xsd:string ;
    ns2:hasActorType "Hacktivist"^^xsd:string ;
    ns2:hasCountry "Norway"^^xsd:string ;
    ns2:hasEventDate "2014-07-09T00:00:00"^^xsd:dateTime ;
    ns2:hasEventSubtype "External Denial of Service"^^xsd:string ;
    ns2:hasEventType "Disruptive"^^xsd:string ;
    ns2:hasIndustry "Finance and Insurance"^^xsd:string ;
    ns2:hasMonth 7 ;
    ns2:hasOrganization "Storebrand"^^xsd:string ;
    ns2:hasYear 2014 ;
    ns2:isType_of ns2:External_Denial_of_Service,
        ns2:Hacktivist ;
    rdfs:comment "Anonymous Norway starts multiple DDoS attacks towards major banks and insurance companies in Norway, including the country's largest telecommunications company, Telenor."^^xsd:string .

ns2:8fd5c6b5eda44cdc a ns2:AttackWebsite,
        owl:NamedIndividual ;
    ns1:associatedCampaigns ns2:Rovio ;
    ns1:description "Protest"^^xsd:string ;
    ns2:behaviour ns2:Protest ;
    ns2:hasActorType "Criminal"^^xsd:string ;
    ns2:hasCountry "Finland"^^xsd:string ;
    ns2:hasEventDate "2014-01-29T00:00:00"^^xsd:dateTime ;
    ns2:hasEventSubtype "Message Manipulation"^^xsd:string ;
    ns2:hasEventType "Disruptive"^^xsd:string ;
    ns2:hasIndustry "Information"^^xsd:string ;
    ns2:hasMonth 1 ;
    ns2:hasOrganization "Rovio"^^xsd:string ;
    ns2:hasYear 2014 ;
    ns2:isType_of ns2:Criminal,
        ns2:Message_Manipulation ;
    rdfs:comment "Angry Birds developer Rovio has its website hijacked. As a result, the official Angry Birds (angrybirds.com) website is defaced by someone protesting reports government spy agencies abuse it and other \"leaky\" mobile apps to mine the personal details of smartphone users."^^xsd:string .

ns2:91ca868cca9622df a ns2:HackerUser,
        owl:NamedIndividual ;
    ns1:associatedCampaigns ns2:openSUSE ;
    ns1:isLaunchedBy ns2:Pakistan ;
    ns2:hasActor "H4x0r HuSsY"^^xsd:string ;
    ns2:hasActorCountry "Pakistan"^^xsd:string ;
    ns2:hasActorType "Hobbyist"^^xsd:string ;
    ns2:hasCountry "Germany"^^xsd:string ;
    ns2:hasEventDate "2014-01-07T00:00:00"^^xsd:dateTime ;
    ns2:hasEventSubtype "Message Manipulation"^^xsd:string ;
    ns2:hasEventType "Disruptive"^^xsd:string ;
    ns2:hasIndustry "Other Services (except Public Administration)"^^xsd:string ;
    ns2:hasMonth 1 ;
    ns2:hasOrganization "openSUSE"^^xsd:string ;
    ns2:hasYear 2014 ;
    ns2:isType_of ns2:Hobbyist,
        ns2:Message_Manipulation ;
    rdfs:comment "The well-known Pakistani hacker H4x0r HuSsY hacks the official Forum of OpenSUSE, defacing it and allegedly compromising the account information of 79,500 registered users."^^xsd:string .

ns2:9328f8f48140c588 a ns2:CyberattackData,
        owl:NamedIndividual ;
    ns1:associatedCampaigns ns2:Community_Health_Systems ;
    ns1:description "Financial"^^xsd:string ;
    ns2:behaviour ns2:Financial ;
    ns2:hasActorType "Criminal"^^xsd:string ;
    ns2:hasCampaign ns2:Tennessee ;
    ns2:hasCountry "United States of America"^^xsd:string ;
    ns2:hasCounty "Williamson"^^xsd:string ;
    ns2:hasEventDate "2014-08-19T00:00:00"^^xsd:dateTime ;
    ns2:hasEventSubtype "Exploitation of Application Server"^^xsd:string ;
    ns2:hasEventType "Exploitive"^^xsd:string ;
    ns2:hasIndustry "Health Care and Social Assistance"^^xsd:string ;
    ns2:hasMonth 8 ;
    ns2:hasOrganization "Community Health Systems"^^xsd:string ;
    ns2:hasState "Tennessee"^^xsd:string ;
    ns2:hasYear 2014 ;
    ns2:isType_of ns2:Criminal,
        ns2:Exploitation_of_Application_Server ;
    rdfs:comment "Community Health Systems, a healthcare system spanning 29 states announces that cybercriminals operating from China stole information on approximately 4.5 million patients, including names, birth dates, and Social Security numbers."^^xsd:string .

ns2:9380971a23c1eefb a ns2:AnonymousAttack,
        owl:NamedIndividual ;
    ns1:associatedCampaigns ns2:Bank_of_Israel ;
    ns1:description "Protest"^^xsd:string ;
    ns2:behaviour ns2:Protest ;
    ns2:hasActor "Anonymous"^^xsd:string ;
    ns2:hasActorType "Hacktivist"^^xsd:string ;
    ns2:hasCountry "Israel"^^xsd:string ;
    ns2:hasEventDate "2014-08-25T00:00:00"^^xsd:dateTime ;
    ns2:hasEventSubtype "External Denial of Service"^^xsd:string ;
    ns2:hasEventType "Disruptive"^^xsd:string ;
    ns2:hasIndustry "Finance and Insurance"^^xsd:string ;
    ns2:hasMonth 8 ;
    ns2:hasOrganization "Bank of Israel"^^xsd:string ;
    ns2:hasYear 2014 ;
    ns2:isType_of ns2:External_Denial_of_Service,
        ns2:Hacktivist ;
    rdfs:comment "In name of #OpSaveGaza, the Anonymous collective claims to have taken down some key Israeli governmental websites, including those of the Israeli Defense Forces, the Bank of Israel, the Israeli Prime Minister."^^xsd:string .

ns2:93e7c1168c223ea1 a ns2:BreachSecurity,
        owl:NamedIndividual ;
    ns1:associatedCampaigns ns2:Paytime_Inc ;
    ns1:description "Financial"^^xsd:string ;
    ns2:behaviour ns2:Financial ;
    ns2:hasActorType "Criminal"^^xsd:string ;
    ns2:hasCampaign ns2:Pennsylvania ;
    ns2:hasCountry "United States of America"^^xsd:string ;
    ns2:hasCounty "Cumberland"^^xsd:string ;
    ns2:hasEventDate "2014-05-16T00:00:00"^^xsd:dateTime ;
    ns2:hasEventSubtype "Exploitation of Application Server"^^xsd:string ;
    ns2:hasEventType "Exploitive"^^xsd:string ;
    ns2:hasIndustry "Professional, Scientific, and Technical Services"^^xsd:string ;
    ns2:hasMonth 5 ;
    ns2:hasOrganization "Paytime Inc."^^xsd:string ;
    ns2:hasState "Pennsylvania"^^xsd:string ;
    ns2:hasYear 2014 ;
    ns2:isType_of ns2:Criminal,
        ns2:Exploitation_of_Application_Server ;
    rdfs:comment "An undisclosed number of individuals may have had personal information compromised after hackers took advantage of a vulnerability in systems belonging to Paytime Inc., a Pennsylvania payroll company."^^xsd:string .

ns2:942b4e4597df6ab9 a ns2:CyberattackData,
        owl:NamedIndividual ;
    ns1:associatedCampaigns ns2:realestate_sy ;
    ns1:isLaunchedBy ns2:Syrian_Arab_Republic ;
    ns2:hasActor "Zer0Pwn"^^xsd:string ;
    ns2:hasActorCountry "Syrian Arab Republic"^^xsd:string ;
    ns2:hasActorType "Hacktivist"^^xsd:string ;
    ns2:hasCountry "Syrian Arab Republic"^^xsd:string ;
    ns2:hasEventDate "2014-04-06T00:00:00"^^xsd:dateTime ;
    ns2:hasEventSubtype "Exploitation of Application Server"^^xsd:string ;
    ns2:hasEventType "Exploitive"^^xsd:string ;
    ns2:hasIndustry "Information"^^xsd:string ;
    ns2:hasMonth 4 ;
    ns2:hasOrganization "realestate.sy"^^xsd:string ;
    ns2:hasYear 2014 ;
    ns2:isType_of ns2:Exploitation_of_Application_Server,
        ns2:Hacktivist ;
    rdfs:comment "Zer0Pwn, a member of the European Cyber Arm (ECA), hacks two Syrian Web sites, Job.sy and RealEstate.sy, and dumps 60,000 accounts."^^xsd:string .

ns2:954331b872c08116 a ns2:AttackMalware,
        owl:NamedIndividual ;
    ns1:associatedCampaigns ns2:Indexeus_org ;
    ns2:hasActor "Pernicious Developers"^^xsd:string ;
    ns2:hasActorType "Hobbyist"^^xsd:string ;
    ns2:hasEventDate "2014-07-19T00:00:00"^^xsd:dateTime ;
    ns2:hasEventSubtype "Message Manipulation"^^xsd:string ;
    ns2:hasEventType "Disruptive"^^xsd:string ;
    ns2:hasIndustry "Professional, Scientific, and Technical Services"^^xsd:string ;
    ns2:hasMonth 7 ;
    ns2:hasOrganization "Indexeus.org"^^xsd:string ;
    ns2:hasYear 2014 ;
    ns2:isType_of ns2:Hobbyist,
        ns2:Message_Manipulation ;
    rdfs:comment "Indexeus.org, the search engine containing a database of stolen usernames and passwords is defaced by a group called Pernicious Developers."^^xsd:string .

ns2:9552aa314bd1f0dd a ns2:Phishing,
        owl:NamedIndividual ;
    ns1:associatedCampaigns ns2:PayPal ;
    ns1:isLaunchedBy ns2:Syrian_Arab_Republic ;
    ns2:hasActor "Syrian Electronic Army"^^xsd:string ;
    ns2:hasActorCountry "Syrian Arab Republic"^^xsd:string ;
    ns2:hasActorType "Hacktivist"^^xsd:string ;
    ns2:hasCountry "India"^^xsd:string ;
    ns2:hasEventDate "2014-02-05T00:00:00"^^xsd:dateTime ;
    ns2:hasEventSubtype "Exploitation of End Hosts"^^xsd:string ;
    ns2:hasEventType "Exploitive"^^xsd:string ;
    ns2:hasIndustry "Information"^^xsd:string ;
    ns2:hasMonth 2 ;
    ns2:hasOrganization "PayPal"^^xsd:string ;
    ns2:hasYear 2014 ;
    ns2:isType_of ns2:Exploitation_of_End_Hosts,
        ns2:Hacktivist ;
    rdfs:comment "Hackers have compromised the eBay and PayPal marketing webpages in the UK, France, and India, causing some visitors to be redirected to fraudulent destinations."^^xsd:string .

ns2:95967c2e3b6cff24 a ns2:AnonymousAttack,
        owl:NamedIndividual ;
    ns1:associatedCampaigns ns2:Gjensidige ;
    ns1:description "Protest"^^xsd:string ;
    ns1:isLaunchedBy ns2:Norway ;
    ns2:behaviour ns2:Protest ;
    ns2:hasActor "Anonymous (Norway)"^^xsd:string ;
    ns2:hasActorCountry "Norway"^^xsd:string ;
    ns2:hasActorType "Hacktivist"^^xsd:string ;
    ns2:hasCountry "Norway"^^xsd:string ;
    ns2:hasEventDate "2014-07-09T00:00:00"^^xsd:dateTime ;
    ns2:hasEventSubtype "External Denial of Service"^^xsd:string ;
    ns2:hasEventType "Disruptive"^^xsd:string ;
    ns2:hasIndustry "Finance and Insurance"^^xsd:string ;
    ns2:hasMonth 7 ;
    ns2:hasOrganization "Gjensidige"^^xsd:string ;
    ns2:hasYear 2014 ;
    ns2:isType_of ns2:External_Denial_of_Service,
        ns2:Hacktivist ;
    rdfs:comment "Anonymous Norway starts multiple DDoS attacks towards major banks and insurance companies in Norway, including the country's largest telecommunications company, Telenor."^^xsd:string .

ns2:967c92f836e90630 a ns2:AttackWebsite,
        owl:NamedIndividual ;
    ns1:associatedCampaigns ns2:Riyadh_Principality_magazine_website ;
    ns1:description "Protest"^^xsd:string ;
    ns1:isLaunchedBy ns2:Syrian_Arab_Republic ;
    ns2:behaviour ns2:Protest ;
    ns2:hasActor "Syrian Electronic Army"^^xsd:string ;
    ns2:hasActorCountry "Syrian Arab Republic"^^xsd:string ;
    ns2:hasActorType "Hacktivist"^^xsd:string ;
    ns2:hasCountry "Saudi Arabia"^^xsd:string ;
    ns2:hasEventDate "2014-01-16T00:00:00"^^xsd:dateTime ;
    ns2:hasEventSubtype "Message Manipulation"^^xsd:string ;
    ns2:hasEventType "Disruptive"^^xsd:string ;
    ns2:hasIndustry "Public Administration"^^xsd:string ;
    ns2:hasMonth 1 ;
    ns2:hasOrganization "Riyadh Principality magazine website"^^xsd:string ;
    ns2:hasYear 2014 ;
    ns2:isType_of ns2:Hacktivist,
        ns2:Message_Manipulation ;
    rdfs:comment "The Syrian Electronic Army deface 16 Saudi Arabian government websites. The targeted sites are the ones of various administrative regions."^^xsd:string .

ns2:9690e16247e03209 a ns2:DDoS,
        owl:NamedIndividual ;
    ns1:associatedCampaigns ns2:PassthePopcorn_me ;
    ns2:hasActorType "Criminal"^^xsd:string ;
    ns2:hasEventDate "2014-01-06T00:00:00"^^xsd:dateTime ;
    ns2:hasEventSubtype "External Denial of Service"^^xsd:string ;
    ns2:hasEventType "Disruptive"^^xsd:string ;
    ns2:hasIndustry "Other Services (except Public Administration)"^^xsd:string ;
    ns2:hasMonth 1 ;
    ns2:hasOrganization "PassthePopcorn.me"^^xsd:string ;
    ns2:hasYear 2014 ;
    ns2:isType_of ns2:Criminal,
        ns2:External_Denial_of_Service ;
    rdfs:comment "Three of the largest private BitTorrent trackers are offline due to prolonged DDoS attacks. The targets are: What.cd, Broadcasthe.net, PassthePopcorn.me."^^xsd:string .

ns2:96958edb3e49bff8 a ns2:HackerSecurity,
        owl:NamedIndividual ;
    ns1:associatedCampaigns ns2:Various_Government_Websites ;
    ns1:isLaunchedBy ns2:Turkey ;
    ns2:hasActor "RedHack"^^xsd:string ;
    ns2:hasActorCountry "Turkey"^^xsd:string ;
    ns2:hasActorType "Hacktivist"^^xsd:string ;
    ns2:hasCountry "Turkey"^^xsd:string ;
    ns2:hasEventDate "2014-01-11T00:00:00"^^xsd:dateTime ;
    ns2:hasEventSubtype "Exploitation of Application Server"^^xsd:string ;
    ns2:hasEventType "Exploitive"^^xsd:string ;
    ns2:hasIndustry "Public Administration"^^xsd:string ;
    ns2:hasMonth 1 ;
    ns2:hasOrganization "Various Government Websites"^^xsd:string ;
    ns2:hasYear 2014 ;
    ns2:isType_of ns2:Exploitation_of_Application_Server,
        ns2:Hacktivist ;
    rdfs:comment "The Infamous RedHack collective hacks the country's Parliament, the Turkish Contractors Association, the Turkish State Railways (TCDD) and the Justice and Development Party (AKP)."^^xsd:string .

ns2:97695ae691196d74 a ns1:MaliciousCodeExecution,
        owl:NamedIndividual ;
    ns1:associatedCampaigns ns2:National_Health_Service ;
    ns2:hasActorType "Criminal"^^xsd:string ;
    ns2:hasCountry "United Kingdom of Great Britain and Northern Ireland"^^xsd:string ;
    ns2:hasEventDate "2014-02-03T00:00:00"^^xsd:dateTime ;
    ns2:hasEventSubtype "Exploitation of Application Server"^^xsd:string ;
    ns2:hasEventType "Exploitive"^^xsd:string ;
    ns2:hasIndustry "Health Care and Social Assistance"^^xsd:string ;
    ns2:hasMonth 2 ;
    ns2:hasOrganization "National Health Service"^^xsd:string ;
    ns2:hasYear 2014 ;
    ns2:isType_of ns2:Criminal,
        ns2:Exploitation_of_Application_Server ;
    rdfs:comment "A coding error on the official website of the United Kingdom's National Health Service (nhs.uk) is abused to implant malicious code on more than 800 pages."^^xsd:string .

ns2:97b63102fda86ab6 a ns2:BreachInformation,
        owl:NamedIndividual ;
    ns1:associatedCampaigns ns2:Shelburne_Country_Store ;
    ns1:description "Financial"^^xsd:string ;
    ns2:behaviour ns2:Financial ;
    ns2:hasActorType "Criminal"^^xsd:string ;
    ns2:hasCampaign ns2:Vermont ;
    ns2:hasCountry "United States of America"^^xsd:string ;
    ns2:hasCounty "Chittenden"^^xsd:string ;
    ns2:hasEventDate "2014-03-26T00:00:00"^^xsd:dateTime ;
    ns2:hasEventSubtype "Exploitation of Application Server"^^xsd:string ;
    ns2:hasEventType "Exploitive"^^xsd:string ;
    ns2:hasIndustry "Retail Trade"^^xsd:string ;
    ns2:hasMonth 3 ;
    ns2:hasOrganization "Shelburne Country Store"^^xsd:string ;
    ns2:hasState "Vermont"^^xsd:string ;
    ns2:hasYear 2014 ;
    ns2:isType_of ns2:Criminal,
        ns2:Exploitation_of_Application_Server ;
    rdfs:comment "Shelburne Country Store notifies an undisclosed number of online customers that their credit card information may have been exposed when the store's payment processing system was breached."^^xsd:string .

ns2:98504b09072946b3 a ns2:BreachInformation,
        owl:NamedIndividual ;
    ns1:associatedCampaigns ns2:Experian ;
    ns1:description "Financial"^^xsd:string ;
    ns2:behaviour ns2:Financial ;
    ns2:hasActorType "Criminal"^^xsd:string ;
    ns2:hasCampaign ns2:California ;
    ns2:hasCountry "United States of America"^^xsd:string ;
    ns2:hasCounty "Orange"^^xsd:string ;
    ns2:hasEventDate "2014-01-30T00:00:00"^^xsd:dateTime ;
    ns2:hasEventSubtype "Exploitation of Application Server"^^xsd:string ;
    ns2:hasEventType "Exploitive"^^xsd:string ;
    ns2:hasIndustry "Administrative and Support and Waste Management and Remediation Services"^^xsd:string ;
    ns2:hasMonth 1 ;
    ns2:hasOrganization "Experian"^^xsd:string ;
    ns2:hasState "California"^^xsd:string ;
    ns2:hasYear 2014 ;
    ns2:isType_of ns2:Criminal,
        ns2:Exploitation_of_Application_Server ;
    rdfs:comment "Experian notifies that an unauthorized access to the consumers' credit reports in Experian's database occurred between January 30 and January 31, and would have involved name and address as well as one or more of  date of birth, Social Security numbers, account information, and whatever information you'd find in a credit report."^^xsd:string .

ns2:9894cecb8a120c7c a ns2:HackerSecurity,
        owl:NamedIndividual ;
    ns1:associatedCampaigns ns2:Deltek ;
    ns1:description "Financial"^^xsd:string ;
    ns2:behaviour ns2:Financial ;
    ns2:hasActorType "Criminal"^^xsd:string ;
    ns2:hasCampaign ns2:Virginia ;
    ns2:hasCountry "United States of America"^^xsd:string ;
    ns2:hasCounty "Fairfax"^^xsd:string ;
    ns2:hasEventDate "2014-04-09T00:00:00"^^xsd:dateTime ;
    ns2:hasEventSubtype "Exploitation of Application Server"^^xsd:string ;
    ns2:hasEventType "Exploitive"^^xsd:string ;
    ns2:hasIndustry "Professional, Scientific, and Technical Services"^^xsd:string ;
    ns2:hasMonth 4 ;
    ns2:hasOrganization "Deltek"^^xsd:string ;
    ns2:hasState "Virginia"^^xsd:string ;
    ns2:hasYear 2014 ;
    ns2:isType_of ns2:Criminal,
        ns2:Exploitation_of_Application_Server ;
    rdfs:comment "An unknown attacker hacks into the GovWin IQ system run by Deltek, and compromises the credentials of roughly 80,000 customers, including payment card data for about 25,000 of those individuals."^^xsd:string .

ns2:98f2fe654de002e9 a ns2:BreachSecurity,
        owl:NamedIndividual ;
    ns1:associatedCampaigns ns2:Bell_Canada ;
    ns2:hasActor "NullCrew"^^xsd:string ;
    ns2:hasActorType "Hacktivist"^^xsd:string ;
    ns2:hasCountry "Canada"^^xsd:string ;
    ns2:hasEventDate "2014-02-01T00:00:00"^^xsd:dateTime ;
    ns2:hasEventSubtype "Exploitation of Application Server"^^xsd:string ;
    ns2:hasEventType "Exploitive"^^xsd:string ;
    ns2:hasIndustry "Information"^^xsd:string ;
    ns2:hasMonth 2 ;
    ns2:hasOrganization "Bell Canada"^^xsd:string ;
    ns2:hasYear 2014 ;
    ns2:isType_of ns2:Exploitation_of_Application_Server,
        ns2:Hacktivist ;
    rdfs:comment "The hacking group NullCrew AKA @NullCrew_FTS claims to have successfully hacked Bell Canada (bell.ca). As a consequence 40,000 credentials are leaked."^^xsd:string .

ns2:99394c91e7407901 a ns2:HackerSecurity,
        owl:NamedIndividual ;
    ns1:associatedCampaigns ns2:Vodafone ;
    ns1:description "Protest"^^xsd:string ;
    ns1:isLaunchedBy ns2:Turkey ;
    ns2:behaviour ns2:Protest ;
    ns2:hasActor "RedHack"^^xsd:string ;
    ns2:hasActorCountry "Turkey"^^xsd:string ;
    ns2:hasActorType "Hacktivist"^^xsd:string ;
    ns2:hasCountry "Turkey"^^xsd:string ;
    ns2:hasEventDate "2014-02-04T00:00:00"^^xsd:dateTime ;
    ns2:hasEventSubtype "Exploitation of Application Server"^^xsd:string ;
    ns2:hasEventType "Exploitive"^^xsd:string ;
    ns2:hasIndustry "Information"^^xsd:string ;
    ns2:hasMonth 2 ;
    ns2:hasOrganization "Vodafone"^^xsd:string ;
    ns2:hasYear 2014 ;
    ns2:isType_of ns2:Exploitation_of_Application_Server,
        ns2:Hacktivist ;
    rdfs:comment "Hackers of the RedHack group claim to have breached the systems of three major telecoms companies: TTNET, Vodafone and Turkcell. After the attack they leak the details of hundreds of individuals from TTNET and 5,000 Vodafone customers."^^xsd:string .

ns2:9a375fe097db7bd9 a ns2:CyberattackInformation,
        owl:NamedIndividual ;
    ns1:associatedCampaigns ns2:Indian_Railways ;
    ns1:isLaunchedBy ns2:Pakistan ;
    ns2:hasActor "H4$N4!N H4XOR"^^xsd:string ;
    ns2:hasActorCountry "Pakistan"^^xsd:string ;
    ns2:hasActorType "Hacktivist"^^xsd:string ;
    ns2:hasCountry "India"^^xsd:string ;
    ns2:hasEventDate "2014-01-27T00:00:00"^^xsd:dateTime ;
    ns2:hasEventSubtype "Message Manipulation"^^xsd:string ;
    ns2:hasEventType "Disruptive"^^xsd:string ;
    ns2:hasIndustry "Transportation and Warehousing"^^xsd:string ;
    ns2:hasMonth 1 ;
    ns2:hasOrganization "Indian Railways"^^xsd:string ;
    ns2:hasYear 2014 ;
    ns2:isType_of ns2:Hacktivist,
        ns2:Message_Manipulation ;
    rdfs:comment "Another episode of the Cyber War between India and Pakistan. The official website of the Indian Railways is once again defaced by Pakistani Hackers."^^xsd:string .

ns2:9b397716d1140be7 a ns2:BreachInformation,
        owl:NamedIndividual ;
    ns1:associatedCampaigns ns2:Rowan_Companies ;
    ns1:description "Financial"^^xsd:string ;
    ns2:behaviour ns2:Financial ;
    ns2:hasActorType "Criminal"^^xsd:string ;
    ns2:hasCampaign ns2:Texas ;
    ns2:hasCountry "United States of America"^^xsd:string ;
    ns2:hasCounty "Harris"^^xsd:string ;
    ns2:hasEventDate "2014-06-08T00:00:00"^^xsd:dateTime ;
    ns2:hasEventSubtype "Exploitation of Application Server"^^xsd:string ;
    ns2:hasEventType "Exploitive"^^xsd:string ;
    ns2:hasIndustry "Mining, Quarrying, and Oil and Gas Extraction"^^xsd:string ;
    ns2:hasMonth 6 ;
    ns2:hasOrganization "Rowan Companies"^^xsd:string ;
    ns2:hasState "Texas"^^xsd:string ;
    ns2:hasYear 2014 ;
    ns2:isType_of ns2:Criminal,
        ns2:Exploitation_of_Application_Server ;
    rdfs:comment "Rowan Companies notifies employees, vendors, and contractors of a system intrusion."^^xsd:string .

ns2:9c102687afe1efc9 a ns2:HackerSecurity,
        owl:NamedIndividual ;
    ns1:associatedCampaigns ns2:Gateway_Savings_and_Loans_Limited ;
    ns1:description "Financial"^^xsd:string ;
    ns2:behaviour ns2:Financial ;
    ns2:hasActorType "Criminal"^^xsd:string ;
    ns2:hasCountry "Nigeria"^^xsd:string ;
    ns2:hasEventDate "2014-07-04T00:00:00"^^xsd:dateTime ;
    ns2:hasEventSubtype "Exploitation of Application Server"^^xsd:string ;
    ns2:hasEventType "Exploitive"^^xsd:string ;
    ns2:hasIndustry "Finance and Insurance"^^xsd:string ;
    ns2:hasMonth 7 ;
    ns2:hasOrganization "Gateway Savings and Loans Limited"^^xsd:string ;
    ns2:hasYear 2014 ;
    ns2:isType_of ns2:Criminal,
        ns2:Exploitation_of_Application_Server ;
    rdfs:comment "Nigerian Police investigates a multi-million fraud by unknown hackers, reportedly hacking into Ogun State-owned mortgage bank, Gateway Savings and Loans Limited, and stealing millions of Naira."^^xsd:string .

ns2:9c2cfdbaaab73780 a ns2:AnonymousAttack,
        owl:NamedIndividual ;
    ns1:associatedCampaigns ns2:Sparebank_1 ;
    ns1:description "Protest"^^xsd:string ;
    ns1:isLaunchedBy ns2:Norway ;
    ns2:behaviour ns2:Protest ;
    ns2:hasActor "Anonymous (Norway)"^^xsd:string ;
    ns2:hasActorCountry "Norway"^^xsd:string ;
    ns2:hasActorType "Hacktivist"^^xsd:string ;
    ns2:hasCountry "Norway"^^xsd:string ;
    ns2:hasEventDate "2014-07-09T00:00:00"^^xsd:dateTime ;
    ns2:hasEventSubtype "External Denial of Service"^^xsd:string ;
    ns2:hasEventType "Disruptive"^^xsd:string ;
    ns2:hasIndustry "Finance and Insurance"^^xsd:string ;
    ns2:hasMonth 7 ;
    ns2:hasOrganization "Sparebank 1"^^xsd:string ;
    ns2:hasYear 2014 ;
    ns2:isType_of ns2:External_Denial_of_Service,
        ns2:Hacktivist ;
    rdfs:comment "Anonymous Norway starts multiple DDoS attacks towards major banks and insurance companies in Norway, including the country's largest telecommunications company, Telenor."^^xsd:string .

ns2:9d5164978e1a86fc a ns2:CyberattackData,
        owl:NamedIndividual ;
    ns1:associatedCampaigns ns2:United_Nations_Integrated_Civil_Society_ ;
    ns1:description "Protest"^^xsd:string ;
    ns1:isLaunchedBy ns2:Turkey ;
    ns2:behaviour ns2:Protest ;
    ns2:hasActor "Turk Guvengligi"^^xsd:string ;
    ns2:hasActorCountry "Turkey"^^xsd:string ;
    ns2:hasActorType "Hacktivist"^^xsd:string ;
    ns2:hasEventDate "2014-07-23T00:00:00"^^xsd:dateTime ;
    ns2:hasEventSubtype "Message Manipulation"^^xsd:string ;
    ns2:hasEventType "Disruptive"^^xsd:string ;
    ns2:hasIndustry "Public Administration"^^xsd:string ;
    ns2:hasMonth 7 ;
    ns2:hasOrganization "United Nations Integrated Civil Society Organizations System"^^xsd:string ;
    ns2:hasYear 2014 ;
    ns2:isType_of ns2:Hacktivist,
        ns2:Message_Manipulation ;
    rdfs:comment "Again an attack in name of #OpSaveGaza. A Turkish hacker going with the handle of Turk Guvenligi defaces two official sub-domains of the United Nations: esango.un.org and escwa.un.org."^^xsd:string .

ns2:9f3ca4c32b7ef821 a ns2:AttackWebsite,
        owl:NamedIndividual ;
    ns1:associatedCampaigns ns2:Website_of_the_Connecticut_Governor ;
    ns1:description "Protest"^^xsd:string ;
    ns2:behaviour ns2:Protest ;
    ns2:hasActor "AnonGhost"^^xsd:string ;
    ns2:hasActorType "Hacktivist"^^xsd:string ;
    ns2:hasCampaign ns2:Connecticut ;
    ns2:hasCountry "United States of America"^^xsd:string ;
    ns2:hasCounty "Hartford"^^xsd:string ;
    ns2:hasEventDate "2014-07-31T00:00:00"^^xsd:dateTime ;
    ns2:hasEventSubtype "Message Manipulation"^^xsd:string ;
    ns2:hasEventType "Disruptive"^^xsd:string ;
    ns2:hasIndustry "Public Administration"^^xsd:string ;
    ns2:hasMonth 7 ;
    ns2:hasOrganization "Website of the Connecticut Governor"^^xsd:string ;
    ns2:hasState "Connecticut"^^xsd:string ;
    ns2:hasYear 2014 ;
    ns2:isType_of ns2:Hacktivist,
        ns2:Message_Manipulation ;
    rdfs:comment "In name of #OpSaveGaza, AnonGhost, defaces the official web portal of State of Connecticut (ct.gov) along with the website of Connecticut's Governor (governor.ct.gov)."^^xsd:string .

ns2:9f51184a30058d54 a ns2:BreachSecurity,
        owl:NamedIndividual ;
    ns1:associatedCampaigns ns2:American_Institutes_for_Research ;
    ns2:hasActorType "Criminal"^^xsd:string ;
    ns2:hasCampaign ns2:Washington_D_C ;
    ns2:hasCountry "United States of America"^^xsd:string ;
    ns2:hasEventDate "2014-05-21T00:00:00"^^xsd:dateTime ;
    ns2:hasEventSubtype "Exploitation of Application Server"^^xsd:string ;
    ns2:hasEventType "Exploitive"^^xsd:string ;
    ns2:hasIndustry "Other Services (except Public Administration)"^^xsd:string ;
    ns2:hasMonth 5 ;
    ns2:hasOrganization "American Institutes for Research"^^xsd:string ;
    ns2:hasState "Washington D.C."^^xsd:string ;
    ns2:hasYear 2014 ;
    ns2:isType_of ns2:Criminal,
        ns2:Exploitation_of_Application_Server ;
    rdfs:comment "About 6,500 current and former employees of the American Institutes for Research (AIR) may have had personal information compromised after unauthorized access was gained to one of the organization's servers."^^xsd:string .

ns2:9fb05008cd7721e7 a ns2:DDoS,
        owl:NamedIndividual ;
    ns1:associatedCampaigns ns2:Steam ;
    ns2:hasActorType "Criminal"^^xsd:string ;
    ns2:hasCampaign ns2:Washington ;
    ns2:hasCountry "United States of America"^^xsd:string ;
    ns2:hasCounty "King"^^xsd:string ;
    ns2:hasEventDate "2014-01-03T00:00:00"^^xsd:dateTime ;
    ns2:hasEventSubtype "External Denial of Service"^^xsd:string ;
    ns2:hasEventType "Disruptive"^^xsd:string ;
    ns2:hasIndustry "Information"^^xsd:string ;
    ns2:hasMonth 1 ;
    ns2:hasOrganization "Steam"^^xsd:string ;
    ns2:hasState "Washington"^^xsd:string ;
    ns2:hasYear 2014 ;
    ns2:isType_of ns2:Criminal,
        ns2:External_Denial_of_Service ;
    rdfs:comment "The servers for Steam, Origin, Battle.net, League of Legends, and several other gaming platforms are brought down temporarily by apparent DDoS attacks that seem to be related to a swatting attack on an individual known for streaming games."^^xsd:string .

ns2:9fee96668b8df8d4 a ns2:HackerUser,
        owl:NamedIndividual ;
    ns1:associatedCampaigns ns2:Griminal ;
    ns2:hasActorType "Criminal"^^xsd:string ;
    ns2:hasCountry "United Kingdom of Great Britain and Northern Ireland"^^xsd:string ;
    ns2:hasEventDate "2014-02-24T00:00:00"^^xsd:dateTime ;
    ns2:hasEventSubtype "Message Manipulation"^^xsd:string ;
    ns2:hasEventType "Disruptive"^^xsd:string ;
    ns2:hasIndustry "Other Services (except Public Administration)"^^xsd:string ;
    ns2:hasMonth 2 ;
    ns2:hasOrganization "Griminal"^^xsd:string ;
    ns2:hasYear 2014 ;
    ns2:isType_of ns2:Criminal,
        ns2:Message_Manipulation ;
    rdfs:comment "Rapper Griminal's Twitter account is hacked and posts suicidal tweets, worrying his fans."^^xsd:string .

ns2:AbleAccess a owl:Class ;
    rdfs:label "able access"^^xsd:string ;
    rdfs:comment "Formal definition for AbleAccess within the cybersecurity domain."^^xsd:string ;
    rdfs:subClassOf ns1:RemoteAccess .

ns2:AccessBreach a owl:Class ;
    rdfs:label "access breach"^^xsd:string ;
    rdfs:comment "Formal definition for AccessBreach within the cybersecurity domain."^^xsd:string ;
    rdfs:subClassOf ns2:Exploit .

ns2:AccessHacker a owl:Class ;
    rdfs:label "access hacker"^^xsd:string ;
    rdfs:comment "Formal definition for AccessHacker within the cybersecurity domain."^^xsd:string ;
    rdfs:subClassOf ns2:Exploit .

ns2:AccessNetwork a owl:Class ;
    rdfs:label "access network"^^xsd:string ;
    rdfs:comment "Formal definition for AccessNetwork within the cybersecurity domain."^^xsd:string ;
    rdfs:subClassOf ns1:RemoteAccess .

ns2:AccessService a owl:Class ;
    rdfs:label "access service"^^xsd:string ;
    rdfs:comment "Formal definition for AccessService within the cybersecurity domain."^^xsd:string ;
    rdfs:subClassOf ns1:RemoteAccess .

ns2:AccessSystem a owl:Class ;
    rdfs:label "access system"^^xsd:string ;
    rdfs:comment "Formal definition for AccessSystem within the cybersecurity domain."^^xsd:string ;
    rdfs:subClassOf ns1:System .

ns2:AccountEmployee a owl:Class ;
    rdfs:label "account employee"^^xsd:string ;
    rdfs:comment "Formal definition for AccountEmployee within the cybersecurity domain."^^xsd:string ;
    rdfs:subClassOf ns2:Account .

ns2:AccountGroup a owl:Class ;
    rdfs:label "account group"^^xsd:string ;
    rdfs:comment "Formal definition for AccountGroup within the cybersecurity domain."^^xsd:string ;
    rdfs:subClassOf ns2:BaseGroup .

ns2:AccountInformation a owl:Class ;
    rdfs:label "account information"^^xsd:string ;
    rdfs:comment "Formal definition for AccountInformation within the cybersecurity domain."^^xsd:string ;
    rdfs:subClassOf ns2:Account .

ns2:AccountUser a owl:Class ;
    rdfs:label "account user"^^xsd:string ;
    rdfs:comment "Formal definition for AccountUser within the cybersecurity domain."^^xsd:string ;
    rdfs:subClassOf ns1:UnauthUser .

ns2:ActorMalware a owl:Class ;
    rdfs:label "actor malware"^^xsd:string ;
    rdfs:comment "Formal definition for ActorMalware within the cybersecurity domain."^^xsd:string ;
    rdfs:subClassOf ns2:Malware .

ns2:ActorSystem a owl:Class ;
    rdfs:label "actor system"^^xsd:string ;
    rdfs:comment "Formal definition for ActorSystem within the cybersecurity domain."^^xsd:string ;
    rdfs:subClassOf ns1:System .

ns2:ActorVictim a owl:Class ;
    rdfs:label "actor victim"^^xsd:string ;
    rdfs:comment "Formal definition for ActorVictim within the cybersecurity domain."^^xsd:string ;
    rdfs:subClassOf ns2:Victim .

ns2:AddressData a owl:Class ;
    rdfs:label "address data"^^xsd:string ;
    rdfs:comment "Formal definition for AddressData within the cybersecurity domain."^^xsd:string ;
    rdfs:subClassOf ns1:Address .

ns2:AddressEmail a owl:Class ;
    rdfs:label "address email"^^xsd:string ;
    rdfs:comment "Formal definition for AddressEmail within the cybersecurity domain."^^xsd:string ;
    rdfs:subClassOf ns1:Address .

ns2:AddressName a owl:Class ;
    rdfs:label "address name"^^xsd:string ;
    rdfs:comment "Formal definition for AddressName within the cybersecurity domain."^^xsd:string ;
    rdfs:subClassOf ns1:Address .

ns2:AddressNumber a owl:Class ;
    rdfs:label "address number"^^xsd:string ;
    rdfs:comment "Formal definition for AddressNumber within the cybersecurity domain."^^xsd:string ;
    rdfs:subClassOf ns1:Address .

ns2:AllegedlyData a owl:Class ;
    rdfs:label "allegedly data"^^xsd:string ;
    rdfs:comment "Formal definition for AllegedlyData within the cybersecurity domain."^^xsd:string ;
    rdfs:subClassOf ns1:DataCorruption .

ns2:AmongVictim a owl:Class ;
    rdfs:label "among victim"^^xsd:string ;
    rdfs:comment "Formal definition for AmongVictim within the cybersecurity domain."^^xsd:string ;
    rdfs:subClassOf ns2:Victim .

ns2:AnonymousCollective a owl:Class ;
    rdfs:label "anonymous collective"^^xsd:string ;
    rdfs:comment "Formal definition for AnonymousCollective within the cybersecurity domain."^^xsd:string ;
    rdfs:subClassOf ns2:EnvironmentalGroup .

ns2:AttackAttacker a owl:Class ;
    rdfs:label "attack attacker"^^xsd:string ;
    rdfs:comment "Formal definition for AttackAttacker within the cybersecurity domain."^^xsd:string ;
    rdfs:subClassOf ns2:AttackPattern .

ns2:AttackBreach a owl:Class ;
    rdfs:label "attack breach"^^xsd:string ;
    rdfs:comment "Formal definition for AttackBreach within the cybersecurity domain."^^xsd:string ;
    rdfs:subClassOf ns2:Exploit .

ns2:AttackClaim a owl:Class ;
    rdfs:label "attack claim"^^xsd:string ;
    rdfs:comment "Formal definition for AttackClaim within the cybersecurity domain."^^xsd:string ;
    rdfs:subClassOf ns2:AttackPattern .

ns2:AttackCollective a owl:Class ;
    rdfs:label "attack collective"^^xsd:string ;
    rdfs:comment "Formal definition for AttackCollective within the cybersecurity domain."^^xsd:string ;
    rdfs:subClassOf ns2:AttackPattern .

ns2:AttackCompany a owl:Class ;
    rdfs:label "attack company"^^xsd:string ;
    rdfs:comment "Formal definition for AttackCompany within the cybersecurity domain."^^xsd:string ;
    rdfs:subClassOf ns2:AttackPattern .

ns2:AttackComputer a owl:Class ;
    rdfs:label "attack computer"^^xsd:string ;
    rdfs:comment "Formal definition for AttackComputer within the cybersecurity domain."^^xsd:string ;
    rdfs:subClassOf ns2:Exploit .

ns2:AttackCyber a owl:Class ;
    rdfs:label "attack cyber"^^xsd:string ;
    rdfs:comment "Formal definition for AttackCyber within the cybersecurity domain."^^xsd:string ;
    rdfs:subClassOf ns1:BotnetAttack .

ns2:AttackData a owl:Class ;
    rdfs:label "attack data"^^xsd:string ;
    rdfs:comment "Formal definition for AttackData within the cybersecurity domain."^^xsd:string ;
    rdfs:subClassOf ns2:AttackPattern .

ns2:AttackDay a owl:Class ;
    rdfs:label "attack day"^^xsd:string ;
    rdfs:comment "Formal definition for AttackDay within the cybersecurity domain."^^xsd:string ;
    rdfs:subClassOf ns2:AttackPattern .

ns2:AttackDdos a owl:Class ;
    rdfs:label "attack ddos"^^xsd:string ;
    rdfs:comment "Formal definition for AttackDdos within the cybersecurity domain."^^xsd:string ;
    rdfs:subClassOf ns2:DDoS .

ns2:AttackDistrict a owl:Class ;
    rdfs:label "attack district"^^xsd:string ;
    rdfs:comment "Formal definition for AttackDistrict within the cybersecurity domain."^^xsd:string ;
    rdfs:subClassOf ns2:AttackPattern .

ns2:AttackFile a owl:Class ;
    rdfs:label "attack file"^^xsd:string ;
    rdfs:comment "Formal definition for AttackFile within the cybersecurity domain."^^xsd:string ;
    rdfs:subClassOf ns2:AttackPattern .

ns2:AttackGang a owl:Class ;
    rdfs:label "attack gang"^^xsd:string ;
    rdfs:comment "Formal definition for AttackGang within the cybersecurity domain."^^xsd:string ;
    rdfs:subClassOf ns2:AttackPattern .

ns2:AttackHacker a owl:Class ;
    rdfs:label "attack hacker"^^xsd:string ;
    rdfs:comment "Formal definition for AttackHacker within the cybersecurity domain."^^xsd:string ;
    rdfs:subClassOf ns2:Exploit .

ns2:AttackHealth a owl:Class ;
    rdfs:label "attack health"^^xsd:string ;
    rdfs:comment "Formal definition for AttackHealth within the cybersecurity domain."^^xsd:string ;
    rdfs:subClassOf ns1:Vulnerability .

ns2:AttackMinistry a owl:Class ;
    rdfs:label "attack ministry"^^xsd:string ;
    rdfs:comment "Formal definition for AttackMinistry within the cybersecurity domain."^^xsd:string ;
    rdfs:subClassOf ns2:AttackPattern .

ns2:AttackNetwork a owl:Class ;
    rdfs:label "attack network"^^xsd:string ;
    rdfs:comment "Formal definition for AttackNetwork within the cybersecurity domain."^^xsd:string ;
    rdfs:subClassOf ns1:BotnetAttack .

ns2:AttackNoname a owl:Class ;
    rdfs:label "attack noname"^^xsd:string ;
    rdfs:comment "Formal definition for AttackNoname within the cybersecurity domain."^^xsd:string ;
    rdfs:subClassOf ns2:AttackPattern .

ns2:AttackNotifies a owl:Class ;
    rdfs:label "attack notifies"^^xsd:string ;
    rdfs:comment "Formal definition for AttackNotifies within the cybersecurity domain."^^xsd:string ;
    rdfs:subClassOf ns2:AttackPattern .

ns2:AttackOfficial a owl:Class ;
    rdfs:label "attack official"^^xsd:string ;
    rdfs:comment "Formal definition for AttackOfficial within the cybersecurity domain."^^xsd:string ;
    rdfs:subClassOf ns2:AttackPattern .

ns2:AttackOperation a owl:Class ;
    rdfs:label "attack operation"^^xsd:string ;
    rdfs:comment "Formal definition for AttackOperation within the cybersecurity domain."^^xsd:string ;
    rdfs:subClassOf ns2:Exploit .

ns2:AttackOrganization a owl:Class ;
    rdfs:label "attack organization"^^xsd:string ;
    rdfs:comment "Formal definition for AttackOrganization within the cybersecurity domain."^^xsd:string ;
    rdfs:subClassOf ns2:AttackPattern .

ns2:AttackPatient a owl:Class ;
    rdfs:label "attack patient"^^xsd:string ;
    rdfs:comment "Formal definition for AttackPatient within the cybersecurity domain."^^xsd:string ;
    rdfs:subClassOf ns2:AttackPattern .

ns2:AttackPeople a owl:Class ;
    rdfs:label "attack people"^^xsd:string ;
    rdfs:comment "Formal definition for AttackPeople within the cybersecurity domain."^^xsd:string ;
    rdfs:subClassOf ns2:AttackPattern .

ns2:AttackProvider a owl:Class ;
    rdfs:label "attack provider"^^xsd:string ;
    rdfs:comment "Formal definition for AttackProvider within the cybersecurity domain."^^xsd:string ;
    rdfs:subClassOf ns2:AttackPattern .

ns2:AttackResponsibility a owl:Class ;
    rdfs:label "attack responsibility"^^xsd:string ;
    rdfs:comment "Formal definition for AttackResponsibility within the cybersecurity domain."^^xsd:string ;
    rdfs:subClassOf ns2:AttackPattern .

ns2:AttackServer a owl:Class ;
    rdfs:label "attack server"^^xsd:string ;
    rdfs:comment "Formal definition for AttackServer within the cybersecurity domain."^^xsd:string ;
    rdfs:subClassOf ns1:BotnetAttack .

ns2:AttackService a owl:Class ;
    rdfs:label "attack service"^^xsd:string ;
    rdfs:comment "Formal definition for AttackService within the cybersecurity domain."^^xsd:string ;
    rdfs:subClassOf ns2:AttackPattern .

ns2:AttackState a owl:Class ;
    rdfs:label "attack state"^^xsd:string ;
    rdfs:comment "Formal definition for AttackState within the cybersecurity domain."^^xsd:string ;
    rdfs:subClassOf ns2:AttackPattern .

ns2:AttackSystem a owl:Class ;
    rdfs:label "attack system"^^xsd:string ;
    rdfs:comment "Formal definition for AttackSystem within the cybersecurity domain."^^xsd:string ;
    rdfs:subClassOf ns1:System .

ns2:AttackTarget a owl:Class ;
    rdfs:label "attack target"^^xsd:string ;
    rdfs:comment "Formal definition for AttackTarget within the cybersecurity domain."^^xsd:string ;
    rdfs:subClassOf ns2:AttackPattern .

ns2:AttackThreat a owl:Class ;
    rdfs:label "attack threat"^^xsd:string ;
    rdfs:comment "Formal definition for AttackThreat within the cybersecurity domain."^^xsd:string ;
    rdfs:subClassOf ns2:AttackPattern .

ns2:AttackTwo a owl:Class ;
    rdfs:label "attack two"^^xsd:string ;
    rdfs:comment "Formal definition for AttackTwo within the cybersecurity domain."^^xsd:string ;
    rdfs:subClassOf ns2:AttackPattern .

ns2:AttackVictim a owl:Class ;
    rdfs:label "attack victim"^^xsd:string ;
    rdfs:comment "Formal definition for AttackVictim within the cybersecurity domain."^^xsd:string ;
    rdfs:subClassOf ns2:Victim .

ns2:BreachComputer a owl:Class ;
    rdfs:label "breach computer"^^xsd:string ;
    rdfs:comment "Formal definition for BreachComputer within the cybersecurity domain."^^xsd:string ;
    rdfs:subClassOf ns2:Exploit .

ns2:BreachFile a owl:Class ;
    rdfs:label "breach file"^^xsd:string ;
    rdfs:comment "Formal definition for BreachFile within the cybersecurity domain."^^xsd:string ;
    rdfs:subClassOf ns2:Exploit .

ns2:BreachGroup a owl:Class ;
    rdfs:label "breach group"^^xsd:string ;
    rdfs:comment "Formal definition for BreachGroup within the cybersecurity domain."^^xsd:string ;
    rdfs:subClassOf ns2:BaseGroup .

ns2:BreachHacker a owl:Class ;
    rdfs:label "breach hacker"^^xsd:string ;
    rdfs:comment "Formal definition for BreachHacker within the cybersecurity domain."^^xsd:string ;
    rdfs:subClassOf ns2:Exploit .

ns2:BreachSensitive a owl:Class ;
    rdfs:label "breach sensitive"^^xsd:string ;
    rdfs:comment "Formal definition for BreachSensitive within the cybersecurity domain."^^xsd:string ;
    rdfs:subClassOf ns1:Vulnerability .

ns2:BreachSystem a owl:Class ;
    rdfs:label "breach system"^^xsd:string ;
    rdfs:comment "Formal definition for BreachSystem within the cybersecurity domain."^^xsd:string ;
    rdfs:subClassOf ns1:System .

ns2:BreachThreat a owl:Class ;
    rdfs:label "breach threat"^^xsd:string ;
    rdfs:comment "Formal definition for BreachThreat within the cybersecurity domain."^^xsd:string ;
    rdfs:subClassOf ns1:Vulnerability .

ns2:BreachVictim a owl:Class ;
    rdfs:label "breach victim"^^xsd:string ;
    rdfs:comment "Formal definition for BreachVictim within the cybersecurity domain."^^xsd:string ;
    rdfs:subClassOf ns2:Victim .

ns2:BreachVulnerability a owl:Class ;
    rdfs:label "breach vulnerability"^^xsd:string ;
    rdfs:comment "Formal definition for BreachVulnerability within the cybersecurity domain."^^xsd:string ;
    rdfs:subClassOf ns2:Exploit .

ns2:CompanyComputer a owl:Class ;
    rdfs:label "company computer"^^xsd:string ;
    rdfs:comment "Formal definition for CompanyComputer within the cybersecurity domain."^^xsd:string ;
    rdfs:subClassOf ns1:Software .

ns2:CompanyCyberattack a owl:Class ;
    rdfs:label "company cyberattack"^^xsd:string ;
    rdfs:comment "Formal definition for CompanyCyberattack within the cybersecurity domain."^^xsd:string ;
    rdfs:subClassOf ns1:BotnetAttack .

ns2:CompanyEmail a owl:Class ;
    rdfs:label "company email"^^xsd:string ;
    rdfs:comment "Formal definition for CompanyEmail within the cybersecurity domain."^^xsd:string ;
    rdfs:subClassOf ns1:Address .

ns2:CompanyGroup a owl:Class ;
    rdfs:label "company group"^^xsd:string ;
    rdfs:comment "Formal definition for CompanyGroup within the cybersecurity domain."^^xsd:string ;
    rdfs:subClassOf ns2:EnvironmentalGroup .

ns2:CompanyHacker a owl:Class ;
    rdfs:label "company hacker"^^xsd:string ;
    rdfs:comment "Formal definition for CompanyHacker within the cybersecurity domain."^^xsd:string ;
    rdfs:subClassOf ns2:Exploit .

ns2:CompanyIncident a owl:Class ;
    rdfs:label "company incident"^^xsd:string ;
    rdfs:comment "Formal definition for CompanyIncident within the cybersecurity domain."^^xsd:string ;
    rdfs:subClassOf ns1:Incident .

ns2:CompanyMalware a owl:Class ;
    rdfs:label "company malware"^^xsd:string ;
    rdfs:comment "Formal definition for CompanyMalware within the cybersecurity domain."^^xsd:string ;
    rdfs:subClassOf ns2:Malware .

ns2:CompanySoftware a owl:Class ;
    rdfs:label "company software"^^xsd:string ;
    rdfs:comment "Formal definition for CompanySoftware within the cybersecurity domain."^^xsd:string ;
    rdfs:subClassOf ns1:Software .

ns2:CompanyState a owl:Class ;
    rdfs:label "company state"^^xsd:string ;
    rdfs:comment "Formal definition for CompanyState within the cybersecurity domain."^^xsd:string ;
    rdfs:subClassOf ns1:NetworkState .

ns2:CompanySystem a owl:Class ;
    rdfs:label "company system"^^xsd:string ;
    rdfs:comment "Formal definition for CompanySystem within the cybersecurity domain."^^xsd:string ;
    rdfs:subClassOf ns1:System .

ns2:CompanyVictim a owl:Class ;
    rdfs:label "company victim"^^xsd:string ;
    rdfs:comment "Formal definition for CompanyVictim within the cybersecurity domain."^^xsd:string ;
    rdfs:subClassOf ns2:Victim .

ns2:CompanyWebsite a owl:Class ;
    rdfs:label "company website"^^xsd:string ;
    rdfs:comment "Formal definition for CompanyWebsite within the cybersecurity domain."^^xsd:string ;
    rdfs:subClassOf ns1:Web .

ns2:ComputerData a owl:Class ;
    rdfs:label "computer data"^^xsd:string ;
    rdfs:comment "Formal definition for ComputerData within the cybersecurity domain."^^xsd:string ;
    rdfs:subClassOf ns1:File .

ns2:ComputerFile a owl:Class ;
    rdfs:label "computer file"^^xsd:string ;
    rdfs:comment "Formal definition for ComputerFile within the cybersecurity domain."^^xsd:string ;
    rdfs:subClassOf ns1:File .

ns2:ComputerInformation a owl:Class ;
    rdfs:label "computer information"^^xsd:string ;
    rdfs:comment "Formal definition for ComputerInformation within the cybersecurity domain."^^xsd:string ;
    rdfs:subClassOf ns1:Hardware .

ns2:ComputerNetwork a owl:Class ;
    rdfs:label "computer network"^^xsd:string ;
    rdfs:comment "Formal definition for ComputerNetwork within the cybersecurity domain."^^xsd:string ;
    rdfs:subClassOf ns2:Network .

ns2:ComputerSystem a owl:Class ;
    rdfs:label "computer system"^^xsd:string ;
    rdfs:comment "Formal definition for ComputerSystem within the cybersecurity domain."^^xsd:string ;
    rdfs:subClassOf ns1:System .

ns2:ComputerUnauthorized a owl:Class ;
    rdfs:label "computer unauthorized"^^xsd:string ;
    rdfs:comment "Formal definition for ComputerUnauthorized within the cybersecurity domain."^^xsd:string ;
    rdfs:subClassOf ns2:Malware .

ns2:ConfidentialFile a owl:Class ;
    rdfs:label "confidential file"^^xsd:string ;
    rdfs:comment "Formal definition for ConfidentialFile within the cybersecurity domain."^^xsd:string ;
    rdfs:subClassOf ns1:File .

ns2:CustomerHacker a owl:Class ;
    rdfs:label "customer hacker"^^xsd:string ;
    rdfs:comment "Formal definition for CustomerHacker within the cybersecurity domain."^^xsd:string ;
    rdfs:subClassOf ns2:Exploit .

ns2:CustomerSystem a owl:Class ;
    rdfs:label "customer system"^^xsd:string ;
    rdfs:comment "Formal definition for CustomerSystem within the cybersecurity domain."^^xsd:string ;
    rdfs:subClassOf ns1:System .

ns2:CveVulnerability a owl:Class ;
    rdfs:label "cve vulnerability"^^xsd:string ;
    rdfs:comment "Formal definition for CveVulnerability within the cybersecurity domain."^^xsd:string ;
    rdfs:subClassOf ns1:Vulnerability .

ns2:CyberGroup a owl:Class ;
    rdfs:label "cyber group"^^xsd:string ;
    rdfs:comment "Formal definition for CyberGroup within the cybersecurity domain."^^xsd:string ;
    rdfs:subClassOf ns2:EnvironmentalGroup .

ns2:CyberattackHit a owl:Class ;
    rdfs:label "cyberattack hit"^^xsd:string ;
    rdfs:comment "Formal definition for CyberattackHit within the cybersecurity domain."^^xsd:string ;
    rdfs:subClassOf ns1:BotnetAttack .

ns2:CyberattackService a owl:Class ;
    rdfs:label "cyberattack service"^^xsd:string ;
    rdfs:comment "Formal definition for CyberattackService within the cybersecurity domain."^^xsd:string ;
    rdfs:subClassOf ns1:BotnetAttack .

ns2:DarkData a owl:Class ;
    rdfs:label "dark data"^^xsd:string ;
    rdfs:comment "Formal definition for DarkData within the cybersecurity domain."^^xsd:string ;
    rdfs:subClassOf ns1:DataCorruption .

ns2:DarkWeb a owl:Class ;
    rdfs:label "dark web"^^xsd:string ;
    rdfs:comment "Formal definition for DarkWeb within the cybersecurity domain."^^xsd:string ;
    rdfs:subClassOf ns1:Web .

ns2:DataFile a owl:Class ;
    rdfs:label "data file"^^xsd:string ;
    rdfs:comment "Formal definition for DataFile within the cybersecurity domain."^^xsd:string ;
    rdfs:subClassOf ns1:File .

ns2:DataGroup a owl:Class ;
    rdfs:label "data group"^^xsd:string ;
    rdfs:comment "Formal definition for DataGroup within the cybersecurity domain."^^xsd:string ;
    rdfs:subClassOf ns2:BaseGroup .

ns2:DataHacker a owl:Class ;
    rdfs:label "data hacker"^^xsd:string ;
    rdfs:comment "Formal definition for DataHacker within the cybersecurity domain."^^xsd:string ;
    rdfs:subClassOf ns1:DataCorruption .

ns2:DataHealth a owl:Class ;
    rdfs:label "data health"^^xsd:string ;
    rdfs:comment "Formal definition for DataHealth within the cybersecurity domain."^^xsd:string ;
    rdfs:subClassOf ns1:DataCorruption .

ns2:DataIncident a owl:Class ;
    rdfs:label "data incident"^^xsd:string ;
    rdfs:comment "Formal definition for DataIncident within the cybersecurity domain."^^xsd:string ;
    rdfs:subClassOf ns1:DataCorruption .

ns2:DataMalware a owl:Class ;
    rdfs:label "data malware"^^xsd:string ;
    rdfs:comment "Formal definition for DataMalware within the cybersecurity domain."^^xsd:string ;
    rdfs:subClassOf ns2:Malware .

ns2:DataNetwork a owl:Class ;
    rdfs:label "data network"^^xsd:string ;
    rdfs:comment "Formal definition for DataNetwork within the cybersecurity domain."^^xsd:string ;
    rdfs:subClassOf ns2:Network .

ns2:DataSite a owl:Class ;
    rdfs:label "data site"^^xsd:string ;
    rdfs:comment "Formal definition for DataSite within the cybersecurity domain."^^xsd:string ;
    rdfs:subClassOf ns1:Web .

ns2:DataSociety a owl:Class ;
    rdfs:label "data society"^^xsd:string ;
    rdfs:comment "Formal definition for DataSociety within the cybersecurity domain."^^xsd:string ;
    rdfs:subClassOf ns1:DataCorruption .

ns2:DataSoftware a owl:Class ;
    rdfs:label "data software"^^xsd:string ;
    rdfs:comment "Formal definition for DataSoftware within the cybersecurity domain."^^xsd:string ;
    rdfs:subClassOf ns1:Software .

ns2:DataState a owl:Class ;
    rdfs:label "data state"^^xsd:string ;
    rdfs:comment "Formal definition for DataState within the cybersecurity domain."^^xsd:string ;
    rdfs:subClassOf ns1:NetworkState .

ns2:DataSystem a owl:Class ;
    rdfs:label "data system"^^xsd:string ;
    rdfs:comment "Formal definition for DataSystem within the cybersecurity domain."^^xsd:string ;
    rdfs:subClassOf ns1:System .

ns2:DataThirdparty a owl:Class ;
    rdfs:label "data thirdparty"^^xsd:string ;
    rdfs:comment "Formal definition for DataThirdparty within the cybersecurity domain."^^xsd:string ;
    rdfs:subClassOf ns1:DataCorruption .

ns2:DataThreat a owl:Class ;
    rdfs:label "data threat"^^xsd:string ;
    rdfs:comment "Formal definition for DataThreat within the cybersecurity domain."^^xsd:string ;
    rdfs:subClassOf ns1:DataCorruption .

ns2:DataUnauthorized a owl:Class ;
    rdfs:label "data unauthorized"^^xsd:string ;
    rdfs:comment "Formal definition for DataUnauthorized within the cybersecurity domain."^^xsd:string ;
    rdfs:subClassOf ns1:DataCorruption .

ns2:DataUser a owl:Class ;
    rdfs:label "data user"^^xsd:string ;
    rdfs:comment "Formal definition for DataUser within the cybersecurity domain."^^xsd:string ;
    rdfs:subClassOf ns1:UnauthUser .

ns2:DataVictim a owl:Class ;
    rdfs:label "data victim"^^xsd:string ;
    rdfs:comment "Formal definition for DataVictim within the cybersecurity domain."^^xsd:string ;
    rdfs:subClassOf ns2:Victim .

ns2:DataVulnerability a owl:Class ;
    rdfs:label "data vulnerability"^^xsd:string ;
    rdfs:comment "Formal definition for DataVulnerability within the cybersecurity domain."^^xsd:string ;
    rdfs:subClassOf ns1:Vulnerability .

ns2:DataWeb a owl:Class ;
    rdfs:label "data web"^^xsd:string ;
    rdfs:comment "Formal definition for DataWeb within the cybersecurity domain."^^xsd:string ;
    rdfs:subClassOf ns1:Web .

ns2:DataWebsite a owl:Class ;
    rdfs:label "data website"^^xsd:string ;
    rdfs:comment "Formal definition for DataWebsite within the cybersecurity domain."^^xsd:string ;
    rdfs:subClassOf ns1:Web .

ns2:DdosService a owl:Class ;
    rdfs:label "ddos service"^^xsd:string ;
    rdfs:comment "Formal definition for DdosService within the cybersecurity domain."^^xsd:string ;
    rdfs:subClassOf ns2:DDoS .

ns2:EmailEmployee a owl:Class ;
    rdfs:label "email employee"^^xsd:string ;
    rdfs:comment "Formal definition for EmailEmployee within the cybersecurity domain."^^xsd:string ;
    rdfs:subClassOf ns1:Address .

ns2:EmailHacker a owl:Class ;
    rdfs:label "email hacker"^^xsd:string ;
    rdfs:comment "Formal definition for EmailHacker within the cybersecurity domain."^^xsd:string ;
    rdfs:subClassOf ns1:BotnetAttack .

ns2:EmailHealth a owl:Class ;
    rdfs:label "email health"^^xsd:string ;
    rdfs:comment "Formal definition for EmailHealth within the cybersecurity domain."^^xsd:string ;
    rdfs:subClassOf ns2:email .

ns2:EmailInformation a owl:Class ;
    rdfs:label "email information"^^xsd:string ;
    rdfs:comment "Formal definition for EmailInformation within the cybersecurity domain."^^xsd:string ;
    rdfs:subClassOf ns1:Address .

ns2:EmailName a owl:Class ;
    rdfs:label "email name"^^xsd:string ;
    rdfs:comment "Formal definition for EmailName within the cybersecurity domain."^^xsd:string ;
    rdfs:subClassOf ns1:Address .

ns2:EmailNumber a owl:Class ;
    rdfs:label "email number"^^xsd:string ;
    rdfs:comment "Formal definition for EmailNumber within the cybersecurity domain."^^xsd:string ;
    rdfs:subClassOf ns1:Address .

ns2:EmailSecurity a owl:Class ;
    rdfs:label "email security"^^xsd:string ;
    rdfs:comment "Formal definition for EmailSecurity within the cybersecurity domain."^^xsd:string ;
    rdfs:subClassOf ns2:email .

ns2:EmailService a owl:Class ;
    rdfs:label "email service"^^xsd:string ;
    rdfs:comment "Formal definition for EmailService within the cybersecurity domain."^^xsd:string ;
    rdfs:subClassOf ns2:email .

ns2:EmailSystem a owl:Class ;
    rdfs:label "email system"^^xsd:string ;
    rdfs:comment "Formal definition for EmailSystem within the cybersecurity domain."^^xsd:string ;
    rdfs:subClassOf ns1:System .

ns2:FileNetwork a owl:Class ;
    rdfs:label "file network"^^xsd:string ;
    rdfs:comment "Formal definition for FileNetwork within the cybersecurity domain."^^xsd:string ;
    rdfs:subClassOf ns2:Network .

ns2:FileSystem a owl:Class ;
    rdfs:label "file system"^^xsd:string ;
    rdfs:comment "Formal definition for FileSystem within the cybersecurity domain."^^xsd:string ;
    rdfs:subClassOf ns1:OperatingSystem .

ns2:GangVictim a owl:Class ;
    rdfs:label "gang victim"^^xsd:string ;
    rdfs:comment "Formal definition for GangVictim within the cybersecurity domain."^^xsd:string ;
    rdfs:subClassOf ns2:Victim .

ns2:GovernmentGroup a owl:Class ;
    rdfs:label "government group"^^xsd:string ;
    rdfs:comment "Formal definition for GovernmentGroup within the cybersecurity domain."^^xsd:string ;
    rdfs:subClassOf ns2:EnvironmentalGroup .

ns2:GroupHacker a owl:Class ;
    rdfs:label "group hacker"^^xsd:string ;
    rdfs:comment "Formal definition for GroupHacker within the cybersecurity domain."^^xsd:string ;
    rdfs:subClassOf ns1:BotnetAttack .

ns2:GroupHacking a owl:Class ;
    rdfs:label "group hacking"^^xsd:string ;
    rdfs:comment "Formal definition for GroupHacking within the cybersecurity domain."^^xsd:string ;
    rdfs:subClassOf ns2:Exploit .

ns2:GroupInformation a owl:Class ;
    rdfs:label "group information"^^xsd:string ;
    rdfs:comment "Formal definition for GroupInformation within the cybersecurity domain."^^xsd:string ;
    rdfs:subClassOf ns2:BaseGroup .

ns2:GroupOrganization a owl:Class ;
    rdfs:label "group organization"^^xsd:string ;
    rdfs:comment "Formal definition for GroupOrganization within the cybersecurity domain."^^xsd:string ;
    rdfs:subClassOf ns2:EnvironmentalGroup .

ns2:GroupService a owl:Class ;
    rdfs:label "group service"^^xsd:string ;
    rdfs:comment "Formal definition for GroupService within the cybersecurity domain."^^xsd:string ;
    rdfs:subClassOf ns2:BaseGroup .

ns2:GroupSystem a owl:Class ;
    rdfs:label "group system"^^xsd:string ;
    rdfs:comment "Formal definition for GroupSystem within the cybersecurity domain."^^xsd:string ;
    rdfs:subClassOf ns1:System .

ns2:GroupThreat a owl:Class ;
    rdfs:label "group threat"^^xsd:string ;
    rdfs:comment "Formal definition for GroupThreat within the cybersecurity domain."^^xsd:string ;
    rdfs:subClassOf ns2:EnvironmentalGroup .

ns2:GroupVictim a owl:Class ;
    rdfs:label "group victim"^^xsd:string ;
    rdfs:comment "Formal definition for GroupVictim within the cybersecurity domain."^^xsd:string ;
    rdfs:subClassOf ns2:Victim .

ns2:GroupWebsite a owl:Class ;
    rdfs:label "group website"^^xsd:string ;
    rdfs:comment "Formal definition for GroupWebsite within the cybersecurity domain."^^xsd:string ;
    rdfs:subClassOf ns2:EnvironmentalGroup .

ns2:HackerService a owl:Class ;
    rdfs:label "hacker service"^^xsd:string ;
    rdfs:comment "Formal definition for HackerService within the cybersecurity domain."^^xsd:string ;
    rdfs:subClassOf ns2:Malware .

ns2:HackerState a owl:Class ;
    rdfs:label "hacker state"^^xsd:string ;
    rdfs:comment "Formal definition for HackerState within the cybersecurity domain."^^xsd:string ;
    rdfs:subClassOf ns1:NetworkState .

ns2:HackerSteal a owl:Class ;
    rdfs:label "hacker steal"^^xsd:string ;
    rdfs:comment "Formal definition for HackerSteal within the cybersecurity domain."^^xsd:string ;
    rdfs:subClassOf ns2:Exploit .

ns2:HackerSystem a owl:Class ;
    rdfs:label "hacker system"^^xsd:string ;
    rdfs:comment "Formal definition for HackerSystem within the cybersecurity domain."^^xsd:string ;
    rdfs:subClassOf ns1:System .

ns2:HackerWebsite a owl:Class ;
    rdfs:label "hacker website"^^xsd:string ;
    rdfs:comment "Formal definition for HackerWebsite within the cybersecurity domain."^^xsd:string ;
    rdfs:subClassOf ns1:BotnetAttack .

ns2:HealthIncident a owl:Class ;
    rdfs:label "health incident"^^xsd:string ;
    rdfs:comment "Formal definition for HealthIncident within the cybersecurity domain."^^xsd:string ;
    rdfs:subClassOf ns1:Incident .

ns2:HealthSystem a owl:Class ;
    rdfs:label "health system"^^xsd:string ;
    rdfs:comment "Formal definition for HealthSystem within the cybersecurity domain."^^xsd:string ;
    rdfs:subClassOf ns1:System .

ns2:High a owl:NamedIndividual .

ns2:IncidentInformation a owl:Class ;
    rdfs:label "incident information"^^xsd:string ;
    rdfs:comment "Formal definition for IncidentInformation within the cybersecurity domain."^^xsd:string ;
    rdfs:subClassOf ns1:Incident .

ns2:InformationNetwork a owl:Class ;
    rdfs:label "information network"^^xsd:string ;
    rdfs:comment "Formal definition for InformationNetwork within the cybersecurity domain."^^xsd:string ;
    rdfs:subClassOf ns2:Network .

ns2:InformationOnline a owl:Class ;
    rdfs:label "information online"^^xsd:string ;
    rdfs:comment "Formal definition for InformationOnline within the cybersecurity domain."^^xsd:string ;
    rdfs:subClassOf ns1:Web .

ns2:InformationParty a owl:Class ;
    rdfs:label "information party"^^xsd:string ;
    rdfs:comment "Formal definition for InformationParty within the cybersecurity domain."^^xsd:string ;
    rdfs:subClassOf ns1:IDPS .

ns2:InformationPhishing a owl:Class ;
    rdfs:label "information phishing"^^xsd:string ;
    rdfs:comment "Formal definition for InformationPhishing within the cybersecurity domain."^^xsd:string ;
    rdfs:subClassOf ns2:Phishing .

ns2:InformationSystem a owl:Class ;
    rdfs:label "information system"^^xsd:string ;
    rdfs:comment "Formal definition for InformationSystem within the cybersecurity domain."^^xsd:string ;
    rdfs:subClassOf ns1:System .

ns2:InformationWebsite a owl:Class ;
    rdfs:label "information website"^^xsd:string ;
    rdfs:comment "Formal definition for InformationWebsite within the cybersecurity domain."^^xsd:string ;
    rdfs:subClassOf ns1:Web .

ns2:KillChain a owl:Class ;
    rdfs:comment "Formal definition for KillChain within the cybersecurity domain."^^xsd:string ;
    rdfs:subClassOf ns1:UCOThing ;
    owl:equivalentClass <http://stix.mitre.org/STIX#KillChain> .

ns2:LeakWeb a owl:Class ;
    rdfs:label "leak web"^^xsd:string ;
    rdfs:comment "Formal definition for LeakWeb within the cybersecurity domain."^^xsd:string ;
    rdfs:subClassOf ns1:Web .

ns2:Low a owl:NamedIndividual .

ns2:MalwareState a owl:Class ;
    rdfs:label "malware state"^^xsd:string ;
    rdfs:comment "Formal definition for MalwareState within the cybersecurity domain."^^xsd:string ;
    rdfs:subClassOf ns2:Malware .

ns2:Medium a owl:NamedIndividual .

ns2:NameWebsite a owl:Class ;
    rdfs:label "name website"^^xsd:string ;
    rdfs:comment "Formal definition for NameWebsite within the cybersecurity domain."^^xsd:string ;
    rdfs:subClassOf ns1:Web .

ns2:NetworkParty a owl:Class ;
    rdfs:label "network party"^^xsd:string ;
    rdfs:comment "Formal definition for NetworkParty within the cybersecurity domain."^^xsd:string ;
    rdfs:subClassOf ns1:NetworkState .

ns2:NetworkSystem a owl:Class ;
    rdfs:label "network system"^^xsd:string ;
    rdfs:comment "Formal definition for NetworkSystem within the cybersecurity domain."^^xsd:string ;
    rdfs:subClassOf ns1:System .

ns2:NetworkThreat a owl:Class ;
    rdfs:label "network threat"^^xsd:string ;
    rdfs:comment "Formal definition for NetworkThreat within the cybersecurity domain."^^xsd:string ;
    rdfs:subClassOf ns1:BotnetAttack .

ns2:NetworkWeb a owl:Class ;
    rdfs:label "network web"^^xsd:string ;
    rdfs:comment "Formal definition for NetworkWeb within the cybersecurity domain."^^xsd:string ;
    rdfs:subClassOf ns1:Web .

ns2:None a owl:NamedIndividual .

ns2:OnlineService a owl:Class ;
    rdfs:label "online service"^^xsd:string ;
    rdfs:comment "Formal definition for OnlineService within the cybersecurity domain."^^xsd:string ;
    rdfs:subClassOf ns1:Web .

ns2:OrganizationSystem a owl:Class ;
    rdfs:label "organization system"^^xsd:string ;
    rdfs:comment "Formal definition for OrganizationSystem within the cybersecurity domain."^^xsd:string ;
    rdfs:subClassOf ns1:System .

ns2:OrganizationVictim a owl:Class ;
    rdfs:label "organization victim"^^xsd:string ;
    rdfs:comment "Formal definition for OrganizationVictim within the cybersecurity domain."^^xsd:string ;
    rdfs:subClassOf ns2:Victim .

ns2:OrganizationWebsite a owl:Class ;
    rdfs:label "organization website"^^xsd:string ;
    rdfs:comment "Formal definition for OrganizationWebsite within the cybersecurity domain."^^xsd:string ;
    rdfs:subClassOf ns1:Web .

ns2:Password a owl:Class ;
    rdfs:comment """A password is a string of characters used to verify the identity of a user during the authentication process. Passwords are typically used in tandem with a username; they are designed to be known only to the user and allow that user to gain access to a device, application or website.

Source: https://www.techtarget.com/searchsecurity/definition/password"""^^xsd:string ;
    rdfs:subClassOf ns2:Account .

ns2:PersonalSystem a owl:Class ;
    rdfs:label "personal system"^^xsd:string ;
    rdfs:comment "Formal definition for PersonalSystem within the cybersecurity domain."^^xsd:string ;
    rdfs:subClassOf ns1:System .

ns2:PortalWeb a owl:Class ;
    rdfs:label "portal web"^^xsd:string ;
    rdfs:comment "Formal definition for PortalWeb within the cybersecurity domain."^^xsd:string ;
    rdfs:subClassOf ns1:Web .

ns2:SecuritySystem a owl:Class ;
    rdfs:label "security system"^^xsd:string ;
    rdfs:comment "Formal definition for SecuritySystem within the cybersecurity domain."^^xsd:string ;
    rdfs:subClassOf ns1:System .

ns2:SecurityThreat a owl:Class ;
    rdfs:label "security threat"^^xsd:string ;
    rdfs:comment "Formal definition for SecurityThreat within the cybersecurity domain."^^xsd:string ;
    rdfs:subClassOf ns1:Vulnerability .

ns2:SecurityVictim a owl:Class ;
    rdfs:label "security victim"^^xsd:string ;
    rdfs:comment "Formal definition for SecurityVictim within the cybersecurity domain."^^xsd:string ;
    rdfs:subClassOf ns2:Victim .

ns2:SecurityWebsite a owl:Class ;
    rdfs:label "security website"^^xsd:string ;
    rdfs:comment "Formal definition for SecurityWebsite within the cybersecurity domain."^^xsd:string ;
    rdfs:subClassOf ns1:Web .

ns2:ServiceSystem a owl:Class ;
    rdfs:label "service system"^^xsd:string ;
    rdfs:comment "Formal definition for ServiceSystem within the cybersecurity domain."^^xsd:string ;
    rdfs:subClassOf ns1:System .

ns2:ServiceWebsite a owl:Class ;
    rdfs:label "service website"^^xsd:string ;
    rdfs:comment "Formal definition for ServiceWebsite within the cybersecurity domain."^^xsd:string ;
    rdfs:subClassOf ns1:Web .

ns2:SeveralWebsite a owl:Class ;
    rdfs:label "several website"^^xsd:string ;
    rdfs:comment "Formal definition for SeveralWebsite within the cybersecurity domain."^^xsd:string ;
    rdfs:subClassOf ns1:Web .

ns2:SiteWeb a owl:Class ;
    rdfs:label "site web"^^xsd:string ;
    rdfs:comment "Formal definition for SiteWeb within the cybersecurity domain."^^xsd:string ;
    rdfs:subClassOf ns1:Web .

ns2:SiteWebsite a owl:Class ;
    rdfs:label "site website"^^xsd:string ;
    rdfs:comment "Formal definition for SiteWebsite within the cybersecurity domain."^^xsd:string ;
    rdfs:subClassOf ns1:Web .

ns2:SocietyWeb a owl:Class ;
    rdfs:label "society web"^^xsd:string ;
    rdfs:comment "Formal definition for SocietyWeb within the cybersecurity domain."^^xsd:string ;
    rdfs:subClassOf ns1:Web .

ns2:StateVictim a owl:Class ;
    rdfs:label "state victim"^^xsd:string ;
    rdfs:comment "Formal definition for StateVictim within the cybersecurity domain."^^xsd:string ;
    rdfs:subClassOf ns2:Victim .

ns2:SystemThreat a owl:Class ;
    rdfs:label "system threat"^^xsd:string ;
    rdfs:comment "Formal definition for SystemThreat within the cybersecurity domain."^^xsd:string ;
    rdfs:subClassOf ns1:System .

ns2:SystemU a owl:Class ;
    rdfs:label "system u"^^xsd:string ;
    rdfs:comment "Formal definition for SystemU within the cybersecurity domain."^^xsd:string ;
    rdfs:subClassOf ns1:System .

ns2:SystemVictim a owl:Class ;
    rdfs:label "system victim"^^xsd:string ;
    rdfs:comment "Formal definition for SystemVictim within the cybersecurity domain."^^xsd:string ;
    rdfs:subClassOf ns2:Victim .

ns2:ThreatVictim a owl:Class ;
    rdfs:label "threat victim"^^xsd:string ;
    rdfs:comment "Formal definition for ThreatVictim within the cybersecurity domain."^^xsd:string ;
    rdfs:subClassOf ns2:Victim .

ns2:ToolVictim a owl:Class ;
    rdfs:label "tool victim"^^xsd:string ;
    rdfs:comment "Formal definition for ToolVictim within the cybersecurity domain."^^xsd:string ;
    rdfs:subClassOf ns2:Victim .

ns2:UVictim a owl:Class ;
    rdfs:label "u victim"^^xsd:string ;
    rdfs:comment "Formal definition for UVictim within the cybersecurity domain."^^xsd:string ;
    rdfs:subClassOf ns2:Victim .

ns2:Unknown a owl:NamedIndividual .

ns2:ViceWeb a owl:Class ;
    rdfs:label "vice web"^^xsd:string ;
    rdfs:comment "Formal definition for ViceWeb within the cybersecurity domain."^^xsd:string ;
    rdfs:subClassOf ns1:Web .

ns2:a1b97d47c1d59772 a ns2:Malware,
        owl:NamedIndividual ;
    ns1:associatedCampaigns ns2:Metro_newspaper ;
    ns1:description "Financial"^^xsd:string ;
    ns2:behaviour ns2:Financial ;
    ns2:hasActorType "Criminal"^^xsd:string ;
    ns2:hasCampaign ns2:New_York ;
    ns2:hasCountry "United States of America"^^xsd:string ;
    ns2:hasCounty "New York"^^xsd:string ;
    ns2:hasEventDate "2014-07-23T00:00:00"^^xsd:dateTime ;
    ns2:hasEventSubtype "Exploitation of Application Server"^^xsd:string ;
    ns2:hasEventType "Exploitive"^^xsd:string ;
    ns2:hasIndustry "Information"^^xsd:string ;
    ns2:hasMonth 7 ;
    ns2:hasOrganization "Metro newspaper"^^xsd:string ;
    ns2:hasState "New York"^^xsd:string ;
    ns2:hasYear 2014 ;
    ns2:isType_of ns2:Criminal,
        ns2:Exploitation_of_Application_Server ;
    rdfs:comment "The United States website of the Metro newspaper (metro.us), which serves an estimatedÃÆÃ'Ãâ 'ÃÆÃ¢â¬Â 'ÃÆÃ'ÃÂ¢Ã¢'Â¬ÃÂ ''ÃÆÃ'Ãâ 'ÃÆÃ¢â¬Â ''ÃÆÃ'Ãâ ''ÃÆÃ''ÃÆ'Ã'ÃÂ 1 millionÃÆÃ'Ãâ 'ÃÆÃ¢â¬Â 'ÃÆÃ'ÃÂ¢Ã¢'Â¬ÃÂ ''ÃÆÃ'Ãâ 'ÃÆÃ¢â¬Â ''ÃÆÃ'Ãâ ''ÃÆÃ''ÃÆ'Ã'ÃÂ visitors every month, is compromised and abused to distribute malware."^^xsd:string .

ns2:a214f05c3e8bfa0a a ns2:BreachInformation,
        owl:NamedIndividual ;
    ns1:associatedCampaigns ns2:St__Joseph_Health_System ;
    ns2:hasActorType "Criminal"^^xsd:string ;
    ns2:hasCampaign ns2:Texas ;
    ns2:hasCountry "United States of America"^^xsd:string ;
    ns2:hasCounty "Brazos"^^xsd:string ;
    ns2:hasEventDate "2014-02-05T00:00:00"^^xsd:dateTime ;
    ns2:hasEventSubtype "Exploitation of Application Server"^^xsd:string ;
    ns2:hasEventType "Exploitive"^^xsd:string ;
    ns2:hasIndustry "Health Care and Social Assistance"^^xsd:string ;
    ns2:hasMonth 2 ;
    ns2:hasOrganization "St. Joseph Health System"^^xsd:string ;
    ns2:hasState "Texas"^^xsd:string ;
    ns2:hasYear 2014 ;
    ns2:isType_of ns2:Criminal,
        ns2:Exploitation_of_Application_Server ;
    rdfs:comment "More than 400,000 patients and employees of St. Joseph Health System are notified that their personal information, including Social Security numbers and, in some cases, bank account information, may have been accessed following an attack on the health system's computer system."^^xsd:string .

ns2:a4ffcbbf008aa8cc a ns2:CyberattackData,
        owl:NamedIndividual ;
    ns1:associatedCampaigns ns2:United_Nations_Internet_Governance_Forum ;
    ns2:hasActor "DeleteSec"^^xsd:string ;
    ns2:hasActorType "Hacktivist"^^xsd:string ;
    ns2:hasEventDate "2014-02-20T00:00:00"^^xsd:dateTime ;
    ns2:hasEventSubtype "Exploitation of Application Server"^^xsd:string ;
    ns2:hasEventType "Exploitive"^^xsd:string ;
    ns2:hasIndustry "Public Administration"^^xsd:string ;
    ns2:hasMonth 2 ;
    ns2:hasOrganization "United Nations Internet Governance Forum"^^xsd:string ;
    ns2:hasYear 2014 ;
    ns2:isType_of ns2:Exploitation_of_Application_Server,
        ns2:Hacktivist ;
    rdfs:comment "The hacker collective @deletesec announces a breach and leak of data from the Internet Governance Forum (intgovforum.org), a United nations based website. The leak contains 3,215 users real names, user names, email addresses and encrypted passwords."^^xsd:string .

ns2:a560f11dba4b509d a ns2:DDoS,
        owl:NamedIndividual ;
    ns1:associatedCampaigns ns2:Cirrus_Communications ;
    ns2:hasActorType "Criminal"^^xsd:string ;
    ns2:hasCountry "Australia"^^xsd:string ;
    ns2:hasEventDate "2014-07-30T00:00:00"^^xsd:dateTime ;
    ns2:hasEventSubtype "External Denial of Service"^^xsd:string ;
    ns2:hasEventType "Disruptive"^^xsd:string ;
    ns2:hasIndustry "Information"^^xsd:string ;
    ns2:hasMonth 7 ;
    ns2:hasOrganization "Cirrus Communications"^^xsd:string ;
    ns2:hasYear 2014 ;
    ns2:isType_of ns2:Criminal,
        ns2:External_Denial_of_Service ;
    rdfs:comment "The largest fixed wireless broadband carrier in Australia, Cirrus Communications, suffers a major DDoS attack, which takes out over half of its network."^^xsd:string .

ns2:a5790cecc85ca6fb a ns2:BreachInformation,
        owl:NamedIndividual ;
    ns1:associatedCampaigns ns2:Muslim_Directory ;
    ns2:hasActor "@th3inf1d3l"^^xsd:string ;
    ns2:hasActorType "Hacktivist"^^xsd:string ;
    ns2:hasCountry "United Kingdom of Great Britain and Northern Ireland"^^xsd:string ;
    ns2:hasEventDate "2014-02-17T00:00:00"^^xsd:dateTime ;
    ns2:hasEventSubtype "Exploitation of Application Server"^^xsd:string ;
    ns2:hasEventType "Exploitive"^^xsd:string ;
    ns2:hasIndustry "Information"^^xsd:string ;
    ns2:hasMonth 2 ;
    ns2:hasOrganization "Muslim Directory"^^xsd:string ;
    ns2:hasYear 2014 ;
    ns2:isType_of ns2:Exploitation_of_Application_Server,
        ns2:Hacktivist ;
    rdfs:comment "A hacker using the handle @th3inf1d3l announces a leak of data from muslimdirectory.co.ukÃÆÃ'Ãâ 'ÃÆÃ¢â¬Â 'ÃÆÃ'ÃÂ¢Ã¢'Â¬ÃÂ ''ÃÆÃ'Ãâ 'ÃÆÃ¢â¬Â ''ÃÆÃ'Ãâ ''ÃÆÃ''ÃÆ'Ã'ÃÂ resulting in 38,903 user credentials being leaked online."^^xsd:string .

ns2:a59b5c2114cbd6d7 a ns2:AccountAttack,
        owl:NamedIndividual ;
    ns1:associatedCampaigns ns2:P__F__Chang_s ;
    ns1:description "Financial"^^xsd:string ;
    ns2:behaviour ns2:Financial ;
    ns2:hasActorType "Criminal"^^xsd:string ;
    ns2:hasCampaign ns2:Arizona ;
    ns2:hasCountry "United States of America"^^xsd:string ;
    ns2:hasCounty "Maricopa"^^xsd:string ;
    ns2:hasEventDate "2014-06-14T00:00:00"^^xsd:dateTime ;
    ns2:hasEventSubtype "Exploitation of Sensors"^^xsd:string ;
    ns2:hasEventType "Exploitive"^^xsd:string ;
    ns2:hasIndustry "Accommodation and Food Services"^^xsd:string ;
    ns2:hasMonth 6 ;
    ns2:hasOrganization "P. F. Chang's"^^xsd:string ;
    ns2:hasState "Arizona"^^xsd:string ;
    ns2:hasYear 2014 ;
    ns2:isType_of ns2:Criminal,
        ns2:Exploitation_of_Sensors ;
    rdfs:comment "Restaurant chain P.F. Chang's Chinese Bistro confirms that customer credit and debit card data had been stolen in a cybercrime attack on its stores."^^xsd:string .

ns2:a64114296e418e05 a ns2:Ransomware,
        owl:NamedIndividual ;
    ns1:associatedCampaigns ns2:Conforama ;
    ns1:description "Financial"^^xsd:string ;
    ns1:isLaunchedBy ns2:Russian_Federation ;
    ns2:behaviour ns2:Financial ;
    ns2:hasActor "ALPHVM"^^xsd:string ;
    ns2:hasActorCountry "Russian Federation"^^xsd:string ;
    ns2:hasActorType "Criminal"^^xsd:string ;
    ns2:hasCountry "France"^^xsd:string ;
    ns2:hasEventDate "2022-11-11T00:00:00"^^xsd:dateTime ;
    ns2:hasEventSubtype "Data Attack"^^xsd:string ;
    ns2:hasEventType "Mixed"^^xsd:string ;
    ns2:hasIndustry "Manufacturing"^^xsd:string ;
    ns2:hasMonth 11 ;
    ns2:hasOrganization "Conforama"^^xsd:string ;
    ns2:hasYear 2022 ;
    ns2:isType_of ns2:Criminal,
        ns2:Data_Attack ;
    rdfs:comment "BlackCat ransomware gang lists Conforama, said to be Europe's second-largest home furnishing retail chain, on its victim list, and claims to have stolen over 1TB of data."^^xsd:string .

ns2:a72bd03b0b4cc9c9 a ns2:DDoS,
        owl:NamedIndividual ;
    ns1:associatedCampaigns ns2:UK_Government_Communications_Headquarter ;
    ns1:description "Protest"^^xsd:string ;
    ns2:behaviour ns2:Protest ;
    ns2:hasActor "Anonymous"^^xsd:string ;
    ns2:hasActorType "Hacktivist"^^xsd:string ;
    ns2:hasCountry "United Kingdom of Great Britain and Northern Ireland"^^xsd:string ;
    ns2:hasEventDate "2014-02-12T00:00:00"^^xsd:dateTime ;
    ns2:hasEventSubtype "External Denial of Service"^^xsd:string ;
    ns2:hasEventType "Disruptive"^^xsd:string ;
    ns2:hasIndustry "Public Administration"^^xsd:string ;
    ns2:hasMonth 2 ;
    ns2:hasOrganization "UK Government Communications Headquarters"^^xsd:string ;
    ns2:hasYear 2014 ;
    ns2:isType_of ns2:External_Denial_of_Service,
        ns2:Hacktivist ;
    rdfs:comment "Even the website of the Government Communications Headquarters (gchq.gov.uk) is disrupted by a DDoS attack."^^xsd:string .

ns2:a7434ec0a8eac864 a ns1:BotnetAttack,
        owl:NamedIndividual ;
    ns1:associatedCampaigns ns2:mumsnet ;
    ns2:hasActorType "Criminal"^^xsd:string ;
    ns2:hasCountry "United Kingdom of Great Britain and Northern Ireland"^^xsd:string ;
    ns2:hasEventDate "2014-04-11T00:00:00"^^xsd:dateTime ;
    ns2:hasEventSubtype "Exploitation of Application Server"^^xsd:string ;
    ns2:hasEventType "Exploitive"^^xsd:string ;
    ns2:hasIndustry "Information"^^xsd:string ;
    ns2:hasMonth 4 ;
    ns2:hasOrganization "mumsnet"^^xsd:string ;
    ns2:hasYear 2014 ;
    ns2:isType_of ns2:Criminal,
        ns2:Exploitation_of_Application_Server ;
    rdfs:comment "Another website victim of Heartbleed. Mumsnet, a popular British parenting website with 1.5 million registered users, reports that users' data has been accessed as a result of the Heartbleed bug."^^xsd:string .

ns2:a75bf7689c90c5d5 a ns2:AccountAttack,
        owl:NamedIndividual ;
    ns1:associatedCampaigns ns2:Michael_s ;
    ns1:description "Financial"^^xsd:string ;
    ns2:behaviour ns2:Financial ;
    ns2:hasActorType "Criminal"^^xsd:string ;
    ns2:hasCampaign ns2:Texas ;
    ns2:hasCountry "United States of America"^^xsd:string ;
    ns2:hasCounty "Dallas"^^xsd:string ;
    ns2:hasEventDate "2014-01-25T00:00:00"^^xsd:dateTime ;
    ns2:hasEventSubtype "Exploitation of Sensors"^^xsd:string ;
    ns2:hasEventType "Exploitive"^^xsd:string ;
    ns2:hasIndustry "Retail Trade"^^xsd:string ;
    ns2:hasMonth 1 ;
    ns2:hasOrganization "Michael's"^^xsd:string ;
    ns2:hasState "Texas"^^xsd:string ;
    ns2:hasYear 2014 ;
    ns2:isType_of ns2:Criminal,
        ns2:Exploitation_of_Sensors ;
    rdfs:comment "Multiple sources in the banking industry say they are tracking a pattern of fraud on cards recently used at Michaels Stores Inc., an Irving, Texas-based arts-and-crafts retailer that maintains more than 1,250 stores across the United States."^^xsd:string .

ns2:a805b7b33ebbcc99 a ns2:BreachSecurity,
        owl:NamedIndividual ;
    ns1:associatedCampaigns ns2:Doge_Vault ;
    ns1:description "Financial"^^xsd:string ;
    ns2:behaviour ns2:Financial ;
    ns2:hasActorType "Criminal"^^xsd:string ;
    ns2:hasEventDate "2014-05-16T00:00:00"^^xsd:dateTime ;
    ns2:hasEventSubtype "Exploitation of Application Server"^^xsd:string ;
    ns2:hasEventType "Exploitive"^^xsd:string ;
    ns2:hasIndustry "Finance and Insurance"^^xsd:string ;
    ns2:hasMonth 5 ;
    ns2:hasOrganization "Doge Vault"^^xsd:string ;
    ns2:hasYear 2014 ;
    ns2:isType_of ns2:Criminal,
        ns2:Exploitation_of_Application_Server ;
    rdfs:comment "Doge Vault, one of the most popular online repositories for the cryptocurrency Dogecoin, formally acknowledges that it has been hacked two days earlier. Losses amount to the equivalent of $74,000. Unfortunately all the Dogecoin addresses are compromised."^^xsd:string .

ns2:a83a8f3c6cc9a062 a ns2:HackerSecurity,
        owl:NamedIndividual ;
    ns1:associatedCampaigns ns2:Cumberland_Valley_School_District ;
    ns2:hasActorType "Criminal"^^xsd:string ;
    ns2:hasCampaign ns2:Pennsylvania ;
    ns2:hasCountry "United States of America"^^xsd:string ;
    ns2:hasCounty "Cumberland"^^xsd:string ;
    ns2:hasEventDate "2014-08-22T00:00:00"^^xsd:dateTime ;
    ns2:hasEventSubtype "Exploitation of Application Server"^^xsd:string ;
    ns2:hasEventType "Exploitive"^^xsd:string ;
    ns2:hasIndustry "Educational Services"^^xsd:string ;
    ns2:hasMonth 8 ;
    ns2:hasOrganization "Cumberland Valley School District"^^xsd:string ;
    ns2:hasState "Pennsylvania"^^xsd:string ;
    ns2:hasYear 2014 ;
    ns2:isType_of ns2:Criminal,
        ns2:Exploitation_of_Application_Server ;
    rdfs:comment "A hacker gains access to the Cumberland Valley School District computer network, forcing the district to notify local police and FBI."^^xsd:string .

ns2:a88a4e5463526b03 a ns2:BreachInformation,
        owl:NamedIndividual ;
    ns1:associatedCampaigns ns2:State_Industrial_Products ;
    ns1:description "Financial"^^xsd:string ;
    ns2:behaviour ns2:Financial ;
    ns2:hasActorType "Criminal"^^xsd:string ;
    ns2:hasCampaign ns2:Ohio ;
    ns2:hasCountry "United States of America"^^xsd:string ;
    ns2:hasCounty "Cuyahoga"^^xsd:string ;
    ns2:hasEventDate "2014-01-30T00:00:00"^^xsd:dateTime ;
    ns2:hasEventSubtype "Exploitation of Application Server"^^xsd:string ;
    ns2:hasEventType "Exploitive"^^xsd:string ;
    ns2:hasMonth 1 ;
    ns2:hasOrganization "State Industrial Products"^^xsd:string ;
    ns2:hasState "Ohio"^^xsd:string ;
    ns2:hasYear 2014 ;
    ns2:isType_of ns2:Criminal,
        ns2:Exploitation_of_Application_Server ;
    rdfs:comment "The FBI alerts State Industrial Products that the personal information, including Social Security numbers, of 500-1000 current and former employees may be at risk after an unauthorized party gained access to the information."^^xsd:string .

ns2:aa85981a4d7bbc18 a ns2:AccessSecurity,
        owl:NamedIndividual ;
    ns1:associatedCampaigns ns2:Government_Secure_Intranet ;
    ns1:description "Political-Espionage"^^xsd:string ;
    ns2:behaviour ns2:Political_Espionage ;
    ns2:hasActorType "Criminal"^^xsd:string ;
    ns2:hasCountry "United Kingdom of Great Britain and Northern Ireland"^^xsd:string ;
    ns2:hasEventDate "2014-06-18T00:00:00"^^xsd:dateTime ;
    ns2:hasEventSubtype "Exploitation of Application Server"^^xsd:string ;
    ns2:hasEventType "Exploitive"^^xsd:string ;
    ns2:hasIndustry "Public Administration"^^xsd:string ;
    ns2:hasMonth 6 ;
    ns2:hasOrganization "Government Secure Intranet"^^xsd:string ;
    ns2:hasYear 2014 ;
    ns2:isType_of ns2:Criminal,
        ns2:Exploitation_of_Application_Server ;
    rdfs:comment "British Cabinet Office minister Francis Maude, declares that a state-sponsored hostile group was able to gain access to a system administrator account on the Government Secure Intranet."^^xsd:string .

ns2:ab2a62f4d730c092 a ns1:BotnetAttack,
        owl:NamedIndividual ;
    ns1:associatedCampaigns ns2:Bharat_Sanchar_Nigam_Limited__BSNL ;
    ns1:isLaunchedBy ns2:India ;
    ns2:hasActor "Kai-H4xOrR"^^xsd:string ;
    ns2:hasActorCountry "India"^^xsd:string ;
    ns2:hasActorType "Hacktivist"^^xsd:string ;
    ns2:hasCountry "India"^^xsd:string ;
    ns2:hasEventDate "2014-05-03T00:00:00"^^xsd:dateTime ;
    ns2:hasEventSubtype "Message Manipulation"^^xsd:string ;
    ns2:hasEventType "Disruptive"^^xsd:string ;
    ns2:hasIndustry "Information"^^xsd:string ;
    ns2:hasMonth 5 ;
    ns2:hasOrganization "Bharat Sanchar Nigam Limited (BSNL)"^^xsd:string ;
    ns2:hasYear 2014 ;
    ns2:isType_of ns2:Hacktivist,
        ns2:Message_Manipulation ;
    rdfs:comment "Kai-H4xOrR, a Pakistani hacker, member of the Pakistan Haxors Crew, defaces the international roaming subdomain (ir.bsnl.co.in) of the Indian telecom company Bharat Sanchar Nigam Limited (BSNL)."^^xsd:string .

ns2:ac8309343d1619dd a ns2:AnonymousAttack,
        owl:NamedIndividual ;
    ns1:associatedCampaigns ns2:Namibian_Government_Portal ;
    ns1:description "Protest"^^xsd:string ;
    ns2:behaviour ns2:Protest ;
    ns2:hasActor "Anonymous"^^xsd:string ;
    ns2:hasActorType "Hacktivist"^^xsd:string ;
    ns2:hasCountry "Namibia"^^xsd:string ;
    ns2:hasEventDate "2014-01-08T00:00:00"^^xsd:dateTime ;
    ns2:hasEventSubtype "External Denial of Service"^^xsd:string ;
    ns2:hasEventType "Disruptive"^^xsd:string ;
    ns2:hasIndustry "Public Administration"^^xsd:string ;
    ns2:hasMonth 1 ;
    ns2:hasOrganization "Namibian Government Portal"^^xsd:string ;
    ns2:hasYear 2014 ;
    ns2:isType_of ns2:External_Denial_of_Service,
        ns2:Hacktivist ;
    rdfs:comment "In the name of OpFunKill the Anonymous take down the Namibia main Government portal gov.na"^^xsd:string .

ns2:accf9ccbc6287d66 a ns2:HackerSecurity,
        owl:NamedIndividual ;
    ns1:associatedCampaigns ns2:Sky_News_Egypt ;
    ns2:hasActor "The BLuE"^^xsd:string ;
    ns2:hasActorType "Hobbyist"^^xsd:string ;
    ns2:hasCountry "Egypt"^^xsd:string ;
    ns2:hasEventDate "2014-06-11T00:00:00"^^xsd:dateTime ;
    ns2:hasEventSubtype "Message Manipulation"^^xsd:string ;
    ns2:hasEventType "Disruptive"^^xsd:string ;
    ns2:hasIndustry "Information"^^xsd:string ;
    ns2:hasMonth 6 ;
    ns2:hasOrganization "Sky News Egypt"^^xsd:string ;
    ns2:hasYear 2014 ;
    ns2:isType_of ns2:Hobbyist,
        ns2:Message_Manipulation ;
    rdfs:comment "A hacker called Hmeidefaces the official website of ESETand 4 of itsSpanish domains."^^xsd:string .

ns2:ada756fe094942ad a ns2:CyberattackInformation,
        owl:NamedIndividual ;
    ns1:associatedCampaigns ns2:Pakistan_Electric_Power_Company ;
    ns1:description "Protest"^^xsd:string ;
    ns1:isLaunchedBy ns2:Pakistan ;
    ns2:behaviour ns2:Protest ;
    ns2:hasActor "Pakistan Haxors Crew"^^xsd:string ;
    ns2:hasActorCountry "Pakistan"^^xsd:string ;
    ns2:hasActorType "Hacktivist"^^xsd:string ;
    ns2:hasCountry "Pakistan"^^xsd:string ;
    ns2:hasEventDate "2014-06-21T00:00:00"^^xsd:dateTime ;
    ns2:hasEventSubtype "Message Manipulation"^^xsd:string ;
    ns2:hasEventType "Disruptive"^^xsd:string ;
    ns2:hasIndustry "Utilities"^^xsd:string ;
    ns2:hasMonth 6 ;
    ns2:hasOrganization "Pakistan Electric Power Company"^^xsd:string ;
    ns2:hasYear 2014 ;
    ns2:isType_of ns2:Hacktivist,
        ns2:Message_Manipulation ;
    rdfs:comment "The official website of Pakistan Electric Power Company Limited (pepco.gov.pk) is defaced by a group of Pakistani hackers called Pakistan Haxors Crew in protest against police brutality."^^xsd:string .

ns2:aecb46587decde3b a ns2:AttackWebsite,
        owl:NamedIndividual ;
    ns1:associatedCampaigns ns2:French_Ministry_of_Interior ;
    ns2:hasActor "AnonGhost"^^xsd:string ;
    ns2:hasActorType "Hacktivist"^^xsd:string ;
    ns2:hasCountry "France"^^xsd:string ;
    ns2:hasEventDate "2015-01-22T00:00:00"^^xsd:dateTime ;
    ns2:hasEventSubtype "Message Manipulation"^^xsd:string ;
    ns2:hasEventType "Disruptive"^^xsd:string ;
    ns2:hasIndustry "Public Administration"^^xsd:string ;
    ns2:hasMonth 1 ;
    ns2:hasOrganization "French Ministry of Interior"^^xsd:string ;
    ns2:hasYear 2015 ;
    ns2:isType_of ns2:Hacktivist,
        ns2:Message_Manipulation ;
    rdfs:comment "The AnonGhost collective defaces several subdomains of the French Interior and Defense Ministries."^^xsd:string .

ns2:aef80185757a2def a ns2:AnonymousAttack,
        owl:NamedIndividual ;
    ns1:associatedCampaigns ns2:Boston_Children_s_Hospital ;
    ns1:description "Protest"^^xsd:string ;
    ns2:behaviour ns2:Protest ;
    ns2:hasActor "Anonymous"^^xsd:string ;
    ns2:hasActorType "Hacktivist"^^xsd:string ;
    ns2:hasCampaign ns2:Massachusetts ;
    ns2:hasCountry "United States of America"^^xsd:string ;
    ns2:hasCounty "Suffolk"^^xsd:string ;
    ns2:hasEventDate "2014-04-28T00:00:00"^^xsd:dateTime ;
    ns2:hasEventSubtype "External Denial of Service"^^xsd:string ;
    ns2:hasEventType "Disruptive"^^xsd:string ;
    ns2:hasIndustry "Health Care and Social Assistance"^^xsd:string ;
    ns2:hasMonth 4 ;
    ns2:hasOrganization "Boston Children's Hospital"^^xsd:string ;
    ns2:hasState "Massachusetts"^^xsd:string ;
    ns2:hasYear 2014 ;
    ns2:isType_of ns2:External_Denial_of_Service,
        ns2:Hacktivist ;
    rdfs:comment "In name of OpJustinaPelletier, the Anonymous take down the website of the Boston Children's Hospital."^^xsd:string .

ns2:af314d9c25919e49 a ns2:AnonymousAttack,
        owl:NamedIndividual ;
    ns1:associatedCampaigns ns2:Globo_TV_Brasil ;
    ns1:description "Protest"^^xsd:string ;
    ns1:isLaunchedBy ns2:Brazil ;
    ns2:behaviour ns2:Protest ;
    ns2:hasActor "Anonymous (Brazil)"^^xsd:string ;
    ns2:hasActorCountry "Brazil"^^xsd:string ;
    ns2:hasActorType "Hacktivist"^^xsd:string ;
    ns2:hasCountry "Brazil"^^xsd:string ;
    ns2:hasEventDate "2014-06-17T00:00:00"^^xsd:dateTime ;
    ns2:hasEventSubtype "Exploitation of Application Server"^^xsd:string ;
    ns2:hasEventType "Exploitive"^^xsd:string ;
    ns2:hasIndustry "Arts, Entertainment, and Recreation"^^xsd:string ;
    ns2:hasMonth 6 ;
    ns2:hasOrganization "Globo TV Brasil"^^xsd:string ;
    ns2:hasYear 2014 ;
    ns2:isType_of ns2:Exploitation_of_Application_Server,
        ns2:Hacktivist ;
    rdfs:comment "As part of #OpWorldCup and #OpHackingCup, Anonymous hacks a number of Brazilian organizations during the World Cup. "^^xsd:string .

ns2:af52b35159acfa04 a ns2:HackerSecurity,
        owl:NamedIndividual ;
    ns1:associatedCampaigns ns2:AVS_TV ;
    ns2:hasActor "DeleteSec"^^xsd:string ;
    ns2:hasActorType "Hacktivist"^^xsd:string ;
    ns2:hasCountry "United States of America"^^xsd:string ;
    ns2:hasEventDate "2014-02-12T00:00:00"^^xsd:dateTime ;
    ns2:hasEventSubtype "Exploitation of Application Server"^^xsd:string ;
    ns2:hasEventType "Exploitive"^^xsd:string ;
    ns2:hasIndustry "Information"^^xsd:string ;
    ns2:hasMonth 2 ;
    ns2:hasOrganization "AVS TV"^^xsd:string ;
    ns2:hasYear 2014 ;
    ns2:isType_of ns2:Exploitation_of_Application_Server,
        ns2:Hacktivist ;
    rdfs:comment "DeleteSec hacks AVS TV (avstv.com) and leaks around 40,000 account credentials of registered users."^^xsd:string .

ns2:b00ee88a9d2ab933 a ns2:BreachInformation,
        owl:NamedIndividual ;
    ns1:associatedCampaigns ns2:University_of_California_Washington_Cent ;
    ns2:hasActorType "Criminal"^^xsd:string ;
    ns2:hasCampaign ns2:Washington_D_C ;
    ns2:hasCountry "United States of America"^^xsd:string ;
    ns2:hasEventDate "2014-06-26T00:00:00"^^xsd:dateTime ;
    ns2:hasEventSubtype "Exploitation of Application Server"^^xsd:string ;
    ns2:hasEventType "Exploitive"^^xsd:string ;
    ns2:hasIndustry "Educational Services"^^xsd:string ;
    ns2:hasMonth 6 ;
    ns2:hasOrganization "University of California Washington Center"^^xsd:string ;
    ns2:hasState "Washington D.C."^^xsd:string ;
    ns2:hasYear 2014 ;
    ns2:isType_of ns2:Criminal,
        ns2:Exploitation_of_Application_Server ;
    rdfs:comment "The University of California, Washington Center (UCDC) notifies alumni of a breach involving their course pre-enrollment system. The attack targeted UCDC's cloud-based provider, GoSignMeUp.com."^^xsd:string .

ns2:b047f3f91273a486 a ns2:Malware,
        owl:NamedIndividual ;
    ns1:associatedCampaigns ns2:Jean_Jacques_Quisquater ;
    ns1:description "Political-Espionage"^^xsd:string ;
    ns1:isLaunchedBy ns2:United_States_of_America ;
    ns2:behaviour ns2:Political_Espionage ;
    ns2:hasActor "National Security Agency"^^xsd:string ;
    ns2:hasActorCountry "United States of America"^^xsd:string ;
    ns2:hasActorType "Nation-State"^^xsd:string ;
    ns2:hasCountry "Belgium"^^xsd:string ;
    ns2:hasEventDate "2014-02-01T00:00:00"^^xsd:dateTime ;
    ns2:hasEventSubtype "Exploitation of End Hosts"^^xsd:string ;
    ns2:hasEventType "Exploitive"^^xsd:string ;
    ns2:hasIndustry "Other Services (except Public Administration)"^^xsd:string ;
    ns2:hasMonth 2 ;
    ns2:hasOrganization "Jean-Jacques Quisquater"^^xsd:string ;
    ns2:hasYear 2014 ;
    ns2:isType_of ns2:Exploitation_of_End_Hosts,
        ns2:Nation_State ;
    rdfs:comment "Jean-Jacques Quisquater, a Belgian cryptographer, is an apparent victim of the NSA's Regin malware."^^xsd:string .

ns2:b0fd742860464bfc a ns2:AnonymousAttack,
        owl:NamedIndividual ;
    ns1:associatedCampaigns ns2:Telenor ;
    ns1:description "Protest"^^xsd:string ;
    ns1:isLaunchedBy ns2:Norway ;
    ns2:behaviour ns2:Protest ;
    ns2:hasActor "Anonymous (Norway)"^^xsd:string ;
    ns2:hasActorCountry "Norway"^^xsd:string ;
    ns2:hasActorType "Hacktivist"^^xsd:string ;
    ns2:hasCountry "Norway"^^xsd:string ;
    ns2:hasEventDate "2014-07-09T00:00:00"^^xsd:dateTime ;
    ns2:hasEventSubtype "External Denial of Service"^^xsd:string ;
    ns2:hasEventType "Disruptive"^^xsd:string ;
    ns2:hasIndustry "Information"^^xsd:string ;
    ns2:hasMonth 7 ;
    ns2:hasOrganization "Telenor"^^xsd:string ;
    ns2:hasYear 2014 ;
    ns2:isType_of ns2:External_Denial_of_Service,
        ns2:Hacktivist ;
    rdfs:comment "Anonymous Norway starts multiple DDoS attacks towards major banks and insurance companies in Norway, including the country's largest telecommunications company, Telenor."^^xsd:string .

ns2:b1a2323cb0b5c776 a ns2:CyberattackInformation,
        owl:NamedIndividual ;
    ns1:associatedCampaigns ns2:Various_Government_Websites ;
    ns1:isLaunchedBy ns2:Azerbaijan ;
    ns2:hasActor "Monte Melkonian Cyber Army (MMCA)"^^xsd:string ;
    ns2:hasActorCountry "Azerbaijan"^^xsd:string ;
    ns2:hasActorType "Hacktivist"^^xsd:string ;
    ns2:hasCountry "Azerbaijan"^^xsd:string ;
    ns2:hasEventDate "2014-08-24T00:00:00"^^xsd:dateTime ;
    ns2:hasEventSubtype "Message Manipulation,External Denial of Service"^^xsd:string ;
    ns2:hasEventType "Disruptive"^^xsd:string ;
    ns2:hasIndustry "Public Administration"^^xsd:string ;
    ns2:hasMonth 8 ;
    ns2:hasOrganization "Various Government Websites"^^xsd:string ;
    ns2:hasYear 2014 ;
    ns2:isType_of ns2:Hacktivist,
        ns2:Message_Manipulation_External_Denial_of_ ;
    rdfs:comment "A group of Armenian hackers going with the handle of Monte Melkonian Cyber Army (MMCA) claim to have defaced several Azerbaijani websites and to have executed a DDoS attack against  Azerbaijani targets reaching 300 Gbps."^^xsd:string .

ns2:b1c433e3938c5448 a ns2:HackerSecurity,
        owl:NamedIndividual ;
    ns1:associatedCampaigns ns2:TTNET ;
    ns1:description "Protest"^^xsd:string ;
    ns1:isLaunchedBy ns2:Turkey ;
    ns2:behaviour ns2:Protest ;
    ns2:hasActor "RedHack"^^xsd:string ;
    ns2:hasActorCountry "Turkey"^^xsd:string ;
    ns2:hasActorType "Hacktivist"^^xsd:string ;
    ns2:hasCountry "Turkey"^^xsd:string ;
    ns2:hasEventDate "2014-02-04T00:00:00"^^xsd:dateTime ;
    ns2:hasEventSubtype "Exploitation of Application Server"^^xsd:string ;
    ns2:hasEventType "Exploitive"^^xsd:string ;
    ns2:hasIndustry "Information"^^xsd:string ;
    ns2:hasMonth 2 ;
    ns2:hasOrganization "TTNET"^^xsd:string ;
    ns2:hasYear 2014 ;
    ns2:isType_of ns2:Exploitation_of_Application_Server,
        ns2:Hacktivist ;
    rdfs:comment "Hackers of the RedHack group claim to have breached the systems of three major telecoms companies: TTNET, Vodafone and Turkcell. After the attack they leak the details of hundreds of individuals from TTNET and 5,000 Vodafone customers."^^xsd:string .

ns2:b1e0786613c7b8d7 a ns2:BreachInformation,
        owl:NamedIndividual ;
    ns1:associatedCampaigns ns2:Well_ca ;
    ns1:description "Financial"^^xsd:string ;
    ns2:behaviour ns2:Financial ;
    ns2:hasActorType "Criminal"^^xsd:string ;
    ns2:hasCountry "Canada"^^xsd:string ;
    ns2:hasEventDate "2014-02-18T00:00:00"^^xsd:dateTime ;
    ns2:hasEventSubtype "Exploitation of Application Server"^^xsd:string ;
    ns2:hasEventType "Exploitive"^^xsd:string ;
    ns2:hasIndustry "Retail Trade"^^xsd:string ;
    ns2:hasMonth 2 ;
    ns2:hasOrganization "Well.ca"^^xsd:string ;
    ns2:hasYear 2014 ;
    ns2:isType_of ns2:Criminal,
        ns2:Exploitation_of_Application_Server ;
    rdfs:comment "Well.ca, a Canadian online retailer for health and beauty products, declares to have suffered a data breach, compromising the credit card information of a few thousandÃÆÃ'Ãâ 'ÃÆÃ¢â¬Â 'ÃÆÃ'ÃÂ¢Ã¢'Â¬ÃÂ ''ÃÆÃ'Ãâ 'ÃÆÃ¢â¬Â ''ÃÆÃ'Ãâ ''ÃÆÃ''ÃÆ'Ã'ÃÂ of its customers."^^xsd:string .

ns2:b22907325a028aa4 a ns2:CyberattackData,
        owl:NamedIndividual ;
    ns1:associatedCampaigns ns2:Comcast ;
    ns2:hasActor "NullCrew"^^xsd:string ;
    ns2:hasActorType "Hacktivist"^^xsd:string ;
    ns2:hasCampaign ns2:Pennsylvania ;
    ns2:hasCountry "United States of America"^^xsd:string ;
    ns2:hasCounty "Philadelphia"^^xsd:string ;
    ns2:hasEventDate "2014-02-05T00:00:00"^^xsd:dateTime ;
    ns2:hasEventSubtype "Exploitation of Application Server"^^xsd:string ;
    ns2:hasEventType "Exploitive"^^xsd:string ;
    ns2:hasIndustry "Information"^^xsd:string ;
    ns2:hasMonth 2 ;
    ns2:hasOrganization "Comcast"^^xsd:string ;
    ns2:hasState "Pennsylvania"^^xsd:string ;
    ns2:hasYear 2014 ;
    ns2:isType_of ns2:Exploitation_of_Application_Server,
        ns2:Hacktivist ;
    rdfs:comment "The NullCrew collective claim to have successfully hacked Comcast, providing a link on Pastebin to unredacted information as evidence."^^xsd:string .

ns2:b25d0d72570f0acf a ns2:HackerSecurity,
        owl:NamedIndividual ;
    ns1:associatedCampaigns ns2:Texas_State_Technical_College ;
    ns1:description "Financial"^^xsd:string ;
    ns2:behaviour ns2:Financial ;
    ns2:hasActorType "Criminal"^^xsd:string ;
    ns2:hasCampaign ns2:Texas ;
    ns2:hasCountry "United States of America"^^xsd:string ;
    ns2:hasCounty "McLennan"^^xsd:string ;
    ns2:hasEventDate "2014-02-19T00:00:00"^^xsd:dateTime ;
    ns2:hasEventSubtype "Exploitation of Application Server"^^xsd:string ;
    ns2:hasEventType "Exploitive"^^xsd:string ;
    ns2:hasIndustry "Educational Services"^^xsd:string ;
    ns2:hasMonth 2 ;
    ns2:hasOrganization "Texas State Technical College"^^xsd:string ;
    ns2:hasState "Texas"^^xsd:string ;
    ns2:hasYear 2014 ;
    ns2:isType_of ns2:Criminal,
        ns2:Exploitation_of_Application_Server ;
    rdfs:comment "Texas State Technical College (tstc.edu) Waco notifies almost 3,000 former students and fewer than 2,000 employees that personal information may have been compromised after an unauthorized party remotely gained access to a server that contained the data."^^xsd:string .

ns2:b295628dc1eaf4e2 a ns2:DDoS,
        owl:NamedIndividual ;
    ns1:associatedCampaigns ns2:Moz ;
    ns1:description "Financial"^^xsd:string ;
    ns2:behaviour ns2:Financial ;
    ns2:hasActorType "Criminal"^^xsd:string ;
    ns2:hasCampaign ns2:Washington ;
    ns2:hasCountry "United States of America"^^xsd:string ;
    ns2:hasCounty "King"^^xsd:string ;
    ns2:hasEventDate "2014-05-17T00:00:00"^^xsd:dateTime ;
    ns2:hasEventSubtype "External Denial of Service"^^xsd:string ;
    ns2:hasEventType "Disruptive"^^xsd:string ;
    ns2:hasIndustry "Information"^^xsd:string ;
    ns2:hasMonth 5 ;
    ns2:hasOrganization "Moz"^^xsd:string ;
    ns2:hasState "Washington"^^xsd:string ;
    ns2:hasYear 2014 ;
    ns2:isType_of ns2:Criminal,
        ns2:External_Denial_of_Service ;
    rdfs:comment "Yet another DDoS attack. This time the victim is moz.com."^^xsd:string .

ns2:b343d7f2a4a12bd7 a ns2:HackerSecurity,
        owl:NamedIndividual ;
    ns1:associatedCampaigns ns2:Russian_Industrial_Investment_Fund ;
    ns1:description "Protest"^^xsd:string ;
    ns1:isLaunchedBy ns2:Russian_Federation ;
    ns2:behaviour ns2:Protest ;
    ns2:hasActor "Russian Cyber Command"^^xsd:string ;
    ns2:hasActorCountry "Russian Federation"^^xsd:string ;
    ns2:hasActorType "Hacktivist"^^xsd:string ;
    ns2:hasCountry "Russian Federation"^^xsd:string ;
    ns2:hasEventDate "2014-03-17T00:00:00"^^xsd:dateTime ;
    ns2:hasEventSubtype "Exploitation of End Hosts"^^xsd:string ;
    ns2:hasEventType "Exploitive"^^xsd:string ;
    ns2:hasIndustry "Public Administration"^^xsd:string ;
    ns2:hasMonth 3 ;
    ns2:hasOrganization "Russian Industrial Investment Fund"^^xsd:string ;
    ns2:hasYear 2014 ;
    ns2:isType_of ns2:Exploitation_of_End_Hosts,
        ns2:Hacktivist ;
    rdfs:comment "Hacktivists of the Russian Cyber Command (@Rucyborg) claim to have hacked the computer of Alexandr Bagnuk, the president of  the Russian Industrial Investment Fund, a semi-governmental investment company established by a decree of the president of Russia."^^xsd:string .

ns2:b343e33bb2bc6944 a ns2:BreachInformation,
        owl:NamedIndividual ;
    ns1:associatedCampaigns ns2:AECOM ;
    ns1:description "Financial"^^xsd:string ;
    ns2:behaviour ns2:Financial ;
    ns2:hasActorType "Criminal"^^xsd:string ;
    ns2:hasCampaign ns2:California ;
    ns2:hasCountry "United States of America"^^xsd:string ;
    ns2:hasCounty "Los Angeles"^^xsd:string ;
    ns2:hasEventDate "2014-07-16T00:00:00"^^xsd:dateTime ;
    ns2:hasEventSubtype "Exploitation of Application Server"^^xsd:string ;
    ns2:hasEventType "Exploitive"^^xsd:string ;
    ns2:hasIndustry "Professional, Scientific, and Technical Services"^^xsd:string ;
    ns2:hasMonth 7 ;
    ns2:hasOrganization "AECOM"^^xsd:string ;
    ns2:hasState "California"^^xsd:string ;
    ns2:hasYear 2014 ;
    ns2:isType_of ns2:Criminal,
        ns2:Exploitation_of_Application_Server ;
    rdfs:comment "AECOM notifies its employees of an intrusion resulting in the exposure of personal information of past and present employees."^^xsd:string .

ns2:b3a12359b1b6b620 a ns2:AnonymousAttack,
        owl:NamedIndividual ;
    ns1:associatedCampaigns ns2:Pakistan_Meteorological_Department ;
    ns2:hasActor "Anonymous"^^xsd:string ;
    ns2:hasActorType "Hacktivist"^^xsd:string ;
    ns2:hasCountry "Pakistan"^^xsd:string ;
    ns2:hasEventDate "2014-08-30T00:00:00"^^xsd:dateTime ;
    ns2:hasEventSubtype "External Denial of Service"^^xsd:string ;
    ns2:hasEventType "Disruptive"^^xsd:string ;
    ns2:hasIndustry "Public Administration"^^xsd:string ;
    ns2:hasMonth 8 ;
    ns2:hasOrganization "Pakistan Meteorological Department"^^xsd:string ;
    ns2:hasYear 2014 ;
    ns2:isType_of ns2:External_Denial_of_Service,
        ns2:Hacktivist ;
    rdfs:comment "In the name of #OpPakistan, Anonymous conducts a massive cyber attack against many Pakistani government websites, including Parkistan Army's recruitment website, government of Punjab's official portal, Pakistan Meteorological Department, Employees Old-Age Benefits Institution, and several other high-profile sites."^^xsd:string .

ns2:b3e92e921cb7d123 a ns2:BreachInformation,
        owl:NamedIndividual ;
    ns1:associatedCampaigns ns2:Bartell_Hotels ;
    ns1:description "Financial"^^xsd:string ;
    ns2:behaviour ns2:Financial ;
    ns2:hasActorType "Criminal"^^xsd:string ;
    ns2:hasCampaign ns2:California ;
    ns2:hasCountry "United States of America"^^xsd:string ;
    ns2:hasCounty "San Diego"^^xsd:string ;
    ns2:hasEventDate "2014-09-03T00:00:00"^^xsd:dateTime ;
    ns2:hasEventSubtype "Exploitation of Sensors"^^xsd:string ;
    ns2:hasEventType "Exploitive"^^xsd:string ;
    ns2:hasIndustry "Accommodation and Food Services"^^xsd:string ;
    ns2:hasMonth 9 ;
    ns2:hasOrganization "Bartell Hotels"^^xsd:string ;
    ns2:hasState "California"^^xsd:string ;
    ns2:hasYear 2014 ;
    ns2:isType_of ns2:Criminal,
        ns2:Exploitation_of_Sensors ;
    rdfs:comment "Bartell Hotels issues a notification that the payment card processing systems used at five of its San Diego locations were compromised and personal information, including credit card numbers, may be at risk. The potential number of affected customers is estimated to be between 40,000 and 45,000."^^xsd:string .

ns2:b405b57184b1ad91 a ns2:HackerSecurity,
        owl:NamedIndividual ;
    ns1:associatedCampaigns ns2:Avast ;
    ns2:hasActorType "Criminal"^^xsd:string ;
    ns2:hasCountry "Czechia"^^xsd:string ;
    ns2:hasEventDate "2014-05-27T00:00:00"^^xsd:dateTime ;
    ns2:hasEventSubtype "Exploitation of Application Server"^^xsd:string ;
    ns2:hasEventType "Exploitive"^^xsd:string ;
    ns2:hasIndustry "Professional, Scientific, and Technical Services"^^xsd:string ;
    ns2:hasMonth 5 ;
    ns2:hasOrganization "Avast"^^xsd:string ;
    ns2:hasYear 2014 ;
    ns2:isType_of ns2:Criminal,
        ns2:Exploitation_of_Application_Server ;
    rdfs:comment "The support forum of Avast is hacked. Attackers get access to cryptographically hashed passwords, usernames, and e-mail addresses for about 400,000 people."^^xsd:string .

ns2:b4125a3225e0f7aa a ns2:CyberattackData,
        owl:NamedIndividual ;
    ns1:associatedCampaigns ns2:Toyota__Guatemala ;
    ns1:isLaunchedBy ns2:Pakistan ;
    ns2:hasActor "Team Cyber Criminals"^^xsd:string ;
    ns2:hasActorCountry "Pakistan"^^xsd:string ;
    ns2:hasActorType "Hobbyist"^^xsd:string ;
    ns2:hasCountry "Guatemala"^^xsd:string ;
    ns2:hasEventDate "2014-03-18T00:00:00"^^xsd:dateTime ;
    ns2:hasEventSubtype "Message Manipulation"^^xsd:string ;
    ns2:hasEventType "Disruptive"^^xsd:string ;
    ns2:hasIndustry "Manufacturing"^^xsd:string ;
    ns2:hasMonth 3 ;
    ns2:hasOrganization "Toyota (Guatemala)"^^xsd:string ;
    ns2:hasYear 2014 ;
    ns2:isType_of ns2:Hobbyist,
        ns2:Message_Manipulation ;
    rdfs:comment "The Guatemala websites of Renault, Toyota and Chevrolet are hacked and defaced by a member of a Pakistani group called Team Cyber Criminals."^^xsd:string .

ns2:b4db6816b51b584d a ns2:Malware,
        owl:NamedIndividual ;
    ns1:associatedCampaigns ns2:University_of_California_Irvine ;
    ns2:hasActorType "Criminal"^^xsd:string ;
    ns2:hasCampaign ns2:California ;
    ns2:hasCountry "United States of America"^^xsd:string ;
    ns2:hasCounty "Orange"^^xsd:string ;
    ns2:hasEventDate "2014-05-15T00:00:00"^^xsd:dateTime ;
    ns2:hasEventSubtype "Exploitation of End Hosts"^^xsd:string ;
    ns2:hasEventType "Exploitive"^^xsd:string ;
    ns2:hasIndustry "Educational Services"^^xsd:string ;
    ns2:hasMonth 5 ;
    ns2:hasOrganization "University of California Irvine"^^xsd:string ;
    ns2:hasState "California"^^xsd:string ;
    ns2:hasYear 2014 ;
    ns2:isType_of ns2:Criminal,
        ns2:Exploitation_of_End_Hosts ;
    rdfs:comment "More than 1,800 University of California (UC), Irvine, students are notified that they may have had personal information compromised after keylogger malware was discovered on three Student Health Center (SHC) computers for about six weeks."^^xsd:string .

ns2:b5558f85db5ac5b9 a ns2:DDoS,
        owl:NamedIndividual ;
    ns1:associatedCampaigns ns2:Aktif_Bank ;
    ns1:isLaunchedBy ns2:Turkey ;
    ns2:hasActor "RedHack"^^xsd:string ;
    ns2:hasActorCountry "Turkey"^^xsd:string ;
    ns2:hasActorType "Hacktivist"^^xsd:string ;
    ns2:hasCountry "Turkey"^^xsd:string ;
    ns2:hasEventDate "2014-04-18T00:00:00"^^xsd:dateTime ;
    ns2:hasEventSubtype "External Denial of Service,Exploitation of Application Server"^^xsd:string ;
    ns2:hasEventType "Mixed"^^xsd:string ;
    ns2:hasIndustry "Finance and Insurance"^^xsd:string ;
    ns2:hasMonth 4 ;
    ns2:hasOrganization "Aktif Bank"^^xsd:string ;
    ns2:hasYear 2014 ;
    ns2:isType_of ns2:External_Denial_of_Service_Exploitation_,
        ns2:Hacktivist ;
    rdfs:comment "Members of the hacktivist collective RedHack claim to have breached into the systems of Aktif Bank (aktifbank.com.tr), Turkey's largest privately owned investment bank. They also launched a distributed denial of service (DDoS) attack on the website."^^xsd:string .

ns2:b58f2e718b212c97 a ns2:BreachSecurity,
        owl:NamedIndividual ;
    ns1:associatedCampaigns ns2:Dennis_East_International ;
    ns1:description "Financial"^^xsd:string ;
    ns2:behaviour ns2:Financial ;
    ns2:hasActorType "Criminal"^^xsd:string ;
    ns2:hasCampaign ns2:Massachusetts ;
    ns2:hasCountry "United States of America"^^xsd:string ;
    ns2:hasCounty "Plymouth"^^xsd:string ;
    ns2:hasEventDate "2014-07-18T00:00:00"^^xsd:dateTime ;
    ns2:hasEventSubtype "Exploitation of Application Server"^^xsd:string ;
    ns2:hasEventType "Exploitive"^^xsd:string ;
    ns2:hasIndustry "Retail Trade"^^xsd:string ;
    ns2:hasMonth 7 ;
    ns2:hasOrganization "Dennis East International"^^xsd:string ;
    ns2:hasState "Massachusetts"^^xsd:string ;
    ns2:hasYear 2014 ;
    ns2:isType_of ns2:Criminal,
        ns2:Exploitation_of_Application_Server ;
    rdfs:comment "Dennis East International (DEI) reports that its website (hosted by an external company Omeganet) experienced two recent security breaches."^^xsd:string .

ns2:b603de25ad5faf51 a ns2:DDoS,
        owl:NamedIndividual ;
    ns1:associatedCampaigns ns2:Namecheap ;
    ns2:hasActorType "Criminal"^^xsd:string ;
    ns2:hasCampaign ns2:Arizona ;
    ns2:hasCountry "United States of America"^^xsd:string ;
    ns2:hasCounty "Maricopa"^^xsd:string ;
    ns2:hasEventDate "2014-02-20T00:00:00"^^xsd:dateTime ;
    ns2:hasEventSubtype "External Denial of Service"^^xsd:string ;
    ns2:hasEventType "Disruptive"^^xsd:string ;
    ns2:hasIndustry "Information"^^xsd:string ;
    ns2:hasMonth 2 ;
    ns2:hasOrganization "Namecheap"^^xsd:string ;
    ns2:hasState "Arizona"^^xsd:string ;
    ns2:hasYear 2014 ;
    ns2:isType_of ns2:Criminal,
        ns2:External_Denial_of_Service ;
    rdfs:comment "The Web-hosting service Namecheap is hit with one of the largest distributed-denial-of-service attacks affecting roughly 300 domain names hosted by Namecheap."^^xsd:string .

ns2:b685dac48a8057ae a ns2:DDoS,
        owl:NamedIndividual ;
    ns1:associatedCampaigns ns2:Undisclosed_online_gambling_website ;
    ns2:hasActorType "Criminal"^^xsd:string ;
    ns2:hasCountry "United States of America"^^xsd:string ;
    ns2:hasEventDate "2014-06-10T00:00:00"^^xsd:dateTime ;
    ns2:hasEventSubtype "External Denial of Service"^^xsd:string ;
    ns2:hasEventType "Disruptive"^^xsd:string ;
    ns2:hasIndustry "Arts, Entertainment, and Recreation"^^xsd:string ;
    ns2:hasMonth 6 ;
    ns2:hasOrganization "Undisclosed online gambling website"^^xsd:string ;
    ns2:hasYear 2014 ;
    ns2:isType_of ns2:Criminal,
        ns2:External_Denial_of_Service ;
    rdfs:comment "Cloud-based security services provider Incapsula states to have fought off a 100 Gbps DDoS attack against an online gambling website."^^xsd:string .

ns2:b6b2ef63fdd9792a a ns2:HackerSecurity,
        owl:NamedIndividual ;
    ns1:associatedCampaigns ns2:Forbes ;
    ns1:description "Protest"^^xsd:string ;
    ns1:isLaunchedBy ns2:Syrian_Arab_Republic ;
    ns2:behaviour ns2:Protest ;
    ns2:hasActor "Syrian Electronic Army"^^xsd:string ;
    ns2:hasActorCountry "Syrian Arab Republic"^^xsd:string ;
    ns2:hasActorType "Hacktivist"^^xsd:string ;
    ns2:hasCampaign ns2:New_Jersey ;
    ns2:hasCountry "United States of America"^^xsd:string ;
    ns2:hasCounty "Hudson"^^xsd:string ;
    ns2:hasEventDate "2014-02-14T00:00:00"^^xsd:dateTime ;
    ns2:hasEventSubtype "Message Manipulation,Exploitation of Application Server"^^xsd:string ;
    ns2:hasEventType "Mixed"^^xsd:string ;
    ns2:hasIndustry "Information"^^xsd:string ;
    ns2:hasMonth 2 ;
    ns2:hasOrganization "Forbes"^^xsd:string ;
    ns2:hasState "New Jersey"^^xsd:string ;
    ns2:hasYear 2014 ;
    ns2:isType_of ns2:Hacktivist,
        ns2:Message_Manipulation_Exploitation_of_App ;
    rdfs:comment "The Syrian Electronic Army hacks Forbes, stealing user data and posting fake stories to its Web site. Forbes acknowledges the hack stating that e-mail addresses may have been exposed but passwords are encrypted. Apparently 1 million user records are spilled."^^xsd:string .

ns2:b6b349b04a7808e7 a ns2:DDoS,
        owl:NamedIndividual ;
    ns1:associatedCampaigns ns2:Xbox_Live ;
    ns2:hasActorType "Criminal"^^xsd:string ;
    ns2:hasCampaign ns2:Washington ;
    ns2:hasCountry "United States of America"^^xsd:string ;
    ns2:hasCounty "King"^^xsd:string ;
    ns2:hasEventDate "2014-08-25T00:00:00"^^xsd:dateTime ;
    ns2:hasEventSubtype "External Denial of Service"^^xsd:string ;
    ns2:hasEventType "Disruptive"^^xsd:string ;
    ns2:hasIndustry "Information"^^xsd:string ;
    ns2:hasMonth 8 ;
    ns2:hasOrganization "Xbox Live"^^xsd:string ;
    ns2:hasState "Washington"^^xsd:string ;
    ns2:hasYear 2014 ;
    ns2:isType_of ns2:Criminal,
        ns2:External_Denial_of_Service ;
    rdfs:comment "Sony admits that a DDoS attack impacted online services, Sony's PlayStation Network and the Sony Entertainment Network. Other affected services involve: Xbox Live, Blizzard's Battle.net, and Grinding Gear Games."^^xsd:string .

ns2:b74d1ff33ee0a1c0 a ns2:BreachInformation,
        owl:NamedIndividual ;
    ns1:associatedCampaigns ns2:Goodwill_Industries ;
    ns1:description "Financial"^^xsd:string ;
    ns2:behaviour ns2:Financial ;
    ns2:hasActorType "Criminal"^^xsd:string ;
    ns2:hasCountry "United States of America"^^xsd:string ;
    ns2:hasEventDate "2014-07-14T00:00:00"^^xsd:dateTime ;
    ns2:hasEventSubtype "Exploitation of Sensors"^^xsd:string ;
    ns2:hasEventType "Exploitive"^^xsd:string ;
    ns2:hasMonth 7 ;
    ns2:hasOrganization "Goodwill Industries"^^xsd:string ;
    ns2:hasYear 2014 ;
    ns2:isType_of ns2:Criminal,
        ns2:Exploitation_of_Sensors ;
    rdfs:comment "Goodwill Industries is the latest victim of the PoS Breach spree. Stores on 21 states report traces of card frauds."^^xsd:string .

ns2:b795c71a1cbaeef4 a ns2:CyberattackData,
        owl:NamedIndividual ;
    ns1:associatedCampaigns ns2:Anonymous ;
    ns1:isLaunchedBy ns2:Israel ;
    ns2:hasActor "Buddhax"^^xsd:string ;
    ns2:hasActorCountry "Israel"^^xsd:string ;
    ns2:hasActorType "Hacktivist"^^xsd:string ;
    ns2:hasEventDate "2014-04-13T00:00:00"^^xsd:dateTime ;
    ns2:hasEventSubtype "Exploitation of End Hosts"^^xsd:string ;
    ns2:hasEventType "Exploitive"^^xsd:string ;
    ns2:hasIndustry "Other Services (except Public Administration)"^^xsd:string ;
    ns2:hasMonth 4 ;
    ns2:hasOrganization "Anonymous"^^xsd:string ;
    ns2:hasYear 2014 ;
    ns2:isType_of ns2:Exploitation_of_End_Hosts,
        ns2:Hacktivist ;
    rdfs:comment "Israeli hackers attacked computers belonging to Anonymous and allied hacker groups, taking pictures with exploited webcams and posting the photos online."^^xsd:string .

ns2:b8651d4d3c681206 a ns2:DDoS,
        owl:NamedIndividual ;
    ns1:associatedCampaigns ns2:Undisclosed_video_game_company ;
    ns2:hasActorType "Criminal"^^xsd:string ;
    ns2:hasCountry "United States of America"^^xsd:string ;
    ns2:hasEventDate "2014-06-24T00:00:00"^^xsd:dateTime ;
    ns2:hasEventSubtype "External Denial of Service"^^xsd:string ;
    ns2:hasEventType "Disruptive"^^xsd:string ;
    ns2:hasIndustry "Information"^^xsd:string ;
    ns2:hasMonth 6 ;
    ns2:hasOrganization "Undisclosed video game company"^^xsd:string ;
    ns2:hasYear 2014 ;
    ns2:isType_of ns2:Criminal,
        ns2:External_Denial_of_Service ;
    rdfs:comment "Incapsula unveils the details of a DDoS attack against an unnamed Video Games company, achieving a peak of 90 million requests for second."^^xsd:string .

ns2:b8e2bed468676dbe a ns2:CyberattackData,
        owl:NamedIndividual ;
    ns1:associatedCampaigns ns2:Wide_Area_and_Sensing_Conference ;
    ns1:description "Protest"^^xsd:string ;
    ns2:behaviour ns2:Protest ;
    ns2:hasActor "@G3NTbl4ck"^^xsd:string ;
    ns2:hasActorType "Hacktivist"^^xsd:string ;
    ns2:hasCountry "United States of America"^^xsd:string ;
    ns2:hasEventDate "2014-02-11T00:00:00"^^xsd:dateTime ;
    ns2:hasEventSubtype "Exploitation of Application Server"^^xsd:string ;
    ns2:hasEventType "Exploitive"^^xsd:string ;
    ns2:hasIndustry "Other Services (except Public Administration)"^^xsd:string ;
    ns2:hasMonth 2 ;
    ns2:hasOrganization "Wide Area and Sensing Conference"^^xsd:string ;
    ns2:hasYear 2014 ;
    ns2:isType_of ns2:Exploitation_of_Application_Server,
        ns2:Hacktivist ;
    rdfs:comment "In name of OpBigBrother, @G3NTbl4ck hacks the Wide Area and Sensing Conference (wasc.rmtech.org) leaking more than 2,000 records."^^xsd:string .

ns2:b91c4a13d00bc120 a ns2:AttackSecurity,
        owl:NamedIndividual ;
    ns1:associatedCampaigns ns2:AT_T ;
    ns1:description "Financial"^^xsd:string ;
    ns2:behaviour ns2:Financial ;
    ns2:hasActorType "Criminal"^^xsd:string ;
    ns2:hasCampaign ns2:Texas ;
    ns2:hasCountry "United States of America"^^xsd:string ;
    ns2:hasCounty "Dallas"^^xsd:string ;
    ns2:hasEventDate "2014-06-16T00:00:00"^^xsd:dateTime ;
    ns2:hasEventSubtype "Exploitation of Application Server"^^xsd:string ;
    ns2:hasEventType "Exploitive"^^xsd:string ;
    ns2:hasIndustry "Information"^^xsd:string ;
    ns2:hasMonth 6 ;
    ns2:hasOrganization "AT&T"^^xsd:string ;
    ns2:hasState "Texas"^^xsd:string ;
    ns2:hasYear 2014 ;
    ns2:isType_of ns2:Criminal,
        ns2:Exploitation_of_Application_Server ;
    rdfs:comment "AT&T confirms that outside attackers (allegedly employees of one of AT&T's service providers) compromised the personal information of an undisclosed number of AT&T Mobility members."^^xsd:string .

ns2:b9bbdafe64918a57 a ns2:CyberattackInformation,
        owl:NamedIndividual ;
    ns1:associatedCampaigns ns2:University_of_Maryland__College_Park ;
    ns2:hasActorType "Criminal"^^xsd:string ;
    ns2:hasCampaign ns2:Maryland ;
    ns2:hasCountry "United States of America"^^xsd:string ;
    ns2:hasCounty "Prince George's"^^xsd:string ;
    ns2:hasEventDate "2014-03-20T00:00:00"^^xsd:dateTime ;
    ns2:hasEventSubtype "Exploitation of End Hosts"^^xsd:string ;
    ns2:hasEventType "Exploitive"^^xsd:string ;
    ns2:hasIndustry "Educational Services"^^xsd:string ;
    ns2:hasMonth 3 ;
    ns2:hasOrganization "University of Maryland, College Park"^^xsd:string ;
    ns2:hasState "Maryland"^^xsd:string ;
    ns2:hasYear 2014 ;
    ns2:isType_of ns2:Criminal,
        ns2:Exploitation_of_End_Hosts ;
    rdfs:comment "The University of Maryland, College Park suffers another cyberattack. The breach is unrelatedï¿½ to last month's cyberattack."^^xsd:string .

ns2:bab9b5a1929df267 a ns2:CyberattackData,
        owl:NamedIndividual ;
    ns1:associatedCampaigns ns2:Hillary_Clinton ;
    ns1:isLaunchedBy ns2:Germany ;
    ns2:hasActor "Bundeswehr's Computer Network Operations Unit (CNO)"^^xsd:string ;
    ns2:hasActorCountry "Germany"^^xsd:string ;
    ns2:hasActorType "Nation-State"^^xsd:string ;
    ns2:hasCountry "United States of America"^^xsd:string ;
    ns2:hasEventDate "2014-08-17T00:00:00"^^xsd:dateTime ;
    ns2:hasEventSubtype "Exploitation of End Hosts"^^xsd:string ;
    ns2:hasEventType "Exploitive"^^xsd:string ;
    ns2:hasIndustry "Public Administration"^^xsd:string ;
    ns2:hasMonth 8 ;
    ns2:hasOrganization "Hillary Clinton"^^xsd:string ;
    ns2:hasYear 2014 ;
    ns2:isType_of ns2:Exploitation_of_End_Hosts,
        ns2:Nation_State ;
    rdfs:comment "According to reports coming from the German media, the German Foreign Intelligence Agency known as Bundesnachrichtendienst (BND) hacked into at least one call during Hillary Clinton's time in office as US Secretary of State."^^xsd:string .

ns2:bb6bbe910e37bbf6 a ns2:HackerSecurity,
        owl:NamedIndividual ;
    ns1:associatedCampaigns ns2:St__Jude_Medical ;
    ns1:description "Industrial-Espionage"^^xsd:string ;
    ns2:behaviour ns2:Industrial_Espionage ;
    ns2:hasActorType "Criminal"^^xsd:string ;
    ns2:hasCampaign ns2:Minnesota ;
    ns2:hasCountry "United States of America"^^xsd:string ;
    ns2:hasCounty "Dakota"^^xsd:string ;
    ns2:hasEventDate "2014-02-10T00:00:00"^^xsd:dateTime ;
    ns2:hasEventSubtype "Exploitation of Application Server"^^xsd:string ;
    ns2:hasEventType "Exploitive"^^xsd:string ;
    ns2:hasMonth 2 ;
    ns2:hasOrganization "St. Jude Medical"^^xsd:string ;
    ns2:hasState "Minnesota"^^xsd:string ;
    ns2:hasYear 2014 ;
    ns2:isType_of ns2:Criminal,
        ns2:Exploitation_of_Application_Server ;
    rdfs:comment "The computer networks of three big medical device makers are breached by unknown attackers likely interested in the companies' intellectual property. The companies in question are Medtronic, Boston Scientific and St. Jude Medical."^^xsd:string .

ns2:bc93c9a68d1edd73 a ns2:AttackWebsite,
        owl:NamedIndividual ;
    ns1:associatedCampaigns ns2:Ateneo_Integrated_Student_Information_Sy ;
    ns1:description "Protest"^^xsd:string ;
    ns2:behaviour ns2:Protest ;
    ns2:hasActor "Pinoy Anonymouz"^^xsd:string ;
    ns2:hasActorType "Hacktivist"^^xsd:string ;
    ns2:hasCountry "Philippines"^^xsd:string ;
    ns2:hasEventDate "2014-02-02T00:00:00"^^xsd:dateTime ;
    ns2:hasEventSubtype "Message Manipulation"^^xsd:string ;
    ns2:hasEventType "Disruptive"^^xsd:string ;
    ns2:hasIndustry "Educational Services"^^xsd:string ;
    ns2:hasMonth 2 ;
    ns2:hasOrganization "Ateneo Integrated Student Information System"^^xsd:string ;
    ns2:hasYear 2014 ;
    ns2:isType_of ns2:Hacktivist,
        ns2:Message_Manipulation ;
    rdfs:comment "A group identified as \"Pinoy Anonymouz\" defaces the website of the Ateneo Integrated Student Information System (AISIS)."^^xsd:string .

ns2:bc998b6181a5a4aa a ns1:ExploitTarget,
        owl:NamedIndividual ;
    ns1:associatedCampaigns ns2:Julie_Bishop ;
    ns1:description "Political-Espionage"^^xsd:string ;
    ns2:behaviour ns2:Political_Espionage ;
    ns2:hasActorType "Criminal"^^xsd:string ;
    ns2:hasCountry "Australia"^^xsd:string ;
    ns2:hasEventDate "2014-08-18T00:00:00"^^xsd:dateTime ;
    ns2:hasEventSubtype "Exploitation of End Hosts"^^xsd:string ;
    ns2:hasEventType "Exploitive"^^xsd:string ;
    ns2:hasIndustry "Public Administration"^^xsd:string ;
    ns2:hasMonth 8 ;
    ns2:hasOrganization "Julie Bishop"^^xsd:string ;
    ns2:hasYear 2014 ;
    ns2:isType_of ns2:Criminal,
        ns2:Exploitation_of_End_Hosts ;
    rdfs:comment "Australian Foreign Minister Julie Bishop is the latest victim to be targeted by suspected state-sponsored phone hackers, having her smartphone seized by local intelligence officials after a two-week international sojourn."^^xsd:string .

ns2:bcd44ee9b24bd5e5 a ns2:DDoS,
        owl:NamedIndividual ;
    ns1:associatedCampaigns ns2:Plenty_of_Fish ;
    ns1:description "Financial"^^xsd:string ;
    ns2:behaviour ns2:Financial ;
    ns2:hasActorType "Criminal"^^xsd:string ;
    ns2:hasCountry "United States of America"^^xsd:string ;
    ns2:hasEventDate "2014-05-20T00:00:00"^^xsd:dateTime ;
    ns2:hasEventSubtype "External Denial of Service"^^xsd:string ;
    ns2:hasEventType "Disruptive"^^xsd:string ;
    ns2:hasIndustry "Other Services (except Public Administration)"^^xsd:string ;
    ns2:hasMonth 5 ;
    ns2:hasOrganization "Plenty of Fish"^^xsd:string ;
    ns2:hasYear 2014 ;
    ns2:isType_of ns2:Criminal,
        ns2:External_Denial_of_Service ;
    rdfs:comment "Plenty of Fish is the latest victim of a DDoS attack."^^xsd:string .

ns2:bd43b6f45f43e990 a ns2:AttackEmail,
        owl:NamedIndividual ;
    ns1:associatedCampaigns ns2:FC_Barcelona ;
    ns1:description "Protest"^^xsd:string ;
    ns1:isLaunchedBy ns2:Syrian_Arab_Republic ;
    ns2:behaviour ns2:Protest ;
    ns2:hasActor "Syrian Electronic Army"^^xsd:string ;
    ns2:hasActorCountry "Syrian Arab Republic"^^xsd:string ;
    ns2:hasActorType "Hacktivist"^^xsd:string ;
    ns2:hasCountry "Spain"^^xsd:string ;
    ns2:hasEventDate "2014-02-19T00:00:00"^^xsd:dateTime ;
    ns2:hasEventSubtype "Message Manipulation"^^xsd:string ;
    ns2:hasEventType "Disruptive"^^xsd:string ;
    ns2:hasIndustry "Arts, Entertainment, and Recreation"^^xsd:string ;
    ns2:hasMonth 2 ;
    ns2:hasOrganization "FC Barcelona"^^xsd:string ;
    ns2:hasYear 2014 ;
    ns2:isType_of ns2:Hacktivist,
        ns2:Message_Manipulation ;
    rdfs:comment "The official Twitter Account of FC Barcelona (@FCBarcelona) is hacked by the Syrian Electronic Army who also post a message against Qatar."^^xsd:string .

ns2:be5a11dd6c0c6c8a a ns2:HackerSecurity,
        owl:NamedIndividual ;
    ns1:associatedCampaigns ns2:hackforums_net ;
    ns1:isLaunchedBy ns2:United_States_of_America ;
    ns2:hasActor "Eg-R1z"^^xsd:string ;
    ns2:hasActorCountry "United States of America"^^xsd:string ;
    ns2:hasActorType "Hacktivist"^^xsd:string ;
    ns2:hasCountry "United States of America"^^xsd:string ;
    ns2:hasEventDate "2014-08-28T00:00:00"^^xsd:dateTime ;
    ns2:hasEventSubtype "Message Manipulation"^^xsd:string ;
    ns2:hasEventType "Disruptive"^^xsd:string ;
    ns2:hasIndustry "Information"^^xsd:string ;
    ns2:hasMonth 8 ;
    ns2:hasOrganization "hackforums.net"^^xsd:string ;
    ns2:hasYear 2014 ;
    ns2:isType_of ns2:Hacktivist,
        ns2:Message_Manipulation ;
    rdfs:comment "Hackforums.net, one of the most popular hacking forums in the world, is defaced by an Egyptian hacker with the online handle Eg-R1z."^^xsd:string .

ns2:befaf7e40d1f2739 a ns2:AnonymousAttack,
        owl:NamedIndividual ;
    ns1:associatedCampaigns ns2:Government_of_Punjab ;
    ns2:hasActor "Anonymous"^^xsd:string ;
    ns2:hasActorType "Hacktivist"^^xsd:string ;
    ns2:hasCountry "Pakistan"^^xsd:string ;
    ns2:hasEventDate "2014-08-30T00:00:00"^^xsd:dateTime ;
    ns2:hasEventSubtype "External Denial of Service"^^xsd:string ;
    ns2:hasEventType "Disruptive"^^xsd:string ;
    ns2:hasIndustry "Public Administration"^^xsd:string ;
    ns2:hasMonth 8 ;
    ns2:hasOrganization "Government of Punjab"^^xsd:string ;
    ns2:hasYear 2014 ;
    ns2:isType_of ns2:External_Denial_of_Service,
        ns2:Hacktivist ;
    rdfs:comment "In the name of #OpPakistan, Anonymous conducts a massive cyber attack against many Pakistani government websites, including Parkistan Army's recruitment website, government of Punjab's official portal, Pakistan Meteorological Department, Employees Old-Age Benefits Institution, and several other high-profile sites."^^xsd:string .

ns2:bf0344b8c02f9b4f a ns2:AttackPhishing,
        owl:NamedIndividual ;
    ns1:associatedCampaigns ns2:ThrustVPS ;
    ns2:hasActorType "Criminal"^^xsd:string ;
    ns2:hasCountry "United Kingdom of Great Britain and Northern Ireland"^^xsd:string ;
    ns2:hasEventDate "2014-01-21T00:00:00"^^xsd:dateTime ;
    ns2:hasEventSubtype "External Denial of Service"^^xsd:string ;
    ns2:hasEventType "Disruptive"^^xsd:string ;
    ns2:hasIndustry "Information"^^xsd:string ;
    ns2:hasMonth 1 ;
    ns2:hasOrganization "ThrustVPS"^^xsd:string ;
    ns2:hasYear 2014 ;
    ns2:isType_of ns2:Criminal,
        ns2:External_Denial_of_Service ;
    rdfs:comment "Virtual private server firm ThrustVPS is the victim of a DDOS and Spear-Phishing attack and, as a precaution, asks to its customers to change passwords."^^xsd:string .

ns2:bf7a5794590c1c93 a ns2:BreachInformation,
        owl:NamedIndividual ;
    ns1:associatedCampaigns ns2:Lea_Michele ;
    ns1:description "Personal Attack"^^xsd:string ;
    ns2:behaviour ns2:Personal_Attack ;
    ns2:hasActorType "Criminal"^^xsd:string ;
    ns2:hasCountry "United States of America"^^xsd:string ;
    ns2:hasEventDate "2014-08-31T00:00:00"^^xsd:dateTime ;
    ns2:hasEventSubtype "Exploitation of Application Server"^^xsd:string ;
    ns2:hasEventType "Exploitive"^^xsd:string ;
    ns2:hasIndustry "Other Services (except Public Administration)"^^xsd:string ;
    ns2:hasMonth 8 ;
    ns2:hasOrganization "Lea Michele"^^xsd:string ;
    ns2:hasYear 2014 ;
    ns2:isType_of ns2:Criminal,
        ns2:Exploitation_of_Application_Server ;
    rdfs:comment "Yet another leak of celebrities pictures. A massive leak of nude and risque photos appearing to be of huge stars like is leaked online, first appearing on 4chan."^^xsd:string .

ns2:bf7a7af20eeb296e a ns2:AttackWebsite,
        owl:NamedIndividual ;
    ns1:associatedCampaigns ns2:Malaysian_Ministry_of_Education ;
    ns2:hasActor "Evil Shadow Team"^^xsd:string ;
    ns2:hasActorType "Hobbyist"^^xsd:string ;
    ns2:hasCountry "Malaysia"^^xsd:string ;
    ns2:hasEventDate "2014-01-03T00:00:00"^^xsd:dateTime ;
    ns2:hasEventSubtype "Message Manipulation"^^xsd:string ;
    ns2:hasEventType "Disruptive"^^xsd:string ;
    ns2:hasIndustry "Public Administration"^^xsd:string ;
    ns2:hasMonth 1 ;
    ns2:hasOrganization "Malaysian Ministry of Education"^^xsd:string ;
    ns2:hasYear 2014 ;
    ns2:isType_of ns2:Hobbyist,
        ns2:Message_Manipulation ;
    rdfs:comment "Hackers belonging to a group called Evil Shadow Team deface the website of Malaysia's Ministry of Education (moe.gov.my)."^^xsd:string .

ns2:bf894d48500a8941 a ns2:DDoS,
        owl:NamedIndividual ;
    ns1:associatedCampaigns ns2:GitHub ;
    ns2:hasActorType "Criminal"^^xsd:string ;
    ns2:hasCampaign ns2:California ;
    ns2:hasCountry "United States of America"^^xsd:string ;
    ns2:hasCounty "San Francisco"^^xsd:string ;
    ns2:hasEventDate "2014-03-21T00:00:00"^^xsd:dateTime ;
    ns2:hasEventSubtype "External Denial of Service"^^xsd:string ;
    ns2:hasEventType "Disruptive"^^xsd:string ;
    ns2:hasIndustry "Information"^^xsd:string ;
    ns2:hasMonth 3 ;
    ns2:hasOrganization "GitHub"^^xsd:string ;
    ns2:hasState "California"^^xsd:string ;
    ns2:hasYear 2014 ;
    ns2:isType_of ns2:Criminal,
        ns2:External_Denial_of_Service ;
    rdfs:comment "Github is the victim of another DDoS attack."^^xsd:string .

ns2:bf93033148a466cb a ns2:CyberattackData,
        owl:NamedIndividual ;
    ns1:associatedCampaigns ns2:Official_Portal_for_Manila__Philippines ;
    ns1:description "Protest"^^xsd:string ;
    ns1:isLaunchedBy ns2:Philippines ;
    ns2:behaviour ns2:Protest ;
    ns2:hasActor "VirtuaL DARKWAR2"^^xsd:string ;
    ns2:hasActorCountry "Philippines"^^xsd:string ;
    ns2:hasActorType "Hacktivist"^^xsd:string ;
    ns2:hasCountry "Philippines"^^xsd:string ;
    ns2:hasEventDate "2014-06-25T00:00:00"^^xsd:dateTime ;
    ns2:hasEventSubtype "Message Manipulation"^^xsd:string ;
    ns2:hasEventType "Disruptive"^^xsd:string ;
    ns2:hasIndustry "Public Administration"^^xsd:string ;
    ns2:hasMonth 6 ;
    ns2:hasOrganization "Official Portal for Manila, Philippines"^^xsd:string ;
    ns2:hasYear 2014 ;
    ns2:isType_of ns2:Hacktivist,
        ns2:Message_Manipulation ;
    rdfs:comment "Two Turkish hackers going with the handle of VirtuaL & DARKWAR2 deface the official web portal of Manila City, Philippines (manila.gov.ph) with anti-America, anti-Israel and anti-Saudi Arabia images."^^xsd:string .

ns2:c01bf67caadc98c5 a ns2:AttackWebsite,
        owl:NamedIndividual ;
    ns1:associatedCampaigns ns2:Almajmah_Principality ;
    ns1:description "Protest"^^xsd:string ;
    ns1:isLaunchedBy ns2:Syrian_Arab_Republic ;
    ns2:behaviour ns2:Protest ;
    ns2:hasActor "Syrian Electronic Army"^^xsd:string ;
    ns2:hasActorCountry "Syrian Arab Republic"^^xsd:string ;
    ns2:hasActorType "Hacktivist"^^xsd:string ;
    ns2:hasCountry "Saudi Arabia"^^xsd:string ;
    ns2:hasEventDate "2014-01-16T00:00:00"^^xsd:dateTime ;
    ns2:hasEventSubtype "Message Manipulation"^^xsd:string ;
    ns2:hasEventType "Disruptive"^^xsd:string ;
    ns2:hasIndustry "Public Administration"^^xsd:string ;
    ns2:hasMonth 1 ;
    ns2:hasOrganization "Almajmah Principality"^^xsd:string ;
    ns2:hasYear 2014 ;
    ns2:isType_of ns2:Hacktivist,
        ns2:Message_Manipulation ;
    rdfs:comment "The Syrian Electronic Army deface 16 Saudi Arabian government websites. The targeted sites are the ones of various administrative regions."^^xsd:string .

ns2:c0db6a0f40c603e4 a ns2:AccountAttack,
        owl:NamedIndividual ;
    ns1:associatedCampaigns ns2:Vibram ;
    ns1:description "Financial"^^xsd:string ;
    ns2:behaviour ns2:Financial ;
    ns2:hasActorType "Criminal"^^xsd:string ;
    ns2:hasCountry "Italy"^^xsd:string ;
    ns2:hasEventDate "2014-08-05T00:00:00"^^xsd:dateTime ;
    ns2:hasEventSubtype "Exploitation of Application Server"^^xsd:string ;
    ns2:hasEventType "Exploitive"^^xsd:string ;
    ns2:hasIndustry "Retail Trade"^^xsd:string ;
    ns2:hasMonth 8 ;
    ns2:hasOrganization "Vibram"^^xsd:string ;
    ns2:hasYear 2014 ;
    ns2:isType_of ns2:Criminal,
        ns2:Exploitation_of_Application_Server ;
    rdfs:comment "Vibram notifies some customers of a hack involving its third-party hosting provider. As a consequence, customers making online purchases at vibramfivefingers.com between June 6 and July 7 may have had their credit card numbers compromised."^^xsd:string .

ns2:c2c6fd0f4210203f a ns2:AttackWebsite,
        owl:NamedIndividual ;
    ns1:associatedCampaigns ns2:French_Ministry_of_Defense ;
    ns2:hasActor "AnonGhost"^^xsd:string ;
    ns2:hasActorType "Hacktivist"^^xsd:string ;
    ns2:hasCountry "France"^^xsd:string ;
    ns2:hasEventDate "2015-01-22T00:00:00"^^xsd:dateTime ;
    ns2:hasEventSubtype "Message Manipulation"^^xsd:string ;
    ns2:hasEventType "Disruptive"^^xsd:string ;
    ns2:hasIndustry "Public Administration"^^xsd:string ;
    ns2:hasMonth 1 ;
    ns2:hasOrganization "French Ministry of Defense"^^xsd:string ;
    ns2:hasYear 2015 ;
    ns2:isType_of ns2:Hacktivist,
        ns2:Message_Manipulation ;
    rdfs:comment "The AnonGhost collective defaces several subdomains of the French Interior and Defense Ministries."^^xsd:string .

ns2:c36d9c3c05911a6f a ns2:EmailPhishing,
        owl:NamedIndividual ;
    ns1:associatedCampaigns ns2:Dmitry_Medvedev_Twitter_account ;
    ns2:hasActor "Shaltai Boltai"^^xsd:string ;
    ns2:hasCountry "Russian Federation"^^xsd:string ;
    ns2:hasEventDate "2014-08-14T00:00:00"^^xsd:dateTime ;
    ns2:hasEventSubtype "Message Manipulation,Exploitation of End Hosts"^^xsd:string ;
    ns2:hasEventType "Mixed"^^xsd:string ;
    ns2:hasIndustry "Public Administration"^^xsd:string ;
    ns2:hasMonth 8 ;
    ns2:hasOrganization "Dmitry Medvedev Twitter account"^^xsd:string ;
    ns2:hasYear 2014 ;
    ns2:isType_of ns2:Message_Manipulation_Exploitation_of_End ;
    rdfs:comment "The Twitter account of Russia's Prime Minister Dmitry Medvedev (@MedvedRussia) is hacked, posting a series of fake messages including a resignation announcement."^^xsd:string .

ns2:c37fffe9643c0807 a ns2:MalwareThreat,
        owl:NamedIndividual ;
    ns1:associatedCampaigns ns2:World_of_Warcraft ;
    ns1:description "Financial"^^xsd:string ;
    ns2:behaviour ns2:Financial ;
    ns2:hasActorType "Criminal"^^xsd:string ;
    ns2:hasCampaign ns2:California ;
    ns2:hasCountry "United States of America"^^xsd:string ;
    ns2:hasCounty "Orange"^^xsd:string ;
    ns2:hasEventDate "2014-01-06T00:00:00"^^xsd:dateTime ;
    ns2:hasEventSubtype "Exploitation of End Hosts"^^xsd:string ;
    ns2:hasEventType "Exploitive"^^xsd:string ;
    ns2:hasIndustry "Information"^^xsd:string ;
    ns2:hasMonth 1 ;
    ns2:hasOrganization "World of Warcraft"^^xsd:string ;
    ns2:hasState "California"^^xsd:string ;
    ns2:hasYear 2014 ;
    ns2:isType_of ns2:Criminal,
        ns2:Exploitation_of_End_Hosts ;
    rdfs:comment "World of Warcraft players are hit with a malicious trojan that hijacks accounts. The malware infects systems by posing as an installer of Curse, a legitimate add-on."^^xsd:string .

ns2:c429dc53aa3f2666 a ns2:BreachInformation,
        owl:NamedIndividual ;
    ns1:associatedCampaigns ns2:Victoria_Justice ;
    ns1:description "Personal Attack"^^xsd:string ;
    ns2:behaviour ns2:Personal_Attack ;
    ns2:hasActorType "Criminal"^^xsd:string ;
    ns2:hasCountry "United States of America"^^xsd:string ;
    ns2:hasEventDate "2014-08-31T00:00:00"^^xsd:dateTime ;
    ns2:hasEventSubtype "Exploitation of Application Server"^^xsd:string ;
    ns2:hasEventType "Exploitive"^^xsd:string ;
    ns2:hasIndustry "Other Services (except Public Administration)"^^xsd:string ;
    ns2:hasMonth 8 ;
    ns2:hasOrganization "Victoria Justice"^^xsd:string ;
    ns2:hasYear 2014 ;
    ns2:isType_of ns2:Criminal,
        ns2:Exploitation_of_Application_Server ;
    rdfs:comment "Yet another leak of celebrities pictures. A massive leak of nude and risque photos appearing to be of huge stars like is leaked online, first appearing on 4chan."^^xsd:string .

ns2:c4f6dab8ebb6ec32 a ns2:AttackWebsite,
        owl:NamedIndividual ;
    ns1:associatedCampaigns ns2:maidanhelp_com_ua ;
    ns2:hasActorType "Criminal"^^xsd:string ;
    ns2:hasCountry "Ukraine"^^xsd:string ;
    ns2:hasEventDate "2014-02-28T00:00:00"^^xsd:dateTime ;
    ns2:hasEventSubtype "External Denial of Service"^^xsd:string ;
    ns2:hasEventType "Disruptive"^^xsd:string ;
    ns2:hasIndustry "Other Services (except Public Administration)"^^xsd:string ;
    ns2:hasMonth 2 ;
    ns2:hasOrganization "maidanhelp.com.ua"^^xsd:string ;
    ns2:hasYear 2014 ;
    ns2:isType_of ns2:Criminal,
        ns2:External_Denial_of_Service ;
    rdfs:comment "Hacktivists continue to launch attacks against Ukrainian government websites. The latest targets are the sites of the parliament, or the Verkhovna Rada (rada.gov.ua), the Right Sector nationalist movement (banderivets.org.ua), but also some Euromaidan websites."^^xsd:string .

ns2:c4fedc39baa29d5c a ns2:AccountAttack,
        owl:NamedIndividual ;
    ns1:associatedCampaigns ns2:Sir_Ian_Botham ;
    ns2:hasActorType "Criminal"^^xsd:string ;
    ns2:hasCountry "United Kingdom of Great Britain and Northern Ireland"^^xsd:string ;
    ns2:hasEventDate "2014-08-18T00:00:00"^^xsd:dateTime ;
    ns2:hasEventSubtype "Message Manipulation"^^xsd:string ;
    ns2:hasEventType "Disruptive"^^xsd:string ;
    ns2:hasIndustry "Other Services (except Public Administration)"^^xsd:string ;
    ns2:hasMonth 8 ;
    ns2:hasOrganization "Sir Ian Botham"^^xsd:string ;
    ns2:hasYear 2014 ;
    ns2:isType_of ns2:Criminal,
        ns2:Message_Manipulation ;
    rdfs:comment "Cricket legend Sir Ian Botham claims his Twitter account was hacked after a picture of a penis was posted on his feed."^^xsd:string .

ns2:c51b0477cc49a421 a ns2:BreachSecurity,
        owl:NamedIndividual ;
    ns1:associatedCampaigns ns2:Createthe_Group ;
    ns2:hasActorType "Criminal"^^xsd:string ;
    ns2:hasCampaign ns2:New_York ;
    ns2:hasCountry "United States of America"^^xsd:string ;
    ns2:hasCounty "New York"^^xsd:string ;
    ns2:hasEventDate "2014-03-26T00:00:00"^^xsd:dateTime ;
    ns2:hasEventSubtype "Exploitation of Application Server"^^xsd:string ;
    ns2:hasEventType "Exploitive"^^xsd:string ;
    ns2:hasIndustry "Professional, Scientific, and Technical Services"^^xsd:string ;
    ns2:hasMonth 3 ;
    ns2:hasOrganization "Createthe Group"^^xsd:string ;
    ns2:hasState "New York"^^xsd:string ;
    ns2:hasYear 2014 ;
    ns2:isType_of ns2:Criminal,
        ns2:Exploitation_of_Application_Server ;
    rdfs:comment "Digital luxury agency Createthe Group notifies to be investigating a security breach involving a number of its luxury, fashion and retail clients."^^xsd:string .

ns2:c5aaa8fc99dc5b4c a ns2:HackerSecurity,
        owl:NamedIndividual ;
    ns1:associatedCampaigns ns2:Association_of_Corporate_Travel_Executiv ;
    ns2:hasActorType "Criminal"^^xsd:string ;
    ns2:hasCountry "United States of America"^^xsd:string ;
    ns2:hasEventDate "2014-08-12T00:00:00"^^xsd:dateTime ;
    ns2:hasEventSubtype "Exploitation of Application Server"^^xsd:string ;
    ns2:hasEventType "Exploitive"^^xsd:string ;
    ns2:hasIndustry "Other Services (except Public Administration)"^^xsd:string ;
    ns2:hasMonth 8 ;
    ns2:hasOrganization "Association of Corporate Travel Executives"^^xsd:string ;
    ns2:hasYear 2014 ;
    ns2:isType_of ns2:Criminal,
        ns2:Exploitation_of_Application_Server ;
    rdfs:comment "Unknown hackers steal the data of all members of the Association of Corporate Travel Executives (ACTE)."^^xsd:string .

ns2:c61174dd489cc0a0 a ns2:HackerSecurity,
        owl:NamedIndividual ;
    ns1:associatedCampaigns ns2:Governor_of_Arizona ;
    ns1:isLaunchedBy ns2:United_States_of_America ;
    ns2:hasActor "Swan"^^xsd:string ;
    ns2:hasActorCountry "United States of America"^^xsd:string ;
    ns2:hasActorType "Hacktivist"^^xsd:string ;
    ns2:hasCampaign ns2:Arizona ;
    ns2:hasCountry "United States of America"^^xsd:string ;
    ns2:hasCounty "Maricopa"^^xsd:string ;
    ns2:hasEventDate "2014-06-21T00:00:00"^^xsd:dateTime ;
    ns2:hasEventSubtype "Message Manipulation"^^xsd:string ;
    ns2:hasEventType "Disruptive"^^xsd:string ;
    ns2:hasIndustry "Public Administration"^^xsd:string ;
    ns2:hasMonth 6 ;
    ns2:hasOrganization "Governor of Arizona"^^xsd:string ;
    ns2:hasState "Arizona"^^xsd:string ;
    ns2:hasYear 2014 ;
    ns2:isType_of ns2:Hacktivist,
        ns2:Message_Manipulation ;
    rdfs:comment "After hacking the Arizona Department of Homeland Security, the Turkish hacker Swan is back, and this time he defaces two official websites of Arizona State Governor Janice K. Brewer."^^xsd:string .

ns2:c62dded89628b0bf a ns2:AccountAttack,
        owl:NamedIndividual ;
    ns1:associatedCampaigns ns2:Staysure ;
    ns1:description "Financial"^^xsd:string ;
    ns2:behaviour ns2:Financial ;
    ns2:hasActorType "Criminal"^^xsd:string ;
    ns2:hasCountry "United Kingdom of Great Britain and Northern Ireland"^^xsd:string ;
    ns2:hasEventDate "2014-01-06T00:00:00"^^xsd:dateTime ;
    ns2:hasEventSubtype "Exploitation of Application Server"^^xsd:string ;
    ns2:hasEventType "Exploitive"^^xsd:string ;
    ns2:hasIndustry "Finance and Insurance"^^xsd:string ;
    ns2:hasMonth 1 ;
    ns2:hasOrganization "Staysure"^^xsd:string ;
    ns2:hasYear 2014 ;
    ns2:isType_of ns2:Criminal,
        ns2:Exploitation_of_Application_Server ;
    rdfs:comment "The travel insurance company Staysure confirms that customer names, addresses and card payment details (including CVV) have been stolen from customers who took out insurance prior to May 2012.  The attack was carried out back in October last year, but the company was slow to react to it."^^xsd:string .

ns2:c654e4a02a860727 a ns2:CyberattackInformation,
        owl:NamedIndividual ;
    ns1:associatedCampaigns ns2:Bitstamp ;
    ns2:hasActorType "Criminal"^^xsd:string ;
    ns2:hasCountry "Slovenia"^^xsd:string ;
    ns2:hasEventDate "2014-02-11T00:00:00"^^xsd:dateTime ;
    ns2:hasEventSubtype "External Denial of Service"^^xsd:string ;
    ns2:hasEventType "Disruptive"^^xsd:string ;
    ns2:hasIndustry "Finance and Insurance"^^xsd:string ;
    ns2:hasMonth 2 ;
    ns2:hasOrganization "Bitstamp"^^xsd:string ;
    ns2:hasYear 2014 ;
    ns2:isType_of ns2:Criminal,
        ns2:External_Denial_of_Service ;
    rdfs:comment "Reuters reports that the virtual currency Bitcoin is being hit by attacks from unknown hackers sending \"mutated\" lines of code into the program that runs the virtual currency. Two exchanges, Bitstamp and Mt. Gox, are affected."^^xsd:string .

ns2:c6828297bc9aac86 a ns2:RansomSystem,
        owl:NamedIndividual ;
    ns1:associatedCampaigns ns2:Domino_s_Pizza ;
    ns1:description "Financial"^^xsd:string ;
    ns1:isLaunchedBy ns2:France ;
    ns2:behaviour ns2:Financial ;
    ns2:hasActor "Rex Mundi"^^xsd:string ;
    ns2:hasActorCountry "France"^^xsd:string ;
    ns2:hasActorType "Criminal"^^xsd:string ;
    ns2:hasCountry "Belgium"^^xsd:string ;
    ns2:hasEventDate "2014-06-13T00:00:00"^^xsd:dateTime ;
    ns2:hasEventSubtype "Exploitation of Application Server"^^xsd:string ;
    ns2:hasEventType "Exploitive"^^xsd:string ;
    ns2:hasIndustry "Accommodation and Food Services"^^xsd:string ;
    ns2:hasMonth 6 ;
    ns2:hasOrganization "Domino's Pizza"^^xsd:string ;
    ns2:hasYear 2014 ;
    ns2:isType_of ns2:Criminal,
        ns2:Exploitation_of_Application_Server ;
    rdfs:comment "Rex Mundi claim to have managed to breach the systems of Domino's Pizza in Belgium and France and obtained access to more than 592,000 records belonging to French customers and over 58,000 records belonging to Belgians. They ask for a ransom in exchange."^^xsd:string .

ns2:c6a598af627071a9 a ns2:DDoS,
        owl:NamedIndividual ;
    ns1:associatedCampaigns ns2:UK_Ministry_of_Justice ;
    ns1:description "Protest"^^xsd:string ;
    ns2:behaviour ns2:Protest ;
    ns2:hasActorType "Criminal"^^xsd:string ;
    ns2:hasCountry "United Kingdom of Great Britain and Northern Ireland"^^xsd:string ;
    ns2:hasEventDate "2014-02-13T00:00:00"^^xsd:dateTime ;
    ns2:hasEventSubtype "External Denial of Service"^^xsd:string ;
    ns2:hasEventType "Disruptive"^^xsd:string ;
    ns2:hasIndustry "Public Administration"^^xsd:string ;
    ns2:hasMonth 2 ;
    ns2:hasOrganization "UK Ministry of Justice"^^xsd:string ;
    ns2:hasYear 2014 ;
    ns2:isType_of ns2:Criminal,
        ns2:External_Denial_of_Service ;
    rdfs:comment "The United Kingdom's Ministry of Justice website, justice.gov.uk, is disrupted by a distributed denial-of-service (DDOS) attack. The Ministry of Justice was targeted for not condemning the NSA's surveillance operations."^^xsd:string .

ns2:c8482e2d2216d7a4 a ns2:HackerSecurity,
        owl:NamedIndividual ;
    ns1:associatedCampaigns ns2:Easton_Bell_Sports ;
    ns1:description "Financial"^^xsd:string ;
    ns2:behaviour ns2:Financial ;
    ns2:hasActorType "Criminal"^^xsd:string ;
    ns2:hasCampaign ns2:California ;
    ns2:hasCountry "United States of America"^^xsd:string ;
    ns2:hasCounty "Los Angeles"^^xsd:string ;
    ns2:hasEventDate "2014-01-21T00:00:00"^^xsd:dateTime ;
    ns2:hasEventSubtype "Exploitation of Application Server"^^xsd:string ;
    ns2:hasEventType "Exploitive"^^xsd:string ;
    ns2:hasIndustry "Manufacturing"^^xsd:string ;
    ns2:hasMonth 1 ;
    ns2:hasOrganization "Easton-Bell Sports"^^xsd:string ;
    ns2:hasState "California"^^xsd:string ;
    ns2:hasYear 2014 ;
    ns2:isType_of ns2:Criminal,
        ns2:Exploitation_of_Application_Server ;
    rdfs:comment "Easton-Bell Sports Inc, a California-based maker of sports equipment and clothing, Declares that hackers stole information on about 6,000 customers who shopped on its website in December."^^xsd:string .

ns2:c8d7bf3a0f0a0d86 a ns2:DDoS,
        owl:NamedIndividual ;
    ns1:associatedCampaigns ns2:Point_DNS ;
    ns2:hasActorType "Criminal"^^xsd:string ;
    ns2:hasCountry "United States of America"^^xsd:string ;
    ns2:hasEventDate "2014-05-09T00:00:00"^^xsd:dateTime ;
    ns2:hasEventSubtype "External Denial of Service"^^xsd:string ;
    ns2:hasEventType "Disruptive"^^xsd:string ;
    ns2:hasIndustry "Professional, Scientific, and Technical Services"^^xsd:string ;
    ns2:hasMonth 5 ;
    ns2:hasOrganization "Point DNS"^^xsd:string ;
    ns2:hasYear 2014 ;
    ns2:isType_of ns2:Criminal,
        ns2:External_Denial_of_Service ;
    rdfs:comment "Domain host Point DNS has been hammered with a high intensity DDoS attack on Friday, knocking servers out for hours."^^xsd:string .

ns2:c9280c5eea13aecd a ns2:CyberattackSystem,
        owl:NamedIndividual ;
    ns1:associatedCampaigns ns2:Pakistan_Government_Establishment_Divisi ;
    ns1:isLaunchedBy ns2:Pakistan ;
    ns2:hasActor "Bl@Ck Dr@GoN; Haxor T0du; Spider64"^^xsd:string ;
    ns2:hasActorCountry "Pakistan"^^xsd:string ;
    ns2:hasActorType "Hacktivist"^^xsd:string ;
    ns2:hasCountry "Pakistan"^^xsd:string ;
    ns2:hasEventDate "2014-04-25T00:00:00"^^xsd:dateTime ;
    ns2:hasEventSubtype "Message Manipulation"^^xsd:string ;
    ns2:hasEventType "Disruptive"^^xsd:string ;
    ns2:hasIndustry "Public Administration"^^xsd:string ;
    ns2:hasMonth 4 ;
    ns2:hasOrganization "Pakistan Government Establishment Division"^^xsd:string ;
    ns2:hasYear 2014 ;
    ns2:isType_of ns2:Hacktivist,
        ns2:Message_Manipulation ;
    rdfs:comment "The cyber battle between Indian and Pakistani hacktivists continues. In name of OpPakistan Indian hackers deface several Pakistani government websites."^^xsd:string .

ns2:c957fdb1f218503e a ns2:AccountAttack,
        owl:NamedIndividual ;
    ns1:associatedCampaigns ns2:EA ;
    ns2:hasActorType "Criminal"^^xsd:string ;
    ns2:hasCampaign ns2:California ;
    ns2:hasCountry "United States of America"^^xsd:string ;
    ns2:hasCounty "San Mateo"^^xsd:string ;
    ns2:hasEventDate "2014-03-19T00:00:00"^^xsd:dateTime ;
    ns2:hasEventSubtype "Message Manipulation,Exploitation of Application Server"^^xsd:string ;
    ns2:hasEventType "Mixed"^^xsd:string ;
    ns2:hasIndustry "Information"^^xsd:string ;
    ns2:hasMonth 3 ;
    ns2:hasOrganization "EA"^^xsd:string ;
    ns2:hasState "California"^^xsd:string ;
    ns2:hasYear 2014 ;
    ns2:isType_of ns2:Criminal,
        ns2:Message_Manipulation_Exploitation_of_App ;
    rdfs:comment "One of Electronic Arts' servers is breached, allowing hackers to create a phony Apple log-in screen that prompts users for personal information."^^xsd:string .

ns2:c99b46869dba53a6 a ns2:AccessSecurity,
        owl:NamedIndividual ;
    ns1:associatedCampaigns ns2:Eircom ;
    ns2:hasActorType "Criminal"^^xsd:string ;
    ns2:hasCountry "Ireland"^^xsd:string ;
    ns2:hasEventDate "2014-04-30T00:00:00"^^xsd:dateTime ;
    ns2:hasEventSubtype "Exploitation of Application Server"^^xsd:string ;
    ns2:hasEventType "Exploitive"^^xsd:string ;
    ns2:hasIndustry "Information"^^xsd:string ;
    ns2:hasMonth 4 ;
    ns2:hasOrganization "Eircom"^^xsd:string ;
    ns2:hasYear 2014 ;
    ns2:isType_of ns2:Criminal,
        ns2:Exploitation_of_Application_Server ;
    rdfs:comment "Eircom is forced to shut down its email service after detecting unauthorized access to the system."^^xsd:string .

ns2:c9c538ff6e0d9ec4 a ns2:HackerSecurity,
        owl:NamedIndividual ;
    ns1:associatedCampaigns ns2:Arizona_Department_of_Homeland_Security ;
    ns1:isLaunchedBy ns2:United_States_of_America ;
    ns2:hasActor "Swan"^^xsd:string ;
    ns2:hasActorCountry "United States of America"^^xsd:string ;
    ns2:hasActorType "Hacktivist"^^xsd:string ;
    ns2:hasCampaign ns2:Arizona ;
    ns2:hasCountry "United States of America"^^xsd:string ;
    ns2:hasCounty "Maricopa"^^xsd:string ;
    ns2:hasEventDate "2014-05-26T00:00:00"^^xsd:dateTime ;
    ns2:hasEventSubtype "Message Manipulation"^^xsd:string ;
    ns2:hasEventType "Disruptive"^^xsd:string ;
    ns2:hasIndustry "Public Administration"^^xsd:string ;
    ns2:hasMonth 5 ;
    ns2:hasOrganization "Arizona Department of Homeland Security"^^xsd:string ;
    ns2:hasState "Arizona"^^xsd:string ;
    ns2:hasYear 2014 ;
    ns2:isType_of ns2:Hacktivist,
        ns2:Message_Manipulation ;
    rdfs:comment "A Turkish hacker going with the handle of Swan defaces the official website of theÃÆÃ'Ãâ 'ÃÆÃ¢â¬Â 'ÃÆÃ'ÃÂ¢Ã¢'Â¬ÃÂ ''ÃÆÃ'Ãâ 'ÃÆÃ¢â¬Â ''ÃÆÃ'Ãâ ''ÃÆÃ''ÃÆ'Ã'ÃÂ Arizona Department of Homeland Security. The hacker also defaces the official website of theÃÆÃ'Ãâ 'ÃÆÃ¢â¬Â 'ÃÆÃ'ÃÂ¢Ã¢'Â¬ÃÂ ''ÃÆÃ'Ãâ 'ÃÆÃ¢â¬Â ''ÃÆÃ'Ãâ ''ÃÆÃ''ÃÆ'Ã'ÃÂ Arizona Commission of Indian Affairs website."^^xsd:string .

ns2:ca3cd0e791329f22 a ns2:HackerSecurity,
        owl:NamedIndividual ;
    ns1:associatedCampaigns ns2:Geekface ;
    ns2:hasActorType "Criminal"^^xsd:string ;
    ns2:hasCountry "United States of America"^^xsd:string ;
    ns2:hasEventDate "2014-08-26T00:00:00"^^xsd:dateTime ;
    ns2:hasEventSubtype "Exploitation of Application Server"^^xsd:string ;
    ns2:hasEventType "Exploitive"^^xsd:string ;
    ns2:hasIndustry "Information"^^xsd:string ;
    ns2:hasMonth 8 ;
    ns2:hasOrganization "Geekface"^^xsd:string ;
    ns2:hasYear 2014 ;
    ns2:isType_of ns2:Criminal,
        ns2:Exploitation_of_Application_Server ;
    rdfs:comment "Geekface notifies its users of an illegitimate access to one of its servers. The data accessed include personal information."^^xsd:string .

ns2:cab43d956a13da96 a ns2:CyberattackInformation,
        owl:NamedIndividual ;
    ns1:associatedCampaigns ns2:Microsoft_News ;
    ns1:description "Protest"^^xsd:string ;
    ns1:isLaunchedBy ns2:Syrian_Arab_Republic ;
    ns2:behaviour ns2:Protest ;
    ns2:hasActor "Syrian Electronic Army"^^xsd:string ;
    ns2:hasActorCountry "Syrian Arab Republic"^^xsd:string ;
    ns2:hasActorType "Hacktivist"^^xsd:string ;
    ns2:hasCampaign ns2:Washington ;
    ns2:hasCountry "United States of America"^^xsd:string ;
    ns2:hasCounty "King"^^xsd:string ;
    ns2:hasEventDate "2014-01-13T00:00:00"^^xsd:dateTime ;
    ns2:hasEventSubtype "Message Manipulation"^^xsd:string ;
    ns2:hasEventType "Disruptive"^^xsd:string ;
    ns2:hasIndustry "Information"^^xsd:string ;
    ns2:hasMonth 1 ;
    ns2:hasOrganization "Microsoft News"^^xsd:string ;
    ns2:hasState "Washington"^^xsd:string ;
    ns2:hasYear 2014 ;
    ns2:isType_of ns2:Hacktivist,
        ns2:Message_Manipulation ;
    rdfs:comment "In the same campaign the Syrian Electronic Army hacks the Twitter Xbox Support account, the Xbox Twitter and Instagram, the Microsoft News Twitter account, and Microsoft employees."^^xsd:string .

ns2:cb17a7bb2c3a2289 a ns2:AccessSecurity,
        owl:NamedIndividual ;
    ns1:associatedCampaigns ns2:University_of_Nebraska_Omaha ;
    ns2:hasActorType "Criminal"^^xsd:string ;
    ns2:hasCampaign ns2:Nebraska ;
    ns2:hasCountry "United States of America"^^xsd:string ;
    ns2:hasCounty "Douglas"^^xsd:string ;
    ns2:hasEventDate "2014-05-16T00:00:00"^^xsd:dateTime ;
    ns2:hasEventSubtype "Exploitation of Application Server"^^xsd:string ;
    ns2:hasEventType "Exploitive"^^xsd:string ;
    ns2:hasIndustry "Educational Services"^^xsd:string ;
    ns2:hasMonth 5 ;
    ns2:hasOrganization "University of Nebraska Omaha"^^xsd:string ;
    ns2:hasState "Nebraska"^^xsd:string ;
    ns2:hasYear 2014 ;
    ns2:isType_of ns2:Criminal,
        ns2:Exploitation_of_Application_Server ;
    rdfs:comment "School officials at University of Nebraska Omaha (unomaha.edu) announce to investigate an unauthorized access to an administrative server within campus security."^^xsd:string .

ns2:cb9e113149a1f5a5 a ns2:DDoS,
        owl:NamedIndividual ;
    ns1:associatedCampaigns ns2:US_Federal_Court_System ;
    ns2:hasActorType "Criminal"^^xsd:string ;
    ns2:hasCountry "United States of America"^^xsd:string ;
    ns2:hasEventDate "2014-01-25T00:00:00"^^xsd:dateTime ;
    ns2:hasEventSubtype "External Denial of Service"^^xsd:string ;
    ns2:hasEventType "Disruptive"^^xsd:string ;
    ns2:hasIndustry "Public Administration"^^xsd:string ;
    ns2:hasMonth 1 ;
    ns2:hasOrganization "US Federal Court System"^^xsd:string ;
    ns2:hasYear 2014 ;
    ns2:isType_of ns2:Criminal,
        ns2:External_Denial_of_Service ;
    rdfs:comment "Several websites of the US federal court system, including the ones of the United States Courts (uscourts.gov) and Public Access to Court Electronic Records (pacer.gov), are taken down by a DDOS attack."^^xsd:string .

ns2:cc9e02f56e0c737b a ns2:HackerSecurity,
        owl:NamedIndividual ;
    ns1:associatedCampaigns ns2:The_Wall_Street_Journal ;
    ns1:description "Financial"^^xsd:string ;
    ns1:isLaunchedBy ns2:Russian_Federation ;
    ns2:behaviour ns2:Financial ;
    ns2:hasActor "W0rm"^^xsd:string ;
    ns2:hasActorCountry "Russian Federation"^^xsd:string ;
    ns2:hasActorType "Criminal"^^xsd:string ;
    ns2:hasCampaign ns2:New_York ;
    ns2:hasCountry "United States of America"^^xsd:string ;
    ns2:hasCounty "New York"^^xsd:string ;
    ns2:hasEventDate "2014-07-23T00:00:00"^^xsd:dateTime ;
    ns2:hasEventSubtype "Exploitation of Application Server"^^xsd:string ;
    ns2:hasEventType "Exploitive"^^xsd:string ;
    ns2:hasIndustry "Information"^^xsd:string ;
    ns2:hasMonth 7 ;
    ns2:hasOrganization "The Wall Street Journal"^^xsd:string ;
    ns2:hasState "New York"^^xsd:string ;
    ns2:hasYear 2014 ;
    ns2:isType_of ns2:Criminal,
        ns2:Exploitation_of_Application_Server ;
    rdfs:comment "W0rm hacks the Wall Street Journal and offers data for sale for 1 bitcoin."^^xsd:string .

ns2:ccf12277d0d0f70e a ns2:AttackWebsite,
        owl:NamedIndividual ;
    ns1:associatedCampaigns ns2:City_of_Binghamton__NY ;
    ns1:description "Protest"^^xsd:string ;
    ns1:isLaunchedBy ns2:United_States_of_America ;
    ns2:behaviour ns2:Protest ;
    ns2:hasActor "Essaji"^^xsd:string ;
    ns2:hasActorCountry "United States of America"^^xsd:string ;
    ns2:hasActorType "Hacktivist"^^xsd:string ;
    ns2:hasCampaign ns2:New_York ;
    ns2:hasCountry "United States of America"^^xsd:string ;
    ns2:hasCounty "Broome"^^xsd:string ;
    ns2:hasEventDate "2014-08-28T00:00:00"^^xsd:dateTime ;
    ns2:hasEventSubtype "Message Manipulation"^^xsd:string ;
    ns2:hasEventType "Disruptive"^^xsd:string ;
    ns2:hasIndustry "Public Administration"^^xsd:string ;
    ns2:hasMonth 8 ;
    ns2:hasOrganization "City of Binghamton, NY"^^xsd:string ;
    ns2:hasState "New York"^^xsd:string ;
    ns2:hasYear 2014 ;
    ns2:isType_of ns2:Hacktivist,
        ns2:Message_Manipulation ;
    rdfs:comment "A Pakistani hacker going with the handle of Essaji, defaces the sub-domain of City of Binghamton, New York, in support for Gaza (firstwardboa.binghamton-ny.gov/)."^^xsd:string .

ns2:cd362799eb135152 a ns2:AgencyAttack,
        owl:NamedIndividual ;
    ns1:associatedCampaigns ns2:Alipay ;
    ns1:description "Financial"^^xsd:string ;
    ns2:behaviour ns2:Financial ;
    ns2:hasActorType "Criminal"^^xsd:string ;
    ns2:hasCountry "China"^^xsd:string ;
    ns2:hasEventDate "2014-01-06T00:00:00"^^xsd:dateTime ;
    ns2:hasEventSubtype "Exploitation of Application Server"^^xsd:string ;
    ns2:hasEventType "Exploitive"^^xsd:string ;
    ns2:hasIndustry "Finance and Insurance"^^xsd:string ;
    ns2:hasMonth 1 ;
    ns2:hasOrganization "Alipay"^^xsd:string ;
    ns2:hasYear 2014 ;
    ns2:isType_of ns2:Criminal,
        ns2:Exploitation_of_Application_Server ;
    rdfs:comment "A former employee of Alipay and two accomplices are in custody, suspected of having sold customers' personal information to e-commerce companies starting in 2010. A total of 20 Gb of data were exfiltrated from the Back-End Systems."^^xsd:string .

ns2:cd6eb42011163bae a ns2:CyberattackData,
        owl:NamedIndividual ;
    ns1:associatedCampaigns ns2:International_Council_of_E_Commerce_Cons ;
    ns2:hasActor "Eugene Belford"^^xsd:string ;
    ns2:hasActorType "Hacktivist"^^xsd:string ;
    ns2:hasCampaign ns2:New_Mexico ;
    ns2:hasCountry "United States of America"^^xsd:string ;
    ns2:hasCounty "Bernalillo"^^xsd:string ;
    ns2:hasEventDate "2014-02-23T00:00:00"^^xsd:dateTime ;
    ns2:hasEventSubtype "Message Manipulation"^^xsd:string ;
    ns2:hasEventType "Disruptive"^^xsd:string ;
    ns2:hasIndustry "Educational Services"^^xsd:string ;
    ns2:hasMonth 2 ;
    ns2:hasOrganization "International Council of E-Commerce Consultants"^^xsd:string ;
    ns2:hasState "New Mexico"^^xsd:string ;
    ns2:hasYear 2014 ;
    ns2:isType_of ns2:Hacktivist,
        ns2:Message_Manipulation ;
    rdfs:comment "The website for EC-Council, an International Council of E-Commerce Consultants, is defacedby a hacker calling himself Eugene Belford. He defaces the site with the passport of Edward Snowden."^^xsd:string .

ns2:ce0f0eaf7166dfcb a ns2:DDoS,
        owl:NamedIndividual ;
    ns1:associatedCampaigns ns2:GitHub ;
    ns2:hasActorType "Criminal"^^xsd:string ;
    ns2:hasCampaign ns2:California ;
    ns2:hasCountry "United States of America"^^xsd:string ;
    ns2:hasCounty "San Francisco"^^xsd:string ;
    ns2:hasEventDate "2014-01-27T00:00:00"^^xsd:dateTime ;
    ns2:hasEventSubtype "External Denial of Service"^^xsd:string ;
    ns2:hasEventType "Disruptive"^^xsd:string ;
    ns2:hasIndustry "Information"^^xsd:string ;
    ns2:hasMonth 1 ;
    ns2:hasOrganization "GitHub"^^xsd:string ;
    ns2:hasState "California"^^xsd:string ;
    ns2:hasYear 2014 ;
    ns2:isType_of ns2:Criminal,
        ns2:External_Denial_of_Service ;
    rdfs:comment "GitHub is taken down by a DDoS Attack."^^xsd:string .

ns2:cf9bdc065210e3c3 a ns2:AccountAttack,
        owl:NamedIndividual ;
    ns1:associatedCampaigns ns2:Julie_Bishop ;
    ns1:description "Financial"^^xsd:string ;
    ns2:behaviour ns2:Financial ;
    ns2:hasActorType "Criminal"^^xsd:string ;
    ns2:hasCountry "Australia"^^xsd:string ;
    ns2:hasEventDate "2014-03-18T00:00:00"^^xsd:dateTime ;
    ns2:hasEventSubtype "Message Manipulation"^^xsd:string ;
    ns2:hasEventType "Disruptive"^^xsd:string ;
    ns2:hasIndustry "Public Administration"^^xsd:string ;
    ns2:hasMonth 3 ;
    ns2:hasOrganization "Julie Bishop"^^xsd:string ;
    ns2:hasYear 2014 ;
    ns2:isType_of ns2:Criminal,
        ns2:Message_Manipulation ;
    rdfs:comment "The verified Twitter account of Julie Bishop, the Australian minister for foreign affairs, has been hacked. The attacker posted some tweets in an effort to lure Bishop's followers to a phishing site."^^xsd:string .

ns2:cfef06ecdbe14973 a ns2:AccountAttack,
        owl:NamedIndividual ;
    ns1:associatedCampaigns ns2:JSTOR ;
    ns2:hasActorType "Criminal"^^xsd:string ;
    ns2:hasCampaign ns2:New_York ;
    ns2:hasCountry "United States of America"^^xsd:string ;
    ns2:hasCounty "New York"^^xsd:string ;
    ns2:hasEventDate "2014-04-02T00:00:00"^^xsd:dateTime ;
    ns2:hasEventSubtype "Exploitation of Application Server"^^xsd:string ;
    ns2:hasEventType "Exploitive"^^xsd:string ;
    ns2:hasIndustry "Information"^^xsd:string ;
    ns2:hasMonth 4 ;
    ns2:hasOrganization "JSTOR"^^xsd:string ;
    ns2:hasState "New York"^^xsd:string ;
    ns2:hasYear 2014 ;
    ns2:isType_of ns2:Criminal,
        ns2:Exploitation_of_Application_Server ;
    rdfs:comment "Digital library JSTOR notifies approximately 800 users that their personal information may be at risk after their MyJSTOR accounts were accessed by an unauthorized third party."^^xsd:string .

ns2:d0a6603ecb21da6f a ns2:AnonymousAttack,
        owl:NamedIndividual ;
    ns1:associatedCampaigns ns2:Bank_of_Israel ;
    ns1:description "Protest"^^xsd:string ;
    ns2:behaviour ns2:Protest ;
    ns2:hasActor "Anonymous"^^xsd:string ;
    ns2:hasActorType "Hacktivist"^^xsd:string ;
    ns2:hasCountry "Israel"^^xsd:string ;
    ns2:hasEventDate "2014-08-25T00:00:00"^^xsd:dateTime ;
    ns2:hasEventSubtype "External Denial of Service"^^xsd:string ;
    ns2:hasEventType "Disruptive"^^xsd:string ;
    ns2:hasIndustry "Finance and Insurance"^^xsd:string ;
    ns2:hasMonth 8 ;
    ns2:hasOrganization "Bank of Israel"^^xsd:string ;
    ns2:hasYear 2014 ;
    ns2:isType_of ns2:External_Denial_of_Service,
        ns2:Hacktivist ;
    rdfs:comment "In name of #OpSaveGaza, the Anonymous collective claims to have taken down some key Israeli governmental websites, including those of the Israeli Defense Forces, the Bank of Israel, the Israeli Prime Minister."^^xsd:string .

ns2:d104b295d54b17a9 a ns2:CyberattackData,
        owl:NamedIndividual ;
    ns1:associatedCampaigns ns2:zerem_co_il ;
    ns1:description "Protest"^^xsd:string ;
    ns1:isLaunchedBy ns2:Iran__Islamic_Republic_of ;
    ns2:behaviour ns2:Protest ;
    ns2:hasActor "Islamic Cyber Resistance"^^xsd:string ;
    ns2:hasActorCountry "Iran (Islamic Republic of)"^^xsd:string ;
    ns2:hasActorType "Hacktivist"^^xsd:string ;
    ns2:hasCountry "Israel"^^xsd:string ;
    ns2:hasEventDate "2014-08-06T00:00:00"^^xsd:dateTime ;
    ns2:hasEventSubtype "Exploitation of Application Server"^^xsd:string ;
    ns2:hasEventType "Exploitive"^^xsd:string ;
    ns2:hasIndustry "Administrative and Support and Waste Management and Remediation Services"^^xsd:string ;
    ns2:hasMonth 8 ;
    ns2:hasOrganization "zerem.co.il"^^xsd:string ;
    ns2:hasYear 2014 ;
    ns2:isType_of ns2:Exploitation_of_Application_Server,
        ns2:Hacktivist ;
    rdfs:comment "A group of Iranian hackers going with the handle of Islamic Cyber Resistance (ICRG), claim to have breached an Israeli job website (zerem.co.il), leaking the personal details of 70,000 registered users. The attack is executed in name of #OpSaveGaza."^^xsd:string .

ns2:d118e152e28e352c a ns2:DefaceHacker,
        owl:NamedIndividual ;
    ns1:associatedCampaigns ns2:Ubuntu ;
    ns2:hasActor "Sultan Haikal; Gantengers Crew"^^xsd:string ;
    ns2:hasActorType "Hacktivist"^^xsd:string ;
    ns2:hasCountry "United Kingdom of Great Britain and Northern Ireland"^^xsd:string ;
    ns2:hasEventDate "2014-01-21T00:00:00"^^xsd:dateTime ;
    ns2:hasEventSubtype "Message Manipulation"^^xsd:string ;
    ns2:hasEventType "Disruptive"^^xsd:string ;
    ns2:hasIndustry "Information"^^xsd:string ;
    ns2:hasMonth 1 ;
    ns2:hasOrganization "Ubuntu"^^xsd:string ;
    ns2:hasYear 2014 ;
    ns2:isType_of ns2:Hacktivist,
        ns2:Message_Manipulation ;
    rdfs:comment "SultanHaikal from Gantengers Crew defaces 6 official domains of Ubuntu One."^^xsd:string .

ns2:d12cbaf0d238a273 a ns2:AccountAttack,
        owl:NamedIndividual ;
    ns1:associatedCampaigns ns2:Church_of_Scotland ;
    ns2:hasActor "@security_511"^^xsd:string ;
    ns2:hasActorType "Hobbyist"^^xsd:string ;
    ns2:hasCountry "United Kingdom of Great Britain and Northern Ireland"^^xsd:string ;
    ns2:hasEventDate "2014-02-21T00:00:00"^^xsd:dateTime ;
    ns2:hasEventSubtype "Exploitation of Application Server"^^xsd:string ;
    ns2:hasEventType "Exploitive"^^xsd:string ;
    ns2:hasIndustry "Other Services (except Public Administration)"^^xsd:string ;
    ns2:hasMonth 2 ;
    ns2:hasOrganization "Church of Scotland"^^xsd:string ;
    ns2:hasYear 2014 ;
    ns2:isType_of ns2:Exploitation_of_Application_Server,
        ns2:Hobbyist ;
    rdfs:comment "Yet another attack by @security_511. This time the victim is the Church of Scotland (churchofscotland.org.uk) and the dumps contains 1,570 user credentials."^^xsd:string .

ns2:d13fc3247f4cdf73 a ns2:BreachSecurity,
        owl:NamedIndividual ;
    ns1:associatedCampaigns ns2:Directors_Guild_of_Canada ;
    ns2:hasActor "ObeySec"^^xsd:string ;
    ns2:hasCountry "Canada"^^xsd:string ;
    ns2:hasEventDate "2014-01-07T00:00:00"^^xsd:dateTime ;
    ns2:hasEventSubtype "Exploitation of Application Server"^^xsd:string ;
    ns2:hasEventType "Exploitive"^^xsd:string ;
    ns2:hasIndustry "Other Services (except Public Administration)"^^xsd:string ;
    ns2:hasMonth 1 ;
    ns2:hasOrganization "Directors Guild of Canada"^^xsd:string ;
    ns2:hasYear 2014 ;
    ns2:isType_of ns2:Exploitation_of_Application_Server ;
    rdfs:comment "A hacker using the handle legionnare  aka ObeySec has hacked the directors guild of Canada (dgc.ca) and leaks 2000+ usernames, email addresses and clear text passwords."^^xsd:string .

ns2:d14123039c06d0e5 a ns2:AttackWebsite,
        owl:NamedIndividual ;
    ns1:associatedCampaigns ns2:Alghat_Principality ;
    ns1:description "Protest"^^xsd:string ;
    ns1:isLaunchedBy ns2:Syrian_Arab_Republic ;
    ns2:behaviour ns2:Protest ;
    ns2:hasActor "Syrian Electronic Army"^^xsd:string ;
    ns2:hasActorCountry "Syrian Arab Republic"^^xsd:string ;
    ns2:hasActorType "Hacktivist"^^xsd:string ;
    ns2:hasCountry "Saudi Arabia"^^xsd:string ;
    ns2:hasEventDate "2014-01-16T00:00:00"^^xsd:dateTime ;
    ns2:hasEventSubtype "Message Manipulation"^^xsd:string ;
    ns2:hasEventType "Disruptive"^^xsd:string ;
    ns2:hasIndustry "Public Administration"^^xsd:string ;
    ns2:hasMonth 1 ;
    ns2:hasOrganization "Alghat Principality"^^xsd:string ;
    ns2:hasYear 2014 ;
    ns2:isType_of ns2:Hacktivist,
        ns2:Message_Manipulation ;
    rdfs:comment "The Syrian Electronic Army deface 16 Saudi Arabian government websites. The targeted sites are the ones of various administrative regions."^^xsd:string .

ns2:d22c983540651bce a ns2:BreachInformation,
        owl:NamedIndividual ;
    ns1:associatedCampaigns ns2:Twitter ;
    ns2:hasActorType "Criminal"^^xsd:string ;
    ns2:hasCampaign ns2:California ;
    ns2:hasCountry "United States of America"^^xsd:string ;
    ns2:hasCounty "San Francisco"^^xsd:string ;
    ns2:hasEventDate "2014-06-10T00:00:00"^^xsd:dateTime ;
    ns2:hasEventSubtype "Exploitation of End Hosts"^^xsd:string ;
    ns2:hasEventType "Exploitive"^^xsd:string ;
    ns2:hasIndustry "Information"^^xsd:string ;
    ns2:hasMonth 6 ;
    ns2:hasOrganization "Twitter"^^xsd:string ;
    ns2:hasState "California"^^xsd:string ;
    ns2:hasYear 2014 ;
    ns2:isType_of ns2:Criminal,
        ns2:Exploitation_of_End_Hosts ;
    rdfs:comment "The names, addresses, and Social Security numbers of a handful of staff at TwitterÃÆÃ'Ãâ 'ÃÆÃ¢â¬Â 'ÃÆÃ'ÃÂ¢Ã¢'Â¬ÃÂ ''ÃÆÃ'Ãâ 'ÃÆÃ¢â¬Â ''ÃÆÃ'Ãâ ''ÃÆÃ''ÃÆ'Ã'ÃÂ (including the CEO) are leaked on the dark wen."^^xsd:string .

ns2:d26c9076706c78bc a ns2:AttackWebsite,
        owl:NamedIndividual ;
    ns1:associatedCampaigns ns2:Ministry_of_Agriculture_and_Rural_Develo ;
    ns1:description "Protest"^^xsd:string ;
    ns2:behaviour ns2:Protest ;
    ns2:hasActor "AnonGhost"^^xsd:string ;
    ns2:hasActorType "Hacktivist"^^xsd:string ;
    ns2:hasCountry "Israel"^^xsd:string ;
    ns2:hasEventDate "2014-03-30T00:00:00"^^xsd:dateTime ;
    ns2:hasEventSubtype "Message Manipulation"^^xsd:string ;
    ns2:hasEventType "Disruptive"^^xsd:string ;
    ns2:hasIndustry "Public Administration"^^xsd:string ;
    ns2:hasMonth 3 ;
    ns2:hasOrganization "Ministry of Agriculture and Rural Development"^^xsd:string ;
    ns2:hasYear 2014 ;
    ns2:isType_of ns2:Hacktivist,
        ns2:Message_Manipulation ;
    rdfs:comment "The pro-Palestinian hacktivist AnonGhost hacks and defaces the official website of Israeli Agricultural Research Organization, which is ran by Israeli Ministry of Agriculture and Rural Development."^^xsd:string .

ns2:d2a4094c00a7ef20 a ns2:AttackMalware,
        owl:NamedIndividual ;
    ns1:associatedCampaigns ns2:Ministry_of_Natural_Resource_and_Environ ;
    ns2:hasActorType "Criminal"^^xsd:string ;
    ns2:hasCountry "Viet Nam"^^xsd:string ;
    ns2:hasEventDate "2014-06-20T00:00:00"^^xsd:dateTime ;
    ns2:hasEventSubtype "Exploitation of End Hosts"^^xsd:string ;
    ns2:hasEventType "Exploitive"^^xsd:string ;
    ns2:hasIndustry "Public Administration"^^xsd:string ;
    ns2:hasMonth 6 ;
    ns2:hasOrganization "Ministry of Natural Resource and Environment"^^xsd:string ;
    ns2:hasYear 2014 ;
    ns2:isType_of ns2:Criminal,
        ns2:Exploitation_of_End_Hosts ;
    rdfs:comment "The Vietnamese Ministry of Natural Resources and Environment (MONRE) is the victim of a targeted attack carried on through a specifically crafted malware distributed via a spear phishing campaign."^^xsd:string .

ns2:d2dc2751775a2d31 a ns2:CyberattackData,
        owl:NamedIndividual ;
    ns1:associatedCampaigns ns2:Azad_Kashmir_Government_Portal ;
    ns1:description "Protest"^^xsd:string ;
    ns1:isLaunchedBy ns2:Pakistan ;
    ns2:behaviour ns2:Protest ;
    ns2:hasActor "Pak Cyber Eaglez"^^xsd:string ;
    ns2:hasActorCountry "Pakistan"^^xsd:string ;
    ns2:hasActorType "Hacktivist"^^xsd:string ;
    ns2:hasCountry "Pakistan"^^xsd:string ;
    ns2:hasEventDate "2014-09-05T00:00:00"^^xsd:dateTime ;
    ns2:hasEventSubtype "Message Manipulation,Exploitation of Application Server"^^xsd:string ;
    ns2:hasEventType "Mixed"^^xsd:string ;
    ns2:hasIndustry "Public Administration"^^xsd:string ;
    ns2:hasMonth 9 ;
    ns2:hasOrganization "Azad Kashmir Government Portal"^^xsd:string ;
    ns2:hasYear 2014 ;
    ns2:isType_of ns2:Hacktivist,
        ns2:Message_Manipulation_Exploitation_of_App ;
    rdfs:comment "The Pak Cyber Eaglez collective breaks into the online portal of the Azad Kashmir government (ajk.gov.pk), defaces some of the pages, and extracts the database with the login credentials."^^xsd:string .

ns2:d2f619a94e830f7a a ns2:AnonymousAttack,
        owl:NamedIndividual ;
    ns1:associatedCampaigns ns2:Presidential_Adviser ;
    ns1:description "Protest"^^xsd:string ;
    ns1:isLaunchedBy ns2:Ukraine ;
    ns2:behaviour ns2:Protest ;
    ns2:hasActor "Anonymous (Ukraine)"^^xsd:string ;
    ns2:hasActorCountry "Ukraine"^^xsd:string ;
    ns2:hasActorType "Hacktivist"^^xsd:string ;
    ns2:hasCountry "Lithuania"^^xsd:string ;
    ns2:hasEventDate "2014-02-13T00:00:00"^^xsd:dateTime ;
    ns2:hasEventSubtype "Exploitation of End Hosts"^^xsd:string ;
    ns2:hasEventType "Exploitive"^^xsd:string ;
    ns2:hasIndustry "Public Administration"^^xsd:string ;
    ns2:hasMonth 2 ;
    ns2:hasOrganization "Presidential Adviser"^^xsd:string ;
    ns2:hasYear 2014 ;
    ns2:isType_of ns2:Exploitation_of_End_Hosts,
        ns2:Hacktivist ;
    rdfs:comment "Again an action in name of Opindependence. This time Anonymous Ukraine hacks the e-mail account of Laurynas Jonavicius (adviser of the President of Lithuania), leaking some emails."^^xsd:string .

ns2:d3191453f656d736 a ns2:CyberattackData,
        owl:NamedIndividual ;
    ns1:associatedCampaigns ns2:Various_Government_Websites ;
    ns1:isLaunchedBy ns2:Syrian_Arab_Republic ;
    ns2:hasActor "Anonymous (Syria)"^^xsd:string ;
    ns2:hasActorCountry "Syrian Arab Republic"^^xsd:string ;
    ns2:hasActorType "Hacktivist"^^xsd:string ;
    ns2:hasCountry "Nigeria"^^xsd:string ;
    ns2:hasEventDate "2014-02-11T00:00:00"^^xsd:dateTime ;
    ns2:hasEventSubtype "Message Manipulation"^^xsd:string ;
    ns2:hasEventType "Disruptive"^^xsd:string ;
    ns2:hasIndustry "Public Administration"^^xsd:string ;
    ns2:hasMonth 2 ;
    ns2:hasOrganization "Various Government Websites"^^xsd:string ;
    ns2:hasYear 2014 ;
    ns2:isType_of ns2:Hacktivist,
        ns2:Message_Manipulation ;
    rdfs:comment "Hackers belonging to a group called Syrian Anonymous deface a total of 25 Nigerian government websites.The list of hacked websites includes the Ministry of Justice, the Ministry of Finance, the Ministry of Education, the Ministry of Power, and many others."^^xsd:string .

ns2:d37641a72e78562d a ns2:AnonymousAttack,
        owl:NamedIndividual ;
    ns1:associatedCampaigns ns2:Regional_Electoral_Court_of_the_Amazon ;
    ns1:description "Protest"^^xsd:string ;
    ns2:behaviour ns2:Protest ;
    ns2:hasActor "Anonymous"^^xsd:string ;
    ns2:hasActorType "Hacktivist"^^xsd:string ;
    ns2:hasCountry "Brazil"^^xsd:string ;
    ns2:hasEventDate "2014-06-17T00:00:00"^^xsd:dateTime ;
    ns2:hasEventSubtype "Exploitation of Application Server"^^xsd:string ;
    ns2:hasEventType "Exploitive"^^xsd:string ;
    ns2:hasIndustry "Public Administration"^^xsd:string ;
    ns2:hasMonth 6 ;
    ns2:hasOrganization "Regional Electoral Court of the Amazon"^^xsd:string ;
    ns2:hasYear 2014 ;
    ns2:isType_of ns2:Exploitation_of_Application_Server,
        ns2:Hacktivist ;
    rdfs:comment "As part of #OpWorldCup and #OpHackingCup, Anonymous hacks a number of Brazilian organizations during the World Cup. "^^xsd:string .

ns2:d4c120063cf54f2d a ns2:AnonymousAttack,
        owl:NamedIndividual ;
    ns1:associatedCampaigns ns2:Ukranian_Democratic_Alliance_for_Reform ;
    ns1:isLaunchedBy ns2:Ukraine ;
    ns2:hasActor "Anonymous (Ukraine)"^^xsd:string ;
    ns2:hasActorCountry "Ukraine"^^xsd:string ;
    ns2:hasActorType "Hacktivist"^^xsd:string ;
    ns2:hasCountry "Ukraine"^^xsd:string ;
    ns2:hasEventDate "2014-02-13T00:00:00"^^xsd:dateTime ;
    ns2:hasEventSubtype "Exploitation of Application Server"^^xsd:string ;
    ns2:hasEventType "Exploitive"^^xsd:string ;
    ns2:hasIndustry "Other Services (except Public Administration)"^^xsd:string ;
    ns2:hasMonth 2 ;
    ns2:hasOrganization "Ukranian Democratic Alliance for Reform"^^xsd:string ;
    ns2:hasYear 2014 ;
    ns2:isType_of ns2:Exploitation_of_Application_Server,
        ns2:Hacktivist ;
    rdfs:comment "In name of OpIndepenence, the collective Anonymous Ukraine hacks Vitali Klitschko's UDAR (Ukrainian Democratic Alliance for Reform) party and leaks some confidential emails."^^xsd:string .

ns2:d56625d63ccc4422 a ns2:AttackWebsite,
        owl:NamedIndividual ;
    ns1:associatedCampaigns ns2:qha_com_ua ;
    ns2:hasActorType "Criminal"^^xsd:string ;
    ns2:hasCountry "Ukraine"^^xsd:string ;
    ns2:hasEventDate "2014-02-28T00:00:00"^^xsd:dateTime ;
    ns2:hasEventSubtype "External Denial of Service"^^xsd:string ;
    ns2:hasEventType "Disruptive"^^xsd:string ;
    ns2:hasIndustry "Other Services (except Public Administration)"^^xsd:string ;
    ns2:hasMonth 2 ;
    ns2:hasOrganization "qha.com.ua"^^xsd:string ;
    ns2:hasYear 2014 ;
    ns2:isType_of ns2:Criminal,
        ns2:External_Denial_of_Service ;
    rdfs:comment "Hacktivists continue to launch attacks against Ukrainian government websites. The latest targets are the sites of the parliament, or the Verkhovna Rada (rada.gov.ua), the Right Sector nationalist movement (banderivets.org.ua), but also some Euromaidan websites."^^xsd:string .

ns2:d59b542d7d6b6ad2 a ns2:BreachSecurity,
        owl:NamedIndividual ;
    ns1:associatedCampaigns ns2:Canada_Revenue_Agency ;
    ns1:description "Financial"^^xsd:string ;
    ns2:behaviour ns2:Financial ;
    ns2:hasActorType "Criminal"^^xsd:string ;
    ns2:hasCountry "Canada"^^xsd:string ;
    ns2:hasEventDate "2014-04-14T00:00:00"^^xsd:dateTime ;
    ns2:hasEventSubtype "Exploitation of Application Server"^^xsd:string ;
    ns2:hasEventType "Exploitive"^^xsd:string ;
    ns2:hasIndustry "Public Administration"^^xsd:string ;
    ns2:hasMonth 4 ;
    ns2:hasOrganization "Canada Revenue Agency"^^xsd:string ;
    ns2:hasYear 2014 ;
    ns2:isType_of ns2:Criminal,
        ns2:Exploitation_of_Application_Server ;
    rdfs:comment "Unknown hackers exploit the Heartbleed vulnerability to steal taxpayer data for at least 900 Canadian citizens, and an unknown number of businesses and officials from the Canadian Revenue Agency (CRA)."^^xsd:string .

ns2:d6006b80c46a43db a ns2:AttackPhishing,
        owl:NamedIndividual ;
    ns1:associatedCampaigns ns2:Israeli_Defense_Contractors ;
    ns1:description "Political-Espionage"^^xsd:string ;
    ns1:isLaunchedBy ns2:China ;
    ns2:behaviour ns2:Political_Espionage ;
    ns2:hasActor "People's Liberation Army Strategic Support Force (PLA Unit 61398)"^^xsd:string ;
    ns2:hasActorCountry "China"^^xsd:string ;
    ns2:hasActorType "Nation-State"^^xsd:string ;
    ns2:hasCountry "Israel"^^xsd:string ;
    ns2:hasEventDate "2014-07-14T00:00:00"^^xsd:dateTime ;
    ns2:hasEventSubtype "Exploitation of Application Server"^^xsd:string ;
    ns2:hasEventType "Exploitive"^^xsd:string ;
    ns2:hasIndustry "Public Administration"^^xsd:string ;
    ns2:hasMonth 7 ;
    ns2:hasOrganization "Israeli Defense Contractors"^^xsd:string ;
    ns2:hasYear 2014 ;
    ns2:isType_of ns2:Exploitation_of_Application_Server,
        ns2:Nation_State ;
    rdfs:comment "Brian Krebs reveals that three Israeli defense contractors responsible for building the Iron DomeÃÆÃ'Ãâ 'ÃÆÃ¢â¬Â 'ÃÆÃ'ÃÂ¢Ã¢'Â¬ÃÂ ''ÃÆÃ'Ãâ 'ÃÆÃ¢â¬Â ''ÃÆÃ'Ãâ ''ÃÆÃ''ÃÆ'Ã'ÃÂ missile shield were compromised by a well-crafted phishing attack and robbed of huge quantities of sensitive documents pertaining to the shield technology."^^xsd:string .

ns2:d65333c0fd8e5564 a ns2:BreachInformation,
        owl:NamedIndividual ;
    ns1:associatedCampaigns ns2:Monsanto ;
    ns2:hasActorType "Criminal"^^xsd:string ;
    ns2:hasCampaign ns2:Missouri ;
    ns2:hasCountry "United States of America"^^xsd:string ;
    ns2:hasCounty "St. Louis"^^xsd:string ;
    ns2:hasEventDate "2014-06-02T00:00:00"^^xsd:dateTime ;
    ns2:hasEventSubtype "Exploitation of Application Server"^^xsd:string ;
    ns2:hasEventType "Exploitive"^^xsd:string ;
    ns2:hasIndustry "Agriculture, Forestry, Fishing and Hunting"^^xsd:string ;
    ns2:hasMonth 6 ;
    ns2:hasOrganization "Monsanto"^^xsd:string ;
    ns2:hasState "Missouri"^^xsd:string ;
    ns2:hasYear 2014 ;
    ns2:isType_of ns2:Criminal,
        ns2:Exploitation_of_Application_Server ;
    rdfs:comment "Monsanto admits that credit card data along with names, addresses and US taxation information for 1300 customers and employees was compromised after hackers broke into its servers in March."^^xsd:string .

ns2:d7aef044f381fb27 a ns2:Malware,
        owl:NamedIndividual ;
    ns1:associatedCampaigns ns2:Edgepark_Medical_Supplies ;
    ns1:description "Financial"^^xsd:string ;
    ns2:behaviour ns2:Financial ;
    ns2:hasActorType "Criminal"^^xsd:string ;
    ns2:hasCampaign ns2:Ohio ;
    ns2:hasCountry "United States of America"^^xsd:string ;
    ns2:hasCounty "Summit"^^xsd:string ;
    ns2:hasEventDate "2014-01-16T00:00:00"^^xsd:dateTime ;
    ns2:hasEventSubtype "Exploitation of Application Server"^^xsd:string ;
    ns2:hasEventType "Exploitive"^^xsd:string ;
    ns2:hasIndustry "Manufacturing"^^xsd:string ;
    ns2:hasMonth 1 ;
    ns2:hasOrganization "Edgepark Medical Supplies"^^xsd:string ;
    ns2:hasState "Ohio"^^xsd:string ;
    ns2:hasYear 2014 ;
    ns2:isType_of ns2:Criminal,
        ns2:Exploitation_of_Application_Server ;
    rdfs:comment "The information, including payment card data, of more than 4,200 individuals is inappropriately accessed after malware is introduced into the computer systems of Edgepark Medical Supplies."^^xsd:string .

ns2:d861834f7fe628e6 a ns2:CyberattackData,
        owl:NamedIndividual ;
    ns1:associatedCampaigns ns2:AlfaNet ;
    ns1:description "Financial"^^xsd:string ;
    ns1:isLaunchedBy ns2:France ;
    ns2:behaviour ns2:Financial ;
    ns2:hasActor "Rex Mundi"^^xsd:string ;
    ns2:hasActorCountry "France"^^xsd:string ;
    ns2:hasActorType "Criminal"^^xsd:string ;
    ns2:hasCountry "Belgium"^^xsd:string ;
    ns2:hasEventDate "2014-04-25T00:00:00"^^xsd:dateTime ;
    ns2:hasEventSubtype "Exploitation of Application Server"^^xsd:string ;
    ns2:hasEventType "Exploitive"^^xsd:string ;
    ns2:hasIndustry "Information"^^xsd:string ;
    ns2:hasMonth 4 ;
    ns2:hasOrganization "AlfaNet"^^xsd:string ;
    ns2:hasYear 2014 ;
    ns2:isType_of ns2:Criminal,
        ns2:Exploitation_of_Application_Server ;
    rdfs:comment "The infamous hacker collective Rex Mundi hacks alfanet.be and blackmails the company, threatening to release all their customer data if they do not pay 15,000 euros."^^xsd:string .

ns2:d8788a0c6236ce7f a ns2:Malware,
        owl:NamedIndividual ;
    ns1:associatedCampaigns ns2:Rosenthal_Wine_Shop ;
    ns1:description "Financial"^^xsd:string ;
    ns2:behaviour ns2:Financial ;
    ns2:hasActorType "Criminal"^^xsd:string ;
    ns2:hasCampaign ns2:New_York ;
    ns2:hasCountry "United States of America"^^xsd:string ;
    ns2:hasCounty "New York"^^xsd:string ;
    ns2:hasEventDate "2014-03-21T00:00:00"^^xsd:dateTime ;
    ns2:hasEventSubtype "Exploitation of Sensors"^^xsd:string ;
    ns2:hasEventType "Exploitive"^^xsd:string ;
    ns2:hasIndustry "Retail Trade"^^xsd:string ;
    ns2:hasMonth 3 ;
    ns2:hasOrganization "Rosenthal Wine Shop"^^xsd:string ;
    ns2:hasState "New York"^^xsd:string ;
    ns2:hasYear 2014 ;
    ns2:isType_of ns2:Criminal,
        ns2:Exploitation_of_Sensors ;
    rdfs:comment "Rosenthal Wine Shop notifies customers that malware may have compromised their payment card information."^^xsd:string .

ns2:d8bf66f42f0e5408 a ns2:CyberattackData,
        owl:NamedIndividual ;
    ns1:associatedCampaigns ns2:United_Nations_Economic_and_Social_Commi ;
    ns1:description "Protest"^^xsd:string ;
    ns1:isLaunchedBy ns2:Turkey ;
    ns2:behaviour ns2:Protest ;
    ns2:hasActor "Turk Guvengligi"^^xsd:string ;
    ns2:hasActorCountry "Turkey"^^xsd:string ;
    ns2:hasActorType "Hacktivist"^^xsd:string ;
    ns2:hasCountry "Lebanon"^^xsd:string ;
    ns2:hasEventDate "2014-07-23T00:00:00"^^xsd:dateTime ;
    ns2:hasEventSubtype "Message Manipulation"^^xsd:string ;
    ns2:hasEventType "Disruptive"^^xsd:string ;
    ns2:hasIndustry "Public Administration"^^xsd:string ;
    ns2:hasMonth 7 ;
    ns2:hasOrganization "United Nations Economic and Social Commission for Western Asia"^^xsd:string ;
    ns2:hasYear 2014 ;
    ns2:isType_of ns2:Hacktivist,
        ns2:Message_Manipulation ;
    rdfs:comment "Again an attack in name of #OpSaveGaza. A Turkish hacker going with the handle of Turk Guvenligi defaces two official sub-domains of the United Nations: esango.un.org and escwa.un.org."^^xsd:string .

ns2:d92febef87134973 a ns2:AgencyAttack,
        owl:NamedIndividual ;
    ns1:associatedCampaigns ns2:US_Embassy_in_Turkey ;
    ns1:description "Protest"^^xsd:string ;
    ns1:isLaunchedBy ns2:Turkey ;
    ns2:behaviour ns2:Protest ;
    ns2:hasActor "RedHack"^^xsd:string ;
    ns2:hasActorCountry "Turkey"^^xsd:string ;
    ns2:hasActorType "Hacktivist"^^xsd:string ;
    ns2:hasCountry "United States of America"^^xsd:string ;
    ns2:hasEventDate "2014-02-12T00:00:00"^^xsd:dateTime ;
    ns2:hasEventSubtype "Exploitation of Application Server"^^xsd:string ;
    ns2:hasEventType "Exploitive"^^xsd:string ;
    ns2:hasIndustry "Public Administration"^^xsd:string ;
    ns2:hasMonth 2 ;
    ns2:hasOrganization "US Embassy in Turkey"^^xsd:string ;
    ns2:hasYear 2014 ;
    ns2:isType_of ns2:Exploitation_of_Application_Server,
        ns2:Hacktivist ;
    rdfs:comment "Hackers of the RedHack collective leak the contact information for 36 staff members of the US Embassy in Turkey. The hacktivists publish a list of names, email addresses, job titles and phone numbers."^^xsd:string .

ns2:d9c35a1a5e460877 a ns2:AttackGroup,
        owl:NamedIndividual ;
    ns1:associatedCampaigns ns2:Corsica_Ferries ;
    ns1:description "Financial"^^xsd:string ;
    ns1:isLaunchedBy ns2:Russian_Federation ;
    ns2:behaviour ns2:Financial ;
    ns2:hasActor "ALPHVM"^^xsd:string ;
    ns2:hasActorCountry "Russian Federation"^^xsd:string ;
    ns2:hasActorType "Criminal"^^xsd:string ;
    ns2:hasCountry "France"^^xsd:string ;
    ns2:hasEventDate "2023-11-07T00:00:00"^^xsd:dateTime ;
    ns2:hasEventSubtype "Exploitation of Application Server"^^xsd:string ;
    ns2:hasEventType "Mixed"^^xsd:string ;
    ns2:hasIndustry "Transportation and Warehousing"^^xsd:string ;
    ns2:hasMonth 11 ;
    ns2:hasOrganization "Corsica Ferries"^^xsd:string ;
    ns2:hasYear 2023 ;
    ns2:isType_of ns2:Criminal,
        ns2:Exploitation_of_Application_Server ;
    rdfs:comment "The ALPHV/BlackCat ransomware group claims responsibility for a cyber attack to Corsica Ferries."^^xsd:string .

ns2:da4e8c0884a40d39 a ns2:AnonymousAttack,
        owl:NamedIndividual ;
    ns1:associatedCampaigns ns2:Denmark_s_Socialist_Party ;
    ns1:description "Protest"^^xsd:string ;
    ns1:isLaunchedBy ns2:Denmark ;
    ns2:behaviour ns2:Protest ;
    ns2:hasActor "Anonymous (Denmark)"^^xsd:string ;
    ns2:hasActorCountry "Denmark"^^xsd:string ;
    ns2:hasCountry "Denmark"^^xsd:string ;
    ns2:hasEventDate "2014-06-11T00:00:00"^^xsd:dateTime ;
    ns2:hasEventSubtype "Exploitation of Application Server"^^xsd:string ;
    ns2:hasEventType "Exploitive"^^xsd:string ;
    ns2:hasIndustry "Other Services (except Public Administration)"^^xsd:string ;
    ns2:hasMonth 6 ;
    ns2:hasOrganization "Denmark's Socialist Party"^^xsd:string ;
    ns2:hasYear 2014 ;
    ns2:isType_of ns2:Exploitation_of_Application_Server ;
    rdfs:comment "The Danish branch of the infamous collective Anonymous targets Denmark's Socialist Party (Socialistisk Folkeparti) for signing and passing mass Internet surveillance bill and leaks  logins and SSNs of a couple of dozens of members."^^xsd:string .

ns2:da629c485fbd050c a ns2:DDoS,
        owl:NamedIndividual ;
    ns1:associatedCampaigns ns2:Battle_net ;
    ns2:hasActorType "Criminal"^^xsd:string ;
    ns2:hasCampaign ns2:California ;
    ns2:hasCountry "United States of America"^^xsd:string ;
    ns2:hasCounty "Orange"^^xsd:string ;
    ns2:hasEventDate "2014-08-25T00:00:00"^^xsd:dateTime ;
    ns2:hasEventSubtype "External Denial of Service"^^xsd:string ;
    ns2:hasEventType "Disruptive"^^xsd:string ;
    ns2:hasIndustry "Information"^^xsd:string ;
    ns2:hasMonth 8 ;
    ns2:hasOrganization "Battle.net"^^xsd:string ;
    ns2:hasState "California"^^xsd:string ;
    ns2:hasYear 2014 ;
    ns2:isType_of ns2:Criminal,
        ns2:External_Denial_of_Service ;
    rdfs:comment "Sony admits that a DDoS attack impacted online services, Sony's PlayStation Network and the Sony Entertainment Network. Other affected services involve: Xbox Live, Blizzard's Battle.net, and Grinding Gear Games."^^xsd:string .

ns2:dae96c0c16442450 a ns2:AccountAttack,
        owl:NamedIndividual ;
    ns1:associatedCampaigns ns2:The_Home_Depot ;
    ns1:description "Financial"^^xsd:string ;
    ns2:behaviour ns2:Financial ;
    ns2:hasActorType "Criminal"^^xsd:string ;
    ns2:hasCampaign ns2:Georgia ;
    ns2:hasCountry "United States of America"^^xsd:string ;
    ns2:hasCounty "Cobb"^^xsd:string ;
    ns2:hasEventDate "2014-09-02T00:00:00"^^xsd:dateTime ;
    ns2:hasEventSubtype "Exploitation of Sensors"^^xsd:string ;
    ns2:hasEventType "Exploitive"^^xsd:string ;
    ns2:hasIndustry "Retail Trade"^^xsd:string ;
    ns2:hasMonth 9 ;
    ns2:hasOrganization "The Home Depot"^^xsd:string ;
    ns2:hasState "Georgia"^^xsd:string ;
    ns2:hasYear 2014 ;
    ns2:isType_of ns2:Criminal,
        ns2:Exploitation_of_Sensors ;
    rdfs:comment "Home Depot confirms that thieves compromised the payment systems in its 2,200 stores in the US and Canada and stole credit and debit card data. Home Depot believes that 56 million credit cards were compromised by criminals."^^xsd:string .

ns2:db026d113e2f54cd a ns2:AnonymousAttack,
        owl:NamedIndividual ;
    ns1:associatedCampaigns ns2:Employees_Old_Age_Benefits_Institution ;
    ns2:hasActor "Anonymous"^^xsd:string ;
    ns2:hasActorType "Hacktivist"^^xsd:string ;
    ns2:hasCountry "Pakistan"^^xsd:string ;
    ns2:hasEventDate "2014-08-30T00:00:00"^^xsd:dateTime ;
    ns2:hasEventSubtype "External Denial of Service"^^xsd:string ;
    ns2:hasEventType "Disruptive"^^xsd:string ;
    ns2:hasIndustry "Public Administration"^^xsd:string ;
    ns2:hasMonth 8 ;
    ns2:hasOrganization "Employees Old-Age Benefits Institution"^^xsd:string ;
    ns2:hasYear 2014 ;
    ns2:isType_of ns2:External_Denial_of_Service,
        ns2:Hacktivist ;
    rdfs:comment "In the name of #OpPakistan, Anonymous conducts a massive cyber attack against many Pakistani government websites, including Parkistan Army's recruitment website, government of Punjab's official portal, Pakistan Meteorological Department, Employees Old-Age Benefits Institution, and several other high-profile sites."^^xsd:string .

ns2:de3960af0f5a82aa a ns2:AttackWebsite,
        owl:NamedIndividual ;
    ns1:associatedCampaigns ns2:Football_Federation_of_Armenia ;
    ns1:description "Protest"^^xsd:string ;
    ns1:isLaunchedBy ns2:Azerbaijan ;
    ns2:behaviour ns2:Protest ;
    ns2:hasActor "Anti-Armenia Team"^^xsd:string ;
    ns2:hasActorCountry "Azerbaijan"^^xsd:string ;
    ns2:hasActorType "Hacktivist"^^xsd:string ;
    ns2:hasCountry "Armenia"^^xsd:string ;
    ns2:hasEventDate "2014-01-23T00:00:00"^^xsd:dateTime ;
    ns2:hasEventSubtype "Message Manipulation"^^xsd:string ;
    ns2:hasEventType "Disruptive"^^xsd:string ;
    ns2:hasIndustry "Arts, Entertainment, and Recreation"^^xsd:string ;
    ns2:hasMonth 1 ;
    ns2:hasOrganization "Football Federation of Armenia"^^xsd:string ;
    ns2:hasYear 2014 ;
    ns2:isType_of ns2:Hacktivist,
        ns2:Message_Manipulation ;
    rdfs:comment "Azerbaijan Hackers from Anti-Armenia Team have hacked and defaced several Armenian government ministries websites."^^xsd:string .

ns2:dea760c72ded238d a ns2:CyberattackData,
        owl:NamedIndividual ;
    ns1:associatedCampaigns ns2:RSA ;
    ns1:isLaunchedBy ns2:Syrian_Arab_Republic ;
    ns2:hasActor "Syrian Electronic Army"^^xsd:string ;
    ns2:hasActorCountry "Syrian Arab Republic"^^xsd:string ;
    ns2:hasActorType "Hacktivist"^^xsd:string ;
    ns2:hasCampaign ns2:California ;
    ns2:hasCountry "United States of America"^^xsd:string ;
    ns2:hasCounty "San Francisco"^^xsd:string ;
    ns2:hasEventDate "2014-04-29T00:00:00"^^xsd:dateTime ;
    ns2:hasEventSubtype "Message Manipulation"^^xsd:string ;
    ns2:hasEventType "Disruptive"^^xsd:string ;
    ns2:hasIndustry "Other Services (except Public Administration)"^^xsd:string ;
    ns2:hasMonth 4 ;
    ns2:hasOrganization "RSA"^^xsd:string ;
    ns2:hasState "California"^^xsd:string ;
    ns2:hasYear 2014 ;
    ns2:isType_of ns2:Hacktivist,
        ns2:Message_Manipulation ;
    rdfs:comment "The Syrian Electronic Army redirects the visitors of the RSA Conference website to a defacement page. The attack is carried out in response to an RSA Conference presentation about the Syrian Electronic Army's hacking methods."^^xsd:string .

ns2:dedcbf306174ff2d a ns2:CyberattackData,
        owl:NamedIndividual ;
    ns1:associatedCampaigns ns2:Ministry_of_Police_Affairs ;
    ns1:description "Protest"^^xsd:string ;
    ns1:isLaunchedBy ns2:Nigeria ;
    ns2:behaviour ns2:Protest ;
    ns2:hasActor "Nigerian Cyber Army"^^xsd:string ;
    ns2:hasActorCountry "Nigeria"^^xsd:string ;
    ns2:hasActorType "Hacktivist"^^xsd:string ;
    ns2:hasCountry "Nigeria"^^xsd:string ;
    ns2:hasEventDate "2014-01-30T00:00:00"^^xsd:dateTime ;
    ns2:hasEventSubtype "Message Manipulation"^^xsd:string ;
    ns2:hasEventType "Disruptive"^^xsd:string ;
    ns2:hasIndustry "Public Administration"^^xsd:string ;
    ns2:hasMonth 1 ;
    ns2:hasOrganization "Ministry of Police Affairs"^^xsd:string ;
    ns2:hasYear 2014 ;
    ns2:isType_of ns2:Hacktivist,
        ns2:Message_Manipulation ;
    rdfs:comment "The official website of Nigeria's Ministry of Police Affairs (policeaffairs.gov.ng) is breached and defaced by hackers of the Nigerian Cyber Army."^^xsd:string .

ns2:df05de81c82f0f37 a ns2:HackerSecurity,
        owl:NamedIndividual ;
    ns1:associatedCampaigns ns2:Financial_Services_Online ;
    ns1:isLaunchedBy ns2:Pakistan ;
    ns2:hasActor "Pakiz Cyber Squad"^^xsd:string ;
    ns2:hasActorCountry "Pakistan"^^xsd:string ;
    ns2:hasCountry "Australia"^^xsd:string ;
    ns2:hasEventDate "2014-01-03T00:00:00"^^xsd:dateTime ;
    ns2:hasEventSubtype "Exploitation of Application Server"^^xsd:string ;
    ns2:hasEventType "Exploitive"^^xsd:string ;
    ns2:hasIndustry "Finance and Insurance"^^xsd:string ;
    ns2:hasMonth 1 ;
    ns2:hasOrganization "Financial Services Online"^^xsd:string ;
    ns2:hasYear 2014 ;
    ns2:isType_of ns2:Exploitation_of_Application_Server ;
    rdfs:comment "A group of Pakistani hackers called Pakiz Cyber Squad hacks Financial Services Online (financialservicesonline.com.au), and dumps 527 affiliate account credentials."^^xsd:string .

ns2:df270e1ea62b9d38 a ns2:BreachSecurity,
        owl:NamedIndividual ;
    ns1:associatedCampaigns ns2:BigBoss_repository ;
    ns2:hasActor "Kim Jong-Cracks"^^xsd:string ;
    ns2:hasEventDate "2014-07-21T00:00:00"^^xsd:dateTime ;
    ns2:hasEventSubtype "Exploitation of Application Server"^^xsd:string ;
    ns2:hasEventType "Exploitive"^^xsd:string ;
    ns2:hasIndustry "Professional, Scientific, and Technical Services"^^xsd:string ;
    ns2:hasMonth 7 ;
    ns2:hasOrganization "BigBoss repository"^^xsd:string ;
    ns2:hasYear 2014 ;
    ns2:isType_of ns2:Exploitation_of_Application_Server ;
    rdfs:comment "BigBoss repository, one of the biggest and most popular repositories for jailbreak tweaks in Cydia, has reportedly been hacked by either an individual or a group of hackers going by the name of Kim Jong-CracksÃ'ÃÂ."^^xsd:string .

ns2:df89a9e5cf4b85f3 a ns2:AccountAttack,
        owl:NamedIndividual ;
    ns1:associatedCampaigns ns2:Jon__Bones__Jones ;
    ns2:hasActorType "Criminal"^^xsd:string ;
    ns2:hasCountry "United States of America"^^xsd:string ;
    ns2:hasEventDate "2014-04-18T00:00:00"^^xsd:dateTime ;
    ns2:hasEventSubtype "Message Manipulation"^^xsd:string ;
    ns2:hasEventType "Disruptive"^^xsd:string ;
    ns2:hasIndustry "Other Services (except Public Administration)"^^xsd:string ;
    ns2:hasMonth 4 ;
    ns2:hasOrganization "Jon \"Bones\" Jones"^^xsd:string ;
    ns2:hasYear 2014 ;
    ns2:isType_of ns2:Criminal,
        ns2:Message_Manipulation ;
    rdfs:comment "Several accounts of the Ultimate Fighting Championship (UFC) fighter Jon BonesÃÆÃ'Ãâ 'ÃÆÃ¢â¬Â 'ÃÆÃ'ÃÂ¢Ã¢'Â¬ÃÂ ''ÃÆÃ'Ãâ 'ÃÆÃ¢â¬Â ''ÃÆÃ'Ãâ ''ÃÆÃ''ÃÆ'Ã'ÃÂ Jones are hacked, posting homophobic comments on Instagram."^^xsd:string .

ns2:discoveryTime a owl:DatatypeProperty ;
    rdfs:domain ns1:Vulnerability ;
    rdfs:range xsd:dateTime .

ns2:e0e9cbcc6e4e0338 a ns2:CyberattackData,
        owl:NamedIndividual ;
    ns1:associatedCampaigns ns2:Telecommunications_Directorate ;
    ns1:description "Protest"^^xsd:string ;
    ns1:isLaunchedBy ns2:Turkey ;
    ns2:behaviour ns2:Protest ;
    ns2:hasActor "RedHack"^^xsd:string ;
    ns2:hasActorCountry "Turkey"^^xsd:string ;
    ns2:hasActorType "Hacktivist"^^xsd:string ;
    ns2:hasCountry "Turkey"^^xsd:string ;
    ns2:hasEventDate "2014-03-28T00:00:00"^^xsd:dateTime ;
    ns2:hasEventSubtype "External Denial of Service"^^xsd:string ;
    ns2:hasEventType "Disruptive"^^xsd:string ;
    ns2:hasIndustry "Public Administration"^^xsd:string ;
    ns2:hasMonth 3 ;
    ns2:hasOrganization "Telecommunications Directorate"^^xsd:string ;
    ns2:hasYear 2014 ;
    ns2:isType_of ns2:External_Denial_of_Service,
        ns2:Hacktivist ;
    rdfs:comment "Hackers of the RedHack group have launched a cyberattack against the official website of Turkey's Telecommunications Directorate (tib.gov.tr) in response to the decision to ban YouTube and Twitter in the country."^^xsd:string .

ns2:e14b207a68308488 a ns2:BreachInformation,
        owl:NamedIndividual ;
    ns1:associatedCampaigns ns2:Kickstarter ;
    ns2:hasActorType "Criminal"^^xsd:string ;
    ns2:hasCampaign ns2:New_York ;
    ns2:hasCountry "United States of America"^^xsd:string ;
    ns2:hasCounty "Kings"^^xsd:string ;
    ns2:hasEventDate "2014-02-16T00:00:00"^^xsd:dateTime ;
    ns2:hasEventSubtype "Exploitation of Application Server"^^xsd:string ;
    ns2:hasEventType "Exploitive"^^xsd:string ;
    ns2:hasIndustry "Other Services (except Public Administration)"^^xsd:string ;
    ns2:hasMonth 2 ;
    ns2:hasOrganization "Kickstarter"^^xsd:string ;
    ns2:hasState "New York"^^xsd:string ;
    ns2:hasYear 2014 ;
    ns2:isType_of ns2:Criminal,
        ns2:Exploitation_of_Application_Server ;
    rdfs:comment "Kickstarter announces that it has become aware of a security breach resulting in the loss of personal customer data like usernames, email addresses, mailing addresses, phone numbers, and encrypted passwords.ÃÆÃ'Ãâ 'ÃÆÃ¢â¬Â 'ÃÆÃ'ÃÂ¢Ã¢'Â¬ÃÂ ''ÃÆÃ'Ãâ 'ÃÆÃ¢â¬Â ''ÃÆÃ'Ãâ ''ÃÆÃ''ÃÆ'Ã'ÃÂ Potentially 5.6 million users have been affected."^^xsd:string .

ns2:e14d6a563ca50169 a ns2:AttackWebsite,
        owl:NamedIndividual ;
    ns1:associatedCampaigns ns2:Syrian_Electronic_Army ;
    ns1:isLaunchedBy ns2:Turkey ;
    ns2:hasActor "TurkGuvenligi"^^xsd:string ;
    ns2:hasActorCountry "Turkey"^^xsd:string ;
    ns2:hasActorType "Hacktivist"^^xsd:string ;
    ns2:hasCountry "Syrian Arab Republic"^^xsd:string ;
    ns2:hasEventDate "2014-01-15T00:00:00"^^xsd:dateTime ;
    ns2:hasEventSubtype "Message Manipulation"^^xsd:string ;
    ns2:hasEventType "Disruptive"^^xsd:string ;
    ns2:hasIndustry "Other Services (except Public Administration)"^^xsd:string ;
    ns2:hasMonth 1 ;
    ns2:hasOrganization "Syrian Electronic Army"^^xsd:string ;
    ns2:hasYear 2014 ;
    ns2:isType_of ns2:Hacktivist,
        ns2:Message_Manipulation ;
    rdfs:comment "The Turkish hacking collective TurkGuvenligi defaces the Syrian Electronic Army's website."^^xsd:string .

ns2:e1d61101802c8490 a ns2:HackerSecurity,
        owl:NamedIndividual ;
    ns1:associatedCampaigns ns2:Vice ;
    ns1:description "Financial"^^xsd:string ;
    ns1:isLaunchedBy ns2:Russian_Federation ;
    ns2:behaviour ns2:Financial ;
    ns2:hasActor "W0rm"^^xsd:string ;
    ns2:hasActorCountry "Russian Federation"^^xsd:string ;
    ns2:hasActorType "Criminal"^^xsd:string ;
    ns2:hasCampaign ns2:New_York ;
    ns2:hasCountry "United States of America"^^xsd:string ;
    ns2:hasCounty "Kings"^^xsd:string ;
    ns2:hasEventDate "2014-07-22T00:00:00"^^xsd:dateTime ;
    ns2:hasEventSubtype "Exploitation of Application Server"^^xsd:string ;
    ns2:hasEventType "Exploitive"^^xsd:string ;
    ns2:hasIndustry "Public Administration"^^xsd:string ;
    ns2:hasMonth 7 ;
    ns2:hasOrganization "Vice"^^xsd:string ;
    ns2:hasState "New York"^^xsd:string ;
    ns2:hasYear 2014 ;
    ns2:isType_of ns2:Criminal,
        ns2:Exploitation_of_Application_Server ;
    rdfs:comment "W0rm hacks vice.com and accesses a list of CMS users. Hacked data includes email addresses and hashed passwords."^^xsd:string .

ns2:e1dd81da1f6d3a67 a ns2:CyberattackInformation,
        owl:NamedIndividual ;
    ns1:associatedCampaigns ns2:AVG ;
    ns2:hasActor "Hmei7; SultanHaikal"^^xsd:string ;
    ns2:hasActorType "Hacktivist"^^xsd:string ;
    ns2:hasCountry "Czechia"^^xsd:string ;
    ns2:hasEventDate "2014-01-15T00:00:00"^^xsd:dateTime ;
    ns2:hasEventSubtype "Message Manipulation"^^xsd:string ;
    ns2:hasEventType "Disruptive"^^xsd:string ;
    ns2:hasIndustry "Information"^^xsd:string ;
    ns2:hasMonth 1 ;
    ns2:hasOrganization "AVG"^^xsd:string ;
    ns2:hasYear 2014 ;
    ns2:isType_of ns2:Hacktivist,
        ns2:Message_Manipulation ;
    rdfs:comment "19 official domains of AVG are defaced by different hackers from Indonesia and Pakistan."^^xsd:string .

ns2:e1ef76e81baabadc a ns2:DDoS,
        owl:NamedIndividual ;
    ns1:associatedCampaigns ns2:popvote_hk ;
    ns2:hasActorType "Criminal"^^xsd:string ;
    ns2:hasCountry "China"^^xsd:string ;
    ns2:hasEventDate "2014-06-23T00:00:00"^^xsd:dateTime ;
    ns2:hasEventSubtype "External Denial of Service"^^xsd:string ;
    ns2:hasEventType "Disruptive"^^xsd:string ;
    ns2:hasIndustry "Other Services (except Public Administration)"^^xsd:string ;
    ns2:hasMonth 6 ;
    ns2:hasOrganization "popvote.hk"^^xsd:string ;
    ns2:hasYear 2014 ;
    ns2:isType_of ns2:Criminal,
        ns2:External_Denial_of_Service ;
    rdfs:comment "One of the largest and most sophisticated DDoS attacks (300 Gbps peak) hits popvote.hk, an online democracy poll canvassing opinion on future Hong Kong elections."^^xsd:string .

ns2:e27b9f14fb1b92b4 a ns2:MalwareVictim,
        owl:NamedIndividual ;
    ns1:associatedCampaigns ns2:Cryptome ;
    ns2:hasActorType "Criminal"^^xsd:string ;
    ns2:hasCountry "United States of America"^^xsd:string ;
    ns2:hasEventDate "2014-06-25T00:00:00"^^xsd:dateTime ;
    ns2:hasEventSubtype "Exploitation of Application Server"^^xsd:string ;
    ns2:hasEventType "Exploitive"^^xsd:string ;
    ns2:hasIndustry "Other Services (except Public Administration)"^^xsd:string ;
    ns2:hasMonth 6 ;
    ns2:hasOrganization "Cryptome"^^xsd:string ;
    ns2:hasYear 2014 ;
    ns2:isType_of ns2:Criminal,
        ns2:Exploitation_of_Application_Server ;
    rdfs:comment "Whistle-blowing site Cryptome is left temporarily unavailable after its service provider NetSol stops routing traffic towards the site following the discovery of a suspect and probably malicious PHP file."^^xsd:string .

ns2:e2fa420876baaf3c a ns2:BreachInformation,
        owl:NamedIndividual ;
    ns1:associatedCampaigns ns2:Ground_ctrl ;
    ns1:description "Financial"^^xsd:string ;
    ns2:behaviour ns2:Financial ;
    ns2:hasActorType "Criminal"^^xsd:string ;
    ns2:hasCampaign ns2:California ;
    ns2:hasCountry "United States of America"^^xsd:string ;
    ns2:hasCounty "Sacramento"^^xsd:string ;
    ns2:hasEventDate "2014-05-07T00:00:00"^^xsd:dateTime ;
    ns2:hasEventSubtype "Exploitation of Application Server"^^xsd:string ;
    ns2:hasEventType "Exploitive"^^xsd:string ;
    ns2:hasIndustry "Professional, Scientific, and Technical Services"^^xsd:string ;
    ns2:hasMonth 5 ;
    ns2:hasOrganization "Ground(ctrl)"^^xsd:string ;
    ns2:hasState "California"^^xsd:string ;
    ns2:hasYear 2014 ;
    ns2:isType_of ns2:Criminal,
        ns2:Exploitation_of_Application_Server ;
    rdfs:comment "Ground(ctrl), a company which builds social networking sites and other services for musicians, begins notifying an undisclosed number of users that their personal information may have been exposed when the company's network was hacked."^^xsd:string .

ns2:e40d30ff13486ecd a ns2:BreachInformation,
        owl:NamedIndividual ;
    ns1:associatedCampaigns ns2:University_of_Pittsburgh_Medical_Center ;
    ns1:description "Financial"^^xsd:string ;
    ns2:behaviour ns2:Financial ;
    ns2:hasActorType "Criminal"^^xsd:string ;
    ns2:hasCampaign ns2:Pennsylvania ;
    ns2:hasCountry "United States of America"^^xsd:string ;
    ns2:hasCounty "Allegheny"^^xsd:string ;
    ns2:hasEventDate "2014-04-17T00:00:00"^^xsd:dateTime ;
    ns2:hasEventSubtype "Exploitation of Application Server"^^xsd:string ;
    ns2:hasEventType "Exploitive"^^xsd:string ;
    ns2:hasIndustry "Health Care and Social Assistance"^^xsd:string ;
    ns2:hasMonth 4 ;
    ns2:hasOrganization "University of Pittsburgh Medical Center"^^xsd:string ;
    ns2:hasState "Pennsylvania"^^xsd:string ;
    ns2:hasYear 2014 ;
    ns2:isType_of ns2:Criminal,
        ns2:Exploitation_of_Application_Server ;
    rdfs:comment "UPMC (University of Pittsburgh Medical Center) reveals the real dimension of a data breach it suffered. Personal information for as many as 27,000 workers might have been compromised."^^xsd:string .

ns2:e4a27262c4edef6f a ns2:DDoS,
        owl:NamedIndividual ;
    ns1:associatedCampaigns ns2:Sony_PlayStation_Network ;
    ns1:isLaunchedBy ns2:Japan ;
    ns2:hasActor "Islamic State"^^xsd:string ;
    ns2:hasActorCountry "Japan"^^xsd:string ;
    ns2:hasActorType "Hacktivist"^^xsd:string ;
    ns2:hasCountry "Japan"^^xsd:string ;
    ns2:hasEventDate "2014-08-25T00:00:00"^^xsd:dateTime ;
    ns2:hasEventSubtype "External Denial of Service"^^xsd:string ;
    ns2:hasEventType "Disruptive"^^xsd:string ;
    ns2:hasIndustry "Information"^^xsd:string ;
    ns2:hasMonth 8 ;
    ns2:hasOrganization "Sony PlayStation Network"^^xsd:string ;
    ns2:hasYear 2014 ;
    ns2:isType_of ns2:External_Denial_of_Service,
        ns2:Hacktivist ;
    rdfs:comment "Sony admits that a DDoS attack impacted online services, Sony's PlayStation Network and the Sony Entertainment Network. Other affected services involve: Xbox Live, Blizzard's Battle.net, and Grinding Gear Games."^^xsd:string .

ns2:e4e84bf7686b80f5 a ns2:BreachInformation,
        owl:NamedIndividual ;
    ns1:associatedCampaigns ns2:British_Gas ;
    ns1:description "Financial"^^xsd:string ;
    ns2:behaviour ns2:Financial ;
    ns2:hasActorType "Criminal"^^xsd:string ;
    ns2:hasCountry "United Kingdom of Great Britain and Northern Ireland"^^xsd:string ;
    ns2:hasEventDate "2014-06-22T00:00:00"^^xsd:dateTime ;
    ns2:hasEventSubtype "Message Manipulation"^^xsd:string ;
    ns2:hasEventType "Disruptive"^^xsd:string ;
    ns2:hasIndustry "Utilities"^^xsd:string ;
    ns2:hasMonth 6 ;
    ns2:hasOrganization "British Gas"^^xsd:string ;
    ns2:hasYear 2014 ;
    ns2:isType_of ns2:Criminal,
        ns2:Message_Manipulation ;
    rdfs:comment "British Gas' support team Twitter account (@BritishGasHelp) is hacked and starts posting very strange tweets."^^xsd:string .

ns2:e5cafdeec693027e a ns2:BreachSecurity,
        owl:NamedIndividual ;
    ns1:associatedCampaigns ns2:Onsite_Health_Diagnostics ;
    ns2:hasActorType "Criminal"^^xsd:string ;
    ns2:hasCampaign ns2:Tennessee ;
    ns2:hasCountry "United States of America"^^xsd:string ;
    ns2:hasCounty "Davidson"^^xsd:string ;
    ns2:hasEventDate "2014-08-13T00:00:00"^^xsd:dateTime ;
    ns2:hasEventSubtype "Exploitation of Application Server"^^xsd:string ;
    ns2:hasEventType "Exploitive"^^xsd:string ;
    ns2:hasIndustry "Health Care and Social Assistance"^^xsd:string ;
    ns2:hasMonth 8 ;
    ns2:hasOrganization "Onsite Health Diagnostics"^^xsd:string ;
    ns2:hasState "Tennessee"^^xsd:string ;
    ns2:hasYear 2014 ;
    ns2:isType_of ns2:Criminal,
        ns2:Exploitation_of_Application_Server ;
    rdfs:comment "More than 60,000 staffers who participated in Tennessee employee health screenings are notified that their personal information may have been accessed by an unknown attacker that hacked into the computer system of Onsite Health Diagnostics, a subcontractor hired by Healthways, the state's wellness contractor."^^xsd:string .

ns2:e5e9ecc17bde32fa a ns2:BreachInformation,
        owl:NamedIndividual ;
    ns1:associatedCampaigns ns2:Ariana_Grande ;
    ns1:description "Personal Attack"^^xsd:string ;
    ns2:behaviour ns2:Personal_Attack ;
    ns2:hasActorType "Criminal"^^xsd:string ;
    ns2:hasCountry "United States of America"^^xsd:string ;
    ns2:hasEventDate "2014-08-31T00:00:00"^^xsd:dateTime ;
    ns2:hasEventSubtype "Exploitation of Application Server"^^xsd:string ;
    ns2:hasEventType "Exploitive"^^xsd:string ;
    ns2:hasIndustry "Other Services (except Public Administration)"^^xsd:string ;
    ns2:hasMonth 8 ;
    ns2:hasOrganization "Ariana Grande"^^xsd:string ;
    ns2:hasYear 2014 ;
    ns2:isType_of ns2:Criminal,
        ns2:Exploitation_of_Application_Server ;
    rdfs:comment "Yet another leak of celebrities pictures. A massive leak of nude and risque photos appearing to be of huge stars like is leaked online, first appearing on 4chan."^^xsd:string .

ns2:e6f10ce74cec9dca a ns2:CyberattackData,
        owl:NamedIndividual ;
    ns1:associatedCampaigns ns2:Renault ;
    ns1:isLaunchedBy ns2:Pakistan ;
    ns2:hasActor "Team Cyber Criminals"^^xsd:string ;
    ns2:hasActorCountry "Pakistan"^^xsd:string ;
    ns2:hasActorType "Hobbyist"^^xsd:string ;
    ns2:hasCountry "Guatemala"^^xsd:string ;
    ns2:hasEventDate "2014-03-18T00:00:00"^^xsd:dateTime ;
    ns2:hasEventSubtype "Message Manipulation"^^xsd:string ;
    ns2:hasEventType "Disruptive"^^xsd:string ;
    ns2:hasIndustry "Manufacturing"^^xsd:string ;
    ns2:hasMonth 3 ;
    ns2:hasOrganization "Renault"^^xsd:string ;
    ns2:hasYear 2014 ;
    ns2:isType_of ns2:Hobbyist,
        ns2:Message_Manipulation ;
    rdfs:comment "The Guatemala websites of Renault, Toyota and Chevrolet are hacked and defaced by a member of a Pakistani group called Team Cyber Criminals."^^xsd:string .

ns2:e73bc26382a87068 a ns2:CyberattackInformation,
        owl:NamedIndividual ;
    ns1:associatedCampaigns ns2:Egyptian_Ministry_of_Information ;
    ns1:isLaunchedBy ns2:Libya ;
    ns2:hasActor "Libyan Cyber Army"^^xsd:string ;
    ns2:hasActorCountry "Libya"^^xsd:string ;
    ns2:hasActorType "Hacktivist"^^xsd:string ;
    ns2:hasCountry "Egypt"^^xsd:string ;
    ns2:hasEventDate "2014-04-28T00:00:00"^^xsd:dateTime ;
    ns2:hasEventSubtype "Message Manipulation"^^xsd:string ;
    ns2:hasEventType "Disruptive"^^xsd:string ;
    ns2:hasIndustry "Public Administration"^^xsd:string ;
    ns2:hasMonth 4 ;
    ns2:hasOrganization "Egyptian Ministry of Information"^^xsd:string ;
    ns2:hasYear 2014 ;
    ns2:isType_of ns2:Hacktivist,
        ns2:Message_Manipulation ;
    rdfs:comment "The official website of theÃ'ÃÂ Egyptian Ministry of Information is hacked and defaced by hackers from a group going with the handle of Libyan Cyber Army."^^xsd:string .

ns2:e788ffac009605ce a ns2:BreachInformation,
        owl:NamedIndividual ;
    ns1:associatedCampaigns ns2:Sheplers ;
    ns1:description "Financial"^^xsd:string ;
    ns2:behaviour ns2:Financial ;
    ns2:hasActorType "Criminal"^^xsd:string ;
    ns2:hasCampaign ns2:Kansas ;
    ns2:hasCountry "United States of America"^^xsd:string ;
    ns2:hasCounty "Sedgwick"^^xsd:string ;
    ns2:hasEventDate "2014-09-04T00:00:00"^^xsd:dateTime ;
    ns2:hasEventSubtype "Exploitation of Sensors"^^xsd:string ;
    ns2:hasEventType "Exploitive"^^xsd:string ;
    ns2:hasIndustry "Retail Trade"^^xsd:string ;
    ns2:hasMonth 9 ;
    ns2:hasOrganization "Sheplers"^^xsd:string ;
    ns2:hasState "Kansas"^^xsd:string ;
    ns2:hasYear 2014 ;
    ns2:isType_of ns2:Criminal,
        ns2:Exploitation_of_Sensors ;
    rdfs:comment "Western wear retailer Sheplers notifies an undisclosed number of customers that their payment card information may have been exposed after hackers gained access to its payment systems."^^xsd:string .

ns2:e79fbdd8a7c2653e a ns2:DDoS,
        owl:NamedIndividual ;
    ns1:associatedCampaigns ns2:Basecamp ;
    ns1:description "Financial"^^xsd:string ;
    ns2:behaviour ns2:Financial ;
    ns2:hasActorType "Criminal"^^xsd:string ;
    ns2:hasCampaign ns2:Illinois ;
    ns2:hasCountry "United States of America"^^xsd:string ;
    ns2:hasCounty "Cook"^^xsd:string ;
    ns2:hasEventDate "2014-03-24T00:00:00"^^xsd:dateTime ;
    ns2:hasEventSubtype "External Denial of Service"^^xsd:string ;
    ns2:hasEventType "Disruptive"^^xsd:string ;
    ns2:hasIndustry "Professional, Scientific, and Technical Services"^^xsd:string ;
    ns2:hasMonth 3 ;
    ns2:hasOrganization "Basecamp"^^xsd:string ;
    ns2:hasState "Illinois"^^xsd:string ;
    ns2:hasYear 2014 ;
    ns2:isType_of ns2:Criminal,
        ns2:External_Denial_of_Service ;
    rdfs:comment "After refusing to pay a ransom, Basecamp is the victim of a DDoS  attack."^^xsd:string .

ns2:e7f89b6053c0c57a a ns2:AttackWebsite,
        owl:NamedIndividual ;
    ns1:associatedCampaigns ns2:PTV_Sports ;
    ns1:description "Protest"^^xsd:string ;
    ns1:isLaunchedBy ns2:Pakistan ;
    ns2:behaviour ns2:Protest ;
    ns2:hasActor "Pakistan Haxors Crew"^^xsd:string ;
    ns2:hasActorCountry "Pakistan"^^xsd:string ;
    ns2:hasActorType "Hacktivist"^^xsd:string ;
    ns2:hasCountry "Pakistan"^^xsd:string ;
    ns2:hasEventDate "2014-06-22T00:00:00"^^xsd:dateTime ;
    ns2:hasEventSubtype "Message Manipulation"^^xsd:string ;
    ns2:hasEventType "Disruptive"^^xsd:string ;
    ns2:hasIndustry "Information"^^xsd:string ;
    ns2:hasMonth 6 ;
    ns2:hasOrganization "PTV Sports"^^xsd:string ;
    ns2:hasYear 2014 ;
    ns2:isType_of ns2:Hacktivist,
        ns2:Message_Manipulation ;
    rdfs:comment "Hackers going with the handle of Pakistan Haxors Crew deface the official website of state owned PTV Sports (sports.ptv.com.pk) to protest against killings and police brutality."^^xsd:string .

ns2:e80ba50c5d06dbf9 a ns2:CyberattackInformation,
        owl:NamedIndividual ;
    ns1:associatedCampaigns ns2:German_Aerospace_Centre ;
    ns1:description "Political-Espionage"^^xsd:string ;
    ns2:behaviour ns2:Political_Espionage ;
    ns2:hasActorType "Criminal"^^xsd:string ;
    ns2:hasCountry "Germany"^^xsd:string ;
    ns2:hasEventDate "2014-04-15T00:00:00"^^xsd:dateTime ;
    ns2:hasEventSubtype "Exploitation of Application Server"^^xsd:string ;
    ns2:hasEventType "Exploitive"^^xsd:string ;
    ns2:hasIndustry "Public Administration"^^xsd:string ;
    ns2:hasMonth 4 ;
    ns2:hasOrganization "German Aerospace Centre"^^xsd:string ;
    ns2:hasYear 2014 ;
    ns2:isType_of ns2:Criminal,
        ns2:Exploitation_of_Application_Server ;
    rdfs:comment "Germany's space research centre in Cologne is the victim of a co-ordinated and covert targeted attack carried out by state-sponsored hackers, according to a Der Spiegel report. Suspects are directed to China."^^xsd:string .

ns2:e85eb01d25ac8a1b a ns2:AttackWebsite,
        owl:NamedIndividual ;
    ns1:associatedCampaigns ns2:Duruma_Principality ;
    ns1:description "Protest"^^xsd:string ;
    ns1:isLaunchedBy ns2:Syrian_Arab_Republic ;
    ns2:behaviour ns2:Protest ;
    ns2:hasActor "Syrian Electronic Army"^^xsd:string ;
    ns2:hasActorCountry "Syrian Arab Republic"^^xsd:string ;
    ns2:hasActorType "Hacktivist"^^xsd:string ;
    ns2:hasCountry "Saudi Arabia"^^xsd:string ;
    ns2:hasEventDate "2014-01-16T00:00:00"^^xsd:dateTime ;
    ns2:hasEventSubtype "Message Manipulation"^^xsd:string ;
    ns2:hasEventType "Disruptive"^^xsd:string ;
    ns2:hasIndustry "Public Administration"^^xsd:string ;
    ns2:hasMonth 1 ;
    ns2:hasOrganization "Duruma Principality"^^xsd:string ;
    ns2:hasYear 2014 ;
    ns2:isType_of ns2:Hacktivist,
        ns2:Message_Manipulation ;
    rdfs:comment "The Syrian Electronic Army deface 16 Saudi Arabian government websites. The targeted sites are the ones of various administrative regions."^^xsd:string .

ns2:e8b2c0cd174903a6 a ns2:BreachInformation,
        owl:NamedIndividual ;
    ns1:associatedCampaigns ns2:Al_Arabiya ;
    ns1:isLaunchedBy ns2:United_Arab_Emirates ;
    ns2:hasActor "NullCrew; TheHorseMenLulz"^^xsd:string ;
    ns2:hasActorCountry "United Arab Emirates"^^xsd:string ;
    ns2:hasActorType "Hacktivist"^^xsd:string ;
    ns2:hasCountry "United Arab Emirates"^^xsd:string ;
    ns2:hasEventDate "2014-04-03T00:00:00"^^xsd:dateTime ;
    ns2:hasEventSubtype "Exploitation of Application Server"^^xsd:string ;
    ns2:hasEventType "Exploitive"^^xsd:string ;
    ns2:hasIndustry "Information"^^xsd:string ;
    ns2:hasMonth 4 ;
    ns2:hasOrganization "Al Arabiya"^^xsd:string ;
    ns2:hasYear 2014 ;
    ns2:isType_of ns2:Exploitation_of_Application_Server,
        ns2:Hacktivist ;
    rdfs:comment "NullCrew and TheHorseMenLulz team up and hack into Al Arabiya servers, publishing a list of the company's mail servers and a link to the root file with the vulnerability used to penetrate the system on Pastebin."^^xsd:string .

ns2:e93191f1884172cb a ns2:AttackWebsite,
        owl:NamedIndividual ;
    ns1:associatedCampaigns ns2:Rawalpindi_Police ;
    ns1:isLaunchedBy ns2:Pakistan ;
    ns2:hasActor "Anti Mortadin!@"^^xsd:string ;
    ns2:hasActorCountry "Pakistan"^^xsd:string ;
    ns2:hasActorType "Hacktivist"^^xsd:string ;
    ns2:hasCountry "Pakistan"^^xsd:string ;
    ns2:hasEventDate "2014-05-16T00:00:00"^^xsd:dateTime ;
    ns2:hasEventSubtype "Message Manipulation"^^xsd:string ;
    ns2:hasEventType "Disruptive"^^xsd:string ;
    ns2:hasIndustry "Public Administration"^^xsd:string ;
    ns2:hasMonth 5 ;
    ns2:hasOrganization "Rawalpindi Police"^^xsd:string ;
    ns2:hasYear 2014 ;
    ns2:isType_of ns2:Hacktivist,
        ns2:Message_Manipulation ;
    rdfs:comment "The official website of the Rawalpindi police in Pakistan (rawalpindipolice.gov.pk) is defaced by  Anti Mortadin!@, a group that appears to support the Taliban."^^xsd:string .

ns2:e937cb21fb0155f6 a ns2:BreachInformation,
        owl:NamedIndividual ;
    ns1:associatedCampaigns ns2:Placemark_Investments ;
    ns1:description "Financial"^^xsd:string ;
    ns2:behaviour ns2:Financial ;
    ns2:hasActorType "Criminal"^^xsd:string ;
    ns2:hasCampaign ns2:Massachusetts ;
    ns2:hasCountry "United States of America"^^xsd:string ;
    ns2:hasCounty "Norfolk"^^xsd:string ;
    ns2:hasEventDate "2014-06-10T00:00:00"^^xsd:dateTime ;
    ns2:hasEventSubtype "Exploitation of Application Server"^^xsd:string ;
    ns2:hasEventType "Exploitive"^^xsd:string ;
    ns2:hasIndustry "Finance and Insurance"^^xsd:string ;
    ns2:hasMonth 6 ;
    ns2:hasOrganization "Placemark Investments"^^xsd:string ;
    ns2:hasState "Massachusetts"^^xsd:string ;
    ns2:hasYear 2014 ;
    ns2:isType_of ns2:Criminal,
        ns2:Exploitation_of_Application_Server ;
    rdfs:comment "Placemark Investments begins notifying an undisclosed number of clients that their personal information may have been exposed when one of its servers was breached."^^xsd:string .

ns2:ea06a6bae8f95b75 a ns2:CyberattackData,
        owl:NamedIndividual ;
    ns1:associatedCampaigns ns2:Various_Government_Websites ;
    ns1:description "Protest"^^xsd:string ;
    ns1:isLaunchedBy ns2:Azerbaijan ;
    ns2:behaviour ns2:Protest ;
    ns2:hasActor "Monte Melkonian Cyber Army (MMCA)"^^xsd:string ;
    ns2:hasActorCountry "Azerbaijan"^^xsd:string ;
    ns2:hasActorType "Hacktivist"^^xsd:string ;
    ns2:hasCountry "Turkey"^^xsd:string ;
    ns2:hasEventDate "2014-08-24T00:00:00"^^xsd:dateTime ;
    ns2:hasEventSubtype "Message Manipulation"^^xsd:string ;
    ns2:hasEventType "Disruptive"^^xsd:string ;
    ns2:hasIndustry "Public Administration"^^xsd:string ;
    ns2:hasMonth 8 ;
    ns2:hasOrganization "Various Government Websites"^^xsd:string ;
    ns2:hasYear 2014 ;
    ns2:isType_of ns2:Hacktivist,
        ns2:Message_Manipulation ;
    rdfs:comment "Armenian hackers fromÃÆÃ'Ãâ 'ÃÆÃ¢â¬Â 'ÃÆÃ'ÃÂ¢Ã¢'Â¬ÃÂ ''ÃÆÃ'Ãâ 'ÃÆÃ¢â¬Â ''ÃÆÃ'Ãâ ''ÃÆÃ''ÃÆ'Ã'ÃÂ Monte Melkonian Cyber Army (MMCA) deface 360+ÃÆÃ'Ãâ 'ÃÆÃ¢â¬Â 'ÃÆÃ'ÃÂ¢Ã¢'Â¬ÃÂ ''ÃÆÃ'Ãâ 'ÃÆÃ¢â¬Â ''ÃÆÃ'Ãâ ''ÃÆÃ''ÃÆ'Ã'ÃÂ Turkish websites demanding the Turkish authorities toÃÆÃ'Ãâ 'ÃÆÃ¢â¬Â 'ÃÆÃ'ÃÂ¢Ã¢'Â¬ÃÂ ''ÃÆÃ'Ãâ 'ÃÆÃ¢â¬Â ''ÃÆÃ'Ãâ ''ÃÆÃ''ÃÆ'Ã'ÃÂ recognize theÃÆÃ'Ãâ 'ÃÆÃ¢â¬Â 'ÃÆÃ'ÃÂ¢Ã¢'Â¬ÃÂ ''ÃÆÃ'Ãâ 'ÃÆÃ¢â¬Â ''ÃÆÃ'Ãâ ''ÃÆÃ''ÃÆ'Ã'ÃÂ allegedÃÆÃ'Ãâ 'ÃÆÃ¢â¬Â 'ÃÆÃ'ÃÂ¢Ã¢'Â¬ÃÂ ''ÃÆÃ'Ãâ 'ÃÆÃ¢â¬Â ''ÃÆÃ'Ãâ ''ÃÆÃ''ÃÆ'Ã'ÃÂ Armenian Genocide in 1915."^^xsd:string .

ns2:eabaccfd9f403ba5 a ns2:AttackWebsite,
        owl:NamedIndividual ;
    ns1:associatedCampaigns ns2:banderivets_org_ua ;
    ns2:hasActorType "Criminal"^^xsd:string ;
    ns2:hasCountry "Ukraine"^^xsd:string ;
    ns2:hasEventDate "2014-02-28T00:00:00"^^xsd:dateTime ;
    ns2:hasEventSubtype "External Denial of Service"^^xsd:string ;
    ns2:hasEventType "Disruptive"^^xsd:string ;
    ns2:hasIndustry "Other Services (except Public Administration)"^^xsd:string ;
    ns2:hasMonth 2 ;
    ns2:hasOrganization "banderivets.org.ua"^^xsd:string ;
    ns2:hasYear 2014 ;
    ns2:isType_of ns2:Criminal,
        ns2:External_Denial_of_Service ;
    rdfs:comment "Hacktivists continue to launch attacks against Ukrainian government websites. The latest targets are the sites of the parliament, or the Verkhovna Rada (rada.gov.ua), the Right Sector nationalist movement (banderivets.org.ua), but also some Euromaidan websites."^^xsd:string .

ns2:ec0194f37b3bb202 a ns2:AccountAttack,
        owl:NamedIndividual ;
    ns1:associatedCampaigns ns2:Mizado_Cocina ;
    ns1:description "Financial"^^xsd:string ;
    ns2:behaviour ns2:Financial ;
    ns2:hasActorType "Criminal"^^xsd:string ;
    ns2:hasCampaign ns2:Louisiana ;
    ns2:hasCountry "United States of America"^^xsd:string ;
    ns2:hasCounty "Orleans"^^xsd:string ;
    ns2:hasEventDate "2014-08-19T00:00:00"^^xsd:dateTime ;
    ns2:hasEventSubtype "Exploitation of Sensors"^^xsd:string ;
    ns2:hasEventType "Exploitive"^^xsd:string ;
    ns2:hasIndustry "Accommodation and Food Services"^^xsd:string ;
    ns2:hasMonth 8 ;
    ns2:hasOrganization "Mizado Cocina"^^xsd:string ;
    ns2:hasState "Louisiana"^^xsd:string ;
    ns2:hasYear 2014 ;
    ns2:isType_of ns2:Criminal,
        ns2:Exploitation_of_Sensors ;
    rdfs:comment "Yet another victim of Backoff: New Orleans restaurant Mizado Cocina says customers' credit and debit card information could have been stolen by a hacker who breached the restaurant's point of sale system between May 9 and July 18."^^xsd:string .

ns2:ec852d184a08d00e a ns2:BreachSecurity,
        owl:NamedIndividual ;
    ns1:associatedCampaigns ns2:Healthcare_gov ;
    ns2:hasActorType "Criminal"^^xsd:string ;
    ns2:hasCountry "United States of America"^^xsd:string ;
    ns2:hasEventDate "2014-09-05T00:00:00"^^xsd:dateTime ;
    ns2:hasEventSubtype "Exploitation of Application Server"^^xsd:string ;
    ns2:hasEventType "Exploitive"^^xsd:string ;
    ns2:hasIndustry "Public Administration"^^xsd:string ;
    ns2:hasMonth 9 ;
    ns2:hasOrganization "Healthcare.gov"^^xsd:string ;
    ns2:hasYear 2014 ;
    ns2:isType_of ns2:Criminal,
        ns2:Exploitation_of_Application_Server ;
    rdfs:comment "The White House discloses to the Wall Street Journal that a hacker has breached healthcare.gov, compromising personal data for millions of Americans."^^xsd:string .

ns2:ecac8b3e60a2f72f a ns2:AccessSecurity,
        owl:NamedIndividual ;
    ns1:associatedCampaigns ns2:Record_Assist_LLC ;
    ns2:hasActorType "Criminal"^^xsd:string ;
    ns2:hasCampaign ns2:Texas ;
    ns2:hasCountry "United States of America"^^xsd:string ;
    ns2:hasCounty "Harris"^^xsd:string ;
    ns2:hasEventDate "2014-01-01T00:00:00"^^xsd:dateTime ;
    ns2:hasEventSubtype "Exploitation of Application Server"^^xsd:string ;
    ns2:hasEventType "Exploitive"^^xsd:string ;
    ns2:hasIndustry "Professional, Scientific, and Technical Services"^^xsd:string ;
    ns2:hasMonth 1 ;
    ns2:hasOrganization "Record Assist LLC"^^xsd:string ;
    ns2:hasState "Texas"^^xsd:string ;
    ns2:hasYear 2014 ;
    ns2:isType_of ns2:Criminal,
        ns2:Exploitation_of_Application_Server ;
    rdfs:comment "Record Assist LLC notifies of an unauthorized access possibly compromising residents' names, addresses, credit card numbers and Social Security numbers."^^xsd:string .

ns2:ecf4db82d4d397ba a ns2:BreachSecurity,
        owl:NamedIndividual ;
    ns1:associatedCampaigns ns2:4chan ;
    ns2:hasActorType "Criminal"^^xsd:string ;
    ns2:hasCountry "United States of America"^^xsd:string ;
    ns2:hasEventDate "2014-04-30T00:00:00"^^xsd:dateTime ;
    ns2:hasEventSubtype "Exploitation of Application Server"^^xsd:string ;
    ns2:hasEventType "Exploitive"^^xsd:string ;
    ns2:hasIndustry "Information"^^xsd:string ;
    ns2:hasMonth 4 ;
    ns2:hasOrganization "4chan"^^xsd:string ;
    ns2:hasYear 2014 ;
    ns2:isType_of ns2:Criminal,
        ns2:Exploitation_of_Application_Server ;
    rdfs:comment "The 4chan image message board, admits it suffered a security breach that saw a hacker gain unauthorised access to user information."^^xsd:string .

ns2:ed5e5f966100f1b0 a ns2:DDoS,
        owl:NamedIndividual ;
    ns1:associatedCampaigns ns2:ancestry_com ;
    ns2:hasActorType "Criminal"^^xsd:string ;
    ns2:hasCampaign ns2:Utah ;
    ns2:hasCountry "United States of America"^^xsd:string ;
    ns2:hasCounty "Utah"^^xsd:string ;
    ns2:hasEventDate "2014-06-18T00:00:00"^^xsd:dateTime ;
    ns2:hasEventSubtype "External Denial of Service"^^xsd:string ;
    ns2:hasEventType "Disruptive"^^xsd:string ;
    ns2:hasIndustry "Retail Trade"^^xsd:string ;
    ns2:hasMonth 6 ;
    ns2:hasOrganization "ancestry.com"^^xsd:string ;
    ns2:hasState "Utah"^^xsd:string ;
    ns2:hasYear 2014 ;
    ns2:isType_of ns2:Criminal,
        ns2:External_Denial_of_Service ;
    rdfs:comment "The genealogy site ancestry.com has been blasted off the internet after reportedly being hit by a DDoS attack."^^xsd:string .

ns2:edf47ba4edec10ef a ns2:AccountAttack,
        owl:NamedIndividual ;
    ns1:associatedCampaigns ns2:Sea_Pines_Resort ;
    ns1:description "Financial"^^xsd:string ;
    ns2:behaviour ns2:Financial ;
    ns2:hasActorType "Criminal"^^xsd:string ;
    ns2:hasCampaign ns2:South_Carolina ;
    ns2:hasCountry "United States of America"^^xsd:string ;
    ns2:hasCounty "Beaufort"^^xsd:string ;
    ns2:hasEventDate "2014-09-05T00:00:00"^^xsd:dateTime ;
    ns2:hasEventSubtype "Exploitation of Sensors"^^xsd:string ;
    ns2:hasEventType "Exploitive"^^xsd:string ;
    ns2:hasIndustry "Accommodation and Food Services"^^xsd:string ;
    ns2:hasMonth 9 ;
    ns2:hasOrganization "Sea Pines Resort"^^xsd:string ;
    ns2:hasState "South Carolina"^^xsd:string ;
    ns2:hasYear 2014 ;
    ns2:isType_of ns2:Criminal,
        ns2:Exploitation_of_Sensors ;
    rdfs:comment "Sea Pines Resort may have been the victims of a computer hack resulting in stolen credit card information."^^xsd:string .

ns2:ee967f9412893ca3 a ns2:BreachInformation,
        owl:NamedIndividual ;
    ns1:associatedCampaigns ns2:Kirsten_Dunst ;
    ns1:description "Personal Attack"^^xsd:string ;
    ns2:behaviour ns2:Personal_Attack ;
    ns2:hasActorType "Criminal"^^xsd:string ;
    ns2:hasCountry "United States of America"^^xsd:string ;
    ns2:hasEventDate "2014-08-31T00:00:00"^^xsd:dateTime ;
    ns2:hasEventSubtype "Exploitation of Application Server"^^xsd:string ;
    ns2:hasEventType "Exploitive"^^xsd:string ;
    ns2:hasIndustry "Other Services (except Public Administration)"^^xsd:string ;
    ns2:hasMonth 8 ;
    ns2:hasOrganization "Kirsten Dunst"^^xsd:string ;
    ns2:hasYear 2014 ;
    ns2:isType_of ns2:Criminal,
        ns2:Exploitation_of_Application_Server ;
    rdfs:comment "Yet another leak of celebrities pictures. A massive leak of nude and risque photos appearing to be of huge stars like is leaked online, first appearing on 4chan."^^xsd:string .

ns2:eefbbb48cfc4a3b0 a ns2:BreachUser,
        ns2:HackUsernames,
        owl:NamedIndividual ;
    ns1:associatedCampaigns ns2:baltimorejewishlife_com ;
    ns2:hasActor "Smitt3nz AKA Rubber"^^xsd:string ;
    ns2:hasCampaign ns2:Maryland ;
    ns2:hasCountry "United States of America"^^xsd:string ;
    ns2:hasCounty "Baltimore"^^xsd:string ;
    ns2:hasEventDate "2014-08-07T00:00:00"^^xsd:dateTime ;
    ns2:hasEventSubtype "Exploitation of Application Server"^^xsd:string ;
    ns2:hasEventType "Exploitive"^^xsd:string ;
    ns2:hasIndustry "Information"^^xsd:string ;
    ns2:hasMonth 8 ;
    ns2:hasOrganization "baltimorejewishlife.com"^^xsd:string ;
    ns2:hasState "Maryland"^^xsd:string ;
    ns2:hasYear 2014 ;
    ns2:isType_of ns2:Exploitation_of_Application_Server ;
    rdfs:comment "@smitt3nz hacks baltimorejewishlife.com and dumps nearly 20,000 usernames and plain text passwords."^^xsd:string .

ns2:f0447ca8970e5037 a ns2:AttackWebsite,
        owl:NamedIndividual ;
    ns1:associatedCampaigns ns2:Tata_Motors ;
    ns1:isLaunchedBy ns2:Pakistan ;
    ns2:hasActor "H4$N4!N H4XOR"^^xsd:string ;
    ns2:hasActorCountry "Pakistan"^^xsd:string ;
    ns2:hasActorType "Hacktivist"^^xsd:string ;
    ns2:hasCountry "India"^^xsd:string ;
    ns2:hasEventDate "2014-05-11T00:00:00"^^xsd:dateTime ;
    ns2:hasEventSubtype "Message Manipulation"^^xsd:string ;
    ns2:hasEventType "Disruptive"^^xsd:string ;
    ns2:hasIndustry "Manufacturing"^^xsd:string ;
    ns2:hasMonth 5 ;
    ns2:hasOrganization "Tata Motors"^^xsd:string ;
    ns2:hasYear 2014 ;
    ns2:isType_of ns2:Hacktivist,
        ns2:Message_Manipulation ;
    rdfs:comment "The Pakistani hacker H4$N4!N H4XOR defaces a subdomain of the official website of Tata Motors (connect.tatamotors.com)."^^xsd:string .

ns2:f05bafeaee63a49c a ns2:AccountAttack,
        owl:NamedIndividual ;
    ns1:associatedCampaigns ns2:Carlson_Rezidor_Hotel_Group ;
    ns1:description "Financial"^^xsd:string ;
    ns2:behaviour ns2:Financial ;
    ns2:hasActorType "Criminal"^^xsd:string ;
    ns2:hasCampaign ns2:Minnesota ;
    ns2:hasCountry "United States of America"^^xsd:string ;
    ns2:hasCounty "Hennepin"^^xsd:string ;
    ns2:hasEventDate "2014-04-11T00:00:00"^^xsd:dateTime ;
    ns2:hasEventSubtype "Exploitation of Application Server"^^xsd:string ;
    ns2:hasEventType "Exploitive"^^xsd:string ;
    ns2:hasIndustry "Accommodation and Food Services"^^xsd:string ;
    ns2:hasMonth 4 ;
    ns2:hasOrganization "Carlson Rezidor Hotel Group"^^xsd:string ;
    ns2:hasState "Minnesota"^^xsd:string ;
    ns2:hasYear 2014 ;
    ns2:isType_of ns2:Criminal,
        ns2:Exploitation_of_Application_Server ;
    rdfs:comment "Hackers steal approximately $35,000 in Club Carlson Gold Points (incentive awards earned from hotel stays and food and beverage purchases) from about 650 customers of the Carlson Rezidor Hotel Group."^^xsd:string .

ns2:f05ee751e92fca2a a ns2:CyberattackInformation,
        owl:NamedIndividual ;
    ns1:associatedCampaigns ns2:Official_website_of_the_President_of_Nep ;
    ns1:isLaunchedBy ns2:India ;
    ns2:hasActor "Dr.3v1l"^^xsd:string ;
    ns2:hasActorCountry "India"^^xsd:string ;
    ns2:hasActorType "Hobbyist"^^xsd:string ;
    ns2:hasCountry "Nepal"^^xsd:string ;
    ns2:hasEventDate "2014-02-08T00:00:00"^^xsd:dateTime ;
    ns2:hasEventSubtype "Message Manipulation,Exploitation of Application Server"^^xsd:string ;
    ns2:hasEventType "Mixed"^^xsd:string ;
    ns2:hasIndustry "Public Administration"^^xsd:string ;
    ns2:hasMonth 2 ;
    ns2:hasOrganization "Official website of the President of Nepal"^^xsd:string ;
    ns2:hasYear 2014 ;
    ns2:isType_of ns2:Hobbyist,
        ns2:Message_Manipulation_Exploitation_of_App ;
    rdfs:comment "Two separate attacks deface the official website of Nepal's Office of the President (presidentofnepal.gov.np). In the first case, the attacker who goes by Dr.3v1l, also leaked some information stolen from the DB. The second attack was carried out by an Indian hacker."^^xsd:string .

ns2:f05fdabbc145a290 a ns2:AttackWebsite,
        owl:NamedIndividual ;
    ns1:associatedCampaigns ns2:Ministry_of_Interior ;
    ns1:description "Protest"^^xsd:string ;
    ns1:isLaunchedBy ns2:Kuwait ;
    ns2:behaviour ns2:Protest ;
    ns2:hasActor "Shmook Amer; Dr.Hjd"^^xsd:string ;
    ns2:hasActorCountry "Kuwait"^^xsd:string ;
    ns2:hasActorType "Hacktivist"^^xsd:string ;
    ns2:hasCountry "Kuwait"^^xsd:string ;
    ns2:hasEventDate "2014-03-30T00:00:00"^^xsd:dateTime ;
    ns2:hasEventSubtype "Message Manipulation"^^xsd:string ;
    ns2:hasEventType "Disruptive"^^xsd:string ;
    ns2:hasIndustry "Public Administration"^^xsd:string ;
    ns2:hasMonth 3 ;
    ns2:hasOrganization "Ministry of Interior"^^xsd:string ;
    ns2:hasYear 2014 ;
    ns2:isType_of ns2:Hacktivist,
        ns2:Message_Manipulation ;
    rdfs:comment "The official website of Kuwait's Ministry of Interior (moi.gov.kw) is hacked and defaced Shmook Amer and Dr.Hjd."^^xsd:string .

ns2:f0b469f82c97b607 a ns2:HackerSecurity,
        owl:NamedIndividual ;
    ns1:associatedCampaigns ns2:National_Research_Council ;
    ns1:description "Political-Espionage"^^xsd:string ;
    ns2:behaviour ns2:Political_Espionage ;
    ns2:hasActorType "Criminal"^^xsd:string ;
    ns2:hasCountry "Canada"^^xsd:string ;
    ns2:hasEventDate "2014-07-29T00:00:00"^^xsd:dateTime ;
    ns2:hasEventSubtype "Exploitation of Application Server"^^xsd:string ;
    ns2:hasEventType "Exploitive"^^xsd:string ;
    ns2:hasIndustry "Public Administration"^^xsd:string ;
    ns2:hasMonth 7 ;
    ns2:hasOrganization "National Research Council"^^xsd:string ;
    ns2:hasYear 2014 ;
    ns2:isType_of ns2:Criminal,
        ns2:Exploitation_of_Application_Server ;
    rdfs:comment "The National Research Council (nrc-cnrc.gc.ca), which handles Canada's research and development efforts on behalf of its government, confirms that its IT infrastructure was hacked. China, which immediately refuses the allegations, is accused of the hack."^^xsd:string .

ns2:f111aef4ced111ad a ns2:AccountAttack,
        owl:NamedIndividual ;
    ns1:associatedCampaigns ns2:Affinity_Gaming ;
    ns1:description "Financial"^^xsd:string ;
    ns2:behaviour ns2:Financial ;
    ns2:hasActorType "Criminal"^^xsd:string ;
    ns2:hasCampaign ns2:Nevada ;
    ns2:hasCountry "United States of America"^^xsd:string ;
    ns2:hasCounty "Clark"^^xsd:string ;
    ns2:hasEventDate "2014-05-05T00:00:00"^^xsd:dateTime ;
    ns2:hasEventSubtype "Exploitation of Sensors"^^xsd:string ;
    ns2:hasEventType "Exploitive"^^xsd:string ;
    ns2:hasIndustry "Arts, Entertainment, and Recreation"^^xsd:string ;
    ns2:hasMonth 5 ;
    ns2:hasOrganization "Affinity Gaming"^^xsd:string ;
    ns2:hasState "Nevada"^^xsd:string ;
    ns2:hasYear 2014 ;
    ns2:isType_of ns2:Criminal,
        ns2:Exploitation_of_Sensors ;
    rdfs:comment "Affinity Gaming notifies an unauthorized intrusion into the system that processes customer credit and debit cards for their casinos. Apparently no credit card data was stolen."^^xsd:string .

ns2:f12be8d6540a346e a ns2:HackerSecurity,
        owl:NamedIndividual ;
    ns1:associatedCampaigns ns2:Sears ;
    ns1:description "Financial"^^xsd:string ;
    ns2:behaviour ns2:Financial ;
    ns2:hasActorType "Criminal"^^xsd:string ;
    ns2:hasCampaign ns2:Illinois ;
    ns2:hasCountry "United States of America"^^xsd:string ;
    ns2:hasCounty "Cook"^^xsd:string ;
    ns2:hasEventDate "2014-02-28T00:00:00"^^xsd:dateTime ;
    ns2:hasEventSubtype "Exploitation of Sensors"^^xsd:string ;
    ns2:hasEventType "Exploitive"^^xsd:string ;
    ns2:hasIndustry "Retail Trade"^^xsd:string ;
    ns2:hasMonth 2 ;
    ns2:hasOrganization "Sears"^^xsd:string ;
    ns2:hasState "Illinois"^^xsd:string ;
    ns2:hasYear 2014 ;
    ns2:isType_of ns2:Criminal,
        ns2:Exploitation_of_Sensors ;
    rdfs:comment "Sears Holdings Corp. (SHLD), investigates a possible security breach after the trail of cyberattacks on other retailers (such as Target)."^^xsd:string .

ns2:f2019e8b2ba452f3 a ns2:AnonymousAttack,
        owl:NamedIndividual ;
    ns1:associatedCampaigns ns2:Danske_Bank ;
    ns1:description "Protest"^^xsd:string ;
    ns1:isLaunchedBy ns2:Norway ;
    ns2:behaviour ns2:Protest ;
    ns2:hasActor "Anonymous (Norway)"^^xsd:string ;
    ns2:hasActorCountry "Norway"^^xsd:string ;
    ns2:hasActorType "Hacktivist"^^xsd:string ;
    ns2:hasCountry "Norway"^^xsd:string ;
    ns2:hasEventDate "2014-07-09T00:00:00"^^xsd:dateTime ;
    ns2:hasEventSubtype "External Denial of Service"^^xsd:string ;
    ns2:hasEventType "Disruptive"^^xsd:string ;
    ns2:hasIndustry "Finance and Insurance"^^xsd:string ;
    ns2:hasMonth 7 ;
    ns2:hasOrganization "Danske Bank"^^xsd:string ;
    ns2:hasYear 2014 ;
    ns2:isType_of ns2:External_Denial_of_Service,
        ns2:Hacktivist ;
    rdfs:comment "Anonymous Norway starts multiple DDoS attacks towards major banks and insurance companies in Norway, including the country's largest telecommunications company, Telenor."^^xsd:string .

ns2:f296db6a1b32cbb3 a ns2:BreachUser,
        owl:NamedIndividual ;
    ns1:associatedCampaigns ns2:MeetMe ;
    ns2:hasActorType "Criminal"^^xsd:string ;
    ns2:hasCampaign ns2:Pennsylvania ;
    ns2:hasCountry "United States of America"^^xsd:string ;
    ns2:hasCounty "Bucks"^^xsd:string ;
    ns2:hasEventDate "2014-08-21T00:00:00"^^xsd:dateTime ;
    ns2:hasEventSubtype "Exploitation of Application Server"^^xsd:string ;
    ns2:hasEventType "Exploitive"^^xsd:string ;
    ns2:hasIndustry "Information"^^xsd:string ;
    ns2:hasMonth 8 ;
    ns2:hasOrganization "MeetMe"^^xsd:string ;
    ns2:hasState "Pennsylvania"^^xsd:string ;
    ns2:hasYear 2014 ;
    ns2:isType_of ns2:Criminal,
        ns2:Exploitation_of_Application_Server ;
    rdfs:comment "MeetMe users logging into the social network between Aug. 5 and Aug. 7 are asked to change their password after unknown hackers breach the MeetMe network and compromised certain user information."^^xsd:string .

ns2:f307b97dea0cf436 a ns2:HackUsernames,
        ns2:HackerSecurity,
        owl:NamedIndividual ;
    ns1:associatedCampaigns ns2:tutorialized_com ;
    ns2:hasActor "SE2mhZVVY7HF4VEV0cOH"^^xsd:string ;
    ns2:hasCountry "United States of America"^^xsd:string ;
    ns2:hasEventDate "2014-04-15T00:00:00"^^xsd:dateTime ;
    ns2:hasEventSubtype "Exploitation of Application Server"^^xsd:string ;
    ns2:hasEventType "Exploitive"^^xsd:string ;
    ns2:hasIndustry "Information"^^xsd:string ;
    ns2:hasMonth 4 ;
    ns2:hasOrganization "tutorialized.com"^^xsd:string ;
    ns2:hasYear 2014 ;
    ns2:isType_of ns2:Exploitation_of_Application_Server ;
    rdfs:comment "A hacker called SE2mhZVVY7HF4VEV0cOH hacks tutorialized.com and dumps 46244 usernames and hashed passwords."^^xsd:string .

ns2:f46392ca819868e4 a ns2:Malware,
        owl:NamedIndividual ;
    ns1:associatedCampaigns ns2:Power_Equipment_Direct ;
    ns1:description "Financial"^^xsd:string ;
    ns2:behaviour ns2:Financial ;
    ns2:hasActorType "Criminal"^^xsd:string ;
    ns2:hasCampaign ns2:Illinois ;
    ns2:hasCountry "United States of America"^^xsd:string ;
    ns2:hasCounty "Will"^^xsd:string ;
    ns2:hasEventDate "2014-06-02T00:00:00"^^xsd:dateTime ;
    ns2:hasEventSubtype "Exploitation of Application Server"^^xsd:string ;
    ns2:hasEventType "Exploitive"^^xsd:string ;
    ns2:hasIndustry "Retail Trade"^^xsd:string ;
    ns2:hasMonth 6 ;
    ns2:hasOrganization "Power Equipment Direct"^^xsd:string ;
    ns2:hasState "Illinois"^^xsd:string ;
    ns2:hasYear 2014 ;
    ns2:isType_of ns2:Criminal,
        ns2:Exploitation_of_Application_Server ;
    rdfs:comment "Power Equipment Direct (PED) notifies an undisclosed number of customers that their personal information may have been accessed when the server that handles the company's checkout process was infected with malware."^^xsd:string .

ns2:f4c56847ff5ae76a a ns2:HackerSecurity,
        owl:NamedIndividual ;
    ns1:associatedCampaigns ns2:Perl_Blogs ;
    ns1:description "Protest"^^xsd:string ;
    ns1:isLaunchedBy ns2:Iran__Islamic_Republic_of ;
    ns2:behaviour ns2:Protest ;
    ns2:hasActor "Islamic Cyber Resistance"^^xsd:string ;
    ns2:hasActorCountry "Iran (Islamic Republic of)"^^xsd:string ;
    ns2:hasActorType "Hacktivist"^^xsd:string ;
    ns2:hasCountry "United States of America"^^xsd:string ;
    ns2:hasEventDate "2014-01-22T00:00:00"^^xsd:dateTime ;
    ns2:hasEventSubtype "Message Manipulation,Exploitation of Application Server"^^xsd:string ;
    ns2:hasEventType "Mixed"^^xsd:string ;
    ns2:hasIndustry "Other Services (except Public Administration)"^^xsd:string ;
    ns2:hasMonth 1 ;
    ns2:hasOrganization "Perl Blogs"^^xsd:string ;
    ns2:hasYear 2014 ;
    ns2:isType_of ns2:Hacktivist,
        ns2:Message_Manipulation_Exploitation_of_App ;
    rdfs:comment "The Islamic Cyber Resistance (ICR) hacks the official Perl blogs (blogs.perl.org) and dumps 2,924 user account credentials. The official web page is also defaced."^^xsd:string .

ns2:f50cd73302ca6b17 a ns2:CyberattackData,
        owl:NamedIndividual ;
    ns1:associatedCampaigns ns2:Xbox_Twitter_account ;
    ns1:isLaunchedBy ns2:Syrian_Arab_Republic ;
    ns2:hasActor "Syrian Electronic Army"^^xsd:string ;
    ns2:hasActorCountry "Syrian Arab Republic"^^xsd:string ;
    ns2:hasActorType "Hacktivist"^^xsd:string ;
    ns2:hasCampaign ns2:Washington ;
    ns2:hasCountry "United States of America"^^xsd:string ;
    ns2:hasCounty "King"^^xsd:string ;
    ns2:hasEventDate "2014-01-13T00:00:00"^^xsd:dateTime ;
    ns2:hasEventSubtype "Message Manipulation"^^xsd:string ;
    ns2:hasEventType "Disruptive"^^xsd:string ;
    ns2:hasIndustry "Information"^^xsd:string ;
    ns2:hasMonth 1 ;
    ns2:hasOrganization "Xbox Twitter account"^^xsd:string ;
    ns2:hasState "Washington"^^xsd:string ;
    ns2:hasYear 2014 ;
    ns2:isType_of ns2:Hacktivist,
        ns2:Message_Manipulation ;
    rdfs:comment "In the same campaign the Syrian Electronic Army hacks the Twitter Xbox Support account, the Xbox Twitter and Instagram, and Microsoft employees."^^xsd:string .

ns2:f527b22e9a675cbf a ns2:CyberattackData,
        owl:NamedIndividual ;
    ns1:associatedCampaigns ns2:Veterans_of_Foreign_Wars ;
    ns1:description "Political-Espionage"^^xsd:string ;
    ns2:behaviour ns2:Political_Espionage ;
    ns2:hasActorType "Criminal"^^xsd:string ;
    ns2:hasCampaign ns2:Missouri ;
    ns2:hasCountry "United States of America"^^xsd:string ;
    ns2:hasCounty "Jackson"^^xsd:string ;
    ns2:hasEventDate "2014-04-15T00:00:00"^^xsd:dateTime ;
    ns2:hasEventSubtype "Exploitation of Application Server"^^xsd:string ;
    ns2:hasEventType "Exploitive"^^xsd:string ;
    ns2:hasIndustry "Other Services (except Public Administration)"^^xsd:string ;
    ns2:hasMonth 4 ;
    ns2:hasOrganization "Veterans of Foreign Wars"^^xsd:string ;
    ns2:hasState "Missouri"^^xsd:string ;
    ns2:hasYear 2014 ;
    ns2:isType_of ns2:Criminal,
        ns2:Exploitation_of_Application_Server ;
    rdfs:comment "About 55,000 members of the Veterans of Foreign Wars of the United States (vfw.org) may have had personal information, including Social Security numbers, compromised after an unauthorized party gained access to a VFW web server using a remote access trojan."^^xsd:string .

ns2:f5dab08ea70d10d7 a ns2:CyberattackData,
        owl:NamedIndividual ;
    ns1:associatedCampaigns ns2:domain_me ;
    ns1:isLaunchedBy ns2:Pakistan ;
    ns2:hasActor "TeaM MaDLeeTs"^^xsd:string ;
    ns2:hasActorCountry "Pakistan"^^xsd:string ;
    ns2:hasActorType "Hacktivist"^^xsd:string ;
    ns2:hasCountry "Montenegro"^^xsd:string ;
    ns2:hasEventDate "2014-01-13T00:00:00"^^xsd:dateTime ;
    ns2:hasEventSubtype "Message Manipulation"^^xsd:string ;
    ns2:hasEventType "Disruptive"^^xsd:string ;
    ns2:hasIndustry "Professional, Scientific, and Technical Services"^^xsd:string ;
    ns2:hasMonth 1 ;
    ns2:hasOrganization "domain.me"^^xsd:string ;
    ns2:hasYear 2014 ;
    ns2:isType_of ns2:Hacktivist,
        ns2:Message_Manipulation ;
    rdfs:comment "Hackers of the Pakistani group TeaM MaDLeeTs hack the organization responsible for the registration of Montenegro domain names (domain.me). As a result of the hack, around 3,500 domain names have been hijacked and redirected to a defacement page."^^xsd:string .

ns2:f5e72d0274452379 a ns2:DDoS,
        owl:NamedIndividual ;
    ns1:associatedCampaigns ns2:Cloudflare ;
    ns2:hasActorType "Criminal"^^xsd:string ;
    ns2:hasCampaign ns2:California ;
    ns2:hasCountry "United States of America"^^xsd:string ;
    ns2:hasCounty "San Francisco"^^xsd:string ;
    ns2:hasEventDate "2014-02-11T00:00:00"^^xsd:dateTime ;
    ns2:hasEventSubtype "External Denial of Service"^^xsd:string ;
    ns2:hasEventType "Disruptive"^^xsd:string ;
    ns2:hasIndustry "Information"^^xsd:string ;
    ns2:hasMonth 2 ;
    ns2:hasOrganization "Cloudflare"^^xsd:string ;
    ns2:hasState "California"^^xsd:string ;
    ns2:hasYear 2014 ;
    ns2:isType_of ns2:Criminal,
        ns2:External_Denial_of_Service ;
    rdfs:comment "A distributed denial-of-service attack targeting Cloudflare reaches 400 gigabits per second,making it the largest DDoS attack ever recorded."^^xsd:string .

ns2:f600c49ea323f9f0 a ns2:CyberattackData,
        owl:NamedIndividual ;
    ns1:associatedCampaigns ns2:Montana_Department_of_Public_Health ;
    ns2:hasActorType "Criminal"^^xsd:string ;
    ns2:hasCampaign ns2:Montana ;
    ns2:hasCountry "United States of America"^^xsd:string ;
    ns2:hasCounty "Lewis and Clark"^^xsd:string ;
    ns2:hasEventDate "2014-06-24T00:00:00"^^xsd:dateTime ;
    ns2:hasEventSubtype "Exploitation of Application Server"^^xsd:string ;
    ns2:hasEventType "Exploitive"^^xsd:string ;
    ns2:hasIndustry "Public Administration"^^xsd:string ;
    ns2:hasMonth 6 ;
    ns2:hasOrganization "Montana Department of Public Health"^^xsd:string ;
    ns2:hasState "Montana"^^xsd:string ;
    ns2:hasYear 2014 ;
    ns2:isType_of ns2:Criminal,
        ns2:Exploitation_of_Application_Server ;
    rdfs:comment "Montana officials notify 1.3 million people that their personal information could have been accessed by hackers who broke into a state health department computer server."^^xsd:string .

ns2:f637d734ed6b7016 a ns2:CyberattackData,
        owl:NamedIndividual ;
    ns1:associatedCampaigns ns2:OmegaNet ;
    ns1:description "Financial"^^xsd:string ;
    ns2:behaviour ns2:Financial ;
    ns2:hasActorType "Criminal"^^xsd:string ;
    ns2:hasCampaign ns2:New_Hampshire ;
    ns2:hasCountry "United States of America"^^xsd:string ;
    ns2:hasCounty "Merrimack"^^xsd:string ;
    ns2:hasEventDate "2014-08-10T00:00:00"^^xsd:dateTime ;
    ns2:hasEventSubtype "Exploitation of Application Server"^^xsd:string ;
    ns2:hasEventType "Exploitive"^^xsd:string ;
    ns2:hasIndustry "Information"^^xsd:string ;
    ns2:hasMonth 8 ;
    ns2:hasOrganization "OmegaNet"^^xsd:string ;
    ns2:hasState "New Hampshire"^^xsd:string ;
    ns2:hasYear 2014 ;
    ns2:isType_of ns2:Criminal,
        ns2:Exploitation_of_Application_Server ;
    rdfs:comment "OmegaNet notifies 10 businesses in New Hampshire of a malware incident that was able to capture sensitive information before it was encrypted."^^xsd:string .

ns2:f64ba2a469e60d5a a ns2:BreachInformation,
        owl:NamedIndividual ;
    ns1:associatedCampaigns ns2:DeKalb_Health ;
    ns1:description "Financial"^^xsd:string ;
    ns2:behaviour ns2:Financial ;
    ns2:hasActorType "Criminal"^^xsd:string ;
    ns2:hasCampaign ns2:Indiana ;
    ns2:hasCountry "United States of America"^^xsd:string ;
    ns2:hasCounty "Dekalb"^^xsd:string ;
    ns2:hasEventDate "2014-04-29T00:00:00"^^xsd:dateTime ;
    ns2:hasEventSubtype "Exploitation of Application Server"^^xsd:string ;
    ns2:hasEventType "Exploitive"^^xsd:string ;
    ns2:hasIndustry "Health Care and Social Assistance"^^xsd:string ;
    ns2:hasMonth 4 ;
    ns2:hasOrganization "DeKalb Health"^^xsd:string ;
    ns2:hasState "Indiana"^^xsd:string ;
    ns2:hasYear 2014 ;
    ns2:isType_of ns2:Criminal,
        ns2:Exploitation_of_Application_Server ;
    rdfs:comment "Dekalb Health notifies that 1,361 records including a mix of names, Social Security numbers, dates of birth, credit card numbers, addresses, phone numbers, passwords, email addresses, insurance information, service types, and other details have been compromised."^^xsd:string .

ns2:f6e7cbfb539e98b7 a ns2:Phishing,
        owl:NamedIndividual ;
    ns1:associatedCampaigns ns2:askmen_com ;
    ns2:hasActorType "Criminal"^^xsd:string ;
    ns2:hasCountry "United States of America"^^xsd:string ;
    ns2:hasEventDate "2014-06-23T00:00:00"^^xsd:dateTime ;
    ns2:hasEventSubtype "Exploitation of Application Server"^^xsd:string ;
    ns2:hasEventType "Exploitive"^^xsd:string ;
    ns2:hasIndustry "Information"^^xsd:string ;
    ns2:hasMonth 6 ;
    ns2:hasOrganization "askmen.com"^^xsd:string ;
    ns2:hasYear 2014 ;
    ns2:isType_of ns2:Criminal,
        ns2:Exploitation_of_Application_Server ;
    rdfs:comment "askmen.com, a portal with more than 14 million readers in the US alone, is the victim of a mass-injection attack with multiple versions of the official website compromised to serve malware to its visitors."^^xsd:string .

ns2:f913a3c729d50c61 a ns2:EmailPhishing,
        owl:NamedIndividual ;
    ns1:associatedCampaigns ns2:Midwest_Orthopaedics ;
    ns2:hasActorType "Criminal"^^xsd:string ;
    ns2:hasCampaign ns2:Illinois ;
    ns2:hasCountry "United States of America"^^xsd:string ;
    ns2:hasCounty "Cook"^^xsd:string ;
    ns2:hasEventDate "2014-04-08T00:00:00"^^xsd:dateTime ;
    ns2:hasEventSubtype "Exploitation of Application Server"^^xsd:string ;
    ns2:hasEventType "Exploitive"^^xsd:string ;
    ns2:hasIndustry "Health Care and Social Assistance"^^xsd:string ;
    ns2:hasMonth 4 ;
    ns2:hasOrganization "Midwest Orthopaedics"^^xsd:string ;
    ns2:hasState "Illinois"^^xsd:string ;
    ns2:hasYear 2014 ;
    ns2:isType_of ns2:Criminal,
        ns2:Exploitation_of_Application_Server ;
    rdfs:comment "More than 1,200 patients of Chicago-based Midwest Orthopaedics at Rush (MOR) may have had personal information compromised after an unknown individual gained unauthorized access to a doctor's personal email account, which contained the data."^^xsd:string .

ns2:fa5aad7d08e246ba a ns2:AttackWebsite,
        owl:NamedIndividual ;
    ns1:associatedCampaigns ns2:Shaqra_Principality ;
    ns1:description "Protest"^^xsd:string ;
    ns1:isLaunchedBy ns2:Syrian_Arab_Republic ;
    ns2:behaviour ns2:Protest ;
    ns2:hasActor "Syrian Electronic Army"^^xsd:string ;
    ns2:hasActorCountry "Syrian Arab Republic"^^xsd:string ;
    ns2:hasActorType "Hacktivist"^^xsd:string ;
    ns2:hasCountry "Saudi Arabia"^^xsd:string ;
    ns2:hasEventDate "2014-01-16T00:00:00"^^xsd:dateTime ;
    ns2:hasEventSubtype "Message Manipulation"^^xsd:string ;
    ns2:hasEventType "Disruptive"^^xsd:string ;
    ns2:hasIndustry "Public Administration"^^xsd:string ;
    ns2:hasMonth 1 ;
    ns2:hasOrganization "Shaqra Principality"^^xsd:string ;
    ns2:hasYear 2014 ;
    ns2:isType_of ns2:Hacktivist,
        ns2:Message_Manipulation ;
    rdfs:comment "The Syrian Electronic Army deface 16 Saudi Arabian government websites. The targeted sites are the ones of various administrative regions."^^xsd:string .

ns2:fac1a37b1776545f a ns2:HackerSecurity,
        owl:NamedIndividual ;
    ns1:associatedCampaigns ns2:Auburn_University ;
    ns2:hasActorType "Criminal"^^xsd:string ;
    ns2:hasCampaign ns2:Alabama ;
    ns2:hasCountry "United States of America"^^xsd:string ;
    ns2:hasCounty "Lee"^^xsd:string ;
    ns2:hasEventDate "2014-03-21T00:00:00"^^xsd:dateTime ;
    ns2:hasEventSubtype "Exploitation of Application Server"^^xsd:string ;
    ns2:hasEventType "Exploitive"^^xsd:string ;
    ns2:hasIndustry "Educational Services"^^xsd:string ;
    ns2:hasMonth 3 ;
    ns2:hasOrganization "Auburn University"^^xsd:string ;
    ns2:hasState "Alabama"^^xsd:string ;
    ns2:hasYear 2014 ;
    ns2:isType_of ns2:Criminal,
        ns2:Exploitation_of_Application_Server ;
    rdfs:comment "An unidentified hacker accesses a compromised server on Auburn University College of Business server that contained personal information allegedly compromising the information of about 14,000 current and former students, faculty and staff."^^xsd:string .

ns2:fbcef4ce517e64de a ns2:AccessSecurity,
        owl:NamedIndividual ;
    ns1:associatedCampaigns ns2:Olmsted_Medical_Center ;
    ns2:hasActorType "Criminal"^^xsd:string ;
    ns2:hasCampaign ns2:Minnesota ;
    ns2:hasCountry "United States of America"^^xsd:string ;
    ns2:hasCounty "Olmsted"^^xsd:string ;
    ns2:hasEventDate "2014-02-03T00:00:00"^^xsd:dateTime ;
    ns2:hasEventSubtype "Exploitation of Application Server"^^xsd:string ;
    ns2:hasEventType "Exploitive"^^xsd:string ;
    ns2:hasIndustry "Health Care and Social Assistance"^^xsd:string ;
    ns2:hasMonth 2 ;
    ns2:hasOrganization "Olmsted Medical Center"^^xsd:string ;
    ns2:hasState "Minnesota"^^xsd:string ;
    ns2:hasYear 2014 ;
    ns2:isType_of ns2:Criminal,
        ns2:Exploitation_of_Application_Server ;
    rdfs:comment "The employee database of the Olmsted Medical Center is unlawfully accessed, exposing the information of about 500 employees."^^xsd:string .

ns2:fd6e79daffb0b490 a ns2:CyberattackSystem,
        owl:NamedIndividual ;
    ns1:associatedCampaigns ns2:Indian_Ministry_of_Railways ;
    ns1:isLaunchedBy ns2:India ;
    ns2:hasActor "rOOX"^^xsd:string ;
    ns2:hasActorCountry "India"^^xsd:string ;
    ns2:hasActorType "Hacktivist"^^xsd:string ;
    ns2:hasCountry "India"^^xsd:string ;
    ns2:hasEventDate "2014-05-11T00:00:00"^^xsd:dateTime ;
    ns2:hasEventSubtype "Message Manipulation"^^xsd:string ;
    ns2:hasEventType "Disruptive"^^xsd:string ;
    ns2:hasIndustry "Transportation and Warehousing"^^xsd:string ;
    ns2:hasMonth 5 ;
    ns2:hasOrganization "Indian Ministry of Railways"^^xsd:string ;
    ns2:hasYear 2014 ;
    ns2:isType_of ns2:Hacktivist,
        ns2:Message_Manipulation ;
    rdfs:comment "Another episode of the Cyber War between India and Pakistan. A Pakistani hacker called rOOX from Team MadLeets defaces the server of Indian Ministry of Railway, which includes around 47 domains."^^xsd:string .

ns2:fd80685909d97d48 a ns2:CyberattackData,
        owl:NamedIndividual ;
    ns1:associatedCampaigns ns2:knowledgeicon_com ;
    ns2:hasActorType "Criminal"^^xsd:string ;
    ns2:hasCountry "India"^^xsd:string ;
    ns2:hasEventDate "2014-04-14T00:00:00"^^xsd:dateTime ;
    ns2:hasEventSubtype "Exploitation of Application Server"^^xsd:string ;
    ns2:hasEventType "Exploitive"^^xsd:string ;
    ns2:hasIndustry "Educational Services"^^xsd:string ;
    ns2:hasMonth 4 ;
    ns2:hasOrganization "knowledgeicon.com"^^xsd:string ;
    ns2:hasYear 2014 ;
    ns2:isType_of ns2:Criminal,
        ns2:Exploitation_of_Application_Server ;
    rdfs:comment "In name of OpKashmir an unknown hacker hacks knowledgeicon.com and dumps 911 email addresses and other personal data."^^xsd:string .

ns2:fe0aa6473cf8e788 a ns2:AttackWebsite,
        owl:NamedIndividual ;
    ns1:associatedCampaigns ns2:Almuzamiyah_Principality ;
    ns1:description "Protest"^^xsd:string ;
    ns1:isLaunchedBy ns2:Syrian_Arab_Republic ;
    ns2:behaviour ns2:Protest ;
    ns2:hasActor "Syrian Electronic Army"^^xsd:string ;
    ns2:hasActorCountry "Syrian Arab Republic"^^xsd:string ;
    ns2:hasActorType "Hacktivist"^^xsd:string ;
    ns2:hasCountry "Saudi Arabia"^^xsd:string ;
    ns2:hasEventDate "2014-01-16T00:00:00"^^xsd:dateTime ;
    ns2:hasEventSubtype "Message Manipulation"^^xsd:string ;
    ns2:hasEventType "Disruptive"^^xsd:string ;
    ns2:hasIndustry "Public Administration"^^xsd:string ;
    ns2:hasMonth 1 ;
    ns2:hasOrganization "Almuzamiyah Principality"^^xsd:string ;
    ns2:hasYear 2014 ;
    ns2:isType_of ns2:Hacktivist,
        ns2:Message_Manipulation ;
    rdfs:comment "The Syrian Electronic Army deface 16 Saudi Arabian government websites. The targeted sites are the ones of various administrative regions."^^xsd:string .

ns2:fe7b2fd7c4b09e8f a ns2:HackerSecurity,
        owl:NamedIndividual ;
    ns1:associatedCampaigns ns2:Turkcell ;
    ns1:description "Protest"^^xsd:string ;
    ns1:isLaunchedBy ns2:Turkey ;
    ns2:behaviour ns2:Protest ;
    ns2:hasActor "RedHack"^^xsd:string ;
    ns2:hasActorCountry "Turkey"^^xsd:string ;
    ns2:hasActorType "Hacktivist"^^xsd:string ;
    ns2:hasCountry "Turkey"^^xsd:string ;
    ns2:hasEventDate "2014-01-16T00:00:00"^^xsd:dateTime ;
    ns2:hasEventSubtype "Exploitation of End Hosts"^^xsd:string ;
    ns2:hasEventType "Exploitive"^^xsd:string ;
    ns2:hasIndustry "Information"^^xsd:string ;
    ns2:hasMonth 1 ;
    ns2:hasOrganization "Turkcell"^^xsd:string ;
    ns2:hasYear 2014 ;
    ns2:isType_of ns2:Exploitation_of_End_Hosts,
        ns2:Hacktivist ;
    rdfs:comment "Hackers of the RedHack collective leak the phone numbers of over 4,000 people who work for Turkcell, the leading mobile phone operator of Turkey."^^xsd:string .

ns2:feec950ff1c3416a a ns2:HackerSecurity,
        owl:NamedIndividual ;
    ns1:associatedCampaigns ns2:Israeli_Defense_Ministry ;
    ns1:description "Political-Espionage"^^xsd:string ;
    ns2:behaviour ns2:Political_Espionage ;
    ns2:hasActorType "Criminal"^^xsd:string ;
    ns2:hasCountry "Israel"^^xsd:string ;
    ns2:hasEventDate "2014-01-26T00:00:00"^^xsd:dateTime ;
    ns2:hasEventSubtype "Exploitation of End Hosts"^^xsd:string ;
    ns2:hasEventType "Exploitive"^^xsd:string ;
    ns2:hasIndustry "Public Administration"^^xsd:string ;
    ns2:hasMonth 1 ;
    ns2:hasOrganization "Israeli Defense Ministry"^^xsd:string ;
    ns2:hasYear 2014 ;
    ns2:isType_of ns2:Criminal,
        ns2:Exploitation_of_End_Hosts ;
    rdfs:comment "Earlier in January, unknown hackers break into an Israeli defense ministry computer via an email attachment tainted with malicious software looking like it had been sent by the country's Shin Bet secret security service."^^xsd:string .

ns2:hasActor a owl:DatatypeProperty ;
    rdfs:domain ns1:Attack,
        ns1:UCOThing ;
    rdfs:range xsd:string ;
    rdfs:subPropertyOf owl:topDataProperty .

ns2:hasActorCountry a owl:DatatypeProperty ;
    rdfs:domain ns1:Attacker,
        ns1:UCOThing ;
    rdfs:range xsd:string ;
    rdfs:subPropertyOf owl:topDataProperty .

ns2:hasActorType a owl:DatatypeProperty ;
    rdfs:domain ns1:Attacker,
        ns1:UCOThing ;
    rdfs:range xsd:string ;
    rdfs:subPropertyOf owl:topDataProperty .

ns2:hasCountry a owl:DatatypeProperty ;
    rdfs:domain ns1:Attack,
        ns1:UCOThing ;
    rdfs:range xsd:string ;
    rdfs:subPropertyOf owl:topDataProperty .

ns2:hasCounty a owl:DatatypeProperty ;
    rdfs:domain ns1:Attack,
        ns1:UCOThing ;
    rdfs:range xsd:string ;
    rdfs:subPropertyOf owl:topDataProperty .

ns2:hasDescription a owl:DatatypeProperty ;
    rdfs:domain ns1:Attack,
        ns1:UCOThing ;
    rdfs:range xsd:string ;
    rdfs:subPropertyOf owl:topDataProperty .

ns2:hasEventDate a owl:DatatypeProperty ;
    rdfs:domain ns1:Incident,
        ns1:UCOThing ;
    rdfs:range xsd:dateTime ;
    rdfs:subPropertyOf owl:topDataProperty .

ns2:hasEventSubtype a owl:DatatypeProperty ;
    rdfs:domain ns1:Incident,
        ns1:UCOThing ;
    rdfs:range xsd:string ;
    rdfs:subPropertyOf owl:topDataProperty .

ns2:hasEventType a owl:DatatypeProperty ;
    rdfs:domain ns1:Incident,
        ns1:UCOThing ;
    rdfs:range xsd:string ;
    rdfs:subPropertyOf owl:topDataProperty .

ns2:hasIndustry a owl:DatatypeProperty ;
    rdfs:domain ns1:Incident,
        ns1:UCOThing ;
    rdfs:range xsd:string ;
    rdfs:subPropertyOf owl:topDataProperty .

ns2:hasMonth a owl:DatatypeProperty ;
    rdfs:domain ns1:Incident,
        ns1:UCOThing ;
    rdfs:range xsd:integer ;
    rdfs:subPropertyOf owl:topDataProperty .

ns2:hasMotive a owl:DatatypeProperty ;
    rdfs:domain ns1:Attack,
        ns1:UCOThing ;
    rdfs:range xsd:string ;
    rdfs:subPropertyOf owl:topDataProperty .

ns2:hasOrganization a owl:DatatypeProperty ;
    rdfs:domain ns1:Incident,
        ns1:UCOThing ;
    rdfs:range xsd:string ;
    rdfs:subPropertyOf owl:topDataProperty .

ns2:hasSourceURL a owl:DatatypeProperty ;
    rdfs:domain ns1:Attack ;
    rdfs:range xsd:anyURI ;
    rdfs:subPropertyOf owl:topDataProperty .

ns2:hasState a owl:DatatypeProperty ;
    rdfs:domain ns1:Attack,
        ns1:UCOThing ;
    rdfs:range xsd:string ;
    rdfs:subPropertyOf owl:topDataProperty .

ns2:hasTime a owl:DatatypeProperty ;
    rdfs:domain ns1:Attack,
        ns1:UCOThing ;
    rdfs:range xsd:dateTime .

ns2:hasTitle a owl:DatatypeProperty ;
    rdfs:domain ns1:Attacker,
        ns1:Campaign,
        ns1:Consequence,
        ns1:CourseofAction,
        ns1:Means,
        ns1:Vulnerability,
        ns2:Indicator ;
    rdfs:range xsd:string ;
    rdfs:subPropertyOf ns1:hasVendor .

ns2:hasYear a owl:DatatypeProperty ;
    rdfs:domain ns1:Incident,
        ns1:UCOThing ;
    rdfs:range xsd:integer ;
    rdfs:subPropertyOf owl:topDataProperty .

<http://cybox.mitre.org/cybox_v1#Observable> a owl:Class ;
    rdfs:comment "Formal definition for Observable within the cybersecurity domain."^^xsd:string ;
    rdfs:subClassOf ns1:UCOThing ;
    owl:equivalentClass ns1:Observable .

<http://ffrdc.ebiquity.umbc.edu/ns/ontology> a owl:Ontology ;
    owl:versionIRI <http://ffrdc.ebiquity.umbc.edu/ns/ontology> .

ns1:Backdoor a owl:Class ;
    rdfs:comment "Formal definition for Backdoor within the cybersecurity domain."^^xsd:string ;
    rdfs:subClassOf [ a owl:Restriction ;
            owl:onProperty ns1:resultsIn ;
            owl:someValuesFrom ns1:RemoteAccess ],
        ns1:MaliciousCodeExecution .

ns1:IDPS a owl:Class ;
    rdfs:comment "Formal definition for IDPS within the cybersecurity domain."^^xsd:string ;
    rdfs:subClassOf ns1:Source .

ns1:Logic a owl:Class ;
    rdfs:comment "Formal definition for Logic within the cybersecurity domain."^^xsd:string ;
    rdfs:subClassOf ns1:TriggeredCode .

ns1:MitnickAttack a owl:Class ;
    rdfs:comment "Formal definition for MitnickAttack within the cybersecurity domain."^^xsd:string ;
    rdfs:seeAlso "http://dbpedia.org/resource/The_Art_of_Intrusion"^^xsd:anyURI ;
    rdfs:subClassOf ns1:Consequence .

ns1:NetFlood a owl:Class ;
    rdfs:comment "Formal definition for NetFlood within the cybersecurity domain."^^xsd:string ;
    rdfs:seeAlso "http://dbpedia.org/describe/?url=http%3A%2F%2Fsw.opencyc.org%2F2008%2F06%2F10%2Fconcept%2Fen%2FTribeFloodNet_DenialOfServiceProgram&sid=7707"^^xsd:anyURI ;
    rdfs:subClassOf ns1:DenialOfService .

ns1:affectsProduct a owl:ObjectProperty ;
    rdfs:domain ns1:Vulnerability ;
    rdfs:range ns1:Product ;
    owl:inverseOf ns2:is_affectsProduct_of .

ns1:associatedCampaigns a owl:ObjectProperty ;
    rdfs:domain ns1:Campaign ;
    rdfs:range ns1:Campaign ;
    owl:inverseOf ns2:is_associatedCampaigns_of .

ns1:exploitsVulnerability a owl:ObjectProperty ;
    rdfs:domain ns1:Means ;
    rdfs:range ns1:Vulnerability ;
    owl:inverseOf ns2:is_exploitsVulnerability_of .

ns1:hasIPv4Address a owl:ObjectProperty ;
    rdfs:domain owl:Thing ;
    rdfs:range owl:Thing ;
    rdfs:subPropertyOf ns1:hasIPAddress ;
    owl:inverseOf ns2:isIPv4Address_of .

ns1:hasIPv6Address a owl:ObjectProperty ;
    rdfs:domain owl:Thing ;
    rdfs:range owl:Thing ;
    rdfs:subPropertyOf ns1:hasIPAddress ;
    owl:inverseOf ns2:isIPv6Address_of .

ns1:hasInformationSource a owl:ObjectProperty ;
    rdfs:domain owl:Thing ;
    rdfs:range owl:Thing ;
    rdfs:subPropertyOf owl:topObjectProperty ;
    owl:inverseOf ns2:isInformationSource_of .

ns1:hasMACAddress a owl:DatatypeProperty,
        owl:FunctionalProperty,
        owl:ObjectProperty ;
    rdfs:domain ns1:System ;
    rdfs:range xsd:string ;
    rdfs:subPropertyOf owl:topObjectProperty ;
    owl:inverseOf ns2:isMACAddress_of .

ns1:hasMitigation a owl:ObjectProperty ;
    rdfs:domain ns1:Vulnerability ;
    rdfs:range ns1:CourseofAction ;
    owl:inverseOf ns2:isMitigation_of .

ns1:hasProduct a owl:ObjectProperty ;
    rdfs:domain ns1:System ;
    rdfs:range ns1:Product ;
    owl:inverseOf ns2:isProduct_of .

ns1:hasSource a owl:DatatypeProperty,
        owl:ObjectProperty ;
    rdfs:domain ns1:Attack,
        ns1:Vulnerability ;
    rdfs:range ns1:Source ;
    rdfs:subPropertyOf ns1:hasSeverityScore ;
    owl:inverseOf ns2:isSource_of .

ns1:hasTerms a owl:FunctionalProperty,
        owl:ObjectProperty ;
    rdfs:domain ns1:Web ;
    rdfs:range ns1:OtherTechnicalTerms ;
    owl:inverseOf ns2:isTerms_of .

ns1:hasVendor a owl:DatatypeProperty ;
    rdfs:domain ns1:Product ;
    rdfs:range xsd:string .

ns1:hasVulnerability a owl:ObjectProperty ;
    rdfs:domain ns1:ExploitTarget,
        ns1:Means,
        ns1:Product ;
    rdfs:range ns1:Vulnerability ;
    owl:inverseOf ns2:isVulnerability_of .

ns1:isLaunchedBy a owl:ObjectProperty ;
    rdfs:domain ns1:Attack,
        ns1:Campaign ;
    rdfs:range ns1:Attacker ;
    owl:inverseOf ns2:is_isLaunchedBy_of .

ns1:isUnderAttack a owl:IrreflexiveProperty,
        owl:ObjectProperty ;
    rdfs:domain ns1:System ;
    rdfs:range ns1:Attack,
        ns1:Consequence ;
    owl:inverseOf ns2:is_isUnderAttack_of .

ns2:40dni_sk a owl:NamedIndividual,
        owl:Thing ;
    rdfs:comment "Entity representing 40dni.sk"^^xsd:string .

ns2:4chan a owl:NamedIndividual,
        owl:Thing ;
    rdfs:comment "Entity representing 4chan"^^xsd:string .

ns2:AECOM a owl:NamedIndividual,
        owl:Thing ;
    rdfs:comment "Entity representing AECOM"^^xsd:string .

ns2:AOL_Mail a owl:NamedIndividual,
        owl:Thing ;
    rdfs:comment "Entity representing AOL Mail"^^xsd:string .

ns2:ARY_News a owl:NamedIndividual,
        owl:Thing ;
    rdfs:comment "Entity representing ARY News"^^xsd:string .

ns2:AT_T a owl:NamedIndividual,
        owl:Thing ;
    rdfs:comment "Entity representing AT&T"^^xsd:string .

ns2:AVG a owl:NamedIndividual,
        owl:Thing ;
    rdfs:comment "Entity representing AVG"^^xsd:string .

ns2:AVS_TV a owl:NamedIndividual,
        owl:Thing ;
    rdfs:comment "Entity representing AVS TV"^^xsd:string .

ns2:Affinity_Gaming a owl:NamedIndividual,
        owl:Thing ;
    rdfs:comment "Entity representing Affinity Gaming"^^xsd:string .

ns2:Afghanistan a ns1:ThreatActor,
        owl:NamedIndividual ;
    rdfs:comment "Entity representing Afghanistan"^^xsd:string .

ns2:Air_France a owl:NamedIndividual,
        owl:Thing ;
    rdfs:comment "Entity representing Air France"^^xsd:string .

ns2:Aktif_Bank a owl:NamedIndividual,
        owl:Thing ;
    rdfs:comment "Entity representing Aktif Bank"^^xsd:string .

ns2:Al_Arabiya a owl:NamedIndividual,
        owl:Thing ;
    rdfs:comment "Entity representing Al Arabiya"^^xsd:string .

ns2:Alabama a owl:NamedIndividual,
        owl:Thing ;
    rdfs:comment "Entity representing Alabama"^^xsd:string .

ns2:Alaska a owl:NamedIndividual,
        owl:Thing ;
    rdfs:comment "Entity representing Alaska"^^xsd:string .

ns2:Alaska_Communications a owl:NamedIndividual,
        owl:Thing ;
    rdfs:comment "Entity representing Alaska Communications"^^xsd:string .

ns2:Albuquerque_Police_Department a owl:NamedIndividual,
        owl:Thing ;
    rdfs:comment "Entity representing Albuquerque Police Department"^^xsd:string .

ns2:Aldoriyah_Principality a owl:NamedIndividual,
        owl:Thing ;
    rdfs:comment "Entity representing Aldoriyah Principality"^^xsd:string .

ns2:Alduwadimi_Principality a owl:NamedIndividual,
        owl:Thing ;
    rdfs:comment "Entity representing Alduwadimi Principality"^^xsd:string .

ns2:AlfaNet a owl:NamedIndividual,
        owl:Thing ;
    rdfs:comment "Entity representing AlfaNet"^^xsd:string .

ns2:Alghat_Principality a owl:NamedIndividual,
        owl:Thing ;
    rdfs:comment "Entity representing Alghat Principality"^^xsd:string .

ns2:Alikhbaria a owl:NamedIndividual,
        owl:Thing ;
    rdfs:comment "Entity representing Alikhbaria"^^xsd:string .

ns2:Alipay a owl:NamedIndividual,
        owl:Thing ;
    rdfs:comment "Entity representing Alipay"^^xsd:string .

ns2:Almajmah_Principality a owl:NamedIndividual,
        owl:Thing ;
    rdfs:comment "Entity representing Almajmah Principality"^^xsd:string .

ns2:Almuzamiyah_Principality a owl:NamedIndividual,
        owl:Thing ;
    rdfs:comment "Entity representing Almuzamiyah Principality"^^xsd:string .

ns2:Alohtah_Principality a owl:NamedIndividual,
        owl:Thing ;
    rdfs:comment "Entity representing Alohtah Principality"^^xsd:string .

ns2:Alquwayiyah_Principality a owl:NamedIndividual,
        owl:Thing ;
    rdfs:comment "Entity representing Alquwayiyah Principality"^^xsd:string .

ns2:Alshariq_Principality a owl:NamedIndividual,
        owl:Thing ;
    rdfs:comment "Entity representing Alshariq Principality"^^xsd:string .

ns2:American_Institutes_for_Research a owl:NamedIndividual,
        owl:Thing ;
    rdfs:comment "Entity representing American Institutes for Research"^^xsd:string .

ns2:Ankara_Chamber_of_Industry a owl:NamedIndividual,
        owl:Thing ;
    rdfs:comment "Entity representing Ankara Chamber of Industry"^^xsd:string .

ns2:Anonymous a owl:NamedIndividual,
        owl:Thing ;
    rdfs:comment "Entity representing Anonymous"^^xsd:string .

ns2:Areva a owl:NamedIndividual,
        owl:Thing ;
    rdfs:comment "Entity representing Areva"^^xsd:string .

ns2:Ariana_Grande a owl:NamedIndividual,
        owl:Thing ;
    rdfs:comment "Entity representing Ariana Grande"^^xsd:string .

ns2:Arizona_Department_of_Homeland_Security a owl:NamedIndividual,
        owl:Thing ;
    rdfs:comment "Entity representing Arizona Department of Homeland Security"^^xsd:string .

ns2:Arkansas a owl:NamedIndividual,
        owl:Thing ;
    rdfs:comment "Entity representing Arkansas"^^xsd:string .

ns2:Arkansas_State_University a owl:NamedIndividual,
        owl:Thing ;
    rdfs:comment "Entity representing Arkansas State University"^^xsd:string .

ns2:Armed_Forces_Training_Authority a owl:NamedIndividual,
        owl:Thing ;
    rdfs:comment "Entity representing Armed Forces Training Authority"^^xsd:string .

ns2:Armenian_President_Website a owl:NamedIndividual,
        owl:Thing ;
    rdfs:comment "Entity representing Armenian President Website"^^xsd:string .

ns2:Artsakh_State_University a owl:NamedIndividual,
        owl:Thing ;
    rdfs:comment "Entity representing Artsakh State University"^^xsd:string .

ns2:Assisted_Living_Concepts a owl:NamedIndividual,
        owl:Thing ;
    rdfs:comment "Entity representing Assisted Living Concepts"^^xsd:string .

ns2:Association_of_Corporate_Travel_Executiv a owl:NamedIndividual,
        owl:Thing ;
    rdfs:comment "Entity representing Association of Corporate Travel Executives"^^xsd:string .

ns2:Ateneo_Integrated_Student_Information_Sy a owl:NamedIndividual,
        owl:Thing ;
    rdfs:comment "Entity representing Ateneo Integrated Student Information System"^^xsd:string .

ns2:AttackGroup a owl:Class ;
    rdfs:label "attack group"^^xsd:string ;
    rdfs:comment "Formal definition for AttackGroup within the cybersecurity domain."^^xsd:string ;
    rdfs:subClassOf ns2:AttackPattern .

ns2:AttackSecurity a owl:Class ;
    rdfs:label "attack security"^^xsd:string ;
    rdfs:comment "Formal definition for AttackSecurity within the cybersecurity domain."^^xsd:string ;
    rdfs:subClassOf ns2:AttackPattern .

ns2:AttackerData a owl:Class ;
    rdfs:label "attacker data"^^xsd:string ;
    rdfs:comment "Formal definition for AttackerData within the cybersecurity domain."^^xsd:string ;
    rdfs:subClassOf ns2:AttackPattern .

ns2:Auburn_University a owl:NamedIndividual,
        owl:Thing ;
    rdfs:comment "Entity representing Auburn University"^^xsd:string .

ns2:Automatic_Systems a owl:NamedIndividual,
        owl:Thing ;
    rdfs:comment "Entity representing Automatic Systems"^^xsd:string .

ns2:Autonation a owl:NamedIndividual,
        owl:Thing ;
    rdfs:comment "Entity representing Autonation"^^xsd:string .

ns2:Avast a owl:NamedIndividual,
        owl:Thing ;
    rdfs:comment "Entity representing Avast"^^xsd:string .

ns2:Azad_Kashmir_Government_Portal a owl:NamedIndividual,
        owl:Thing ;
    rdfs:comment "Entity representing Azad Kashmir Government Portal"^^xsd:string .

ns2:Bangalore_City_Police a owl:NamedIndividual,
        owl:Thing ;
    rdfs:comment "Entity representing Bangalore City Police"^^xsd:string .

ns2:Bangladesh a ns1:ThreatActor,
        owl:NamedIndividual ;
    rdfs:comment "Entity representing Bangladesh"^^xsd:string .

ns2:Bangladesh_Airport_Armed_Police a owl:NamedIndividual,
        owl:Thing ;
    rdfs:comment "Entity representing Bangladesh Airport Armed Police"^^xsd:string .

ns2:Bank_of_the_West a owl:NamedIndividual,
        owl:Thing ;
    rdfs:comment "Entity representing Bank of the West"^^xsd:string .

ns2:Barry_University a owl:NamedIndividual,
        owl:Thing ;
    rdfs:comment "Entity representing Barry University"^^xsd:string .

ns2:Bartell_Hotels a owl:NamedIndividual,
        owl:Thing ;
    rdfs:comment "Entity representing Bartell Hotels"^^xsd:string .

ns2:Basecamp a owl:NamedIndividual,
        owl:Thing ;
    rdfs:comment "Entity representing Basecamp"^^xsd:string .

ns2:Belgian_Foreign_Ministry a owl:NamedIndividual,
        owl:Thing ;
    rdfs:comment "Entity representing Belgian Foreign Ministry"^^xsd:string .

ns2:Bell_Canada a owl:NamedIndividual,
        owl:Thing ;
    rdfs:comment "Entity representing Bell Canada"^^xsd:string .

ns2:BigBoss_repository a owl:NamedIndividual,
        owl:Thing ;
    rdfs:comment "Entity representing BigBoss repository"^^xsd:string .

ns2:BigMoneyJobs_com a owl:NamedIndividual,
        owl:Thing ;
    rdfs:comment "Entity representing BigMoneyJobs.com"^^xsd:string .

ns2:Bihar_Bharatiya_Janata_Party a owl:NamedIndividual,
        owl:Thing ;
    rdfs:comment "Entity representing Bihar Bharatiya Janata Party"^^xsd:string .

ns2:Board_of_Control_for_Cricket_in_India a owl:NamedIndividual,
        owl:Thing ;
    rdfs:comment "Entity representing Board of Control for Cricket in India"^^xsd:string .

ns2:Boeing a owl:NamedIndividual,
        owl:Thing ;
    rdfs:comment "Entity representing Boeing"^^xsd:string .

ns2:Boston_Children_s_Hospital a owl:NamedIndividual,
        owl:Thing ;
    rdfs:comment "Entity representing Boston Children's Hospital"^^xsd:string .

ns2:Boston_Scientific a owl:NamedIndividual,
        owl:Thing ;
    rdfs:comment "Entity representing Boston Scientific"^^xsd:string .

ns2:Boxee_tv a owl:NamedIndividual,
        owl:Thing ;
    rdfs:comment "Entity representing Boxee.tv"^^xsd:string .

ns2:Brazil a ns1:ThreatActor,
        owl:NamedIndividual ;
    rdfs:comment "Entity representing Brazil"^^xsd:string .

ns2:Brazilian_Ministry_of_External_Relations a owl:NamedIndividual,
        owl:Thing ;
    rdfs:comment "Entity representing Brazilian Ministry of External Relations"^^xsd:string .

ns2:BreachData a owl:Class ;
    rdfs:label "breach data"^^xsd:string ;
    rdfs:comment "Formal definition for BreachData within the cybersecurity domain."^^xsd:string ;
    rdfs:subClassOf ns2:DataBreach .

ns2:British_Academy_of_Film_and_Television_A a owl:NamedIndividual,
        owl:Thing ;
    rdfs:comment "Entity representing British Academy of Film and Television Arts"^^xsd:string .

ns2:British_Gas a owl:NamedIndividual,
        owl:Thing ;
    rdfs:comment "Entity representing British Gas"^^xsd:string .

ns2:British_National_Party a owl:NamedIndividual,
        owl:Thing ;
    rdfs:comment "Entity representing British National Party"^^xsd:string .

ns2:Broadcasthe_net a owl:NamedIndividual,
        owl:Thing ;
    rdfs:comment "Entity representing Broadcasthe.net"^^xsd:string .

ns2:Bulk_Reef_Supply a owl:NamedIndividual,
        owl:Thing ;
    rdfs:comment "Entity representing Bulk Reef Supply"^^xsd:string .

ns2:Butler_University a owl:NamedIndividual,
        owl:Thing ;
    rdfs:comment "Entity representing Butler University"^^xsd:string .

ns2:CNET a owl:NamedIndividual,
        owl:Thing ;
    rdfs:comment "Entity representing CNET"^^xsd:string .

ns2:CNN a owl:NamedIndividual,
        owl:Thing ;
    rdfs:comment "Entity representing CNN"^^xsd:string .

ns2:Cabinet_Ministry_of_Pakistan a owl:NamedIndividual,
        owl:Thing ;
    rdfs:comment "Entity representing Cabinet Ministry of Pakistan"^^xsd:string .

ns2:California_Department_of_Motor_Vehicles a owl:NamedIndividual,
        owl:Thing ;
    rdfs:comment "Entity representing California Department of Motor Vehicles"^^xsd:string .

ns2:California_State_University a owl:NamedIndividual,
        owl:Thing ;
    rdfs:comment "Entity representing California State University"^^xsd:string .

ns2:Canada_Revenue_Agency a owl:NamedIndividual,
        owl:Thing ;
    rdfs:comment "Entity representing Canada Revenue Agency"^^xsd:string .

ns2:Carlo_Ancelotti a owl:NamedIndividual,
        owl:Thing ;
    rdfs:comment "Entity representing Carlo Ancelotti"^^xsd:string .

ns2:Carlson_Rezidor_Hotel_Group a owl:NamedIndividual,
        owl:Thing ;
    rdfs:comment "Entity representing Carlson Rezidor Hotel Group"^^xsd:string .

ns2:Cemig_Telecom a owl:NamedIndividual,
        owl:Thing ;
    rdfs:comment "Entity representing Cemig Telecom"^^xsd:string .

ns2:Centrais_El_tricas_do_Norte_do_Brasil a owl:NamedIndividual,
        owl:Thing ;
    rdfs:comment "Entity representing Centrais El tricas do Norte do Brasil"^^xsd:string .

ns2:Central_Bank_of_Turkey a owl:NamedIndividual,
        owl:Thing ;
    rdfs:comment "Entity representing Central Bank of Turkey"^^xsd:string .

ns2:Cerberus a owl:NamedIndividual,
        owl:Thing ;
    rdfs:comment "Entity representing Cerberus"^^xsd:string .

ns2:Certification_ESET_Spain a owl:NamedIndividual,
        owl:Thing ;
    rdfs:comment "Entity representing Certification ESET Spain"^^xsd:string .

ns2:Chevrolet a owl:NamedIndividual,
        owl:Thing ;
    rdfs:comment "Entity representing Chevrolet"^^xsd:string .

ns2:Chicago_Yacht_Club a owl:NamedIndividual,
        owl:Thing ;
    rdfs:comment "Entity representing Chicago Yacht Club"^^xsd:string .

ns2:Children_s_Mercy_Hospital a owl:NamedIndividual,
        owl:Thing ;
    rdfs:comment "Entity representing Children's Mercy Hospital"^^xsd:string .

ns2:Church_of_Cyprus a owl:NamedIndividual,
        owl:Thing ;
    rdfs:comment "Entity representing Church of Cyprus"^^xsd:string .

ns2:Church_of_Scotland a owl:NamedIndividual,
        owl:Thing ;
    rdfs:comment "Entity representing Church of Scotland"^^xsd:string .

ns2:Cirrus_Communications a owl:NamedIndividual,
        owl:Thing ;
    rdfs:comment "Entity representing Cirrus Communications"^^xsd:string .

ns2:City_To_Bay_Fun_Run a owl:NamedIndividual,
        owl:Thing ;
    rdfs:comment "Entity representing City To Bay Fun Run"^^xsd:string .

ns2:City_of_Amasya a owl:NamedIndividual,
        owl:Thing ;
    rdfs:comment "Entity representing City of Amasya"^^xsd:string .

ns2:City_of_Binghamton__NY a owl:NamedIndividual,
        owl:Thing ;
    rdfs:comment "Entity representing City of Binghamton, NY"^^xsd:string .

ns2:City_of_Dubois__PA a owl:NamedIndividual,
        owl:Thing ;
    rdfs:comment "Entity representing City of Dubois, PA"^^xsd:string .

ns2:ClamCase a owl:NamedIndividual,
        owl:Thing ;
    rdfs:comment "Entity representing ClamCase"^^xsd:string .

ns2:Cloudflare a owl:NamedIndividual,
        owl:Thing ;
    rdfs:comment "Entity representing Cloudflare"^^xsd:string .

ns2:Club_Penguin a owl:NamedIndividual,
        owl:Thing ;
    rdfs:comment "Entity representing Club Penguin"^^xsd:string .

ns2:Code_Spaces a owl:NamedIndividual,
        owl:Thing ;
    rdfs:comment "Entity representing Code Spaces"^^xsd:string .

ns2:CoinEX_pw a owl:NamedIndividual,
        owl:Thing ;
    rdfs:comment "Entity representing CoinEX.pw"^^xsd:string .

ns2:College_in_Shanghai_s_Songjiang_District a owl:NamedIndividual,
        owl:Thing ;
    rdfs:comment "Entity representing College in Shanghai's Songjiang District"^^xsd:string .

ns2:College_of_Physicians_and_Surgeons a owl:NamedIndividual,
        owl:Thing ;
    rdfs:comment "Entity representing College of Physicians and Surgeons"^^xsd:string .

ns2:Colorado a owl:NamedIndividual,
        owl:Thing ;
    rdfs:comment "Entity representing Colorado"^^xsd:string .

ns2:Comcast a owl:NamedIndividual,
        owl:Thing ;
    rdfs:comment "Entity representing Comcast"^^xsd:string .

ns2:Community_Health_Systems a owl:NamedIndividual,
        owl:Thing ;
    rdfs:comment "Entity representing Community Health Systems"^^xsd:string .

ns2:Conforama a owl:NamedIndividual,
        owl:Thing ;
    rdfs:comment "Entity representing Conforama"^^xsd:string .

ns2:Connecticut_State_Government_website a owl:NamedIndividual,
        owl:Thing ;
    rdfs:comment "Entity representing Connecticut State Government website"^^xsd:string .

ns2:Corsica_Ferries a owl:NamedIndividual,
        owl:Thing ;
    rdfs:comment "Entity representing Corsica Ferries"^^xsd:string .

ns2:Craftsman_Book a owl:NamedIndividual,
        owl:Thing ;
    rdfs:comment "Entity representing Craftsman Book"^^xsd:string .

ns2:Createthe_Group a owl:NamedIndividual,
        owl:Thing ;
    rdfs:comment "Entity representing Createthe Group"^^xsd:string .

ns2:Cryptome a owl:NamedIndividual,
        owl:Thing ;
    rdfs:comment "Entity representing Cryptome"^^xsd:string .

ns2:Cumberland_Valley_School_District a owl:NamedIndividual,
        owl:Thing ;
    rdfs:comment "Entity representing Cumberland Valley School District"^^xsd:string .

ns2:DNB a owl:NamedIndividual,
        owl:Thing ;
    rdfs:comment "Entity representing DNB"^^xsd:string .

ns2:Dairy_Queen a owl:NamedIndividual,
        owl:Thing ;
    rdfs:comment "Entity representing Dairy Queen"^^xsd:string .

ns2:Danske_Bank a owl:NamedIndividual,
        owl:Thing ;
    rdfs:comment "Entity representing Danske Bank"^^xsd:string .

ns2:Dartmouth_Hitchcock a owl:NamedIndividual,
        owl:Thing ;
    rdfs:comment "Entity representing Dartmouth-Hitchcock"^^xsd:string .

ns2:DataSecurity a owl:Class ;
    rdfs:label "data security"^^xsd:string ;
    rdfs:comment "Formal definition for DataSecurity within the cybersecurity domain."^^xsd:string ;
    rdfs:subClassOf ns1:DataCorruption .

ns2:Data_Attack_Exploitation_of_Application_ a owl:NamedIndividual,
        owl:Thing ;
    rdfs:comment "Entity representing Data Attack,Exploitation of Application Server,Message Manipulation"^^xsd:string .

ns2:Data_Attack_External_Denial_of_Service a owl:NamedIndividual,
        owl:Thing ;
    rdfs:comment "Entity representing Data Attack,External Denial of Service"^^xsd:string .

ns2:Data_Attack_Message_Manipulation_Exploit a owl:NamedIndividual,
        owl:Thing ;
    rdfs:comment "Entity representing Data Attack,Message Manipulation,Exploitation of Application Server,External Denial of Service"^^xsd:string .

ns2:DeKalb_Health a owl:NamedIndividual,
        owl:Thing ;
    rdfs:comment "Entity representing DeKalb Health"^^xsd:string .

ns2:Delaware_Treasury_Division a owl:NamedIndividual,
        owl:Thing ;
    rdfs:comment "Entity representing Delaware Treasury Division"^^xsd:string .

ns2:Deltek a owl:NamedIndividual,
        owl:Thing ;
    rdfs:comment "Entity representing Deltek"^^xsd:string .

ns2:Denmark a ns1:ThreatActor,
        owl:NamedIndividual ;
    rdfs:comment "Entity representing Denmark"^^xsd:string .

ns2:Denmark_s_Socialist_Party a owl:NamedIndividual,
        owl:Thing ;
    rdfs:comment "Entity representing Denmark's Socialist Party"^^xsd:string .

ns2:Dennis_East_International a owl:NamedIndividual,
        owl:Thing ;
    rdfs:comment "Entity representing Dennis East International"^^xsd:string .

ns2:Department_of_Agriculture a owl:NamedIndividual,
        owl:Thing ;
    rdfs:comment "Entity representing Department of Agriculture"^^xsd:string .

ns2:Department_of_Culture__Media_and_Sport a owl:NamedIndividual,
        owl:Thing ;
    rdfs:comment "Entity representing Department of Culture, Media and Sport"^^xsd:string .

ns2:Department_of_Homeland_Securiety a owl:NamedIndividual,
        owl:Thing ;
    rdfs:comment "Entity representing Department of Homeland Securiety"^^xsd:string .

ns2:Directorate_General_Public_Relations__Go a owl:NamedIndividual,
        owl:Thing ;
    rdfs:comment "Entity representing Directorate General Public Relations, Government of the Punjab"^^xsd:string .

ns2:Directors_Guild_of_Canada a owl:NamedIndividual,
        owl:Thing ;
    rdfs:comment "Entity representing Directors Guild of Canada"^^xsd:string .

ns2:Dmitry_Medvedev_Twitter_account a owl:NamedIndividual,
        owl:Thing ;
    rdfs:comment "Entity representing Dmitry Medvedev Twitter account"^^xsd:string .

ns2:Dnipropetrovsk_Department_of_Law_Enforce a owl:NamedIndividual,
        owl:Thing ;
    rdfs:comment "Entity representing Dnipropetrovsk Department of Law Enforcement"^^xsd:string .

ns2:Doge_Vault a owl:NamedIndividual,
        owl:Thing ;
    rdfs:comment "Entity representing Doge Vault"^^xsd:string .

ns2:Dominion_Resources a owl:NamedIndividual,
        owl:Thing ;
    rdfs:comment "Entity representing Dominion Resources"^^xsd:string .

ns2:Domino_s_Pizza a owl:NamedIndividual,
        owl:Thing ;
    rdfs:comment "Entity representing Domino's Pizza"^^xsd:string .

ns2:Dota_2 a owl:NamedIndividual,
        owl:Thing ;
    rdfs:comment "Entity representing Dota 2"^^xsd:string .

ns2:Dr__Micharl_M__Krop_Senior_High_School a owl:NamedIndividual,
        owl:Thing ;
    rdfs:comment "Entity representing Dr. Micharl M. Krop Senior High School"^^xsd:string .

ns2:Dubai_Police a owl:NamedIndividual,
        owl:Thing ;
    rdfs:comment "Entity representing Dubai Police"^^xsd:string .

ns2:Duruma_Principality a owl:NamedIndividual,
        owl:Thing ;
    rdfs:comment "Entity representing Duruma Principality"^^xsd:string .

ns2:EA a owl:NamedIndividual,
        owl:Thing ;
    rdfs:comment "Entity representing EA"^^xsd:string .

ns2:EA_com a owl:NamedIndividual,
        owl:Thing ;
    rdfs:comment "Entity representing EA.com"^^xsd:string .

ns2:ESET_Security_Forum a owl:NamedIndividual,
        owl:Thing ;
    rdfs:comment "Entity representing ESET Security Forum"^^xsd:string .

ns2:ESET_s_Spain_domain a owl:NamedIndividual,
        owl:Thing ;
    rdfs:comment "Entity representing ESET's Spain domain"^^xsd:string .

ns2:Earth_Hour_Philippines a owl:NamedIndividual,
        owl:Thing ;
    rdfs:comment "Entity representing Earth Hour Philippines"^^xsd:string .

ns2:Easton_Bell_Sports a owl:NamedIndividual,
        owl:Thing ;
    rdfs:comment "Entity representing Easton-Bell Sports"^^xsd:string .

ns2:Ecuador a ns1:ThreatActor,
        owl:NamedIndividual ;
    rdfs:comment "Entity representing Ecuador"^^xsd:string .

ns2:Edgepark_Medical_Supplies a owl:NamedIndividual,
        owl:Thing ;
    rdfs:comment "Entity representing Edgepark Medical Supplies"^^xsd:string .

ns2:Egyptian_Ministry_of_Information a owl:NamedIndividual,
        owl:Thing ;
    rdfs:comment "Entity representing Egyptian Ministry of Information"^^xsd:string .

ns2:Eircom a owl:NamedIndividual,
        owl:Thing ;
    rdfs:comment "Entity representing Eircom"^^xsd:string .

ns2:El_Agave_Restaurant a owl:NamedIndividual,
        owl:Thing ;
    rdfs:comment "Entity representing El Agave Restaurant"^^xsd:string .

ns2:Embassy_of_India_in_Russia a owl:NamedIndividual,
        owl:Thing ;
    rdfs:comment "Entity representing Embassy of India in Russia"^^xsd:string .

ns2:Employees_Old_Age_Benefits_Institution a owl:NamedIndividual,
        owl:Thing ;
    rdfs:comment "Entity representing Employees Old-Age Benefits Institution"^^xsd:string .

ns2:Energie_Steiermark a owl:NamedIndividual,
        owl:Thing ;
    rdfs:comment "Entity representing Energie Steiermark"^^xsd:string .

ns2:European_Central_Bank a owl:NamedIndividual,
        owl:Thing ;
    rdfs:comment "Entity representing European Central Bank"^^xsd:string .

ns2:European_Court_of_Human_Rights a owl:NamedIndividual,
        owl:Thing ;
    rdfs:comment "Entity representing European Court of Human Rights"^^xsd:string .

ns2:Experian a owl:NamedIndividual,
        owl:Thing ;
    rdfs:comment "Entity representing Experian"^^xsd:string .

ns2:Exploitation_of_Data_in_Transit a owl:NamedIndividual,
        owl:Thing ;
    rdfs:comment "Entity representing Exploitation of Data in Transit"^^xsd:string .

ns2:Exploitation_of_Network_Infrastructure a owl:NamedIndividual,
        owl:Thing ;
    rdfs:comment "Entity representing Exploitation of Network Infrastructure"^^xsd:string .

ns2:External_Denial_of_Service_Exploitation_ a owl:NamedIndividual,
        owl:Thing ;
    rdfs:comment "Entity representing External Denial of Service,Exploitation of Application Server"^^xsd:string .

ns2:FBI_Fusion_Center a owl:NamedIndividual,
        owl:Thing ;
    rdfs:comment "Entity representing FBI Fusion Center"^^xsd:string .

ns2:FC_Barcelona a owl:NamedIndividual,
        owl:Thing ;
    rdfs:comment "Entity representing FC Barcelona"^^xsd:string .

ns2:Federal_Customs_Service a owl:NamedIndividual,
        owl:Thing ;
    rdfs:comment "Entity representing Federal Customs Service"^^xsd:string .

ns2:Federal_Police_of_Brazil a owl:NamedIndividual,
        owl:Thing ;
    rdfs:comment "Entity representing Federal Police of Brazil"^^xsd:string .

ns2:Feedly a owl:NamedIndividual,
        owl:Thing ;
    rdfs:comment "Entity representing Feedly"^^xsd:string .

ns2:Ferguson_Police a owl:NamedIndividual,
        owl:Thing ;
    rdfs:comment "Entity representing Ferguson Police"^^xsd:string .

ns2:Financial_Services_Online a owl:NamedIndividual,
        owl:Thing ;
    rdfs:comment "Entity representing Financial Services Online"^^xsd:string .

ns2:Finnish_Foreign_Ministry a owl:NamedIndividual,
        owl:Thing ;
    rdfs:comment "Entity representing Finnish Foreign Ministry"^^xsd:string .

ns2:Flight_Centre_Travel_Group a owl:NamedIndividual,
        owl:Thing ;
    rdfs:comment "Entity representing Flight Centre Travel Group"^^xsd:string .

ns2:Football_Federation_of_Armenia a owl:NamedIndividual,
        owl:Thing ;
    rdfs:comment "Entity representing Football Federation of Armenia"^^xsd:string .

ns2:Forbes a owl:NamedIndividual,
        owl:Thing ;
    rdfs:comment "Entity representing Forbes"^^xsd:string .

ns2:Frankie_Grande a owl:NamedIndividual,
        owl:Thing ;
    rdfs:comment "Entity representing Frankie Grande"^^xsd:string .

ns2:French_Ministry_of_Defense a owl:NamedIndividual,
        owl:Thing ;
    rdfs:comment "Entity representing French Ministry of Defense"^^xsd:string .

ns2:French_Ministry_of_Interior a owl:NamedIndividual,
        owl:Thing ;
    rdfs:comment "Entity representing French Ministry of Interior"^^xsd:string .

ns2:Froco_Fresh_Frozen a owl:NamedIndividual,
        owl:Thing ;
    rdfs:comment "Entity representing Froco Fresh Frozen"^^xsd:string .

ns2:Fullerton_Police_Department a owl:NamedIndividual,
        owl:Thing ;
    rdfs:comment "Entity representing Fullerton Police Department"^^xsd:string .

ns2:Gamma_Group a owl:NamedIndividual,
        owl:Thing ;
    rdfs:comment "Entity representing Gamma Group"^^xsd:string .

ns2:Gary_Barlow a owl:NamedIndividual,
        owl:Thing ;
    rdfs:comment "Entity representing Gary Barlow"^^xsd:string .

ns2:Gas_Distribution_Authority_of_Sakarya a owl:NamedIndividual,
        owl:Thing ;
    rdfs:comment "Entity representing Gas Distribution Authority of Sakarya"^^xsd:string .

ns2:Gateway_Savings_and_Loans_Limited a owl:NamedIndividual,
        owl:Thing ;
    rdfs:comment "Entity representing Gateway Savings and Loans Limited"^^xsd:string .

ns2:Geekface a owl:NamedIndividual,
        owl:Thing ;
    rdfs:comment "Entity representing Geekface"^^xsd:string .

ns2:General_Directorate_of_the_EGO a owl:NamedIndividual,
        owl:Thing ;
    rdfs:comment "Entity representing General Directorate of the EGO"^^xsd:string .

ns2:German_Aerospace_Centre a owl:NamedIndividual,
        owl:Thing ;
    rdfs:comment "Entity representing German Aerospace Centre"^^xsd:string .

ns2:Germany a ns1:ThreatActor,
        owl:NamedIndividual ;
    rdfs:comment "Entity representing Germany"^^xsd:string .

ns2:Gingerbread_Shed_Corporation a owl:NamedIndividual,
        owl:Thing ;
    rdfs:comment "Entity representing Gingerbread Shed Corporation"^^xsd:string .

ns2:Give_Me_Coins a owl:NamedIndividual,
        owl:Thing ;
    rdfs:comment "Entity representing Give Me Coins"^^xsd:string .

ns2:Gjensidige a owl:NamedIndividual,
        owl:Thing ;
    rdfs:comment "Entity representing Gjensidige"^^xsd:string .

ns2:Globo_TV_Brasil a owl:NamedIndividual,
        owl:Thing ;
    rdfs:comment "Entity representing Globo TV Brasil"^^xsd:string .

ns2:Goodwill_Industries a owl:NamedIndividual,
        owl:Thing ;
    rdfs:comment "Entity representing Goodwill Industries"^^xsd:string .

ns2:Government_Secure_Intranet a owl:NamedIndividual,
        owl:Thing ;
    rdfs:comment "Entity representing Government Secure Intranet"^^xsd:string .

ns2:Government_of_Punjab a owl:NamedIndividual,
        owl:Thing ;
    rdfs:comment "Entity representing Government of Punjab"^^xsd:string .

ns2:Governor_of_Arizona a owl:NamedIndividual,
        owl:Thing ;
    rdfs:comment "Entity representing Governor of Arizona"^^xsd:string .

ns2:Griminal a owl:NamedIndividual,
        owl:Thing ;
    rdfs:comment "Entity representing Griminal"^^xsd:string .

ns2:Grinding_Gear_Games a owl:NamedIndividual,
        owl:Thing ;
    rdfs:comment "Entity representing Grinding Gear Games"^^xsd:string .

ns2:Ground_ctrl a owl:NamedIndividual,
        owl:Thing ;
    rdfs:comment "Entity representing Ground(ctrl)"^^xsd:string .

ns2:Haaretz a owl:NamedIndividual,
        owl:Thing ;
    rdfs:comment "Entity representing Haaretz"^^xsd:string .

ns2:Harley_Medical_Group a owl:NamedIndividual,
        owl:Thing ;
    rdfs:comment "Entity representing Harley Medical Group"^^xsd:string .

ns2:Healthcare_gov a owl:NamedIndividual,
        owl:Thing ;
    rdfs:comment "Entity representing Healthcare.gov"^^xsd:string .

ns2:Hillary_Clinton a owl:NamedIndividual,
        owl:Thing ;
    rdfs:comment "Entity representing Hillary Clinton"^^xsd:string .

ns2:Hootsuite a owl:NamedIndividual,
        owl:Thing ;
    rdfs:comment "Entity representing Hootsuite"^^xsd:string .

ns2:Houston_Astros a owl:NamedIndividual,
        owl:Thing ;
    rdfs:comment "Entity representing Houston Astros"^^xsd:string .

ns2:Huraymila_Principality a owl:NamedIndividual,
        owl:Thing ;
    rdfs:comment "Entity representing Huraymila Principality"^^xsd:string .

ns2:INVALSI a owl:NamedIndividual,
        owl:Thing ;
    rdfs:comment "Entity representing INVALSI"^^xsd:string .

ns2:Idaho a owl:NamedIndividual,
        owl:Thing ;
    rdfs:comment "Entity representing Idaho"^^xsd:string .

ns2:Indexeus_org a owl:NamedIndividual,
        owl:Thing ;
    rdfs:comment "Entity representing Indexeus.org"^^xsd:string .

ns2:Indian_Ministry_of_Railways a owl:NamedIndividual,
        owl:Thing ;
    rdfs:comment "Entity representing Indian Ministry of Railways"^^xsd:string .

ns2:Indian_Railways a owl:NamedIndividual,
        owl:Thing ;
    rdfs:comment "Entity representing Indian Railways"^^xsd:string .

ns2:International_Civil_Aviation_Organizatio a owl:NamedIndividual,
        owl:Thing ;
    rdfs:comment "Entity representing International Civil Aviation Organization"^^xsd:string .

ns2:International_Council_of_E_Commerce_Cons a owl:NamedIndividual,
        owl:Thing ;
    rdfs:comment "Entity representing International Council of E-Commerce Consultants"^^xsd:string .

ns2:Iowa a owl:NamedIndividual,
        owl:Thing ;
    rdfs:comment "Entity representing Iowa"^^xsd:string .

ns2:Iowa_State_University a owl:NamedIndividual,
        owl:Thing ;
    rdfs:comment "Entity representing Iowa State University"^^xsd:string .

ns2:Israel_Defense a owl:NamedIndividual,
        owl:Thing ;
    rdfs:comment "Entity representing Israel Defense"^^xsd:string .

ns2:Israeli_Channel_10 a owl:NamedIndividual,
        owl:Thing ;
    rdfs:comment "Entity representing Israeli Channel 10"^^xsd:string .

ns2:Israeli_Defense_Contractors a owl:NamedIndividual,
        owl:Thing ;
    rdfs:comment "Entity representing Israeli Defense Contractors"^^xsd:string .

ns2:Israeli_Defense_Ministry a owl:NamedIndividual,
        owl:Thing ;
    rdfs:comment "Entity representing Israeli Defense Ministry"^^xsd:string .

ns2:Israeli_Embassy_for_Uzbekistan a owl:NamedIndividual,
        owl:Thing ;
    rdfs:comment "Entity representing Israeli Embassy for Uzbekistan"^^xsd:string .

ns2:JCM_Partners a owl:NamedIndividual,
        owl:Thing ;
    rdfs:comment "Entity representing JCM Partners"^^xsd:string .

ns2:JPMorgan a owl:NamedIndividual,
        owl:Thing ;
    rdfs:comment "Entity representing JPMorgan"^^xsd:string .

ns2:JSTOR a owl:NamedIndividual,
        owl:Thing ;
    rdfs:comment "Entity representing JSTOR"^^xsd:string .

ns2:Japan a ns1:ThreatActor,
        owl:NamedIndividual ;
    rdfs:comment "Entity representing Japan"^^xsd:string .

ns2:Jean_Jacques_Quisquater a owl:NamedIndividual,
        owl:Thing ;
    rdfs:comment "Entity representing Jean-Jacques Quisquater"^^xsd:string .

ns2:Jennifer_Lawrence a owl:NamedIndividual,
        owl:Thing ;
    rdfs:comment "Entity representing Jennifer Lawrence"^^xsd:string .

ns2:Jon__Bones__Jones a owl:NamedIndividual,
        owl:Thing ;
    rdfs:comment "Entity representing Jon \"Bones\" Jones"^^xsd:string .

ns2:Justice_Minister_Judith_Collins a owl:NamedIndividual,
        owl:Thing ;
    rdfs:comment "Entity representing Justice Minister Judith Collins"^^xsd:string .

ns2:Kaiser_Permanente a owl:NamedIndividual,
        owl:Thing ;
    rdfs:comment "Entity representing Kaiser Permanente"^^xsd:string .

ns2:Kali a owl:NamedIndividual,
        owl:Thing ;
    rdfs:comment "Entity representing Kali"^^xsd:string .

ns2:Kansas_Interactive_Testing_Engine a owl:NamedIndividual,
        owl:Thing ;
    rdfs:comment "Entity representing Kansas Interactive Testing Engine"^^xsd:string .

ns2:Kars_Municipality a owl:NamedIndividual,
        owl:Thing ;
    rdfs:comment "Entity representing Kars Municipality"^^xsd:string .

ns2:Kate_Upton a owl:NamedIndividual,
        owl:Thing ;
    rdfs:comment "Entity representing Kate Upton"^^xsd:string .

ns2:Kenyan_Defence_Forces a owl:NamedIndividual,
        owl:Thing ;
    rdfs:comment "Entity representing Kenyan Defence Forces"^^xsd:string .

ns2:Kickstarter a owl:NamedIndividual,
        owl:Thing ;
    rdfs:comment "Entity representing Kickstarter"^^xsd:string .

ns2:Kirsten_Dunst a owl:NamedIndividual,
        owl:Thing ;
    rdfs:comment "Entity representing Kirsten Dunst"^^xsd:string .

ns2:Klas_Telecom a owl:NamedIndividual,
        owl:Thing ;
    rdfs:comment "Entity representing Klas Telecom"^^xsd:string .

ns2:Korea__the_Republic_of a ns1:ThreatActor,
        owl:NamedIndividual ;
    rdfs:comment "Entity representing Korea (the Republic of)"^^xsd:string .

ns2:Kuwait a ns1:ThreatActor,
        owl:NamedIndividual ;
    rdfs:comment "Entity representing Kuwait"^^xsd:string .

ns2:Lal_Krishna_Advani_website a owl:NamedIndividual,
        owl:Thing ;
    rdfs:comment "Entity representing Lal Krishna Advani website"^^xsd:string .

ns2:Las_Vegas_Sands_Corp a owl:NamedIndividual,
        owl:Thing ;
    rdfs:comment "Entity representing Las Vegas Sands Corp"^^xsd:string .

ns2:Lea_Michele a owl:NamedIndividual,
        owl:Thing ;
    rdfs:comment "Entity representing Lea Michele"^^xsd:string .

ns2:League_of_Legends a owl:NamedIndividual,
        owl:Thing ;
    rdfs:comment "Entity representing League of Legends"^^xsd:string .

ns2:Linkin_Park a owl:NamedIndividual,
        owl:Thing ;
    rdfs:comment "Entity representing Linkin Park"^^xsd:string .

ns2:Lockheed_Martin a owl:NamedIndividual,
        owl:Thing ;
    rdfs:comment "Entity representing Lockheed Martin"^^xsd:string .

ns2:Lubbock_Cardiology_Clinic a owl:NamedIndividual,
        owl:Thing ;
    rdfs:comment "Entity representing Lubbock Cardiology Clinic"^^xsd:string .

ns2:Lutheran_Church_of_Australia a owl:NamedIndividual,
        owl:Thing ;
    rdfs:comment "Entity representing Lutheran Church of Australia"^^xsd:string .

ns2:MMMOOO a owl:NamedIndividual,
        owl:Thing ;
    rdfs:comment "Entity representing MMMOOO"^^xsd:string .

ns2:Mad_Mimi a owl:NamedIndividual,
        owl:Thing ;
    rdfs:comment "Entity representing Mad Mimi"^^xsd:string .

ns2:Malaysia_Airlines a owl:NamedIndividual,
        owl:Thing ;
    rdfs:comment "Entity representing Malaysia Airlines"^^xsd:string .

ns2:Malaysian_Department_of_Civil_Aviation a owl:NamedIndividual,
        owl:Thing ;
    rdfs:comment "Entity representing Malaysian Department of Civil Aviation"^^xsd:string .

ns2:Malaysian_Ministry_of_Education a owl:NamedIndividual,
        owl:Thing ;
    rdfs:comment "Entity representing Malaysian Ministry of Education"^^xsd:string .

ns2:Malaysian_National_Security_Council a owl:NamedIndividual,
        owl:Thing ;
    rdfs:comment "Entity representing Malaysian National Security Council"^^xsd:string .

ns2:MalwareThreat a owl:Class ;
    rdfs:label "malware threat"^^xsd:string ;
    rdfs:comment "Formal definition for MalwareThreat within the cybersecurity domain."^^xsd:string ;
    rdfs:subClassOf ns2:Malware .

ns2:MalwareVictim a owl:Class ;
    rdfs:label "malware victim"^^xsd:string ;
    rdfs:comment "Formal definition for MalwareVictim within the cybersecurity domain."^^xsd:string ;
    rdfs:subClassOf ns2:Malware .

ns2:MangaGamer a owl:NamedIndividual,
        owl:Thing ;
    rdfs:comment "Entity representing MangaGamer"^^xsd:string .

ns2:MarkMonitor a owl:NamedIndividual,
        owl:Thing ;
    rdfs:comment "Entity representing MarkMonitor"^^xsd:string .

ns2:Massachusetts_Institute_of_Technology a owl:NamedIndividual,
        owl:Thing ;
    rdfs:comment "Entity representing Massachusetts Institute of Technology"^^xsd:string .

ns2:McKayla_Maroney a owl:NamedIndividual,
        owl:Thing ;
    rdfs:comment "Entity representing McKayla Maroney"^^xsd:string .

ns2:Medtronic a owl:NamedIndividual,
        owl:Thing ;
    rdfs:comment "Entity representing Medtronic"^^xsd:string .

ns2:MeetMe a owl:NamedIndividual,
        owl:Thing ;
    rdfs:comment "Entity representing MeetMe"^^xsd:string .

ns2:Mercantile_Communications_Pvt a owl:NamedIndividual,
        owl:Thing ;
    rdfs:comment "Entity representing Mercantile Communications Pvt"^^xsd:string .

ns2:Message_Manipulation_Exploitation_of_End a owl:NamedIndividual,
        owl:Thing ;
    rdfs:comment "Entity representing Message Manipulation,Exploitation of End Hosts"^^xsd:string .

ns2:Message_Manipulation_External_Denial_of_ a owl:NamedIndividual,
        owl:Thing ;
    rdfs:comment "Entity representing Message Manipulation,External Denial of Service"^^xsd:string .

ns2:Meteo_France__meteofrance_com a owl:NamedIndividual,
        owl:Thing ;
    rdfs:comment "Entity representing Meteo France (meteofrance.com)"^^xsd:string .

ns2:Metro_newspaper a owl:NamedIndividual,
        owl:Thing ;
    rdfs:comment "Entity representing Metro newspaper"^^xsd:string .

ns2:Metropolitan_Companies__Inc a owl:NamedIndividual,
        owl:Thing ;
    rdfs:comment "Entity representing Metropolitan Companies, Inc."^^xsd:string .

ns2:Mexico a ns1:ThreatActor,
        owl:NamedIndividual ;
    rdfs:comment "Entity representing Mexico"^^xsd:string .

ns2:Michael_s a owl:NamedIndividual,
        owl:Thing ;
    rdfs:comment "Entity representing Michael's"^^xsd:string .

ns2:Microsoft_News a owl:NamedIndividual,
        owl:Thing ;
    rdfs:comment "Entity representing Microsoft News"^^xsd:string .

ns2:Midwest_Orthopaedics a owl:NamedIndividual,
        owl:Thing ;
    rdfs:comment "Entity representing Midwest Orthopaedics"^^xsd:string .

ns2:Ministry_of_Agriculture_and_Rural_Develo a owl:NamedIndividual,
        owl:Thing ;
    rdfs:comment "Entity representing Ministry of Agriculture and Rural Development"^^xsd:string .

ns2:Ministry_of_Communications_and_Informati a owl:NamedIndividual,
        owl:Thing ;
    rdfs:comment "Entity representing Ministry of Communications and Information Technology"^^xsd:string .

ns2:Ministry_of_Defense_of_Pakistan a owl:NamedIndividual,
        owl:Thing ;
    rdfs:comment "Entity representing Ministry of Defense of Pakistan"^^xsd:string .

ns2:Ministry_of_Education_of_Armenia a owl:NamedIndividual,
        owl:Thing ;
    rdfs:comment "Entity representing Ministry of Education of Armenia"^^xsd:string .

ns2:Ministry_of_Health a owl:NamedIndividual,
        owl:Thing ;
    rdfs:comment "Entity representing Ministry of Health"^^xsd:string .

ns2:Ministry_of_Interior a owl:NamedIndividual,
        owl:Thing ;
    rdfs:comment "Entity representing Ministry of Interior"^^xsd:string .

ns2:Ministry_of_Natural_Resource_and_Environ a owl:NamedIndividual,
        owl:Thing ;
    rdfs:comment "Entity representing Ministry of Natural Resource and Environment"^^xsd:string .

ns2:Ministry_of_Police_Affairs a owl:NamedIndividual,
        owl:Thing ;
    rdfs:comment "Entity representing Ministry of Police Affairs"^^xsd:string .

ns2:Mizado_Cocina a owl:NamedIndividual,
        owl:Thing ;
    rdfs:comment "Entity representing Mizado Cocina"^^xsd:string .

ns2:Monju_Nuclear_Power_Plant a owl:NamedIndividual,
        owl:Thing ;
    rdfs:comment "Entity representing Monju Nuclear Power Plant"^^xsd:string .

ns2:Montana a owl:NamedIndividual,
        owl:Thing ;
    rdfs:comment "Entity representing Montana"^^xsd:string .

ns2:Montana_Department_of_Public_Health a owl:NamedIndividual,
        owl:Thing ;
    rdfs:comment "Entity representing Montana Department of Public Health"^^xsd:string .

ns2:Moshtix a owl:NamedIndividual,
        owl:Thing ;
    rdfs:comment "Entity representing Moshtix"^^xsd:string .

ns2:Mossad a owl:NamedIndividual,
        owl:Thing ;
    rdfs:comment "Entity representing Mossad"^^xsd:string .

ns2:Move__Inc a owl:NamedIndividual,
        owl:Thing ;
    rdfs:comment "Entity representing Move, Inc."^^xsd:string .

ns2:Moz a owl:NamedIndividual,
        owl:Thing ;
    rdfs:comment "Entity representing Moz"^^xsd:string .

ns2:Mt__Gox a owl:NamedIndividual,
        owl:Thing ;
    rdfs:comment "Entity representing Mt. Gox"^^xsd:string .

ns2:Muslim_Directory a owl:NamedIndividual,
        owl:Thing ;
    rdfs:comment "Entity representing Muslim Directory"^^xsd:string .

ns2:MyCause a owl:NamedIndividual,
        owl:Thing ;
    rdfs:comment "Entity representing MyCause"^^xsd:string .

ns2:Namecheap a owl:NamedIndividual,
        owl:Thing ;
    rdfs:comment "Entity representing Namecheap"^^xsd:string .

ns2:Namibian_Government_Portal a owl:NamedIndividual,
        owl:Thing ;
    rdfs:comment "Entity representing Namibian Government Portal"^^xsd:string .

ns2:National_Health_Service a owl:NamedIndividual,
        owl:Thing ;
    rdfs:comment "Entity representing National Health Service"^^xsd:string .

ns2:National_Informatics_Center a owl:NamedIndividual,
        owl:Thing ;
    rdfs:comment "Entity representing National Informatics Center"^^xsd:string .

ns2:National_Portal_of_India a owl:NamedIndividual,
        owl:Thing ;
    rdfs:comment "Entity representing National Portal of India"^^xsd:string .

ns2:National_Research_Council a owl:NamedIndividual,
        owl:Thing ;
    rdfs:comment "Entity representing National Research Council"^^xsd:string .

ns2:National_Socialist_Party_of_Canada a owl:NamedIndividual,
        owl:Thing ;
    rdfs:comment "Entity representing National-Socialist Party of Canada"^^xsd:string .

ns2:Naver a owl:NamedIndividual,
        owl:Thing ;
    rdfs:comment "Entity representing Naver"^^xsd:string .

ns2:Nebraska a owl:NamedIndividual,
        owl:Thing ;
    rdfs:comment "Entity representing Nebraska"^^xsd:string .

ns2:Neiman_Marcus a owl:NamedIndividual,
        owl:Thing ;
    rdfs:comment "Entity representing Neiman Marcus"^^xsd:string .

ns2:Network_Information_Center_of_Paraguay a owl:NamedIndividual,
        owl:Thing ;
    rdfs:comment "Entity representing Network Information Center of Paraguay"^^xsd:string .

ns2:New_Jersey a owl:NamedIndividual,
        owl:Thing ;
    rdfs:comment "Entity representing New Jersey"^^xsd:string .

ns2:New_York_Board_of_Elections a owl:NamedIndividual,
        owl:Thing ;
    rdfs:comment "Entity representing New York Board of Elections"^^xsd:string .

ns2:New_Zealand a ns1:ThreatActor,
        owl:NamedIndividual ;
    rdfs:comment "Entity representing New Zealand"^^xsd:string .

ns2:New_Zealand_National_Institute_of_Water_ a owl:NamedIndividual,
        owl:Thing ;
    rdfs:comment "Entity representing New Zealand National Institute of Water and Atmospheric Research"^^xsd:string .

ns2:Nordea a owl:NamedIndividual,
        owl:Thing ;
    rdfs:comment "Entity representing Nordea"^^xsd:string .

ns2:North_Carolina a owl:NamedIndividual,
        owl:Thing ;
    rdfs:comment "Entity representing North Carolina"^^xsd:string .

ns2:North_East_King_County_Regional_Public_S a owl:NamedIndividual,
        owl:Thing ;
    rdfs:comment "Entity representing North East King County Regional Public Safety Communication Agency (NORCOM)"^^xsd:string .

ns2:Nuclear_Regulatory_Commission a owl:NamedIndividual,
        owl:Thing ;
    rdfs:comment "Entity representing Nuclear Regulatory Commission"^^xsd:string .

ns2:Office a owl:NamedIndividual,
        owl:Thing ;
    rdfs:comment "Entity representing Office"^^xsd:string .

ns2:Office_of_Personnel_Management a owl:NamedIndividual,
        owl:Thing ;
    rdfs:comment "Entity representing Office of Personnel Management"^^xsd:string .

ns2:Office_of_the_Israeli_Prime_Minister a owl:NamedIndividual,
        owl:Thing ;
    rdfs:comment "Entity representing Office of the Israeli Prime Minister"^^xsd:string .

ns2:Office_of_the_Prime_Minister_of_Ukraine a owl:NamedIndividual,
        owl:Thing ;
    rdfs:comment "Entity representing Office of the Prime Minister of Ukraine"^^xsd:string .

ns2:Official_Portal_for_Manila__Philippines a owl:NamedIndividual,
        owl:Thing ;
    rdfs:comment "Entity representing Official Portal for Manila, Philippines"^^xsd:string .

ns2:Ohio_State_Government a owl:NamedIndividual,
        owl:Thing ;
    rdfs:comment "Entity representing Ohio State Government"^^xsd:string .

ns2:Olmsted_Medical_Center a owl:NamedIndividual,
        owl:Thing ;
    rdfs:comment "Entity representing Olmsted Medical Center"^^xsd:string .

ns2:OmegaNet a owl:NamedIndividual,
        owl:Thing ;
    rdfs:comment "Entity representing OmegaNet"^^xsd:string .

ns2:Onsite_Health_Diagnostics a owl:NamedIndividual,
        owl:Thing ;
    rdfs:comment "Entity representing Onsite Health Diagnostics"^^xsd:string .

ns2:Oregon a owl:NamedIndividual,
        owl:Thing ;
    rdfs:comment "Entity representing Oregon"^^xsd:string .

ns2:Origin a owl:NamedIndividual,
        owl:Thing ;
    rdfs:comment "Entity representing Origin"^^xsd:string .

ns2:Otto_Pizza a owl:NamedIndividual,
        owl:Thing ;
    rdfs:comment "Entity representing Otto Pizza"^^xsd:string .

ns2:PTV_Sports a owl:NamedIndividual,
        owl:Thing ;
    rdfs:comment "Entity representing PTV Sports"^^xsd:string .

ns2:P__F__Chang_s a owl:NamedIndividual,
        owl:Thing ;
    rdfs:comment "Entity representing P. F. Chang's"^^xsd:string .

ns2:Pakistan_Electric_Power_Company a owl:NamedIndividual,
        owl:Thing ;
    rdfs:comment "Entity representing Pakistan Electric Power Company"^^xsd:string .

ns2:Pakistan_Government_Establishment_Divisi a owl:NamedIndividual,
        owl:Thing ;
    rdfs:comment "Entity representing Pakistan Government Establishment Division"^^xsd:string .

ns2:Pakistan_Manpower_Institute a owl:NamedIndividual,
        owl:Thing ;
    rdfs:comment "Entity representing Pakistan Manpower Institute"^^xsd:string .

ns2:Pakistan_Meteorological_Department a owl:NamedIndividual,
        owl:Thing ;
    rdfs:comment "Entity representing Pakistan Meteorological Department"^^xsd:string .

ns2:Pakistan_Ministry_of_Interior a owl:NamedIndividual,
        owl:Thing ;
    rdfs:comment "Entity representing Pakistan Ministry of Interior"^^xsd:string .

ns2:Pakistan_Ministry_of_Railways a owl:NamedIndividual,
        owl:Thing ;
    rdfs:comment "Entity representing Pakistan Ministry of Railways"^^xsd:string .

ns2:Pakistan_National_Portal a owl:NamedIndividual,
        owl:Thing ;
    rdfs:comment "Entity representing Pakistan National Portal"^^xsd:string .

ns2:Pakistan_Official_Portal a owl:NamedIndividual,
        owl:Thing ;
    rdfs:comment "Entity representing Pakistan Official Portal"^^xsd:string .

ns2:Pakistani_Consulate_in_Jeddah a owl:NamedIndividual,
        owl:Thing ;
    rdfs:comment "Entity representing Pakistani Consulate in Jeddah"^^xsd:string .

ns2:Palestine__State_of a ns1:ThreatActor,
        owl:NamedIndividual ;
    rdfs:comment "Entity representing Palestine, State of"^^xsd:string .

ns2:Parkistan_Army a owl:NamedIndividual,
        owl:Thing ;
    rdfs:comment "Entity representing Parkistan Army"^^xsd:string .

ns2:PassthePopcorn_me a owl:NamedIndividual,
        owl:Thing ;
    rdfs:comment "Entity representing PassthePopcorn.me"^^xsd:string .

ns2:PayPal a owl:NamedIndividual,
        owl:Thing ;
    rdfs:comment "Entity representing PayPal"^^xsd:string .

ns2:Paytime_Inc a owl:NamedIndividual,
        owl:Thing ;
    rdfs:comment "Entity representing Paytime Inc."^^xsd:string .

ns2:Penn_State_College_of_Medicine a owl:NamedIndividual,
        owl:Thing ;
    rdfs:comment "Entity representing Penn State College of Medicine"^^xsd:string .

ns2:Perl_Blogs a owl:NamedIndividual,
        owl:Thing ;
    rdfs:comment "Entity representing Perl Blogs"^^xsd:string .

ns2:Peru a ns1:ThreatActor,
        owl:NamedIndividual ;
    rdfs:comment "Entity representing Peru"^^xsd:string .

ns2:PharmaNet a owl:NamedIndividual,
        owl:Thing ;
    rdfs:comment "Entity representing PharmaNet"^^xsd:string .

ns2:Philippines a ns1:ThreatActor,
        owl:NamedIndividual ;
    rdfs:comment "Entity representing Philippines"^^xsd:string .

ns2:Placemark_Investments a owl:NamedIndividual,
        owl:Thing ;
    rdfs:comment "Entity representing Placemark Investments"^^xsd:string .

ns2:Plenty_of_Fish a owl:NamedIndividual,
        owl:Thing ;
    rdfs:comment "Entity representing Plenty of Fish"^^xsd:string .

ns2:Plexor a owl:NamedIndividual,
        owl:Thing ;
    rdfs:comment "Entity representing Plexor"^^xsd:string .

ns2:Point_DNS a owl:NamedIndividual,
        owl:Thing ;
    rdfs:comment "Entity representing Point DNS"^^xsd:string .

ns2:Power_Equipment_Direct a owl:NamedIndividual,
        owl:Thing ;
    rdfs:comment "Entity representing Power Equipment Direct"^^xsd:string .

ns2:Presidential_Adviser a owl:NamedIndividual,
        owl:Thing ;
    rdfs:comment "Entity representing Presidential Adviser"^^xsd:string .

ns2:PrezidentBank a owl:NamedIndividual,
        owl:Thing ;
    rdfs:comment "Entity representing PrezidentBank"^^xsd:string .

ns2:Privatbank a owl:NamedIndividual,
        owl:Thing ;
    rdfs:comment "Entity representing Privatbank"^^xsd:string .

ns2:RSA a owl:NamedIndividual,
        owl:Thing ;
    rdfs:comment "Entity representing RSA"^^xsd:string .

ns2:Rafael_Correa_Twitter_account a owl:NamedIndividual,
        owl:Thing ;
    rdfs:comment "Entity representing Rafael Correa Twitter account"^^xsd:string .

ns2:RansomSystem a owl:Class ;
    rdfs:label "ransom system"^^xsd:string ;
    rdfs:comment "Formal definition for RansomSystem within the cybersecurity domain."^^xsd:string ;
    rdfs:subClassOf ns2:Malware .

ns2:Rawalpindi_Police a owl:NamedIndividual,
        owl:Thing ;
    rdfs:comment "Entity representing Rawalpindi Police"^^xsd:string .

ns2:ReadingRockets_org a owl:NamedIndividual,
        owl:Thing ;
    rdfs:comment "Entity representing ReadingRockets.org"^^xsd:string .

ns2:Record_Assist_LLC a owl:NamedIndividual,
        owl:Thing ;
    rdfs:comment "Entity representing Record Assist LLC"^^xsd:string .

ns2:Regional_Electoral_Court_of_the_Amazon a owl:NamedIndividual,
        owl:Thing ;
    rdfs:comment "Entity representing Regional Electoral Court of the Amazon"^^xsd:string .

ns2:Renault a owl:NamedIndividual,
        owl:Thing ;
    rdfs:comment "Entity representing Renault"^^xsd:string .

ns2:Rescator a owl:NamedIndividual,
        owl:Thing ;
    rdfs:comment "Entity representing Rescator"^^xsd:string .

ns2:Reuters a owl:NamedIndividual,
        owl:Thing ;
    rdfs:comment "Entity representing Reuters"^^xsd:string .

ns2:Riyadh_Principality a owl:NamedIndividual,
        owl:Thing ;
    rdfs:comment "Entity representing Riyadh Principality"^^xsd:string .

ns2:Riyadh_Principality_magazine_website a owl:NamedIndividual,
        owl:Thing ;
    rdfs:comment "Entity representing Riyadh Principality magazine website"^^xsd:string .

ns2:Road_sign_in_San_Francisco a owl:NamedIndividual,
        owl:Thing ;
    rdfs:comment "Entity representing Road sign in San Francisco"^^xsd:string .

ns2:Rosenthal_Wine_Shop a owl:NamedIndividual,
        owl:Thing ;
    rdfs:comment "Entity representing Rosenthal Wine Shop"^^xsd:string .

ns2:Rovio a owl:NamedIndividual,
        owl:Thing ;
    rdfs:comment "Entity representing Rovio"^^xsd:string .

ns2:Rowan_Companies a owl:NamedIndividual,
        owl:Thing ;
    rdfs:comment "Entity representing Rowan Companies"^^xsd:string .

ns2:Rumah_Principality a owl:NamedIndividual,
        owl:Thing ;
    rdfs:comment "Entity representing Rumah Principality"^^xsd:string .

ns2:Rural_King a owl:NamedIndividual,
        owl:Thing ;
    rdfs:comment "Entity representing Rural King"^^xsd:string .

ns2:Russian_Industrial_Investment_Fund a owl:NamedIndividual,
        owl:Thing ;
    rdfs:comment "Entity representing Russian Industrial Investment Fund"^^xsd:string .

ns2:Sabotage a owl:NamedIndividual,
        owl:Thing ;
    rdfs:comment "Entity representing Sabotage"^^xsd:string .

ns2:Sao_Paulo_State_Government a owl:NamedIndividual,
        owl:Thing ;
    rdfs:comment "Entity representing Sao Paulo State Government"^^xsd:string .

ns2:Score a owl:NamedIndividual,
        owl:Thing ;
    rdfs:comment "Entity representing Score"^^xsd:string .

ns2:Sea_Pines_Resort a owl:NamedIndividual,
        owl:Thing ;
    rdfs:comment "Entity representing Sea Pines Resort"^^xsd:string .

ns2:Sears a owl:NamedIndividual,
        owl:Thing ;
    rdfs:comment "Entity representing Sears"^^xsd:string .

ns2:Service_Coordination_Inc a owl:NamedIndividual,
        owl:Thing ;
    rdfs:comment "Entity representing Service Coordination Inc."^^xsd:string .

ns2:Shaqra_Principality a owl:NamedIndividual,
        owl:Thing ;
    rdfs:comment "Entity representing Shaqra Principality"^^xsd:string .

ns2:Shelburne_Country_Store a owl:NamedIndividual,
        owl:Thing ;
    rdfs:comment "Entity representing Shelburne Country Store"^^xsd:string .

ns2:Sheplers a owl:NamedIndividual,
        owl:Thing ;
    rdfs:comment "Entity representing Sheplers"^^xsd:string .

ns2:Silk_Road a owl:NamedIndividual,
        owl:Thing ;
    rdfs:comment "Entity representing Silk Road"^^xsd:string .

ns2:SingPass a owl:NamedIndividual,
        owl:Thing ;
    rdfs:comment "Entity representing SingPass"^^xsd:string .

ns2:Singapore_government_employees a owl:NamedIndividual,
        owl:Thing ;
    rdfs:comment "Entity representing Singapore government employees"^^xsd:string .

ns2:Sir_Ian_Botham a owl:NamedIndividual,
        owl:Thing ;
    rdfs:comment "Entity representing Sir Ian Botham"^^xsd:string .

ns2:Sky_News_Egypt a owl:NamedIndividual,
        owl:Thing ;
    rdfs:comment "Entity representing Sky News Egypt"^^xsd:string .

ns2:Skype_s_Social_Media a owl:NamedIndividual,
        owl:Thing ;
    rdfs:comment "Entity representing Skype's Social Media"^^xsd:string .

ns2:Snapchat a owl:NamedIndividual,
        owl:Thing ;
    rdfs:comment "Entity representing Snapchat"^^xsd:string .

ns2:Soma_Municipality a owl:NamedIndividual,
        owl:Thing ;
    rdfs:comment "Entity representing Soma Municipality"^^xsd:string .

ns2:Sony_PlayStation_Network a owl:NamedIndividual,
        owl:Thing ;
    rdfs:comment "Entity representing Sony PlayStation Network"^^xsd:string .

ns2:Sorenson_Communications a owl:NamedIndividual,
        owl:Thing ;
    rdfs:comment "Entity representing Sorenson Communications"^^xsd:string .

ns2:South_Carolina a owl:NamedIndividual,
        owl:Thing ;
    rdfs:comment "Entity representing South Carolina"^^xsd:string .

ns2:Sparebank_1 a owl:NamedIndividual,
        owl:Thing ;
    rdfs:comment "Entity representing Sparebank 1"^^xsd:string .

ns2:Spec_s a owl:NamedIndividual,
        owl:Thing ;
    rdfs:comment "Entity representing Spec's"^^xsd:string .

ns2:Spirol_International a owl:NamedIndividual,
        owl:Thing ;
    rdfs:comment "Entity representing Spirol International"^^xsd:string .

ns2:Splash_Car_Wash a owl:NamedIndividual,
        owl:Thing ;
    rdfs:comment "Entity representing Splash Car Wash"^^xsd:string .

ns2:Spotify a owl:NamedIndividual,
        owl:Thing ;
    rdfs:comment "Entity representing Spotify"^^xsd:string .

ns2:St__Aldhelm_s_Academy a owl:NamedIndividual,
        owl:Thing ;
    rdfs:comment "Entity representing St. Aldhelm's Academy"^^xsd:string .

ns2:St__Joseph_Health_System a owl:NamedIndividual,
        owl:Thing ;
    rdfs:comment "Entity representing St. Joseph Health System"^^xsd:string .

ns2:St__Jude_Medical a owl:NamedIndividual,
        owl:Thing ;
    rdfs:comment "Entity representing St. Jude Medical"^^xsd:string .

ns2:St__Louis_County_Police a owl:NamedIndividual,
        owl:Thing ;
    rdfs:comment "Entity representing St. Louis County Police"^^xsd:string .

ns2:Stanford_University a owl:NamedIndividual,
        owl:Thing ;
    rdfs:comment "Entity representing Stanford University"^^xsd:string .

ns2:State_Industrial_Products a owl:NamedIndividual,
        owl:Thing ;
    rdfs:comment "Entity representing State Industrial Products"^^xsd:string .

ns2:Staysure a owl:NamedIndividual,
        owl:Thing ;
    rdfs:comment "Entity representing Staysure"^^xsd:string .

ns2:Steam a owl:NamedIndividual,
        owl:Thing ;
    rdfs:comment "Entity representing Steam"^^xsd:string .

ns2:Storebrand a owl:NamedIndividual,
        owl:Thing ;
    rdfs:comment "Entity representing Storebrand"^^xsd:string .

ns2:Summit_County_Fair a owl:NamedIndividual,
        owl:Thing ;
    rdfs:comment "Entity representing Summit County Fair"^^xsd:string .

ns2:Supercell_Facebook_Pages a owl:NamedIndividual,
        owl:Thing ;
    rdfs:comment "Entity representing Supercell Facebook Pages"^^xsd:string .

ns2:Supervalu a owl:NamedIndividual,
        owl:Thing ;
    rdfs:comment "Entity representing Supervalu"^^xsd:string .

ns2:Synology_NAS_Boxes a owl:NamedIndividual,
        owl:Thing ;
    rdfs:comment "Entity representing Synology NAS Boxes"^^xsd:string .

ns2:Syrian_Electronic_Army a owl:NamedIndividual,
        owl:Thing ;
    rdfs:comment "Entity representing Syrian Electronic Army"^^xsd:string .

ns2:Syrian_National_Coalition a owl:NamedIndividual,
        owl:Thing ;
    rdfs:comment "Entity representing Syrian National Coalition"^^xsd:string .

ns2:TTNET a owl:NamedIndividual,
        owl:Thing ;
    rdfs:comment "Entity representing TTNET"^^xsd:string .

ns2:Tails_OS a owl:NamedIndividual,
        owl:Thing ;
    rdfs:comment "Entity representing Tails OS"^^xsd:string .

ns2:Taj_Mahal_Website a owl:NamedIndividual,
        owl:Thing ;
    rdfs:comment "Entity representing Taj Mahal Website"^^xsd:string .

ns2:Tajikistan_Domain_Registrar a owl:NamedIndividual,
        owl:Thing ;
    rdfs:comment "Entity representing Tajikistan Domain Registrar"^^xsd:string .

ns2:Tata_Motors a owl:NamedIndividual,
        owl:Thing ;
    rdfs:comment "Entity representing Tata Motors"^^xsd:string .

ns2:Tehreek_e_Taliban_Pakistan a owl:NamedIndividual,
        owl:Thing ;
    rdfs:comment "Entity representing Tehreek e Taliban Pakistan"^^xsd:string .

ns2:Telecommunications_Directorate a owl:NamedIndividual,
        owl:Thing ;
    rdfs:comment "Entity representing Telecommunications Directorate"^^xsd:string .

ns2:Telenor a owl:NamedIndividual,
        owl:Thing ;
    rdfs:comment "Entity representing Telenor"^^xsd:string .

ns2:TemporalGroup a owl:Class ;
    rdfs:comment "Formal definition for TemporalGroup within the cybersecurity domain."^^xsd:string ;
    rdfs:subClassOf ns1:UCOThing .

ns2:Terrorist a ns1:ThreatActor,
        owl:NamedIndividual ;
    rdfs:comment "Entity representing Terrorist"^^xsd:string .

ns2:Texas_State_Technical_College a owl:NamedIndividual,
        owl:Thing ;
    rdfs:comment "Entity representing Texas State Technical College"^^xsd:string .

ns2:Thadiq_Principality a owl:NamedIndividual,
        owl:Thing ;
    rdfs:comment "Entity representing Thadiq Principality"^^xsd:string .

ns2:TheNaturalOnline_com a owl:NamedIndividual,
        owl:Thing ;
    rdfs:comment "Entity representing TheNaturalOnline.com"^^xsd:string .

ns2:The_Home_Depot a owl:NamedIndividual,
        owl:Thing ;
    rdfs:comment "Entity representing The Home Depot"^^xsd:string .

ns2:The_Houstonian_Hotel a owl:NamedIndividual,
        owl:Thing ;
    rdfs:comment "Entity representing The Houstonian Hotel"^^xsd:string .

ns2:The_Straight_Dope a owl:NamedIndividual,
        owl:Thing ;
    rdfs:comment "Entity representing The Straight Dope"^^xsd:string .

ns2:ThrustVPS a owl:NamedIndividual,
        owl:Thing ;
    rdfs:comment "Entity representing ThrustVPS"^^xsd:string .

ns2:Total_Bank a owl:NamedIndividual,
        owl:Thing ;
    rdfs:comment "Entity representing Total Bank"^^xsd:string .

ns2:Toyota__Guatemala a owl:NamedIndividual,
        owl:Thing ;
    rdfs:comment "Entity representing Toyota (Guatemala)"^^xsd:string .

ns2:Turkish_Ministry_of_Education a owl:NamedIndividual,
        owl:Thing ;
    rdfs:comment "Entity representing Turkish Ministry of Education"^^xsd:string .

ns2:Turkmenbashi_Bank a owl:NamedIndividual,
        owl:Thing ;
    rdfs:comment "Entity representing Turkmenbashi Bank"^^xsd:string .

ns2:Twitter a owl:NamedIndividual,
        owl:Thing ;
    rdfs:comment "Entity representing Twitter"^^xsd:string .

ns2:Typepad a owl:NamedIndividual,
        owl:Thing ;
    rdfs:comment "Entity representing Typepad"^^xsd:string .

ns2:UK_Government_Communications_Headquarter a owl:NamedIndividual,
        owl:Thing ;
    rdfs:comment "Entity representing UK Government Communications Headquarters"^^xsd:string .

ns2:UK_Ministry_of_Justice a owl:NamedIndividual,
        owl:Thing ;
    rdfs:comment "Entity representing UK Ministry of Justice"^^xsd:string .

ns2:UPS a owl:NamedIndividual,
        owl:Thing ;
    rdfs:comment "Entity representing UPS"^^xsd:string .

ns2:USIS a owl:NamedIndividual,
        owl:Thing ;
    rdfs:comment "Entity representing USIS"^^xsd:string .

ns2:US_Army a owl:NamedIndividual,
        owl:Thing ;
    rdfs:comment "Entity representing US Army"^^xsd:string .

ns2:US_Embassy_in_Turkey a owl:NamedIndividual,
        owl:Thing ;
    rdfs:comment "Entity representing US Embassy in Turkey"^^xsd:string .

ns2:US_Federal_Court_System a owl:NamedIndividual,
        owl:Thing ;
    rdfs:comment "Entity representing US Federal Court System"^^xsd:string .

ns2:Ubuntu a owl:NamedIndividual,
        owl:Thing ;
    rdfs:comment "Entity representing Ubuntu"^^xsd:string .

ns2:Ukrainian_Election_Commission a owl:NamedIndividual,
        owl:Thing ;
    rdfs:comment "Entity representing Ukrainian Election Commission"^^xsd:string .

ns2:Ukranian_Democratic_Alliance_for_Reform a owl:NamedIndividual,
        owl:Thing ;
    rdfs:comment "Entity representing Ukranian Democratic Alliance for Reform"^^xsd:string .

ns2:UltraDNS a owl:NamedIndividual,
        owl:Thing ;
    rdfs:comment "Entity representing UltraDNS"^^xsd:string .

ns2:Undisclosed_industrial_software_company a owl:NamedIndividual,
        owl:Thing ;
    rdfs:comment "Entity representing Undisclosed industrial software company"^^xsd:string .

ns2:Undisclosed_number_of_Delaware_restauran a owl:NamedIndividual,
        owl:Thing ;
    rdfs:comment "Entity representing Undisclosed number of Delaware restaurants"^^xsd:string .

ns2:Undisclosed_online_gambling_website a owl:NamedIndividual,
        owl:Thing ;
    rdfs:comment "Entity representing Undisclosed online gambling website"^^xsd:string .

ns2:Undisclosed_video_game_company a owl:NamedIndividual,
        owl:Thing ;
    rdfs:comment "Entity representing Undisclosed video game company"^^xsd:string .

ns2:United_Arab_Emirates a ns1:ThreatActor,
        owl:NamedIndividual ;
    rdfs:comment "Entity representing United Arab Emirates"^^xsd:string .

ns2:United_Kingdom_of_Great_Britain_and_Nort a ns1:ThreatActor,
        owl:NamedIndividual ;
    rdfs:comment "Entity representing United Kingdom of Great Britain and Northern Ireland"^^xsd:string .

ns2:United_Nations_Economic_and_Social_Commi a owl:NamedIndividual,
        owl:Thing ;
    rdfs:comment "Entity representing United Nations Economic and Social Commission for Western Asia"^^xsd:string .

ns2:United_Nations_Integrated_Civil_Society_ a owl:NamedIndividual,
        owl:Thing ;
    rdfs:comment "Entity representing United Nations Integrated Civil Society Organizations System"^^xsd:string .

ns2:United_Nations_Internet_Governance_Forum a owl:NamedIndividual,
        owl:Thing ;
    rdfs:comment "Entity representing United Nations Internet Governance Forum"^^xsd:string .

ns2:United_Socialist_Party_of_Venezuela a owl:NamedIndividual,
        owl:Thing ;
    rdfs:comment "Entity representing United Socialist Party of Venezuela"^^xsd:string .

ns2:University_of_California_Irvine a owl:NamedIndividual,
        owl:Thing ;
    rdfs:comment "Entity representing University of California Irvine"^^xsd:string .

ns2:University_of_California_Washington_Cent a owl:NamedIndividual,
        owl:Thing ;
    rdfs:comment "Entity representing University of California Washington Center"^^xsd:string .

ns2:University_of_Louisiana_at_Monroe a owl:NamedIndividual,
        owl:Thing ;
    rdfs:comment "Entity representing University of Louisiana at Monroe"^^xsd:string .

ns2:University_of_Nebraska_Omaha a owl:NamedIndividual,
        owl:Thing ;
    rdfs:comment "Entity representing University of Nebraska Omaha"^^xsd:string .

ns2:University_of_North_Carolina_Wilmington a owl:NamedIndividual,
        owl:Thing ;
    rdfs:comment "Entity representing University of North Carolina Wilmington"^^xsd:string .

ns2:University_of_Pittsburgh_Medical_Center a owl:NamedIndividual,
        owl:Thing ;
    rdfs:comment "Entity representing University of Pittsburgh Medical Center"^^xsd:string .

ns2:University_of_Virginia a owl:NamedIndividual,
        owl:Thing ;
    rdfs:comment "Entity representing University of Virginia"^^xsd:string .

ns2:University_of_West_Florida a owl:NamedIndividual,
        owl:Thing ;
    rdfs:comment "Entity representing University of West Florida"^^xsd:string .

ns2:University_of_Wisconsin_Parkside a owl:NamedIndividual,
        owl:Thing ;
    rdfs:comment "Entity representing University of Wisconsin Parkside"^^xsd:string .

ns2:Username a owl:Class ;
    rdfs:comment """A username is a phrase, word, or combination of characters used to identify and gain access to a computer or computer network. User accounts, user names, user IDs, and login IDs are all examples of usernames.

Source: https://passcamp.com/blog/what-is-a-username/"""^^xsd:string ;
    rdfs:subClassOf ns2:Account .

ns2:Valley_View_Hospital a owl:NamedIndividual,
        owl:Thing ;
    rdfs:comment "Entity representing Valley View Hospital"^^xsd:string .

ns2:Verkhovna_Rada a owl:NamedIndividual,
        owl:Thing ;
    rdfs:comment "Entity representing Verkhovna Rada"^^xsd:string .

ns2:Vermont a owl:NamedIndividual,
        owl:Thing ;
    rdfs:comment "Entity representing Vermont"^^xsd:string .

ns2:Veterans_of_Foreign_Wars a owl:NamedIndividual,
        owl:Thing ;
    rdfs:comment "Entity representing Veterans of Foreign Wars"^^xsd:string .

ns2:Vibram a owl:NamedIndividual,
        owl:Thing ;
    rdfs:comment "Entity representing Vibram"^^xsd:string .

ns2:Vice a owl:NamedIndividual,
        owl:Thing ;
    rdfs:comment "Entity representing Vice"^^xsd:string .

ns2:Victoria_Justice a owl:NamedIndividual,
        owl:Thing ;
    rdfs:comment "Entity representing Victoria Justice"^^xsd:string .

ns2:Vodafone a owl:NamedIndividual,
        owl:Thing ;
    rdfs:comment "Entity representing Vodafone"^^xsd:string .

ns2:Website_of_the_Connecticut_Governor a owl:NamedIndividual,
        owl:Thing ;
    rdfs:comment "Entity representing Website of the Connecticut Governor"^^xsd:string .

ns2:Website_of_the_Israeli_Prime_Minister a owl:NamedIndividual,
        owl:Thing ;
    rdfs:comment "Entity representing Website of the Israeli Prime Minister"^^xsd:string .

ns2:Well_ca a owl:NamedIndividual,
        owl:Thing ;
    rdfs:comment "Entity representing Well.ca"^^xsd:string .

ns2:West_Bengal_Public_Health_Engineering_De a owl:NamedIndividual,
        owl:Thing ;
    rdfs:comment "Entity representing West Bengal Public Health Engineering Department"^^xsd:string .

ns2:What_cd a owl:NamedIndividual,
        owl:Thing ;
    rdfs:comment "Entity representing What.cd"^^xsd:string .

ns2:Wide_Area_and_Sensing_Conference a owl:NamedIndividual,
        owl:Thing ;
    rdfs:comment "Entity representing Wide Area and Sensing Conference"^^xsd:string .

ns2:WooThemes a owl:NamedIndividual,
        owl:Thing ;
    rdfs:comment "Entity representing WooThemes"^^xsd:string .

ns2:World_Wildlife_Fund a owl:NamedIndividual,
        owl:Thing ;
    rdfs:comment "Entity representing World Wildlife Fund"^^xsd:string .

ns2:World_of_Tanks a owl:NamedIndividual,
        owl:Thing ;
    rdfs:comment "Entity representing World of Tanks"^^xsd:string .

ns2:World_of_Warcraft a owl:NamedIndividual,
        owl:Thing ;
    rdfs:comment "Entity representing World of Warcraft"^^xsd:string .

ns2:Wurm_Online a owl:NamedIndividual,
        owl:Thing ;
    rdfs:comment "Entity representing Wurm Online"^^xsd:string .

ns2:Xbox_Instagram_account a owl:NamedIndividual,
        owl:Thing ;
    rdfs:comment "Entity representing Xbox Instagram account"^^xsd:string .

ns2:Xbox_Live a owl:NamedIndividual,
        owl:Thing ;
    rdfs:comment "Entity representing Xbox Live"^^xsd:string .

ns2:Xbox_Twitter_account a owl:NamedIndividual,
        owl:Thing ;
    rdfs:comment "Entity representing Xbox Twitter account"^^xsd:string .

ns2:Youth_for_Achievements a owl:NamedIndividual,
        owl:Thing ;
    rdfs:comment "Entity representing Youth for Achievements"^^xsd:string .

ns2:ancestry_com a owl:NamedIndividual,
        owl:Thing ;
    rdfs:comment "Entity representing ancestry.com"^^xsd:string .

ns2:antiwar_com a owl:NamedIndividual,
        owl:Thing ;
    rdfs:comment "Entity representing antiwar.com"^^xsd:string .

ns2:askmen_com a owl:NamedIndividual,
        owl:Thing ;
    rdfs:comment "Entity representing askmen.com"^^xsd:string .

ns2:baltimorejewishlife_com a owl:NamedIndividual,
        owl:Thing ;
    rdfs:comment "Entity representing baltimorejewishlife.com"^^xsd:string .

ns2:banderivets_org_ua a owl:NamedIndividual,
        owl:Thing ;
    rdfs:comment "Entity representing banderivets.org.ua"^^xsd:string .

ns2:comicbookdb_com a owl:NamedIndividual,
        owl:Thing ;
    rdfs:comment "Entity representing comicbookdb.com"^^xsd:string .

ns2:domain_me a owl:NamedIndividual,
        owl:Thing ;
    rdfs:comment "Entity representing domain.me"^^xsd:string .

ns2:eyeofdubai_ae a owl:NamedIndividual,
        owl:Thing ;
    rdfs:comment "Entity representing eyeofdubai.ae"^^xsd:string .

ns2:hackforums_net a owl:NamedIndividual,
        owl:Thing ;
    rdfs:comment "Entity representing hackforums.net"^^xsd:string .

ns2:hasAffectedSoftware a owl:ObjectProperty ;
    rdfs:comment "The Affected_Software field captures the list of platforms and software that are affected by this vulnerability. It is implemented through the CybOX Observables, the suggested CybOX objects to use are the Product Object, the Device Object, the System Object, and the Code Object."^^xsd:string ;
    rdfs:domain owl:Thing ;
    rdfs:range owl:Thing ;
    rdfs:seeAlso "http://stixproject.github.io/data-model/1.2/et/VulnerabilityType/"^^xsd:string ;
    owl:equivalentProperty ns2:hasObservable ;
    owl:inverseOf ns2:isAffectedSoftware_of .

ns2:hasAssociatedCampaign a owl:ObjectProperty ;
    rdfs:domain ns1:Attacker,
        ns1:Campaign ;
    rdfs:range ns1:Campaign ;
    owl:inverseOf ns2:isAssociatedCampaign_of .

ns2:hasAttacker a owl:ObjectProperty ;
    rdfs:domain ns1:Attack ;
    rdfs:range ns1:Attacker ;
    rdfs:subPropertyOf ns1:hasMeans ;
    owl:inverseOf ns2:isAttacker_of .

ns2:hasCOAType a owl:ObjectProperty ;
    rdfs:domain ns1:CourseofAction ;
    rdfs:range owl:Thing ;
    owl:inverseOf ns2:isCOAType_of .

ns2:hasCVE_ID a owl:ObjectProperty ;
    rdfs:domain ns1:Vulnerability ;
    rdfs:range ns2:CVE ;
    owl:inverseOf ns2:isCVE_ID_of .

ns2:hasCVSSScore a owl:ObjectProperty ;
    rdfs:domain ns1:Vulnerability ;
    rdfs:range ns2:CVSSScoreType ;
    owl:inverseOf ns2:isCVSSScore_of .

ns2:hasCampaign a owl:ObjectProperty ;
    rdfs:domain ns2:Indicator ;
    rdfs:range ns1:Campaign ;
    owl:inverseOf ns2:isCampaign_of .

ns2:hasConfidenceValue a owl:DatatypeProperty,
        owl:ObjectProperty ;
    rdfs:domain ns1:Attack,
        ns1:Attacker,
        ns1:Campaign,
        ns2:Indicator,
        ns2:StatementType ;
    rdfs:range ns2:ConfidenceType,
        xsd:float ;
    owl:inverseOf ns2:isConfidenceValue_of .

ns2:hasConfiguration a owl:ObjectProperty ;
    rdfs:domain ns1:ExploitTarget ;
    rdfs:range ns2:CCE ;
    owl:inverseOf ns2:isConfiguration_of .

ns2:hasCost a owl:ObjectProperty ;
    rdfs:domain ns1:CourseofAction ;
    rdfs:range ns2:StatementType ;
    rdfs:subPropertyOf owl:topObjectProperty ;
    owl:inverseOf ns2:isCost_of .

ns2:hasEfficacy a owl:ObjectProperty ;
    rdfs:domain ns1:CourseofAction ;
    rdfs:range ns2:StatementType ;
    owl:inverseOf ns2:isEfficacy_of .

ns2:hasImpact a owl:ObjectProperty ;
    rdfs:domain ns1:CourseofAction,
        ns2:Indicator ;
    rdfs:range ns2:StatementType ;
    owl:inverseOf ns2:isImpact_of .

ns2:hasIncident a owl:ObjectProperty ;
    rdfs:domain ns1:Campaign ;
    rdfs:range ns1:Incident ;
    owl:inverseOf ns2:isIncident_of .

ns2:hasIndicator a owl:ObjectProperty ;
    rdfs:domain ns1:Attack,
        ns1:Campaign ;
    rdfs:range ns2:Indicator ;
    owl:inverseOf ns2:isIndicator_of .

ns2:hasIntendedEffect a owl:ObjectProperty ;
    rdfs:domain ns1:Attacker,
        ns1:Campaign,
        ns1:Means ;
    rdfs:range ns2:StatementType ;
    owl:inverseOf ns2:isIntendedEffect_of .

ns2:hasKernel a owl:ObjectProperty ;
    rdfs:domain ns1:OperatingSystem ;
    rdfs:range ns1:KernelModule ;
    owl:inverseOf ns2:isKernel_of .

ns2:hasKillChain a owl:ObjectProperty ;
    rdfs:domain ns1:Means ;
    rdfs:range <http://stix.mitre.org/STIX#KillChain> ;
    owl:inverseOf ns2:isKillChain_of .

ns2:hasKillChainPhase a owl:ObjectProperty ;
    rdfs:domain ns1:Means,
        ns2:Indicator ;
    rdfs:range ns2:KillChainPhase ;
    owl:inverseOf ns2:isKillChainPise_of .

ns2:hasMotivation a owl:ObjectProperty ;
    rdfs:domain ns1:Attacker ;
    rdfs:range ns2:StatementType ;
    owl:inverseOf ns2:isMotivation_of .

ns2:hasOSVDB a owl:ObjectProperty ;
    rdfs:domain ns1:Vulnerability ;
    rdfs:range ns2:OSVDB ;
    owl:inverseOf ns2:isOSVDB_of .

ns2:hasObservedMeans a owl:ObjectProperty ;
    rdfs:domain ns1:Attacker ;
    rdfs:range ns1:Means ;
    rdfs:subPropertyOf owl:topObjectProperty ;
    owl:inverseOf ns2:isObservedMeans_of .

ns2:hasParameterObservables a owl:ObjectProperty ;
    rdfs:domain ns1:CourseofAction ;
    rdfs:range ns1:Consequence ;
    owl:inverseOf ns2:isParameterObservables_of .

ns2:hasRelatedCOA a owl:ObjectProperty ;
    rdfs:domain ns1:CourseofAction ;
    rdfs:range ns1:CourseofAction ;
    owl:inverseOf ns2:isRelatedCOA_of .

ns2:hasRelatedIncident a owl:ObjectProperty ;
    rdfs:domain ns1:Attacker ;
    rdfs:range ns1:Incident ;
    owl:inverseOf ns2:isRelatedIncident_of .

ns2:hasRelatedIndicator a owl:ObjectProperty ;
    rdfs:domain ns2:Indicator ;
    rdfs:range ns2:Indicator ;
    owl:inverseOf ns2:isRelatedIndicator_of .

ns2:hasRelatedMeans a owl:ObjectProperty ;
    rdfs:domain ns1:Means ;
    rdfs:range ns1:Means ;
    owl:inverseOf ns2:isRelatedMeans_of .

ns2:hasRequestedCOA a owl:ObjectProperty ;
    rdfs:domain ns1:Attack ;
    rdfs:range ns1:CourseofAction ;
    rdfs:subPropertyOf owl:topObjectProperty ;
    owl:inverseOf ns2:isRequestedCOA_of .

ns2:hasSoftware a owl:ObjectProperty ;
    rdfs:domain ns1:Observable ;
    rdfs:range ns1:Software ;
    owl:inverseOf ns2:isSoftware_of .

ns2:hasSophistication a owl:ObjectProperty ;
    rdfs:domain ns1:Attacker ;
    rdfs:range ns2:StatementType ;
    owl:inverseOf ns2:isSophistication_of .

ns2:hasStage a owl:ObjectProperty ;
    rdfs:comment "hasStage is used to denote stage/phase of a particular course of action represented as nominals"^^xsd:string ;
    rdfs:domain ns1:CourseofAction ;
    rdfs:range [ a owl:Class ;
            owl:oneOf ( ns2:Remedy ns2:Response ) ] ;
    owl:inverseOf ns2:isStage_of .

ns2:hasStatus a owl:ObjectProperty ;
    rdfs:domain ns1:Campaign ;
    rdfs:range owl:Thing ;
    owl:inverseOf ns2:isStatus_of .

ns2:hasSuggestedCOA a owl:ObjectProperty ;
    rdfs:domain ns2:Indicator ;
    rdfs:range ns1:CourseofAction ;
    owl:inverseOf ns2:isSuggestedCOA_of .

ns2:hasTakenCOA a owl:ObjectProperty ;
    rdfs:domain ns1:Attack ;
    rdfs:range ns1:CourseofAction ;
    rdfs:subPropertyOf owl:topObjectProperty ;
    owl:inverseOf ns2:isTakenCOA_of .

ns2:hasType a owl:ObjectProperty ;
    rdfs:domain ns1:Attacker ;
    rdfs:range ns2:StatementType ;
    owl:inverseOf ns2:isType_of .

ns2:hasWeakness a owl:ObjectProperty ;
    rdfs:domain ns1:ExploitTarget ;
    rdfs:range ns1:CWE ;
    rdfs:subPropertyOf owl:topObjectProperty ;
    owl:inverseOf ns2:isWeakness_of .

ns2:helpmaidan_org_ua a owl:NamedIndividual,
        owl:Thing ;
    rdfs:comment "Entity representing helpmaidan.org.ua"^^xsd:string .

ns2:iiNet a owl:NamedIndividual,
        owl:Thing ;
    rdfs:comment "Entity representing iiNet"^^xsd:string .

ns2:isAffectedSoftware_of a owl:ObjectProperty ;
    rdfs:domain owl:Thing ;
    rdfs:range owl:Thing ;
    owl:inverseOf ns2:hasAffectedSoftware .

ns2:isAssociatedCampaign_of a owl:ObjectProperty ;
    rdfs:domain ns1:Campaign ;
    rdfs:range ns1:Attacker,
        ns1:Campaign ;
    owl:inverseOf ns2:hasAssociatedCampaign .

ns2:isAttacker_of a owl:ObjectProperty ;
    rdfs:domain ns1:Attacker ;
    rdfs:range ns1:Attack ;
    owl:inverseOf ns2:hasAttacker .

ns2:isCOAType_of a owl:ObjectProperty ;
    rdfs:domain owl:Thing ;
    rdfs:range ns1:CourseofAction ;
    owl:inverseOf ns2:hasCOAType .

ns2:isCVE_ID_of a owl:ObjectProperty ;
    rdfs:domain ns2:CVE ;
    rdfs:range ns1:Vulnerability ;
    owl:inverseOf ns2:hasCVE_ID .

ns2:isCVSSScore_of a owl:ObjectProperty ;
    rdfs:domain ns2:CVSSScoreType ;
    rdfs:range ns1:Vulnerability ;
    owl:inverseOf ns2:hasCVSSScore .

ns2:isCampaign_of a owl:ObjectProperty ;
    rdfs:domain ns1:Campaign ;
    rdfs:range ns2:Indicator ;
    owl:inverseOf ns2:hasCampaign .

ns2:isConfidenceValue_of a owl:ObjectProperty ;
    rdfs:domain ns2:ConfidenceType ;
    owl:inverseOf ns2:hasConfidenceValue .

ns2:isConfiguration_of a owl:ObjectProperty ;
    rdfs:domain ns2:CCE ;
    rdfs:range ns1:ExploitTarget ;
    owl:inverseOf ns2:hasConfiguration .

ns2:isConsequence_of a owl:ObjectProperty ;
    rdfs:domain ns1:Consequence ;
    rdfs:range ns1:Vulnerability ;
    owl:inverseOf ns1:hasConsequence .

ns2:isCost_of a owl:ObjectProperty ;
    rdfs:domain ns2:StatementType ;
    rdfs:range ns1:CourseofAction ;
    owl:inverseOf ns2:hasCost .

ns2:isEfficacy_of a owl:ObjectProperty ;
    rdfs:domain ns2:StatementType ;
    rdfs:range ns1:CourseofAction ;
    owl:inverseOf ns2:hasEfficacy .

ns2:isIPAddress_of a owl:ObjectProperty ;
    rdfs:domain ns1:IPAddress ;
    rdfs:range ns1:System ;
    owl:inverseOf ns1:hasIPAddress .

ns2:isIPv4Address_of a owl:ObjectProperty ;
    rdfs:domain owl:Thing ;
    rdfs:range owl:Thing ;
    owl:inverseOf ns1:hasIPv4Address .

ns2:isIPv6Address_of a owl:ObjectProperty ;
    rdfs:domain owl:Thing ;
    rdfs:range owl:Thing ;
    owl:inverseOf ns1:hasIPv6Address .

ns2:isImpact_of a owl:ObjectProperty ;
    rdfs:domain ns2:StatementType ;
    rdfs:range ns1:CourseofAction,
        ns2:Indicator ;
    owl:inverseOf ns2:hasImpact .

ns2:isIncident_of a owl:ObjectProperty ;
    rdfs:domain ns1:Incident ;
    rdfs:range ns1:Campaign ;
    owl:inverseOf ns2:hasIncident .

ns2:isIndicator_of a owl:ObjectProperty ;
    rdfs:domain ns2:Indicator ;
    rdfs:range ns1:Attack,
        ns1:Campaign ;
    owl:inverseOf ns2:hasIndicator .

ns2:isInformationSource_of a owl:ObjectProperty ;
    rdfs:domain owl:Thing ;
    rdfs:range owl:Thing ;
    owl:inverseOf ns1:hasInformationSource .

ns2:isIntendedEffect_of a owl:ObjectProperty ;
    rdfs:domain ns2:StatementType ;
    rdfs:range ns1:Attacker,
        ns1:Campaign,
        ns1:Means ;
    owl:inverseOf ns2:hasIntendedEffect .

ns2:isKernel_of a owl:ObjectProperty ;
    rdfs:domain ns1:KernelModule ;
    rdfs:range ns1:OperatingSystem ;
    owl:inverseOf ns2:hasKernel .

ns2:isKillChainPise_of a owl:ObjectProperty ;
    rdfs:domain ns2:KillChainPhase ;
    rdfs:range ns1:Means,
        ns2:Indicator ;
    owl:inverseOf ns2:hasKillChainPhase .

ns2:isKillChain_of a owl:ObjectProperty ;
    rdfs:domain <http://stix.mitre.org/STIX#KillChain> ;
    rdfs:range ns1:Means ;
    owl:inverseOf ns2:hasKillChain .

ns2:isMACAddress_of a owl:ObjectProperty ;
    owl:inverseOf ns1:hasMACAddress .

ns2:isMeans_of a owl:ObjectProperty ;
    rdfs:domain ns1:Means ;
    rdfs:range ns1:Attack,
        ns1:Campaign,
        ns1:Vulnerability,
        ns2:Indicator ;
    owl:inverseOf ns1:hasMeans .

ns2:isMitigation_of a owl:ObjectProperty ;
    rdfs:domain ns1:CourseofAction ;
    rdfs:range ns1:Vulnerability ;
    owl:inverseOf ns1:hasMitigation .

ns2:isMotivation_of a owl:ObjectProperty ;
    rdfs:domain ns2:StatementType ;
    rdfs:range ns1:Attacker ;
    owl:inverseOf ns2:hasMotivation .

ns2:isOSVDB_of a owl:ObjectProperty ;
    rdfs:domain ns2:OSVDB ;
    rdfs:range ns1:Vulnerability ;
    owl:inverseOf ns2:hasOSVDB .

ns2:isObservable_of a owl:ObjectProperty ;
    rdfs:domain ns1:Observable ;
    rdfs:range ns1:Attack,
        ns1:Vulnerability,
        ns2:Indicator ;
    owl:inverseOf ns2:hasObservable .

ns2:isObservedMeans_of a owl:ObjectProperty ;
    rdfs:domain ns1:Means ;
    rdfs:range ns1:Attacker ;
    owl:inverseOf ns2:hasObservedMeans .

ns2:isParameterObservables_of a owl:ObjectProperty ;
    rdfs:domain ns1:Consequence ;
    rdfs:range ns1:CourseofAction ;
    owl:inverseOf ns2:hasParameterObservables .

ns2:isProduct_of a owl:ObjectProperty ;
    rdfs:domain ns1:Product ;
    rdfs:range ns1:System ;
    owl:inverseOf ns1:hasProduct .

ns2:isRelatedCOA_of a owl:ObjectProperty ;
    rdfs:domain ns1:CourseofAction ;
    rdfs:range ns1:CourseofAction ;
    owl:inverseOf ns2:hasRelatedCOA .

ns2:isRelatedIncident_of a owl:ObjectProperty ;
    rdfs:domain ns1:Incident ;
    rdfs:range ns1:Attacker ;
    owl:inverseOf ns2:hasRelatedIncident .

ns2:isRelatedIndicator_of a owl:ObjectProperty ;
    rdfs:domain ns2:Indicator ;
    rdfs:range ns2:Indicator ;
    owl:inverseOf ns2:hasRelatedIndicator .

ns2:isRelatedMeans_of a owl:ObjectProperty ;
    rdfs:domain ns1:Means ;
    rdfs:range ns1:Means ;
    owl:inverseOf ns2:hasRelatedMeans .

ns2:isRequestedCOA_of a owl:ObjectProperty ;
    rdfs:domain ns1:CourseofAction ;
    rdfs:range ns1:Attack ;
    owl:inverseOf ns2:hasRequestedCOA .

ns2:isSoftware_of a owl:ObjectProperty ;
    rdfs:domain ns1:Software ;
    rdfs:range ns1:Observable ;
    owl:inverseOf ns2:hasSoftware .

ns2:isSophistication_of a owl:ObjectProperty ;
    rdfs:domain ns2:StatementType ;
    rdfs:range ns1:Attacker ;
    owl:inverseOf ns2:hasSophistication .

ns2:isSource_of a owl:ObjectProperty ;
    rdfs:domain ns1:Source ;
    rdfs:range ns1:Attack,
        ns1:Vulnerability ;
    owl:inverseOf ns1:hasSource .

ns2:isStage_of a owl:ObjectProperty ;
    rdfs:domain [ a owl:Class ;
            owl:oneOf ( ns2:Remedy ns2:Response ) ] ;
    rdfs:range ns1:CourseofAction ;
    owl:inverseOf ns2:hasStage .

ns2:isStatus_of a owl:ObjectProperty ;
    rdfs:domain owl:Thing ;
    rdfs:range ns1:Campaign ;
    owl:inverseOf ns2:hasStatus .

ns2:isSuggestedCOA_of a owl:ObjectProperty ;
    rdfs:domain ns1:CourseofAction ;
    rdfs:range ns2:Indicator ;
    owl:inverseOf ns2:hasSuggestedCOA .

ns2:isTakenCOA_of a owl:ObjectProperty ;
    rdfs:domain ns1:CourseofAction ;
    rdfs:range ns1:Attack ;
    owl:inverseOf ns2:hasTakenCOA .

ns2:isTerms_of a owl:ObjectProperty ;
    rdfs:domain ns1:OtherTechnicalTerms ;
    rdfs:range ns1:Web ;
    owl:inverseOf ns1:hasTerms .

ns2:isType_of a owl:ObjectProperty ;
    rdfs:domain ns2:StatementType ;
    rdfs:range ns1:Attacker ;
    owl:inverseOf ns2:hasType .

ns2:isVulnerability_of a owl:ObjectProperty ;
    rdfs:domain ns1:Vulnerability ;
    rdfs:range ns1:ExploitTarget,
        ns1:Means,
        ns1:Product ;
    owl:inverseOf ns1:hasVulnerability .

ns2:isWeakness_of a owl:ObjectProperty ;
    rdfs:domain ns1:CWE ;
    rdfs:range ns1:ExploitTarget ;
    owl:inverseOf ns2:hasWeakness .

ns2:is_affectsProduct_of a owl:ObjectProperty ;
    rdfs:domain ns1:Product ;
    rdfs:range ns1:Vulnerability ;
    owl:inverseOf ns1:affectsProduct .

ns2:is_associatedCampaigns_of a owl:ObjectProperty ;
    rdfs:domain ns1:Campaign ;
    rdfs:range ns1:Campaign ;
    owl:inverseOf ns1:associatedCampaigns .

ns2:is_behaviour_of a owl:ObjectProperty ;
    rdfs:domain [ a owl:Class ;
            owl:unionOf ( ns2:AttackPattern ns2:Exploit ns2:Malware ) ] ;
    rdfs:range ns1:TTP ;
    owl:inverseOf ns2:behaviour .

ns2:is_exploitsVulnerability_of a owl:ObjectProperty ;
    rdfs:domain ns1:Vulnerability ;
    rdfs:range ns1:Means ;
    owl:inverseOf ns1:exploitsVulnerability .

ns2:is_isLaunchedBy_of a owl:ObjectProperty ;
    rdfs:domain ns1:Attacker ;
    rdfs:range ns1:Attack,
        ns1:Campaign ;
    owl:inverseOf ns1:isLaunchedBy .

ns2:is_isUnderAttack_of a owl:ObjectProperty ;
    rdfs:domain ns1:Attack,
        ns1:Consequence ;
    rdfs:range ns1:System ;
    owl:inverseOf ns1:isUnderAttack .

ns2:is_usesAttacks_of a owl:ObjectProperty ;
    rdfs:domain ns1:Attack ;
    rdfs:range ns1:Campaign ;
    owl:inverseOf ns1:usesAttacks .

ns2:job_sy a owl:NamedIndividual,
        owl:Thing ;
    rdfs:comment "Entity representing job.sy"^^xsd:string .

ns2:knowledgeicon_com a owl:NamedIndividual,
        owl:Thing ;
    rdfs:comment "Entity representing knowledgeicon.com"^^xsd:string .

ns2:maidanhelp_com_ua a owl:NamedIndividual,
        owl:Thing ;
    rdfs:comment "Entity representing maidanhelp.com.ua"^^xsd:string .

ns2:maidansupport_com a owl:NamedIndividual,
        owl:Thing ;
    rdfs:comment "Entity representing maidansupport.com"^^xsd:string .

ns2:marigold_in a owl:NamedIndividual,
        owl:Thing ;
    rdfs:comment "Entity representing marigold.in"^^xsd:string .

ns2:mumsnet a owl:NamedIndividual,
        owl:Thing ;
    rdfs:comment "Entity representing mumsnet"^^xsd:string .

ns2:openSUSE a owl:NamedIndividual,
        owl:Thing ;
    rdfs:comment "Entity representing openSUSE"^^xsd:string .

ns2:popvote_hk a owl:NamedIndividual,
        owl:Thing ;
    rdfs:comment "Entity representing popvote.hk"^^xsd:string .

ns2:qha_com_ua a owl:NamedIndividual,
        owl:Thing ;
    rdfs:comment "Entity representing qha.com.ua"^^xsd:string .

ns2:realestate_sy a owl:NamedIndividual,
        owl:Thing ;
    rdfs:comment "Entity representing realestate.sy"^^xsd:string .

ns2:tutorialized_com a owl:NamedIndividual,
        owl:Thing ;
    rdfs:comment "Entity representing tutorialized.com"^^xsd:string .

ns2:wirelessemporium_com a owl:NamedIndividual,
        owl:Thing ;
    rdfs:comment "Entity representing wirelessemporium.com"^^xsd:string .

ns2:zerem_co_il a owl:NamedIndividual,
        owl:Thing ;
    rdfs:comment "Entity representing zerem.co.il"^^xsd:string .

<http://stix.mitre.org/STIX#KillChainPhase> a owl:Class ;
    rdfs:comment "Formal definition for KillChainPhase within the cybersecurity domain."^^xsd:string ;
    rdfs:subClassOf ns1:UCOThing .

ns1:DirectoryExposure a owl:Class ;
    rdfs:comment "Formal definition for DirectoryExposure within the cybersecurity domain."^^xsd:string ;
    rdfs:subClassOf ns1:LossOfConf .

ns1:InputValidationError a owl:Class ;
    rdfs:comment "Formal definition for InputValidationError within the cybersecurity domain."^^xsd:string ;
    rdfs:subClassOf [ a owl:Restriction ;
            owl:onProperty ns1:resultsIn ;
            owl:someValuesFrom ns1:LossOfConf ],
        ns1:Means .

ns1:MeansOrConsequence a owl:Class ;
    rdfs:comment "Formal definition for MeansOrConsequence within the cybersecurity domain."^^xsd:string ;
    rdfs:subClassOf ns1:UCOThing .

ns1:OtherTechnicalTerms a owl:Class ;
    rdfs:comment "Formal definition for OtherTechnicalTerms within the cybersecurity domain."^^xsd:string ;
    rdfs:subClassOf ns1:UCOThing .

ns1:SelfPropagatingCode a owl:Class ;
    rdfs:comment "Formal definition for SelfPropagatingCode within the cybersecurity domain."^^xsd:string ;
    rdfs:subClassOf [ a owl:Restriction ;
            owl:onProperty ns1:resultsIn ;
            owl:someValuesFrom ns1:LossOfConf ],
        ns1:MaliciousCodeExecution .

ns1:TriggeredCode a owl:Class ;
    rdfs:comment "Formal definition for TriggeredCode within the cybersecurity domain."^^xsd:string ;
    rdfs:subClassOf [ a owl:Restriction ;
            owl:onProperty ns1:resultsIn ;
            owl:someValuesFrom ns1:LossOfConf ],
        [ a owl:Restriction ;
            owl:onProperty ns1:resultsIn ;
            owl:someValuesFrom ns1:LossOfIntegrity ],
        ns1:MaliciousCodeExecution .

ns1:hasConsequence a owl:ObjectProperty ;
    rdfs:domain ns1:Vulnerability ;
    rdfs:range ns1:Consequence ;
    owl:inverseOf ns2:isConsequence_of .

ns1:usesAttacks a owl:ObjectProperty ;
    rdfs:domain ns1:Campaign ;
    rdfs:range ns1:Attack ;
    owl:inverseOf ns2:is_usesAttacks_of .

ns2:AttackEmail a owl:Class ;
    rdfs:label "attack email"^^xsd:string ;
    rdfs:comment "Formal definition for AttackEmail within the cybersecurity domain."^^xsd:string ;
    rdfs:subClassOf ns1:BotnetAttack .

ns2:AttackInformation a owl:Class ;
    rdfs:label "attack information"^^xsd:string ;
    rdfs:comment "Formal definition for AttackInformation within the cybersecurity domain."^^xsd:string ;
    rdfs:subClassOf ns2:AttackPattern .

ns2:AttackPhishing a owl:Class ;
    rdfs:label "attack phishing"^^xsd:string ;
    rdfs:comment "Formal definition for AttackPhishing within the cybersecurity domain."^^xsd:string ;
    rdfs:subClassOf ns1:BotnetAttack .

ns2:AttackSchool a owl:Class ;
    rdfs:label "attack school"^^xsd:string ;
    rdfs:comment "Formal definition for AttackSchool within the cybersecurity domain."^^xsd:string ;
    rdfs:subClassOf ns2:AttackPattern .

ns2:Bank_of_Israel a owl:NamedIndividual,
        owl:Thing ;
    rdfs:comment "Entity representing Bank of Israel"^^xsd:string .

ns2:Battle_net a owl:NamedIndividual,
        owl:Thing ;
    rdfs:comment "Entity representing Battle.net"^^xsd:string .

ns2:Bharat_Sanchar_Nigam_Limited__BSNL a owl:NamedIndividual,
        owl:Thing ;
    rdfs:comment "Entity representing Bharat Sanchar Nigam Limited (BSNL)"^^xsd:string .

ns2:Bitstamp a owl:NamedIndividual,
        owl:Thing ;
    rdfs:comment "Entity representing Bitstamp"^^xsd:string .

ns2:BreachUser a owl:Class ;
    rdfs:label "breach user"^^xsd:string ;
    rdfs:comment "Formal definition for BreachUser within the cybersecurity domain."^^xsd:string ;
    rdfs:subClassOf ns2:Exploit .

ns2:CCE a owl:Class ;
    rdfs:comment "Formal definition for CCE within the cybersecurity domain."^^xsd:string ;
    rdfs:subClassOf ns1:UCOThing .

ns2:CVE a owl:Class ;
    rdfs:comment """The details of the CVE class are in another ontology yet to be imported.
CVE is not equal to Vulnerability because Vulnerability also refers to OSVDB_ID"""^^xsd:string ;
    rdfs:subClassOf ns1:UCOThing .

ns2:CVSSScoreType a owl:Class ;
    rdfs:comment "Formal definition for CVSSScoreType within the cybersecurity domain."^^xsd:string ;
    rdfs:subClassOf ns1:UCOThing ;
    owl:equivalentClass [ a owl:Class ;
            owl:unionOf ( ns2:BaseGroup ns2:EnvironmentalGroup ns2:TemporalGroup ) ] .

ns2:ConfidenceType a owl:Class ;
    rdfs:comment "Formal definition for ConfidenceType within the cybersecurity domain."^^xsd:string ;
    rdfs:subClassOf ns1:CourseofAction .

ns2:DataBreach a owl:Class ;
    rdfs:label "data breach"^^xsd:string ;
    rdfs:comment """A data breach is any security incident in which unauthorized parties access sensitive or confidential information, including personal data (Social Security numbers, bank account numbers, healthcare data) and corporate data (customer records, intellectual property, financial information).

Source: https://www.ibm.com/think/topics/data-breach"""^^xsd:string ;
    rdfs:subClassOf ns1:Consequence ;
    owl:equivalentClass ns2:DataLeak .

ns2:DataLeak a owl:Class ;
    rdfs:label "data leak"^^xsd:string ;
    rdfs:comment """Data leakage occurs when sensitive information is exposed to unauthorized parties. For example, a misconfigured cloud storage server might allow easy access to personally identifiable information (PII) and trade secrets. The most common vectors for data leakage stem from human error such as an employee misplacing their laptop or sharing sensitive information over email and messaging platforms. Hackers can use exposed data to commit identity theft, steal credit card details or sell the data on the dark web.

Source: https://www.ibm.com/think/topics/data-leakage"""^^xsd:string ;
    rdfs:subClassOf ns1:Consequence,
        ns2:DataLeak .

ns2:Delaware a owl:NamedIndividual,
        owl:Thing ;
    rdfs:comment "Entity representing Delaware"^^xsd:string .

ns2:ESET a owl:NamedIndividual,
        owl:Thing ;
    rdfs:comment "Entity representing ESET"^^xsd:string .

ns2:Evernote a owl:NamedIndividual,
        owl:Thing ;
    rdfs:comment "Entity representing Evernote"^^xsd:string .

ns2:Georgia a owl:NamedIndividual,
        owl:Thing ;
    rdfs:comment "Entity representing Georgia"^^xsd:string .

ns2:GitHub a owl:NamedIndividual,
        owl:Thing ;
    rdfs:comment "Entity representing GitHub"^^xsd:string .

ns2:Indiana a owl:NamedIndividual,
        owl:Thing ;
    rdfs:comment "Entity representing Indiana"^^xsd:string .

ns2:Indonesia a ns1:ThreatActor,
        owl:NamedIndividual ;
    rdfs:comment "Entity representing Indonesia"^^xsd:string .

ns2:Israel a ns1:ThreatActor,
        owl:NamedIndividual ;
    rdfs:comment "Entity representing Israel"^^xsd:string .

ns2:Israel_Defense_Forces a owl:NamedIndividual,
        owl:Thing ;
    rdfs:comment "Entity representing Israel Defense Forces"^^xsd:string .

ns2:Julie_Bishop a owl:NamedIndividual,
        owl:Thing ;
    rdfs:comment "Entity representing Julie Bishop"^^xsd:string .

ns2:Kansas a owl:NamedIndividual,
        owl:Thing ;
    rdfs:comment "Entity representing Kansas"^^xsd:string .

ns2:KillChainPhase a owl:Class ;
    rdfs:comment "Formal definition for KillChainPhase within the cybersecurity domain."^^xsd:string ;
    rdfs:subClassOf ns1:UCOThing ;
    owl:equivalentClass <http://stix.mitre.org/STIX#KillChainPhase> .

ns2:Libya a ns1:ThreatActor,
        owl:NamedIndividual ;
    rdfs:comment "Entity representing Libya"^^xsd:string .

ns2:Louisiana a owl:NamedIndividual,
        owl:Thing ;
    rdfs:comment "Entity representing Louisiana"^^xsd:string .

ns2:Monsanto a owl:NamedIndividual,
        owl:Thing ;
    rdfs:comment "Entity representing Monsanto"^^xsd:string .

ns2:Nevada a owl:NamedIndividual,
        owl:Thing ;
    rdfs:comment "Entity representing Nevada"^^xsd:string .

ns2:New_Hampshire a owl:NamedIndividual,
        owl:Thing ;
    rdfs:comment "Entity representing New Hampshire"^^xsd:string .

ns2:New_Mexico a owl:NamedIndividual,
        owl:Thing ;
    rdfs:comment "Entity representing New Mexico"^^xsd:string .

ns2:Nigeria a ns1:ThreatActor,
        owl:NamedIndividual ;
    rdfs:comment "Entity representing Nigeria"^^xsd:string .

ns2:OSVDB a owl:Class ;
    rdfs:comment "Formal definition for OSVDB within the cybersecurity domain."^^xsd:string ;
    rdfs:subClassOf ns1:UCOThing .

ns2:Official_website_of_the_President_of_Nep a owl:NamedIndividual,
        owl:Thing ;
    rdfs:comment "Entity representing Official website of the President of Nepal"^^xsd:string .

ns2:Ransomware a owl:Class ;
    rdfs:comment """Ransomware is a type of malware from cryptovirology that threatens to publish the victim's personal data or permanently block access to it unless a ransom is paid. While some simple ransomware may lock the system without damaging any files, more advanced malware uses a technique called cryptoviral extortion. It encrypts the victim's files, making them inaccessible, and demands a ransom payment to decrypt them.

Source: https://dbpedia.org/page/Ransomware"""^^xsd:string ;
    rdfs:subClassOf ns2:Malware .

ns2:Remedy a owl:NamedIndividual .

ns2:Response a owl:NamedIndividual .

ns2:Saudi_Arabia a ns1:ThreatActor,
        owl:NamedIndividual ;
    rdfs:comment "Entity representing Saudi Arabia"^^xsd:string .

ns2:Tennessee a owl:NamedIndividual,
        owl:Thing ;
    rdfs:comment "Entity representing Tennessee"^^xsd:string .

ns2:The_Wall_Street_Journal a owl:NamedIndividual,
        owl:Thing ;
    rdfs:comment "Entity representing The Wall Street Journal"^^xsd:string .

ns2:Turkcell a owl:NamedIndividual,
        owl:Thing ;
    rdfs:comment "Entity representing Turkcell"^^xsd:string .

ns2:University_of_Maryland__College_Park a owl:NamedIndividual,
        owl:Thing ;
    rdfs:comment "Entity representing University of Maryland, College Park"^^xsd:string .

ns2:Wisconsin a owl:NamedIndividual,
        owl:Thing ;
    rdfs:comment "Entity representing Wisconsin"^^xsd:string .

ns2:behaviour a owl:ObjectProperty ;
    rdfs:domain ns1:TTP ;
    rdfs:range [ a owl:Class ;
            owl:unionOf ( ns2:AttackPattern ns2:Exploit ns2:Malware ) ] ;
    owl:inverseOf ns2:is_behaviour_of .

ns2:eBay a owl:NamedIndividual,
        owl:Thing ;
    rdfs:comment "Entity representing eBay"^^xsd:string .

ns2:hasObservable a owl:ObjectProperty ;
    rdfs:domain ns1:Attack,
        ns1:Vulnerability,
        ns2:Indicator ;
    rdfs:range ns1:Observable ;
    owl:inverseOf ns2:isObservable_of .

ns1:Hardware a owl:Class ;
    rdfs:comment "Formal definition for Hardware within the cybersecurity domain."^^xsd:string ;
    rdfs:seeAlso "http://dbpedia.org/resource/Computer_hardware"^^xsd:anyURI ;
    rdfs:subClassOf ns1:UCOThing .

ns1:KernelModule a owl:Class ;
    rdfs:comment "Formal definition for KernelModule within the cybersecurity domain."^^xsd:string ;
    rdfs:seeAlso "http://dbpedia.org/resource/Loadable_kernel_module"^^xsd:anyURI ;
    rdfs:subClassOf ns1:Software .

ns1:LossOfIntegrity a owl:Class ;
    rdfs:comment "Formal definition for LossOfIntegrity within the cybersecurity domain."^^xsd:string ;
    rdfs:subClassOf ns1:Consequence .

ns1:OperatingSystem a owl:Class ;
    rdfs:comment "Formal definition for OperatingSystem within the cybersecurity domain."^^xsd:string ;
    rdfs:seeAlso "http://dbpedia.org/ontology/operatingSystem"^^xsd:anyURI ;
    rdfs:subClassOf ns1:Software .

ns1:TTP a owl:Class ;
    rdfs:comment """Tactics, Techniques and Procedures (TTP) are representations of the behavior or modus operandi of cyber adversaries.

Source: https://stix.mitre.org/about/documents/STIX_Whitepaper_v1.1.pdf"""^^xsd:string ;
    rdfs:subClassOf ns1:UCOThing .

ns1:UnauthUser a owl:Class ;
    rdfs:comment "Formal definition for UnauthUser within the cybersecurity domain."^^xsd:string ;
    rdfs:subClassOf ns1:PrivilegeEsc .

ns1:hasIPAddress a owl:ObjectProperty ;
    rdfs:domain ns1:System ;
    rdfs:range ns1:IPAddress ;
    rdfs:subPropertyOf owl:topObjectProperty ;
    owl:inverseOf ns2:isIPAddress_of .

ns1:hasMeans a owl:ObjectProperty ;
    rdfs:domain ns1:Attack,
        ns1:Campaign,
        ns1:Vulnerability,
        ns2:Indicator ;
    rdfs:range ns1:Means ;
    owl:inverseOf ns2:isMeans_of .

ns2:AccessAttack a owl:Class ;
    rdfs:label "access attack"^^xsd:string ;
    rdfs:comment "Formal definition for AccessAttack within the cybersecurity domain."^^xsd:string ;
    rdfs:subClassOf ns2:Exploit .

ns2:AgencyAttack a owl:Class ;
    rdfs:label "agency attack"^^xsd:string ;
    rdfs:comment "Formal definition for AgencyAttack within the cybersecurity domain."^^xsd:string ;
    rdfs:subClassOf ns2:AttackPattern .

ns2:AttackMalware a owl:Class ;
    rdfs:label "attack malware"^^xsd:string ;
    rdfs:comment "Formal definition for AttackMalware within the cybersecurity domain."^^xsd:string ;
    rdfs:subClassOf ns2:Malware .

ns2:HackUsernames a owl:Class ;
    rdfs:label "hack usernames"^^xsd:string ;
    rdfs:comment "Formal definition for HackUsernames within the cybersecurity domain."^^xsd:string ;
    rdfs:subClassOf ns2:Username .

ns2:HackerUser a owl:Class ;
    rdfs:label "hacker user"^^xsd:string ;
    rdfs:comment "Formal definition for HackerUser within the cybersecurity domain."^^xsd:string ;
    rdfs:subClassOf ns1:UnauthUser .

ns2:Ohio a owl:NamedIndividual,
        owl:Thing ;
    rdfs:comment "Entity representing Ohio"^^xsd:string .

ns2:Utah a owl:NamedIndividual,
        owl:Thing ;
    rdfs:comment "Entity representing Utah"^^xsd:string .

ns2:email a owl:Class ;
    rdfs:comment """Email or electronic mail is the method of sending messages from a computer or mobile device from one user to one or more users via the Internet. Emails travel across different time zones within a snap of a finger and hence are considered an effective mode of communication for both personal and professional purposes.

Source: https://www.zoho.com/mail/glossary/what-is-email.html"""^^xsd:string ;
    rdfs:subClassOf ns2:Account .

<http://stix.mitre.org/STIX#KillChain> a owl:Class ;
    rdfs:comment "Formal definition for KillChain within the cybersecurity domain."^^xsd:string ;
    rdfs:subClassOf ns1:UCOThing .

ns1:File a owl:Class ;
    rdfs:comment """A computer file is a resource for storing information, which is available to a computer program and is usually based on some kind of durable storage. A file is "durable" in the sense that it remains available for other programs to use after the program that created it has finished executing. Computer files can be considered as the modern counterpart of paper documents which traditionally are kept in office and library files, and this is the source of the term.

http://dbpedia.org/page/Computer_file"""^^xsd:anyURI ;
    rdfs:subClassOf ns1:UCOThing .

ns1:IPAddress a owl:Class ;
    rdfs:comment "Formal definition for IPAddress within the cybersecurity domain."^^xsd:string ;
    rdfs:seeAlso "http://dbpedia.org/resource/IP_address"^^xsd:anyURI ;
    rdfs:subClassOf ns1:Address .

ns1:LogicExploit a owl:Class ;
    rdfs:comment "Formal definition for LogicExploit within the cybersecurity domain."^^xsd:string ;
    rdfs:subClassOf ns1:Logic .

ns1:PrivilegeEsc a owl:Class ;
    rdfs:comment "Formal definition for PrivilegeEsc within the cybersecurity domain."^^xsd:string ;
    rdfs:subClassOf ns1:LossOfConf .

ns2:Connecticut a owl:NamedIndividual,
        owl:Thing ;
    rdfs:comment "Entity representing Connecticut"^^xsd:string .

ns2:Data_Attack a owl:NamedIndividual,
        owl:Thing ;
    rdfs:comment "Entity representing Data Attack"^^xsd:string .

ns2:EmailPhishing a owl:Class ;
    rdfs:label "email phishing"^^xsd:string ;
    rdfs:comment "Formal definition for EmailPhishing within the cybersecurity domain."^^xsd:string ;
    rdfs:subClassOf ns2:Phishing .

ns2:France a ns1:ThreatActor,
        owl:NamedIndividual ;
    rdfs:comment "Entity representing France"^^xsd:string .

ns2:Network a owl:Class ;
    rdfs:comment """A network is defined as the connection of at least two computer systems, either by a cable or a wireless connection. The simplest network is a combination of two computers connected by a cable. This type of network is called a peer-to-peer network. There is no hierarchy in this network; both participants have equal privileges. Each computer has access to the data of the other device and can share resources such as disk space, applications or peripheral devices (printers, etc.).

Source: https://www.ionos.com/digitalguide/server/know-how/what-is-a-network/"""^^xsd:string ;
    rdfs:subClassOf ns1:UCOThing .

ns2:Washington_D_C a owl:NamedIndividual,
        owl:Thing ;
    rdfs:comment "Entity representing Washington D.C."^^xsd:string .

ns1:Source a owl:Class ;
    rdfs:comment "Formal definition for Source within the cybersecurity domain."^^xsd:string ;
    rdfs:subClassOf ns1:UCOThing .

ns2:Account a owl:Class ;
    rdfs:comment ""^^xsd:string,
        """An online account is a private, secure account that you create with a business or
website to access and save personal information specific to you and that
website/business. An online account is created with your personal information,
including a username and password, so you can access it later. 

Source: https://www.browncountylibrary.org/wp-content/uploads/2022/01/JobGuide_IntrotoOnlineAccounts.pdf"""^^xsd:string ;
    rdfs:subClassOf ns1:UCOThing .

ns2:Arizona a owl:NamedIndividual,
        owl:Thing ;
    rdfs:comment "Entity representing Arizona"^^xsd:string .

ns2:China a ns1:ThreatActor,
        owl:NamedIndividual ;
    rdfs:comment "Entity representing China"^^xsd:string .

ns2:Florida a owl:NamedIndividual,
        owl:Thing ;
    rdfs:comment "Entity representing Florida"^^xsd:string .

ns2:Industrial_Espionage a owl:NamedIndividual,
        owl:Thing ;
    rdfs:comment "Entity representing Industrial-Espionage"^^xsd:string .

ns2:Iran__Islamic_Republic_of a ns1:ThreatActor,
        owl:NamedIndividual ;
    rdfs:comment "Entity representing Iran (Islamic Republic of)"^^xsd:string .

ns2:Massachusetts a owl:NamedIndividual,
        owl:Thing ;
    rdfs:comment "Entity representing Massachusetts"^^xsd:string .

ns2:Missouri a owl:NamedIndividual,
        owl:Thing ;
    rdfs:comment "Entity representing Missouri"^^xsd:string .

ns2:Nation_State a ns1:ThreatActor,
        owl:NamedIndividual ;
    rdfs:comment "Entity representing Nation-State"^^xsd:string .

ns2:Virginia a owl:NamedIndividual,
        owl:Thing ;
    rdfs:comment "Entity representing Virginia"^^xsd:string .

ns1:Observable a owl:Class ;
    rdfs:comment """Observables are the “base” construct within the STIX architecture. Observables are stateful properties or measurable events pertinent to the operation of computers and networks. Information about a file (name, hash, size, etc.), a registry key value, a service being started, or an HTTP request being sent are all simple examples of observables. STIX leverages CybOX for its representation of Observables.

Source: https://stix.mitre.org/about/documents/STIX_Whitepaper_v1.1.pdf"""^^xsd:string ;
    rdfs:subClassOf ns1:UCOThing .

ns1:RemoteAccess a owl:Class ;
    rdfs:comment "Formal definition for RemoteAccess within the cybersecurity domain."^^xsd:string ;
    rdfs:seeAlso "http://en.wikipedia.org/wiki/Remote_Access_Trojans_(RATs)"^^xsd:anyURI ;
    rdfs:subClassOf ns1:Consequence ;
    owl:equivalentClass [ a owl:Restriction ;
            owl:onProperty ns1:resultsIn ;
            owl:someValuesFrom ns1:PrivilegeEsc ] .

ns2:BaseGroup a owl:Class ;
    rdfs:comment "Formal definition for BaseGroup within the cybersecurity domain."^^xsd:string ;
    rdfs:subClassOf ns1:UCOThing .

ns2:DefaceHacker a owl:Class ;
    rdfs:label "deface hacker"^^xsd:string ;
    rdfs:comment "Formal definition for DefaceHacker within the cybersecurity domain."^^xsd:string ;
    rdfs:subClassOf ns2:Exploit .

ns2:Exploitation_of_Application_Server_Explo a owl:NamedIndividual,
        owl:Thing ;
    rdfs:comment "Entity representing Exploitation of Application Server,Exploitation of Network Infrastructure"^^xsd:string .

ns2:Maryland a owl:NamedIndividual,
        owl:Thing ;
    rdfs:comment "Entity representing Maryland"^^xsd:string .

ns1:ExploitTarget a owl:Class ;
    rdfs:comment """ExploitTargets are vulnerabilities or weaknesses in software, systems, networks or configurations that are targeted for exploitation by the TTP of a ThreatActor.

Source: https://stix.mitre.org/about/documents/STIX_Whitepaper_v1.1.pdf"""^^xsd:string ;
    rdfs:subClassOf ns1:UCOThing .

ns1:LossOfConf a owl:Class ;
    rdfs:comment "Formal definition for LossOfConf within the cybersecurity domain."^^xsd:string ;
    rdfs:subClassOf ns1:Consequence .

ns1:NetworkState a owl:Class ;
    rdfs:comment "Formal definition for NetworkState within the cybersecurity domain."^^xsd:string ;
    rdfs:subClassOf ns1:UCOThing .

ns1:Probe a owl:Class ;
    rdfs:comment "Formal definition for Probe within the cybersecurity domain."^^xsd:string ;
    rdfs:subClassOf [ a owl:Restriction ;
            owl:onProperty ns1:resultsIn ;
            owl:someValuesFrom ns1:DirectoryExposure ],
        [ a owl:Restriction ;
            owl:onProperty ns1:resultsIn ;
            owl:someValuesFrom ns1:MitnickAttack ],
        ns1:Means .

ns1:Product a owl:Class ;
    rdfs:comment "Formal definition for Product within the cybersecurity domain."^^xsd:string ;
    rdfs:subClassOf ns1:UCOThing ;
    owl:equivalentClass [ a owl:Class ;
            owl:unionOf ( ns1:Hardware ns1:Software ) ] .

ns2:Azerbaijan a ns1:ThreatActor,
        owl:NamedIndividual ;
    rdfs:comment "Entity representing Azerbaijan"^^xsd:string .

ns2:Illinois a owl:NamedIndividual,
        owl:Thing ;
    rdfs:comment "Entity representing Illinois"^^xsd:string .

ns2:India a ns1:ThreatActor,
        owl:NamedIndividual ;
    rdfs:comment "Entity representing India"^^xsd:string .

ns2:Norway a ns1:ThreatActor,
        owl:NamedIndividual ;
    rdfs:comment "Entity representing Norway"^^xsd:string .

ns2:Pennsylvania a owl:NamedIndividual,
        owl:Thing ;
    rdfs:comment "Entity representing Pennsylvania"^^xsd:string .

ns2:Russian_Federation a ns1:ThreatActor,
        owl:NamedIndividual ;
    rdfs:comment "Entity representing Russian Federation"^^xsd:string .

ns2:Ukraine a ns1:ThreatActor,
        owl:NamedIndividual ;
    rdfs:comment "Entity representing Ukraine"^^xsd:string .

ns1:MaliciousCodeExecution a owl:Class ;
    rdfs:comment "Formal definition for MaliciousCodeExecution within the cybersecurity domain."^^xsd:string ;
    rdfs:seeAlso "http://dbpedia.org/resource/Arbitrary_code_execution"^^xsd:anyURI ;
    rdfs:subClassOf ns1:Means .

ns2:EnvironmentalGroup a owl:Class ;
    rdfs:comment "Formal definition for EnvironmentalGroup within the cybersecurity domain."^^xsd:string ;
    rdfs:subClassOf ns1:UCOThing .

ns2:Message_Manipulation_Exploitation_of_App a owl:NamedIndividual,
        owl:Thing ;
    rdfs:comment "Entity representing Message Manipulation,Exploitation of Application Server"^^xsd:string .

ns2:Minnesota a owl:NamedIndividual,
        owl:Thing ;
    rdfs:comment "Entity representing Minnesota"^^xsd:string .

ns2:Personal_Attack a owl:NamedIndividual,
        owl:Thing ;
    rdfs:comment "Entity representing Personal Attack"^^xsd:string .

ns1:Software a owl:Class ;
    rdfs:comment "Formal definition for Software within the cybersecurity domain."^^xsd:string ;
    rdfs:seeAlso "http://dbpedia.org/ontology/Software"^^xsd:anyURI ;
    rdfs:subClassOf ns1:UCOThing .

ns1:hasSeverityScore a owl:DatatypeProperty ;
    rdfs:domain owl:Thing ;
    rdfs:range xsd:string .

ns2:CyberattackSystem a owl:Class ;
    rdfs:label "cyberattack system"^^xsd:string ;
    rdfs:comment "Formal definition for CyberattackSystem within the cybersecurity domain."^^xsd:string ;
    rdfs:subClassOf ns1:BotnetAttack .

ns2:Various_Government_Websites a owl:NamedIndividual,
        owl:Thing ;
    rdfs:comment "Entity representing Various Government Websites"^^xsd:string .

ns1:CWE a owl:Class ;
    rdfs:comment "Formal definition for CWE within the cybersecurity domain."^^xsd:string ;
    rdfs:subClassOf ns1:UCOThing .

ns1:DataCorruption a owl:Class ;
    rdfs:comment "Formal definition for DataCorruption within the cybersecurity domain."^^xsd:string ;
    rdfs:subClassOf ns1:LossOfIntegrity .

ns1:DenialOfService a owl:Class ;
    rdfs:comment "Formal definition for DenialOfService within the cybersecurity domain."^^xsd:string ;
    rdfs:seeAlso "http://dbpedia.org/resource/Denial-of-service_attack"^^xsd:anyURI ;
    rdfs:subClassOf ns1:Consequence .

ns2:AccessSecurity a owl:Class ;
    rdfs:label "access security"^^xsd:string ;
    rdfs:comment "Formal definition for AccessSecurity within the cybersecurity domain."^^xsd:string ;
    rdfs:subClassOf ns1:RemoteAccess .

ns2:United_States_of_America a ns1:ThreatActor,
        owl:NamedIndividual ;
    rdfs:comment "Entity representing United States of America"^^xsd:string .

ns2:Washington a owl:NamedIndividual,
        owl:Thing ;
    rdfs:comment "Entity representing Washington"^^xsd:string .

ns1:Address a owl:Class ;
    rdfs:comment "Formal definition for Address within the cybersecurity domain."^^xsd:string ;
    rdfs:subClassOf ns1:UCOThing .

ns2:Phishing a owl:Class ;
    rdfs:comment """Phishing is a type of cyberattack that uses fraudulent emails, text messages, phone calls or websites to trick people into sharing sensitive data, downloading malware or otherwise exposing themselves to cybercrime.

Source: https://www.ibm.com/think/topics/phishing"""^^xsd:string ;
    rdfs:subClassOf ns1:Consequence .

ns2:Texas a owl:NamedIndividual,
        owl:Thing ;
    rdfs:comment "Entity representing Texas"^^xsd:string .

ns1:Process a owl:Class ;
    rdfs:comment "Formal definition for Process within the cybersecurity domain."^^xsd:string ;
    rdfs:seeAlso "http://dbpedia.org/resource/Category:Process_(computing)"^^xsd:anyURI ;
    rdfs:subClassOf ns1:UCOThing .

ns1:Incident a owl:Class ;
    rdfs:comment """Incidents are discrete instances of Indicators affecting an organization along with information discovered or decided during an incident response investigation.

Source: https://stix.mitre.org/about/documents/STIX_Whitepaper_v1.1.pdf"""^^xsd:string ;
    rdfs:subClassOf ns1:UCOThing .

ns2:New_York a owl:NamedIndividual,
        owl:Thing ;
    rdfs:comment "Entity representing New York"^^xsd:string .

ns2:StatementType a owl:Class ;
    rdfs:comment "Formal definition for StatementType within the cybersecurity domain."^^xsd:string ;
    rdfs:subClassOf ns1:UCOThing .

ns2:Victim a owl:Class ;
    rdfs:comment "Formal definition for Victim within the cybersecurity domain."^^xsd:string ;
    rdfs:subClassOf ns1:UCOThing .

ns2:Political_Espionage a owl:NamedIndividual,
        owl:Thing ;
    rdfs:comment "Entity representing Political-Espionage"^^xsd:string .

ns2:Exploitation_of_Sensors a owl:NamedIndividual,
        owl:Thing ;
    rdfs:comment "Entity representing Exploitation of Sensors"^^xsd:string .

ns1:Consequence a owl:Class ;
    rdfs:comment "Formal definition for Consequence within the cybersecurity domain."^^xsd:string ;
    rdfs:subClassOf ns1:MeansOrConsequence ;
    owl:equivalentClass ns1:Observable .

ns2:Turkey a ns1:ThreatActor,
        owl:NamedIndividual ;
    rdfs:comment "Entity representing Turkey"^^xsd:string .

ns2:Indicator a owl:Class ;
    rdfs:comment "Formal definition for Indicator within the cybersecurity domain."^^xsd:string ;
    rdfs:subClassOf ns1:UCOThing .

ns1:Attacker a owl:Class ;
    rdfs:comment """EquivalentClass: ThreatActor
ThreatActors are characterizations of malicious actors (or adversaries) representing a cyber attack threat including presumed intent and historically observed behavior.

Source: https://stix.mitre.org/about/documents/STIX_Whitepaper_v1.1.pdf"""^^xsd:string ;
    rdfs:subClassOf ns1:UCOThing ;
    owl:equivalentClass ns1:ThreatActor .

ns1:resultsIn a owl:IrreflexiveProperty,
        owl:ObjectProperty ;
    rdfs:domain ns1:Means ;
    rdfs:range ns1:Consequence .

ns2:BreachSecurity a owl:Class ;
    rdfs:label "breach security"^^xsd:string ;
    rdfs:comment "Formal definition for BreachSecurity within the cybersecurity domain."^^xsd:string ;
    rdfs:subClassOf ns2:Exploit .

ns2:Exploit a owl:Class ;
    rdfs:comment "Formal definition for Exploit within the cybersecurity domain."^^xsd:string ;
    rdfs:subClassOf ns1:UCOThing .

ns1:Web a owl:Class ;
    rdfs:comment "Formal definition for Web within the cybersecurity domain."^^xsd:string ;
    rdfs:subClassOf ns1:Source .

ns2:Hobbyist a ns1:ThreatActor,
        owl:NamedIndividual ;
    rdfs:comment "Entity representing Hobbyist"^^xsd:string .

ns2:Malware a owl:Class ;
    rdfs:comment "Formal definition for Malware within the cybersecurity domain."^^xsd:string ;
    rdfs:subClassOf ns1:UCOThing .

ns1:BotnetAttack a owl:Class ;
    rdfs:comment "Formal definition for BotnetAttack within the cybersecurity domain."^^xsd:string ;
    rdfs:seeAlso "http://dbpedia.org/resource/Botnet"^^xsd:anyURI ;
    rdfs:subClassOf ns1:Consequence .

ns1:Campaign a owl:Class ;
    rdfs:comment """Campaigns are instances of ThreatActors pursuing an intent, as observed through sets of Incidents and/or TTP, potentially across organizations.

Source: https://stix.mitre.org/about/documents/STIX_Whitepaper_v1.1.pdf"""^^xsd:string ;
    rdfs:subClassOf [ a owl:Restriction ;
            owl:minQualifiedCardinality "1"^^xsd:nonNegativeInteger ;
            owl:onClass ns1:Attack ;
            owl:onProperty ns1:usesAttacks ],
        ns1:UCOThing .

ns1:CourseofAction a owl:Class ;
    rdfs:comment """CoursesOfAction are specific measures to be taken to address threat whether they are corrective or preventative to address ExploitTargets, or responsive to counter or mitigate the potential impacts of Incidents.

Source: https://stix.mitre.org/about/documents/STIX_Whitepaper_v1.1.pdf"""^^xsd:string ;
    rdfs:subClassOf ns1:UCOThing .

ns2:CyberattackInformation a owl:Class ;
    rdfs:label "cyberattack information"^^xsd:string ;
    rdfs:comment "Formal definition for CyberattackInformation within the cybersecurity domain."^^xsd:string ;
    rdfs:subClassOf ns1:BotnetAttack .

ns2:Exploitation_of_End_Hosts a owl:NamedIndividual,
        owl:Thing ;
    rdfs:comment "Entity representing Exploitation of End Hosts"^^xsd:string .

ns2:Pakistan a ns1:ThreatActor,
        owl:NamedIndividual ;
    rdfs:comment "Entity representing Pakistan"^^xsd:string .

ns1:System a owl:Class ;
    rdfs:comment "Formal definition for System within the cybersecurity domain."^^xsd:string ;
    rdfs:seeAlso "http://dbpedia.org/resource/Computer"^^xsd:anyURI ;
    rdfs:subClassOf ns1:UCOThing .

xsd:string rdfs:comment "Campaigns are instances of ThreatActors pursuing an intent, as observed through sets of Incidents and/or TTP, potentially across organizations."^^xsd:string .

ns1:Attack a owl:Class ;
    rdfs:comment """An attack (noun) is the use of an exploit(s) by an adversary to take advantage of a weakness(s) with the intent of achieving a negative technical impact(s).

Source: https://capec.mitre.org/about/glossary.html#Attack

From the bove definition, "the use of an exploit(s)" is means, "an adversary" is attacker, and "negative technical impact(s)" is consequence."""^^xsd:string ;
    rdfs:subClassOf ns1:UCOThing ;
    owl:equivalentClass [ a owl:Restriction ;
            owl:minQualifiedCardinality "1"^^xsd:nonNegativeInteger ;
            owl:onClass ns1:Consequence ;
            owl:onProperty ns1:hasConsequence ],
        [ a owl:Restriction ;
            owl:minQualifiedCardinality "1"^^xsd:nonNegativeInteger ;
            owl:onClass ns1:Means ;
            owl:onProperty ns1:hasMeans ],
        ns1:Incident .

ns1:Means a owl:Class ;
    rdfs:comment "Formal definition for Means within the cybersecurity domain."^^xsd:string ;
    rdfs:subClassOf [ a owl:Restriction ;
            owl:onProperty ns1:resultsIn ;
            owl:someValuesFrom ns1:Consequence ],
        ns1:MeansOrConsequence ;
    owl:equivalentClass [ a owl:Restriction ;
            owl:onProperty ns2:behaviour ;
            owl:someValuesFrom [ a owl:Class ;
                    owl:unionOf ( ns2:AttackPattern ns2:Exploit ns2:Malware ) ] ],
        ns1:TTP .

ns2:AttackPattern a owl:Class ;
    rdfs:comment "Formal definition for AttackPattern within the cybersecurity domain."^^xsd:string ;
    rdfs:subClassOf ns1:UCOThing .

ns2:Syrian_Arab_Republic a ns1:ThreatActor,
        owl:NamedIndividual ;
    rdfs:comment "Entity representing Syrian Arab Republic"^^xsd:string .

ns2:AnonymousAttack a owl:Class ;
    rdfs:label "anonymous attack"^^xsd:string ;
    rdfs:comment "Formal definition for AnonymousAttack within the cybersecurity domain."^^xsd:string ;
    rdfs:subClassOf ns1:BotnetAttack .

ns1:ThreatActor a owl:Class ;
    rdfs:comment """ThreatActors are characterizations of malicious actors (or adversaries) representing a cyber attack threat including presumed intent and historically observed behavior.

Source: https://stix.mitre.org/about/documents/STIX_Whitepaper_v1.1.pdf"""^^xsd:string ;
    rdfs:subClassOf ns1:UCOThing .

ns2:California a owl:NamedIndividual,
        owl:Thing ;
    rdfs:comment "Entity representing California"^^xsd:string .

ns1:Vulnerability a owl:Class ;
    rdfs:comment "Formal definition for Vulnerability within the cybersecurity domain."^^xsd:string ;
    rdfs:seeAlso "http://dbpedia.org/resource/Vulnerability_(computing)"^^xsd:anyURI ;
    rdfs:subClassOf ns1:UCOThing .

ns2:AccountAttack a owl:Class ;
    rdfs:label "account attack"^^xsd:string ;
    rdfs:comment "Formal definition for AccountAttack within the cybersecurity domain."^^xsd:string ;
    rdfs:subClassOf ns1:BotnetAttack .

ns2:DDoS a owl:Class ;
    rdfs:comment """Distributed denial-of-service attacks are a type of denial-of-service attack (DoS attack), a category that includes all cyberattacks that slow or stop applications or services. DDoS attacks are unique in that they send attack traffic from multiple sources all at once—potentially making then harder to recognize and defend against—which puts the “distributed” into “distributed denial-of-service.”

Source: https://www.ibm.com/think/topics/ddos"""^^xsd:string ;
    rdfs:subClassOf ns1:BotnetAttack,
        ns1:DenialOfService .

ns2:BreachInformation a owl:Class ;
    rdfs:label "breach information"^^xsd:string ;
    rdfs:comment "Formal definition for BreachInformation within the cybersecurity domain."^^xsd:string ;
    rdfs:subClassOf ns2:DataBreach .

ns2:CyberattackData a owl:Class ;
    rdfs:label "cyberattack data"^^xsd:string ;
    rdfs:comment "Formal definition for CyberattackData within the cybersecurity domain."^^xsd:string ;
    rdfs:subClassOf ns1:BotnetAttack .

ns1:UCOThing a owl:Class ;
    rdfs:comment "Formal definition for UCOThing within the cybersecurity domain."^^xsd:string .

ns2:AttackWebsite a owl:Class ;
    rdfs:label "attack website"^^xsd:string ;
    rdfs:comment "Formal definition for AttackWebsite within the cybersecurity domain."^^xsd:string ;
    rdfs:subClassOf ns1:BotnetAttack .

ns2:HackerSecurity a owl:Class ;
    rdfs:label "hacker security"^^xsd:string ;
    rdfs:comment "Formal definition for HackerSecurity within the cybersecurity domain."^^xsd:string ;
    rdfs:subClassOf ns2:Exploit .

ns2:External_Denial_of_Service a owl:NamedIndividual,
        owl:Thing ;
    rdfs:comment "Entity representing External Denial of Service"^^xsd:string .

ns2:Financial a owl:NamedIndividual,
        owl:Thing ;
    rdfs:comment "Entity representing Financial"^^xsd:string .

ns2:Protest a owl:NamedIndividual,
        owl:Thing ;
    rdfs:comment "Entity representing Protest"^^xsd:string .

ns2:Message_Manipulation a owl:NamedIndividual,
        owl:Thing ;
    rdfs:comment "Entity representing Message Manipulation"^^xsd:string .

ns2:Hacktivist a ns1:ThreatActor,
        owl:NamedIndividual ;
    rdfs:comment "Entity representing Hacktivist"^^xsd:string .

ns2:Exploitation_of_Application_Server a owl:NamedIndividual,
        owl:Thing ;
    rdfs:comment "Entity representing Exploitation of Application Server"^^xsd:string .

ns2:Criminal a ns1:ThreatActor,
        owl:NamedIndividual ;
    rdfs:comment "Entity representing Criminal"^^xsd:string .

[] a owl:Axiom ;
    rdfs:comment """An attack (noun) is the use of an exploit(s) by an adversary to take advantage of a weakness(s) with the intent of achieving a negative technical impact(s).

Source: https://capec.mitre.org/about/glossary.html#Attack

From the bove definition, "the use of an exploit(s)" is means, "an adversary" is attacker, and "to take advantage of... with the intent of achieving a negative technical impact(s)" is consequence."""^^xsd:string ;
    owl:annotatedProperty rdfs:comment ;
    owl:annotatedSource ns1:Attack ;
    owl:annotatedTarget """An attack (noun) is the use of an exploit(s) by an adversary to take advantage of a weakness(s) with the intent of achieving a negative technical impact(s).

Source: https://capec.mitre.org/about/glossary.html#Attack

From the bove definition, "the use of an exploit(s)" is means, "an adversary" is attacker, and "negative technical impact(s)" is consequence."""^^xsd:string .

